PREFIX : <https://linked.data.gov.au/def/borehole-start-point-setting/>
PREFIX agldwgstatus: <https://linked.data.gov.au/def/reg-statuses/>
PREFIX cs: <https://linked.data.gov.au/def/borehole-start-point-setting>
PREFIX dcat: <http://www.w3.org/ns/dcat#>
PREFIX dcterms: <http://purl.org/dc/terms/>
PREFIX dataroles: <https://linked.data.gov.au/def/data-roles/>
PREFIX owl: <http://www.w3.org/2002/07/owl#>
PREFIX prov: <http://www.w3.org/ns/prov#>
PREFIX rdfs: <http://www.w3.org/2000/01/rdf-schema#>
PREFIX reg: <http://purl.org/linked-data/registry#>
PREFIX schema: <https://schema.org/>
PREFIX skos: <http://www.w3.org/2004/02/skos/core#>
PREFIX xsd: <http://www.w3.org/2001/XMLSchema#>
PREFIX theme: <https://linked.data.gov.au/def/gswa-vocabulary-themes/>

<https://linked.data.gov.au/def/borehole-start-point/from-pre-existing-hole>
    a skos:Concept ;
    dcterms:source "http://linked.data.gov.au/def/borehole-start-point/from-pre-existing-hole"^^xsd:anyURI ;
    rdfs:isDefinedBy <https://linked.data.gov.au/def/borehole-start-point> ;
    skos:definition "Indicates that the borehole was drilled from a pre-existing hole, whether at surface or underground."@en ;
    skos:inScheme cs: ;
    skos:prefLabel "from pre-existing hole"@en ;
    skos:topConceptOf cs: ;
.

<https://linked.data.gov.au/def/borehole-start-point/open-pit-floor-or-wall>
    a skos:Concept ;
    dcterms:source "http://linked.data.gov.au/def/borehole-start-point/open-pit-floor-or-wall"^^xsd:anyURI ;
    rdfs:isDefinedBy <https://linked.data.gov.au/def/borehole-start-point> ;
    skos:definition "Indicates that the borehole was drilled from an open pit floor or open pit wall."@en ;
    skos:inScheme cs: ;
    skos:prefLabel "open pit floor or wall"@en ;
.

<https://linked.data.gov.au/def/borehole-start-point/underground>
    a skos:Concept ;
    dcterms:source "http://linked.data.gov.au/def/borehole-start-point/underground"^^xsd:anyURI ;
    rdfs:isDefinedBy <https://linked.data.gov.au/def/borehole-start-point> ;
    skos:definition "Indicates that the borehole was drilled from an underground location."@en ;
    skos:inScheme cs: ;
    skos:prefLabel "underground"@en ;
    skos:topConceptOf cs: ;
.

:manmade-surface
    a skos:Concept ;
    rdfs:isDefinedBy cs: ;
    skos:definition "Indicates that the borehole was drilled from an artificially made or engineered surface, commonly near a natural ground surface. This concept includes drilling originating from tailings and waste dumps, as well as excavations such as quarries and open pit mines."@en ;
    skos:historyNote "Compiled by GSWA" ;
    skos:inScheme cs: ;
    skos:narrower
        <https://linked.data.gov.au/def/borehole-start-point/open-pit-floor-or-wall> ,
        :mining-byproduct-surface ;
    skos:prefLabel "man-made surface"@en ;
.

:mining-byproduct-surface
    a skos:Concept ;
    rdfs:isDefinedBy cs: ;
    skos:definition "Indicates that the borehole was drilled from artificially made surfaces related to byproducts of exploration and mining operations, such as tailings and waste dumps."@en ;
    skos:historyNote "Compiled by GSWA" ;
    skos:inScheme cs: ;
    skos:prefLabel "mining byproduct surface"@en ;
.

:natural-ground-surface
    a skos:Concept ;
    rdfs:isDefinedBy cs: ;
    skos:closeMatch <https://linked.data.gov.au/def/borehole-start-point/natural-ground-surface> ;
    skos:definition "Indicates that the borehole was drilled from the natural ground surface or from ground with limited disturbance carried out in preparation for drilling, i.e. shallow excavation works, drill pads, cut and fill."@en ;
    skos:historyNote "Compiled by GSWA" ;
    skos:inScheme cs: ;
    skos:prefLabel "natural ground surface"@en ;
.

:offshore
    a skos:Concept ;
    rdfs:isDefinedBy cs: ;
    skos:closeMatch <https://linked.data.gov.au/def/borehole-start-point/offshore> ;
    skos:definition "Indicates that the borehole was drilled in marine waters / open sea from a floating vessel or fixed platform, such as a drill ship, jackup or semisubmersible rig, petroleum platform or a marine research vessel, on the seaward side of the baseline of the territorial sea (as defined in the Seas and Submerged Lands Act 1973, Registered 11 September 2019)."@en ;
    skos:historyNote """This concept is defined in conjunction with 'onshore' by taking into account the definition of territorial sea and its baseline as defined in the Seas and Submerged Lands Act 1973, Registered 11 September 2019
https://www.legislation.gov.au/Details/C2008C00402""" ;
    skos:inScheme cs: ;
    skos:prefLabel "offshore"@en ;
    skos:topConceptOf cs: ;
.

:onshore
    a skos:Concept ;
    rdfs:isDefinedBy cs: ;
    skos:definition "Indicates that the borehole was drilled from or near the natural ground surface. This includes drilling originating on land and on internal waters, i.e. those bodies of water that are located on the landward side of the baseline of the territorial sea (as defined in the Seas and Submerged Lands Act 1973, Registered 11 September 2019)."@en ;
    skos:historyNote """This concept is defined in conjunction with 'offshore' by taking into account the definition of territorial sea and its baseline as defined in the Seas and Submerged Lands Act 1973, Registered 11 September 2019
https://www.legislation.gov.au/Details/C2008C00399""" ;
    skos:inScheme cs: ;
    skos:narrower
        :manmade-surface ,
        :natural-ground-surface ;
    skos:prefLabel "onshore"@en ;
    skos:topConceptOf cs: ;
.

<https://linked.data.gov.au/org/gswa>
    a schema:Organization ;
    schema:name "Geological Survey of Western Australia" ;
    schema:url "https://dmp.wa.gov.au/Geological-Survey/Geological-Survey-262.aspx"^^xsd:anyURI ;
.

:1.0 schema:name "1.0" .

cs:
    a skos:ConceptScheme ;
    dcterms:created "2023-09-06"^^xsd:date ;
    dcterms:creator <https://linked.data.gov.au/org/gswa> ;
    dcterms:identifier "borehole-start-point-setting"^^xsd:token ;
    dcterms:modified "2023-09-06"^^xsd:date ;
    dcterms:publisher <https://linked.data.gov.au/org/gswa> ;
    owl:versionIRI :1.0 ;
    owl:versionInfo "1.0" ;
    reg:status agldwgstatus:stable ;
    skos:definition "Indicates the nature of the borehole start point location, i.e. the general setting and type of surrounding where the borehole is positioned (e.g. onshore, offshore, etc.)."@en ;
    skos:hasTopConcept
        <https://linked.data.gov.au/def/borehole-start-point/from-pre-existing-hole> ,
        <https://linked.data.gov.au/def/borehole-start-point/underground> ,
        :offshore ,
        :onshore ;
    skos:historyNote "Terms and definitions are predominantly sourced from the Geological Survey of Queensland's (GSQ) Borehole start point vocabulary (http:/linked.data.gov.au/def/borehole-start-point), with some modifications and additional concepts."@en ;
    skos:prefLabel "Borehole start point setting"@en ;
    schema:keywords theme:resources ;
    prov:qualifiedAttribution
        [
            dcat:hadRole dataroles:custodian ;
            prov:agent [
                    a schema:Person ;
                    schema:email ""^^xsd:anyURI ;
                    schema:name "Erin Gray" ;
                ]
        ] ,
        [
            dcat:hadRole dataroles:custodian ;
            prov:agent [
                    a schema:Person ;
                    schema:email ""^^xsd:anyURI ;
                    schema:name "Angela Riganti" ;
                ]
        ] ;
.

<https://linked.data.gov.au/def/borehole-start-point> schema:name "Borehole Start Point Vocabulary" .
<https://linked.data.gov.au/def/borehole-start-point/natural-ground-surface> schema:name "natural ground surface" .
<https://linked.data.gov.au/def/borehole-start-point/offshore> schema:name "offshore" .