PREFIX : <https://linked.data.gov.au/def/CRIRSCO-mineral-resource-reporting/>
PREFIX cs: <https://linked.data.gov.au/def/CRIRSCO-mineral-resource-reporting>
PREFIX dcat: <http://www.w3.org/ns/dcat#>
PREFIX dataroles: <https://linked.data.gov.au/def/data-roles/>
PREFIX owl: <http://www.w3.org/2002/07/owl#>
PREFIX prov: <http://www.w3.org/ns/prov#>
PREFIX rdfs: <http://www.w3.org/2000/01/rdf-schema#>
PREFIX reg: <http://purl.org/linked-data/registry#>
PREFIX schema: <https://schema.org/>
PREFIX skos: <http://www.w3.org/2004/02/skos/core#>
PREFIX xsd: <http://www.w3.org/2001/XMLSchema#>
PREFIX theme: <https://linked.data.gov.au/def/gswa-vocabulary-themes/>

:Competent-Person
    a skos:Concept ;
    rdfs:isDefinedBy cs: ;
    skos:closeMatch <https://linked.data.gov.au/def/JORC-Code/Competent-Person> ;
    skos:definition "A Competent Person is a minerals industry professional, who is a [National Reporting Organisation (NRO) to insert appropriate membership class and name of Professional Organisation (PO)] or other Recognised Professional Organisations (RPOs) with enforceable disciplinary processes including the powers to suspend or expel a member. A Competent Person must have a minimum of five years relevant experience in the style of mineralisation or type of deposit under consideration and in the activity which that person is undertaking."@en ;
    skos:historyNote "https://www.crirsco.com/template/" ;
    skos:inScheme cs: ;
    skos:prefLabel "Competent Person"@en ;
    skos:topConceptOf cs: ;
    schema:citation "https://www.crirsco.com/docs/CRIRSCO_International_Reporting_Template_November_2019.pdf"^^xsd:anyURI ;
.

:Exploration-Results
    a skos:Concept ;
    rdfs:isDefinedBy cs: ;
    skos:closeMatch <https://linked.data.gov.au/def/JORC-Code/Exploration-Results> ;
    skos:definition "Exploration Results include data and information generated by mineral exploration programmes that might be of use to investors, but which do not form part of a declaration of Mineral Resources or Mineral Reserves."@en ;
    skos:historyNote "https://www.crirsco.com/template/" ;
    skos:inScheme cs: ;
    skos:prefLabel "Exploration Results"@en ;
    skos:topConceptOf cs: ;
    schema:citation "https://www.crirsco.com/docs/CRIRSCO_International_Reporting_Template_November_2019.pdf"^^xsd:anyURI ;
.

:Exploration-Target
    a skos:Concept ;
    rdfs:isDefinedBy cs: ;
    skos:closeMatch <https://linked.data.gov.au/def/JORC-Code/Exploration-Target> ;
    skos:definition "An Exploration Target is a statement or estimate of the exploration potential of a mineral deposit in a defined geological setting where the statement or estimate, quoted as a range of tonnes and a range of grade or quality, relates to mineralisation for which there has been insufficient exploration to estimate Mineral Resources."@en ;
    skos:historyNote "https://www.crirsco.com/template/" ;
    skos:inScheme cs: ;
    skos:prefLabel "Exploration Target"@en ;
    skos:topConceptOf cs: ;
    schema:citation "https://www.crirsco.com/docs/CRIRSCO_International_Reporting_Template_November_2019.pdf"^^xsd:anyURI ;
.

:Feasibility-Study
    a skos:Concept ;
    rdfs:isDefinedBy cs: ;
    skos:closeMatch <https://linked.data.gov.au/def/JORC-Code/Feasibility-Study> ;
    skos:definition "A Feasibility Study is a comprehensive technical and economic study of the selected development option for a mineral project that includes appropriately detailed assessments of applicable Modifying Factors together with any other relevant operational factors and detailed financial analysis that are necessary to demonstrate at the time of reporting that extraction is reasonably justified (economically mineable). The results of the study may reasonably serve as the basis for a final decision by a proponent or financial institution to proceed with, or finance, the development of the project. The confidence level of the study will be higher than that of a Pre-Feasibility Study."@en ;
    skos:historyNote "https://www.crirsco.com/template/" ;
    skos:inScheme cs: ;
    skos:prefLabel "Feasibility Study"@en ;
    skos:topConceptOf cs: ;
    schema:citation "https://www.crirsco.com/docs/CRIRSCO_International_Reporting_Template_November_2019.pdf"^^xsd:anyURI ;
.

:Indicated-Resource
    a skos:Concept ;
    rdfs:isDefinedBy cs: ;
    skos:broadMatch <https://linked.data.gov.au/def/JORC-Code/Mineral-Resource> ;
    skos:closeMatch <https://linked.data.gov.au/def/JORC-Code/Indicated-Mineral-Resource> ;
    skos:definition "An Indicated Mineral Resource is that part of a Mineral Resource for which quantity, grade or quality, densities, shape and physical characteristics are estimated with sufficient confidence to allow the application of Modifying Factors in sufficient detail to support mine planning and evaluation of the economic viability of the deposit. Geological evidence is derived from adequately detailed and reliable exploration, sampling and testing and is sufficient to assume geological and grade or quality continuity between points of observation. An Indicated Mineral Resource has a lower level of confidence than that applying to a Measured Mineral Resource and may only be converted to a Probable Mineral Reserve."@en ;
    skos:historyNote "https://www.crirsco.com/template/" ;
    skos:inScheme cs: ;
    skos:prefLabel "Indicated Resource"@en ;
    schema:citation "https://www.crirsco.com/docs/CRIRSCO_International_Reporting_Template_November_2019.pdf"^^xsd:anyURI ;
.

:Inferred-Resource
    a skos:Concept ;
    rdfs:isDefinedBy cs: ;
    skos:broadMatch <https://linked.data.gov.au/def/JORC-Code/Mineral-Resource> ;
    skos:closeMatch <https://linked.data.gov.au/def/JORC-Code/Inferred-Mineral-Resource> ;
    skos:definition "An Inferred Mineral Resource is that part of a Mineral Resource for which quantity and grade or quality are estimated on the basis of limited geological evidence and sampling. Geological evidence is sufficient to imply but not verify geological and grade or quality continuity. An Inferred Resource has a lower level of confidence than that applying to an Indicated Mineral Resource and must not be converted to a Mineral Reserve. It is reasonably expected that the majority of Inferred Mineral Resources could be upgraded to Indicated Mineral Resources with continued exploration."@en ;
    skos:historyNote "https://www.crirsco.com/template/" ;
    skos:inScheme cs: ;
    skos:prefLabel "Inferred Resource"@en ;
    schema:citation "https://www.crirsco.com/docs/CRIRSCO_International_Reporting_Template_November_2019.pdf"^^xsd:anyURI ;
.

:Measured-Resource
    a skos:Concept ;
    rdfs:isDefinedBy cs: ;
    skos:broadMatch <https://linked.data.gov.au/def/JORC-Code/Mineral-Resource> ;
    skos:closeMatch <https://linked.data.gov.au/def/JORC-Code/Measured-Mineral-Resource> ;
    skos:definition "A Measured Mineral Resource is that part of a Mineral Resource for which quantity, grade or quality, densities, shape, and physical characteristics are estimated with confidence sufficient to allow the application of Modifying Factors to support detailed mine planning and final evaluation of the economic viability of the deposit. Geological evidence is derived from detailed and reliable exploration, sampling and testing and is sufficient to confirm geological and grade or quality continuity between points of observation. A Measured Mineral Resource has a higher level of confidence than that applying to either an Indicated Mineral Resource or an Inferred Mineral Resource. It may be converted to a Proved Mineral Reserve or to a Probable Mineral Reserve."@en ;
    skos:historyNote "https://www.crirsco.com/template/" ;
    skos:inScheme cs: ;
    skos:prefLabel "Measured Resource"@en ;
    schema:citation "https://www.crirsco.com/docs/CRIRSCO_International_Reporting_Template_November_2019.pdf"^^xsd:anyURI ;
.

:Mineral
    a skos:Concept ;
    rdfs:isDefinedBy cs: ;
    skos:definition "A Mineral is any substance, extracted for value, occurring naturally in or on the Earth, in or under water or in tailings, residues or stockpiles, having been formed by or subjected to a geological process but excludes, water, oil and gas."@en ;
    skos:historyNote "https://www.crirsco.com/template/" ;
    skos:inScheme cs: ;
    skos:prefLabel "Mineral"@en ;
    skos:topConceptOf cs: ;
    schema:citation "https://www.crirsco.com/docs/CRIRSCO_International_Reporting_Template_November_2019.pdf"^^xsd:anyURI ;
.

:Mineral-Reserve
    a skos:Concept ;
    rdfs:isDefinedBy cs: ;
    skos:closeMatch <https://linked.data.gov.au/def/JORC-Code/Ore-Reserve> ;
    skos:definition "A Mineral Reserve is the economically mineable part of a Measured and/or Indicated Mineral Resource. It includes diluting materials and allowances for losses, which may occur when the material is mined or extracted and is defined by studies at Pre-Feasibility or Feasibility level as appropriate that include application of Modifying Factors. Such studies demonstrate that, at the time of reporting, extraction could reasonably be justified. The reference point at which Mineral Reserves are defined, usually the point where the ore is delivered to the processing plant, must be stated. It is important that, in all situations where the reference point is different, such as for a saleable product, a clarifying statement is included to ensure that the reader is fully informed as to what is being reported."@en ;
    skos:historyNote "https://www.crirsco.com/template/" ;
    skos:inScheme cs: ;
    skos:narrower
        :Probable-Reserve ,
        :Proved-Reserve ;
    skos:prefLabel "Mineral Reserve"@en ;
    skos:topConceptOf cs: ;
    schema:citation "https://www.crirsco.com/docs/CRIRSCO_International_Reporting_Template_November_2019.pdf"^^xsd:anyURI ;
.

:Mineral-Resource
    a skos:Concept ;
    rdfs:isDefinedBy cs: ;
    skos:closeMatch <https://linked.data.gov.au/def/JORC-Code/Mineral-Resource> ;
    skos:definition "A Mineral Resource is a concentration or occurrence of solid material of economic interest in or on the Earth’s crust in such form, grade or quality and quantity that there are reasonable prospects for eventual economic extraction. The location, quantity, grade or quality, continuity and other geological characteristics of a Mineral Resource are known, estimated or interpreted from specific geological evidence and knowledge, including sampling. Mineral Resources are subdivided, in order of increasing geological confidence into Inferred, Indicated and Measured categories."@en ;
    skos:historyNote "https://www.crirsco.com/template/" ;
    skos:inScheme cs: ;
    skos:narrower
        :Indicated-Resource ,
        :Inferred-Resource ,
        :Measured-Resource ;
    skos:prefLabel "Mineral Resource"@en ;
    skos:topConceptOf cs: ;
    schema:citation "https://www.crirsco.com/docs/CRIRSCO_International_Reporting_Template_November_2019.pdf"^^xsd:anyURI ;
.

:Modifying-Factors
    a skos:Concept ;
    rdfs:isDefinedBy cs: ;
    skos:closeMatch <https://linked.data.gov.au/def/JORC-Code/Modifying-Factors> ;
    skos:definition "Modifying Factors are considerations used to convert Mineral Resources to Mineral Reserves. These include, but are not restricted to, mining, processing, metallurgical, infrastructure, economic, marketing, legal, environmental, social and governmental factors."@en ;
    skos:historyNote "https://www.crirsco.com/template/" ;
    skos:inScheme cs: ;
    skos:prefLabel "Modifying Factors"@en ;
    skos:topConceptOf cs: ;
    schema:citation "https://www.crirsco.com/docs/CRIRSCO_International_Reporting_Template_November_2019.pdf"^^xsd:anyURI ;
.

:Pre-Feasibility-Study
    a skos:Concept ;
    rdfs:isDefinedBy cs: ;
    skos:closeMatch <https://linked.data.gov.au/def/JORC-Code/Pre-Feasibility-Study> ;
    skos:definition "A Pre-Feasibility Study is a comprehensive study of a range of options for the technical and economic viability of a mineral project that has advanced to a stage where a preferred mining method, in the case of underground mining, or the pit configuration, in the case of an open pit, is established and an effective method of mineral processing is determined. It includes a financial analysis based on reasonable assumptions on the Modifying Factors and the evaluation of any other relevant factors which are sufficient for a Competent Person, acting reasonably, to determine if all or part of the Mineral Resource may be converted to a Mineral Reserve at the time of reporting. A Pre-Feasibility Study is at a lower confidence level than a Feasibility Study."@en ;
    skos:historyNote "https://www.crirsco.com/template/" ;
    skos:inScheme cs: ;
    skos:prefLabel "Pre-Feasibility Study"@en ;
    skos:topConceptOf cs: ;
    schema:citation "https://www.crirsco.com/docs/CRIRSCO_International_Reporting_Template_November_2019.pdf"^^xsd:anyURI ;
.

:Probable-Reserve
    a skos:Concept ;
    rdfs:isDefinedBy cs: ;
    skos:broadMatch <https://linked.data.gov.au/def/JORC-Code/Ore-Reserve> ;
    skos:closeMatch <https://linked.data.gov.au/def/JORC-Code/Probable-Ore-Reserve> ;
    skos:definition "A Probable Mineral Reserve is the economically mineable part of an Indicated, and in some circumstances, a Measured Mineral Resource. The confidence in the Modifying Factors applying to a Probable Mineral Reserve is lower than that applying to a Proved Mineral Reserve."@en ;
    skos:historyNote "https://www.crirsco.com/template/" ;
    skos:inScheme cs: ;
    skos:prefLabel "Probable Reserve"@en ;
    schema:citation "https://www.crirsco.com/docs/CRIRSCO_International_Reporting_Template_November_2019.pdf"^^xsd:anyURI ;
.

:Proved-Reserve
    a skos:Concept ;
    rdfs:isDefinedBy cs: ;
    skos:broadMatch <https://linked.data.gov.au/def/JORC-Code/Ore-Reserve> ;
    skos:closeMatch <https://linked.data.gov.au/def/JORC-Code/Proved-Ore-Reserve> ;
    skos:definition "A Proved Mineral Reserve is the economically mineable part of a Measured Mineral Resource. A Proved Mineral Reserve implies a high degree of confidence in the Modifying Factors."@en ;
    skos:historyNote "https://www.crirsco.com/template/" ;
    skos:inScheme cs: ;
    skos:prefLabel "Proved Reserve"@en ;
    schema:citation "https://www.crirsco.com/docs/CRIRSCO_International_Reporting_Template_November_2019.pdf"^^xsd:anyURI ;
.

:Public-reports
    a skos:Concept ;
    rdfs:isDefinedBy cs: ;
    skos:closeMatch <https://linked.data.gov.au/def/JORC-Code/Public-reports> ;
    skos:definition "Public Reports are reports prepared for the purpose of informing investors or potential investors and their advisers on Exploration Targets, Exploration Results, Mineral Resources or Mineral Reserves. They include but are not limited to annual and quarterly company reports, media releases, information memoranda, technical papers, website postings and public presentations."@en ;
    skos:historyNote "https://www.crirsco.com/template/" ;
    skos:inScheme cs: ;
    skos:prefLabel "Public reports"@en ;
    skos:topConceptOf cs: ;
    schema:citation "https://www.crirsco.com/docs/CRIRSCO_International_Reporting_Template_November_2019.pdf"^^xsd:anyURI ;
.

:Scoping-Study
    a skos:Concept ;
    rdfs:isDefinedBy cs: ;
    skos:closeMatch <https://linked.data.gov.au/def/JORC-Code/Scoping-Study> ;
    skos:definition "A Scoping Study is an order of magnitude technical and economic study of the potential viability of Mineral Resources that includes appropriate assessments of realistically assumed Modifying Factors together with any other relevant operational factors that are necessary to demonstrate at the time of reporting that progress to a Pre‐Feasibility Study can be reasonably justified."@en ;
    skos:historyNote "https://www.crirsco.com/template/" ;
    skos:inScheme cs: ;
    skos:prefLabel "Scoping Study"@en ;
    skos:topConceptOf cs: ;
    schema:citation "https://www.crirsco.com/docs/CRIRSCO_International_Reporting_Template_November_2019.pdf"^^xsd:anyURI ;
.

<https://linked.data.gov.au/org/gswa>
    a schema:Organization ;
    schema:name "Geological Survey of Western Australia" ;
    schema:url "https://www.dmp.wa.gov.au/Geological-Survey/Geological-Survey-262.aspx"^^xsd:anyURI ;
.

:1.1 schema:name "1.1" .

cs:
    a skos:ConceptScheme ;
    reg:status <https://linked.data.gov.au/def/reg-statuses/accepted> ;
    owl:versionIRI :1.1 ;
    skos:definition "Terminology defined by the Committee for Mineral Reserves International Reporting Standards (CRIRSCO; https://www.crirsco.com/) based on the International Reporting Template (IRT; https://www.crirsco.com/docs/CRIRSCO_International_Reporting_Template_November_2019.pdf). The IRT is a document that draws on the best of the CRIRSCO-style reporting standards, the JORC Code (Australasia), SAMREC Code (South Africa), Reporting Code (UK / Western Europe), CIM Guidelines (Canada), SME Guide (USA) and Certification Code (Chile). These reporting standards are recognized and adopted worldwide for market-related reporting and financial investment."@en ;
    skos:hasTopConcept
        :Competent-Person ,
        :Exploration-Results ,
        :Exploration-Target ,
        :Feasibility-Study ,
        :Mineral ,
        :Mineral-Reserve ,
        :Mineral-Resource ,
        :Modifying-Factors ,
        :Pre-Feasibility-Study ,
        :Public-reports ,
        :Scoping-Study ;
    skos:historyNote """https://www.crirsco.com/docs/CRIRSCO_International_Reporting_Template_November_2019.pdf. 
The CRIRSCO Code is closely related to the JORC Code used in Australasia to report mineral resources (sl), as required by the Mines and Mineral Deposits (MINEDEX) system maintained by the Geological Survey of Western Australia."""@en ;
    skos:prefLabel "CRIRSCO mineral resource reporting"@en ;
    prov:qualifiedAttribution
        [
            dcat:hadRole dataroles:custodian ;
            prov:agent
                [
                    a schema:Person ;
                    schema:email ""^^xsd:anyURI ;
                    schema:name "Angela Riganti" ;
                ] ;
        ] ,
        [
            dcat:hadRole dataroles:custodian ;
            prov:agent
                [
                    a schema:Person ;
                    schema:email ""^^xsd:anyURI ;
                    schema:name "Erin Gray" ;
                ] ;
        ] ;
    schema:creator <https://linked.data.gov.au/org/gswa> ;
    schema:dateCreated "2023-11-01"^^xsd:date ;
    schema:dateModified "2023-12-04"^^xsd:date ;
    schema:publisher <https://linked.data.gov.au/org/gswa> ;
    schema:version "1.1: updated IRI to use lowercase characters" ;
    schema:keywords
        theme:resources-mineral ,
        theme:legislation ;
.
