PREFIX : <https://linked.data.gov.au/def/earthsci-for/>
PREFIX cs: <https://linked.data.gov.au/def/earthsci-for>
PREFIX dcat: <http://www.w3.org/ns/dcat#>
PREFIX isoroles: <https://linked.data.gov.au/def/data-roles/>
PREFIX owl: <http://www.w3.org/2002/07/owl#>
PREFIX prov: <http://www.w3.org/ns/prov#>
PREFIX rdfs: <http://www.w3.org/2000/01/rdf-schema#>
PREFIX schema: <https://schema.org/>
PREFIX skos: <http://www.w3.org/2004/02/skos/core#>
PREFIX xsd: <http://www.w3.org/2001/XMLSchema#>
PREFIX reg: <http://purl.org/linked-data/registry#>
PREFIX agldwgstatus: <https://linked.data.gov.au/def/reg-statuses/>

:active-seismic
    a skos:Concept ;
    rdfs:isDefinedBy cs: ;
    skos:broader :seismic-surveys ;
    skos:definition "A seismic method that involves monitoring artificially induced signals."@en ;
    skos:historyNote "Definition adapted from Glossary of geology (5th edition revised; Neuendorf et al., 2011)." ;
    skos:inScheme cs: ;
    skos:prefLabel "active seismic"@en ;
    schema:citation "https://glossary.americangeosciences.org/term/activemethod"^^xsd:anyURI ;
.

:airborne-spectral-imaging
    a skos:Concept ;
    rdfs:isDefinedBy cs: ;
    skos:broader :spectral-imaging ;
    skos:definition "Remotely sensed spectral imaging obtained from an airborne platform."@en ;
    skos:exactMatch <https://linked.data.gov.au/def/earth-science-data-category/airborne-spectral> ;
    skos:historyNote "Definition from Geological Survey of Queensland Earth science data category vocabulary." ;
    skos:inScheme cs: ;
    skos:prefLabel "airborne spectral imaging"@en ;
    schema:citation "https://linked.data.gov.au/def/earth-science-data-category/airborne-spectral"^^xsd:anyURI ;
.

:applied-geophysics
    a skos:Concept ;
    rdfs:isDefinedBy
        cs: ,
        <https://linked.data.gov.au/def/anzsrc-for/2020> ;
    skos:broader :geophysics ;
    skos:definition "A discipline concerned with investigating the Earth from the surface to a depth of several kilometres, specifically aiming to meet the growing demands for natural resources and geo-energies, to respond to the effects of climate change, to provide critical data for civil engineers, and to forecast the effects of natural hazards."@en ;
    skos:historyNote "From the Fields of Research vocabulary from the Australian and New Zealand Standard Research Classification (ANZSRC, 2020). Definition from https://erdw.ethz.ch/en/studies/master/applied-geophysics.html." ;
    skos:inScheme cs: ;
    skos:prefLabel "applied geophysics"@en ;
    schema:citation "https://erdw.ethz.ch/en/studies/master/applied-geophysics.html"^^xsd:anyURI ;
    skos:exactMatch <https://linked.data.gov.au/def/anzsrc-for/2020/370601> ;
    skos:notation "370601"^^<https://linked.data.gov.au/def/anzsrc-for/2020> ;
.

:applied-mineralogy
    a skos:Concept ;
    rdfs:isDefinedBy cs: ;
    skos:broader :mineralogy ;
    skos:definition "Applied mineralogy is located at the intersection of natural sciences and engineering sciences/technology and deals with the entire line of raw material, from extraction/preparation to processing and disposal, i.e. the application of mineralogical information to understanding and solving problems encountered during exploration and mining, and during processing of ores, concentrates, smelter products, and related materials. It involves characterizing minerals and materials, and interpreting the data with respect to exploration, mineral processing, tailings disposal and treatment, hydrometallurgy, pyrometallurgy, and refining."@en ;
    skos:historyNote """Definition adapted from:
1) Petruk, W 2000, Chapter 1: General principles of applied mineralogy, in Applied Mineralogy in the Mining Industry, edited by W Petruk: Amsterdam, Elsevier Science p. 1–26, doi.org/10.1016/B978-044450077-9/50003-1
2) Götze, J and Göbbels, M 2023, Introduction, in Introduction to Applied Mineralogy: Springer, Berlin, Heidelberg, p. 1–2, doi.org/10.1007/978-3-662-64867-4_1.""" ;
    skos:inScheme cs: ;
    skos:prefLabel "applied mineralogy"@en ;
    schema:citation
        "https://link.springer.com/chapter/10.1007/978-3-662-64867-4_1"^^xsd:anyURI ,
        "https://www.sciencedirect.com/science/article/abs/pii/B9780444500779500031"^^xsd:anyURI ;
.

:archival-repository-and-related-studies
    a skos:Concept ;
    rdfs:isDefinedBy
        cs: ,
        <https://linked.data.gov.au/def/anzsrc-for/2020> ;
    skos:altLabel
        "archival science"@en ,
        "archival studies"@en ;
    skos:broader :heritage-archive-and-museum-studies ;
    skos:definition "Archival science, or archival studies, is the study and theory of building and curating archives, i.e. collections of documents, recordings, photographs and various other materials in physical or digital formats, for the purpose of acquiring, evaluating, and accessing recorded materials."@en ;
    skos:exactMatch <https://linked.data.gov.au/def/anzsrc-for/2020/430201> ;
    skos:historyNote "From the Fields of Research vocabulary from the Australian and New Zealand Standard Research Classification (ANZSRC, 2020). Definition adapted from Wikipedia." ;
    skos:inScheme cs: ;
    skos:notation "430201"^^<https://linked.data.gov.au/def/anzsrc-for/2020> ;
    skos:prefLabel "archival, repository and related studies"@en ;
    schema:citation "https://en.wikipedia.org/wiki/Archival_science"^^xsd:anyURI ;
.

:astrobiology
    a skos:Concept ;
    rdfs:isDefinedBy
        cs: ,
        <https://linked.data.gov.au/def/anzsrc-for/2020> ;
    skos:broader :astronomical-sciences ;
    skos:definition "The field of science concerned with the study of life in the universe and attempting to solve the mystery of how life emerged on Earth. This includes the search for life beyond Earth, studying environments that could support life as well as investigating interactions between planets and their stars and exploring how this could influence life. Astrobiology is very much an interdisciplinary endeavour encompassing a wide range of scientific fields such as, but not limited to; biology, astronomy, chemistry, geology, atmospheric science, oceanography, and even aeronautical engineering."@en ;
    skos:exactMatch <https://linked.data.gov.au/def/anzsrc-for/2020/510101> ;
    skos:historyNote "From the Fields of Research vocabulary from the Australian and New Zealand Standard Research Classification (ANZSRC, 2020). Definition adapted from www.space.com." ;
    skos:inScheme cs: ;
    skos:notation "510101"^^<https://linked.data.gov.au/def/anzsrc-for/2020> ;
    skos:prefLabel "astrobiology"@en ;
    schema:citation "https://www.space.com/astrobiology-what-is-it"^^xsd:anyURI ;
.

:basement-geology
    a skos:Concept ;
    rdfs:isDefinedBy cs: ;
    skos:altLabel "bedrock geology"@en ;
    skos:broader :geology ;
    skos:definition "The study of the undifferentiated complex of rocks that underlies the rocks of interest in an area, i.e. the crust of the Earth below sedimentary deposits and regolith, extending downward to the Mohorovičić discontinuity. Basement geology may be self-referential in that it is also the study of defining what constitutes basement at regional and local scales, and whether geologically or economically defined."@en ;
    skos:exactMatch <https://linked.data.gov.au/def/earth-science-data-category/basement-geology> ;
    skos:historyNote "Definition adapted from Glossary of geology (5th edition revised; Neuendorf et. al., 2011), Wikipedia and the Geological Survey of Queensland Earth science data category vocabulary." ;
    skos:inScheme cs: ;
    skos:prefLabel "basement geology"@en ;
    schema:citation
        "https://en.wikipedia.org/wiki/Basement_(geology)"^^xsd:anyURI ,
        "https://glossary.americangeosciences.org/term/basement"^^xsd:anyURI ,
        "https://linked.data.gov.au/def/earth-science-data-category/basement-geology"^^xsd:anyURI ;
.

:basin-analysis
    a skos:Concept ;
    rdfs:isDefinedBy cs: ;
    skos:altLabel "sedimentary basin analysis"@en ;
    skos:broadMatch <https://linked.data.gov.au/def/anzsrc-for/2020/370510> ;
    skos:broader :geology ;
    skos:definition "A geological method of studying sedimentary basins and their potential for energy/mineral commodities, by analysing the sediment fill itself (its composition, primary structures, and internal architecture) to synthesize the basin's geological history/evolution."@en ;
    skos:exactMatch <https://linked.data.gov.au/def/earth-science-data-category/basin-analysis> ;
    skos:historyNote "Definition adapted from Wikipedia and the Geological Survey of Queensland Earth science data category vocabulary." ;
    skos:inScheme cs: ;
    skos:prefLabel "basin analysis"@en ;
    schema:citation
        "https://en.wikipedia.org/wiki/Sedimentary_basin_analysis"^^xsd:anyURI ,
        "https://linked.data.gov.au/def/earth-science-data-category/basin-analysis"^^xsd:anyURI ;
.

:biogeochemistry
    a skos:Concept ;
    rdfs:isDefinedBy
        cs: ,
        <https://linked.data.gov.au/def/earth-science-data-category> ;
    skos:broader :geochemistry ;
    skos:definition "A highly interdisciplinary field involving the integration of biology, geology and chemistry, and encompassing the study of the chemical, physical, geological and biological processes and reactions that govern the composition of the natural environment (including the biosphere, hydrosphere, atmosphere, pedosphere and the lithosphere)."@en ;
    skos:exactMatch <https://linked.data.gov.au/def/earth-science-data-category/biogeochemistry> ;
    skos:historyNote "Definition from Geological Survey of Queensland Earth science data category vocabulary." ;
    skos:inScheme cs: ;
    skos:prefLabel "biogeochemistry"@en ;
    schema:citation "https://linked.data.gov.au/def/earth-science-data-category/biogeochemistry"^^xsd:anyURI ;
.

:biogeology
    a skos:Concept ;
    rdfs:isDefinedBy cs: ;
    skos:broader :geobiology ;
    skos:definition "The interdisciplinary study of biology and geology, embracing interactions between the Earth's biosphere and geosphere (i.e. lithosphere, hydrosphere, atmosphere and cryosphere). It encompasses the biological aspects of geology, e.g. systematic paleontology, the study of organically influenced sedimentation, or the identification of a concealed rock unit by the type of plant growing at the surface above it."@en ;
    skos:exactMatch <https://linked.data.gov.au/def/earth-science-data-category/biogeology> ;
    skos:historyNote """Definition adapted from:
1) Glossary of geology (5th edition revised; Neuendorf et. al., 2011)
2) Yin, H, Xie, S, Qing, J, Yan, J and Luo, G 2008, Discussion on geobiology, biogeology and geobiofacies: Sci. China Ser. D-Earth Sci., v. 51, p. 1516–1524, doi:10.1007/s11430-008-0120-6.""" ;
    skos:inScheme cs: ;
    skos:prefLabel "biogeology"@en ;
    schema:citation
        "https://linked.data.gov.au/def/earth-science-data-category/biogeology"^^xsd:anyURI ,
        "https://en.wikipedia.org/wiki/Biogeology"^^xsd:anyURI ,
        "https://glossary.americangeosciences.org/term/biogeology"^^xsd:anyURI ,
        "https://link.springer.com/article/10.1007/s11430-008-0120-6"^^xsd:anyURI ;
.

:biostratigraphic-age-determination
    a skos:Concept ;
    rdfs:isDefinedBy cs: ;
    skos:broader :geochronology ;
    skos:definition "The correlation and age determination of rocks through the use of fossils, i.e. the determination of approximate absolute ages from the distribution of fossil assemblages in strata and primarily based on a number of time scales that related absolute age to the established sequence of (primarily planktonic) fossil events."@en ;
    skos:historyNote "Definition adapted from AAPG Wiki." ;
    skos:inScheme cs: ;
    skos:prefLabel "biostratigraphic age determination"@en ;
    schema:citation
        "https://glossary.americangeosciences.org/term/biostratigraphy"^^xsd:anyURI ,
        "https://wiki.aapg.org/Biostratigraphic_correlation_and_age_determination"^^xsd:anyURI ;
.

:borehole-logging
    a skos:Concept ;
    rdfs:isDefinedBy cs: ;
    skos:broader :logging ;
    skos:definition "Boreheole (or well) logging is the practice of making a detailed record (a well log, report or graph) of the geological materials and formations penetrated by a borehole. The log may be based either on visual inspection of samples brought to the surface (geological logs) or on physical measurements made on these samples or by instruments lowered into the hole (geophysical logs). Some types of geophysical well logs can be done during any phase of a well's history: drilling, completing, producing, or abandoning. Logging is performed in boreholes drilled for the oil and gas, groundwater, mineral and geothermal exploration, as well as part of environmental, geotechnical or geological studies."@en ;
    skos:historyNote "Definition adapted from Wikipedia." ;
    skos:inScheme cs: ;
    skos:prefLabel "borehole logging"@en ;
    schema:citation
        "https://en.wikipedia.org/wiki/Well_logging"^^xsd:anyURI ,
        "https://www.sciencedirect.com/topics/earth-and-planetary-sciences/borehole-logging"^^xsd:anyURI ;
.

:carbon-geostorage-geology
    a skos:Concept ;
    rdfs:isDefinedBy cs: ;
    skos:broader :geology ;
    skos:definition "Studies related to the identification of deep, subsurface geological sites that are suitable to act as reservoirs for the long-term storage of injected CO₂, to reduce greenhouse-gas emissions to the atmosphere."@en ;
    skos:exactMatch <https://linked.data.gov.au/def/earth-science-data-category/carbon-geostorage-geology> ;
    skos:historyNote "Definition from Geological Survey of Queensland Earth science data category vocabulary." ;
    skos:inScheme cs: ;
    skos:prefLabel "carbon geostorage geology"@en ;
    schema:citation "https://linked.data.gov.au/def/earth-science-data-category/carbon-geostorage-geology"^^xsd:anyURI ;
.

:cartography-and-digital-mapping
    a skos:Concept ;
    rdfs:isDefinedBy
        cs: ,
        <https://linked.data.gov.au/def/anzsrc-for/2020> ;
    skos:broader :geomatic-engineering ;
    skos:definition "The science and art of making maps and charts, and the specific use of digital technologies (mapping tools and software) to create seamless geographical displays of data as an image on a computer screen."@en ;
    skos:exactMatch <https://linked.data.gov.au/def/anzsrc-for/2020/401301> ;
    skos:historyNote "Definition compiled by the Geological survey of western Australia from multiple sources." ;
    skos:inScheme cs: ;
    skos:notation "401301"^^<https://linked.data.gov.au/def/anzsrc-for/2020> ;
    skos:prefLabel "cartography and digital mapping"@en ;
    schema:citation
        "https://glossary.americangeosciences.org/term/cartography"^^xsd:anyURI ,
        "https://maptelligent.com/blog/what-is-digital-mapping/"^^xsd:anyURI ,
        "https://www.ga.gov.au/scientific-topics/national-location-information/digital-mapping-australia"^^xsd:anyURI ;
.

:chemostratigraphy
    a skos:Concept ;
    rdfs:isDefinedBy cs: ;
    skos:altLabel "chemical stratigraphy"@en ;
    skos:broader :stratigraphy ;
    skos:definition "Chemostratigraphy, or chemical stratigraphy, is the study of the chemical signatures and their variations within lithological sequences to determine stratigraphic relationships. It includes the element of stratigraphy that deals with chemical signals as recorded in the stratigraphic record to identify spatial–temporal variations in the concentration and distribution of particular elements and isotopes (e.g. carbonate cycles and isotope cycles)."@en ;
    skos:historyNote "Definition adapted from Wikipedia and Glossary of geology (5th edition revised; Neuendorf et al., 2011)." ;
    skos:inScheme cs: ;
    skos:prefLabel "chemostratigraphy"@en ;
    schema:citation
        "https://en.wikipedia.org/wiki/Chemostratigraphy"^^xsd:anyURI ,
        "https://glossary.americangeosciences.org/term/chemostratigraphy"^^xsd:anyURI ;
.

:chronostratigraphy
    a skos:Concept ;
    rdfs:isDefinedBy cs: ;
    skos:broader :stratigraphy ;
    skos:definition "The branch of stratigraphy that deals with the age of strata and their time relations."@en ;
    skos:historyNote "Definition adapted from Glossary of geology (5th edition revised; Neuendorf et al., 2011)." ;
    skos:inScheme cs: ;
    skos:prefLabel "chronostratigraphy"@en ;
    schema:citation "https://glossary.americangeosciences.org/term/chronostratigraphy"^^xsd:anyURI ;
.

:climatology
    a skos:Concept ;
    rdfs:isDefinedBy
        cs: ,
        <https://linked.data.gov.au/def/anzsrc-for/2020> ;
    skos:altLabel "climate science"@en ;
    skos:broader :climate-change-science ;
    skos:definition "Climatology or climate science is the scientific study of Earth's climate, typically defined as weather conditions averaged over a period of at least 30 years. Climate concerns the atmospheric condition during an extended to indefinite period of time; weather is the condition of the atmosphere during a relative brief period of time and is studied by within the field of meteorology."@en ;
    skos:exactMatch <https://linked.data.gov.au/def/anzsrc-for/2020/370202> ;
    skos:historyNote "From the Fields of Research vocabulary from the Australian and New Zealand Standard Research Classification (ANZSRC, 2020). Definition adapted from Wikipedia." ;
    skos:inScheme cs: ;
    skos:notation "370202"^^<https://linked.data.gov.au/def/anzsrc-for/2020> ;
    skos:prefLabel "climatology"@en ;
    schema:citation "https://en.wikipedia.org/wiki/Climatology"^^xsd:anyURI ;
.

:coal-geology
    a skos:Concept ;
    rdfs:isDefinedBy cs: ;
    skos:broadMatch <https://linked.data.gov.au/def/earth-science-data-category/petroleum-and-coal-geology> ;
    skos:broader :energy-geoscience ;
    skos:definition "Coal geology includes the study of the sedimentation of coals and coal-bearing sequences; their stratigraphy, age and geographic distribution; their physical properties, including coal rank and quality, and the associated classification of coals; their hydrogeological characteristics; contained gases, and the contribution of coal deposits (amongst other rock types) to accumulations of oil and natural gas."@en ;
    skos:exactMatch <https://linked.data.gov.au/def/earth-science-data-category/coal-geology> ;
    skos:historyNote """Definition adapted from:
Thomas, L 2013, Coal Geology, Second Edition: John Wiley & Sons, Ltd, 444p., doi.10.1002/9781118385685.""" ;
    skos:inScheme cs: ;
    skos:prefLabel "coal geology"@en ;
    schema:citation "https://onlinelibrary.wiley.com/doi/book/10.1002/9781118385685"^^xsd:anyURI ;
.

:collection-management
    a skos:Concept ;
    rdfs:isDefinedBy cs: ;
    skos:broader :heritage-archive-and-museum-studies ;
    skos:definition "Collection management refers to the development, storage, and preservation of cultural and natural property, as well as objects of contemporary culture (including contemporary art, literature, technology, and documents) in museums, libraries, archives and private collections. The primary goal of collections management is to meet the needs of the individual collector or collecting institution's mission statement, while also ensuring the long-term safety and sustainability of the objects within the collector's care. Collections management consists primarily of the administrative responsibilities associated with collection development and maintenance (information, preservation, movement, documentation, exhibitions and access processes), and is closely related to collections care, that is the physical preservation for posterity of items in the collections."@en ;
    skos:historyNote """Definition adapted from:
1) Matassa, F 2018, Museum Collections Management, Facet Publishing, Cambridge University press, 258p., doi.10.29085/9781856048699
2) Wikipedia.""" ;
    skos:inScheme cs: ;
    skos:prefLabel "collection management"@en ;
    schema:citation
        "F 2018"^^xsd:anyURI ,
        "Matassa"^^xsd:anyURI ,
        "Museum Collections Management: Facet publishing"^^xsd:anyURI ,
        "https://doi.org/10.29085/9781856048699"^^xsd:anyURI ,
        "https://en.wikipedia.org/wiki/Collections_management"^^xsd:anyURI ;
.

:computational-modelling-and-simulation-in-earth-sciences
    a skos:Concept ;
    rdfs:isDefinedBy
        cs: ,
        <https://linked.data.gov.au/def/anzsrc-for/2020> ;
    skos:altLabel "computational geoscience"@en ;
    skos:broader :geoinformatics ;
    skos:definition "A multidisciplinary field that combines geoscience with advanced mathematical modelling, simulation, numerical modelling, visualization and data analysis techniques. Computational geoscience uses large-scale, nonlinear models that couple multiple physical, chemical, and biological processes across various length and time scales to improve our understanding of the Earth system and its complexities, addressing geoscience grand challenges, and providing decision-support tools for geoscience policy makers and industry. The emergence of computation as a powerful tool for prediction and decision-making in the geosciences is driven by advances in the rapid expansion of our ability to instrument and observe the Earth, sustained improvements in computational models and solution methods for complex geoscience systems, and the relentless growth in computing power."@en ;
    skos:exactMatch <https://linked.data.gov.au/def/anzsrc-for/2020/370401> ;
    skos:historyNote """From the Fields of Research vocabulary from the Australian and New Zealand Standard Research Classification (ANZSRC, 2020). Definition adapted from adapted from:
1) https://link.springer.com/journal/10596
2) https://cse.umn.edu/esci/computational-geoscience.""" ;
    skos:inScheme cs: ;
    skos:notation "370401"^^<https://linked.data.gov.au/def/anzsrc-for/2020> ;
    skos:prefLabel "computational modelling and simulation in earth sciences"@en ;
    schema:citation
        "https://cse.umn.edu/esci/computational-geoscience"^^xsd:anyURI ,
        "https://link.springer.com/journal/10596"^^xsd:anyURI ;
.

:computed-tomography
    a skos:Concept ;
    rdfs:isDefinedBy cs: ;
    skos:broader :tomography ;
    skos:definition "Computed tomography (CT) is a method for imaging and analysing features in rock, mineral or soil specimens in three dimensions using energy attenuation of photons (X-ray tomography), neutrons (neutron tomography), ultrasonic waves (ultrasound tomography), or using magnetic resonance (magnetic resonance imaging). The detected data are used to reconstruct the internal distribution of materials."@en ;
    skos:historyNote """Definition adapted from:
Carlson, WD 2006, Three-dimensional imaging of earth and planetary materials: Earth and Planetary Science Letters, v. 249(3–4), p. 133–147, ISSN 0012-821X, doi.org/10.1016/j.epsl.2006.06.020.""" ;
    skos:inScheme cs: ;
    skos:notation "CT"^^xsd:token ;
    skos:prefLabel "computed tomography"@en ;
    schema:citation
        "http://dx.doi.org/10.1016/j.jsg.2014.02.005"^^xsd:anyURI ,
        "https://doi.org/10.1016/j.epsl.2006.06.020"^^xsd:anyURI ;
.

:conventional-reservoir-geology
    a skos:Concept ;
    rdfs:isDefinedBy cs: ;
    skos:broader :petroleum-geology ;
    skos:definition "The study of conventional (carbonate and clastic) petroleum systems that contain hydrocarbon accumulations and are defined as those where buoyant forces keep hydrocarbons in place below the sealing caprocks and permit petroleum (oil and/or natural gas) to flow readily from reservoirs into wellbores; i.e. are accessible by standard oilfield techniques and typically do not require advanced drilling, completions, and reservoir stimulation methods. Studies of conventional reservoir include assessment of rock properties, particularly porosity, permeability and compressibility, and of the timing and mechanism of trap formation, as petroleum source rocks, reservoir rocks, impermeable caprocks/seals must form in a favourable sequence to allow accumulation in reservoir rocks (following petroleum generation in source rocks and its ensuing migration therefrom)."@en ;
    skos:exactMatch <https://linked.data.gov.au/def/earth-science-data-category/conventional-reservoir-geology> ;
    skos:historyNote "Definition from Geological Survey of Queensland Earth science data category vocabulary." ;
    skos:inScheme cs: ;
    skos:prefLabel "conventional reservoir geology"@en ;
    schema:citation "https://linked.data.gov.au/def/earth-science-data-category/conventional-reservoir-geology"^^xsd:anyURI ;
.

:core-and-surface-sample-petrophysics
    a skos:Concept ;
    rdfs:isDefinedBy cs: ;
    skos:broader :petrophysics ;
    skos:definition "Studies related to the measurement of petrophysical properties in samples collected in the field or from drillcores."@en ;
    skos:historyNote "Compiled by Geological Survey of Western Australia from multiple sources." ;
    skos:inScheme cs: ;
    skos:prefLabel "core and surface sample petrophysics"@en ;
.

:core-logging
    a skos:Concept ;
    rdfs:isDefinedBy cs: ;
    skos:broader :logging ;
    skos:definition "Core logging is the systematic recording and analysis of drillcores, to provide geological understanding of the materials penetrated by a borehole, and to assist in resource estimation. It employs different methods and techniques to characterize subsurface minerals, rocks and formations, as well as their geometry, structure and relationships relative to depth — by observation, measurements and analysis. Although a large proportion of drilling is carried out in the pursuit of mineral and energy resources, core logging is also a critical component of other investigations (e.g. stratigraphic, geotechnical, etc.)."@en ;
    skos:historyNote "Compiled by the Geological Survey of Western Australia from various sources." ;
    skos:inScheme cs: ;
    skos:prefLabel "core logging"@en ;
    schema:citation
        "https://glossary.americangeosciences.org/term/logging"^^xsd:anyURI ,
        "https://www.britannica.com/technology/well-logging#ref14978"^^xsd:anyURI ,
        "https://www.sciencedirect.com/topics/earth-and-planetary-sciences/core-logging"^^xsd:anyURI ;
.

:core-spectral-imaging
    a skos:Concept ;
    rdfs:isDefinedBy cs: ;
    skos:broader :spectral-imaging ;
    skos:definition "Spectral imaging (typically hyperspectral) of rock samples such as core."@en ;
    skos:exactMatch <https://linked.data.gov.au/def/earth-science-data-category/core-spectral> ;
    skos:historyNote "Definition from Geological Survey of Queensland Earth science data category vocabulary." ;
    skos:inScheme cs: ;
    skos:prefLabel "core spectral imaging"@en ;
    schema:citation "https://linked.data.gov.au/def/earth-science-data-category/core-spectral"^^xsd:anyURI ;
.

:crystallography
    a skos:Concept ;
    rdfs:isDefinedBy cs: ;
    skos:broadMatch <https://linked.data.gov.au/def/anzsrc-for/2020/370506> ;
    skos:broader :mineralogy-and-crystallography ;
    skos:definition "The study of crystals, i.e. of homogeneous, solid bodies of chemical element, compound, or isomorphous mixture, having regularly repeating atomic arrangement that may be outwardly expressed by plane faces. It comprises studies of crystal growth, structure, physical properties and their classification by form. It includes optical crystallography (the branch dealing with the optical properties of crystals) and structural crystallography (the study of the internal arrangement and spacing of atoms and molecules composing crystalline solids)."@en ;
    skos:historyNote "Definition adapted from Glossary of geology (5th edition revised; Neuendorf et al., 2011)." ;
    skos:inScheme cs: ;
    skos:prefLabel "crystallography"@en ;
    schema:citation
        "https://glossary.americangeosciences.org/term/crystallography"^^xsd:anyURI ,
        "https://glossary.americangeosciences.org/term/opticalcrystallography"^^xsd:anyURI ,
        "https://glossary.americangeosciences.org/term/structuralcrystallography"^^xsd:anyURI ;
.

:data-mining-and-knowledge-discovery
    a skos:Concept ;
    rdfs:isDefinedBy
        cs: ,
        <https://linked.data.gov.au/def/anzsrc-for/2020> ;
    skos:broader :data-science-and-data-management ;
    skos:definition "The process of extracting and discovering patterns in large datasets involving methods at the intersection of machine learning, statistics, and database systems. Data mining is an interdisciplinary subfield of computer science and statistics with an overall goal of extracting information (with intelligent methods) from a dataset and transforming the information into a comprehensible structure for further use."@en ;
    skos:exactMatch <https://linked.data.gov.au/def/anzsrc-for/2020/460502> ;
    skos:historyNote "From the Fields of Research vocabulary from the Australian and New Zealand Standard Research Classification (ANZSRC, 2020). Definition adapted from Wikipedia." ;
    skos:inScheme cs: ;
    skos:notation "460502"^^<https://linked.data.gov.au/def/anzsrc-for/2020> ;
    skos:prefLabel "data mining and knowledge discovery"@en ;
    schema:citation "https://en.wikipedia.org/wiki/Data_mining"^^xsd:anyURI ;
.

:deep-learning
    a skos:Concept ;
    rdfs:isDefinedBy cs: ;
    skos:broader :artificial-intelligence ;
    skos:definition "Deep learning is a subset of machine learning methods that utilize neural networks for representation learning, i.e. simulate the complex decision-making power of the human brain. The field takes inspiration from biological neuroscience and is centered around stacking artificial neurons into layers and 'training' them to process data. The adjective 'deep' refers to the use of multiple layers (ranging from three to several hundred or thousands) in the network.'"@en ;
    skos:historyNote "Definition adapted from Wikipedia and IBM website." ;
    skos:inScheme cs: ;
    skos:prefLabel "deep learning"@en ;
    schema:citation
        "https://en.wikipedia.org/wiki/Deep_learning"^^xsd:anyURI ,
        "https://www.ibm.com/topics/deep-learning"^^xsd:anyURI ;
.

:dendrochronology
    a skos:Concept ;
    rdfs:isDefinedBy cs: ;
    skos:altLabel "dendrogeochronology"@en ;
    skos:broader :geochronology ;
    skos:definition "The study of annual growth rings of trees for dating of the recent past."@en ;
    skos:historyNote "Definition adapted from Glossary of geology (5th edition revised; Neuendorf et. al., 2011)." ;
    skos:inScheme cs: ;
    skos:prefLabel "dendrochronology"@en ;
    schema:citation "https://glossary.americangeosciences.org/term/dendrochronology"^^xsd:anyURI ;
.

:descriptive-mineralogy
    a skos:Concept ;
    rdfs:isDefinedBy cs: ;
    skos:broader :mineralogy ;
    skos:definition "Descriptive mineralogy includes a description of the crystallographic, general physical and chemical characters of each mineral species, and provides an account of their mode of occurrence and characteristic associations. For minerals possessing an economic value, it includes a brief statement of their uses and industrial applications."@en ;
    skos:historyNote """Definition from:
Mukherjee, S 2011, Descriptive mineralogy, in Applied Mineralogy: Springer, Dordrecht, p. 155–209, doi.org/10.1007/978-94-007-1162-4_7.""" ;
    skos:inScheme cs: ;
    skos:prefLabel "descriptive mineralogy"@en ;
    schema:citation "https://link.springer.com/chapter/10.1007/978-94-007-1162-4_7"^^xsd:anyURI ;
.

:digital-heritage
    a skos:Concept ;
    rdfs:isDefinedBy
        cs: ,
        <https://linked.data.gov.au/def/anzsrc-for/2020> ;
    skos:broader :heritage-archive-and-museum-studies ;
    skos:definition "Digital heritage is the use of digital media in the service of understanding and preserving cultural or natural heritage; more specifically, according to the Charter on the Preservation of Digital Heritage of UNESCO, digital heritage is defined as embracing 'cultural, educational, scientific and administrative resources, as well as technical, legal, medical and other kinds of information created digitally, or converted into digital form from existing analogue resources'. The main goal of the digitization of cultural and natural heritage is to enable the preservation and permanent access of current and future generations to culturally and scientific important objects at all scales."@en ;
    skos:exactMatch <https://linked.data.gov.au/def/anzsrc-for/2020/430204> ;
    skos:historyNote "From the Fields of Research vocabulary from the Australian and New Zealand Standard Research Classification (ANZSRC, 2020). Definition adapted from Wikipedia." ;
    skos:inScheme cs: ;
    skos:notation "430204"^^<https://linked.data.gov.au/def/anzsrc-for/2020> ;
    skos:prefLabel "digital heritage"@en ;
    schema:citation "https://en.wikipedia.org/wiki/Digital_heritage"^^xsd:anyURI ;
.

:downhole-petrophysics
    a skos:Concept ;
    rdfs:isDefinedBy cs: ;
    skos:altLabel "borehole petrophysics"@en ;
    skos:broader :petrophysics ;
    skos:definition "Downhole, or borehole, geophysical surveys measure the physical properties of rocks along a subsurface drillhole."@en ;
    skos:historyNote "Compiled by Geological Survey of Western Australia from multiple sources." ;
    skos:inScheme cs: ;
    skos:prefLabel "downhole petrophysics"@en ;
    schema:citation "https://www.geologyforinvestors.com/down-hole-geophysics-mineral-exporation/"^^xsd:anyURI ;
.

:drilling
    a skos:Concept ;
    rdfs:isDefinedBy cs: ;
    skos:broader :resource-geoscience ;
    skos:definition "Studies related to and associated with the technological advancement of drilling operations, aimed at mitigating the drilling operational deficiencies and instabilities that could hinder operational performance activities and the economic part of drilling development with great effort to minimize their environmental footprint. It includes geoscience-related results obtained during the testing of improved or emerging technologies."@en ;
    skos:historyNote """Definition adapted from: 
Teodoriu, C and Opeyemi, B 2021, An outlook of drilling technologies and innovations: present status and future trends: Energies, 14, 4499, doi.10.3390/en14154499.""" ;
    skos:inScheme cs: ;
    skos:prefLabel "drilling"@en ;
    schema:citation "https://www.researchgate.net/publication/353469134_An_Outlook_of_Drilling_Technologies_and_Innovations_Present_Status_and_Future_Trends"^^xsd:anyURI ;
.

:drilling-engineering
    a skos:Concept ;
    rdfs:isDefinedBy cs: ;
    skos:broader :resources-engineering ;
    skos:closeMatch <https://linked.data.gov.au/def/earth-science-data-category/drilling-engineering> ;
    skos:definition "The science of designing as well as safely and economically making a hole (also called a well or wellbore) from the surface through a rock (or formation) to target potential energy or mineral resources in the subsurface and facilitate the evaluation of the geological intervals penetrated."@en ;
    skos:historyNote "Compiled by the Geological Survey of Western Australia. Definition adapted from Wikipedia." ;
    skos:inScheme cs: ;
    skos:prefLabel "drilling engineering"@en ;
    schema:citation
        "https://linked.data.gov.au/def/earth-science-data-category/drilling-engineering"^^xsd:anyURI ,
        "https://wiki.seg.org/wiki/Drilling_engineering"^^xsd:anyURI ;
.

:earth-and-space-science-informatics
    a skos:Concept ;
    rdfs:isDefinedBy
        cs: ,
        <https://linked.data.gov.au/def/anzsrc-for/2020> ;
    skos:broader :geoinformatics ;
    skos:definition "Earth and Space Science Informatics (ESSI) encompasses a broad field that addresses data management practices, computation and analysis, and hardware and software infrastructure. It involves collaborative work to assess, design, implement, and promote practices and tools that enable effective data management, discovery, integration, and reuse for interdisciplinary work in Earth and space science (ESS) disciplines."@en ;
    skos:exactMatch <https://linked.data.gov.au/def/anzsrc-for/2020/370402> ;
    skos:historyNote "From the Fields of Research vocabulary from the Australian and New Zealand Standard Research Classification (ANZSRC, 2020). Definition adapted from https://agupubs.onlinelibrary.wiley.com/doi/full/10.1029/2021EA002108." ;
    skos:inScheme cs: ;
    skos:notation
        "370402"^^<https://linked.data.gov.au/def/anzsrc-for/2020> ,
        "ESSI"^^<https://linked.data.gov.au/def/anzsrc-for/2020> ;
    skos:prefLabel "Earth and space science informatics"@en ;
    schema:citation "https://agupubs.onlinelibrary.wiley.com/doi/full/10.1029/2021EA002108"^^xsd:anyURI ;
.

:earth-system-science
    a skos:Concept ;
    rdfs:isDefinedBy cs: ;
    skos:definition "The study of Earth as an integrated system, particularly the physical, chemical, biological and human interactions that determine the past, current and future states of the Earth. Earth System Science is the study of the interactions and interdependencies within and between the Earth’s various physical, chemical and biological “spheres” (lithosphere, hydrosphere, biosphere, atmosphere, cryosphere), and the impacts that changes to any of these may have for the entire Earth System (including humans)."@en ;
    skos:historyNote "Definition adapted from Wikipedia." ;
    skos:inScheme cs: ;
    skos:prefLabel "earth system science"@en ;
    skos:topConceptOf cs: ;
    schema:citation "https://en.wikipedia.org/wiki/Earth_system_science"^^xsd:anyURI ;
.

:ecology
    a skos:Concept ;
    rdfs:isDefinedBy
        cs: ,
        <https://linked.data.gov.au/def/anzsrc-for/2020> ;
    skos:broader :biological-sciences ;
    skos:definition "A branch of biology concerning interactions among organisms and their biophysical environment, which includes both biotic and abiotic components."@en ;
    skos:exactMatch
        <https://linked.data.gov.au/def/anzsrc-for/2020/3103> ,
        <https://linked.data.gov.au/def/earth-science-data-category/ecology> ;
    skos:historyNote "From the Fields of Research vocabulary from the Australian and New Zealand Standard Research Classification (ANZSRC, 2020). Definition from Geological Survey of Queensland Earth science data category vocabulary." ;
    skos:inScheme cs: ;
    skos:notation "3103"^^<https://linked.data.gov.au/def/anzsrc-for/2020> ;
    skos:prefLabel "ecology"@en ;
    schema:citation "https://linked.data.gov.au/def/earth-science-data-category/ecology"^^xsd:anyURI ;
.

:economic-analysis
    a skos:Concept ;
    rdfs:isDefinedBy cs: ;
    skos:broader :resource-geoscience ;
    skos:definition "A discipline that investigates and promotes understanding of economic and policy issues associated with the production and use of mineral and energy commodities."@en ;
    skos:historyNote "Definition adapted from Wikipedia." ;
    skos:inScheme cs: ;
    skos:prefLabel "economic analysis"@en ;
    schema:citation "https://en.wikipedia.org/wiki/Mineral_economics"^^xsd:anyURI ;
.

:electrical-geophysics
    a skos:Concept ;
    rdfs:isDefinedBy cs: ;
    skos:broader :electrical-and-electromagnetic-methods-in-geophysics ;
    skos:definition "The use of geophysical methods to detect and image different electrical properties of the subsurface, by measuring naturally occurring (i.e. passive) or artificially introduced (i.e. active) voltage potentials, electrical currents, and/or electromagnetic fields. Subsurface electrical properties can be measured galvanically via direct electrode connection to the ground or inductively via electromagnetic field induction through the subsurface. The Electrical resistivity technique is used to determine the resistivity of subsurface materials, the Induced Polarization (IP) technique is used to measure the decay of voltage in the ground, and the Self-Potential (SP) technique looks for natural voltage sources underground."@en ;
    skos:exactMatch <https://linked.data.gov.au/def/earth-science-data-category/electrical-geophysics> ;
    skos:historyNote "Definition adapted from United States Environmental Protection Agency." ;
    skos:inScheme cs: ;
    skos:prefLabel "electrical geophysics"@en ;
    schema:citation "https://www.epa.gov/environmental-geophysics/electrical-methods"^^xsd:anyURI ;
.

:electromagnetic-geophysics
    a skos:Concept ;
    rdfs:isDefinedBy cs: ;
    skos:broader :electrical-and-electromagnetic-methods-in-geophysics ;
    skos:definition "The use of geophysical methods to detect and image the electrical properties of the subsurface by inducing electromagnetic (EM) energy within the subsurface (i.e. propagation of electromagnetic fields composed of an alternating electric intensity and magnetizing force) and measuring the response of earth materials."@en ;
    skos:exactMatch <https://linked.data.gov.au/def/earth-science-data-category/electromagnetic-geophysics> ;
    skos:historyNote "Definition adapted from United States Environmental Protection Agency." ;
    skos:inScheme cs: ;
    skos:notation "EM"^^xsd:token ;
    skos:prefLabel "electromagnetic geophysics"@en ;
    schema:citation
        "https://www.epa.gov/environmental-geophysics/electromagnetic-methods"^^xsd:anyURI ,
        "https://www.sciencedirect.com/topics/earth-and-planetary-sciences/electromagnetic-survey"^^xsd:anyURI ;
.

:elevation
    a skos:Concept ;
    rdfs:isDefinedBy cs: ;
    skos:broader :geodesy ;
    skos:definition "The measurement and modelling of the elevation of geographic locations, i.e. of the height above or below a fixed reference point, most commonly a reference geoid (a mathematical model of the Earth's sea level as an equipotential gravitational surface)."@en ;
    skos:historyNote "Definition adapted from Wikipedia." ;
    skos:inScheme cs: ;
    skos:prefLabel "elevation"@en ;
    schema:citation "https://en.wikipedia.org/wiki/Elevation"^^xsd:anyURI ;
.

:energy-exploration
    a skos:Concept ;
    rdfs:isDefinedBy cs: ;
    skos:broader :energy-geoscience ;
    skos:definition "The search for deposits of useful fossil fuels and energy resources. It includes multidisciplinary approaches, including geological studies, remote sensing, photogeology, geophysical and geochemical methods, and both surface and below ground investigations."@en ;
    skos:historyNote "Definition adapted from Glossary of geology (5th edition revised; Neuendorf et al., 2011)." ;
    skos:inScheme cs: ;
    skos:prefLabel "energy exploration"@en ;
    schema:citation "https://glossary.americangeosciences.org/term/exploration"^^xsd:anyURI ;
.

:engineering-geology
    a skos:Concept ;
    rdfs:isDefinedBy cs: ;
    skos:broader :geology ;
    skos:definition "The application of geology to engineering study for the purpose of assuring that the geological factors regarding the location, design, construction, operation and maintenance of engineering works are recognized and accounted for. Engineering geologists provide geological and geotechnical recommendations, analysis, and design associated with human development and various types of structures. The realm of the engineering geologist is essentially in the area of Earth-structure interactions, or investigation of how the Earth or Earth processes impact human-made structures and human activities."@en ;
    skos:historyNote "Definition adapted from Wikipedia." ;
    skos:inScheme cs: ;
    skos:prefLabel "engineering geology"@en ;
    schema:citation "https://en.wikipedia.org/wiki/Engineering_geology"^^xsd:anyURI ;
.

:environmental-engineering
    a skos:Concept ;
    rdfs:isDefinedBy
        cs: ,
        <https://linked.data.gov.au/def/anzsrc-for/2020> ;
    skos:broader :engineering ;
    skos:definition "A professional engineering discipline related to environmental science that encompasses broad scientific topics like chemistry, biology, ecology, geology, hydraulics, hydrology, microbiology, and mathematics to create solutions that will protect and also improve the health of living organisms and improve the quality of the environment."@en ;
    skos:exactMatch
        <https://linked.data.gov.au/def/anzsrc-for/2020/4011> ,
        <https://linked.data.gov.au/def/earth-science-data-category/environmental-engineering> ;
    skos:historyNote "From the Fields of Research vocabulary from the Australian and New Zealand Standard Research Classification (ANZSRC, 2020). Definition adapted from Wikipedia." ;
    skos:inScheme cs: ;
    skos:notation "4011"^^<https://linked.data.gov.au/def/anzsrc-for/2020> ;
    skos:prefLabel "environmental engineering"@en ;
    schema:citation "https://en.wikipedia.org/wiki/Environmental_engineering"^^xsd:anyURI ;
.

:environmental-geochemistry
    a skos:Concept ;
    rdfs:isDefinedBy cs: ;
    skos:broader :environmental-sciences ;
    skos:definition "The study of the effect on humans (and life in general) of the distribution and interrelations of the chemical elements and radioactivity among surficial rocks, water, air, and biota."@en ;
    skos:historyNote "Definition adapted from Glossary of geology (5th edition revised; Neuendorf et al., 2011)." ;
    skos:inScheme cs: ;
    skos:prefLabel "environmental geochemistry"@en ;
    schema:citation "https://glossary.americangeosciences.org/term/environmentalgeochemistry"^^xsd:anyURI ;
.

:experimental-mineralogy
    a skos:Concept ;
    rdfs:isDefinedBy cs: ;
    skos:broader :mineralogy ;
    skos:definition "Experimental mineralogy and petrology are the Earth science disciplines that model or simulate mineralogical, petrological, and geochemical processes within the laboratory in order to understand the physical and chemical properties of minerals, rocks, melts, and fluids and their interactions."@en ;
    skos:historyNote """Definition from:
Geiger, CA and Kawamoto, T 2017, Experimental Mineralogy and Petrology, Encyclopedia of Geochemistry, Encyclopedia of Earth Sciences Series, edited by W White: Springer, Cham, doi.org/10.1007/978-3-319-39193-9_311-2.""" ;
    skos:inScheme cs: ;
    skos:prefLabel "experimental mineralogy"@en ;
    schema:citation "https://link.springer.com/referenceworkentry/10.1007/978-3-319-39193-9_311-1"^^xsd:anyURI ;
.

:experimental-petrology
    a skos:Concept ;
    rdfs:isDefinedBy cs: ;
    skos:broader :petrology ;
    skos:definition "A discipline that employs high-pressure, high-temperature apparatus to investigate the geochemistry and phase relations of natural or synthetic materials at elevated pressures and temperatures. Experiments are particularly useful for investigating rocks of the lower crust and upper mantle that rarely survive the journey to the surface in pristine condition. They are also one of the prime sources of information about completely inaccessible rocks, such as those in the Earth's lower mantle and in the mantles of the other terrestrial planets and the Moon. The work of experimental petrologists has laid a foundation on which modern understanding of igneous and metamorphic processes has been built."@en ;
    skos:historyNote "Definition adapted from Wikipedia." ;
    skos:inScheme cs: ;
    skos:prefLabel "experimental petrology"@en ;
    schema:citation "https://en.wikipedia.org/wiki/Petrology"^^xsd:anyURI ;
.

:exploration-geochemistry
    a skos:Concept ;
    rdfs:isDefinedBy
        cs: ,
        <https://linked.data.gov.au/def/anzsrc-for/2020> ;
    skos:broader :geochemistry ;
    skos:definition "Geochemistry that is specifically focused on identification of mineralization, its dispersion haloes, alteration patterns and distribution. It specifically focuses on the enrichment or depletion of certain elements (including pathfinders) having a genetic affinity to the target mineralization. Exploration geochemistry is typical of exploration stages aiming at locating mineral deposits but also applies to the near-mine exploration conducted to further locate and delineate resources."@en ;
    skos:exactMatch <https://linked.data.gov.au/def/anzsrc-for/2020/370301> ;
    skos:historyNote """Definition adapted from: 
Moon, C 2021, Exploration Geochemistry, in Encyclopedia of Geology (Second Edition), edited by D Alderton and SA Elias: Academic Press, p. 209–218, doi.org/10.1016/B978-0-08-102908-4.00017-5.""" ;
    skos:inScheme cs: ;
    skos:notation "370301"^^<https://linked.data.gov.au/def/anzsrc-for/2020> ;
    skos:prefLabel "exploration geochemistry"@en ;
    schema:citation
        "https://www.sciencedirect.com/science/article/abs/pii/B9780081029084000175"^^xsd:anyURI ,
        "https://www.sciencedirect.com/science/article/abs/pii/B9780128140222000058"^^xsd:anyURI ;
.

:extraterrestrial-geology
    a skos:Concept ;
    rdfs:isDefinedBy
        cs: ,
        <https://linked.data.gov.au/def/anzsrc-for/2020> ;
    skos:altLabel
        "astrogeology"@en ,
        "exogeology"@en ,
        "planetary geology"@en ;
    skos:broader :geology ;
    skos:definition "A planetary science discipline concerned with the geology of celestial bodies such as the planets and their moons, asteroids, comets, and meteorites, i.e. a science that applies principles and techniques of geology, geochemistry, and geophysics to the study of the nature, origin, and history of the condensed matter and gases in the solar system and beyond. It includes a) remote-sensing observations and in situ manned exploration of other planetary bodies, such as the Moon and Mars, Venus, Mercury, and 'earthlike' or 'rocky' satellite moons of the giant planets; b) the study of the chemistry, mineralogy (cosmic mineralogy), and history of objects that occur on the Earth but are of known or possible extraterrestrial origin (such as meteorites and tektites) or that are returned to the Earth (such as lunar samples); and c) the study of the effects of extraterrestrial processes (such as meteorite impact, solar energy changes, and tides) on the Earth in the present and past."@en ;
    skos:exactMatch
        <https://linked.data.gov.au/def/anzsrc-for/2020/370507> ,
        <https://linked.data.gov.au/def/earth-science-data-category/extraterrestrial-geology> ;
    skos:historyNote "Adapted from the Fields of Research vocabulary from the Australian and New Zealand Standard Research Classification (ANZSRC, 2020). Definition adapted from Glossary of geology (5th edition revised; Neuendorf et. al., 2011) and Wikipedia." ;
    skos:inScheme cs: ;
    skos:notation "370507"^^<https://linked.data.gov.au/def/anzsrc-for/2020> ;
    skos:prefLabel "extraterrestrial geology"@en ;
    schema:citation
        "https://en.wikipedia.org/wiki/Planetary_geology"^^xsd:anyURI ,
        "https://glossary.americangeosciences.org/term/planetarygeology"^^xsd:anyURI ;
.

:fluid-extract-geochemistry
    a skos:Concept ;
    rdfs:isDefinedBy
        cs: ,
        <https://linked.data.gov.au/def/earth-science-data-category> ;
    skos:broader :geochemistry ;
    skos:definition "Analysis of the chemical and physical properties of fluids extracted from rocks and geological materials in the subsurface."@en ;
    skos:exactMatch <https://linked.data.gov.au/def/earth-science-data-category/fluid-extract-geochemistry> ;
    skos:historyNote "Definition from Geological Survey of Queensland Earth science data category vocabulary." ;
    skos:inScheme cs: ;
    skos:prefLabel "fluid extract geochemistry"@en ;
    schema:citation "https://linked.data.gov.au/def/earth-science-data-category/fluid-extract-geochemistry"^^xsd:anyURI ;
.

:fluid-inclusion-geochemistry
    a skos:Concept ;
    rdfs:isDefinedBy cs: ;
    skos:broader :geochemistry ;
    skos:definition "The study of the composition, stratigraphy and petrology of liquids and/or gases contained within tiny (usually in the order of micrometres) cavities formed either by the entrapment in crystal irregularities of fluids from which the mineral/rock crystallized, or by any process after the crystallization of the host mineral is essentially complete (e.g. healing of fractures within a crystal)."@en ;
    skos:historyNote "Compiled by the Geological Survey of Western Australia. Definition adapted from Glossary of geology (5th edition, revised; Neuendorf et al., 2011)." ;
    skos:inScheme cs: ;
    skos:prefLabel "fluid inclusion geochemistry"@en ;
    schema:citation
        "https://glossary.americangeosciences.org/term/fluidinclusion"^^xsd:anyURI ,
        "https://glossary.americangeosciences.org/term/primaryfluidinclusion"^^xsd:anyURI ,
        "https://glossary.americangeosciences.org/term/secondaryinclusion"^^xsd:anyURI ;
.

:fluid-inclusion-petrology
    a skos:Concept ;
    rdfs:isDefinedBy cs: ;
    skos:altLabel
        "fluid inclusion analysis"@en ,
        "fluid inclusion studies"@en ;
    skos:broader :petrology ;
    skos:definition "The study of tiny encapsulations of fluids that trap oil, gas, water and solid phases in minerals and rocks to determine parameters such as temperature, pressure, salinity, density and depth of trapping — thereby providing direct information about the conditions of formation. In the case of hydrocarbon exploration, these studies are conducted to assess the fluid history of the rock/sedimentary basin and the prevailing thermal conditions, to determine whether oil and gas are likely to be found at a particular location, as well as the source and type of hydrocarbon present."@en ;
    skos:historyNote "Compiled by Geological Survey of Western Australia from multiple sources." ;
    skos:inScheme cs: ;
    skos:prefLabel "fluid inclusion petrology"@en ;
    schema:citation
        "https://www.csiro.au/en/research/technology-space/energy/Offshore-oil-and-gas/Fluid-inclusion-analysis"^^xsd:anyURI ,
        "https://www.researchgate.net/publication/275337661_Study_of_Fluid_Inclusions_Methods_Techniques_and_Applications"^^xsd:anyURI ;
.

:forensic-geology
    a skos:Concept ;
    rdfs:isDefinedBy cs: ;
    skos:altLabel "geoforensics"@en ;
    skos:broader :geology ;
    skos:definition "The study of trace evidence provided by Earth materials that is used to answer questions raised by the legal system, specifically the potential to link a suspect to a particular crime or a particular crime scene."@en ;
    skos:historyNote "Definition from Wikipedia." ;
    skos:inScheme cs: ;
    skos:prefLabel "forensic geology"@en ;
    schema:citation "https://en.wikipedia.org/wiki/Forensic_geology"^^xsd:anyURI ;
.

:functional-morphology
    a skos:Concept ;
    rdfs:isDefinedBy cs: ;
    skos:broader :morphological-paleontology ;
    skos:definition "Functional morphology is an interpretative subdiscipline of paleobiology, and is the study of the form, structure and function of organisms or parts of organisms in terms of the biological roles that they play (i.e. function and behaviour)."@en ;
    skos:historyNote """Definition adapted from:
Cowen, R 1979, Morphology, functional: in Paleontology, Encyclopedia of Earth Science; Springer, Berlin, Heidelberg, doi:10.1007/3-540-31078-9_89.""" ;
    skos:inScheme cs: ;
    skos:prefLabel "functional morphology"@en ;
    schema:citation "https://glossary.americangeosciences.org/term/functionalmorphology"^^xsd:anyURI ;
.

:gemmology
    a skos:Concept ;
    rdfs:isDefinedBy cs: ;
    skos:altLabel "gemology"@en ;
    skos:broader :mineralogy-and-crystallography ;
    skos:definition "The science and study of natural and artificial gemstones, including their source, description, geology, origin, identification, grading and appraisal."@en ;
    skos:exactMatch <https://linked.data.gov.au/def/earth-science-data-category/gemmology> ;
    skos:historyNote "Definition adapted from Glossary of geology (5th edition revised; Neuendorf et al., 2011)." ;
    skos:inScheme cs: ;
    skos:prefLabel "gemmology"@en ;
    schema:citation "https://glossary.americangeosciences.org/term/gemology"^^xsd:anyURI ;
.

:genetic-mineralogy
    a skos:Concept ;
    rdfs:isDefinedBy cs: ;
    skos:broader :mineralogy ;
    skos:definition "The empirical investigation of the principles that control mineral formation in the geological environment, including mineral paragenesis and the physical and chemical parameters of formation and alteration (mineral ontogenesis); the quantitative geothermometric, geobarometric, and chemical studies of mineral-forming systems; and experimental modelling of crystal growth in the laboratory."@en ;
    skos:historyNote """Definition from: 
Wenk H-R and Bulakh A, 2004, Mineral genesis: in Minerals: Their Constitution and Origin, Cambridge University Press, p. 276–287.""" ;
    skos:inScheme cs: ;
    skos:prefLabel "genetic mineralogy"@en ;
    schema:citation "https://assets.cambridge.org/97805215/29587/frontmatter/9780521529587_frontmatter.pdf"^^xsd:anyURI ;
.

:geoarcheology
    a skos:Concept ;
    rdfs:isDefinedBy cs: ;
    skos:altLabel "geoarchaeology"@en ;
    skos:broader :archeology ;
    skos:definition "A multi-disciplinary approach that uses the techniques and subject matter of geography, geology, geophysics and other Earth sciences to examine topics which inform archeological and chronological knowledge and thought. Geoarcheologists study the natural physical processes that affect archeological sites such as geomorphology, the formation of sites through geological processes and the effects on buried sites and artifacts post-deposition."@en ;
    skos:historyNote "Definition adapted from Wikipedia." ;
    skos:inScheme cs: ;
    skos:prefLabel "geoarcheology"@en ;
    schema:citation "https://en.wikipedia.org/wiki/Geoarchaeology"^^xsd:anyURI ;
.

:geochemistry-not-elsewhere-classified
    a skos:Concept ;
    rdfs:isDefinedBy
        cs: ,
        <https://linked.data.gov.au/def/anzsrc-for/2020> ;
    skos:broader :geochemistry ;
    skos:definition "Geochemical data and information not otherwise described by other sub-categories of geochemistry."@en ;
    skos:exactMatch
        <https://linked.data.gov.au/def/anzsrc-for/2020/370399> ,
        <https://linked.data.gov.au/def/earth-science-data-category/geochemistry-not-elsewhere-classified> ;
    skos:historyNote "From the Fields of Research vocabulary from the Australian and New Zealand Standard Research Classification (ANZSRC, 2020). Definition from Geological Survey of Queensland Earth science data category vocabulary." ;
    skos:inScheme cs: ;
    skos:notation "370399"^^<https://linked.data.gov.au/def/anzsrc-for/2020> ;
    skos:prefLabel "geochemistry not elsewhere classified"@en ;
    schema:citation "https://linked.data.gov.au/def/earth-science-data-category/geochemistry-not-elsewhere-classified"^^xsd:anyURI ;
.

:geoconservation
    a skos:Concept ;
    rdfs:isDefinedBy cs: ;
    skos:broader :land-use-and-environmental-planning ;
    skos:definition "The practice of protecting and managing sites and landscapes which have value for their geology or geomorphology. The identification (cf. geoheritage) and conservation of these geological sites is through government agencies and local geological societies. The designation of these sites is done through an analysis of the site, and the production of proper management infrastructure. The principles of geoconservation are to create a means of protection for the sites and assess their value to the geological and wider community. Typically the conservation of geodiversity at a site or within a landscape takes place alongside that of biodiversity."@en ;
    skos:historyNote "Compiled by the Geological Survey of Western Australia. Definition adapted from Wikipedia." ;
    skos:inScheme cs: ;
    skos:prefLabel "geoconservation"@en ;
    schema:citation "https://en.wikipedia.org/wiki/Geoconservation"^^xsd:anyURI ;
.

:geodynamics
    a skos:Concept ;
    rdfs:isDefinedBy
        cs: ,
        <https://linked.data.gov.au/def/anzsrc-for/2020> ;
    skos:broader :geophysics ;
    skos:definition "A subfield of geophysics dealing with the forces and processes of the interior of the Earth. It applies physics, chemistry and mathematics to the understanding of how mantle convection leads to plate tectonics and geological phenomena such as seafloor spreading, mountain building, volcanoes, earthquakes, faulting and so on. It also attempts to probe the internal activities of the Earth by measuring magnetic fields, gravity, and seismic waves, as well as the mineralogy of rocks and their isotopic composition."@en ;
    skos:exactMatch
        <https://linked.data.gov.au/def/anzsrc-for/2020/370604> ,
        <https://linked.data.gov.au/def/earth-science-data-category/geodynamics> ;
    skos:historyNote "From the Fields of Research vocabulary from the Australian and New Zealand Standard Research Classification (ANZSRC, 2020). Definition adapted from Glossary of geology (5th edition revised; Neuendorf et al., 2011) and Wikipedia." ;
    skos:inScheme cs: ;
    skos:notation "370604"^^<https://linked.data.gov.au/def/anzsrc-for/2020> ;
    skos:prefLabel "geodynamics"@en ;
    schema:citation "https://en.wikipedia.org/wiki/Geodynamics"^^xsd:anyURI ;
.

:geoethics
    a skos:Concept ;
    rdfs:isDefinedBy cs: ;
    skos:broader :earth-sciences ;
    skos:definition "The branch of ethics that considers the interaction of human activity with the physical world and with the practice of the Earth Sciences. It comprises scientific research and philosophical reflection on the values governing human behaviours wherever they interact with the Earth system, including the ethical, social, and cultural implications of the activities of geoscientists when conducting scientific and technological research and practice."@en ;
    skos:historyNote "Definition adapted from Wikipedia." ;
    skos:inScheme cs: ;
    skos:prefLabel "geoethics"@en ;
    schema:citation "https://en.wikipedia.org/wiki/Geoethics"^^xsd:anyURI ;
.

:geographic-information-science
    a skos:Concept ;
    rdfs:isDefinedBy cs: ;
    skos:altLabel "GIScience"@en ;
    skos:broader :geomatic-engineering ;
    skos:definition "Geographic Information Science (GIScience) is the basic research field that seeks to redefine geographic concepts and their use in the context of geographic information systems. GIScience also examines the impacts of GIS on individuals and society, and the influences of society on GIS. GIScience re-examines some of the most fundamental themes in traditional spatially oriented fields such as geography, cartography, and geodesy, while incorporating more recent developments in cognitive and information science"@en ;
    skos:historyNote """Definition adapted from:
1) Wikipedia
2) ISO/TR 19122:2004(en) - Geographic information / Geomatics.""" ;
    skos:inScheme cs: ;
    skos:prefLabel "Geographic Information Science (GIScience)"@en ;
    schema:citation "https://www.iso.org/obp/ui/#iso:std:iso:tr:19122:en"^^xsd:anyURI ;
.

:geohazard
    a skos:Concept ;
    rdfs:isDefinedBy cs: ;
    skos:broader :geology ;
    skos:definition "The study of adverse geological conditions capable of causing widespread damage or loss of property and life. These hazards are geological and environmental conditions and involve long-term or short-term geological processes. Geohazards can be relatively small features (e.g. geyser) but can also attain huge dimensions (e.g. submarine or surface landslide) and affect local and regional socio-economics to a large extent (e.g. tsunamis, volcanic eruptions)."@en ;
    skos:historyNote "Definition adapted from Wikipedia." ;
    skos:inScheme cs: ;
    skos:prefLabel "geohazard"@en ;
    schema:citation "https://en.wikipedia.org/wiki/Geological_hazard"^^xsd:anyURI ;
.

:geoheritage
    a skos:Concept ;
    rdfs:isDefinedBy cs: ;
    skos:broader <https://linked.data.gov.au/def/earthsci-for/history-heritage-and-archeology> ;
    skos:definition "The identification of global, national, state-wide, or local features of geology (such as igneous, metamorphic, sedimentary, stratigraphic, structural, geochemical, mineralogical, paleontological, geomorphical, pedological, and hydrological attributes) that are: (a) intrinsically important or culturally important sites; (b) offer information or insights into the formation or evolution of the Earth, or into the history of science, or (c) that can be used for research, teaching, or reference. Geoheritage is inextricably linked to geoconservation, for the preservation of these sites for posterity."@en ;
    skos:historyNote """Definition adapted from:
Brocx, M and Semeniuk, V 2007, Geoheritage and geoconservation — history, definition, scope and scale: Journal of the Royal Society of Western Australia, v. 90, p. 53–87.""" ;
    skos:inScheme cs: ;
    skos:prefLabel "geoheritage"@en ;
    schema:citation
        "https://en.wikipedia.org/wiki/Geoheritage"^^xsd:anyURI ,
        "https://www.demirs.wa.gov.au/geoheritage"^^xsd:anyURI ;
.

:geoinformatics-not-elsewhere-classified
    a skos:Concept ;
    rdfs:isDefinedBy
        cs: ,
        <https://linked.data.gov.au/def/anzsrc-for/2020> ;
    skos:broader :geoinformatics ;
    skos:definition "Geoinformatics data and information not otherwise described by other sub-categories of geoinformatics."@en ;
    skos:exactMatch <https://linked.data.gov.au/def/anzsrc-for/2020/370499> ;
    skos:historyNote "From the Fields of Research vocabulary from the Australian and New Zealand Standard Research Classification (ANZSRC, 2020)." ;
    skos:inScheme cs: ;
    skos:notation "370499"^^<https://linked.data.gov.au/def/anzsrc-for/2020> ;
    skos:prefLabel "geoinformatics not elsewhere classified"@en ;
.

:geological-mapping
    a skos:Concept ;
    rdfs:isDefinedBy cs: ;
    skos:altLabel "geoscience mapping"@en ;
    skos:broader :geology ;
    skos:definition "The process of making observations in the field, as well as collecting and studying samples of Earth's materials to understand the geology of an area, and more specifically to produce a diagram, drawing, or other graphical representation of the area in question, by means of signs and/or symbols and with the means of orientation indicated, so that the relative position and size of each feature on the map corresponds to its correct geographical situation according to a definite and established scale and projection."@en ;
    skos:historyNote "Compiled by the Geological Survey of Western Australia" ;
    skos:inScheme cs: ;
    skos:prefLabel "geological mapping"@en ;
    schema:citation "https://glossary.americangeosciences.org/term/map"^^xsd:anyURI ;
.

:geological-modelling
    a skos:Concept ;
    rdfs:isDefinedBy cs: ;
    skos:altLabel
        "geo-modelling"@en ,
        "geomodelling"@en ;
    skos:broader :geoscience-data-visualisation ;
    skos:definition "The applied science of creating computerized representations of portions of the Earth’s subsurface based on geophysical and geological observations made on and below the Earth surface."@en ;
    skos:historyNote "Compiled by Geological Survey of Western Australia. Definition adapted from https://courses.lumenlearning.com/geo/chapter/geologic-modelling/." ;
    skos:inScheme cs: ;
    skos:prefLabel "geological modelling"@en ;
    schema:citation "https://courses.lumenlearning.com/geo/chapter/geologic-modelling/"^^xsd:anyURI ;
.

:geology-not-elsewhere-classified
    a skos:Concept ;
    rdfs:isDefinedBy
        cs: ,
        <https://linked.data.gov.au/def/anzsrc-for/2020> ;
    skos:broader :geology ;
    skos:definition "Geological data and information not otherwise described by other sub-categories of geology."@en ;
    skos:exactMatch
        <https://linked.data.gov.au/def/anzsrc-for/2020/370599> ,
        <https://linked.data.gov.au/def/earth-science-data-category/geology-not-elsewhere-classified> ;
    skos:historyNote "From the Fields of Research vocabulary from the Australian and New Zealand Standard Research Classification (ANZSRC, 2020)." ;
    skos:inScheme cs: ;
    skos:notation "370599"^^<https://linked.data.gov.au/def/anzsrc-for/2020> ;
    skos:prefLabel "geology not elsewhere classified"@en ;
    schema:citation "https://linked.data.gov.au/def/earth-science-data-category/geology-not-elsewhere-classified"^^xsd:anyURI ;
.

:geomatic-engineering-not-elsewhere-classified
    a skos:Concept ;
    rdfs:isDefinedBy
        cs: ,
        <https://linked.data.gov.au/def/anzsrc-for/2020> ;
    skos:broader :geomatic-engineering ;
    skos:definition "Geomatic engineering data and information not otherwise described by other sub-categories of geomatics engineering."@en ;
    skos:exactMatch <https://linked.data.gov.au/def/anzsrc-for/2020/401399> ;
    skos:historyNote "From the Fields of Research vocabulary from the Australian and New Zealand Standard Research Classification (ANZSRC, 2020)." ;
    skos:inScheme cs: ;
    skos:notation "401399"^^<https://linked.data.gov.au/def/anzsrc-for/2020> ;
    skos:prefLabel "geomatic engineering not elsewhere classified"@en ;
.

:geomatics
    a skos:Concept ;
    rdfs:isDefinedBy cs: ;
    skos:altLabel "spatial science"@en ;
    skos:broader :geomatic-engineering ;
    skos:definition "The discipline concerned with the collection, distribution, storage, analysis, processing, presentation of geographic data or geographic information, as well as the products, services and tools involved in the collection, integration and management of geographic (geospatial) data."@en ;
    skos:historyNote """Definition adapted from:
1) Wikipedia
2) ISO/TR 19122:2004(en) - Geographic information / Geomatics.""" ;
    skos:inScheme cs: ;
    skos:prefLabel "geomatics"@en ;
    schema:citation
        "https://en.wikipedia.org/wiki/Geomatics"^^xsd:anyURI ,
        "https://www.appliedgeomatics.net/about-us.html"^^xsd:anyURI ,
        "https://www.iso.org/obp/ui/#iso:std:iso:tr:19122:en"^^xsd:anyURI ;
.

:geomechanics-and-resources-geotechnical-engineering
    a skos:Concept ;
    rdfs:isDefinedBy
        cs: ,
        <https://linked.data.gov.au/def/anzsrc-for/2020> ;
    skos:broader :resources-engineering ;
    skos:definition "A branch at the intersection of geology and engineering that embraces the fundamentals of structural geology and a knowledge of the response, or strain, of earth materials (soil and rocks) to deformation or changes caused by the application of stress and/or strain energy, as well as the application of such studies to solve engineering problems in the design of engineering works."@en ;
    skos:exactMatch <https://linked.data.gov.au/def/anzsrc-for/2020/401902> ;
    skos:historyNote "Definition adapted from Glossary of geology (5th edition revised; Neuendorf et al., 2011) and Wikipedia." ;
    skos:inScheme cs: ;
    skos:narrowMatch <https://linked.data.gov.au/def/earth-science-data-category/geomechanics-and-resources-geotechnical-engineering> ;
    skos:notation "401902"^^<https://linked.data.gov.au/def/anzsrc-for/2020> ;
    skos:prefLabel "geomechanics and resources geotechnical engineering"@en ;
    schema:citation
        "https://en.wikipedia.org/wiki/Geomechanics"^^xsd:anyURI ,
        "https://glossary.americangeosciences.org/term/geomechanics"^^xsd:anyURI ,
        "https://linked.data.gov.au/def/earth-science-data-category/geomechanics-and-resources-geotechnical-engineering"^^xsd:anyURI ;
.

:geometallurgy
    a skos:Concept ;
    rdfs:isDefinedBy cs: ;
    skos:broader :mining-geology ;
    skos:definition "The practice of combining geology or geostatistics with extractive metallurgy, to create a spatially or geologically based predictive model to optimize the efficiency of mineral processing plants. Geometallurgy specifically maps the 3D variability in petrophysical and mineralogical properties of an entire orebody, to define domains that require different mining and metallurgical processing techniques, to maximize recovery of the saleable product at minimum cost."@en ;
    skos:historyNote "Definition compiled by the Geological Survey of Western Australia (partly adapted from Wikipedia)." ;
    skos:inScheme cs: ;
    skos:prefLabel "geometallurgy"@en ;
    schema:citation "https://en.wikipedia.org/wiki/Geometallurgy"^^xsd:anyURI ;
.

:geomorphology-and-earth-surface-processes
    a skos:Concept ;
    rdfs:isDefinedBy
        cs: ,
        <https://linked.data.gov.au/def/anzsrc-for/2020> ;
    skos:altLabel
        "physical geology"@en ,
        "physiographic geology"@en ;
    skos:broader :physical-geography-and-environmental-geoscience ;
    skos:closeMatch <https://linked.data.gov.au/def/earth-science-data-category/geomorphology-and-regolith-and-landscape-evolution> ;
    skos:definition "The scientific study of the general configuration of the Earth's surface, i.e. of the origin and evolution of topographic and bathymetric features created by physical, chemical or biological processes operating at or near the Earth's surface. Specifically studies dealing with the classification, description, nature, origin, processes, and development of present landforms and their relationships to underlying structures, and of the history of geological changes as recorded by these surface features. Geomorphology overlaps in meaning with physiography, with 'physiography' commonly regarded as a more descriptive and 'geomorphology' as a more interpretative study of landforms."@en ;
    skos:exactMatch <https://linked.data.gov.au/def/anzsrc-for/2020/370901> ;
    skos:historyNote "From the Fields of Research vocabulary from the Australian and New Zealand Standard Research Classification (ANZSRC, 2020). Definition adapted from Glossary of geology (5th edition revised; Neuendorf et al., 2011) and Wikipedia." ;
    skos:inScheme cs: ;
    skos:notation "370901"^^<https://linked.data.gov.au/def/anzsrc-for/2020> ;
    skos:prefLabel "geomorphology and earth surface processes"@en ;
    schema:citation
        "https://en.wikipedia.org/wiki/Geomorphology"^^xsd:anyURI ,
        "https://glossary.americangeosciences.org/term/geomorphology"^^xsd:anyURI ,
        "https://glossary.americangeosciences.org/term/physiography"^^xsd:anyURI ;
.

:geophysical-fluid-dynamics
    a skos:Concept ;
    rdfs:isDefinedBy cs: ;
    skos:broader :geophysics ;
    skos:definition "The study of fluid dynamics of naturally occurring flows, such as lava flows, oceans, and planetary atmospheres, on Earth and other planets."@en ;
    skos:exactMatch <https://linked.data.gov.au/def/earth-science-data-category/geophysical-fluid-dynamics> ;
    skos:historyNote "Definition adapted from Wikipedia." ;
    skos:inScheme cs: ;
    skos:prefLabel "geophysical fluid dynamics"@en ;
    schema:citation "https://en.wikipedia.org/wiki/Geophysical_fluid_dynamics"^^xsd:anyURI ;
.

:geophysical-modelling
    a skos:Concept ;
    rdfs:isDefinedBy cs: ;
    skos:broader :geoscience-data-visualisation ;
    skos:definition "The applied science of creating computerized representations of the Earth based on geophysical and geological observations and their interpretation. Geophysical models are a simplified concept and/or visualization of how one or more physical properties are distributed within the Earth. They are generally an object, a halfspace, 1D (layered earth), 2D, or 3D."@en ;
    skos:historyNote "Compiled by Geological Survey of Western Australia. Definition adapted from multiple sources." ;
    skos:inScheme cs: ;
    skos:prefLabel "geophysical modelling"@en ;
    schema:citation
        "https://emrlibrary.gov.yk.ca/ygs/MR/MR-10/MR-10_AppendixB_Mira AGIC Glossary of Useful Terms.pdf"^^xsd:anyURI ,
        "https://www.scitechnol.com/scholarly/geophysical-modeling-and-interpretation-journals-articles-ppts-list.php"^^xsd:anyURI ;
.

:geophysics-not-elsewhere-classified
    a skos:Concept ;
    rdfs:isDefinedBy
        cs: ,
        <https://linked.data.gov.au/def/anzsrc-for/2020> ;
    skos:broader :geophysics ;
    skos:definition "Geophysical data and information not otherwise described by other sub-categories of geophysics."@en ;
    skos:exactMatch
        <https://linked.data.gov.au/def/anzsrc-for/2020/370699> ,
        <https://linked.data.gov.au/def/earth-science-data-category/geophysics-not-elsewhere-classified> ;
    skos:historyNote "From the Fields of Research vocabulary from the Australian and New Zealand Standard Research Classification (ANZSRC, 2020)." ;
    skos:inScheme cs: ;
    skos:notation "370699"^^<https://linked.data.gov.au/def/anzsrc-for/2020> ;
    skos:prefLabel "geophysics not elsewhere classified"@en ;
.

:geoscience-communication
    a skos:Concept ;
    rdfs:isDefinedBy cs: ;
    skos:altLabel "Earth science communication"@en ;
    skos:broader :stakeholder-engagement ;
    skos:definition "A variety of practices that transmit scientific ideas, methods, knowledge, and research to non-expert audiences in an accessible, understandable, or useful way, with a particular focus on subjects related to Earth's physical features, processes, and systems."@en ;
    skos:historyNote "Compiled by the Geological Survey of Western Australia." ;
    skos:inScheme cs: ;
    skos:prefLabel "geoscience communication"@en ;
    schema:citation "https://link.springer.com/chapter/10.1007/978-981-97-2815-2_1"^^xsd:anyURI ;
.

:geoscience-education
    a skos:Concept ;
    rdfs:isDefinedBy cs: ;
    skos:altLabel "Earth science education"@en ;
    skos:broader :stakeholder-engagement ;
    skos:definition "Also known as Earth science education, it is the study of Earth's physical features, processes, and systems, as well as the natural and human-induced events that shape it. It encompasses a wide range of disciplines, including geology, oceanography, meteorology, climatology, environmental science, and more. Geoscience education plays a crucial role in fostering scientific literacy, environmental awareness, and sustainable development, as well as in preparing future generations of geoscientists, policymakers, educators, and citizens."@en ;
    skos:historyNote "Compiled by the Geological Survey of Western Australia. Definition adapted from Wikipedia." ;
    skos:inScheme cs: ;
    skos:prefLabel "geoscience education"@en ;
    schema:citation "https://en.wikipedia.org/wiki/Geoscience_education"^^xsd:anyURI ;
.

:geospatial-information-systems-and-geospatial-data-modelling
    a skos:Concept ;
    rdfs:isDefinedBy
        cs: ,
        <https://linked.data.gov.au/def/anzsrc-for/2020> ;
    skos:broader :geomatic-engineering ;
    skos:definition "The application of geographic information systems (GIS), i.e. an integrated computer hardware and software, to store, manage, analyse, edit, output, visualize and model geographic data."@en ;
    skos:exactMatch <https://linked.data.gov.au/def/anzsrc-for/2020/401302> ;
    skos:historyNote "From the Fields of Research vocabulary from the Australian and New Zealand Standard Research Classification (ANZSRC, 2020). Definition adapted from Wikipedia." ;
    skos:inScheme cs: ;
    skos:notation "401302"^^<https://linked.data.gov.au/def/anzsrc-for/2020> ;
    skos:prefLabel "geospatial information systems and geospatial data modelling"@en ;
    schema:citation "https://en.wikipedia.org/wiki/Geographic_information_system"^^xsd:anyURI ;
.

:geostatistics
    a skos:Concept ;
    rdfs:isDefinedBy cs: ;
    skos:broader :geomathematics ;
    skos:definition "A branch of statistics focusing on spatial or spatiotemporal datasets, developed originally to predict probability distributions of ore grades for mining operations, but now applied also in petroleum geology, hydrogeology, hydrology, meteorology, oceanography, geochemistry, geometallurgy, geography, forestry, environmental control, landscape ecology, soil science and agriculture."@en ;
    skos:historyNote "Definition from Wikipedia." ;
    skos:inScheme cs: ;
    skos:prefLabel "geostatistics"@en ;
    schema:citation "https://en.wikipedia.org/wiki/Geostatistics"^^xsd:anyURI ;
.

:geostorage-engineering
    a skos:Concept ;
    rdfs:isDefinedBy cs: ;
    skos:broader :resources-engineering ;
    skos:definition "Engineering applied to the capture and storage of materials (commonly liquids and gases, and especially greenhouse gases) or energy (commonly gas or heat) in the subsurface of the Earth."@en ;
    skos:exactMatch <https://linked.data.gov.au/def/earth-science-data-category/geostorage-engineering> ;
    skos:historyNote "Definition adapted from University of New south Wales website and Geological Survey of Queensland Earth science data category vocabulary." ;
    skos:inScheme cs: ;
    skos:prefLabel "geostorage engineering"@en ;
    schema:citation
        "https://linked.data.gov.au/def/earth-science-data-category/geostorage-engineering"^^xsd:anyURI ,
        "https://www.unsw.edu.au/news/2021/07/geostorage--why-is-it-so-important-in-the-zero-carbon-world-"^^xsd:anyURI ;
.

:geotechnical-engineering
    a skos:Concept ;
    rdfs:isDefinedBy cs: ;
    skos:altLabel "geotechnics"@en ;
    skos:broader :geology ;
    skos:definition "A field at the intersection of geology and engineering dealing with the study of the engineering behaviours of earth materials to address engineering problems. It uses soil and rock mechanics for practical applications in, amongst other disciplines, mining engineering, petroleum engineering, coastal engineering, and onshore/offshore construction."@en ;
    skos:historyNote "Definition adapted from Wikipedia." ;
    skos:inScheme cs: ;
    skos:prefLabel "geotechnical engineering"@en ;
    schema:citation "https://en.wikipedia.org/wiki/Geotechnical_engineering"^^xsd:anyURI ;
.

:geothermal-resource-geology
    a skos:Concept ;
    rdfs:isDefinedBy cs: ;
    skos:broader :energy-geoscience ;
    skos:definition "The study of the accessible thermal energy stored within the Earth's crust, in order to access and extract it. It includes studies of related geological systems and the methods, materials and operations used in the production of energy."@en ;
    skos:exactMatch <https://linked.data.gov.au/def/earth-science-data-category/geothermal-resource-geology> ;
    skos:historyNote "Definition adapted from Glossary of geology (5th edition revised; Neuendorf et al., 2011) and Wikipedia." ;
    skos:inScheme cs: ;
    skos:prefLabel "geothermal resource geology"@en ;
    schema:citation
        "https://en.wikipedia.org/wiki/Geothermal_energy"^^xsd:anyURI ,
        "https://glossary.americangeosciences.org/term/geothermalresource"^^xsd:anyURI ;
.

:geothermics
    a skos:Concept ;
    rdfs:isDefinedBy cs: ;
    skos:broadMatch <https://linked.data.gov.au/def/anzsrc-for/2020/370605> ;
    skos:broader :geothermics-and-radiometrics ;
    skos:definition "A subdiscipline of geophysics that studies the thermal state of the interior of the solid Earth and of the thermal properties of Earth materials. Components of geothermal research are temperature distribution within the Earth, terrestrial heat flow, heat generation, thermal properties of Earth materials, volcanology, geothermal energy, hydrocarbon formation, fluid flow, and permafrost. Cf. temperature studies."@en ;
    skos:historyNote "Definition adapted from Glossary of geology (5th edition revised; Neuendorf et al., 2011)." ;
    skos:inScheme cs: ;
    skos:prefLabel "geothermics"@en ;
    schema:citation "https://glossary.americangeosciences.org/term/geothermics"^^xsd:anyURI ;
.

:geotourism
    a skos:Concept ;
    rdfs:isDefinedBy cs: ;
    skos:broader :land-use-and-environmental-planning ;
    skos:definition "Tourism that sustains or enhances the distinctive geographical character of a place — its environment, heritage, aesthetics, culture, and the well-being of its residents."@en ;
    skos:historyNote "Compiled by the Geological Survey of Western Australia. Definition from the Australian Geoscience Council." ;
    skos:inScheme cs: ;
    skos:prefLabel "geotourism"@en ;
    schema:citation "https://www.agc.org.au/wp-content/uploads/2023/06/Understanding-Geotourism-GeoRegions-and-Geoparks-in-Australia-NGS-June-2023.pdf"^^xsd:anyURI ;
.

:glaciology
    a skos:Concept ;
    rdfs:isDefinedBy
        cs: ,
        <https://linked.data.gov.au/def/anzsrc-for/2020> ;
    skos:altLabel "cryology"@en ;
    skos:broader :physical-geography-and-environmental-geoscience ;
    skos:definition "The scientific discipline concerned with all aspects of ice and solid water on landmasses. It deals with the structure and properties of glaciers and ice sheets, their physical properties, formation and distribution, the dynamics of ice flow, and the interactions of ice accumulation with climate."@en ;
    skos:exactMatch
        <https://linked.data.gov.au/def/anzsrc-for/2020/370902> ,
        <https://linked.data.gov.au/def/earth-science-data-category/glaciology> ;
    skos:historyNote "From the Fields of Research vocabulary from the Australian and New Zealand Standard Research Classification (ANZSRC, 2020). Definition adapted from Glossary of geology (5th edition revised; Neuendorf et al., 2011) and Wikipedia." ;
    skos:inScheme cs: ;
    skos:notation "370902"^^<https://linked.data.gov.au/def/anzsrc-for/2020> ;
    skos:prefLabel "glaciology"@en ;
    schema:citation
        "https://glossary.americangeosciences.org/term/glaciology"^^xsd:anyURI ,
        "https://www.britannica.com/science/glaciology"^^xsd:anyURI ;
.

:grade-control
    a skos:Concept ;
    rdfs:isDefinedBy cs: ;
    skos:broader :mining-geology ;
    skos:definition "Grade control is the process aiming to maximize the value of ore mined and fed into the mill. This is commonly achieved by systematic, closely-spaced drilling to check the quality and grade of the ore while mining is underway. Drillhole data, other sampling data and geological mapping can all be used to delineate ore for mining purposes, thus ‘controlling the grade’ of feedstock to the mill."@en ;
    skos:historyNote "Definition compiled by the Geological Survey of Western Australia." ;
    skos:inScheme cs: ;
    skos:prefLabel "grade control"@en ;
.

:gravity-gradiometry
    a skos:Concept ;
    rdfs:isDefinedBy cs: ;
    skos:broader :gravimetrics ;
    skos:definition "The study of variations (anomalies) in the Earth's gravity field via measurements of the spatial gradient of gravitational acceleration."@en ;
    skos:exactMatch <https://linked.data.gov.au/def/earth-science-data-category/gravity-gradiometry> ;
    skos:historyNote "Definition adapted from Wikipedia." ;
    skos:inScheme cs: ;
    skos:prefLabel "gravity gradiometry"@en ;
    schema:citation "https://en.wikipedia.org/wiki/Gravity_gradiometry"^^xsd:anyURI ;
.

:ground-spectral-imaging
    a skos:Concept ;
    rdfs:isDefinedBy cs: ;
    skos:broader :spectral-imaging ;
    skos:definition "Spectral imaging obtained in the field or at a mine site, especially using portable devices (e.g. pXRF); applications include characterization of outcrops and materials, mine wall face mapping, and ore grade classification."@en ;
    skos:historyNote "Compiled by the Geological Survey of Western Australia." ;
    skos:inScheme cs: ;
    skos:prefLabel "ground spectral imaging"@en ;
.

:heritage-and-conservation
    a skos:Concept ;
    rdfs:isDefinedBy
        cs: ,
        <https://linked.data.gov.au/def/anzsrc-for/2020> ;
    skos:broader :heritage-archive-and-museum-studies ;
    skos:definition "Heritage conservation seeks to sustain the values of heritage (including both natural and cultural heritage) landscapes, places and objects, individually and collectively, so that the community and visitors can continue to appreciate, experience and learn from them and about them, and so that they can be passed on to future generations. More specifically, this field refers to the more practical or applied aspects of site or object restoration, preventative activities, and/or remedial treatments."@en ;
    skos:exactMatch <https://linked.data.gov.au/def/anzsrc-for/2020/430205> ;
    skos:historyNote "Adapted from the Fields of Research vocabulary from the Australian and New Zealand Standard Research Classification (ANZSRC, 2020). Definition adapted from New South Wales Heritage Office's 'Interpreting Heritage places and items: guidelines'." ;
    skos:inScheme cs: ;
    skos:notation "430205"^^<https://linked.data.gov.au/def/anzsrc-for/2020> ;
    skos:prefLabel "heritage and conservation"@en ;
    schema:citation
        "https://onlinelibrary.wiley.com/doi/full/10.1002/gch2.202100084"^^xsd:anyURI ,
        "https://www.environment.nsw.gov.au/-/media/OEH/Corporate-Site/Documents/Heritage/interpreting-heritage-places-and-items-guidelines.pdf"^^xsd:anyURI ,
        "https://www.heritage21.com.au/owners-of-heritage-buildings/what-is-heritage-conservation/"^^xsd:anyURI ;
.

:heritage-collections-and-interpretations
    a skos:Concept ;
    rdfs:isDefinedBy
        cs: ,
        <https://linked.data.gov.au/def/anzsrc-for/2020> ;
    skos:broader :heritage-archive-and-museum-studies ;
    skos:definition "The study of collections, their heritage values and the ways of presenting their significance (interpretation) as a 'means of communicating ideas and feelings which help people enrich their understanding and appreciation of their world and their role within it' (Australian Heritage Commission)."@en ;
    skos:exactMatch <https://linked.data.gov.au/def/anzsrc-for/2020/430206> ;
    skos:historyNote "Adapted from the Fields of Research vocabulary from the Australian and New Zealand Standard Research Classification (ANZSRC, 2020). Definition adapted from NSW Heritage Office's 'Interpreting Heritage places and items: guidelines'." ;
    skos:inScheme cs: ;
    skos:notation "430206"^^<https://linked.data.gov.au/def/anzsrc-for/2020> ;
    skos:prefLabel "heritage collections and interpretations"@en ;
    schema:citation
        "https://en.wikipedia.org/wiki/Australian_Heritage_Commission"^^xsd:anyURI ,
        "https://www.environment.nsw.gov.au/-/media/OEH/Corporate-Site/Documents/Heritage/interpreting-heritage-places-and-items-guidelines.pdf"^^xsd:anyURI ;
.

:heritage-archive-and-museum-studies-not-elsewhere-classified
    a skos:Concept ;
    rdfs:isDefinedBy
        cs: ,
        <https://linked.data.gov.au/def/anzsrc-for/2020> ;
    skos:broader :heritage-archive-and-museum-studies ;
    skos:definition "The study of collections, their heritage values and the ways of presenting their significance (interpretation) as a 'means of communicating ideas and feelings which help people enrich their understanding and appreciation of their world and their role within it' (Australian Heritage Commission)."@en ;
    skos:exactMatch <https://linked.data.gov.au/def/anzsrc-for/2020/430299> ;
    skos:historyNote "Adapted from the Fields of Research vocabulary from the Australian and New Zealand Standard Research Classification (ANZSRC, 2020). Definition adapted from NSW Heritage Office's 'Interpreting Heritage places and items: guidelines'." ;
    skos:inScheme cs: ;
    skos:notation "430299"^^<https://linked.data.gov.au/def/anzsrc-for/2020> ;
    skos:prefLabel "heritage collections and interpretations"@en ;
    schema:citation
        "https://en.wikipedia.org/wiki/Australian_Heritage_Commission"^^xsd:anyURI ,
        "https://www.environment.nsw.gov.au/-/media/OEH/Corporate-Site/Documents/Heritage/interpreting-heritage-places-and-items-guidelines.pdf"^^xsd:anyURI ;
.

:heritage-tourism-visitor-and-audience-studies
    a skos:Concept ;
    rdfs:isDefinedBy
        cs: ,
        <https://linked.data.gov.au/def/anzsrc-for/2020> ;
    skos:broader :heritage-archive-and-museum-studies ;
    skos:definition "Heritage tourism is a form of non-business travel whereby tourists engage with the heritage, tangible and intangible, moveable and immovable, abstract or concrete, natural or cultural, of a region through activities, experiences, and purchases which facilitate a connection to the people, objects, and places of the past (including geological sites) associated with the locations being visited. Studies associated with this field refer to the management of such sites, the evaluation of the impact of visitors and the assessment of tourist satisfaction and emotional experiences during the visit."@en ;
    skos:exactMatch <https://linked.data.gov.au/def/anzsrc-for/2020/430207> ;
    skos:historyNote "Adapted from the Fields of Research vocabulary from the Australian and New Zealand Standard Research Classification (ANZSRC, 2020). Definition compiled by Geological Survey of Western Australia from multiple sources." ;
    skos:inScheme cs: ;
    skos:notation "430207"^^<https://linked.data.gov.au/def/anzsrc-for/2020> ;
    skos:prefLabel "heritage tourism, visitor and audience studies"@en ;
    schema:citation
        "https://en.wikipedia.org/wiki/Heritage_tourism"^^xsd:anyURI ,
        "https://sciendo.com/article/10.2478/cjot-2019-0007"^^xsd:anyURI ,
        "https://www.sciencedirect.com/science/article/abs/pii/S2211973617301320"^^xsd:anyURI ;
.

:historical-geology
    a skos:Concept ;
    rdfs:isDefinedBy cs: ;
    skos:altLabel
        "palaeogeology"@en ,
        "paleogeology"@en ;
    skos:broader :geology ;
    skos:definition "The branch of geology concerned with the reconstruction and comprehension of the geological history of the Earth, i.e. the evolution of the Earth and its life forms from its origins to the present day. This discipline examines the vastness of geological time, measured in billions of years, and investigates changes in the Earth (gradual and sudden) over this deep time. It focuses on geological processes, such as plate tectonics, that have changed the Earth's surface and subsurface over time and the use of methods including stratigraphy, structural geology, paleontology, and sedimentology to tell the sequence of these events. It also focuses on the evolution of life during different time periods in the geologic time scale. Not to be confused with history of geology."@en ;
    skos:exactMatch <https://linked.data.gov.au/def/earth-science-data-category/historical-geology> ;
    skos:historyNote "Definition adapted from Glossary of geology (5th edition revised; Neuendorf et al., 2011) and Wikipedia." ;
    skos:inScheme cs: ;
    skos:prefLabel "historical geology"@en ;
    schema:citation
        "https://en.wikipedia.org/wiki/Historical_geology"^^xsd:anyURI ,
        "https://glossary.americangeosciences.org/term/historicalgeology"^^xsd:anyURI ;
.

:history-of-geology
    a skos:Concept ;
    rdfs:isDefinedBy cs: ;
    skos:broader :geology ;
    skos:definition "That branch of the history of science that documents the development of geological knowledge, including the history of observations of geological features, the history of theories to explain their origin, and the history of the organization and development of geological institutions and societies. The biographical study of geologists is included. Not to be confused with historical geology."@en ;
    skos:exactMatch <https://linked.data.gov.au/def/earth-science-data-category/history-of-geology> ;
    skos:historyNote "Definition adapted from Glossary of geology (5th edition revised; Neuendorf et al., 2011)." ;
    skos:inScheme cs: ;
    skos:prefLabel "history of geology"@en ;
    schema:citation "https://glossary.americangeosciences.org/term/historyofgeology"^^xsd:anyURI ;
.

:hydrogeochemistry
    a skos:Concept ;
    rdfs:isDefinedBy cs: ;
    skos:altLabel "water chemistry"@en ;
    skos:broader :geochemistry ;
    skos:definition "The chemistry of ground and surface waters, particularly the relationships between the chemical characteristics and quality of waters and the areal and regional geology. On a broader scale, the science that uses the tools and principles of chemistry to explain the mechanisms behind major geological systems such as the Earth's crust and its oceans."@en ;
    skos:exactMatch <https://linked.data.gov.au/def/earth-science-data-category/hydrogeochemistry> ;
    skos:historyNote "Compiled by the Geological Survey of Western Australia. Definition adapted from Glossary of geology (5th edition, revised; Neuendorf et al., 2011) and Geological Survey of Queensland Earth science data category vocabulary." ;
    skos:inScheme cs: ;
    skos:prefLabel "hydrogeochemistry"@en ;
    schema:citation
        "https://glossary.americangeosciences.org/term/hydrogeochemistry"^^xsd:anyURI ,
        "https://linked.data.gov.au/def/earth-science-data-category/hydrogeochemistry"^^xsd:anyURI ;
.

:hydrogeology
    a skos:Concept ;
    rdfs:isDefinedBy cs: ;
    skos:altLabel
        "geohydrology"@en ,
        "groundwater geology"@en ;
    skos:broader :physical-geography-and-environmental-geoscience ;
    skos:definition "The area of geology that deals with the distribution and movement of subsurface water (i.e. groundwater) in the soil and rocks of the Earth's crust, and with related geological aspects of surface waters."@en ;
    skos:exactMatch <https://linked.data.gov.au/def/earth-science-data-category/hydrogeology> ;
    skos:historyNote "Definition adapted from Glossary of geology (5th edition revised; Neuendorf et al., 2011) and Wikipedia." ;
    skos:inScheme cs: ;
    skos:prefLabel "hydrogeology"@en ;
    schema:citation "https://glossary.americangeosciences.org/term/hydrogeology"^^xsd:anyURI ;
.

:ichnology
    a skos:Concept ;
    rdfs:isDefinedBy cs: ;
    skos:broader :paleontology ;
    skos:definition "The study of the fossilized tracks, trails, burrows and excavations made by animals and more broadly the study of bioturbation, which is the reworking of sediment by animals. Ichnofossils or trace fossils are used to interpret paleoecological aspects of sedimentary environments."@en ;
    skos:exactMatch <https://linked.data.gov.au/def/earth-science-data-category/ichnology> ;
    skos:historyNote """Definition adapted from:
Gingras, MK 2021, Ichnology, in Encyclopedia of Geology (Second Edition), edited by D Alderton and SA Elias: Academic Press, p. 669–680, doi.10.1016/B978-0-08-102908-4.00197-1.""" ;
    skos:inScheme cs: ;
    skos:prefLabel "ichnology"@en ;
    schema:citation
        "https://glossary.americangeosciences.org/term/ichnology"^^xsd:anyURI ,
        "https://www.dictionary.com/browse/ichnology"^^xsd:anyURI ,
        "https://www.sciencedirect.com/science/article/pii/B9780081029084001971"^^xsd:anyURI ,
        "https://www.sciencedirect.com/topics/earth-and-planetary-sciences/ichnology"^^xsd:anyURI ;
.

:igneous-petrology
    a skos:Concept ;
    rdfs:isDefinedBy cs: ;
    skos:broadMatch
        <https://linked.data.gov.au/def/anzsrc-for/2020/370503> ,
        <https://linked.data.gov.au/def/earth-science-data-category/igneous-and-metamorphic-petrology> ;
    skos:broader :petrology ;
    skos:definition "The branch of petrology that describes the composition, characteristics, textures, occurrence and origin of igneous rocks, i.e. those that are formed from magma. It relies heavily on the use of chemistry, chemical methods, and phase diagrams."@en ;
    skos:historyNote "Definition adapted from Wikipedia." ;
    skos:inScheme cs: ;
    skos:prefLabel "igneous petrology"@en ;
    schema:citation "https://en.wikipedia.org/wiki/Igneous_petrology"^^xsd:anyURI ;
.

:information-management
    a skos:Concept ;
    rdfs:isDefinedBy cs: ;
    skos:broader :information-and-computing-sciences ;
    skos:definition "Information management (IM) is the appropriate and optimized capture, storage, retrieval, and use of information. It may be personal information management or organizational. Information management for organizations concerns a cycle of organizational activity: the acquisition of information from one or more sources, the custodianship and the distribution of that information to those who need it, and its ultimate disposal through archiving or deletion and extraction."@en ;
    skos:historyNote "Compiled by the Geological Survey of Western Australia. Definition adapted from Wikipedia." ;
    skos:inScheme cs: ;
    skos:notation "IM"^^xsd:token ;
    skos:prefLabel "information management"@en ;
    schema:citation "https://en.wikipedia.org/wiki/Information_management"^^xsd:anyURI ;
.

:information-systems
    a skos:Concept ;
    rdfs:isDefinedBy
        cs: ,
        <https://linked.data.gov.au/def/anzsrc-for/2020> ;
    skos:broader :information-and-computing-sciences ;
    skos:definition "An information system (IS) is a formal, integrated set of components for the collection, storage and processing of data, aimed at providing information, contributing to knowledge and delivering digital products that facilitate decision-making."@en ;
    skos:exactMatch <https://linked.data.gov.au/def/anzsrc-for/2020/4609> ;
    skos:historyNote "From the Fields of Research vocabulary from the Australian and New Zealand Standard Research Classification (ANZSRC, 2020). Definition adapted from Wikipedia." ;
    skos:inScheme cs: ;
    skos:notation
        "IS"^^xsd:token ,
        "4609"^^<https://linked.data.gov.au/def/anzsrc-for/2020> ;
    skos:prefLabel "information systems"@en ;
    schema:citation
        "https://en.wikipedia.org/wiki/Information_system"^^xsd:anyURI ,
        "https://www.britannica.com/topic/information-system"^^xsd:anyURI ;
.

:inorganic-geochemistry
    a skos:Concept ;
    rdfs:isDefinedBy
        cs: ,
        <https://linked.data.gov.au/def/anzsrc-for/2020> ;
    skos:broader :geochemistry ;
    skos:definition "The broader field for the study of the chemistry of inorganic rocks, minerals, and other Earth materials that are not currently or once living."@en ;
    skos:exactMatch
        <https://linked.data.gov.au/def/anzsrc-for/2020/370302> ,
        <https://linked.data.gov.au/def/earth-science-data-category/inorganic-geochemistry> ;
    skos:historyNote "From the Fields of Research vocabulary from the Australian and New Zealand Standard Research Classification (ANZSRC, 2020). Definition adapted from Geological Survey of Queensland Earth science data category vocabulary." ;
    skos:inScheme cs: ;
    skos:notation "370302"^^<https://linked.data.gov.au/def/anzsrc-for/2020> ;
    skos:prefLabel "inorganic geochemistry"@en ;
    schema:citation "https://linked.data.gov.au/def/earth-science-data-category/inorganic-geochemistry"^^xsd:anyURI ;
.

:intangible-heritage
    a skos:Concept ;
    rdfs:isDefinedBy
        cs: ,
        <https://linked.data.gov.au/def/anzsrc-for/2020> ;
    skos:broader :heritage-archive-and-museum-studies ;
    skos:definition "The part of cultural heritage that deals with items that have no physical existence, such as past and current traditions or living expressions inherited from our ancestors and passed on to our descendants (e.g. oral traditions, performing arts, social practices, rituals, festive events), knowledge and practices concerning nature and the universe, or the knowledge and skills to produce traditional crafts."@en ;
    skos:exactMatch <https://linked.data.gov.au/def/anzsrc-for/2020/430208> ;
    skos:historyNote "Adapted from the Fields of Research vocabulary from the Australian and New Zealand Standard Research Classification (ANZSRC, 2020). Definition adapted from UNESCO." ;
    skos:inScheme cs: ;
    skos:notation "430208"^^<https://linked.data.gov.au/def/anzsrc-for/2020> ;
    skos:prefLabel "intangible heritage"@en ;
    schema:citation "https://ich.unesco.org/en/what-is-intangible-heritage-00003"^^xsd:anyURI ;
.

:invertebrate-paleontology
    a skos:Concept ;
    rdfs:isDefinedBy cs: ;
    skos:altLabel
        "invertebrate palaeontology"@en ,
        "invertebrate palaeozoology"@en ,
        "invertebrate paleozoology"@en ;
    skos:broader :paleontology ;
    skos:definition "The branch of paleontology that studies the morphologic, taxonomic, systematic, stratigraphic, and biogeographic characteristics of organisms of the 'invertebrate' phyla, i.e. of those animals that lack notochords (non-vertebrates)."@en ;
    skos:exactMatch <https://linked.data.gov.au/def/earth-science-data-category/invertebrate-paleontology> ;
    skos:historyNote "Definition adapted from https://journals.ku.edu/InvertebratePaleo and https://www.floridamuseum.ufl.edu/invertpaleo/." ;
    skos:inScheme cs: ;
    skos:prefLabel "invertebrate paleontology"@en ;
    schema:citation
        "https://en.wikipedia.org/wiki/Invertebrate_paleontology"^^xsd:anyURI ,
        "https://glossary.americangeosciences.org/term/invertebratepaleontology"^^xsd:anyURI ,
        "https://journals.ku.edu/InvertebratePaleo"^^xsd:anyURI ,
        "https://www.floridamuseum.ufl.edu/invertpaleo/"^^xsd:anyURI ;
.

:laboratory-spectral-imaging
    a skos:Concept ;
    rdfs:isDefinedBy cs: ;
    skos:broader :spectral-imaging ;
    skos:definition "Spectral imaging and mapping obtained under controlled laboratory conditions, e.g. for the qualitative and quantitative mineral identification and phase relationships."@en ;
    skos:historyNote "Compiled by the Geological Survey of Western Australia." ;
    skos:inScheme cs: ;
    skos:prefLabel "laboratory spectral imaging"@en ;
.

:lithogeochemistry
    a skos:Concept ;
    rdfs:isDefinedBy cs: ;
    skos:altLabel
        "whole rock chemistry"@en ,
        "whole-rock chemistry"@en ;
    skos:broader :geochemistry ;
    skos:definition "The study of the complete chemical composition of whole rocks, considering the main and trace elements, but also isotopes."@en ;
    skos:historyNote """Compiled by the Geological Survey of Western Australia. Definition adapted from:
Alexandre, P 2021, Lithogeochemistry, in Practical Geochemistry, Springer Textbooks in Earth Sciences, Geography and Environment, Springer, Cham, doi:10.1007/978-3-030-72453-5_3.""" ;
    skos:inScheme cs: ;
    skos:prefLabel "lithogeochemistry"@en ;
    schema:citation
        "https://glossary.americangeosciences.org/term/lithogeochemistry"^^xsd:anyURI ,
        "https://link.springer.com/chapter/10.1007/978-3-030-72453-5_3"^^xsd:anyURI ;
.

:lithostratigraphy
    a skos:Concept ;
    rdfs:isDefinedBy cs: ;
    skos:altLabel "lithological stratigraphy"@en ;
    skos:broader :stratigraphy ;
    skos:definition "The element of stratigraphy that deals with the description and systematic organization of the rocks of the Earth's crust into distinctive named units based on the lithological character of the rocks and their stratigraphic relations. In the petroleum industry, lithostratigraphy specifically refers to the study and correlation of strata to elucidate Earth's history on the basis of their lithology or the nature of the well log response, mineral content, grain size, texture, and colour of rocks."@en ;
    skos:historyNote "Definition adapted from Glossary of geology (5th edition revised; Neuendorf, 2011) and Schlumberger Oilfield Glossary." ;
    skos:inScheme cs: ;
    skos:prefLabel "lithostratigraphy"@en ;
    schema:citation
        "https://glossary.americangeosciences.org/term/lithostratigraphy"^^xsd:anyURI ,
        "https://glossary.slb.com/en/terms/l/lithostratigraphy"^^xsd:anyURI ;
.

:local-geology
    a skos:Concept ;
    rdfs:isDefinedBy cs: ;
    skos:broader :geology ;
    skos:definition "A comprehensive study of the geological and geographical features of a subdivision of or area within a region (in this context defined as an area of land that has common natural features)."@en ;
    skos:exactMatch <https://linked.data.gov.au/def/earth-science-data-category/local-geology> ;
    skos:historyNote "Compiled by the Geological Survey of Western Australia" ;
    skos:inScheme cs: ;
    skos:prefLabel "local geology"@en ;
    schema:citation "https://www.ncesc.com/geographic-faq/can-a-region-be-bigger-than-a-country/"^^xsd:anyURI ;
.

:machine-learning
    a skos:Concept ;
    rdfs:isDefinedBy cs: ;
    skos:broader :artificial-intelligence ;
    skos:definition "Machine learning (ML) is the field of study in artificial intelligence concerned with the development and study of statistical algorithms that can learn from data and generalize to unseen data, and thus perform tasks without explicit instructions."@en ;
    skos:historyNote "Definition adapted from Wikipedia and MITSloan website." ;
    skos:inScheme cs: ;
    skos:notation "ML"^^xsd:token ;
    skos:prefLabel "machine learning"@en ;
    schema:citation
        "https://en.wikipedia.org/wiki/Machine_learning"^^xsd:anyURI ,
        "https://mitsloan.mit.edu/ideas-made-to-matter/machine-learning-explained"^^xsd:anyURI ;
.

:magnetics
    a skos:Concept ;
    rdfs:isDefinedBy cs: ;
    skos:broadMatch <https://linked.data.gov.au/def/anzsrc-for/2020/370607> ;
    skos:broader :magnetism-and-paleomagnetism ;
    skos:definition "The study of the Earth's magnetic field via non-invasive geophysical methods which measure perturbations in the Earth’s magnetic field caused by magnetic minerals in crustal rocks, specifically to image anomalies caused by source bodies within the subsurface."@en ;
    skos:exactMatch <https://linked.data.gov.au/def/earth-science-data-category/magnetics> ;
    skos:historyNote "Definition adapted from Glossary of geology (5th edition revised; Neuendorf et al., 2011)." ;
    skos:inScheme cs: ;
    skos:prefLabel "magnetics"@en ;
    schema:citation "https://www.ga.gov.au/scientific-topics/disciplines/geophysics/magnetics"^^xsd:anyURI ;
.

:magnetostratigraphy
    a skos:Concept ;
    rdfs:isDefinedBy cs: ;
    skos:broader :stratigraphy ;
    skos:definition "The element of stratigraphy that deals with the magnetic characteristics of rock units. Specifically the geophysical correlation technique used to date sedimentary rocks lacking fossils and volcanic sequences by collecting oriented samples at measured intervals throughout a section and measuring the characteristic remanent magnetization."@en ;
    skos:historyNote "Definition adapted from Glossary of geology (5th edition revised; Neuendorf, 2011) and Wikipedia." ;
    skos:inScheme cs: ;
    skos:prefLabel "magnetostratigraphy"@en ;
    schema:citation
        "https://en.wikipedia.org/wiki/Magnetostratigraphy"^^xsd:anyURI ,
        "https://glossary.americangeosciences.org/term/magnetostratigraphy"^^xsd:anyURI ;
.

:magnetotellurics
    a skos:Concept ;
    rdfs:isDefinedBy cs: ;
    skos:broader :electrical-and-electromagnetic-methods-in-geophysics ;
    skos:definition "Magnetotellurics (MT) is a passive geophysical method used to infer the Earth's subsurface electrical resistivity/conductivity from measurements of natural variations of geomagnetic and geoelectric field at the Earth's surface, i.e. the use of natural electromagnetic signals to image subsurface electrical conductivity structure through electromagnetic induction."@en ;
    skos:exactMatch <https://linked.data.gov.au/def/earth-science-data-category/magnetotellurics> ;
    skos:historyNote """Definition adapted from:
1) Wikipedia
2) Unsworth, M 2007, Magnetotellurics, in Encyclopedia of Geomagnetism and Paleomagnetism, edited by D Gubbins and E Herrero-Bervera: Springer, Dordrecht, doi.10.1007/978-1-4020-4423-6_207.""" ;
    skos:inScheme cs: ;
    skos:notation "MT"^^xsd:token ;
    skos:prefLabel "magnetotellurics"@en ;
    schema:citation
        "https://en.wikipedia.org/wiki/Magnetotellurics"^^xsd:anyURI ,
        "https://link.springer.com/referenceworkentry/10.1007/978-1-4020-4423-6_207"^^xsd:anyURI ;
.

:maritime-archeology
    a skos:Concept ;
    rdfs:isDefinedBy
        cs: ,
        <https://linked.data.gov.au/def/anzsrc-for/2020> ;
    skos:altLabel
        "marine archaeology"@en ,
        "marine archeology"@en ,
        "maritime archaeology"@en ;
    skos:broader :archeology ;
    skos:definition "Maritime archeology (also known as marine archeology) is a discipline of archeology that specifically studies human interaction with the sea, lakes and rivers through the study of associated physical remains, be they vessels, shore-side facilities, port-related structures, cargoes, human remains and submerged landscapes."@en ;
    skos:historyNote "From the Fields of Research vocabulary from the Australian and New Zealand Standard Research Classification (ANZSRC, 2020). Definition adapted from Wikipedia." ;
    skos:inScheme cs: ;
    skos:prefLabel "maritime archeology"@en ;
    schema:citation "https://en.wikipedia.org/wiki/Maritime_archaeology"^^xsd:anyURI ;
    skos:exactMatch <https://linked.data.gov.au/def/anzsrc-for/2020/430108> ;
    skos:notation "430108"^^<https://linked.data.gov.au/def/anzsrc-for/2020> ;
.

:materials-conservation
    a skos:Concept ;
    rdfs:isDefinedBy
        cs: ,
        <https://linked.data.gov.au/def/anzsrc-for/2020> ;
    skos:broader :heritage-archive-and-museum-studies ;
    skos:definition "The technical aspects related to the protection and care of materials to avoid their physical deterioration while actively ensuring their preservation for posterity."@en ;
    skos:exactMatch <https://linked.data.gov.au/def/anzsrc-for/2020/430209> ;
    skos:historyNote "From the Fields of Research vocabulary from the Australian and New Zealand Standard Research Classification (ANZSRC, 2020)." ;
    skos:inScheme cs: ;
    skos:notation "430209"^^<https://linked.data.gov.au/def/anzsrc-for/2020> ;
    skos:prefLabel "materials conservation"@en ;
    schema:citation "https://en.wikipedia.org/wiki/Conservation_and_restoration_of_cultural_property"^^xsd:anyURI ;
.

:medical-geology
    a skos:Concept ;
    rdfs:isDefinedBy cs: ;
    skos:altLabel
        "hydrobiogeochemoepidemiopathoecology"@en ,
        "regional pathology"@en ;
    skos:broader :geology ;
    skos:definition "An interdisciplinary scientific field studying the influence of natural geological factors on human and animal health. Broadly, medical geology studies exposure to or deficiency of trace elements and minerals (the distribution of trace elements as related to nutrition, or the geographic patterns of disease); inhalation of ambient and anthropogenic mineral dusts and volcanic emissions; transportation, modification and concentration of organic compounds; the occurrence of toxic elements in unusual quantities in parts of the Earth's crust; and exposure to radionuclides, microbes and pathogens."@en ;
    skos:historyNote "Definition adapted from Wikipedia and Glossary of geology (5th edition revised; Neuendorf, 2011)." ;
    skos:inScheme cs: ;
    skos:prefLabel "medical geology"@en ;
    schema:citation
        "https://en.wikipedia.org/wiki/Medical_geology"^^xsd:anyURI ,
        "https://glossary.americangeosciences.org/term/medicalgeology"^^xsd:anyURI ;
.

:metamorphic-petrology
    a skos:Concept ;
    rdfs:isDefinedBy cs: ;
    skos:altLabel "metamorphic history"@en ;
    skos:broadMatch
        <https://linked.data.gov.au/def/anzsrc-for/2020/370503> ,
        <https://linked.data.gov.au/def/earth-science-data-category/igneous-and-metamorphic-petrology> ;
    skos:broader :petrology ;
    skos:definition "The branch of petrology that describes the composition, characteristics, textures, occurrence and origin of metamorphic rocks, i.e. those derived from the transformation of existing rocks into new types. It relies heavily on the use of chemistry, chemical methods, and phase diagrams."@en ;
    skos:historyNote "Definition adapted from Wikipedia." ;
    skos:inScheme cs: ;
    skos:prefLabel "metamorphic petrology"@en ;
    schema:citation "https://en.wikipedia.org/wiki/Petrology"^^xsd:anyURI ;
.

:microbial-paleobiology
    a skos:Concept ;
    rdfs:isDefinedBy cs: ;
    skos:broader :paleontology ;
    skos:definition "The systematic study of fossil microbialites and other evidence of/for microbes and microbially influenced features in the geological record, focussing on their morphology, classification, and environmental and biostratigraphic significance. Microbial paleobiology commonly intersects with disciplines such as geobiology, astrobiology and biostratigraphy, and is commonly employed in studies concerned with the origins of life on Earth."@en ;
    skos:historyNote "Compiled by Geological Survey of Western Australia." ;
    skos:inScheme cs: ;
    skos:prefLabel "microbial paleobiology"@en ;
    schema:citation "https://en.wikipedia.org/wiki/Microbialite"^^xsd:anyURI ;
.

:military-geology
    a skos:Concept ;
    rdfs:isDefinedBy cs: ;
    skos:broader :geology ;
    skos:definition "The application of geological theory to warfare and the peacetime practices of the military. Military geologists are used for terrain analysis (geomorphology, soil science), engineering (building of roads and airfields), and the identification of resources (e.g. water supply or construction materials), and to research the effects of military practices on Earth's and planets' geology. The peacetime application of military geology includes the building of infrastructure, typically during local emergencies or foreign peacekeeping deployments."@en ;
    skos:historyNote "Definition adapted from Wikipedia and Glossary of geology (5th edition revised; Neuendorf, 2011)." ;
    skos:inScheme cs: ;
    skos:prefLabel "military geology"@en ;
    schema:citation
        "https://en.wikipedia.org/wiki/Military_geology"^^xsd:anyURI ,
        "https://glossary.americangeosciences.org/term/militarygeology"^^xsd:anyURI ;
.

:mineral-chemistry
    a skos:Concept ;
    rdfs:isDefinedBy cs: ;
    skos:broader :geochemistry ;
    skos:definition "The study of the chemical composition of minerals, i.e. of naturally occurring inorganic element or compound with a defined chemical composition and crystal structure, i.e. having a periodically repeating arrangement of atoms and characteristic chemical composition, resulting in distinctive physical properties. It includes the analysis of the major, minor, trace and isotope elemental composition of a mineral, as well as the bonding of these elements in the mineral’s crystal structure."@en ;
    skos:historyNote "Compiled by the Geological Survey of Western Australia. Definition adapted from Glossary of geology (5th edition, revised; Neuendorf et al., 2011)." ;
    skos:inScheme cs: ;
    skos:prefLabel "mineral chemistry"@en ;
    schema:citation "https://glossary.americangeosciences.org/term/mineral"^^xsd:anyURI ;
.

:mineral-exploration-geology
    a skos:Concept ;
    rdfs:isDefinedBy cs: ;
    skos:broader :mineral-resource-geology ;
    skos:definition "Studies related to the search for deposits of useful minerals. It may include geological reconnaissance, geological mapping, remote sensing analysis, geophysical and geochemical methods, and both surface and subsurface (e.g. drilling and underground) investigations. Also studies to establish the nature of a known mineral deposit, in preparatory to development and exploitation; in this sense exploration goes beyond discovery, and is a broader term than prospecting."@en ;
    skos:historyNote "Definition adapted from Glossary of geology (5th edition revised; Neuendorf et al., 2011)." ;
    skos:inScheme cs: ;
    skos:prefLabel "mineral exploration geology"@en ;
    schema:citation "https://glossary.americangeosciences.org/term/exploration"^^xsd:anyURI ;
.

:mineral-system-analysis
    a skos:Concept ;
    rdfs:isDefinedBy cs: ;
    skos:broader :mineral-resource-geology ;
    skos:definition "Understanding the combination of geologic processes that are required to form and preserve ore deposits at all scales. It recognises seven critical geological processes: source of mineralizing fluid, source of metals, fluid pathway, thermal gradient, energy source, structural focusing of fluids, and chemical or physical trap for metal precipitation."@en ;
    skos:historyNote """Definition adapted from:
1) McCuaig, TC, Beresford, S and Hronsky, J 2010, Translating the mineral systems approach into an effective exploration targeting system: Ore Geology Reviews, v. 38, p. 128–138.
2) Wyborn, LAI, Heinrich, CA and Jaques, AL 1994, Australian Proterozoic mineral systems: Essential ingredients and mappable criteria: Proceedings of the Australasian Institute of Mining and Metallurgy Annual Conference, Darwin, 5–9 August 1994, p. 109–115.""" ;
    skos:inScheme cs: ;
    skos:prefLabel "mineral system analysis"@en ;
.

:molecular-paleontology
    a skos:Concept ;
    rdfs:isDefinedBy cs: ;
    skos:broader :paleontology ;
    skos:definition "The application of molecular analytical techniques to fossil or subfossil material in order to test for the presence of original biomolecules. These molecules may be proteins, DNA, carbohydrates or lipids, or their diagenetic products."@en ;
    skos:historyNote """Definition adapted from:
Schweitzer, MH 2004, Molecular paleontology: some current advances and problems: Annales de Paléontologie, v. 90(2), p. 81–102, doi:10.1016/j.annpal.2004.02.001.""" ;
    skos:inScheme cs: ;
    skos:prefLabel "molecular paleontology"@en ;
    schema:citation
        "https://en.wikipedia.org/wiki/Molecular_paleontology"^^xsd:anyURI ,
        "https://glossary.americangeosciences.org/term/molecularpaleontology"^^xsd:anyURI ,
        "https://www.sciencedirect.com/science/article/abs/pii/S0753396904000138"^^xsd:anyURI ;
.

:natural-hazards
    a skos:Concept ;
    rdfs:isDefinedBy
        cs: ,
        <https://linked.data.gov.au/def/anzsrc-for/2020> ;
    skos:broader :physical-geography-and-environmental-geoscience ;
    skos:definition "The study of natural phenomena that might have a negative effect on humans or the environment, specifically hazards encompassing geological and meteorological phenomena such as earthquakes, volcanic eruptions, wildfires, cyclonic storms, floods, droughts, avalanches and landslides, as well as phenomena such as natural radioactivity."@en ;
    skos:exactMatch
        <https://linked.data.gov.au/def/anzsrc-for/2020/370903> ,
        <https://linked.data.gov.au/def/earth-science-data-category/natural-hazards> ;
    skos:historyNote "From the Fields of Research vocabulary from the Australian and New Zealand Standard Research Classification (ANZSRC, 2020). Definition adapted from Glossary of geology (5th edition revised; Neuendorf et al., 2011) and Wikipedia." ;
    skos:inScheme cs: ;
    skos:notation "370903"^^<https://linked.data.gov.au/def/anzsrc-for/2020> ;
    skos:prefLabel "natural hazards"@en ;
    schema:citation "https://en.wikipedia.org/wiki/Natural_disaster"^^xsd:anyURI ;
.

:neotectonics
    a skos:Concept ;
    rdfs:isDefinedBy cs: ;
    skos:broader :tectonics ;
    skos:definition "The study of the post-Miocene structures and structural history of the Earth's crust."@en ;
    skos:historyNote "Definition adapted from Glossary of geology (5th edition revised; Neuendorf et al., 2011)." ;
    skos:inScheme cs: ;
    skos:prefLabel "neotectonics"@en ;
    schema:citation "https://glossary.americangeosciences.org/term/neotectonics"^^xsd:anyURI ;
.

:non-radiogenic-isotope-geochemistry
    a skos:Concept ;
    rdfs:isDefinedBy cs: ;
    skos:altLabel "stable isotope geochemistry"@en ;
    skos:broader :isotope-geochemistry ;
    skos:definition "The branch of isotope geochemistry focusing on non-radiogenic (or stable) isotope systems, i.e. those where a nuclide is not known to undergo radioactive decay."@en ;
    skos:historyNote "Compiled by the Geological Survey of Western Australia. Definition adapted from Glossary of geology (5th edition, revised; Neuendorf et al., 2011)." ;
    skos:inScheme cs: ;
    skos:prefLabel "non-radiogenic isotope geochemistry"@en ;
    schema:citation "https://glossary.americangeosciences.org/term/stableisotope"^^xsd:anyURI ;
.

:non-radiogenic-system-age-determination
    a skos:Concept ;
    rdfs:isDefinedBy cs: ;
    skos:altLabel "stable isotope age determination"@en ;
    skos:broader :isotope-age-determination ;
    skos:definition "The branch of geochronology / isotope geochemistry focusing on non-radiogenic (or stable) isotope systems, i.e. those where a nuclide is not known to undergo radioactive decay, to determine the numerical age of suitable geological materials."@en ;
    skos:historyNote "Definition adapted from Glossary of geology (5th edition revised; Neuendorf et al., 2011)." ;
    skos:inScheme cs: ;
    skos:prefLabel "non-radiogenic system age determination"@en ;
    schema:citation "https://glossary.americangeosciences.org/term/stableisotope"^^xsd:anyURI ;
.

:oceanography
    a skos:Concept ;
    rdfs:isDefinedBy cs: ;
    skos:broader :marine-geoscience ;
    skos:definition "The study of the ocean, including its physical, chemical, biologic, and geological aspects."@en ;
    skos:historyNote "Definition adapted from Wikipedia." ;
    skos:inScheme cs: ;
    skos:prefLabel "oceanography"@en ;
    schema:citation "https://glossary.americangeosciences.org/term/oceanography"^^xsd:anyURI ;
.

:ore-geology
    a skos:Concept ;
    rdfs:isDefinedBy cs: ;
    skos:broader :mineral-resource-geology ;
    skos:definition "The study of economically valuable minerals (ores) in the Earth's crust, including their formation, distribution, and extraction methods."@en ;
    skos:historyNote "Definition adapted from Glossary of geology (5th edition revised; Neuendorf et al., 2011)." ;
    skos:inScheme cs: ;
    skos:prefLabel "ore geology"@en ;
    schema:citation "https://glossary.americangeosciences.org/term/ore"^^xsd:anyURI ;
.

:ore-microscopy
    a skos:Concept ;
    rdfs:isDefinedBy cs: ;
    skos:altLabel "ore petrography"@en ;
    skos:broader :petrography ;
    skos:definition "The microscopic study of metallic ores using reflected light."@en ;
    skos:historyNote """Definition adapted from:
Castroviejo, R 2023, A practical guide to ore microscopy—Volume 1: mineral identification, Springer International Publishing: Cham, Switzerland, 980p., doi.10.1007/978-3-031-12654-3.""" ;
    skos:inScheme cs: ;
    skos:prefLabel "ore microscopy"@en ;
    schema:citation "https://link.springer.com/book/10.1007/978-3-031-12654-3"^^xsd:anyURI ;
.

:ore-petrology
    a skos:Concept ;
    rdfs:isDefinedBy cs: ;
    skos:altLabel "economic petrology"@en ;
    skos:broader :petrology ;
    skos:definition "The branch of petrology that describes the composition, characteristics, textures, occurrence and origin of ore minerals, i.e. of naturally occurring minerals that contain valuable elements or minerals in sufficient quantities to be economically mined and processed for their desired metal or mineral content."@en ;
    skos:historyNote "Definition adapted from https://geologyscience.com/ore-genesis/ore-minerals/." ;
    skos:inScheme cs: ;
    skos:prefLabel "ore petrology"@en ;
    schema:citation "https://geologyscience.com/ore-genesis/ore-minerals/"^^xsd:anyURI ;
.

:organic-petrology
    a skos:Concept ;
    rdfs:isDefinedBy cs: ;
    skos:broader :petrology ;
    skos:definition "Organic petrology involves the study of organic matter (OM) in rocks, including its origin and thermal maturity due to burial within the Earth's crust."@en ;
    skos:exactMatch <https://linked.data.gov.au/def/earth-science-data-category/organic-petrology> ;
    skos:historyNote "Definition from Geological Survey of Queensland Earth science data category vocabulary." ;
    skos:inScheme cs: ;
    skos:notation ""^^xsd:token ;
    skos:prefLabel "organic petrology"@en ;
    schema:citation
        "https://research.csiro.au/oilandgas/wp-content/uploads/sites/49/2015/10/Organic-Petrology-2015.pdf"^^xsd:anyURI ,
        "https://linked.data.gov.au/def/earth-science-data-category/organic-petrology"^^xsd:anyURI ;
.

:paleobiogeography
    a skos:Concept ;
    rdfs:isDefinedBy cs: ;
    skos:altLabel "palaeobiogeography"@en ;
    skos:broader :paleontology ;
    skos:definition "That branch of paleontology that treats the geographic distribution of organisms in past geological time, especially with regard to the ecologic, climatologic, and evolutionary factors involved. It includes the more specialized paleophytogeography and paleozoogeography subdisciplines."@en ;
    skos:historyNote "Definition adapted from Glossary of geology (5th edition revised; Neuendorf et al., 2011)." ;
    skos:inScheme cs: ;
    skos:prefLabel "paleobiogeography"@en ;
    schema:citation "https://glossary.americangeosciences.org/term/paleobiogeography"^^xsd:anyURI ;
.

:paleobotany
    a skos:Concept ;
    rdfs:isDefinedBy cs: ;
    skos:altLabel "palaeobotany"@en ;
    skos:broader :paleontology ;
    skos:definition "The branch of paleontology that studies the morphologic, taxonomic, systematic, stratigraphic, and biogeographic characteristics of plants, fungi and algae from geological contexts, and their use for the biological reconstruction of past environments (paleogeography), as well as the evolutionary history of plants and allied kingdoms, with a bearing upon the evolution of life in general. These fossils can be impressions or compressions of the plants left on the rock's surface, or 'petrified' objects, such as wood, which preserve the original plant material in rocklike form."@en ;
    skos:exactMatch <https://linked.data.gov.au/def/earth-science-data-category/paleobotany> ;
    skos:historyNote "Compiled by Geological Survey of Western Australia from multiple sources." ;
    skos:inScheme cs: ;
    skos:prefLabel "paleobotany"@en ;
    schema:citation
        "https://en.wikipedia.org/wiki/Paleobotany"^^xsd:anyURI ,
        "https://glossary.americangeosciences.org/term/paleobotany"^^xsd:anyURI ,
        "https://www.cmnh.org/paleobotany-paleoecology"^^xsd:anyURI ;
.

:paleoecology
    a skos:Concept ;
    rdfs:isDefinedBy cs: ;
    skos:altLabel "palaeoecology"@en ;
    skos:broader :paleontology ;
    skos:definition "A subdiscipline of paleontology concerned with reconstructing past biota, populations, communities, landscapes, environments, and ecosystems from available geological and biological (fossil) evidence. It encompasses the study of interactions between organisms and/or interactions between organisms and their environments across geological timescales, including reconstructions of past ecosystems and environments using this information."@en ;
    skos:historyNote """Definition adapted from:
1) Birks, HJB 2008, Palaeoecology, in Encyclopedia of Ecology, Academic Press, p. 2623–2634, doi:10.1016/B978-008045405-4.00525-5)
2) Wikipedia.""" ;
    skos:inScheme cs: ;
    skos:prefLabel "paleoecology"@en ;
    schema:citation
        "https://glossary.americangeosciences.org/term/paleoecology"^^xsd:anyURI ,
        "https://www.sciencedirect.com/science/article/abs/pii/B9780080454054005255"^^xsd:anyURI ;
.

:paleoenvironmental-reconstruction
    a skos:Concept ;
    rdfs:isDefinedBy cs: ;
    skos:altLabel "palaeoenvironmental reconstruction"@en ;
    skos:broader :paleoclimatology ;
    skos:definition "The reconstruction of past environments and their climates within regions or across regions, based on the sediments, soils, strata, and associated biological remains."@en ;
    skos:historyNote """Definition adapted from:
Holliday, VT and Mandel, RD 2024, Paleoenvironmental Reconstruction, in Encyclopedia of Geoarchaeology, edited by AS Gilbert, P Goldberg, RD Mandel and V Aldeias, Encyclopedia of Earth Sciences Series: Springer, Cham. doi.org/10.1007/978-1-4020-4409-0_191.""" ;
    skos:inScheme cs: ;
    skos:prefLabel "paleoenvironmental reconstruction"@en ;
    schema:citation "https://link.springer.com/referenceworkentry/10.1007/978-3-030-44600-0_191-1"^^xsd:anyURI ;
.

:paleomagnetic-age-determination
    a skos:Concept ;
    rdfs:isDefinedBy cs: ;
    skos:broader :geochronology ;
    skos:definition "The dating of geological materials by comparing the magnetic signature in rocks to known changes in the Earth's magnetic field (based on movements of the magnetic north pole over geological time). It is based on matching the changes in the paleomagnetic field recorded in lava flows or sediments with their corresponding dates in the magnetic polarity time scale. When applied to archeology, it is referred to as archeomagnetics."@en ;
    skos:historyNote "Definition adapted from Wikipedia and Glossary of geology (5th edition revised; Neuendorf et al., 2011)." ;
    skos:inScheme cs: ;
    skos:prefLabel "paleomagnetic age determination"@en ;
    schema:citation
        "https://en.wikipedia.org/wiki/Geochronology"^^xsd:anyURI ,
        "https://glossary.americangeosciences.org/term/paleomagneticstratigraphy"^^xsd:anyURI ;
.

:paleomagnetism
    a skos:Concept ;
    rdfs:isDefinedBy cs: ;
    skos:altLabel "palaeomagnetism"@en ;
    skos:broadMatch <https://linked.data.gov.au/def/anzsrc-for/2020/370607> ;
    skos:broader :magnetism-and-paleomagnetism ;
    skos:definition "The study of natural remanent magnetization of Earth materials (rocks, sediments and archeological materials) in order to determine the direction, and indirectly intensity, of the Earth's magnetic field in the geological past."@en ;
    skos:historyNote "Definition adapted from Glossary of geology (5th edition revised; Neuendorf et al., 2011)." ;
    skos:inScheme cs: ;
    skos:prefLabel "paleomagnetism"@en ;
    schema:citation
        "https://en.wikipedia.org/wiki/Paleomagnetism"^^xsd:anyURI ,
        "https://glossary.americangeosciences.org/term/paleomagnetism"^^xsd:anyURI ;
.

:palynology
    a skos:Concept ;
    rdfs:isDefinedBy cs: ;
    skos:broader :micropaleontology ;
    skos:definition "Originally, the study of pollen and spores, extant and fossil (paleopalynology), including stratigraphic and paleoecological applications. Now includes the study of a wide range of other robust-walled, acid-insoluble microscopic remains of various plants, animals, fungal spores and protists, including kerogen and unidentifiable organic matter."@en ;
    skos:exactMatch <https://linked.data.gov.au/def/earth-science-data-category/palynology> ;
    skos:historyNote """Definition adapted from:
Traverse, A 2008, Paleopalynology: Springer, Dordrecht, The Netherlands, 813p.""" ;
    skos:inScheme cs: ;
    skos:prefLabel "palynology"@en ;
    schema:citation "https://en.wikipedia.org/wiki/Palynology"^^xsd:anyURI ;
.

:passive-seismic
    a skos:Concept ;
    rdfs:isDefinedBy cs: ;
    skos:broader :seismic-surveys ;
    skos:definition "The detection of natural low frequency earth movements, commonly with the purpose of discerning geological structures and locating underground oil, gas, or other resources."@en ;
    skos:exactMatch <https://linked.data.gov.au/def/earth-science-data-category/passive-seismic> ;
    skos:historyNote "Definition adapted from Wikipedia and Glossary of geology (5th edition revised; Neuendorf et al., 2011)." ;
    skos:inScheme cs: ;
    skos:prefLabel "passive seismic"@en ;
    schema:citation
        "https://en.wikipedia.org/wiki/Passive_seismic"^^xsd:anyURI ,
        "https://glossary.americangeosciences.org/term/passivemethod"^^xsd:anyURI ;
.

:pedology-and-pedometrics
    a skos:Concept ;
    rdfs:isDefinedBy
        cs: ,
        <https://linked.data.gov.au/def/anzsrc-for/2020> ;
    skos:broader :soil-sciences ;
    skos:definition "One of the disciplines of soil science, pedology is the study of soil morphology, genesis, and classification. Pedometrics specifically refers to the use of quantitative methods for the study of soil distribution and genesis."@en ;
    skos:exactMatch <https://linked.data.gov.au/def/anzsrc-for/2020/410602> ;
    skos:historyNote "From the Fields of Research vocabulary from the Australian and New Zealand Standard Research Classification (ANZSRC, 2020). Definition adapted from Glossary of geology (5th edition revised; Neuendorf et al., 2011)." ;
    skos:inScheme cs: ;
    skos:notation "410602"^^<https://linked.data.gov.au/def/anzsrc-for/2020> ;
    skos:prefLabel "pedology and pedometrics"@en ;
    schema:citation
        "https://glossary.americangeosciences.org/term/pedology"^^xsd:anyURI ,
        "https://www.sciencedirect.com/topics/earth-and-planetary-sciences/pedometrics"^^xsd:anyURI ;
.

:petroleum-and-reservoir-engineering
    a skos:Concept ;
    rdfs:isDefinedBy
        cs: ,
        <https://linked.data.gov.au/def/anzsrc-for/2020> ;
    skos:broader :resources-engineering ;
    skos:definition "The fields of engineering concerned with activities related to the production of hydrocarbons to determine the way in which a reservoir is developed and depleted, i.e. the study and application of scientific and engineering principles to the fluid flow through a porous medium during the development and production of oil and gas reservoirs so as to obtain a high economic recovery."@en ;
    skos:exactMatch
        <https://linked.data.gov.au/def/anzsrc-for/2020/401907> ,
        <https://linked.data.gov.au/def/earth-science-data-category/reservoir-engineering> ;
    skos:historyNote "From the Fields of Research vocabulary from the Australian and New Zealand Standard Research Classification (ANZSRC, 2020). Definition adapted from Wikipedia." ;
    skos:inScheme cs: ;
    skos:notation "401907"^^<https://linked.data.gov.au/def/anzsrc-for/2020> ;
    skos:prefLabel "petroleum and reservoir engineering"@en ;
    schema:citation
        "https://en.wikipedia.org/wiki/Petroleum_engineering"^^xsd:anyURI ,
        "https://en.wikipedia.org/wiki/Reservoir_engineering"^^xsd:anyURI ;
.

:petroleum-geochemistry
    a skos:Concept ;
    rdfs:isDefinedBy cs: ;
    skos:altLabel "gas and oil analysis"@en ;
    skos:broader :organic-geochemistry ;
    skos:definition "The characterization of the physical properties and elemental analysis of oil and gas, used to interpret the type of source rock and correlate to a source rock, determine the thermal maturity of the oil and gas (and hence the maturity of the source rock), potential dating of the source rock, and compare oil and gas composition between different fields or within a field."@en ;
    skos:historyNote "Compiled by the Geological Survey of Western Australia." ;
    skos:inScheme cs: ;
    skos:prefLabel "petroleum geochemistry"@en ;
.

:phylogenetics
    a skos:Concept ;
    rdfs:isDefinedBy cs: ;
    skos:altLabel "phylogenetic systematics"@en ;
    skos:broader :evolutionary-paleontology ;
    skos:definition "An approach to systematics (the study of the kinds and diversity of organisms and the relationships between them) that attempts to recover the phylogenetic (genealogical) relationships among groups of organisms, and produces classifications that reflect exactly those genealogical relationships."@en ;
    skos:historyNote "Definition adapted from Glossary of geology (5th edition revised; Neuendorf et al., 2011)." ;
    skos:inScheme cs: ;
    skos:prefLabel "phylogenetics"@en ;
    schema:citation "https://glossary.americangeosciences.org/term/phylogeneticsystematics"^^xsd:anyURI ;
.

:physical-geography-and-environmental-geoscience-not-elsewhere-classified
    a skos:Concept ;
    rdfs:isDefinedBy
        cs: ,
        <https://linked.data.gov.au/def/anzsrc-for/2020> ;
    skos:broader :physical-geography-and-environmental-geoscience ;
    skos:definition "Physical geographical and environmental science data and information not otherwise described by other sub-categories of physical geography."@en ;
    skos:exactMatch
        <https://linked.data.gov.au/def/anzsrc-for/2020/370999> ,
        <https://linked.data.gov.au/def/earth-science-data-category/physical-geography-and-environmental-geoscience-not-elsewhere-classified> ;
    skos:historyNote "From the Fields of Research vocabulary from the Australian and New Zealand Standard Research Classification (ANZSRC, 2020). Definition adapted from Glossary of geology (5th edition revised; Neuendorf et al., 2011) and Wikipedia." ;
    skos:inScheme cs: ;
    skos:notation "370999"^^<https://linked.data.gov.au/def/anzsrc-for/2020> ;
    skos:prefLabel "physical geography and environmental geoscience not elsewhere classified"@en ;
.

:policy-and-administration
    a skos:Concept ;
    rdfs:isDefinedBy
        cs: ,
        <https://linked.data.gov.au/def/anzsrc-for/2020> ;
    skos:broader :human-society ;
    skos:definition "Public administration is the planning, preparation, and execution of policy meant to build and strengthen civil society. Policy, in this context, refers to prudence or wisdom in the management of affairs, or management procedures based primarily on material interest."@en ;
    skos:exactMatch <https://linked.data.gov.au/def/anzsrc-for/2020/4407> ;
    skos:historyNote "From the Fields of Research vocabulary from the Australian and New Zealand Standard Research Classification (ANZSRC, 2020). Definition adapted from the Merriam-Webster dictionary." ;
    skos:inScheme cs: ;
    skos:notation "4407"^^<https://linked.data.gov.au/def/anzsrc-for/2020> ;
    skos:prefLabel "policy and administration"@en ;
    schema:citation "https://www.merriam-webster.com/dictionary/policy"^^xsd:anyURI ;
.

:prospecting
    a skos:Concept ;
    rdfs:isDefinedBy cs: ;
    skos:broader :mineral-resource-geology ;
    skos:definition "The field search for valuable commodities, mineral specimens (e.g. gold nuggets, crystals), lapidary material, and mineral deposits — usually with the ultimate objective of economic development by mining operations. Prospectors may be divided into two general categories: those with academic, scientific training and those with only field training or in the purely amateur category."@en ;
    skos:historyNote """Definition adapted from:
Fairbridge, RW 1988, Prospecting, in General Geology, Encyclopedia of Earth Science: Springer, Boston, MA, doi.10.1007/0-387-30844-X_93.""" ;
    skos:inScheme cs: ;
    skos:prefLabel "prospecting"@en ;
    schema:citation
        "https://en.wikipedia.org/wiki/Prospecting"^^xsd:anyURI ,
        "https://glossary.americangeosciences.org/term/prospecting"^^xsd:anyURI ,
        "https://link.springer.com/referenceworkentry/10.1007/0-387-30844-X_93"^^xsd:anyURI ;
.

:prospectivity-analysis
    a skos:Concept ;
    rdfs:isDefinedBy cs: ;
    skos:altLabel "prospectivity studies"@en ;
    skos:broader :mineral-resource-geology ;
    skos:definition "A predictive tool typically used for mineral exploration targeting at the broad regional- to camp-scale. It is less effective and less frequently used at the project- to deposit-scale where predictive tools compete with direct detection techniques. It includes the delineation of prospective areas based on personal experience and interpretation of available geological, geochemical and geophysical data, as well as statistical data analysis/modelling, and in combination GIS-based spatial datasets and/or soft computational models (e.g. fuzzy logic)."@en ;
    skos:historyNote """Definition adapted from:
Porwal, AK and Kreuzer, OP 2010, Introduction to the Special Issue: Mineral prospectivity analysis and quantitative resource estimation: Ore Geology Reviews, v. 38(3), p. 121-127, doi:10.1016/j.oregeorev.2010.06.002.""" ;
    skos:inScheme cs: ;
    skos:prefLabel "prospectivity analysis"@en ;
    schema:citation "https://www.sciencedirect.com/science/article/pii/S0169136810000636#bib50"^^xsd:anyURI ;
.

:quantitative-mineralogy
    a skos:Concept ;
    rdfs:isDefinedBy cs: ;
    skos:broader :mineralogy ;
    skos:definition "A discipline focused on the quantitative measurements of the mineralogy, chemistry, morphology and microstructures of minerals and mineral assemblages using a range of analytical techniques (e.g. modal analysis, X-ray diffractometry, infrared and Raman spectroscopy, refractometry, spectral mapping, etc.). Specifically, quantitative mineral methodologies are utilized to measure and/or constrain mineral abundances, as well as to provide mineral grade and texture information for geological and mineral processing applications."@en ;
    skos:historyNote """Definition from:
Keulen, N, Malkki, SN and Graham, S 2020, Automated Quantitative Mineralogy Applied to Metamorphic Rocks, in Applications of SEM Automated Mineralogy: From Ore Deposits over Processing to Secondary Resource Characterization), edited by B Schulz: Minerals, v.10(1), 47, doi:10.3390/min10010047.""" ;
    skos:inScheme cs: ;
    skos:prefLabel "quantitative mineralogy"@en ;
    schema:citation
        "https://www.ceecthefuture.org/resources/libs-mineralogy-quantitative-mineralogy-on-the-belt"^^xsd:anyURI ,
        "https://www.mdpi.com/2075-163X/10/1/47"^^xsd:anyURI ;
.

:quarry-and-extractive-resource-geology
    a skos:Concept ;
    rdfs:isDefinedBy cs: ;
    skos:altLabel
        "basic raw materials geology"@en ,
        "industrial minerals geology"@en ;
    skos:broader :resource-geoscience ;
    skos:definition "The study of industrial mineral resources, i.e. geological materials that are mined/quarried for their commercial value and are not fuel (fuel minerals or mineral fuels) or sources of metals (metallic minerals) but are used in their natural state or after beneficiation either as raw materials or as additives in a wide range of applications based on their physical and/or chemical properties. These studies include the quantification of the physical properties, chemical properties, volumes, and limitations to development of quarry products. Quarry resources (also referred to as basic raw materials or industrial minerals) include, but may not be limited to, sand (including silica sand), clay, hard rock (including dimension stone), limestone (including metallurgical limestone), agricultural lime, gravel, gypsum, other construction and road building materials and materials which may substitute these raw materials."@en ;
    skos:exactMatch <https://linked.data.gov.au/def/earth-science-data-category/quarry-resource-geology> ;
    skos:historyNote "Compiled by Geological Survey of western Australia." ;
    skos:inScheme cs: ;
    skos:prefLabel "quarry and extractive resource geology"@en ;
    schema:citation
        "https://en.wikipedia.org/wiki/Industrial_mineral"^^xsd:anyURI ,
        "https://www.dmp.wa.gov.au/Geological-Survey/Basic-Raw-Materials-1411.aspx"^^xsd:anyURI ;
.

:quaternary-environments
    a skos:Concept ;
    rdfs:isDefinedBy
        cs: ,
        <https://linked.data.gov.au/def/anzsrc-for/2020> ;
    skos:broader :physical-geography-and-environmental-geoscience ;
    skos:definition "The branch of geology that study environmental changes from 2.58 million years ago to the present. In particular, Quaternary geology study the process and deposits that developed during the Quaternary, a period characterized by glacial–interglacial cycles."@en ;
    skos:exactMatch
        <https://linked.data.gov.au/def/anzsrc-for/2020/370905> ,
        <https://linked.data.gov.au/def/earth-science-data-category/quaternary-environments> ;
    skos:historyNote "From the Fields of Research vocabulary from the Australian and New Zealand Standard Research Classification (ANZSRC, 2020). Definition adapted from Glossary of geology (5th edition revised; Neuendorf et al., 2011) and Wikipedia." ;
    skos:inScheme cs: ;
    skos:notation "370905"^^<https://linked.data.gov.au/def/anzsrc-for/2020> ;
    skos:prefLabel "quaternary environments"@en ;
    schema:citation "https://en.wikipedia.org/wiki/Quaternary_science"^^xsd:anyURI ;
.

:radiogenic-age-determination
    a skos:Concept ;
    rdfs:isDefinedBy cs: ;
    skos:broader :geochronology ;
    skos:definition "The dating of geological materials by using the effects of radioactivity other than the natural decay from a parent to a daughter isotope. It includes methods such as fission tracks (measure of the density of track marking left in a material by the spontaneous fission of uranium-238 impurities), luminescence (measure of the effect of background radiation on certain minerals), and electron spin resonance (ESR), measure of the amount of unpaired electrons in crystalline structures that were previously exposed to natural radiation). The term radiogenic here is used as in Colman et al. (1987)."@en ;
    skos:historyNote """Compiled by the Geological Survey of Western Australia. Definition based on:
Colman, SM, Pierce, KL and Birkeland, PW 1987, Suggested terminology for Quaternary dating methods: Quaternary Research, v. 28(2), p. 314–319, doi:10.1016/0033-5894(87)90070-6.""" ;
    skos:inScheme cs: ;
    skos:prefLabel "radiogenic age determination"@en ;
    schema:citation "https://www.sciencedirect.com/science/article/pii/0033589487900706"^^xsd:anyURI ;
.

:radiogenic-isotope-geochemistry
    a skos:Concept ;
    rdfs:isDefinedBy cs: ;
    skos:broader :isotope-geochemistry ;
    skos:definition "The branch of isotope geochemistry focusing on radiogenic isotope systems, i.e. those where a daughter isotope is produced from the decay of a radioactive parent isotope."@en ;
    skos:historyNote """Compiled by the Geological Survey of Western Australia. Definition adapted from:
Banner, YL 2004, Radiogenic isotopes: systematics and applications to earth surface processes and chemical stratigraphy: Earth-Science Reviews, v. 65(3–4), p. 141–194, ISSN 0012-8252, doi:10.1016/S0012-8252(03)00086-2.""" ;
    skos:inScheme cs: ;
    skos:prefLabel "radiogenic isotope geochemistry"@en ;
    schema:citation "https://www.sciencedirect.com/science/article/abs/pii/S0012825203000862"^^xsd:anyURI ;
.

:radiogenic-isotopic-system-age-determination
    a skos:Concept ;
    rdfs:isDefinedBy cs: ;
    skos:altLabel
        "radioactive dating"@en ,
        "radiogenic dating"@en ,
        "radiometric age determination"@en ,
        "radiometric dating"@en ;
    skos:broader :isotope-age-determination ;
    skos:definition "The branch of geochronology / isotope geochemistry focusing on radiogenic isotope systems, i.e. those where a daughter isotope is produced from the decay of a radioactive parent isotope, to determine the numerical age of suitable geological materials."@en ;
    skos:historyNote """Definition adapted from:
Banner, YL 2004, Radiogenic isotopes: systematics and applications to earth surface processes and chemical stratigraphy: Earth Science Reviews, v. 65(3–4), p. 141–194, doi:10.1016/S0012-8252(03)00086-2.""" ;
    skos:inScheme cs: ;
    skos:prefLabel "radiogenic (isotopic) system age determination"@en ;
    schema:citation
        "https://en.wikipedia.org/wiki/Radiometric_dating"^^xsd:anyURI ,
        "https://www.sciencedirect.com/science/article/abs/pii/S0012825203000862"^^xsd:anyURI ;
.

:radiometrics
    a skos:Concept ;
    rdfs:isDefinedBy cs: ;
    skos:altLabel "gamma-ray spectrometry"@en ;
    skos:broadMatch
        <https://linked.data.gov.au/def/anzsrc-for/2020/370605> ,
        <https://linked.data.gov.au/def/earth-science-data-category/geothermics-and-radiometrics> ;
    skos:broader :geothermics-and-radiometrics ;
    skos:definition "The radiometric, or gamma-ray spectrometric method is a geophysical process used to estimate concentrations of the radioelements potassium, uranium and thorium in the near surface."@en ;
    skos:historyNote "Definition adapted from Geoscience Australia website." ;
    skos:inScheme cs: ;
    skos:prefLabel "radiometrics"@en ;
    schema:citation "https://www.ga.gov.au/scientific-topics/disciplines/geophysics/radiometrics"^^xsd:anyURI ;
.

:regional-geology
    a skos:Concept ;
    rdfs:isDefinedBy cs: ;
    skos:broader :geology ;
    skos:definition "The geological study of large-scale regions, providing a link between global and local geology, and a framework for site-specific studies."@en ;
    skos:exactMatch <https://linked.data.gov.au/def/earth-science-data-category/regional-geology> ;
    skos:historyNote """Definition adapted from: 
Roberts, DG and Bally, AW (Eds), 2012, Regional Geology and Tectonics: Phanerozoic Rift Systems and Sedimentary Basins: Elsevier, 528p., doi.10.1016/B978-0-444-56356-9.00019-5.""" ;
    skos:inScheme cs: ;
    skos:prefLabel "regional geology"@en ;
    schema:citation "https://doi.org/10.1016/C2010-0-67671-1"^^xsd:anyURI ;
.

:regional-mineralogy
    a skos:Concept ;
    rdfs:isDefinedBy cs: ;
    skos:broader :mineralogy ;
    skos:definition "The mineralogical study of specific geographic regions, from ore deposits clusters to large metallogenic provinces. It includes evaluation of location and the spatial distribution of minerals and mineral assemblages in relation to the geological history of the province (region) or the formation of the deposit. Regional mineralogy can include mineral regional fingerprinting, and directly links to metallogeny and genetic mineralogy."@en ;
    skos:historyNote "Compiled by the Geological Survey of Western Australia based on the Lomonosov-Fund website from Moscow State University." ;
    skos:inScheme cs: ;
    skos:prefLabel "regional mineralogy"@en ;
    schema:citation "http://www.lomonosov-fund.ru/enc/ru/encyclopedia"^^xsd:anyURI ;
.

:regolith-and-landscape-evolution
    a skos:Concept ;
    rdfs:isDefinedBy
        cs: ,
        <https://linked.data.gov.au/def/anzsrc-for/2020> ;
    skos:altLabel
        "surface geology"@en ,
        "surficial geology"@en ;
    skos:broader :physical-geography-and-environmental-geoscience ;
    skos:closeMatch <https://linked.data.gov.au/def/earth-science-data-category/surface-geology> ;
    skos:definition "The study of the geology of surficial deposits, i.e. those at or near the Earth's surface. It includes the study of soils and unconsolidated sediments, their geological features and structures, and their relationships to the underlying bedrock."@en ;
    skos:exactMatch <https://linked.data.gov.au/def/anzsrc-for/2020/370906> ;
    skos:historyNote "From the Fields of Research vocabulary from the Australian and New Zealand Standard Research Classification (ANZSRC, 2020). Definition adapted from Glossary of geology (5th edition revised; Neuendorf et al., 2011)." ;
    skos:inScheme cs: ;
    skos:notation "370906"^^<https://linked.data.gov.au/def/anzsrc-for/2020> ;
    skos:prefLabel "regolith and landscape evolution"@en ;
    schema:citation "https://glossary.americangeosciences.org/term/regolithweath"^^xsd:anyURI ;
.

:rehabilitation
    a skos:Concept ;
    rdfs:isDefinedBy cs: ;
    skos:broader :environmental-management ;
    skos:definition "The stage in the life-cycle of a project or mine where the resources have been extracted and the site or part thereof is being rehabilitated back to its original condition or an acceptable environmental standard."@en ;
    skos:exactMatch <http://linked.data.gov.au/def/site-status/rehabilitation> ;
    skos:historyNote "Definition adapted from Geological Survey of Queensland Site status vocabulary." ;
    skos:inScheme cs: ;
    skos:prefLabel "rehabilitation"@en ;
    schema:citation "http://linked.data.gov.au/def/site-status/rehabilitation"^^xsd:anyURI ;
.

:renewable-energy-geoscience
    a skos:Concept ;
    rdfs:isDefinedBy cs: ;
    skos:broader :energy-geoscience ;
    skos:definition "Geoscience studies related to the definition and exploitation of energy derived from natural resources such as sunlight, wind, rain, tides, waves, and geothermal heat, that are replenished either through natural reproduction or other recurring processes in a finite amount of time on a human time scale."@en ;
    skos:historyNote "Definition adapted from Wikipedia." ;
    skos:inScheme cs: ;
    skos:prefLabel "renewable energy geoscience"@en ;
    schema:citation "https://en.wikipedia.org/wiki/Renewable_resource"^^xsd:anyURI ;
.

:reservoir-analysis
    a skos:Concept ;
    rdfs:isDefinedBy cs: ;
    skos:altLabel "reservoir characterization"@en ;
    skos:broader :energy-geoscience ;
    skos:definition "A characterization of a reservoir that incorporates all the characteristics of the reservoir that are pertinent to its ability to store hydrocarbons and also to produce them. Reservoir characterization models are used to simulate the behaviour of the fluids within the reservoir under different sets of circumstances and to find the optimal production techniques that will maximize the production. Typically, a reservoir analysis incorporates interpretation of depositional facies and diagenesis, mineralogical and textural maturity parameters obtained from macro/meso (e.g. cores, sidewall cores, cuttings) and micro (e.g. thin sections, scanning electron microscope work) samples, as well as direct and indirect measurements of porosity, permeability and grain density from well log analysis and core and mechanical sidewall cores. Image logs are used to determine fracture density where applicable. Regional reservoir distribution and thickness is derived from multiple well reservoir data, seismic interpretation and depth mapping."@en ;
    skos:historyNote "Definition adapted from Glossary of geology (5th edition revised; Neuendorf et al., 2011) and AAPG Wiki (https://wiki.aapg.org/)." ;
    skos:inScheme cs: ;
    skos:prefLabel "reservoir analysis"@en ;
    schema:citation
        "https://glossary.slb.com/en/terms/r/reservoir_characterization"^^xsd:anyURI ,
        "https://wiki.aapg.org/Reservoir_system"^^xsd:anyURI ,
        "https://wiki.aapg.org/Reservoir_system_analysis"^^xsd:anyURI ;
.

:rock-mechanics
    a skos:Concept ;
    rdfs:isDefinedBy cs: ;
    skos:altLabel "geomechanics"@en ;
    skos:broadMatch <https://linked.data.gov.au/def/anzsrc-for/2020/370608> ;
    skos:broader :petrophysics-and-rock-mechanics ;
    skos:closeMatch <https://linked.data.gov.au/def/earth-science-data-category/geomechanics-and-resources-geotechnical-engineering> ;
    skos:definition "A theoretical and applied science of the physical behaviour of rocks and rock masses. In relation to geology, it is the branch of mechanics concerned with the response of rock and rock masses to the force fields of their physical environment."@en ;
    skos:historyNote "Compiled by Geological Survey of Western Australia from multiple sources." ;
    skos:inScheme cs: ;
    skos:prefLabel "rock mechanics"@en ;
    schema:citation
        "https://en.wikipedia.org/wiki/Rock_mechanics"^^xsd:anyURI ,
        "https://glossary.americangeosciences.org/term/rockmechanics"^^xsd:anyURI ;
.

:satellite-based-positioning
    a skos:Concept ;
    rdfs:isDefinedBy
        cs: ,
        <https://linked.data.gov.au/def/anzsrc-for/2020> ;
    skos:broader :geomatic-engineering ;
    skos:definition "The use of satellites to determine the location (geographic position) of a receiver on Earth. The technique involves measuring the range between the receiver and the satellite, and the range measurement used to calculate the receiver's position using observation equations and least squares. The technique is used in global and regional satellite navigation systems."@en ;
    skos:exactMatch <https://linked.data.gov.au/def/anzsrc-for/2020/401305> ;
    skos:historyNote "From the Fields of Research vocabulary from the Australian and New Zealand Standard Research Classification (ANZSRC, 2020). Definition compiled from multiple sources." ;
    skos:inScheme cs: ;
    skos:notation "401305"^^<https://linked.data.gov.au/def/anzsrc-for/2020> ;
    skos:prefLabel "satellite-based positioning"@en ;
    schema:citation
        "https://en.wikipedia.org/wiki/Geopositioning"^^xsd:anyURI ,
        "https://en.wikipedia.org/wiki/Global_Positioning_System"^^xsd:anyURI ,
        "https://www.intechopen.com/chapters/45193"^^xsd:anyURI ;
.

:satellite-spectral-imaging
    a skos:Concept ;
    rdfs:isDefinedBy cs: ;
    skos:broader :spectral-imaging ;
    skos:definition "Remotely sensed spectral imaging obtained from a platform in orbit outside the atmosphere of Earth."@en ;
    skos:exactMatch <https://linked.data.gov.au/def/earth-science-data-category/satellite-spectral> ;
    skos:historyNote "Definition adapted from Wikipedia." ;
    skos:inScheme cs: ;
    skos:prefLabel "satellite spectral imaging"@en ;
    schema:citation "https://en.wikipedia.org/wiki/Satellite_imagery"^^xsd:anyURI ;
.

:seal-analysis
    a skos:Concept ;
    rdfs:isDefinedBy cs: ;
    skos:broader :energy-geoscience ;
    skos:definition "A characterization of regional caprocks and intraformational barriers (seals) to understand their capacity to trap fluids (oil, gas, etc.); specifically to determine seal capacity (i.e. the capillary pressure, or column height, at which a trapped fluid commences to leak through a seal rock) and conduct fault seal analysis (a measure of the capacity of a fault to leak or seal hydrocarbons)."@en ;
    skos:historyNote """Definition adapted from:
Daniel, RF and Kaldi, G 2008, Evaluating seal capacity of caprocks and intraformational barriers for the geosequestration of CO₂: Abstracts for the PESA Eastern Australian Basins Symposium III, Sydney, 14–17 September 2008, p. 475.""" ;
    skos:inScheme cs: ;
    skos:prefLabel "seal analysis"@en ;
    schema:citation
        "https://digital.library.adelaide.edu.au/dspace/bitstream/2440/49635/1/Daniel_Kaldi.pdf"^^xsd:anyURI ,
        "https://wiki.aapg.org/Quantitative_fault_seal_analysis"^^xsd:anyURI ;
.

:sedimentary-petrology
    a skos:Concept ;
    rdfs:isDefinedBy cs: ;
    skos:broader :petrology ;
    skos:definition "The study of the composition, characteristics, occurrence, and origin of sediments and sedimentary rocks."@en ;
    skos:exactMatch <https://linked.data.gov.au/def/earth-science-data-category/sedimentary-petrology> ;
    skos:historyNote "Definition adapted from Glossary of geology (5th edition revised; Neuendorf et al., 2011)." ;
    skos:inScheme cs: ;
    skos:notation ""^^xsd:token ;
    skos:prefLabel "sedimentary petrology"@en ;
    schema:citation "https://glossary.americangeosciences.org/term/sedimentarypetrology"^^xsd:anyURI ;
.

:sedimentology
    a skos:Concept ;
    rdfs:isDefinedBy
        cs: ,
        <https://linked.data.gov.au/def/anzsrc-for/2020> ;
    skos:broader :geology ;
    skos:definition "The scientific study of sedimentary rocks and of the processes by which they were formed; the description, classification, origin, and interpretation of sediments."@en ;
    skos:exactMatch
        <https://linked.data.gov.au/def/anzsrc-for/2020/370509> ,
        <https://linked.data.gov.au/def/earth-science-data-category/sedimentology> ;
    skos:historyNote "From the Fields of Research vocabulary from the Australian and New Zealand Standard Research Classification (ANZSRC, 2020). Definition adapted from Glossary of geology (5th edition revised; Neuendorf, 2011)." ;
    skos:inScheme cs: ;
    skos:notation "370509"^^<https://linked.data.gov.au/def/anzsrc-for/2020> ;
    skos:prefLabel "sedimentology"@en ;
    schema:citation "https://glossary.americangeosciences.org/term/sedimentology"^^xsd:anyURI ;
.

:seismic-stratigraphy
    a skos:Concept ;
    rdfs:isDefinedBy cs: ;
    skos:broader :stratigraphy ;
    skos:definition "The study of stratigraphy and depositional facies as interpreted from seismic data; an integrated stratigraphic and sedimentologic technique to interpret seismic reflection data for stratigraphic correlation and to predict depositional environments and lithology."@en ;
    skos:historyNote "Definition adapted from Wikipedia and Glossary of geology (5th edition revised; Neuendorf et al., 2011)." ;
    skos:inScheme cs: ;
    skos:prefLabel "seismic stratigraphy"@en ;
    schema:citation
        "https://en.wikipedia.org/wiki/Seismic_stratigraphy"^^xsd:anyURI ,
        "https://glossary.americangeosciences.org/term/seismicstratigraphy"^^xsd:anyURI ;
.

:seismic-tomography
    a skos:Concept ;
    rdfs:isDefinedBy cs: ;
    skos:broader :tomography ;
    skos:definition "Seismic tomography is a technique for imaging the subsurface of the Earth with seismic waves produced by controlled ‘active’ sources such as vibrations or explosions, or natural ‘passive’ sources such as earthquakes, wind, waves or human activity. P-, S-, and surface waves can be used for tomographic models of different resolutions based on seismic wavelength, wave source distance, and the seismograph array coverage. The data received at seismometers are used to solve an inverse problem, wherein the locations of reflection and refraction of the wave paths are determined. This solution can be used to create 3D images of velocity anomalies which may be interpreted as structural, thermal, or compositional variations."@en ;
    skos:historyNote "Definition adapted from Wikipedia." ;
    skos:inScheme cs: ;
    skos:prefLabel "seismic tomography"@en ;
    schema:citation "https://en.wikipedia.org/wiki/Seismic_tomography"^^xsd:anyURI ;
.

:sequence-stratigraphy
    a skos:Concept ;
    rdfs:isDefinedBy cs: ;
    skos:broadMatch <https://linked.data.gov.au/def/anzsrc-for/2020/370510> ;
    skos:broader :stratigraphy ;
    skos:definition "The study of rock relationships within a chronostratigraphic framework of repetitive, genetically related strata bounded by surfaces of erosion or nondeposition, or their correlative conformities (Van Wagoner et al., 1990). Specifically, a field of study in which basin-filling sedimentary deposits, called sequences, are interpreted in a framework of eustasy, sedimentation and subsidence through time in order to correlate strata and predict the stratigraphy of relatively unknown areas."@en ;
    skos:historyNote "Definition adapted from Glossary of geology (5th edition revised; Neuendorf et al., 2011) and Schlumberger Oilfield Glossary." ;
    skos:inScheme cs: ;
    skos:prefLabel "sequence stratigraphy"@en ;
    schema:citation
        "https://glossary.americangeosciences.org/term/sequencestratigraphy"^^xsd:anyURI ,
        "https://glossary.slb.com/en/terms/s/sequence_stratigraphy"^^xsd:anyURI ;
.

:soil-chemistry
    a skos:Concept ;
    rdfs:isDefinedBy cs: ;
    skos:broader :regolith-chemistry ;
    skos:definition "The study of the chemical composition of the unconsolidated mineral or organic material on the surface of the earth that serves as a natural medium for the growth of land plants, and whose formation is conditioned by relief and controlled by genetic and environmental factors such as climate (including water and temperature effects) and biological activity (macro- and micro-organisms) acting on parent material over a period of time."@en ;
    skos:historyNote "Compiled by the Geological Survey of Western Australia. Definition adapted from Glossary of geology (5th edition, revised; Neuendorf et al., 2011)." ;
    skos:inScheme cs: ;
    skos:prefLabel "soil chemistry"@en ;
    schema:citation "https://glossary.americangeosciences.org/term/soilsoil"^^xsd:anyURI ;
.

:source-rock-analysis
    a skos:Concept ;
    rdfs:isDefinedBy cs: ;
    skos:broader :organic-geochemistry ;
    skos:definition "The evaluation of the lithological sources of hydrocarbons, i.e. those rocks which contain organic matter and are (or have been) generating and/or expelling hydrocarbons to form accumulations."@en ;
    skos:historyNote "Definition adapted from https://wiki.aapg.org/Source_rock." ;
    skos:inScheme cs: ;
    skos:prefLabel "source-rock analysis"@en ;
    schema:citation
        "https://glossary.slb.com/en/terms/s/source_rock"^^xsd:anyURI ,
        "https://wiki.aapg.org/Source_rock"^^xsd:anyURI ;
.

:speleology
    a skos:Concept ;
    rdfs:isDefinedBy cs: ;
    skos:broader :geology ;
    skos:definition "The exploration and scientific study of caves and other karst features, both physical and biological, including their composition and mineralogy, structure (morphology), physical properties, history, ecology, and the processes by which they form (speleogenesis) and change over time (speleomorphology)."@en ;
    skos:historyNote "Definition adapted from Wikipedia and Glossary of geology (5th edition revised; Neuendorf, 2011)." ;
    skos:inScheme cs: ;
    skos:prefLabel "speleology"@en ;
    schema:citation
        "https://en.wikipedia.org/wiki/Speleology"^^xsd:anyURI ,
        "https://glossary.americangeosciences.org/term/speleology"^^xsd:anyURI ;
.

:structural-geology
    a skos:Concept ;
    rdfs:isDefinedBy cs: ;
    skos:broadMatch <https://linked.data.gov.au/def/anzsrc-for/2020/370511> ;
    skos:broader :structural-geology-and-tectonics ;
    skos:definition "The branch of geology that deals with the form (geometry), spatial arrangement, and internal structure of the rocks, and especially with the description, representation, and analysis of structures (e.g. bedding, folds, faults and fractures), chiefly on a meso- to macroscopic scale. The subject is similar to tectonics, but the latter is generally used for the broader regional or historical phases."@en ;
    skos:exactMatch <https://linked.data.gov.au/def/earth-science-data-category/structural-geology> ;
    skos:historyNote "Definition adapted from Glossary of geology (5th edition revised; Neuendorf, 2011) and Schlumberger Oilfield Glossary." ;
    skos:inScheme cs: ;
    skos:prefLabel "structural geology"@en ;
    schema:citation
        "https://glossary.americangeosciences.org/term/structuralgeology"^^xsd:anyURI ,
        "https://glossary.slb.com/en/terms/s/structural"^^xsd:anyURI ;
.

:surface-processes
    a skos:Concept ;
    rdfs:isDefinedBy cs: ;
    skos:broader :physical-geography-and-environmental-geoscience ;
    skos:definition "The study of the form, physical properties, composition, function, and evolution of Earth’s surface, a dynamic interface where physical, chemical, biological, and human processes cause and are affected by forces in the Earth system, with impact-feedback loops that occur over a wide range of temporal and spatial scales."@en ;
    skos:historyNote """Definition adapted from:
National Research Council, 2010, 1 The Importance of Earth Surface Processes, Landscapes on the Edge: New Horizons for Research on Earth's Surface, Washington, DC: The National Academies Press. doi: 10.17226/12700.""" ;
    skos:inScheme cs: ;
    skos:prefLabel "surface processes"@en ;
    schema:citation "https://nap.nationalacademies.org/read/12700/chapter/3"^^xsd:anyURI ;
.

:surface-water-hydrology
    a skos:Concept ;
    rdfs:isDefinedBy
        cs: ,
        <https://linked.data.gov.au/def/anzsrc-for/2020> ;
    skos:broader :physical-geography-and-environmental-geoscience ;
    skos:definition "The subfield of hydrology concerned with above-earth water, in contrast to groundwater hydrology that deals with water below the surface of the Earth. Its applications include rainfall and runoff, the routes that surface water takes (for example through rivers or reservoirs), and the occurrence of floods and droughts."@en ;
    skos:exactMatch
        <https://linked.data.gov.au/def/anzsrc-for/2020/370704> ,
        <https://linked.data.gov.au/def/earth-science-data-category/surfacewater-hydrology> ;
    skos:historyNote "From the Fields of Research vocabulary from the Australian and New Zealand Standard Research Classification (ANZSRC, 2020). Definition adapted from Glossary of geology (5th edition revised; Neuendorf et al., 2011) and Wikipedia." ;
    skos:inScheme cs: ;
    skos:notation "370704"^^<https://linked.data.gov.au/def/anzsrc-for/2020> ;
    skos:prefLabel "surface water hydrology"@en ;
    schema:citation
        "https://en.wikipedia.org/wiki/Surface-water_hydrology"^^xsd:anyURI ,
        "https://glossary.americangeosciences.org/term/hydrology"^^xsd:anyURI ;
.

:surveying
    a skos:Concept ;
    rdfs:isDefinedBy
        cs: ,
        <https://linked.data.gov.au/def/anzsrc-for/2020> ;
    skos:broadMatch <https://linked.data.gov.au/def/anzsrc-for/2020/401306> ;
    skos:broader :geomatic-engineering ;
    skos:definition "The applied science of determining the two-dimensional or three-dimensional positions of points necessary to determine the area of any part of the Earth's (or other planetary body) surface, the lengths and directions of the boundary lines, and the contour of the surface, and of accurately delineating the whole on paper/digitally."@en ;
    skos:exactMatch <https://linked.data.gov.au/def/earth-science-data-category/surveying> ;
    skos:historyNote "Adapted from the Fields of Research vocabulary from the Australian and New Zealand Standard Research Classification (ANZSRC, 2020). Definition adapted from Glossary of geology (5th edition revised; Neuendorf et al., 2011) and Wikipedia." ;
    skos:inScheme cs: ;
    skos:notation "401306"^^<https://linked.data.gov.au/def/anzsrc-for/2020> ;
    skos:prefLabel "surveying"@en ;
    schema:citation
        "https://en.wikipedia.org/wiki/Surveying"^^xsd:anyURI ,
        "https://glossary.americangeosciences.org/term/surveying"^^xsd:anyURI ;
.

:taphonomy
    a skos:Concept ;
    rdfs:isDefinedBy cs: ;
    skos:altLabel "para-ecology"@en ;
    skos:broader :paleontology ;
    skos:definition "The branch of paleontology concerned with all processes occurring after the death of an organism until its discovery. It includes biostratonomy and fossil diagenesis."@en ;
    skos:historyNote """Definition adapted from:
Behrensmeyer, AK and Kidwell, SM 1985, Taphonomy's contributions to paleobiology: Paleobiology, v. 11(1), p. 105-119, http://www.jstor.org/stable/2400427.""" ;
    skos:inScheme cs: ;
    skos:prefLabel "taphonomy"@en ;
    schema:citation
        "http://www.jstor.org/stable/2400427"^^xsd:anyURI ,
        "https://glossary.americangeosciences.org/term/taphonomy"^^xsd:anyURI ;
.

:taxonomy
    a skos:Concept ;
    rdfs:isDefinedBy cs: ;
    skos:broader :evolutionary-paleontology ;
    skos:definition "The theory and practice of identifying, describing, naming, and classifying organisms. The terms taxonomy and systematics are usually distinguished, the latter having broader connotation, but they may also be used more or less synonymously."@en ;
    skos:historyNote "Definition adapted from Glossary of geology (5th edition revised; Neuendorf et al., 2011)." ;
    skos:inScheme cs: ;
    skos:prefLabel "taxonomy"@en ;
    schema:citation "https://glossary.americangeosciences.org/term/taxonomy"^^xsd:anyURI ;
.

:tephrochronology
    a skos:Concept ;
    rdfs:isDefinedBy cs: ;
    skos:broader :geochronology ;
    skos:definition "The collection, preparation, petrographic description, and approximate dating of tephra. The technique uses discrete layers of tephra (volcanic ash from a single eruption) to create a chronological framework in which paleoenvironmental or archeological records can be placed. The premise of the technique is that each volcanic event produces ash with a unique chemical 'fingerprint' that allows the deposit to be identified across the area affected by fallout. Thus, once the volcanic event has been independently dated, the tephra horizon will act as time marker (as such it is a variant of the basic geological technique of stratigraphy)."@en ;
    skos:historyNote "Definition adapted from Wikipedia and Glossary of geology (5th edition revised; Neuendorf et al., 2011)." ;
    skos:inScheme cs: ;
    skos:prefLabel "tephrochronology"@en ;
    schema:citation
        "https://en.wikipedia.org/wiki/Tephrochronology"^^xsd:anyURI ,
        "https://glossary.americangeosciences.org/term/tephrochronology"^^xsd:anyURI ;
.

:thermochronology
    a skos:Concept ;
    rdfs:isDefinedBy cs: ;
    skos:broader :geochronology ;
    skos:definition "The study of the thermal evolution of a region of a planet. Thermochronologists use radiometric dating (the determination of the age of a sample based on the rate of decay of a radioactive nuclide) along with closure temperatures (i.e. the temperature of the mineral being studied at the time given by the date recorded) to understand the thermal history of a specific rock, mineral, or geological unit."@en ;
    skos:historyNote "Definition adapted from Wikipedia and Glossary of geology (5th edition revised; Neuendorf et al., 2011)." ;
    skos:inScheme cs: ;
    skos:prefLabel "thermochronology"@en ;
    schema:citation
        "https://en.wikipedia.org/wiki/Thermochronology"^^xsd:anyURI ,
        "https://glossary.americangeosciences.org/term/thermochronology"^^xsd:anyURI ;
.

:unconventional-reservoir-geology
    a skos:Concept ;
    rdfs:isDefinedBy cs: ;
    skos:broader :petroleum-geology ;
    skos:definition "The geological study of unconventional petroleum systems, which comprise formations with tight gas, tight oil, oil sands, oil shale, bitumen, gas shales, coal seam gas/coalbed methane, and gas hydrates, and are defined as those where petroleum is distributed throughout the reservoir at basin-wide scale and in which buoyant forces or the influence of a water column on the location of hydrocarbons in the reservoir are not significant."@en ;
    skos:exactMatch <https://linked.data.gov.au/def/earth-science-data-category/unconventional-reservoir-geology> ;
    skos:historyNote "Definition from Geological Survey of Queensland Earth science data category vocabulary." ;
    skos:inScheme cs: ;
    skos:prefLabel "unconventional reservoir geology"@en ;
    schema:citation "https://linked.data.gov.au/def/earth-science-data-category/unconventional-reservoir-geology"^^xsd:anyURI ;
.

:urban-geology
    a skos:Concept ;
    rdfs:isDefinedBy cs: ;
    skos:broader :environmental-geology ;
    skos:definition "The application of geological knowledge and principles to the planning and management of cities and their surroundings. It includes geological studies for physical planning, waste disposal, land use, water-resources management, and extraction of usable raw materials."@en ;
    skos:historyNote "Definition adapted from Glossary of geology (5th edition revised; Neuendorf et al., 2011)." ;
    skos:inScheme cs: ;
    skos:prefLabel "urban geology"@en ;
    schema:citation "https://glossary.americangeosciences.org/term/urbangeology"^^xsd:anyURI ;
.

:varve-chronology
    a skos:Concept ;
    rdfs:isDefinedBy cs: ;
    skos:altLabel "varve analysis"@en ;
    skos:broader :geochronology ;
    skos:definition "A dating method that utilizes the seasonal (summer and winter) sedimentological variations of deposits in lakes that undergo an annual freeze-up, by counting and measuring thicknesses in annual paired layers of sediments. Because each year’s sediment accumulation varies in thickness according to the climatic conditions of the melt season, any long sequence of varve measurements provides a distinctive 'signature' and can be correlated for moderate distances from lake basin to lake basin. Counting and correlation of varves have been used to measure the ages of Pleistocene glacial deposits."@en ;
    skos:historyNote """Definition adapted from:
1) Mörner , N-A (ed.), 2014, Geochronology - Methods and Case Studies: InTech, doi:10.5772/57041
2) Glossary of geology (5th edition revised; Neuendorf et al., 2011).""" ;
    skos:inScheme cs: ;
    skos:prefLabel "varve chronology"@en ;
    schema:citation
        "https://glossary.americangeosciences.org/term/varve"^^xsd:anyURI ,
        "https://www.britannica.com/science/varve-analysis"^^xsd:anyURI ,
        "https://www.intechopen.com/chapters/46984"^^xsd:anyURI ;
.

:vertebrate-paleontology
    a skos:Concept ;
    rdfs:isDefinedBy cs: ;
    skos:altLabel "vertebrate paleozoology"@en ;
    skos:broader :paleontology ;
    skos:definition "The branch of paleontology that studies the morphologic, taxonomic, systematic, stratigraphic, and biogeographic characteristics of Phylum Chordata. This includes modern vertebrates, non-vertebrate chordates (such as lancets and turnicates), and extinct groups of uncertain placement (such as conodonts)."@en ;
    skos:historyNote "Compiled by Geological Survey of Western Australia from multiple sources." ;
    skos:inScheme cs: ;
    skos:prefLabel "vertebrate paleontology"@en ;
    schema:citation
        "https://en.wikipedia.org/wiki/Vertebrate_paleontology"^^xsd:anyURI ,
        "https://glossary.americangeosciences.org/term/vertebratepaleontology"^^xsd:anyURI ;
.

:volcanology
    a skos:Concept ;
    rdfs:isDefinedBy
        cs: ,
        <https://linked.data.gov.au/def/anzsrc-for/2020> ;
    skos:altLabel "vulcanology"@en ;
    skos:broader :geology ;
    skos:definition "The branch of geology that deals with volcanism (e.g. volcanoes, lava, magma), its causes and related geological, geophysical and geochemical phenomena."@en ;
    skos:exactMatch
        <https://linked.data.gov.au/def/anzsrc-for/2020/370512> ,
        <https://linked.data.gov.au/def/earth-science-data-category/volcanology> ;
    skos:historyNote "From the Fields of Research vocabulary from the Australian and New Zealand Standard Research Classification (ANZSRC, 2020). Definition adapted from Glossary of geology (5th edition revised; Neuendorf et al., 2011) and Wikipedia." ;
    skos:inScheme cs: ;
    skos:notation "370512"^^<https://linked.data.gov.au/def/anzsrc-for/2020> ;
    skos:prefLabel "volcanology"@en ;
    schema:citation
        "https://en.wikipedia.org/wiki/Volcanology"^^xsd:anyURI ,
        "https://glossary.americangeosciences.org/term/volcanology"^^xsd:anyURI ;
.

<https://orcid.org/0000-0002-7645-5031>
    a schema:Person ;
    schema:email ""^^xsd:anyURI ;
    schema:name "0000 0002 7645 5031" ;
.

:astronomical-sciences
    a skos:Concept ;
    rdfs:isDefinedBy
        cs: ,
        <https://linked.data.gov.au/def/anzsrc-for/2020> ;
    skos:broader :physical-sciences ;
    skos:definition "The natural sciences that study celestial objects and the phenomena that occur in the cosmos. It uses mathematics, physics, and chemistry to explain their origin and their overall evolution. Objects of interest include planets, moons, stars, nebulae, galaxies, meteoroids, asteroids, and comets or, more generally, everything that originates beyond Earth's atmosphere."@en ;
    skos:exactMatch <https://linked.data.gov.au/def/anzsrc-for/2020/5101> ;
    skos:historyNote "From the Fields of Research vocabulary from the Australian and New Zealand Standard Research Classification (ANZSRC, 2020). Definition adapted from Wikipedia." ;
    skos:inScheme cs: ;
    skos:narrower :astrobiology ;
    skos:notation "5101"^^<https://linked.data.gov.au/def/anzsrc-for/2020> ;
    skos:prefLabel "astronomical sciences"@en ;
    schema:citation "https://en.wikipedia.org/wiki/Astronomy"^^xsd:anyURI ;
.

:atmospheric-sciences
    a skos:Concept ;
    rdfs:isDefinedBy
        cs: ,
        <https://linked.data.gov.au/def/anzsrc-for/2020> ;
    skos:broader :earth-sciences ;
    skos:definition "The study of the Earth's atmosphere and its various inner-working physical processes."@en ;
    skos:exactMatch
        <https://linked.data.gov.au/def/anzsrc-for/2020/3701> ,
        <https://linked.data.gov.au/def/earth-science-data-category/atmospheric-sciences> ;
    skos:historyNote "From the Fields of Research vocabulary from the Australian and New Zealand Standard Research Classification (ANZSRC, 2020); definition from Geological Survey of Queensland Earth science data category vocabulary." ;
    skos:inScheme cs: ;
    skos:narrower :climate-change-science ;
    skos:notation "3701"^^<https://linked.data.gov.au/def/anzsrc-for/2020> ;
    skos:prefLabel "atmospheric sciences"@en ;
    schema:citation "https://linked.data.gov.au/def/earth-science-data-category/atmospheric-sciences"^^xsd:anyURI ;
.

:biological-sciences
    a skos:Concept ;
    rdfs:isDefinedBy
        cs: ,
        <https://linked.data.gov.au/def/anzsrc-for/2020> ;
    skos:definition "The natural science that studies life and living organisms, including their physical structure, chemical processes, molecular interactions, physiological mechanisms, development and evolution."@en ;
    skos:exactMatch
        <https://linked.data.gov.au/def/anzsrc-for/2020/31> ,
        <https://linked.data.gov.au/def/earth-science-data-category/biological-sciences> ;
    skos:historyNote "From the Fields of Research vocabulary from the Australian and New Zealand Standard Research Classification (ANZSRC, 2020). Definition from Geological Survey of Queensland Earth science data category vocabulary." ;
    skos:inScheme cs: ;
    skos:narrower :ecology ;
    skos:notation "31"^^<https://linked.data.gov.au/def/anzsrc-for/2020> ;
    skos:prefLabel "biological sciences"@en ;
    skos:topConceptOf cs: ;
    schema:citation "https://linked.data.gov.au/def/earth-science-data-category/biological-sciences"^^xsd:anyURI ;
.

:biostratigraphy
    a skos:Concept ;
    rdfs:isDefinedBy cs: ;
    skos:broadMatch <https://linked.data.gov.au/def/anzsrc-for/2020/370510> ;
    skos:broader
        :paleontology ,
        :stratigraphy ;
    skos:definition "The element of stratigraphy that deals with the distribution of fossils in the stratigraphic record and the organization of strata into units on the basis of their contained fossils, specifically to date and correlate strata to elucidate Earth's history. In the petroleum industry, biostratigraphy often denotes the use of terrestrial (pollen and spores) and marine (diatoms, foraminifera, nanofossils) microfossils to determine the numerical or relative age and depositional environment of a particular formation, source rock, or reservoir of interest."@en ;
    skos:historyNote "Definition adapted from Schlumberger Oilfield Glossary and Glossary of geology (5th edition revised; Neuendorf, 2011)." ;
    skos:inScheme cs: ;
    skos:prefLabel "biostratigraphy"@en ;
    schema:citation
        "https://glossary.americangeosciences.org/term/biostratigraphy"^^xsd:anyURI ,
        "https://glossary.slb.com/en/terms/b/biostratigraphy"^^xsd:anyURI ;
.

:built-environment-and-design
    a skos:Concept ;
    rdfs:isDefinedBy
        cs: ,
        <https://linked.data.gov.au/def/anzsrc-for/2020> ;
    skos:definition "Built environment refers to human-made conditions and physical features, and is commonly used in architecture, landscape architecture, urban and regional planning, public health, sociology, and anthropology, among others. These curated spaces provide the setting for human activity and were created to fulfill human desires and needs. The term can refer to a plethora of components including the traditionally associated buildings, cities, public infrastructure, transportation, open space, as well as more conceptual components like farmlands, dammed rivers, wildlife management, and even domesticated animals. Studies of the built environment often highlight the connection between physical space and social consequences. It impacts the environment and how society physically manoeuvers and functions, as well as less tangible aspects of society such as socioeconomic inequity and health."@en ;
    skos:exactMatch
        <https://linked.data.gov.au/def/anzsrc-for/2020/33> ,
        <https://linked.data.gov.au/def/earth-science-data-category/built-environment-and-design> ;
    skos:historyNote "From the Fields of Research vocabulary from the Australian and New Zealand Standard Research Classification (ANZSRC, 2020). Definition adapted from Wikipedia." ;
    skos:inScheme cs: ;
    skos:narrower :urban-and-regional-planning ;
    skos:notation "33"^^<https://linked.data.gov.au/def/anzsrc-for/2020> ;
    skos:prefLabel "built environment and design"@en ;
    skos:topConceptOf cs: ;
    schema:citation "https://en.wikipedia.org/wiki/Built_environment"^^xsd:anyURI ;
.

:climate-change-science
    a skos:Concept ;
    rdfs:isDefinedBy
        cs: ,
        <https://linked.data.gov.au/def/anzsrc-for/2020> ;
    skos:broader :atmospheric-sciences ;
    skos:definition "Climate change science is the study of changes in the statistical properties of the climate system that persists for several decades or longer — usually at least 30 years. In a broader sense, climate change science also includes previous long-term changes to Earth's climate. These statistical properties include averages, variability and extremes. Climate change may be due to natural processes, such as changes in the Sun’s radiation, volcanoes activity or internal variability in the climate system, or due to human influences such as changes in the composition of the atmosphere or land use caused by human activity (e.g. burning of fossil fuels, deforestation). In common usage, climate change is often used interchangeably to describe global warming — the ongoing increase in global average temperature — and its effects on Earth's climate system."@en ;
    skos:exactMatch <https://linked.data.gov.au/def/anzsrc-for/2020/3702> ;
    skos:historyNote "From the Fields of Research vocabulary from the Australian and New Zealand Standard Research Classification (ANZSRC, 2020). Definition adapted from Wikipedia." ;
    skos:inScheme cs: ;
    skos:narrower :climatology ;
    skos:notation "3702"^^<https://linked.data.gov.au/def/anzsrc-for/2020> ;
    skos:prefLabel "climate change science"@en ;
    schema:citation
        "https://en.wikipedia.org/wiki/Climate_change"^^xsd:anyURI ,
        "https://www.science.org.au/learning/general-audience/science-climate-change/1-what-is-climate-change"^^xsd:anyURI ;
.

:data-science-and-data-management
    a skos:Concept ;
    rdfs:isDefinedBy
        cs: ,
        <https://linked.data.gov.au/def/anzsrc-for/2020> ;
    skos:altLabel "data management and data science"@en ;
    skos:broader :information-and-computing-sciences ;
    skos:definition "Data science is an interdisciplinary academic field that uses statistics, scientific computing, scientific methods, processes, algorithms, and systems to extract or extrapolate knowledge and insights from noisy, structured, and unstructured data. Data management is the practice of collecting, organizing, protecting, and storing an organization’s data so it can be analysed for business decisions or provided to third parties."@en ;
    skos:historyNote "From the Fields of Research vocabulary from the Australian and New Zealand Standard Research Classification (ANZSRC, 2020). Definition adapted from Wikipedia." ;
    skos:inScheme cs: ;
    skos:narrower :data-mining-and-knowledge-discovery ;
    skos:prefLabel "data science and data management"@en ;
    schema:citation
        "https://en.wikipedia.org/wiki/Data_science"^^xsd:anyURI ,
        "https://www.tableau.com/learn/articles/what-is-data-management"^^xsd:anyURI ;
    skos:exactMatch <https://linked.data.gov.au/def/anzsrc-for/2020/4605> ;
    skos:notation "4605"^^<https://linked.data.gov.au/def/anzsrc-for/2020> ;
.

:environmental-geology
    a skos:Concept ;
    rdfs:isDefinedBy cs: ;
    skos:broader :geology ;
    skos:definition "A multidisciplinary, applied science concerned with the practical application of the principles of geology in the solving of environmental problems created by humans and their activities. Environmental geology is specifically concerned with Earth processes, Earth resources, and engineering properties of Earth materials that are relevant to: 1) the protection of human health and natural ecosystems from adverse biochemical and/or geochemical reactions to naturally occurring chemicals or to chemicals and chemical compounds released into the environment by human activities; and 2) the protection of life, safety, and well-being human from natural processes, such as floods, hurricanes, earthquakes and landslides, through land-use planning."@en ;
    skos:historyNote "Definition adapted from Wikipedia and Glossary of geology (5th edition revised; Neuendorf et al., 2011)." ;
    skos:inScheme cs: ;
    skos:narrower :urban-geology ;
    skos:prefLabel "environmental geology"@en ;
    schema:citation
        "https://en.wikipedia.org/wiki/Environmental_geology"^^xsd:anyURI ,
        "https://glossary.americangeosciences.org/term/environmentalgeology"^^xsd:anyURI ;
.

:environmental-management
    a skos:Concept ;
    rdfs:isDefinedBy cs: ;
    skos:broader :environmental-sciences ;
    skos:definition "Environmental resource management or environmental management is the management of the interaction and impact of human societies on the environment (and not the management of the environment itself)."@en ;
    skos:historyNote "Definition adapted from Wikipedia." ;
    skos:inScheme cs: ;
    skos:narrower :rehabilitation ;
    skos:prefLabel "environmental management"@en ;
    schema:citation "https://en.wikipedia.org/wiki/Environmental_resource_management"^^xsd:anyURI ;
.

:geobiology
    a skos:Concept ;
    rdfs:isDefinedBy cs: ;
    skos:broader :geology ;
    skos:definition "An interdisciplinary study of life sciences and Earth sciences, i.e. the field of scientific research that explores the interactions between the physical Earth and the biosphere to investigate the evolutionary interconnectedness of life and Earth — it deals with process (how organisms affect the Earth and vice versa), as well as history (how the Earth and life have changed together). There is considerable overlap with the fields of ecology, evolutionary biology, microbiology, paleontology, and particularly soil science and biogeochemistry. Geobiology applies the principles and methods of biology, geology and soil science to the study of the ancient history of the co-evolution of life and Earth as well as the role of life in the modern world. Geobiological studies tend to be focused on micro-organisms, and on the role that life plays in altering the chemical and physical environment of the pedosphere, which exists at the intersection of the lithosphere, atmosphere, hydrosphere and/or cryosphere. It differs from biogeochemistry in that the focus is on processes and organisms over space and time rather than on global chemical cycles."@en ;
    skos:historyNote """Compiled by the Geological Survey of Western Australia. Definition adapted from:
1) Wikipedia
2) Yin, H, Xie, S, Qing, J, Yan, J and Luo, G 2008, Discussion on geobiology, biogeology and geobiofacies: Sci. China Ser. D-Earth Sci., v. 51, p. 1516–1524), doi:10.1007/s11430-008-0120-6).""" ;
    skos:inScheme cs: ;
    skos:narrower :biogeology ;
    skos:prefLabel "geobiology"@en ;
    schema:citation
        "https://en.wikipedia.org/wiki/Geobiology"^^xsd:anyURI ,
        "https://glossary.americangeosciences.org/term/geobiology"^^xsd:anyURI ,
        "https://link.springer.com/article/10.1007/s11430-008-0120-6"^^xsd:anyURI ,
        "https://onlinelibrary.wiley.com/journal/14724669"^^xsd:anyURI ;
.

:geodesy
    a skos:Concept ;
    rdfs:isDefinedBy
        cs: ,
        <https://linked.data.gov.au/def/anzsrc-for/2020> ;
    skos:broader :geophysics ;
    skos:definition "The science of measuring and representing the geometry (size and shape) of the Earth and the precise location of points on its surface; it includes the determination of the gravitational field of the Earth and the study of temporal variations such as Earth tides, polar motion, and rotation of the Earth."@en ;
    skos:exactMatch <https://linked.data.gov.au/def/anzsrc-for/2020/370603> ;
    skos:historyNote "From the Fields of Research vocabulary from the Australian and New Zealand Standard Research Classification (ANZSRC, 2020). Definition adapted from Glossary of geology (5th edition revised; Neuendorf et al., 2011) and Wikipedia." ;
    skos:inScheme cs: ;
    skos:narrower :elevation ;
    skos:notation "370603"^^<https://linked.data.gov.au/def/anzsrc-for/2020> ;
    skos:prefLabel "geodesy"@en ;
    schema:citation
        "https://en.wikipedia.org/wiki/Geodesy"^^xsd:anyURI ,
        "https://glossary.americangeosciences.org/term/geodesy"^^xsd:anyURI ;
.

:geomathematics
    a skos:Concept ;
    rdfs:isDefinedBy cs: ;
    skos:altLabel
        "mathematical geology"@en ,
        "mathematical geoscience"@en ;
    skos:broader :geology ;
    skos:definition "The development and application of mathematical methods and principles to process geoscientific data for geological feature imaging or for understanding (modelling) geological processes, from the atomic to planetary scale, across the entire spectrum of geoscientific disciplines."@en ;
    skos:historyNote "Definition compiled by the Geological Survey of Western Australia." ;
    skos:inScheme cs: ;
    skos:narrower :geostatistics ;
    skos:prefLabel "geomathematics"@en ;
    schema:citation "https://en.wikipedia.org/wiki/Geomathematics"^^xsd:anyURI ;
.

:gravimetrics
    a skos:Concept ;
    rdfs:isDefinedBy
        cs: ,
        <https://linked.data.gov.au/def/anzsrc-for/2020> ;
    skos:altLabel "gravity"@en ;
    skos:broader :geophysics ;
    skos:definition "The measure of changes in gravity due to variations in the density of the rocks to remotely map the distribution of different rock types and the structure of rocks in the Earth's subsurface."@en ;
    skos:exactMatch
        <https://linked.data.gov.au/def/anzsrc-for/2020/370606> ,
        <https://linked.data.gov.au/def/earth-science-data-category/gravity> ;
    skos:historyNote "From the Fields of Research vocabulary from the Australian and New Zealand Standard Research Classification (ANZSRC, 2020). Definition adapted from Glossary of geology (5th edition revised; Neuendorf et al., 2011)." ;
    skos:inScheme cs: ;
    skos:narrower :gravity-gradiometry ;
    skos:notation "370606"^^<https://linked.data.gov.au/def/anzsrc-for/2020> ;
    skos:prefLabel "gravimetrics"@en ;
    schema:citation "https://glossary.americangeosciences.org/term/gravimetric"^^xsd:anyURI ;
.

:human-society
    a skos:Concept ;
    rdfs:isDefinedBy
        cs: ,
        <https://linked.data.gov.au/def/anzsrc-for/2020> ;
    skos:definition "The study of a group of individuals involved in persistent social interaction or of a large social group sharing the same spatial or social territory, typically subject to the same political authority and dominant cultural expectations."@en ;
    skos:exactMatch <https://linked.data.gov.au/def/anzsrc-for/2020/44> ;
    skos:historyNote "From the Fields of Research vocabulary from the Australian and New Zealand Standard Research Classification (ANZSRC, 2020). Definition adapted from Wikipedia." ;
    skos:inScheme cs: ;
    skos:narrower :policy-and-administration ;
    skos:notation "44"^^<https://linked.data.gov.au/def/anzsrc-for/2020> ;
    skos:prefLabel "human society"@en ;
    skos:topConceptOf cs: ;
    schema:citation "https://en.wikipedia.org/wiki/Society"^^xsd:anyURI ;
.

:marine-geoscience
    a skos:Concept ;
    rdfs:isDefinedBy cs: ;
    skos:altLabel
        "geological oceanography"@en ,
        "marine geology"@en ;
    skos:broader :geology ;
    skos:definition "The study of the history and structure of the ocean floor. It involves geophysical, geochemical, sedimentological and paleontological investigations of the ocean floor and coastal zone."@en ;
    skos:exactMatch
        <https://linked.data.gov.au/def/anzsrc-for/2020/370504> ,
        <https://linked.data.gov.au/def/earth-science-data-category/marine-geoscience> ;
    skos:historyNote "From the Fields of Research vocabulary from the Australian and New Zealand Standard Research Classification (ANZSRC, 2020). Definition adapted from Wikipedia." ;
    skos:inScheme cs: ;
    skos:narrower :oceanography ;
    skos:notation "370504"^^<https://linked.data.gov.au/def/anzsrc-for/2020> ;
    skos:prefLabel "marine geoscience"@en ;
    schema:citation "https://en.wikipedia.org/wiki/Marine_geology"^^xsd:anyURI ;
.

:micropaleontology
    a skos:Concept ;
    rdfs:isDefinedBy cs: ;
    skos:broader :paleontology ;
    skos:definition "The systematic study of microfossils (i.e. fossils too small to be observed without the aid of a microscope), their morphology, classification, and environmental and biostratigraphic significance. Microfossils can represent the remains, or partial remains, of a wide range of organism kingdoms and phyla, but palynomorphs are generally excluded."@en ;
    skos:exactMatch <https://linked.data.gov.au/def/earth-science-data-category/micropaleontology> ;
    skos:historyNote """Definition adapted from:
Saraswati, PK and Srinivasan, MS 2015, Micropaleontology: principles and applications: Springer Cham, 224p., doi.10.1007/978-3-319-14574-7.""" ;
    skos:inScheme cs: ;
    skos:narrower :palynology ;
    skos:prefLabel "micropaleontology"@en ;
    schema:citation
        "https://doi.org/10.1007/978-3-319-14574-7"^^xsd:anyURI ,
        "https://glossary.americangeosciences.org/term/micropaleontology"^^xsd:anyURI ;
.

:morphological-paleontology
    a skos:Concept ;
    rdfs:isDefinedBy cs: ;
    skos:altLabel
        "palaeomorphology"@en ,
        "paleomorphology"@en ;
    skos:broader :paleontology ;
    skos:definition "A branch of paleontology that deals with the form and structure of organisms based on their fossil remains; especially a study of the forms, relations, and phylogenetic development of biological structures apart from their functions."@en ;
    skos:historyNote "Definition adapted from Glossary of geology (5th edition revised; Neuendorf et al., 2011)." ;
    skos:inScheme cs: ;
    skos:narrower :functional-morphology ;
    skos:prefLabel "morphological paleontology"@en ;
    schema:citation "https://glossary.americangeosciences.org/term/morphologypaleont"^^xsd:anyURI ;
.

:paleoclimatology
    a skos:Concept ;
    rdfs:isDefinedBy
        cs: ,
        <https://linked.data.gov.au/def/anzsrc-for/2020> ;
    skos:altLabel "palaeoclimatology"@en ;
    skos:broader :physical-geography-and-environmental-geoscience ;
    skos:definition "The study of climates prior to the period of instrumental records, and of the causes of their variation, on either a local, regional or worldwide basis. It uses a variety of proxy methods from the Earth and life sciences to obtain data preserved within rocks, sediments, ice sheets, tree rings, corals, shells, and microfossils to determine the past states of the Earth's various climate regions and its atmospheric system."@en ;
    skos:exactMatch
        <https://linked.data.gov.au/def/anzsrc-for/2020/370904> ,
        <https://linked.data.gov.au/def/earth-science-data-category/paleoclimatology> ;
    skos:historyNote "From the Fields of Research vocabulary from the Australian and New Zealand Standard Research Classification (ANZSRC, 2020). Definition adapted from Glossary of geology (5th edition revised; Neuendorf et al., 2011) and Wikipedia." ;
    skos:inScheme cs: ;
    skos:narrower :paleoenvironmental-reconstruction ;
    skos:notation "370904"^^<https://linked.data.gov.au/def/anzsrc-for/2020> ;
    skos:prefLabel "paleoclimatology"@en ;
    schema:citation
        "https://en.wikipedia.org/wiki/Paleoclimatology"^^xsd:anyURI ,
        "https://glossary.americangeosciences.org/term/paleoclimatology"^^xsd:anyURI ;
.

:petrography
    a skos:Concept ;
    rdfs:isDefinedBy cs: ;
    skos:broader :petrology ;
    skos:definition "That branch of geology dealing with the description and systematic classification of rocks and especially by means of microscopic examination of thin sections. Petrography is more restricted in scope than petrology and overlaps considerably with mineralogy."@en ;
    skos:historyNote "Definition adapted from Glossary of geology (5th edition revised; Neuendorf et al., 2011)." ;
    skos:inScheme cs: ;
    skos:narrower :ore-microscopy ;
    skos:prefLabel "petrography"@en ;
    schema:citation "https://glossary.americangeosciences.org/term/petrography"^^xsd:anyURI ;
.

:photogrammetry-and-remote-sensing
    a skos:Concept ;
    rdfs:isDefinedBy
        cs: ,
        <https://linked.data.gov.au/def/anzsrc-for/2020> ;
    skos:altLabel "photogeology"@en ;
    skos:broader :geomatic-engineering ;
    skos:definition "The science and technology of collecting/measuring, processing, analysing and interpreting information from noncontact imaging and other sensor systems that record the interaction between electromagnetic energy and matter, i.e. the acquisition of information about an object or phenomenon by using a recording device that is not in physical contact with the subject being studied. Aerial photographs and imagery acquired from a satellite or drone are examples of remotely sensed information."@en ;
    skos:exactMatch <https://linked.data.gov.au/def/anzsrc-for/2020/401304> ;
    skos:historyNote "From the Fields of Research vocabulary from the Australian and New Zealand Standard Research Classification (ANZSRC, 2020). Definition adapted from Glossary of geology (5th edition revised; Neuendorf et al., 2011) and Wikipedia." ;
    skos:inScheme cs: ;
    skos:narrowMatch <https://linked.data.gov.au/def/earth-science-data-category/remote-sensing> ;
    skos:narrower :spectral-imaging ;
    skos:notation "401304"^^<https://linked.data.gov.au/def/anzsrc-for/2020> ;
    skos:prefLabel "photogrammetry and remote sensing"@en ;
    schema:citation
        "https://en.wikipedia.org/wiki/Photogrammetry"^^xsd:anyURI ,
        "https://en.wikipedia.org/wiki/Remote_sensing"^^xsd:anyURI ,
        "https://gisgeography.com/hyperspectral-imaging/"^^xsd:anyURI ,
        "https://glossary.americangeosciences.org/term/remotesensing"^^xsd:anyURI ;
.

:physical-sciences
    a skos:Concept ;
    rdfs:isDefinedBy
        cs: ,
        <https://linked.data.gov.au/def/anzsrc-for/2020> ;
    skos:definition "The systematic study of the inorganic world, as distinct from the study of the organic world, which is the province of biological science. Physical science is ordinarily thought of as consisting of four broad areas: astronomy, physics, chemistry, and the Earth sciences. Each of these is in turn divided into fields and subfields."@en ;
    skos:exactMatch <https://linked.data.gov.au/def/anzsrc-for/2020/51> ;
    skos:historyNote "From the Fields of Research vocabulary from the Australian and New Zealand Standard Research Classification (ANZSRC, 2020). Definition adapted from www.britannica.com." ;
    skos:inScheme cs: ;
    skos:narrower :astronomical-sciences ;
    skos:notation "51"^^<https://linked.data.gov.au/def/anzsrc-for/2020> ;
    skos:prefLabel "physical sciences"@en ;
    skos:topConceptOf cs: ;
    schema:citation "https://www.britannica.com/science/physical-science"^^xsd:anyURI ;
.

:regolith-chemistry
    a skos:Concept ;
    rdfs:isDefinedBy cs: ;
    skos:broader :geochemistry ;
    skos:definition "The study of the chemical composition of materials and components making up the surficial, weathered, and usually unconsolidated layer that nearly everywhere forms the surface of the land and overlies or covers the bedrock. Regolith includes rock debris of all kinds, volcanic ash, glacial drift, alluvium, loess and eolian deposits, vegetal accumulations, and soil."@en ;
    skos:historyNote "Compiled by the Geological Survey of Western Australia. Definition adapted from Glossary of geology (5th edition, revised; Neuendorf et al., 2011)." ;
    skos:inScheme cs: ;
    skos:narrower :soil-chemistry ;
    skos:prefLabel "regolith chemistry"@en ;
    schema:citation "https://glossary.americangeosciences.org/term/regolithweath"^^xsd:anyURI ;
.

:seismology-and-seismic-exploration
    a skos:Concept ;
    rdfs:isDefinedBy
        cs: ,
        <https://linked.data.gov.au/def/anzsrc-for/2020> ;
    skos:broader :geophysics ;
    skos:definition "The scientific study of earthquakes and the propagation of elastic waves both natural and artificially generated through the Earth or through other planetary bodies. The field also includes studies of earthquake environmental effects such as tsunamis as well as diverse seismic sources such as volcanic, tectonic, oceanic, atmospheric, and artificial processes such as explosions. Seismic exploration is a method of exploration geophysics that uses the principles of seismology to estimate the properties of the Earth's subsurface from artificially generated seismic waves."@en ;
    skos:exactMatch
        <https://linked.data.gov.au/def/anzsrc-for/2020/370609> ,
        <https://linked.data.gov.au/def/earth-science-data-category/seismology-and-seismic-exploration> ;
    skos:historyNote "From the Fields of Research vocabulary from the Australian and New Zealand Standard Research Classification (ANZSRC, 2020). Definition adapted from Wikipedia and Glossary of geology (5th edition revised; Neuendorf et al., 2011)." ;
    skos:inScheme cs: ;
    skos:narrower :seismic-surveys ;
    skos:notation "370609"^^<https://linked.data.gov.au/def/anzsrc-for/2020> ;
    skos:prefLabel "seismology and seismic exploration"@en ;
    schema:citation
        "https://en.wikipedia.org/wiki/Seismology"^^xsd:anyURI ,
        "https://glossary.americangeosciences.org/term/seismology"^^xsd:anyURI ;
.

:soil-sciences
    a skos:Concept ;
    rdfs:isDefinedBy
        cs: ,
        <https://linked.data.gov.au/def/anzsrc-for/2020> ;
    skos:broader :environmental-sciences ;
    skos:definition "The science dealing with soils as a natural resource on the surface of the Earth including (a) soil formation, soil classification and mapping; (b) physical, chemical, biological, and fertility properties of soils per se; and (c) these properties in relation to the use and management of soils."@en ;
    skos:exactMatch <https://linked.data.gov.au/def/anzsrc-for/2020/4106> ;
    skos:historyNote "From the Fields of Research vocabulary from the Australian and New Zealand Standard Research Classification (ANZSRC, 2020). Definition adapted from Glossary of geology (5th edition revised; Neuendorf et al., 2011)." ;
    skos:inScheme cs: ;
    skos:narrower :pedology-and-pedometrics ;
    skos:notation "4106"^^<https://linked.data.gov.au/def/anzsrc-for/2020> ;
    skos:prefLabel "soil sciences"@en ;
    schema:citation "https://glossary.americangeosciences.org/term/soilscience"^^xsd:anyURI ;
.

:tectonics
    a skos:Concept ;
    rdfs:isDefinedBy cs: ;
    skos:broadMatch <https://linked.data.gov.au/def/anzsrc-for/2020/370511> ;
    skos:broader :structural-geology-and-tectonics ;
    skos:definition "The branch of geology dealing with the broad architecture of the outer part of the Earth, i.e. the regional assembling of structural or deformational features, a study of their mutual relations, origin and historical evolution. It is closely related to structural geology, with which the distinctions are blurred, but tectonics generally deals with larger features."@en ;
    skos:historyNote "Definition adapted from Glossary of geology (5th edition revised; Neuendorf et al., 2011)." ;
    skos:inScheme cs: ;
    skos:narrower :neotectonics ;
    skos:prefLabel "tectonics"@en ;
    schema:citation "https://glossary.americangeosciences.org/term/tectonics"^^xsd:anyURI ;
.

:urban-and-regional-planning
    a skos:Concept ;
    rdfs:isDefinedBy
        cs: ,
        <https://linked.data.gov.au/def/anzsrc-for/2020> ;
    skos:broader :built-environment-and-design ;
    skos:definition "Urban planning, also known as town planning, city planning, regional planning, or rural planning in specific contexts, is a technical and political process that is focused on the development and design of land use and the built environment, including air, water, and the infrastructure passing into and out of urban areas, such as transportation, communications, and distribution networks, and their accessibility. Traditionally, urban planning followed a top-down approach in master planning the physical layout of human settlements, with a primary focus on public welfare (i.e. considerations of efficiency, sanitation, protection and use of the environment) as well as effects of the master plans on the social and economic activities. Over time, urban planning's focus has shifted to social and environmental factors to be a tool to improve the health and well-being of people while maintaining sustainability standards."@en ;
    skos:exactMatch
        <https://linked.data.gov.au/def/anzsrc-for/2020/3304> ,
        <https://linked.data.gov.au/def/earth-science-data-category/urban-and-regional-planning> ;
    skos:historyNote "From the Fields of Research vocabulary from the Australian and New Zealand Standard Research Classification (ANZSRC, 2020). Definition adapted from Wikipedia." ;
    skos:inScheme cs: ;
    skos:narrower :land-use-and-environmental-planning ;
    skos:notation "3304"^^<https://linked.data.gov.au/def/anzsrc-for/2020> ;
    skos:prefLabel "urban and regional planning"@en ;
    schema:citation "https://en.wikipedia.org/wiki/Urban_planning"^^xsd:anyURI ;
.

<https://linked.data.gov.au/org/gswa>
    a schema:Organization ;
    schema:name "Gswa" ;
    schema:url ""^^xsd:anyURI ;
.

:archeology
    a skos:Concept ;
    rdfs:isDefinedBy
        cs: ,
        <https://linked.data.gov.au/def/anzsrc-for/2020> ;
    skos:altLabel "archaeology"@en ;
    skos:broader :history-heritage-and-archeology ;
    skos:definition "The study of human cultures through the recovery and analysis of their material relics."@en ;
    skos:exactMatch <https://linked.data.gov.au/def/anzsrc-for/2020/4301> ;
    skos:historyNote "From the Fields of Research vocabulary from the Australian and New Zealand Standard Research Classification (ANZSRC, 2020). Definition adapted from Glossary of geology (5th edition revised; Neuendorf et al., 2011)." ;
    skos:inScheme cs: ;
    skos:narrower
        :geoarcheology ,
        :maritime-archeology ;
    skos:notation "4301"^^<https://linked.data.gov.au/def/anzsrc-for/2020> ;
    skos:prefLabel "archeology"@en ;
    schema:citation "https://glossary.americangeosciences.org/term/archaeology"^^xsd:anyURI ;
.

:artificial-intelligence
    a skos:Concept ;
    rdfs:isDefinedBy
        cs: ,
        <https://linked.data.gov.au/def/anzsrc-for/2020> ;
    skos:broader :information-and-computing-sciences ;
    skos:definition "Artificial intelligence (AI), in its broadest sense, is intelligence exhibited by machines, particularly computer systems, i.e. the capability of machines/computers to imitate intelligent human behaviour without being explicitly programmed. By extension, a field of research in computer science that develops and studies methods and software that enable machines to perceive their environment and uses learning and intelligence to take actions that maximize their chances of achieving defined goals."@en ;
    skos:exactMatch <https://linked.data.gov.au/def/anzsrc-for/2020/4602> ;
    skos:historyNote "From the Fields of Research vocabulary from the Australian and New Zealand Standard Research Classification (ANZSRC, 2020). Definition adapted from Wikipedia." ;
    skos:inScheme cs: ;
    skos:narrower
        :deep-learning ,
        :machine-learning ;
    skos:notation
        "AI"^^xsd:token ,
        "4602"^^<https://linked.data.gov.au/def/anzsrc-for/2020> ;
    skos:prefLabel "artificial intelligence"@en ;
    schema:citation "https://en.wikipedia.org/wiki/Artificial_intelligence"^^xsd:anyURI ;
.

:evolutionary-paleontology
    a skos:Concept ;
    rdfs:isDefinedBy cs: ;
    skos:altLabel
        "evolutionary paleobiology"@en ,
        "evolutionary systematics"@en ;
    skos:broader :paleontology ;
    skos:definition "Evolutionary paleontology (also called evolutionary paleobiology) is paleontology’s intersection with evolutionary biology. Its main aims are to reconstruct the history of life on Earth (historical paleontology, phylogeny) and the patterns and causes of evolutionary change and extinction (biological and physical processes and unique historical events)."@en ;
    skos:historyNote "Definition adapted from https://www.eolss.net/sample-chapters/c01/e6-15-04-04.pdf." ;
    skos:inScheme cs: ;
    skos:narrower
        :phylogenetics ,
        :taxonomy ;
    skos:prefLabel "evolutionary paleontology"@en ;
    schema:citation
        "https://glossary.americangeosciences.org/term/evolutionarysystematics"^^xsd:anyURI ,
        "https://www.cambridge.org/core/books/abs/cambridge-encyclopedia-of-darwin-and-evolutionary-thought/evolutionary-paleontology/5BDCDBF889B070957B30FA42D5D1A6B4"^^xsd:anyURI ,
        "https://www.eolss.net/sample-chapters/c01/e6-15-04-04.pdf"^^xsd:anyURI ;
.

:geoscience-data-visualisation
    a skos:Concept ;
    rdfs:isDefinedBy
        cs: ,
        <https://linked.data.gov.au/def/anzsrc-for/2020> ;
    skos:broader :geoinformatics ;
    skos:definition "The developing of tools that promote geoscience data integration and synthesis, and also facilitate quantitative cross-disciplinary access to data."@en ;
    skos:exactMatch <https://linked.data.gov.au/def/anzsrc-for/2020/370403> ;
    skos:historyNote """From the Fields of Research vocabulary from the Australian and New Zealand Standard Research Classification (ANZSRC, 2020). Definition adapted from:
Ferrini, V, Carbotte, S, Ryan, W and Chan, S 2013, Geoscience data visualization and analysis using GeoMapApp: EGU General Assembly 2013, 7–12 April, 2013, Vienna, Austria, EGU2013-6699.""" ;
    skos:inScheme cs: ;
    skos:narrower
        :geological-modelling ,
        :geophysical-modelling ;
    skos:notation "370403"^^<https://linked.data.gov.au/def/anzsrc-for/2020> ;
    skos:prefLabel "geoscience data visualisation"@en ;
    schema:citation "https://meetingorganizer.copernicus.org/EGU2013/EGU2013-6699.pdf"^^xsd:anyURI ;
.

:geothermics-and-radiometrics
    a skos:Concept ;
    rdfs:isDefinedBy
        cs: ,
        <https://linked.data.gov.au/def/anzsrc-for/2020> ;
    skos:broader :geophysics ;
    skos:definition "The study of heatflow and radioactive activity within the Earth."@en ;
    skos:exactMatch <https://linked.data.gov.au/def/anzsrc-for/2020/370605> ;
    skos:historyNote "From the Fields of Research vocabulary from the Australian and New Zealand Standard Research Classification (ANZSRC, 2020)." ;
    skos:inScheme cs: ;
    skos:narrower
        :geothermics ,
        :radiometrics ;
    skos:notation "370605"^^<https://linked.data.gov.au/def/anzsrc-for/2020> ;
    skos:prefLabel "geothermics and radiometrics"@en ;
.

:isotope-age-determination
    a skos:Concept ;
    rdfs:isDefinedBy cs: ;
    skos:altLabel "isotope dating"@en ;
    skos:broader :geochronology ;
    skos:definition "The application of natural variations in the relative abundances of isotopes of various elements, measured by isotope-ratio mass spectrometry, to reveal information about the ages of rock, air or water bodies, or processes of mixing between them."@en ;
    skos:historyNote "Definition adapted from Wikipedia." ;
    skos:inScheme cs: ;
    skos:narrower
        :non-radiogenic-system-age-determination ,
        :radiogenic-isotopic-system-age-determination ;
    skos:prefLabel "isotope age determination"@en ;
    schema:citation "https://en.wikipedia.org/wiki/Isotope_geochemistry"^^xsd:anyURI ;
.

:isotope-geochemistry
    a skos:Concept ;
    rdfs:isDefinedBy
        cs: ,
        <https://linked.data.gov.au/def/anzsrc-for/2020> ;
    skos:broader :geochemistry ;
    skos:definition "The determination of the relative and absolute concentrations of the elements and their isotopes in the Earth and on Earth's surface."@en ;
    skos:exactMatch
        <https://linked.data.gov.au/def/anzsrc-for/2020/370303> ,
        <https://linked.data.gov.au/def/earth-science-data-category/isotope-geochemistry> ;
    skos:historyNote """From the Fields of Research vocabulary from the Australian and New Zealand Standard Research Classification (ANZSRC, 2020). Definition adapted from:
Kendall, C and Caldwell, EA 1998, Chapter 2: Fundamentals of Isotope Geochemistry, in Isotope Tracers in Catchment Hydrology, edited by C Kendall and JJ McDonnell: Amsterdam, Elsevier Science, p. 51–86.""" ;
    skos:inScheme cs: ;
    skos:narrower
        :non-radiogenic-isotope-geochemistry ,
        :radiogenic-isotope-geochemistry ;
    skos:notation "370303"^^<https://linked.data.gov.au/def/anzsrc-for/2020> ;
    skos:prefLabel "isotope geochemistry"@en ;
    schema:citation "https://wwwrcamnl.wr.usgs.gov/isoig/isopubs/itchch2.html"^^xsd:anyURI ;
.

:land-use-and-environmental-planning
    a skos:Concept ;
    rdfs:isDefinedBy
        cs: ,
        <https://linked.data.gov.au/def/anzsrc-for/2020> ;
    skos:broader :urban-and-regional-planning ;
    skos:definition "Land-use and environmental planning involves the regulation and commitment of land-use, as to how the landscape is used (whether for food production, forestry, nature conservation, water storage, urban development, mining, etc.), to ensure the most efficient, effective and beneficial management and utilization of resources, and to provide optimal environmental and social outcomes."@en ;
    skos:exactMatch
        <https://linked.data.gov.au/def/anzsrc-for/2020/330404> ,
        <https://linked.data.gov.au/def/earth-science-data-category/land-use-and-environmental-planning> ;
    skos:historyNote "From the Fields of Research vocabulary from the Australian and New Zealand Standard Research Classification (ANZSRC, 2020). Definition from Geological Survey of Queensland Earth science data category vocabulary." ;
    skos:inScheme cs: ;
    skos:narrower
        :geoconservation ,
        :geotourism ;
    skos:notation "330404"^^<https://linked.data.gov.au/def/anzsrc-for/2020> ;
    skos:prefLabel "land use and environmental planning"@en ;
    schema:citation "https://linked.data.gov.au/def/earth-science-data-category/land-use-and-environmental-planning"^^xsd:anyURI ;
.

:logging
    a skos:Concept ;
    rdfs:isDefinedBy cs: ;
    skos:broader :resource-geoscience ;
    skos:definition "The acquisition of a continuous record as a function of depth, usually graphic and plotted to scale, of observations, analyses or measurements made on the geological materials of the section exposed in a borehole or of the sample (drillcore or cuttings) obtained from it."@en ;
    skos:historyNote "Definition adapted from Glossary of geology (5th edition revised; Neuendorf et al., 2011)." ;
    skos:inScheme cs: ;
    skos:narrower
        :borehole-logging ,
        :core-logging ;
    skos:prefLabel "logging"@en ;
    schema:citation
        "https://glossary.americangeosciences.org/term/log"^^xsd:anyURI ,
        "https://glossary.americangeosciences.org/term/logging"^^xsd:anyURI ;
.

:magnetism-and-paleomagnetism
    a skos:Concept ;
    rdfs:isDefinedBy
        cs: ,
        <https://linked.data.gov.au/def/anzsrc-for/2020> ;
    skos:altLabel "magnetism and palaeomagnetism"@en ;
    skos:broader :geophysics ;
    skos:definition "The study of physical phenomena associated with moving electricity in conductive rocks or the permanent magnetic effects of naturally magnetic rocks, and the study of natural remanent magnetization of Earth materials in order to determine the direction, and indirectly intensity, of the Earth's magnetic field in the geological past."@en ;
    skos:exactMatch <https://linked.data.gov.au/def/anzsrc-for/2020/370607> ;
    skos:historyNote "From the Fields of Research vocabulary from the Australian and New Zealand Standard Research Classification (ANZSRC, 2020). Definition adapted from Glossary of geology (5th edition revised; Neuendorf et al., 2011)." ;
    skos:inScheme cs: ;
    skos:narrower
        :magnetics ,
        :paleomagnetism ;
    skos:notation "370607"^^<https://linked.data.gov.au/def/anzsrc-for/2020> ;
    skos:prefLabel "magnetism and paleomagnetism"@en ;
    schema:citation
        "https://glossary.americangeosciences.org/term/magnetism"^^xsd:anyURI ,
        "https://glossary.americangeosciences.org/term/paleomagnetism"^^xsd:anyURI ;
.

:mining-geology
    a skos:Concept ;
    rdfs:isDefinedBy cs: ;
    skos:broader :mineral-resource-geology ;
    skos:definition "Studies related to the process of extracting metallic or non-metallic mineral deposits from the Earth. The term may also include the preliminary treatment of extracted materials, e.g. cleaning or sizing."@en ;
    skos:historyNote "Definition adapted from Glossary of geology (5th edition revised; Neuendorf et al., 2011)." ;
    skos:inScheme cs: ;
    skos:narrower
        :geometallurgy ,
        :grade-control ;
    skos:prefLabel "mining geology"@en ;
    schema:citation "https://glossary.americangeosciences.org/term/mining"^^xsd:anyURI ;
.

:organic-geochemistry
    a skos:Concept ;
    rdfs:isDefinedBy
        cs: ,
        <https://linked.data.gov.au/def/anzsrc-for/2020> ;
    skos:broader :geochemistry ;
    skos:definition "The study of the role of processes and compounds that are derived from living or once-living organisms, i.e. the study of the transformation undergone by organic matter of all types, whether of biological or man-made origin, in the Earth System. The transformations involved vary from those mediated by biological processes involved in the production of living tissue and the operation of food-chains, to those controlled by temperature and pressure at depth in the crust. Photochemical processes in the atmosphere and hydrosphere can also be important in controlling the environmental behaviour of some organic compounds."@en ;
    skos:exactMatch
        <https://linked.data.gov.au/def/anzsrc-for/2020/370304> ,
        <https://linked.data.gov.au/def/earth-science-data-category/organic-geochemistry> ;
    skos:historyNote """From the Fields of Research vocabulary from the Australian and New Zealand Standard Research Classification (ANZSRC, 2020). Definition adapted from: 
Killops, SD and Killops, VJ 2013, Introduction to Organic Geochemistry: John Wiley & Sons, 408p.""" ;
    skos:inScheme cs: ;
    skos:narrower
        :petroleum-geochemistry ,
        :source-rock-analysis ;
    skos:notation "370304"^^<https://linked.data.gov.au/def/anzsrc-for/2020> ;
    skos:prefLabel "organic geochemistry"@en ;
    schema:citation "https://onlinelibrary.wiley.com/doi/book/10.1002/9781118697214?msockid=10a50a46387a65d7304119c539486416"^^xsd:anyURI ;
.

:petroleum-geology
    a skos:Concept ;
    rdfs:isDefinedBy cs: ;
    skos:broadMatch <https://linked.data.gov.au/def/earth-science-data-category/petroleum-and-coal-geology> ;
    skos:broader :energy-geoscience ;
    skos:definition "Study of the mode of origin and conditions of accumulation of hydrocarbons in the Earth's crust; their exploration, involving application of the techniques of geophysics, geochemistry, paleontology, stratigraphy, and tectonics; and their evaluation. It includes the assessment of petroleum systems and their composite parts: source, migration pathways, reservoir, seal, and method of entrapment."@en ;
    skos:exactMatch <https://linked.data.gov.au/def/earth-science-data-category/petroleum-geology> ;
    skos:historyNote """Definition adapted from:
Allaby, M 2008, A dictionary of Earth sciences, 4th edition: Oxford University Press, doi.10.1093/acref/9780199211944.001.00010.""" ;
    skos:inScheme cs: ;
    skos:narrower
        :conventional-reservoir-geology ,
        :unconventional-reservoir-geology ;
    skos:prefLabel "petroleum geology"@en ;
    schema:citation "https://www.oxfordreference.com/display/10.1093/oi/authority.20110803100320627"^^xsd:anyURI ;
.

:petrophysics
    a skos:Concept ;
    rdfs:isDefinedBy cs: ;
    skos:broadMatch <https://linked.data.gov.au/def/anzsrc-for/2020/370608> ;
    skos:broader :petrophysics-and-rock-mechanics ;
    skos:definition "The study of the physical and chemical properties of rocks in relation to their interaction with fluids. A major application of petrophysics is in studying reservoirs for the hydrocarbon industry (especially the distribution of the pore system and its contained hydrocarbons and water)."@en ;
    skos:exactMatch <https://linked.data.gov.au/def/earth-science-data-category/petrophysics> ;
    skos:historyNote "Compiled by Geological Survey of Western Australia from multiple sources." ;
    skos:inScheme cs: ;
    skos:narrower
        :core-and-surface-sample-petrophysics ,
        :downhole-petrophysics ;
    skos:prefLabel "petrophysics"@en ;
    schema:citation
        "https://en.wikipedia.org/wiki/Petrophysics"^^xsd:anyURI ,
        "https://glossary.americangeosciences.org/term/petrophysics"^^xsd:anyURI ;
.

:petrophysics-and-rock-mechanics
    a skos:Concept ;
    rdfs:isDefinedBy
        cs: ,
        <https://linked.data.gov.au/def/anzsrc-for/2020> ;
    skos:broader :geophysics ;
    skos:definition "The study of the physical and mechanical properties of rocks. Petrophysics focuses on how the microstructure of porous geological materials affects their mechanical, electrical, thermal, fluid flow, and sonic properties. Rock mechanics considers the mechanical or geomechanical properties of rocks, including reservoir strength, elastic properties, hardness, ultrasonic behaviour, index characteristics, and in situ stresses."@en ;
    skos:exactMatch <https://linked.data.gov.au/def/anzsrc-for/2020/370608> ;
    skos:historyNote "From the Fields of Research vocabulary from the Australian and New Zealand Standard Research Classification (ANZSRC, 2020). Compiled by Geological Survey of Western Australia from multiple sources." ;
    skos:inScheme cs: ;
    skos:narrower
        :petrophysics ,
        :rock-mechanics ;
    skos:notation "370608"^^<https://linked.data.gov.au/def/anzsrc-for/2020> ;
    skos:prefLabel "petrophysics and rock mechanics"@en ;
    schema:citation
        "https://en.wikipedia.org/wiki/Petrophysics"^^xsd:anyURI ,
        "https://environment.leeds.ac.uk/institute-applied-geoscience/doc/petrophysics-geomechanics-2"^^xsd:anyURI ;
.

:seismic-surveys
    a skos:Concept ;
    rdfs:isDefinedBy cs: ;
    skos:altLabel "seismic surveying"@en ;
    skos:broader :seismology-and-seismic-exploration ;
    skos:definition "The science of the acquisition, processing, and analysis of seismic datasets measured and recorded with reference to a particular area of the Earth's surface, to evaluate the subsurface."@en ;
    skos:exactMatch <https://linked.data.gov.au/def/earth-science-data-category/seismic-surveys> ;
    skos:historyNote "Definition from Geological Survey of Queensland Earth science data category vocabulary." ;
    skos:inScheme cs: ;
    skos:narrower
        :active-seismic ,
        :passive-seismic ;
    skos:prefLabel "seismic surveys"@en ;
    schema:citation "https://linked.data.gov.au/def/earth-science-data-category/seismic-surveys"^^xsd:anyURI ;
.

:stakeholder-engagement
    a skos:Concept ;
    rdfs:isDefinedBy cs: ;
    skos:definition "The systematic identification, analysis, planning, and implementation of actions designed to influence stakeholders. This process identifies the needs of key groups and ensures those needs are met."@en ;
    skos:historyNote "Compiled by the Geological Survey of Western Australia. Definition adapted from the Association for Project Management (www.apm.org.uk)." ;
    skos:inScheme cs: ;
    skos:narrower
        :geoscience-communication ,
        :geoscience-education ;
    skos:prefLabel "stakeholder engagement"@en ;
    skos:topConceptOf cs: ;
    schema:citation "https://www.apm.org.uk/resources/find-a-resource/stakeholder-engagement/"^^xsd:anyURI ;
.

:structural-geology-and-tectonics
    a skos:Concept ;
    rdfs:isDefinedBy
        cs: ,
        <https://linked.data.gov.au/def/anzsrc-for/2020> ;
    skos:broader :geology ;
    skos:definition "The branches of geology that, combined, focus on the manifestation of plate tectonic motions in the deformation of Earth's crust and lithosphere, from the scale of mountain ranges to individual faults and folds, and on timescales from deep Earth history to present-day tectonism and associated natural hazards."@en ;
    skos:exactMatch <https://linked.data.gov.au/def/anzsrc-for/2020/370511> ;
    skos:historyNote "From the Fields of Research vocabulary from the Australian and New Zealand Standard Research Classification (ANZSRC, 2020). Definition adapted from: https://epsci.stanford.edu/structural-geology-tectonics-geomechanics." ;
    skos:inScheme cs: ;
    skos:narrower
        :structural-geology ,
        :tectonics ;
    skos:notation "370511"^^<https://linked.data.gov.au/def/anzsrc-for/2020> ;
    skos:prefLabel "structural geology and tectonics"@en ;
    schema:citation
        "https://epsci.stanford.edu/structural-geology-tectonics-geomechanics"^^xsd:anyURI ,
        "https://glossary.americangeosciences.org/term/structuralgeology"^^xsd:anyURI ,
        "https://glossary.slb.com/en/terms/s/structural"^^xsd:anyURI ;
.

:tomography
    a skos:Concept ;
    rdfs:isDefinedBy cs: ;
    skos:broader :geophysics ;
    skos:definition "The non-destructive, three-dimensional characterization of earth and planetary materials that uses material-penetrating energy sources. Tomography methods in Earth Science include experiments in controlled laboratory settings such as computed tomography of rock samples or soils, and field experiments such as seismic tomography of the Solid Earth."@en ;
    skos:historyNote "Definition adapted from Glossary of geology (5th edition revised; Neuendorf et al., 2011) and Wikipedia." ;
    skos:inScheme cs: ;
    skos:narrower
        :computed-tomography ,
        :seismic-tomography ;
    skos:prefLabel "tomography"@en ;
    schema:citation
        "https://en.wikipedia.org/wiki/Seismic_tomography"^^xsd:anyURI ,
        "https://en.wikipedia.org/wiki/Tomography"^^xsd:anyURI ,
        "https://glossary.americangeosciences.org/term/tomography"^^xsd:anyURI ;
.

:electrical-and-electromagnetic-methods-in-geophysics
    a skos:Concept ;
    rdfs:isDefinedBy cs: ;
    skos:broader :geophysics ;
    skos:definition "Geophysical methods that involve the use of electrical and electromagnetic fields to study the subsurface properties of the Earth. These methods exploit the interaction between electromagnetic waves and the electrical conductivity, permittivity, and magnetic susceptibility of subsurface materials."@en ;
    skos:exactMatch <https://linked.data.gov.au/def/earth-science-data-category/electrical-and-electromagnetic-methods-in-geophysics> ;
    skos:historyNote "Definition adapted from https://geologyscience.com/geology-branches/." ;
    skos:inScheme cs: ;
    skos:narrower
        :electrical-geophysics ,
        :electromagnetic-geophysics ,
        :magnetotellurics ;
    skos:notation "370602"^^<https://linked.data.gov.au/def/anzsrc-for/2020> ;
    skos:prefLabel "electrical and electromagnetic methods in geophysics"@en ;
    schema:citation "https://geologyscience.com/geology-branches/geophysics/electromagnetic-em-methods/"^^xsd:anyURI ;
.

:engineering
    a skos:Concept ;
    rdfs:isDefinedBy
        cs: ,
        <https://linked.data.gov.au/def/anzsrc-for/2020> ;
    skos:definition "The practice of using natural science, mathematics, and the (engineering) design process to solve technical problems, increase efficiency and productivity, and improve systems. More specifically, 'the creative application of scientific principles to design or develop structures, machines, apparatus, or manufacturing processes, or works utilizing them singly or in combination; or to construct or operate the same with full cognizance of their design; or to forecast their behaviour under specific operating conditions; all as respects an intended function, economics of operation and safety to life and property' (American Engineers' Council for Professional Development)."@en ;
    skos:exactMatch <https://linked.data.gov.au/def/anzsrc-for/2020/40> ;
    skos:historyNote "From the Fields of Research vocabulary from the Australian and New Zealand Standard Research Classification (ANZSRC, 2020). Definition adapted from Wikipedia." ;
    skos:inScheme cs: ;
    skos:narrower
        :environmental-engineering ,
        :geomatic-engineering ,
        :resources-engineering ;
    skos:notation "40"^^<https://linked.data.gov.au/def/anzsrc-for/2020> ;
    skos:prefLabel "engineering"@en ;
    skos:topConceptOf cs: ;
    schema:citation
        "https://en.wikipedia.org/wiki/American_Engineers%27_Council_for_Professional_Development"^^xsd:anyURI ,
        "https://en.wikipedia.org/wiki/Engineering"^^xsd:anyURI ;
.

:environmental-sciences
    a skos:Concept ;
    rdfs:isDefinedBy
        cs: ,
        <https://linked.data.gov.au/def/anzsrc-for/2020> ;
    skos:definition "An interdisciplinary academic field that integrates physical, biological and information sciences to the study of the environment, and the solution of environmental problems. It specifically addresses: (1) social and political decision making and policy setting relative to the environment or environmental ethics, (2) the planning and management of natural and human resources with an emphasis on the social and political aspects, and (3) legal and regulatory aspects of environmental protection activities carried out by the government under its powers."@en ;
    skos:exactMatch
        <https://linked.data.gov.au/def/anzsrc-for/2020/41> ,
        <https://linked.data.gov.au/def/earth-science-data-category/environmental-sciences> ;
    skos:historyNote "From the Fields of Research vocabulary from the Australian and New Zealand Standard Research Classification (ANZSRC, 2020). Definition adapted from Glossary of geology (5th edition revised; Neuendorf et al., 2011) and Wikipedia." ;
    skos:inScheme cs: ;
    skos:narrower
        :environmental-geochemistry ,
        :environmental-management ,
        :soil-sciences ;
    skos:notation "41"^^<https://linked.data.gov.au/def/anzsrc-for/2020> ;
    skos:prefLabel "environmental sciences"@en ;
    skos:topConceptOf cs: ;
    schema:citation
        "https://en.wikipedia.org/wiki/Environmental_science"^^xsd:anyURI ,
        "https://glossary.americangeosciences.org/term/environmentalscience"^^xsd:anyURI ;
.

:history-heritage-and-archeology
    a skos:Concept ;
    rdfs:isDefinedBy
        cs: ,
        <https://linked.data.gov.au/def/anzsrc-for/2020> ;
    skos:definition "Collectively, the study of practices, items and places designated as significant, including the investigation and interpretation of past human events (history), the identification, conservation and presentation of significant places, processes and items (heritage), and the study of human cultures through recovered artefacts or relics (archeology). Although history and archeology imply the interpretation of human culture, heritage and museum studies can be applied to concepts of both natural (abiotic or biotic) or cultural significance."@en ;
    skos:exactMatch <https://linked.data.gov.au/def/anzsrc-for/2020/43> ;
    skos:historyNote "From the Fields of Research vocabulary from the Australian and New Zealand Standard Research Classification (ANZSRC, 2020). Definition compiled by the Geological Survey of Western Australia." ;
    skos:inScheme cs: ;
    skos:narrower
        :archeology ,
        :geoheritage ,
        :heritage-archive-and-museum-studies ;
    skos:notation "43"^^<https://linked.data.gov.au/def/anzsrc-for/2020> ;
    skos:prefLabel "history, heritage and archeology"@en ;
    skos:topConceptOf cs: ;
.

:mineralogy-and-crystallography
    a skos:Concept ;
    rdfs:isDefinedBy
        cs: ,
        <https://linked.data.gov.au/def/anzsrc-for/2020> ;
    skos:broadMatch <https://linked.data.gov.au/def/earth-science-data-category/mineralogy-and-crystallography> ;
    skos:broader :geology ;
    skos:definition "The scientific study of the chemistry, crystal structure, and physical properties of minerals and mineralized artifacts."@en ;
    skos:exactMatch <https://linked.data.gov.au/def/anzsrc-for/2020/370505> ;
    skos:historyNote "From the Fields of Research vocabulary from the Australian and New Zealand Standard Research Classification (ANZSRC, 2020). Definition adapted from Wikipedia." ;
    skos:inScheme cs: ;
    skos:narrower
        :crystallography ,
        :gemmology ,
        :mineralogy ;
    skos:notation "370505"^^<https://linked.data.gov.au/def/anzsrc-for/2020> ;
    skos:prefLabel "mineralogy and crystallography"@en ;
    schema:citation
        "https://en.wikipedia.org/wiki/Crystallography"^^xsd:anyURI ,
        "https://en.wikipedia.org/wiki/Mineralogy"^^xsd:anyURI ;
.

:geoinformatics
    a skos:Concept ;
    rdfs:isDefinedBy
        cs: ,
        <https://linked.data.gov.au/def/anzsrc-for/2020> ;
    skos:broader :earth-sciences ;
    skos:definition "The application of modern information technology/computational systems to organize, preserve, and distribute geoscience data, and to facilitate and advance their analysis, i.e. the science and technology that develop and use data, software, and computing facilities in the cyberinfrastructure ecosystem to address the needs of geosciences and related branches of science and engineering."@en ;
    skos:exactMatch <https://linked.data.gov.au/def/anzsrc-for/2020/3704> ;
    skos:historyNote "From the Fields of Research vocabulary from the Australian and New Zealand Standard Research Classification (ANZSRC, 2020). Definition adapted from Glossary of geology (5th edition, revised; Neuendorf et al., 2011) and Wikipedia." ;
    skos:inScheme cs: ;
    skos:narrower
        :computational-modelling-and-simulation-in-earth-sciences ,
        :earth-and-space-science-informatics ,
        :geoinformatics-not-elsewhere-classified ,
        :geoscience-data-visualisation ;
    skos:notation "3704"^^<https://linked.data.gov.au/def/anzsrc-for/2020> ;
    skos:prefLabel "geoinformatics"@en ;
    schema:citation
        "https://en.wikipedia.org/wiki/Geoinformatics"^^xsd:anyURI ,
        "https://glossary.americangeosciences.org/term/geoinformatics"^^xsd:anyURI ;
.

:information-and-computing-sciences
    a skos:Concept ;
    rdfs:isDefinedBy
        cs: ,
        <https://linked.data.gov.au/def/anzsrc-for/2020> ;
    skos:altLabel "information and computer science"@en ;
    skos:definition "Information and computing (or computer) science (ICS) or computer and information science (CIS) (or sciences) is a field that emphasizes both computing and informatics, upholding the strong association between the fields of information sciences and computer sciences and treating computers as a tool rather than a field. Information science is primarily concerned with gathering, storing, disseminating, sharing and protecting any and all forms of information — it is a broad field, covering a myriad of different areas but is often referenced alongside computer science because of the incredibly useful nature of computers and computer programs in helping those studying and doing research in the field, particularly in helping to analyse data and in spotting patterns too broad for a human to intuitively perceive."@en ;
    skos:exactMatch
        <https://linked.data.gov.au/def/anzsrc-for/2020/46> ,
        <https://linked.data.gov.au/def/earth-science-data-category/information-and-computing-sciences> ;
    skos:historyNote "From the Fields of Research vocabulary from the Australian and New Zealand Standard Research Classification (ANZSRC, 2020). Definition adapted from Wikipedia." ;
    skos:inScheme cs: ;
    skos:narrower
        :artificial-intelligence ,
        :data-science-and-data-management ,
        :information-management ,
        :information-systems ;
    skos:notation
        "CIS"^^xsd:token ,
        "ICS"^^xsd:token ,
        "46"^^<https://linked.data.gov.au/def/anzsrc-for/2020> ;
    skos:prefLabel "information and computing sciences"@en ;
    skos:topConceptOf cs: ;
    schema:citation "https://en.wikipedia.org/wiki/Information_and_computer_science"^^xsd:anyURI ;
.

:resources-engineering
    a skos:Concept ;
    rdfs:isDefinedBy
        cs: ,
        <https://linked.data.gov.au/def/anzsrc-for/2020> ;
    skos:broadMatch <https://linked.data.gov.au/def/anzsrc-for/2020/4019> ;
    skos:broader :engineering ;
    skos:definition "Engineering that applies various branches of science in order to create new technology that aims to protect, maintain, extract, and establish sustainable natural resources."@en ;
    skos:exactMatch <https://linked.data.gov.au/def/earth-science-data-category/resources-engineering> ;
    skos:historyNote "From the Fields of Research vocabulary from the Australian and New Zealand Standard Research Classification (ANZSRC, 2020). Definition adapted from Wikipedia." ;
    skos:inScheme cs: ;
    skos:narrower
        :drilling-engineering ,
        :geomechanics-and-resources-geotechnical-engineering ,
        :geostorage-engineering ,
        :petroleum-and-reservoir-engineering ;
    skos:notation "4019"^^<https://linked.data.gov.au/def/anzsrc-for/2020> ;
    skos:prefLabel "resources engineering"@en ;
    schema:citation "https://en.wikipedia.org/wiki/Natural_resources_engineering"^^xsd:anyURI ;
.

:spectral-imaging
    a skos:Concept ;
    rdfs:isDefinedBy cs: ;
    skos:altLabel "spectroscopy"@en ;
    skos:broader :photogrammetry-and-remote-sensing ;
    skos:definition "The use of multiple bands across the electromagnetic spectrum to create a dataset that contains many images of the same object, where each one of them is measured at a different wavelength. It includes multispectral imaging that typically captures three to fifteen spectral bands, and hyperspectral imaging that combines spectroscopy and digital photography to capture hundreds of wavelength bands."@en ;
    skos:exactMatch <https://linked.data.gov.au/def/earth-science-data-category/spectral-imaging> ;
    skos:historyNote """Definition adapted from:
1) Glossary of geology (5th edition revised; Neuendorf et al., 2011)
2) Wikipedia
3) Garini, Y and Tauber, E 2013, Spectral Imaging: Methods, Design, and Applications, in Biomedical Optical Imaging Technologies, Biological and Medical Physics, Biomedical Engineering, edited by R Liang: Springer, Berlin, Heidelberg, doi.org/10.1007/978-3-642-28391-8_4.""" ;
    skos:inScheme cs: ;
    skos:narrower
        :airborne-spectral-imaging ,
        :core-spectral-imaging ,
        :ground-spectral-imaging ,
        :laboratory-spectral-imaging ,
        :satellite-spectral-imaging ;
    skos:prefLabel "spectral imaging"@en ;
    schema:citation
        "https://en.wikipedia.org/wiki/Spectral_imaging"^^xsd:anyURI ,
        "https://glossary.americangeosciences.org/term/spectroscopy"^^xsd:anyURI ,
        "https://link.springer.com/chapter/10.1007/978-3-642-28391-8_4"^^xsd:anyURI ;
.

:mineral-resource-geology
    a skos:Concept ;
    rdfs:isDefinedBy cs: ;
    skos:broader :resource-geoscience ;
    skos:definition "The study of concentrations of inorganic, naturally occurring, typically solid, typically non-renewable materials that are of intrinsic economic interest in or on the Earth's crust in such form, quality and quantity that there are reasonable prospects for eventual economic extraction. It includes the study of mineral systems, i.e. the combination of geological processes that are required to form and preserve an ore deposit. Also included is the characterization of orebodies (e.g. quantification of physical properties and chemical properties, and delineation of volumes, grades and geometry), and of limitations to the development and exploitation of mineral occurrences."@en ;
    skos:exactMatch <https://linked.data.gov.au/def/earth-science-data-category/mineral-resource-geology> ;
    skos:historyNote "Definition adapted from Wikipedia." ;
    skos:inScheme cs: ;
    skos:narrower
        :mineral-exploration-geology ,
        :mineral-system-analysis ,
        :mining-geology ,
        :ore-geology ,
        :prospecting ,
        :prospectivity-analysis ;
    skos:prefLabel "mineral resource geology"@en ;
    schema:citation
        "https://en.wikipedia.org/wiki/Mineral_resource_classification"^^xsd:anyURI ,
        "https://www.studysmarter.co.uk/explanations/environmental-science/physical-environment/mineral-resources/"^^xsd:anyURI ;
.

:mineralogy
    a skos:Concept ;
    rdfs:isDefinedBy cs: ;
    skos:broader :mineralogy-and-crystallography ;
    skos:definition "The scientific study of minerals, their formation, occurrence, physical and chemical properties, composition, and classification."@en ;
    skos:historyNote "Definition from Glossary of geology (5th edition revised; Neuendorf et al., 2011)." ;
    skos:inScheme cs: ;
    skos:narrower
        :applied-mineralogy ,
        :descriptive-mineralogy ,
        :experimental-mineralogy ,
        :genetic-mineralogy ,
        :quantitative-mineralogy ,
        :regional-mineralogy ;
    skos:prefLabel "mineralogy"@en ;
    schema:citation "https://glossary.americangeosciences.org/term/mineralogy"^^xsd:anyURI ;
.

:resource-geoscience
    a skos:Concept ;
    rdfs:isDefinedBy
        cs: ,
        <https://linked.data.gov.au/def/anzsrc-for/2020> ;
    skos:altLabel
        "economic geology"@en ,
        "resource geology"@en ;
    skos:broader :geology ;
    skos:definition "The study of fuels, metals and other materials of economic interest; it is concerned with the distribution, value and availability of resources, and the cost and benefits of their recovery."@en ;
    skos:exactMatch
        <https://linked.data.gov.au/def/anzsrc-for/2020/370508> ,
        <https://linked.data.gov.au/def/earth-science-data-category/resource-geology> ;
    skos:historyNote "From the Fields of Research vocabulary from the Australian and New Zealand Standard Research Classification (ANZSRC, 2020). Definition adapted from www.encyclopedia.com." ;
    skos:inScheme cs: ;
    skos:narrower
        :drilling ,
        :economic-analysis ,
        :energy-geoscience ,
        :logging ,
        :mineral-resource-geology ,
        :quarry-and-extractive-resource-geology ;
    skos:notation "370508"^^<https://linked.data.gov.au/def/anzsrc-for/2020> ;
    skos:prefLabel "resource geoscience"@en ;
    schema:citation "https://www.encyclopedia.com/science/news-wires-white-papers-and-books/economic-geology"^^xsd:anyURI ;
.

:earth-sciences
    a skos:Concept ;
    rdfs:isDefinedBy
        cs: ,
        <https://linked.data.gov.au/def/anzsrc-for/2020> ;
    skos:altLabel "geosciences"@en ;
    skos:definition "An all-embracing term for all fields of natural sciences related to the planet Earth. It is occasionally used as a synonym for geology or geological sciences, but this usage is misleading because in its wider scope earth science may be considered to include such subjects as meteorology, physical oceanography, soil chemistry, and agronomy."@en ;
    skos:exactMatch
        <https://linked.data.gov.au/def/anzsrc-for/2020/37> ,
        <https://linked.data.gov.au/def/earth-science-data-category/earth-sciences> ;
    skos:historyNote "From the Fields of Research vocabulary from the Australian and New Zealand Standard Research Classification (ANZSRC, 2020). Definition adapted from Glossary of geology (5th edition, revised; Neuendorf et al., 2011)." ;
    skos:inScheme cs: ;
    skos:narrower
        :atmospheric-sciences ,
        :geochemistry ,
        :geoethics ,
        :geoinformatics ,
        :geology ,
        :geophysics ,
        :physical-geography-and-environmental-geoscience ;
    skos:notation "37"^^<https://linked.data.gov.au/def/anzsrc-for/2020> ;
    skos:prefLabel "earth sciences"@en ;
    skos:topConceptOf cs: ;
    schema:citation "https://glossary.americangeosciences.org/term/earthscience"^^xsd:anyURI ;
.

:energy-geoscience
    a skos:Concept ;
    rdfs:isDefinedBy cs: ;
    skos:broader :resource-geoscience ;
    skos:definition "A branch of geology that focuses on the study of conventional, non-conventional and renewable natural resources used for energy production, i.e. including fossil fuels (like coal, oil, and natural gas), renewable energy resources (like wind, solar, and geothermal), and nuclear resources. This field involves understanding the formation, distribution, extraction, and environmental impacts of these energy resource."@en ;
    skos:historyNote "Definition adapted from https://www.sciencedirect.com/journal/energy-geoscience." ;
    skos:inScheme cs: ;
    skos:narrower
        :coal-geology ,
        :energy-exploration ,
        :geothermal-resource-geology ,
        :petroleum-geology ,
        :renewable-energy-geoscience ,
        :reservoir-analysis ,
        :seal-analysis ;
    skos:prefLabel "energy geoscience"@en ;
    schema:citation "https://www.sciencedirect.com/journal/energy-geoscience"^^xsd:anyURI ;
.

:stratigraphy
    a skos:Concept ;
    rdfs:isDefinedBy
        cs: ,
        <https://linked.data.gov.au/def/anzsrc-for/2020> ;
    skos:broader :geology ;
    skos:definition "The study of the history, composition, relative ages and distribution of strata, and the interpretation of strata to elucidate Earth's history. The comparison, or correlation, of separated strata can include study of their form, distribution, lithology, fossil content, geophysical and geochemical properties, relative or numerical/absolute age, and their interpretation in terms of environment or mode of origin, and geological history."@en ;
    skos:exactMatch
        <https://linked.data.gov.au/def/anzsrc-for/2020/370510> ,
        <https://linked.data.gov.au/def/earth-science-data-category/stratigraphy> ;
    skos:historyNote "From the Fields of Research vocabulary from the Australian and New Zealand Standard Research Classification (ANZSRC, 2020). Definition adapted from Schlumberger Oilfield Glossary and Glossary of geology (5th edition revised; Neuendorf, 2011)." ;
    skos:inScheme cs: ;
    skos:narrower
        :biostratigraphy ,
        :chemostratigraphy ,
        :chronostratigraphy ,
        :lithostratigraphy ,
        :magnetostratigraphy ,
        :seismic-stratigraphy ,
        :sequence-stratigraphy ;
    skos:notation "370510"^^<https://linked.data.gov.au/def/anzsrc-for/2020> ;
    skos:prefLabel "stratigraphy"@en ;
    schema:citation
        "https://glossary.americangeosciences.org/term/stratigraphy"^^xsd:anyURI ,
        "https://glossary.slb.com/en/terms/s/stratigraphy"^^xsd:anyURI ;
.

:geochronology
    a skos:Concept ;
    rdfs:isDefinedBy
        cs: ,
        <https://linked.data.gov.au/def/anzsrc-for/2020> ;
    skos:broader :geology ;
    skos:definition "The science of dating and determining the time sequence of events in the history of the Earth, i.e. the study of the relative or numerical/absolute age of rocks, minerals and fossils. Numerical age is the measurement of age in years ('numerical' is preferred to 'absolute' ages, as the latter typically have some amount of error and are inexact) whereas relative age, in contrast, is the approximate age of rocks, fossils or minerals made by determining the age of the material relative to the age of and relationships with other surrounding material."@en ;
    skos:exactMatch
        <https://linked.data.gov.au/def/anzsrc-for/2020/370502> ,
        <https://linked.data.gov.au/def/earth-science-data-category/geochronology> ;
    skos:historyNote "From the Fields of Research vocabulary from the Australian and New Zealand Standard Research Classification (ANZSRC, 2020). Definition adapted from Glossary of geology (5th edition revised; Neuendorf et. al., 2011) and Schlumberger Oilfield Glossary." ;
    skos:inScheme cs: ;
    skos:narrower
        :biostratigraphic-age-determination ,
        :dendrochronology ,
        :isotope-age-determination ,
        :paleomagnetic-age-determination ,
        :radiogenic-age-determination ,
        :tephrochronology ,
        :thermochronology ,
        :varve-chronology ;
    skos:notation "370502"^^<https://linked.data.gov.au/def/anzsrc-for/2020> ;
    skos:prefLabel "geochronology"@en ;
    schema:citation
        "https://glossary.americangeosciences.org/term/geochronology"^^xsd:anyURI ,
        "https://glossary.slb.com/terms/g/geochronology"^^xsd:anyURI ;
.

:geomatic-engineering
    a skos:Concept ;
    rdfs:isDefinedBy
        cs: ,
        <https://linked.data.gov.au/def/anzsrc-for/2020> ;
    skos:altLabel "surveying engineering"@en ;
    skos:broader :engineering ;
    skos:definition "A professional engineering discipline that focuses on spatial information (i.e. information that has a location) to design, develop, and operate systems for collecting and analysing spatial information about the land, the oceans, natural resources, and man-made features."@en ;
    skos:exactMatch
        <https://linked.data.gov.au/def/anzsrc-for/2020/4013> ,
        <https://linked.data.gov.au/def/earth-science-data-category/geomatic-engineering> ;
    skos:historyNote "From the Fields of Research vocabulary from the Australian and New Zealand Standard Research Classification (ANZSRC, 2020). Definition adapted from Wikipedia." ;
    skos:inScheme cs: ;
    skos:narrower
        :cartography-and-digital-mapping ,
        :geographic-information-science ,
        :geomatic-engineering-not-elsewhere-classified ,
        :geomatics ,
        :geospatial-information-systems-and-geospatial-data-modelling ,
        :photogrammetry-and-remote-sensing ,
        :satellite-based-positioning ,
        :surveying ;
    skos:notation "4013"^^<https://linked.data.gov.au/def/anzsrc-for/2020> ;
    skos:prefLabel "geomatic engineering"@en ;
    schema:citation "https://en.wikipedia.org/wiki/Geomatics"^^xsd:anyURI ;
.

:petrology
    a skos:Concept ;
    rdfs:isDefinedBy
        cs: ,
        <https://linked.data.gov.au/def/anzsrc-for/2020> ;
    skos:broadMatch <https://linked.data.gov.au/def/anzsrc-for/2020/370503> ;
    skos:broader :geology ;
    skos:definition "That branch of geology dealing with the origin, occurrence, structure, and history of rocks, including the conditions under which they form. Petrology is broader in scope than petrography."@en ;
    skos:exactMatch <https://linked.data.gov.au/def/earth-science-data-category/petrology> ;
    skos:historyNote "From the Fields of Research vocabulary from the Australian and New Zealand Standard Research Classification (ANZSRC, 2020). Definition adapted from Glossary of geology (5th edition revised; Neuendorf et al., 2011)." ;
    skos:inScheme cs: ;
    skos:narrower
        :experimental-petrology ,
        :fluid-inclusion-petrology ,
        :igneous-petrology ,
        :metamorphic-petrology ,
        :ore-petrology ,
        :organic-petrology ,
        :petrography ,
        :sedimentary-petrology ;
    skos:notation "370503"^^<https://linked.data.gov.au/def/anzsrc-for/2020> ;
    skos:prefLabel "petrology"@en ;
    schema:citation "https://glossary.americangeosciences.org/term/petrology"^^xsd:anyURI ;
.

:heritage-archive-and-museum-studies
    a skos:Concept ;
    rdfs:isDefinedBy
        cs: ,
        <https://linked.data.gov.au/def/anzsrc-for/2020> ;
    skos:broader :history-heritage-and-archeology ;
    skos:definition "Studies related to the identification, collection, curation, conservation, interpretation, use and management of cultural and natural heritage, by examining the variety of locations through which this happens such as objects and collections, museums, heritage places, intangible cultural heritage, and international heritage practice."@en ;
    skos:exactMatch <https://linked.data.gov.au/def/anzsrc-for/2020/4302> ;
    skos:historyNote "From the Fields of Research vocabulary from the Australian and New Zealand Standard Research Classification (ANZSRC, 2020). Definition compiled by Geological Survey of Western Australia from multiple sources." ;
    skos:inScheme cs: ;
    skos:narrower
        :archival-repository-and-related-studies ,
        :collection-management ,
        :digital-heritage ,
        :heritage-and-conservation ,
        :heritage-archive-and-museum-studies-not-elsewhere-classified ,
        :heritage-collections-and-interpretations ,
        :heritage-tourism-visitor-and-audience-studies ,
        :intangible-heritage ,
        :materials-conservation ;
    skos:notation "4302"^^<https://linked.data.gov.au/def/anzsrc-for/2020> ;
    skos:prefLabel "heritage, archive and museum studies"@en ;
    schema:citation
        "https://en.wikipedia.org/wiki/Archival_science"^^xsd:anyURI ,
        "https://en.wikipedia.org/wiki/Heritage_studies"^^xsd:anyURI ,
        "https://en.wikipedia.org/wiki/Museology"^^xsd:anyURI ,
        "https://www.deakin.edu.au/courses/unit?unit=AIM719"^^xsd:anyURI ;
.

:physical-geography-and-environmental-geoscience
    a skos:Concept ;
    rdfs:isDefinedBy
        cs: ,
        <https://linked.data.gov.au/def/anzsrc-for/2020> ;
    skos:broader :earth-sciences ;
    skos:definition "The branch of natural science which deals with the classification, form, processes, extent and patterns of natural phenomena in the natural environment such as the atmosphere, hydrosphere, biosphere, and geosphere. It differs chiefly from geology in that it considers conditions of the Earth primarily over shorter time scales (e.g. Quaternary and/or modern rates). It is more inclusive than geomorphology, dealing not only with landforms but also climate, oceans, atmosphere, soils, geologic processes, natural resources, and the biogeographical distribution of animal and plant life."@en ;
    skos:exactMatch <https://linked.data.gov.au/def/anzsrc-for/2020/3709> ;
    skos:historyNote "From the Fields of Research vocabulary from the Australian and New Zealand Standard Research Classification (ANZSRC, 2020). Definition adapted from Glossary of geology (5th edition revised; Neuendorf et al., 2011) and Wikipedia." ;
    skos:inScheme cs: ;
    skos:narrowMatch <https://linked.data.gov.au/def/earth-science-data-category/physical-geography> ;
    skos:narrower
        :geomorphology-and-earth-surface-processes ,
        :glaciology ,
        :hydrogeology ,
        :natural-hazards ,
        :paleoclimatology ,
        :physical-geography-and-environmental-geoscience-not-elsewhere-classified ,
        :quaternary-environments ,
        :regolith-and-landscape-evolution ,
        :surface-processes ,
        :surface-water-hydrology ;
    skos:notation "3709"^^<https://linked.data.gov.au/def/anzsrc-for/2020> ;
    skos:prefLabel "physical geography and environmental geoscience"@en ;
    schema:citation
        "https://en.wikipedia.org/wiki/Physical_geography"^^xsd:anyURI ,
        "https://glossary.americangeosciences.org/term/physicalgeography"^^xsd:anyURI ;
.

:geochemistry
    a skos:Concept ;
    rdfs:isDefinedBy
        cs: ,
        <https://linked.data.gov.au/def/anzsrc-for/2020> ;
    skos:broader :earth-sciences ;
    skos:definition "The study of the distribution and amounts of the chemical elements in minerals, ores, rocks, soils, water, the atmosphere on Earth and within solid bodies of the solar system, including the distribution, circulation and abundance of elements (and their ions and isotopes), molecules, minerals, rocks and fluids."@en ;
    skos:exactMatch
        <https://linked.data.gov.au/def/anzsrc-for/2020/3703> ,
        <https://linked.data.gov.au/def/earth-science-data-category/geochemistry> ;
    skos:historyNote "From the Fields of Research vocabulary from the Australian and New Zealand Standard Research Classification (ANZSRC, 2020). Definition adapted from Glossary of geology (5th edition, revised; Neuendorf et al., 2011)." ;
    skos:inScheme cs: ;
    skos:narrower
        :biogeochemistry ,
        :exploration-geochemistry ,
        :fluid-extract-geochemistry ,
        :fluid-inclusion-geochemistry ,
        :geochemistry-not-elsewhere-classified ,
        :hydrogeochemistry ,
        :inorganic-geochemistry ,
        :isotope-geochemistry ,
        :lithogeochemistry ,
        :mineral-chemistry ,
        :organic-geochemistry ,
        :regolith-chemistry ;
    skos:notation "3703"^^<https://linked.data.gov.au/def/anzsrc-for/2020> ;
    skos:prefLabel "geochemistry"@en ;
    schema:citation
        "https://glossary.americangeosciences.org/term/geochemistry"^^xsd:anyURI ,
        "https://glossary.slb.com/en/terms/g/geochemistry"^^xsd:anyURI ;
.

:geophysics
    a skos:Concept ;
    rdfs:isDefinedBy
        cs: ,
        <https://linked.data.gov.au/def/anzsrc-for/2020> ;
    skos:broader :earth-sciences ;
    skos:definition "A natural science concerned with the physical processes and physical properties of the Earth and its surrounding space environment, and the use of quantitative methods for their analysis. It includes several disciplines focusing on the study of the Earth's electrical, gravitational and magnetic fields and the propagation of elastic (seismic) waves within it."@en ;
    skos:exactMatch
        <https://linked.data.gov.au/def/anzsrc-for/2020/3706> ,
        <https://linked.data.gov.au/def/earth-science-data-category/geophysics> ;
    skos:historyNote "From the Fields of Research vocabulary from the Australian and New Zealand Standard Research Classification (ANZSRC, 2020). Definition adapted from Glossary of geology (5th edition revised; Neuendorf et al., 2011) and Wikipedia." ;
    skos:inScheme cs: ;
    skos:narrower
        :applied-geophysics ,
        :electrical-and-electromagnetic-methods-in-geophysics ,
        :geodesy ,
        :geodynamics ,
        :geophysical-fluid-dynamics ,
        :geophysics-not-elsewhere-classified ,
        :geothermics-and-radiometrics ,
        :gravimetrics ,
        :magnetism-and-paleomagnetism ,
        :petrophysics-and-rock-mechanics ,
        :seismology-and-seismic-exploration ,
        :tomography ;
    skos:notation "3706"^^<https://linked.data.gov.au/def/anzsrc-for/2020> ;
    skos:prefLabel "geophysics"@en ;
    schema:citation
        "https://en.wikipedia.org/wiki/Geophysics"^^xsd:anyURI ,
        "https://glossary.americangeosciences.org/term/geophysics"^^xsd:anyURI ,
        "https://glossary.slb.com/en/terms/g/geophysics"^^xsd:anyURI ;
.

:paleontology
    a skos:Concept ;
    rdfs:isDefinedBy
        cs: ,
        <https://linked.data.gov.au/def/anzsrc-for/2020> ;
    skos:altLabel
        "palaeobiology"@en ,
        "palaeontology"@en ,
        "paleobiology"@en ;
    skos:broader :geology ;
    skos:definition "The scientific study of life in the geological past through the analysis of fossils, including those of microscopic size, and of traces representing preserved behaviour, preserved in rocks. It is concerned with all aspects of the biology of ancient life forms: their shape and structure, evolutionary patterns, taxonomic relationships with each other and with modern living species, geographic distribution, and interrelationships with the environment."@en ;
    skos:exactMatch
        <https://linked.data.gov.au/def/anzsrc-for/2020/370506> ,
        <https://linked.data.gov.au/def/earth-science-data-category/paleontology> ;
    skos:historyNote "From the Fields of Research vocabulary from the Australian and New Zealand Standard Research Classification (ANZSRC, 2020). Definition adapted from https://www.britannica.com/science/paleontology." ;
    skos:inScheme cs: ;
    skos:narrower
        :biostratigraphy ,
        :evolutionary-paleontology ,
        :ichnology ,
        :invertebrate-paleontology ,
        :microbial-paleobiology ,
        :micropaleontology ,
        :molecular-paleontology ,
        :morphological-paleontology ,
        :paleobiogeography ,
        :paleobotany ,
        :paleoecology ,
        :taphonomy ,
        :vertebrate-paleontology ;
    skos:notation "370506"^^<https://linked.data.gov.au/def/anzsrc-for/2020> ;
    skos:prefLabel "paleontology"@en ;
    schema:citation
        "https://glossary.americangeosciences.org/term/paleontology"^^xsd:anyURI ,
        "https://www.britannica.com/science/paleontology"^^xsd:anyURI ;
.

:geology
    a skos:Concept ;
    rdfs:isDefinedBy
        cs: ,
        <https://linked.data.gov.au/def/anzsrc-for/2020> ;
    skos:broader :earth-sciences ;
    skos:definition "An Earth science concerned with the planet Earth and the rocks/materials of which it is made, the processes that act on these materials and by which these change over time, the products formed, to understand the history of the planet and its life forms since its origin, and including the study of physical forces that act on the Earth, the chemistry of its constituent materials, and the biology of its past inhabitants as revealed by fossils. Geology can also include the study of the solid features of any terrestrial planet or natural satellite such as Mars or the Moon. Modern geology significantly overlaps all other earth sciences, including hydrology and the atmospheric sciences, and so is treated as one major aspect of integrated Earth system science and planetary science."@en ;
    skos:exactMatch
        <https://linked.data.gov.au/def/anzsrc-for/2020/3705> ,
        <https://linked.data.gov.au/def/earth-science-data-category/geology> ;
    skos:historyNote "From the Fields of Research vocabulary from the Australian and New Zealand Standard Research Classification (ANZSRC, 2020). Definition adapted from Glossary of geology (Neuendorf et. al., 2011, 5th edition revised) and Wikipedia." ;
    skos:inScheme cs: ;
    skos:narrower
        :basement-geology ,
        :basin-analysis ,
        :carbon-geostorage-geology ,
        :engineering-geology ,
        :environmental-geology ,
        :extraterrestrial-geology ,
        :forensic-geology ,
        :geobiology ,
        :geochronology ,
        :geohazard ,
        :geological-mapping ,
        :geology-not-elsewhere-classified ,
        :geomathematics ,
        :geotechnical-engineering ,
        :historical-geology ,
        :history-of-geology ,
        :local-geology ,
        :marine-geoscience ,
        :medical-geology ,
        :military-geology ,
        :mineralogy-and-crystallography ,
        :paleontology ,
        :petrology ,
        :regional-geology ,
        :resource-geoscience ,
        :sedimentology ,
        :speleology ,
        :stratigraphy ,
        :structural-geology-and-tectonics ,
        :volcanology ;
    skos:notation "3705"^^<https://linked.data.gov.au/def/anzsrc-for/2020> ;
    skos:prefLabel "geology"@en ;
    schema:citation
        "https://en.wikipedia.org/wiki/Geology"^^xsd:anyURI ,
        "https://glossary.americangeosciences.org/term/geology"^^xsd:anyURI ;
.

:1.0 schema:name "1.0" .

cs:
    a skos:ConceptScheme ;
    owl:versionIRI :1.0 ;
    skos:definition "A categorization of disciplines or topics that the broad field of Earth science can be subdivided into, i.e. a listing of the Fields of Research, or subjects, to which a geoscience dataset, publication, observation/activity, or entity pertains. The vocabulary also contains relevant disciplines that intersect with the various Earth science fields, such as biological sciences and built environment and design, as well as entries related to collection and heritage management. Notations included are those from the 2020 ANZSRC listing (see History Note) or in common use in the geoscience community. "@en ;
    skos:hasTopConcept
        :biological-sciences ,
        :built-environment-and-design ,
        :earth-sciences ,
        :earth-system-science ,
        :engineering ,
        :environmental-sciences ,
        :heritage-archive-and-museum-studies-not-elsewhere-classified ,
        :history-heritage-and-archeology ,
        :human-society ,
        :information-and-computing-sciences ,
        :physical-sciences ,
        :stakeholder-engagement ;
    skos:historyNote "The listing combines Earth Science-related entries in the Fields of Research vocabulary from the 2020 Australian and New Zealand Standard Research Classification (ANZSRC, https://vocabs.ardc.edu.au/viewById/316 and https://www.abs.gov.au/statistics/classifications/australian-and-new-zealand-standard-research-classification-anzsrc/latest-release), selected additions from the Geological Survey of Queensland (GSQ)'s Earth Science Data Category vocabulary (https://linked.data.gov.au/def/earth-science-data-category), and supplementary concepts of relevance to the work of the Geological Survey of Western Australia (GSWA) and partner industry and research institutions. Definitions used are largely derived from: (a) the Glossary of Geology (Neuendorf, KKE, Mehl Jr, JP and Jackson, JA (editors) 2011, Glossary of geology (5th edition, revised): American Geosciences Institute, Alexandria, Virginia, USA, 800p.), (b) Wikipedia (https://www.wikipedia.org/), (c) the GSQ's earth Science Data Category vocabulary (https://linked.data.gov.au/def/earth-science-data-category), and many other online resources."@en ;
    skos:prefLabel "Earth science fields of research"@en ;
    prov:qualifiedAttribution
        [
            dcat:hadRole isoroles:custodian ;
            prov:agent <https://orcid.org/0000-0002-7645-5031> ;
        ] ,
        [
            dcat:hadRole isoroles:custodian ;
            prov:agent
                [
                    a schema:Person ;
                    schema:email ""^^xsd:anyURI ;
                    schema:name "Erin Gray" ;
                ] ;
        ] ;
    schema:creator <https://linked.data.gov.au/org/gswa> ;
    schema:dateCreated "2023-05-15"^^xsd:date ;
    schema:dateModified "2024-10-23"^^xsd:date ;
    schema:keywords <https://linked.data.gov.au/def/gswa-vocabulary-themes/geology-framework> ;
    schema:publisher <https://linked.data.gov.au/org/gswa> ;
    schema:version "1.0" ;
    reg:status agldwgstatus:stable ;
.

<https://linked.data.gov.au/def/earth-science-data-category> schema:name "Earth Science Data Category Vocabulary" .
<https://linked.data.gov.au/def/earth-science-data-category/airborne-spectral> schema:name "airborne spectral" .
<https://linked.data.gov.au/def/earth-science-data-category/atmospheric-sciences> schema:name "atmospheric sciences" .
<https://linked.data.gov.au/def/earth-science-data-category/basement-geology> schema:name "basement geology" .
<https://linked.data.gov.au/def/earth-science-data-category/basin-analysis> schema:name "basin analysis" .
<https://linked.data.gov.au/def/earth-science-data-category/biogeochemistry> schema:name "biogeochemistry" .
<https://linked.data.gov.au/def/earth-science-data-category/biogeology> schema:name "biogeology" .
<https://linked.data.gov.au/def/earth-science-data-category/biological-sciences> schema:name "biological sciences" .
<https://linked.data.gov.au/def/earth-science-data-category/built-environment-and-design> schema:name "built environment and design" .
<https://linked.data.gov.au/def/earth-science-data-category/carbon-geostorage-geology> schema:name "carbon geostorage geology" .
<https://linked.data.gov.au/def/earth-science-data-category/coal-geology> schema:name "coal geology" .
<https://linked.data.gov.au/def/earth-science-data-category/conventional-reservoir-geology> schema:name "conventional reservoir geology" .
<https://linked.data.gov.au/def/earth-science-data-category/core-spectral> schema:name "core spectral" .
<https://linked.data.gov.au/def/earth-science-data-category/drilling-engineering> schema:name "drilling engineering" .
<https://linked.data.gov.au/def/earth-science-data-category/earth-sciences> schema:name "earth sciences" .
<https://linked.data.gov.au/def/earth-science-data-category/ecology> schema:name "ecology" .
<https://linked.data.gov.au/def/earth-science-data-category/electrical-and-electromagnetic-methods-in-geophysics> schema:name "electrical and electromagnetic methods in geophysics" .
<https://linked.data.gov.au/def/earth-science-data-category/electrical-geophysics> schema:name "electrical geophysics" .
<https://linked.data.gov.au/def/earth-science-data-category/electromagnetic-geophysics> schema:name "electromagnetic geophysics" .
<https://linked.data.gov.au/def/earth-science-data-category/environmental-engineering> schema:name "environmental engineering" .
<https://linked.data.gov.au/def/earth-science-data-category/environmental-sciences> schema:name "environmental sciences" .
<https://linked.data.gov.au/def/earth-science-data-category/extraterrestrial-geology> schema:name "extraterrestrial geology" .
<https://linked.data.gov.au/def/earth-science-data-category/fluid-extract-geochemistry> schema:name "fluid extract geochemistry" .
<https://linked.data.gov.au/def/earth-science-data-category/gemmology> schema:name "gemmology" .
<https://linked.data.gov.au/def/earth-science-data-category/geochemistry> schema:name "geochemistry" .
<https://linked.data.gov.au/def/earth-science-data-category/geochemistry-not-elsewhere-classified> schema:name "geochemistry not elsewhere classified" .
<https://linked.data.gov.au/def/earth-science-data-category/geochronology> schema:name "geochronology" .
<https://linked.data.gov.au/def/earth-science-data-category/geodynamics> schema:name "geodynamics" .
<https://linked.data.gov.au/def/earth-science-data-category/geology> schema:name "geology" .
<https://linked.data.gov.au/def/earth-science-data-category/geology-not-elsewhere-classified> schema:name "geology not elsewhere classified" .
<https://linked.data.gov.au/def/earth-science-data-category/geomatic-engineering> schema:name "geomatic engineering" .
<https://linked.data.gov.au/def/earth-science-data-category/geomechanics-and-resources-geotechnical-engineering> schema:name "geomechanics and resources geotechnical engineering" .
<https://linked.data.gov.au/def/earth-science-data-category/geomorphology-and-regolith-and-landscape-evolution> schema:name "geomorphology and regolith and landscape evolution" .
<https://linked.data.gov.au/def/earth-science-data-category/geophysical-fluid-dynamics> schema:name "geophysical fluid dynamics" .
<https://linked.data.gov.au/def/earth-science-data-category/geophysics> schema:name "geophysics" .
<https://linked.data.gov.au/def/earth-science-data-category/geophysics-not-elsewhere-classified> schema:name "geophysics not elsewhere classified" .
<https://linked.data.gov.au/def/earth-science-data-category/geostorage-engineering> schema:name "geostorage engineering" .
<https://linked.data.gov.au/def/earth-science-data-category/geothermal-resource-geology> schema:name "geothermal resource geology" .
<https://linked.data.gov.au/def/earth-science-data-category/geothermics-and-radiometrics> schema:name "geothermics and radiometrics" .
<https://linked.data.gov.au/def/earth-science-data-category/glaciology> schema:name "glaciology" .
<https://linked.data.gov.au/def/earth-science-data-category/gravity> schema:name "gravity" .
<https://linked.data.gov.au/def/earth-science-data-category/gravity-gradiometry> schema:name "gravity gradiometry" .
<https://linked.data.gov.au/def/earth-science-data-category/historical-geology> schema:name "historical geology" .
<https://linked.data.gov.au/def/earth-science-data-category/history-of-geology> schema:name "history of geology" .
<https://linked.data.gov.au/def/earth-science-data-category/hydrogeochemistry> schema:name "hydrogeochemistry" .
<https://linked.data.gov.au/def/earth-science-data-category/hydrogeology> schema:name "hydrogeology" .
<https://linked.data.gov.au/def/earth-science-data-category/ichnology> schema:name "ichnology" .
<https://linked.data.gov.au/def/earth-science-data-category/igneous-and-metamorphic-petrology> schema:name "igneous and metamorphic petrology" .
<https://linked.data.gov.au/def/earth-science-data-category/information-and-computing-sciences> schema:name "information and computing sciences" .
<https://linked.data.gov.au/def/earth-science-data-category/inorganic-geochemistry> schema:name "inorganic geochemistry" .
<https://linked.data.gov.au/def/earth-science-data-category/invertebrate-paleontology> schema:name "invertebrate paleontology" .
<https://linked.data.gov.au/def/earth-science-data-category/isotope-geochemistry> schema:name "isotope geochemistry" .
<https://linked.data.gov.au/def/earth-science-data-category/land-use-and-environmental-planning> schema:name "land use and environmental planning" .
<https://linked.data.gov.au/def/earth-science-data-category/local-geology> schema:name "local geology" .
<https://linked.data.gov.au/def/earth-science-data-category/magnetics> schema:name "magnetics" .
<https://linked.data.gov.au/def/earth-science-data-category/magnetotellurics> schema:name "magnetotellurics" .
<https://linked.data.gov.au/def/earth-science-data-category/marine-geoscience> schema:name "marine geoscience" .
<https://linked.data.gov.au/def/earth-science-data-category/micropaleontology> schema:name "micropaleontology" .
<https://linked.data.gov.au/def/earth-science-data-category/mineral-resource-geology> schema:name "mineral resource geology" .
<https://linked.data.gov.au/def/earth-science-data-category/mineralogy-and-crystallography> schema:name "mineralogy and crystallography" .
<https://linked.data.gov.au/def/earth-science-data-category/natural-hazards> schema:name "natural hazards" .
<https://linked.data.gov.au/def/earth-science-data-category/organic-geochemistry> schema:name "organic geochemistry" .
<https://linked.data.gov.au/def/earth-science-data-category/organic-petrology> schema:name "organic petrology" .
<https://linked.data.gov.au/def/earth-science-data-category/paleobotany> schema:name "paleobotany" .
<https://linked.data.gov.au/def/earth-science-data-category/paleoclimatology> schema:name "paleoclimatology" .
<https://linked.data.gov.au/def/earth-science-data-category/paleontology> schema:name "paleontology" .
<https://linked.data.gov.au/def/earth-science-data-category/palynology> schema:name "palynology" .
<https://linked.data.gov.au/def/earth-science-data-category/passive-seismic> schema:name "passive seismic" .
<https://linked.data.gov.au/def/earth-science-data-category/petroleum-and-coal-geology> schema:name "petroleum and coal geology" .
<https://linked.data.gov.au/def/earth-science-data-category/petroleum-geology> schema:name "petroleum geology" .
<https://linked.data.gov.au/def/earth-science-data-category/petrology> schema:name "petrology" .
<https://linked.data.gov.au/def/earth-science-data-category/petrophysics> schema:name "petrophysics" .
<https://linked.data.gov.au/def/earth-science-data-category/physical-geography> schema:name "physical geography" .
<https://linked.data.gov.au/def/earth-science-data-category/physical-geography-and-environmental-geoscience-not-elsewhere-classified> schema:name "physical geography and environmental geoscience not elsewhere classified" .
<https://linked.data.gov.au/def/earth-science-data-category/quarry-resource-geology> schema:name "quarry resource geology" .
<https://linked.data.gov.au/def/earth-science-data-category/quaternary-environments> schema:name "quaternary environments" .
<https://linked.data.gov.au/def/earth-science-data-category/regional-geology> schema:name "regional geology" .
<https://linked.data.gov.au/def/earth-science-data-category/remote-sensing> schema:name "remote sensing" .
<https://linked.data.gov.au/def/earth-science-data-category/reservoir-engineering> schema:name "reservoir engineering" .
<https://linked.data.gov.au/def/earth-science-data-category/resource-geology> schema:name "resource geology" .
<https://linked.data.gov.au/def/earth-science-data-category/resources-engineering> schema:name "resources engineering" .
<https://linked.data.gov.au/def/earth-science-data-category/satellite-spectral> schema:name "satellite spectral" .
<https://linked.data.gov.au/def/earth-science-data-category/sedimentary-petrology> schema:name "sedimentary petrology" .
<https://linked.data.gov.au/def/earth-science-data-category/sedimentology> schema:name "sedimentology" .
<https://linked.data.gov.au/def/earth-science-data-category/seismic-surveys> schema:name "seismic surveys" .
<https://linked.data.gov.au/def/earth-science-data-category/seismology-and-seismic-exploration> schema:name "seismology and seismic exploration" .
<https://linked.data.gov.au/def/earth-science-data-category/spectral-imaging> schema:name "spectral imaging" .
<https://linked.data.gov.au/def/earth-science-data-category/stratigraphy> schema:name "stratigraphy" .
<https://linked.data.gov.au/def/earth-science-data-category/structural-geology> schema:name "structural geology" .
<https://linked.data.gov.au/def/earth-science-data-category/surface-geology> schema:name "surface geology" .
<https://linked.data.gov.au/def/earth-science-data-category/surfacewater-hydrology> schema:name "surfacewater hydrology" .
<https://linked.data.gov.au/def/earth-science-data-category/surveying> schema:name "surveying" .
<https://linked.data.gov.au/def/earth-science-data-category/unconventional-reservoir-geology> schema:name "unconventional reservoir geology" .
<https://linked.data.gov.au/def/earth-science-data-category/urban-and-regional-planning> schema:name "urban and regional planning" .
<https://linked.data.gov.au/def/earth-science-data-category/volcanology> schema:name "volcanology" .

<https://linked.data.gov.au/def/anzsrc-for/2020>
    schema:name "1297.0 ANZSRC - Australian and New Zealand Standard Research Classification, 2020: Fields of Research (FoR)"@en ;
.

<https://linked.data.gov.au/def/anzsrc-for/2020/31>
    schema:description "This division covers biological sciences."@en ;
    schema:name "BIOLOGICAL SCIENCES"@en ;
.

<https://linked.data.gov.au/def/anzsrc-for/2020/3103>
    schema:description "This group covers ecology other than its environmental applications."@en ;
    schema:name "Ecology"@en ;
.

<https://linked.data.gov.au/def/anzsrc-for/2020/33>
    schema:description """This division covers built environment and design.
It includes:
• architecture;
• building;
• design; and
• urban and regional planning."""@en ;
    schema:name "BUILT ENVIRONMENT AND DESIGN"@en ;
.

<https://linked.data.gov.au/def/anzsrc-for/2020/3304>
    schema:description "This group covers urban and regional planning."@en ;
    schema:name "Urban and regional planning"@en ;
.

<https://linked.data.gov.au/def/anzsrc-for/2020/330404>
    schema:name "Land use and environmental planning"@en ;
.

<https://linked.data.gov.au/def/anzsrc-for/2020/37>
    schema:description "This division covers the earth sciences."@en ;
    schema:name "EARTH SCIENCES"@en ;
.

<https://linked.data.gov.au/def/anzsrc-for/2020/3701>
    schema:description "This group covers atmospheric sciences."@en ;
    schema:name "Atmospheric sciences"@en ;
.

<https://linked.data.gov.au/def/anzsrc-for/2020/3702>
    schema:description "This group covers climate change science."@en ;
    schema:name "Climate change science"@en ;
.

<https://linked.data.gov.au/def/anzsrc-for/2020/370202>
    schema:name "Climatology"@en ;
.

<https://linked.data.gov.au/def/anzsrc-for/2020/3703>
    schema:description "This group covers geochemistry."@en ;
    schema:name "Geochemistry"@en ;
.

<https://linked.data.gov.au/def/anzsrc-for/2020/370301>
    schema:name "Exploration geochemistry"@en ;
.

<https://linked.data.gov.au/def/anzsrc-for/2020/370302>
    schema:name "Inorganic geochemistry"@en ;
.

<https://linked.data.gov.au/def/anzsrc-for/2020/370303>
    schema:name "Isotope geochemistry"@en ;
.

<https://linked.data.gov.au/def/anzsrc-for/2020/370304>
    schema:name "Organic geochemistry"@en ;
.

<https://linked.data.gov.au/def/anzsrc-for/2020/370399>
    schema:name "Geochemistry not elsewhere classified"@en ;
.

<https://linked.data.gov.au/def/anzsrc-for/2020/3704>
    schema:description "This group covers geoinformatics."@en ;
    schema:name "Geoinformatics"@en ;
.

<https://linked.data.gov.au/def/anzsrc-for/2020/370401>
    schema:name "Computational modelling and simulation in earth sciences"@en ;
.

<https://linked.data.gov.au/def/anzsrc-for/2020/370402>
    schema:name "Earth and space science informatics"@en ;
.

<https://linked.data.gov.au/def/anzsrc-for/2020/370403>
    schema:name "Geoscience data visualisation"@en ;
.

<https://linked.data.gov.au/def/anzsrc-for/2020/370499>
    schema:name "Geoinformatics not elsewhere classified"@en ;
.

<https://linked.data.gov.au/def/anzsrc-for/2020/3705>
    schema:description """This group covers geology.
It includes palaeontology, including palaeozoology, palaeobotany and palynology, other than that associated with palaeoecological studies."""@en ;
    schema:name "Geology"@en ;
.

<https://linked.data.gov.au/def/anzsrc-for/2020/370502>
    schema:name "Geochronology"@en ;
.

<https://linked.data.gov.au/def/anzsrc-for/2020/370503>
    schema:name "Igneous and metamorphic petrology"@en ;
.

<https://linked.data.gov.au/def/anzsrc-for/2020/370504>
    schema:name "Marine geoscience"@en ;
.

<https://linked.data.gov.au/def/anzsrc-for/2020/370505>
    schema:name "Mineralogy and crystallography"@en ;
.

<https://linked.data.gov.au/def/anzsrc-for/2020/370506>
    schema:name "Palaeontology (incl. palynology)"@en ;
.

<https://linked.data.gov.au/def/anzsrc-for/2020/370507>
    schema:name "Planetary geology"@en ;
.

<https://linked.data.gov.au/def/anzsrc-for/2020/370508>
    schema:name "Resource geoscience"@en ;
.

<https://linked.data.gov.au/def/anzsrc-for/2020/370509>
    schema:name "Sedimentology"@en ;
.

<https://linked.data.gov.au/def/anzsrc-for/2020/370510>
    schema:name "Stratigraphy (incl. biostratigraphy, sequence stratigraphy and basin analysis)"@en ;
.

<https://linked.data.gov.au/def/anzsrc-for/2020/370511>
    schema:name "Structural geology and tectonics"@en ;
.

<https://linked.data.gov.au/def/anzsrc-for/2020/370512>
    schema:name "Volcanology"@en ;
.

<https://linked.data.gov.au/def/anzsrc-for/2020/370599>
    schema:name "Geology not elsewhere classified"@en ;
.

<https://linked.data.gov.au/def/anzsrc-for/2020/3706>
    schema:description "This group covers geophysics."@en ;
    schema:name "Geophysics"@en ;
.

<https://linked.data.gov.au/def/anzsrc-for/2020/370601>
    schema:name "Applied geophysics"@en ;
.

<https://linked.data.gov.au/def/anzsrc-for/2020/370603>
    schema:name "Geodesy"@en ;
.

<https://linked.data.gov.au/def/anzsrc-for/2020/370604>
    schema:name "Geodynamics"@en ;
.

<https://linked.data.gov.au/def/anzsrc-for/2020/370605>
    schema:name "Geothermics and radiometrics"@en ;
.

<https://linked.data.gov.au/def/anzsrc-for/2020/370606>
    schema:name "Gravimetrics"@en ;
.

<https://linked.data.gov.au/def/anzsrc-for/2020/370607>
    schema:name "Magnetism and palaeomagnetism"@en ;
.

<https://linked.data.gov.au/def/anzsrc-for/2020/370608>
    schema:name "Petrophysics and rock mechanics"@en ;
.

<https://linked.data.gov.au/def/anzsrc-for/2020/370609>
    schema:name "Seismology and seismic exploration"@en ;
.

<https://linked.data.gov.au/def/anzsrc-for/2020/370699>
    schema:name "Geophysics not elsewhere classified"@en ;
.

<https://linked.data.gov.au/def/anzsrc-for/2020/370704>
    schema:name "Surface water hydrology"@en ;
.

<https://linked.data.gov.au/def/anzsrc-for/2020/3709>
    schema:description "This group covers physical geography and environmental geoscience"@en ;
    schema:name "Physical geography and environmental geoscience"@en ;
.

<https://linked.data.gov.au/def/anzsrc-for/2020/370901>
    schema:name "Geomorphology and earth surface processes"@en ;
.

<https://linked.data.gov.au/def/anzsrc-for/2020/370902>
    schema:name "Glaciology"@en ;
.

<https://linked.data.gov.au/def/anzsrc-for/2020/370903>
    schema:name "Natural hazards"@en ;
.

<https://linked.data.gov.au/def/anzsrc-for/2020/370904>
    schema:name "Palaeoclimatology"@en ;
.

<https://linked.data.gov.au/def/anzsrc-for/2020/370905>
    schema:name "Quaternary environments"@en ;
.

<https://linked.data.gov.au/def/anzsrc-for/2020/370906>
    schema:name "Regolith and landscape evolution"@en ;
.

<https://linked.data.gov.au/def/anzsrc-for/2020/370999>
    schema:name "Physical geography and environmental geoscience not elsewhere classified"@en ;
.

<https://linked.data.gov.au/def/anzsrc-for/2020/40>
    schema:description "This division covers engineering."@en ;
    schema:name "ENGINEERING"@en ;
.

<https://linked.data.gov.au/def/anzsrc-for/2020/4011>
    schema:description "This group covers environmental engineering."@en ;
    schema:name "Environmental engineering"@en ;
.

<https://linked.data.gov.au/def/anzsrc-for/2020/4013>
    schema:description "This group covers geomatic engineering."@en ;
    schema:name "Geomatic engineering"@en ;
.

<https://linked.data.gov.au/def/anzsrc-for/2020/401301>
    schema:name "Cartography and digital mapping"@en ;
.

<https://linked.data.gov.au/def/anzsrc-for/2020/401302>
    schema:name "Geospatial information systems and geospatial data modelling"@en ;
.

<https://linked.data.gov.au/def/anzsrc-for/2020/401304>
    schema:name "Photogrammetry and remote sensing"@en ;
.

<https://linked.data.gov.au/def/anzsrc-for/2020/401305>
    schema:name "Satellite-based positioning"@en ;
.

<https://linked.data.gov.au/def/anzsrc-for/2020/401306>
    schema:name "Surveying (incl. hydrographic surveying)"@en ;
.

<https://linked.data.gov.au/def/anzsrc-for/2020/401399>
    schema:name "Geomatic engineering not elsewhere classified"@en ;
.

<https://linked.data.gov.au/def/anzsrc-for/2020/4019>
    schema:description "This group covers resources engineering and extractive metallurgy."@en ;
    schema:name "Resources engineering and extractive metallurgy"@en ;
.

<https://linked.data.gov.au/def/anzsrc-for/2020/401902>
    schema:name "Geomechanics and resources geotechnical engineering"@en ;
.

<https://linked.data.gov.au/def/anzsrc-for/2020/401907>
    schema:name "Petroleum and reservoir engineering"@en ;
.

<https://linked.data.gov.au/def/anzsrc-for/2020/41>
    schema:description "This division covers environmental sciences."@en ;
    schema:name "ENVIRONMENTAL SCIENCES"@en ;
.

<https://linked.data.gov.au/def/anzsrc-for/2020/4106>
    schema:description "This group covers soil sciences."@en ;
    schema:name "Soil sciences"@en ;
.

<https://linked.data.gov.au/def/anzsrc-for/2020/410602>
    schema:name "Pedology and pedometrics"@en ;
.

<https://linked.data.gov.au/def/anzsrc-for/2020/43>
    schema:description "This division covers history, heritage and archaeology."@en ;
    schema:name "HISTORY, HERITAGE AND ARCHAEOLOGY"@en ;
.

<https://linked.data.gov.au/def/anzsrc-for/2020/4301>
    schema:description "This group covers archaeology."@en ;
    schema:name "Archaeology"@en ;
.

<https://linked.data.gov.au/def/anzsrc-for/2020/430108>
    schema:name "Maritime archaeology"@en ;
.

<https://linked.data.gov.au/def/anzsrc-for/2020/4302>
    schema:description "This group covers heritage, archive and museum studies. It includes heritage and cultural conservation."@en ;
    schema:name "Heritage, archive and museum studies"@en ;
.

<https://linked.data.gov.au/def/anzsrc-for/2020/430201>
    schema:name "Archival, repository and related studies"@en ;
.

<https://linked.data.gov.au/def/anzsrc-for/2020/430204>
    schema:name "Digital heritage"@en ;
.

<https://linked.data.gov.au/def/anzsrc-for/2020/430205>
    schema:name "Heritage and cultural conservation"@en ;
.

<https://linked.data.gov.au/def/anzsrc-for/2020/430206>
    schema:name "Heritage collections and interpretations"@en ;
.

<https://linked.data.gov.au/def/anzsrc-for/2020/430207>
    schema:name "Heritage tourism, visitor and audience studies"@en ;
.

<https://linked.data.gov.au/def/anzsrc-for/2020/430208>
    schema:name "Intangible heritage"@en ;
.

<https://linked.data.gov.au/def/anzsrc-for/2020/430209>
    schema:name "Materials conservation"@en ;
.

<https://linked.data.gov.au/def/anzsrc-for/2020/44>
    schema:description "This division covers human society."@en ;
    schema:name "HUMAN SOCIETY"@en ;
.

<https://linked.data.gov.au/def/anzsrc-for/2020/4407>
    schema:description "This group covers policy and administration."@en ;
    schema:name "Policy and administration"@en ;
.

<https://linked.data.gov.au/def/anzsrc-for/2020/46>
    schema:description "This division covers information and computing sciences."@en ;
    schema:name "INFORMATION AND COMPUTING SCIENCES"@en ;
.

<https://linked.data.gov.au/def/anzsrc-for/2020/4602>
    schema:description "This group covers artificial intelligence other than Machine learning and computer vision."@en ;
    schema:name "Artificial intelligence"@en ;
.

<https://linked.data.gov.au/def/anzsrc-for/2020/4605>
    schema:description "This group covers methods and computing systems for working with data sets."@en ;
    schema:name "Data management and data science"@en ;
.

<https://linked.data.gov.au/def/anzsrc-for/2020/460502>
    schema:name "Data mining and knowledge discovery"@en ;
.

<https://linked.data.gov.au/def/anzsrc-for/2020/4609>
    schema:description "This group covers systems that manage information for organisational purposes."@en ;
    schema:name "Information systems"@en ;
.

<https://linked.data.gov.au/def/anzsrc-for/2020/51>
    schema:description "This division covers the physical sciences. It includes biological physics (other than human biophysics), medical physics and synchrotron and accelerator technologies."@en ;
    schema:name "PHYSICAL SCIENCES"@en ;
.

<https://linked.data.gov.au/def/anzsrc-for/2020/5101>
    schema:description "This group covers astronomical sciences, including cosmology."@en ;
    schema:name "Astronomical sciences"@en ;
.

<https://linked.data.gov.au/def/anzsrc-for/2020/510101>
    schema:name "Astrobiology"@en ;
.

<https://linked.data.gov.au/def/anzsrc-for/2020/430299>
    schema:name "Heritage, archive and museum studies not elsewhere classified"@en ;
.


<http://linked.data.gov.au/def/site-status/rehabilitation> schema:name "Rehabilitation"@en .