PREFIX : <https://linked.data.gov.au/def/gswa-rock-classification-scheme/>
PREFIX cs: <https://linked.data.gov.au/def/gswa-rock-classification-scheme>
PREFIX dcat: <http://www.w3.org/ns/dcat#>
PREFIX isoroles: <https://linked.data.gov.au/def/data-roles/>
PREFIX owl: <http://www.w3.org/2002/07/owl#>
PREFIX prov: <http://www.w3.org/ns/prov#>
PREFIX rdfs: <http://www.w3.org/2000/01/rdf-schema#>
PREFIX reg: <http://purl.org/linked-data/registry#>
PREFIX schema: <https://schema.org/>
PREFIX skos: <http://www.w3.org/2004/02/skos/core#>
PREFIX xsd: <http://www.w3.org/2001/XMLSchema#>
PREFIX theme: <https://linked.data.gov.au/def/gswa-vocabulary-themes/>

:gswa-rock-code
    a rdfs:Datatype ;
    schema:name "GSWA rock code" ;
    schema:description "GSWA's codes used for mapping lithologies and lithostratigraphic/lithotectonic units" ;

.

:alkali-feldspar-granite
    a skos:Concept ;
    rdfs:isDefinedBy cs: ;
    skos:broader :igneous-felsic-intrusive ;
    skos:definition "A special term for a variety of granite in which plagioclase is less than 10% of the total feldspar. Now defined modally in QAPF field 2 (Fig. 2.4, p. 22). (Le Maitre et al., 2005, p. 52)"@en ;
    skos:exactMatch
        <http://inspire.ec.europa.eu/codelist/LithologyValue/alkaliFeldsparGranite> ,
        <http://resource.geosciml.org/classifier/cgi/lithology/alkali_feldspar_granite> ;
    skos:historyNote "Based on the IUGS classification of igneous rocks (Le Maitre et al., 2005)." ;
    skos:inScheme cs: ;
    skos:notation "gf"^^:gswa-rock-code ;
    skos:prefLabel "alkali feldspar granite"@en ;
    schema:citation "https://glossary.americangeosciences.org/term/alkalifeldspargranite"^^xsd:anyURI ;
.

:alkali-feldspar-syenite
    a skos:Concept ;
    rdfs:isDefinedBy cs: ;
    skos:broader :igneous-felsic-intrusive ;
    skos:definition "A special term for a variety of syenite in which plagioclase is less than 10% of the total feldspar. Now defined modally in QAPF field 6 (Fig. 2.4, p. 22). (Le Maitre et al., 2005, p. 52)"@en ;
    skos:exactMatch
        <http://inspire.ec.europa.eu/codelist/LithologyValue/alkaliFeldsparSyenite> ,
        <http://resource.geosciml.org/classifier/cgi/lithology/alkali_feldspar_syenite> ;
    skos:historyNote "Based on the IUGS classification of igneous rocks (Le Maitre et al., 2005)." ;
    skos:inScheme cs: ;
    skos:notation "gs"^^:gswa-rock-code ;
    skos:prefLabel "alkali feldspar syenite"@en ;
    schema:citation "https://glossary.americangeosciences.org/term/alkalifeldsparsyenite"^^xsd:anyURI ;
.

:amphibolite
    a skos:Concept ;
    rdfs:isDefinedBy cs: ;
    skos:broader :meta-igneous-mafic ;
    skos:definition "Gneissose or granofelsic metamorphic rock mainly consisting of green, brown or black amphibole and plagioclase (including albite) and derived from an unspecified intrusive, extrusive or volcaniclastic protolith. Amphibole and plagioclase combined form more than 75% of the rock, with both being present as major constituents; the amphibole constitutes more than 50% of the total mafic constituents and is present in an amount of ≥30%. Other common minerals include quartz, clinopyroxene, garnet, epidote-group minerals, biotite, titanite and scapolite. Amphibolites are mostly present in amphibolite-facies metamorphic complexes, or in the highest subfacies of the greenschist facies. Adapted from Fettes and Desmons (2007, p. 128)."@en ;
    skos:exactMatch
        <http://inspire.ec.europa.eu/codelist/LithologyValue/amphibolite> ,
        <http://resource.geosciml.org/classifier/cgi/lithology/amphibolite> ;
    skos:historyNote "Based on the IUGS classification of metamorphic rocks (Fettes and Desmons, 2007) and GSWA usage." ;
    skos:inScheme cs: ;
    skos:notation "mwa"^^:gswa-rock-code ;
    skos:prefLabel "amphibolite"@en ;
    schema:citation "https://glossary.americangeosciences.org/term/amphibolite"^^xsd:anyURI ;
.

:amphibolite-derived-from-intrusive-rock
    a skos:Concept ;
    rdfs:isDefinedBy cs: ;
    skos:broader :meta-igneous-mafic-intrusive ;
    skos:definition "Gneissose or granofelsic metamorphic rock mainly consisting of green, brown or black amphibole and plagioclase (including albite) and derived from an intrusive protolith. Amphibole and plagioclase combined form more than 75% of the rock, with both being present as major constituents; the amphibole constitutes more than 50% of the total mafic constituents and is present in an amount greater than or equal to 30%. Other common minerals include quartz, clinopyroxene, garnet, epidote-group minerals, biotite, titanite and scapolite. Amphibolites are mostly present in amphibolite-facies metamorphic complexes, or in the highest subfacies of the greenschist facies. Adapted from Fettes and Desmons (2007, p. 128)."@en ;
    skos:historyNote "Based on the IUGS classification of metamorphic rocks (Fettes and Desmons, 2007)." ;
    skos:inScheme cs: ;
    skos:notation "moa"^^:gswa-rock-code ;
    skos:prefLabel "amphibolite derived from intrusive rock"@en ;
.

:amphibolite-derived-from-volcanic-rock
    a skos:Concept ;
    rdfs:isDefinedBy cs: ;
    skos:broader :meta-igneous-mafic-volcanic ;
    skos:definition "Gneissose or granofelsic metamorphic rock mainly consisting of green, brown or black amphibole and plagioclase (including albite) and derived from a volcanic protolith. Amphibole and plagioclase combined form more than 75% of the rock, with both being present as major constituents; the amphibole constitutes more than 50% of the total mafic constituents and is present in an amount of greater or equal to 30%. Other common minerals include quartz, clinopyroxene, garnet, epidote-group minerals, biotite, titanite and scapolite. Amphibolites are mostly present in amphibolite-facies metamorphic complexes, or in the highest subfacies of the greenschist facies. Adapted from Fettes and Desmons (2007, p. 128). GSWA's rock classification scheme prefers the use of volcanic terminology for any igneous rock formed on or near the Earth's surface, i.e. for those hypabyssal or subvolcanic rocks such as dykes, sills, and cryptodomes that are demonstrably both spatially and temporally associated with extrusive volcanic rocks."@en ;
    skos:historyNote "Based on the IUGS classification of metamorphic rocks (Fettes and Desmons, 2007)." ;
    skos:inScheme cs: ;
    skos:notation "mba"^^:gswa-rock-code ;
    skos:prefLabel "amphibolite derived from volcanic rock"@en ;
    schema:citation "https://glossary.americangeosciences.org/term/amphibolite"^^xsd:anyURI ;
.

:amphibolitic-fault-rock
    a skos:Concept ;
    rdfs:isDefinedBy cs: ;
    skos:broader :metamorphic-protolith-unknown-fault-rock ;
    skos:definition "A rock formed as a result of deformation in a fault zone and distinguished by the abundance of amphiboles. In GSWA usage, this term is reserved for fault rocks for which a protolith cannot be conclusively established."@en ;
    skos:historyNote "Compiled by the Geological Survey of Western Australia" ;
    skos:inScheme cs: ;
    skos:notation "mya"^^:gswa-rock-code ;
    skos:prefLabel "amphibolitic fault rock"@en ;
.

:amphibolitic-gneiss
    a skos:Concept ;
    rdfs:isDefinedBy cs: ;
    skos:broader :metamorphic-protolith-unknown-gneiss ;
    skos:definition "A gneiss distinguished by the abundance of amphiboles. In GSWA usage, this term is reserved for a gneiss for which a protolith cannot be conclusively established. See also definition of gneiss/gneissose structure in Fettes and Desmons (2007, p. 154–155)."@en ;
    skos:historyNote "Based on the IUGS classification of metamorphic rocks (Fettes and Desmons, 2007) and GSWA usage." ;
    skos:inScheme cs: ;
    skos:notation "mna"^^:gswa-rock-code ;
    skos:prefLabel "amphibolitic gneiss"@en ;
    schema:citation "https://glossary.americangeosciences.org/term/gneiss"^^xsd:anyURI ;
.

:amphibolitic-granofels-hornfels
    a skos:Concept ;
    rdfs:isDefinedBy cs: ;
    skos:broader :metamorphic-protolith-unknown-granofels-hornfels ;
    skos:definition "A granofels/hornfels distinguished by the abundance of amphiboles. In GSWA usage, this term is reserved for a granofels/hornfels for which a protolith cannot be conclusively established."@en ;
    skos:historyNote "Compiled by the Geological Survey of Western Australia" ;
    skos:inScheme cs: ;
    skos:notation "mea"^^:gswa-rock-code ;
    skos:prefLabel "amphibolitic granofels/hornfels"@en ;
.

:amphibolitic-schist
    a skos:Concept ;
    rdfs:isDefinedBy cs: ;
    skos:broader :metamorphic-protolith-unknown-schist ;
    skos:definition "A schist distinguished by the abundance of amphiboles. In GSWA usage, this term is reserved for a schist for which a protolith cannot be conclusively established. See also definition of schist/schistose structure in Fettes and Desmons, 2007, p. 193)."@en ;
    skos:historyNote "Based on the IUGS classification of metamorphic rocks (Fettes and Desmons, 2007) and GSWA usage." ;
    skos:inScheme cs: ;
    skos:notation "msa"^^:gswa-rock-code ;
    skos:prefLabel "amphibolitic schist"@en ;
.

:andesite
    a skos:Concept ;
    rdfs:isDefinedBy cs: ;
    skos:broader :igneous-felsic-volcanic ;
    skos:definition "An intermediate volcanic rock, usually porphyritic, consisting of plagioclase (frequently zoned from labradorite to oligoclase), pyroxene, hornblende and/or biotite. Now defined modally in QAPF fields 9 and 10 (Fig. 2.11, p. 31) and, if modes are not available, chemically in TAS field O2 (Fig. 2.14, p. 35). Definition from Le Maitre et al. (2005, p. 56). GSWA's rock classification scheme prefers the use of volcanic terminology for any igneous rock formed on or near the Earth's surface, i.e. for those hypabyssal or subvolcanic rocks such as dykes, sills, and cryptodomes that are demonstrably both spatially and temporally associated with extrusive volcanic rocks."@en ;
    skos:exactMatch
        <http://inspire.ec.europa.eu/codelist/LithologyValue/andesite> ,
        <http://resource.geosciml.org/classifier/cgi/lithology/andesite> ;
    skos:historyNote "Based on the IUGS classification of igneous rocks (Le Maitre et al., 2005)." ;
    skos:inScheme cs: ;
    skos:notation "fa"^^:gswa-rock-code ;
    skos:prefLabel "andesite"@en ;
    schema:citation "https://glossary.americangeosciences.org/term/andesite"^^xsd:anyURI ;
.

:anhydrite-evaporite
    a skos:Concept ;
    rdfs:isDefinedBy cs: ;
    skos:altLabel "anhydrite evaporite"@en ;
    skos:broader :evaporite ;
    skos:definition "An evaporite consisting predominantly of the mineral anhydrite, i.e. of anhydrous calcium sulfate (CaSO₄)."@en ;
    skos:historyNote "Compiled by the Geological Survey of Western Australia" ;
    skos:inScheme cs: ;
    skos:notation "cva"^^:gswa-rock-code ;
    skos:prefLabel "anhydrite (evaporite)"@en ;
    schema:citation "https://glossary.americangeosciences.org/term/anhydrite"^^xsd:anyURI ;
.

:anorthosite
    a skos:Concept ;
    rdfs:isDefinedBy cs: ;
    skos:altLabel "plagioclasite"@en ;
    skos:broader :igneous-mafic-intrusive ;
    skos:definition "A leucocratic intrusive rock consisting essentially of plagioclase commonly with small amounts of pyroxene. Now defined modally in QAPF field 10 (Fig. 2.4, p. 22). The term is synonymous with plagioclasite. (Le Maitre et al., 2005, p. 57)"@en ;
    skos:exactMatch
        <http://inspire.ec.europa.eu/codelist/LithologyValue/anorthosite> ,
        <http://resource.geosciml.org/classifier/cgi/lithology/anorthosite> ;
    skos:historyNote "Based on the IUGS classification of igneous rocks (Le Maitre et al., 2005)." ;
    skos:inScheme cs: ;
    skos:notation "oa"^^:gswa-rock-code ;
    skos:prefLabel "anorthosite"@en ;
    schema:citation "https://glossary.americangeosciences.org/term/anorthosite"^^xsd:anyURI ;
.

:anthracite
    a skos:Concept ;
    rdfs:isDefinedBy cs: ;
    skos:altLabel
        "hard coal"@en ,
        "kilkenny coal"@en ,
        "stone coal"@en ;
    skos:broader :coal ;
    skos:definition "Coal of the highest metamorphic rank, in which fixed-carbon content is between 92% and 98% and less than 14% volatile matter (on a dry, mineral-matter-free basis). It is hard and black, and has a semi-metallic lustre and semi-conchoidal fracture. Anthracite ignites with difficulty and burns with a short blue flame, without smoke. Adapted from Glossary of geology (5th edition revised; Neuendorf et al., 2011)."@en ;
    skos:exactMatch
        <http://inspire.ec.europa.eu/codelist/LithologyValue/anthraciteCoal> ,
        <http://resource.geosciml.org/classifier/cgi/lithology/anthracite_coal> ;
    skos:historyNote "Forsman, JP and Hunt, JM 1958, Insoluble organic matter (kerogen) in sedimentary rocks: Geochimica et Cosmochimica Acta, v. 15(3), p. 170–182, doi.org/10.1016/0016-7037(58)90055-3." ;
    skos:inScheme cs: ;
    skos:notation "coh"^^:gswa-rock-code ;
    skos:prefLabel "anthracite"@en ;
    schema:citation "https://glossary.americangeosciences.org/term/anthracite"^^xsd:anyURI ;
.

:banded-iron-formation
    a skos:Concept ;
    rdfs:isDefinedBy cs: ;
    skos:altLabel "BIF"@en ;
    skos:broader :iron-formation ;
    skos:definition "Banded iron-formation (BIF) is an iron formation that shows marked banding, generally of iron-rich minerals and chert or fine-grained quartz. Adapted from Glossary of geology (5th edition revised; Neuendorf et al., 2011)."@en ;
    skos:historyNote "Beukes, NJ and Gutzmer, J 2008, Origin and paleoenvironmental significance of major iron formations at the Archean-Paleoproterozoic boundary: Reviews in Economic Geology, v. 15, p. 5–47, doi:10.5382/Rev.15.01." ;
    skos:inScheme cs: ;
    skos:notation "cib"^^:gswa-rock-code ;
    skos:prefLabel "banded iron-formation"@en ;
    schema:citation "https://glossary.americangeosciences.org/term/bandedironformation"^^xsd:anyURI ;
.

:baryte
    a skos:Concept ;
    rdfs:isDefinedBy cs: ;
    skos:broader :sedimentary-other-chemical-or-biochemical ;
    skos:definition "A mappable concentration of the mineral baryte, a white, yellow, or colourless orthorhombic barium sulfate (BaSO4). Baryte occurs in tabular crystals, in granular form, or in compact masses resembling marble, deposited via either biogenic or evaporitic processes. Adapted from Glossary of geology (5th edition revised; Neuendorf et al., 2011)."@en ;
    skos:historyNote "Compiled by the Geological Survey of Western Australia" ;
    skos:inScheme cs: ;
    skos:notation "cb"^^:gswa-rock-code ;
    skos:prefLabel "baryte"@en ;
    schema:citation "https://glossary.americangeosciences.org/term/barite"^^xsd:anyURI ;
.

:baryte-vein
    a skos:Concept ;
    rdfs:isDefinedBy cs: ;
    skos:broader :hydrothermal ;
    skos:definition "A rock comprising baryte of pegmatitic or hydrothermal origin, as vein-filling material."@en ;
    skos:historyNote "Compiled by the Geological Survey of Western Australia" ;
    skos:inScheme cs: ;
    skos:notation "zb"^^:gswa-rock-code ;
    skos:prefLabel "baryte vein"@en ;
.

:basalt
    a skos:Concept ;
    rdfs:isDefinedBy cs: ;
    skos:broader :igneous-mafic-volcanic ;
    skos:definition "A dark-coloured volcanic rock consisting essentially of calcic plagioclase and pyroxene. Olivine and minor foids or minor interstitial quartz may also be present. Now defined modally in QAPF fields 9 and 10 (Fig. 2.11, p. 31) and, if modes are not available, chemically in TAS field B (Fig. 2.14, p. 35). Definition from Le Maitre et al. (2005, p. 60). The GSWA's rock classification scheme prefers the use of volcanic terminology for any igneous rock formed on or near the Earth's surface, i.e. for those hypabyssal or subvolcanic rocks such as dykes, sills, and cryptodomes that are demonstrably both spatially and temporally associated with extrusive volcanic rocks."@en ;
    skos:exactMatch
        <http://inspire.ec.europa.eu/codelist/LithologyValue/basalt> ,
        <http://resource.geosciml.org/classifier/cgi/lithology/basalt> ;
    skos:historyNote "Based on the IUGS classification of igneous rocks (Le Maitre et al., 2005)." ;
    skos:inScheme cs: ;
    skos:notation "bb"^^:gswa-rock-code ;
    skos:prefLabel "basalt"@en ;
    schema:citation "https://glossary.americangeosciences.org/term/basaltpetrology"^^xsd:anyURI ;
.

:basaltic-andesite
    a skos:Concept ;
    rdfs:isDefinedBy cs: ;
    skos:broader :igneous-mafic-volcanic ;
    skos:definition "A volcanic rock with plagioclase of variable composition and the ferromagnesian minerals more commonly found in basalts, e.g. olivine. Now defined chemically in TAS field O1. Definition from Le Maitre et al. (2005, p. 61). The GSWA's rock classification scheme prefers the use of volcanic terminology for any igneous rock formed on or near the Earth's surface, i.e. for those hypabyssal or subvolcanic rocks such as dykes, sills, and cryptodomes that are demonstrably both spatially and temporally associated with extrusive volcanic rocks."@en ;
    skos:historyNote "Based on the IUGS classification of igneous rocks (Le Maitre et al., 2005)." ;
    skos:inScheme cs: ;
    skos:notation "bd"^^:gswa-rock-code ;
    skos:prefLabel "basaltic andesite"@en ;
    schema:citation "https://glossary.americangeosciences.org/term/basalticandesite"^^xsd:anyURI ;
.

:bituminous-coal
    a skos:Concept ;
    rdfs:isDefinedBy cs: ;
    skos:altLabel
        "black coal"@en ,
        "soft coal"@en ;
    skos:broader :coal ;
    skos:definition "Coal that ranks between sub-bituminous coal and anthracite, contains more than 14% volatile matter (on a dry, ash-free basis) and has a calorific value of more than 11,500 BTU/lb (26.75 MJ/kg) (moist, mineral-matter-free) or more than 10 500 BTU/lb (24.42 MJ/kg) if agglomerating. It is dark brown to black in colour and burns with a smoky flame. Bituminous coal is the most abundant rank of coal. Adapted from Glossary of geology (5th edition revised; Neuendorf et al., 2011)."@en ;
    skos:exactMatch
        <http://inspire.ec.europa.eu/codelist/LithologyValue/bituminousCoal> ,
        <http://resource.geosciml.org/classifier/cgi/lithology/bituminous_coal> ;
    skos:historyNote "Forsman, JP and Hunt, JM 1958, Insoluble organic matter (kerogen) in sedimentary rocks: Geochimica et Cosmochimica Acta, v. 15(3), p. 170–182, doi.org/10.1016/0016-7037(58)90055-3." ;
    skos:inScheme cs: ;
    skos:notation "coc"^^:gswa-rock-code ;
    skos:prefLabel "bituminous coal"@en ;
    schema:citation "https://glossary.americangeosciences.org/term/bituminouscoal"^^xsd:anyURI ;
.

:blastomylonite
    a skos:Concept ;
    rdfs:isDefinedBy cs: ;
    skos:broader :metamorphic-protolith-unknown-fault-rock ;
    skos:definition "Fault rock that is cohesive and characterized by a well-developed schistosity resulting from tectonic reduction of grain size for more than 90% of the rock volume, and displays a significant degree of grain growth related to or following deformation. Definition adapted from Fossen (2016) and Fettes and Desmons (2007, p. 134)."@en ;
    skos:historyNote "Fossen, H 2016, Structural geology (2nd edition): Cambridge University Press, Cambridge, United Kingdom, 524p." ;
    skos:inScheme cs: ;
    skos:notation "myn"^^:gswa-rock-code ;
    skos:prefLabel "blastomylonite"@en ;
    schema:citation "https://glossary.americangeosciences.org/term/blastomylonite"^^xsd:anyURI ;
.

:blueschist
    a skos:Concept ;
    rdfs:isDefinedBy cs: ;
    skos:broader :meta-igneous-mafic ;
    skos:definition "Schist whose bluish colour is due to the presence of sodic amphibole. More precise terms should be used wherever possible (e.g. glaucophane schist). The term is also used as a facies name and if used in this sense the facies context should be made clear by saying blueschist-facies rock (or schist, or gneiss, or granofels). (Fettes and Desmons, 2007, p. 135)"@en ;
    skos:historyNote "Based on the IUGS classification of metamorphic rocks (Fettes and Desmons, 2007)." ;
    skos:inScheme cs: ;
    skos:notation "mwj"^^:gswa-rock-code ;
    skos:prefLabel "blueschist"@en ;
    schema:citation "https://glossary.americangeosciences.org/term/blueschist"^^xsd:anyURI ;
.

:boulder-conglomerate
    a skos:Concept ;
    rdfs:isDefinedBy cs: ;
    skos:altLabel "boulderstone"@en ;
    skos:broader :conglomerate ;
    skos:definition "A consolidated rock consisting mainly of boulders (clasts greater than 256 mm or -8 phi units in size). Adapted from Glossary of geology (5th edition revised; Neuendorf et al., 2011)."@en ;
    skos:historyNote "Wentworth, CK 1922, A scale of grade and class terms for clastic sediments: The Journal of Geology, v. 30, no. 5, p. 377–392, doi:10.1086/622910." ;
    skos:inScheme cs: ;
    skos:notation "sb"^^:gswa-rock-code ;
    skos:prefLabel "boulder conglomerate"@en ;
    schema:citation "https://glossary.americangeosciences.org/term/boulderconglomerate"^^xsd:anyURI ;
.

:calc-silicate-gneiss
    a skos:Concept ;
    rdfs:isDefinedBy cs: ;
    skos:broader :calc-silicate-rock ;
    skos:definition "A gneissose rock mainly composed of calc-silicate minerals (i.e. calcium-rich silicate minerals) and containing less than 5% volume of carbonate minerals (calcite and/or aragonite and/or dolomite). Adapted from Fettes and Desmons (2007, p. 137)."@en ;
    skos:historyNote "Based on the IUGS classification of metamorphic rocks (Fettes and Desmons, 2007)." ;
    skos:inScheme cs: ;
    skos:notation "mkqn"^^:gswa-rock-code ;
    skos:prefLabel "calc-silicate gneiss"@en ;
.

:calc-silicate-granofels-hornfels
    a skos:Concept ;
    rdfs:isDefinedBy cs: ;
    skos:altLabel "tactite"@en ;
    skos:broader :calc-silicate-rock ;
    skos:definition "A granofels/hornfels mainly composed of calc-silicate minerals (i.e. calcium-rich silicate minerals) and containing less than 5% volume of carbonate minerals (calcite and/or aragonite and/or dolomite) (adapted from Fettes and Desmons, 2007, p. 137). A calc-silicate rock formed by contact metasomatism of a carbonate or marly rock (i.e. a calc-silicate hornfels) is also referred to as tactite (Fettes and Desmons, 2007, p. 199)."@en ;
    skos:historyNote "Based on the IUGS classification of metamorphic rocks (Fettes and Desmons, 2007)." ;
    skos:inScheme cs: ;
    skos:notation "mkqe"^^:gswa-rock-code ;
    skos:prefLabel "calc-silicate granofels/hornfels"@en ;
.

:calc-silicate-schist
    a skos:Concept ;
    rdfs:isDefinedBy cs: ;
    skos:broader :calc-silicate-rock ;
    skos:definition "A schistose rock mainly composed of calc-silicate minerals (i.e. calcium-rich silicate minerals) and containing less than 5% volume of carbonate minerals (calcite and/or aragonite and/or dolomite). Adapted from Fettes and Desmons (2007, p. 137)"@en ;
    skos:historyNote "Based on the IUGS classification of metamorphic rocks (Fettes and Desmons, 2007)." ;
    skos:inScheme cs: ;
    skos:notation "mkqs"^^:gswa-rock-code ;
    skos:prefLabel "calc-silicate schist"@en ;
.

:calcarenite
    a skos:Concept ;
    rdfs:isDefinedBy cs: ;
    skos:altLabel "calcareous sandstone"@en ;
    skos:broader :limestone ;
    skos:definition "A limestone consisting predominantly (more than 50%) of sand-size, detrital carbonate grains; a consolidated calcareous sand. The term was introduced by Grabau (1903). (Glossary of geology, 5th edition revised; Neuendorf et al., 2011)"@en ;
    skos:historyNote "Grabau, AW 1903, Paleozoic coral reefs: Geological Society of America Bulletin, v. 14, p. 337–352." ;
    skos:inScheme cs: ;
    skos:notation "kla"^^:gswa-rock-code ;
    skos:prefLabel "calcarenite"@en ;
    schema:citation "https://glossary.americangeosciences.org/term/calcarenite"^^xsd:anyURI ;
.

:calcareous-sandstone
    a skos:Concept ;
    rdfs:isDefinedBy cs: ;
    skos:broader :sandstone ;
    skos:definition "A terrigenous sandstone that is cemented with calcite. Adapted from Glossary of geology (5th edition revised; Neuendorf et al., 2011)."@en ;
    skos:historyNote "Based on the Glossary of geology (5th edition, revised; Neuendorf et al. 2011)." ;
    skos:inScheme cs: ;
    skos:notation "stk"^^:gswa-rock-code ;
    skos:prefLabel "calcareous sandstone"@en ;
    schema:citation "https://glossary.americangeosciences.org/term/calcareoussandstone"^^xsd:anyURI ;
.

:calcilutite
    a skos:Concept ;
    rdfs:isDefinedBy cs: ;
    skos:altLabel
        "calcisiltite"@en ,
        "micritic limestone"@en ;
    skos:broader :limestone ;
    skos:definition "A limestone consisting predominantly (more than 50%) of detrital calcite particles of silt and/or clay size; a consolidated carbonate mud. The term was introduced by Grabau (1903). Adapted from Glossary of geology (5th edition revised; Neuendorf et al., 2011)."@en ;
    skos:historyNote "Grabau, AW 1903, Paleozoic coral reefs: Geological Society of America Bulletin, v. 14, p. 337–352." ;
    skos:inScheme cs: ;
    skos:notation "kll"^^:gswa-rock-code ;
    skos:prefLabel "calcilutite"@en ;
    schema:citation "https://glossary.americangeosciences.org/term/calcilutite"^^xsd:anyURI ;
.

:calcirudite
    a skos:Concept ;
    rdfs:isDefinedBy cs: ;
    skos:broader :limestone ;
    skos:definition "A limestone consisting predominantly (more than 50%) of detrital calcite particles larger than sand size (larger than 2 mm in diameter), and commonly also cemented with calcareous material; a consolidated calcareous gravel or rubble, or a limestone conglomerate or breccia. The term was introduced by Grabau (1903). Adapted from Glossary of geology (5th edition revised; Neuendorf et al., 2011)."@en ;
    skos:historyNote "Grabau, AW 1903, Paleozoic coral reefs: Geological Society of America Bulletin, v. 14, p. 337–352." ;
    skos:inScheme cs: ;
    skos:notation "klr"^^:gswa-rock-code ;
    skos:prefLabel "calcirudite"@en ;
    schema:citation "https://glossary.americangeosciences.org/term/calcirudite"^^xsd:anyURI ;
.

:calcite-carbonatite
    a skos:Concept ;
    rdfs:isDefinedBy cs: ;
    skos:altLabel
        "alvikite"@en ,
        "sövite"@en ;
    skos:broader :igneous-carbonatite ;
    skos:definition "A variety of carbonatite in which the main carbonate is calcite (section 2.3, p. 10). If the rock is coarse-grained it may be called sövite; if medium- to fine-grained, alvikite. Adapted from Le Maitre et al. (2005, p. 10, 66, 53 and 143)."@en ;
    skos:historyNote "Based on the IUGS classification of igneous rocks (Le Maitre et al., 2005)." ;
    skos:inScheme cs: ;
    skos:notation "rc"^^:gswa-rock-code ;
    skos:prefLabel "calcite-carbonatite"@en ;
    schema:citation "https://glossary.americangeosciences.org/term/carbonatite"^^xsd:anyURI ;
.

:calcite-evaporite
    a skos:Concept ;
    rdfs:isDefinedBy cs: ;
    skos:altLabel "calcite/carbonate evaporite"@en ;
    skos:broader :evaporite ;
    skos:definition "An evaporite consisting predominantly of the mineral calcite, i.e. of anhydrous calcium carbonate (CaCO₃)."@en ;
    skos:historyNote "Compiled by the Geological Survey of Western Australia" ;
    skos:inScheme cs: ;
    skos:notation "cve"^^:gswa-rock-code ;
    skos:prefLabel "calcite (evaporite)"@en ;
    schema:citation "https://glossary.americangeosciences.org/term/calcite"^^xsd:anyURI ;
.

:calcite-vein
    a skos:Concept ;
    rdfs:isDefinedBy cs: ;
    skos:broader :hydrothermal ;
    skos:definition "A rock comprising calcite of hydrothermal origin, as vein-filling material."@en ;
    skos:historyNote "Compiled by the Geological Survey of Western Australia" ;
    skos:inScheme cs: ;
    skos:notation "zk"^^:gswa-rock-code ;
    skos:prefLabel "calcite vein"@en ;
.

:camptonite
    a skos:Concept ;
    rdfs:isDefinedBy cs: ;
    skos:broader :igneous-lamprophyres ;
    skos:definition "A variety of lamprophyre composed of phenocrysts of combinations of olivine, kaersutite, titanian augite, and Ti-rich biotite in a matrix of the same minerals (minus olivine) with plagioclase and sometimes subordinate alkali feldspar and feldspathoids. A volatile-rich basanite or alkali basalt. Now defined in the lamprophyre classification (Table 2.9, p. 19). (Le Maitre et al., 2005, p. 67)"@en ;
    skos:historyNote "Based on the IUGS classification of igneous rocks (Le Maitre et al., 2005)." ;
    skos:inScheme cs: ;
    skos:notation "yc"^^:gswa-rock-code ;
    skos:prefLabel "camptonite"@en ;
.

:carbonate-altered-meta-igneous-mafic-rock
    a skos:Concept ;
    rdfs:isDefinedBy cs: ;
    skos:broader :meta-igneous-mafic ;
    skos:definition "A mafic igneous rock affected by carbon dioxide metasomatism, whereby the interaction of the rock with CO2 fluids has resulted in the formation of carbonate minerals (such as calcite and dolomite), and for which an intrusive, extrusive or volcaniclastic protolith cannot be conclusively identified. There is no implication on the timing of alteration relative to other metamorphic processes (e.g. regional metamorphism) that may have affected the rock."@en ;
    skos:historyNote "Based on the IUGS classification of metamorphic rocks (Fettes and Desmons, 2007) and GSWA usage." ;
    skos:inScheme cs: ;
    skos:notation "mwk"^^:gswa-rock-code ;
    skos:prefLabel "carbonate-altered meta-igneous mafic rock"@en ;
.

:carbonate-altered-metamafic-volcanic-rock
    a skos:Concept ;
    rdfs:isDefinedBy cs: ;
    skos:broader :meta-igneous-mafic-volcanic ;
    skos:definition "A mafic volcanic rock affected by carbon dioxide metasomatism, whereby the interaction of the rock with CO₂ fluids has resulted in the formation of carbonate minerals (such as calcite and dolomite). There is no implication on the timing of alteration relative to other metamorphic processes (e.g. regional metamorphism) that may have affected the rock. GSWA's rock classification scheme prefers the use of volcanic terminology for any igneous rock formed on or near the Earth's surface, i.e. for those hypabyssal or subvolcanic rocks such as dykes, sills, and cryptodomes that are demonstrably both spatially and temporally associated with extrusive volcanic rocks."@en ;
    skos:historyNote "Compiled by the Geological Survey of Western Australia" ;
    skos:inScheme cs: ;
    skos:notation "mbk"^^:gswa-rock-code ;
    skos:prefLabel "carbonate-altered metamafic volcanic rock"@en ;
    schema:citation "https://glossary.americangeosciences.org/term/carbonatization"^^xsd:anyURI ;
.

:carbonate-fault-rock
    a skos:Concept ;
    rdfs:isDefinedBy cs: ;
    skos:broader :metamorphic-protolith-unknown-fault-rock ;
    skos:definition "A rock formed as a result of deformation in a fault zone and distinguished by the abundance of carbonate mineral phases. In GSWA usage, this term is reserved for fault rocks for which a protolith cannot be conclusively established."@en ;
    skos:historyNote "Compiled by the Geological Survey of Western Australia" ;
    skos:inScheme cs: ;
    skos:notation "myk"^^:gswa-rock-code ;
    skos:prefLabel "carbonate fault rock"@en ;
.

:carbonate-gneiss
    a skos:Concept ;
    rdfs:isDefinedBy cs: ;
    skos:broader :metamorphic-protolith-unknown-gneiss ;
    skos:definition "A gneiss distinguished by the abundance of carbonate mineral phases. In GSWA usage, this term is reserved for a gneiss for which a protolith cannot be conclusively established. See also definition of gneiss/gneissose structure in Fettes and Desmons (2007, p. 154–155)."@en ;
    skos:historyNote "Based on the IUGS classification of metamorphic rocks (Fettes and Desmons, 2007) and GSWA usage." ;
    skos:inScheme cs: ;
    skos:notation "mnk"^^:gswa-rock-code ;
    skos:prefLabel "carbonate gneiss"@en ;
    schema:citation "https://glossary.americangeosciences.org/term/gneiss"^^xsd:anyURI ;
.

:carbonate-gneiss-sedimentary
    a skos:Concept ;
    rdfs:isDefinedBy cs: ;
    skos:broader :metasedimentary-carbonate ;
    skos:definition "A metamorphosed sedimentary carbonate rock displaying a gneissose structure, i.e. a gneiss derived from a sedimentary rock consisting mostly of carbonates. See also definition of gneiss/gneissose structure in Fettes and Desmons (2007, p. 154–155)."@en ;
    skos:historyNote "Compiled by the Geological Survey of Western Australia" ;
    skos:inScheme cs: ;
    skos:notation "mkn"^^:gswa-rock-code ;
    skos:prefLabel "carbonate gneiss (sedimentary)"@en ;
.

:carbonate-granofels-hornfels
    a skos:Concept ;
    rdfs:isDefinedBy cs: ;
    skos:broader :metamorphic-protolith-unknown-granofels-hornfels ;
    skos:definition "A granofels/hornfels distinguished by the abundance of carbonate mineral phases. In GSWA usage, this term is reserved for a granofels/hornfels for which a protolith cannot be conclusively established."@en ;
    skos:historyNote "Compiled by the Geological Survey of Western Australia" ;
    skos:inScheme cs: ;
    skos:notation "mek"^^:gswa-rock-code ;
    skos:prefLabel "carbonate granofels/hornfels"@en ;
.

:carbonate-granofels-hornfels-sedimentary
    a skos:Concept ;
    rdfs:isDefinedBy cs: ;
    skos:broader :metasedimentary-carbonate ;
    skos:definition "A metamorphosed sedimentary carbonate rock displaying a granofelsic structure, i.e. a granofels/hornfels derived from a sedimentary rock consisting mostly of carbonates. See also definition of granofels/granofelsic structure in Fettes and Desmons (2007, p. 156); hornfels are granofels formed by contact metamorphism (Fettes and Desmons, 2007, p. 159)."@en ;
    skos:historyNote "Compiled by the Geological Survey of Western Australia" ;
    skos:inScheme cs: ;
    skos:notation "mke"^^:gswa-rock-code ;
    skos:prefLabel "carbonate granofels/hornfels (sedimentary)"@en ;
.

:carbonate-rock
    a skos:Concept ;
    rdfs:isDefinedBy cs: ;
    skos:altLabel "calcareous rock"@en ;
    skos:broader :sedimentary-carbonate ;
    skos:definition "A sedimentary rock consisting of more than 50% by weight of carbonate minerals, otherwise uncategorized. Adapted from Glossary of geology (5th edition revised; Neuendorf et al., 2011)."@en ;
    skos:exactMatch
        <http://inspire.ec.europa.eu/codelist/LithologyValue/carbonateSedimentaryRock> ,
        <http://resource.geosciml.org/classifier/cgi/lithology/carbonate_sedimentary_rock> ;
    skos:historyNote "Compiled by the Geological Survey of Western Australia" ;
    skos:inScheme cs: ;
    skos:notation "k"^^:gswa-rock-code ;
    skos:prefLabel "carbonate rock"@en ;
    schema:citation "https://glossary.americangeosciences.org/term/carbonaterock"^^xsd:anyURI ;
.

:carbonate-rock-undivided
    a skos:Concept ;
    rdfs:isDefinedBy cs: ;
    skos:altLabel "calcareous rock"@en ;
    skos:broader :sedimentary-carbonate ;
    skos:definition "A sedimentary rock consisting of more than 50% by weight of carbonate minerals, otherwise uncategorised (adapted from Glossary of geology (2011, 5th edition revised). GSWA usage of this term is restricted to rocks that are partially weathered or are identified using remote sensing imagery, and the use of the related code/notation is limited to GSWA's Explanatory Notes System."@en ;
    skos:historyNote "Compiled by the Geological Survey of Western Australia" ;
    skos:inScheme cs: ;
    skos:notation "kn"^^:gswa-rock-code ;
    skos:prefLabel "carbonate rock; undivided"@en ;
    schema:citation "https://glossary.americangeosciences.org/term/carbonaterock"^^xsd:anyURI ;
.

:carbonate-schist
    a skos:Concept ;
    rdfs:isDefinedBy cs: ;
    skos:broader :metamorphic-protolith-unknown-schist ;
    skos:definition "A schist distinguished by the abundance of carbonate mineral phases. In GSWA usage, this term is reserved for a schist for which a protolith cannot be conclusively established. See also definition of schist/schistose structure in Fettes and Desmons, 2007, p. 193)."@en ;
    skos:historyNote "Based on the IUGS classification of metamorphic rocks (Fettes and Desmons, 2007) and GSWA usage." ;
    skos:inScheme cs: ;
    skos:notation "msk"^^:gswa-rock-code ;
    skos:prefLabel "carbonate schist"@en ;
.

:carbonate-schist-sedimentary
    a skos:Concept ;
    rdfs:isDefinedBy cs: ;
    skos:broader :metasedimentary-carbonate ;
    skos:definition "A metamorphosed sedimentary carbonate rock displaying a schistose structure, i.e. a schist derived from a sedimentary rock consisting mostly of carbonates. See also definition of gneiss/gneissose structure in Fettes and Desmons (2007, p. 154–155)."@en ;
    skos:historyNote "Compiled by the Geological Survey of Western Australia" ;
    skos:inScheme cs: ;
    skos:notation "mks"^^:gswa-rock-code ;
    skos:prefLabel "carbonate schist (sedimentary)"@en ;
.

:carbonate-with-lesser-siliciclastic
    a skos:Concept ;
    rdfs:isDefinedBy cs: ;
    skos:broader :sedimentary-carbonate ;
    skos:definition "Limestone and/or dolomite interleaved with siliciclastic rocks at outcrop scale."@en ;
    skos:historyNote "Compiled by the Geological Survey of Western Australia" ;
    skos:inScheme cs: ;
    skos:notation "kt"^^:gswa-rock-code ;
    skos:prefLabel "carbonate + lesser siliciclastic"@en ;
.

:carbonatite
    a skos:Concept ;
    rdfs:isDefinedBy cs: ;
    skos:broader :igneous-carbonatite ;
    skos:definition "A collective term for an igneous (intrusive, extrusive or volcaniclastic) rock in which the modal amount of primary carbonate minerals is greater than 50%, but otherwise uncategorized (section 2.3, p. 10). Adapted from Le Maitre et al. (2005, p. 68)."@en ;
    skos:exactMatch
        <http://inspire.ec.europa.eu/codelist/LithologyValue/carbonatite> ,
        <http://resource.geosciml.org/classifier/cgi/lithology/carbonatite> ;
    skos:historyNote "Based on the IUGS classification of igneous rocks (Le Maitre et al., 2005)." ;
    skos:inScheme cs: ;
    skos:notation "r"^^:gswa-rock-code ;
    skos:prefLabel "carbonatite"@en ;
    schema:citation "https://glossary.americangeosciences.org/term/carbonatite"^^xsd:anyURI ;
.

:carbonatitic-rock-undivided
    a skos:Concept ;
    rdfs:isDefinedBy cs: ;
    skos:broader :igneous-carbonatite ;
    skos:definition "An igneous (intrusive, extrusive or volcaniclastic) carbonate-rich rock, otherwise uncategorized. GSWA usage of this term is restricted to rocks that are partially weathered or are identified using remote sensing imagery, and the use of the related code/notation is limited to GSWA's Explanatory Notes System."@en ;
    skos:historyNote "Compiled by the Geological Survey of Western Australia" ;
    skos:inScheme cs: ;
    skos:notation "rn"^^:gswa-rock-code ;
    skos:prefLabel "carbonatitic rock; undivided"@en ;
.

:carbonatitic-volcaniclastic-breccia
    a skos:Concept ;
    rdfs:isDefinedBy cs: ;
    skos:broader :igneous-carbonatite ;
    skos:definition "A volcaniclastic rock composed mostly of angular fragments greater than 2 mm in size consisting of either (a) pyroclastic detritus or (b) terrigenous volcanic detritus of epiclastic origin, with more than 50% modal carbonates. 'Volcaniclastic' includes all clastic volcanic materials formed by any process of fragmentation, dispersed by any kind of transporting agent, deposited in any environment, or mixed in any significant portion with non-volcanic fragments."@en ;
    skos:historyNote "Compiled by the Geological Survey of Western Australia" ;
    skos:inScheme cs: ;
    skos:notation "rvb"^^:gswa-rock-code ;
    skos:prefLabel "carbonatitic volcaniclastic breccia"@en ;
.

:carbonatitic-volcaniclastic-breccia-sandstone
    a skos:Concept ;
    rdfs:isDefinedBy cs: ;
    skos:broader :igneous-carbonatite ;
    skos:definition "A volcaniclastic rock composed mostly of angular fragments ranging in size from sand (0.0625 – 2 mm) and above, consisting of either (a) pyroclastic detritus or (b) terrigenous volcanic detritus of epiclastic origin, and with more than 50% modal carbonates. 'Volcaniclastic' includes all clastic volcanic materials formed by any process of fragmentation, dispersed by any kind of transporting agent, deposited in any environment, or mixed in any significant portion w, and with an overall mafic composition."@en ;
    skos:historyNote "Compiled by the Geological Survey of Western Australia" ;
    skos:inScheme cs: ;
    skos:notation "rvbs"^^:gswa-rock-code ;
    skos:prefLabel "carbonatitic volcaniclastic breccia-sandstone"@en ;
.

:carbonatitic-volcaniclastic-conglomerate
    a skos:Concept ;
    rdfs:isDefinedBy cs: ;
    skos:broader :igneous-carbonatite ;
    skos:definition "A conglomerate consisting of either (a) pyroclastic detritus or (b) terrigenous volcanic detritus of epiclastic origin, and with more than 50% modal carbonates. 'Volcaniclastic' includes all clastic volcanic materials formed by any process of fragmentation, dispersed by any kind of transporting agent, deposited in any environment, or mixed in any significant portion with non-volcanic fragments."@en ;
    skos:historyNote "Compiled by the Geological Survey of Western Australia" ;
    skos:inScheme cs: ;
    skos:notation "rvc"^^:gswa-rock-code ;
    skos:prefLabel "carbonatitic volcaniclastic conglomerate"@en ;
.

:carbonatitic-volcaniclastic-granule-pebble-breccia
    a skos:Concept ;
    rdfs:isDefinedBy cs: ;
    skos:broader :igneous-carbonatite ;
    skos:definition "A breccia composed mostly of angular fragments ranging in size from granule (2–4 mm) to pebble (4–32 mm) consisting of either (a) pyroclastic detritus or (b) terrigenous volcanic detritus of epiclastic origin, and with more than 50% modal carbonates. 'Volcaniclastic' includes all clastic volcanic materials formed by any process of fragmentation, dispersed by any kind of transporting agent, deposited in any environment, or mixed in any significant portion with non-volcanic fragments."@en ;
    skos:historyNote "Compiled by the Geological Survey of Western Australia" ;
    skos:inScheme cs: ;
    skos:notation "rvg"^^:gswa-rock-code ;
    skos:prefLabel "carbonatitic volcaniclastic granule/pebble breccia"@en ;
.

:carbonatitic-volcaniclastic-mudstone
    a skos:Concept ;
    rdfs:isDefinedBy cs: ;
    skos:broader :igneous-carbonatite ;
    skos:definition "A mudstone (grain size ranging from silt to clay (i.e. less than 0.0625 mm) consisting of either (a) pyroclastic detritus or (b) terrigenous volcanic detritus of epiclastic origin, and with more than 50% modal carbonates. 'Volcaniclastic' includes all clastic volcanic materials formed by any process of fragmentation, dispersed by any kind of transporting agent, deposited in any environment, or mixed in any significant portion with non-volcanic fragments."@en ;
    skos:historyNote "Compiled by the Geological Survey of Western Australia" ;
    skos:inScheme cs: ;
    skos:notation "rvsm"^^:gswa-rock-code ;
    skos:prefLabel "carbonatitic volcaniclastic mudstone"@en ;
.

:carbonatitic-volcaniclastic-rock
    a skos:Concept ;
    rdfs:isDefinedBy cs: ;
    skos:broader :igneous-carbonatite ;
    skos:definition "A volcaniclastic rock consisting of either (a) pyroclastic detritus or (b) terrigenous volcanic detritus of epiclastic origin and with more than 50% modal carbonates, but otherwise uncategorized. 'Volcaniclastic' includes all clastic volcanic materials formed by any process of fragmentation, dispersed by any kind of transporting agent, deposited in any environment, or mixed in any significant portion with non-volcanic fragments."@en ;
    skos:historyNote "Compiled by the Geological Survey of Western Australia" ;
    skos:inScheme cs: ;
    skos:notation "rvr"^^:gswa-rock-code ;
    skos:prefLabel "carbonatitic volcaniclastic rock"@en ;
.

:carbonatitic-volcaniclastic-sandstone
    a skos:Concept ;
    rdfs:isDefinedBy cs: ;
    skos:broader :igneous-carbonatite ;
    skos:definition "A sandstone (grain size 0.0625 – 2 mm) consisting of either (a) pyroclastic detritus or (b) terrigenous volcanic detritus of epiclastic origin, and with more than 50% modal carbonates. 'Volcaniclastic' includes all clastic volcanic materials formed by any process of fragmentation, dispersed by any kind of transporting agent, deposited in any environment, or mixed in any significant portion with non-volcanic fragments."@en ;
    skos:historyNote "Compiled by the Geological Survey of Western Australia" ;
    skos:inScheme cs: ;
    skos:notation "rvs"^^:gswa-rock-code ;
    skos:prefLabel "carbonatitic volcaniclastic sandstone"@en ;
.

:carbonatitic-volcaniclastic-sandstone-siltstone
    a skos:Concept ;
    rdfs:isDefinedBy cs: ;
    skos:broader :igneous-carbonatite ;
    skos:definition "A volcaniclastic rock composed mostly of fragments ranging in size from sand (0.0625 – 2 mm) to silt (0.0039 – 0.0625 mm) of either (a) pyroclastic detritus or (b) terrigenous volcanic detritus of epiclastic origin, and with more than 50% modal carbonates. 'Volcaniclastic' includes all clastic volcanic materials formed by any process of fragmentation, dispersed by any kind of transporting agent, deposited in any environment, or mixed in any significant portion with non-volcanic fragments."@en ;
    skos:historyNote "Compiled by the Geological Survey of Western Australia" ;
    skos:inScheme cs: ;
    skos:notation "rvss"^^:gswa-rock-code ;
    skos:prefLabel "carbonatitic volcaniclastic sandstone-siltstone"@en ;
.

:carbonatitic-volcaniclastic-sediment-matrix-breccia
    a skos:Concept ;
    rdfs:isDefinedBy cs: ;
    skos:broader :igneous-carbonatite ;
    skos:definition "A commonly monomictic breccia with more than 50% modal carbonates composed of angular, coarse igneous fragments cemented by a fine-grained matrix that is clastic though not necessarily strictly sedimentary in origin. 'Volcaniclastic' includes all clastic volcanic materials formed by any process of fragmentation, dispersed by any kind of transporting agent, deposited in any environment, or mixed in any significant portion with non-volcanic fragments."@en ;
    skos:historyNote "Compiled by the Geological Survey of Western Australia" ;
    skos:inScheme cs: ;
    skos:notation "rvsb"^^:gswa-rock-code ;
    skos:prefLabel "carbonatitic volcaniclastic sediment-matrix breccia"@en ;
.

:cataclasite
    a skos:Concept ;
    rdfs:isDefinedBy cs: ;
    skos:altLabel "mesocataclasite"@en ;
    skos:broader :metamorphic-protolith-unknown-fault-rock ;
    skos:definition "A cohesive fault rock with a poorly developed or absent schistosity, characterized by generally angular porphyroclasts and lithic fragments in a finer-grained matrix of similar composition that constitutes between 50 and 90% of the rock volume. Definition adapted from Fossen (2016) and Fettes and Desmons (2007, p. 138)."@en ;
    skos:historyNote "Fossen, H 2016, Structural geology (2nd edition): Cambridge University Press, Cambridge, United Kingdom, 524p." ;
    skos:inScheme cs: ;
    skos:notation "myx"^^:gswa-rock-code ;
    skos:prefLabel "cataclasite"@en ;
    schema:citation "https://glossary.americangeosciences.org/term/cataclasite"^^xsd:anyURI ;
.

:chalk
    a skos:Concept ;
    rdfs:isDefinedBy cs: ;
    skos:broader :sedimentary-other-chemical-or-biochemical ;
    skos:definition "A soft, pure, earthy, fine-textured, usually white to light grey or buff limestone of marine origin, consisting almost wholly (90–99%) of calcite, formed mainly by calcareous tests of floating microorganisms (chiefly foraminifers) and of comminuted remains of calcareous algae (such as coccoliths and rhabdoliths), set in a structureless matrix of very finely crystalline calcite. The rock is porous, somewhat friable, and only slightly coherent. It may include the remains of bottom-dwelling organisms (e.g. echinoderms and bivalves), and nodules of chert and pyrite. Adapted from Glossary of geology (5th edition revised; Neuendorf et al., 2011)."@en ;
    skos:exactMatch
        <http://inspire.ec.europa.eu/codelist/LithologyValue/chalk> ,
        <http://resource.geosciml.org/classifier/cgi/lithology/chalk> ;
    skos:historyNote "Based on the Glossary of geology (5th edition, revised; Neuendorf et al. 2011)." ;
    skos:inScheme cs: ;
    skos:notation "ch"^^:gswa-rock-code ;
    skos:prefLabel "chalk"@en ;
    schema:citation "https://glossary.americangeosciences.org/term/chalk"^^xsd:anyURI ;
.

:chemical-or-biochemical-rock
    a skos:Concept ;
    rdfs:isDefinedBy cs: ;
    skos:broader :sedimentary-other-chemical-or-biochemical ;
    skos:definition "A sedimentary rock composed primarily of material formed directly by (a) precipitation from solution or colloidal suspension (as by evaporation), (b) by the deposition of insoluble precipitates (as by mixing solutions of two soluble salts), or (c) resulting directly or indirectly from the chemical processes and activities of living organisms — otherwise uncategorised. It generally has a crystalline texture. Adapted from Glossary of geology (5th edition revised; Neuendorf et al., 2011)."@en ;
    skos:historyNote "Based on the Glossary of geology (5th edition, revised; Neuendorf et al. 2011)." ;
    skos:inScheme cs: ;
    skos:notation "c"^^:gswa-rock-code ;
    skos:prefLabel "chemical or biochemical rock"@en ;
    schema:citation
        "https://glossary.americangeosciences.org/term/biochemicalrock"^^xsd:anyURI ,
        "https://glossary.americangeosciences.org/term/chemicalrock"^^xsd:anyURI ;
.

:chemical-or-biochemical-rock-undivided
    a skos:Concept ;
    rdfs:isDefinedBy cs: ;
    skos:broader :sedimentary-other-chemical-or-biochemical ;
    skos:definition "A sedimentary rock composed primarily of material formed by precipitation from solution or colloidal suspension, by the deposition of insoluble precipitates, or resulting from the chemical processes and activities of living organisms — otherwise uncategorized. Adapted from Glossary of geology (5th edition revised; Neuendorf et al., 2011). GSWA usage of this term is restricted to rocks that are partially weathered or are identified using remote sensing imagery, and the use of the related code/notation is limited to GSWA's Explanatory Notes System."@en ;
    skos:historyNote "Compiled by the Geological Survey of Western Australia" ;
    skos:inScheme cs: ;
    skos:notation "cn"^^:gswa-rock-code ;
    skos:prefLabel "chemical or biochemical rock; undivided"@en ;
    schema:citation
        "https://glossary.americangeosciences.org/term/biochemicalrock"^^xsd:anyURI ,
        "https://glossary.americangeosciences.org/term/chemicalrock"^^xsd:anyURI ;
.

:chert
    a skos:Concept ;
    rdfs:isDefinedBy cs: ;
    skos:altLabel "flint"@en ;
    skos:broader :sedimentary-other-chemical-or-biochemical ;
    skos:definition "A hard, extremely dense or compact, dull to semivitreous, microcrystalline or cryptocrystalline sedimentary rock, consisting dominantly of interlocking crystals of quartz less than about 30 μm in diameter; it may contain amorphous silica (opal) or cryptocrystalline quartz (chalcedony). It sometimes contains impurities such as calcite, iron oxide, and the remains of siliceous and other organisms. It has a tough, splintery to conchoidal fracture, and may be white or variously coloured grey, green, blue, pink, red, yellow, brown, and black. Chert occurs principally as nodular or concretionary segregations (chert nodules) in limestones and dolomites, and as areally extensive layered deposits (bedded chert ); it may be an original organic or inorganic precipitate or a replacement product. The term flint is essentially synonymous, although it has been used for the dark variety of chert. Adapted from Glossary of geology (5th edition revised; Neuendorf et al., 2011)."@en ;
    skos:historyNote "Based on the Glossary of geology (5th edition, revised; Neuendorf et al. 2011)." ;
    skos:inScheme cs: ;
    skos:notation "cc"^^:gswa-rock-code ;
    skos:prefLabel "chert"@en ;
    schema:citation "https://glossary.americangeosciences.org/term/chert"^^xsd:anyURI ;
.

:chloritic-fault-rock
    a skos:Concept ;
    rdfs:isDefinedBy cs: ;
    skos:broader :metamorphic-protolith-unknown-fault-rock ;
    skos:definition "A rock formed as a result of deformation in a fault zone and distinguished by the abundance of chlorite minerals. In GSWA usage, this term is reserved for fault rocks for which a protolith cannot be conclusively established."@en ;
    skos:historyNote "Compiled by the Geological Survey of Western Australia" ;
    skos:inScheme cs: ;
    skos:notation "myc"^^:gswa-rock-code ;
    skos:prefLabel "chloritic fault rock"@en ;
.

:chloritic-gneiss
    a skos:Concept ;
    rdfs:isDefinedBy cs: ;
    skos:broader :metamorphic-protolith-unknown-gneiss ;
    skos:definition "A gneiss distinguished by the abundance of chlorite minerals. In GSWA usage, this term is reserved for a gneiss for which a protolith cannot be conclusively established. See also definition of gneiss/gneissose structure in Fettes and Desmons (2007, p. 154–155)."@en ;
    skos:historyNote "Based on the IUGS classification of metamorphic rocks (Fettes and Desmons, 2007) and GSWA usage." ;
    skos:inScheme cs: ;
    skos:notation "mnc"^^:gswa-rock-code ;
    skos:prefLabel "chloritic gneiss"@en ;
    schema:citation "https://glossary.americangeosciences.org/term/gneiss"^^xsd:anyURI ;
.

:chloritic-granofels-hornfels
    a skos:Concept ;
    rdfs:isDefinedBy cs: ;
    skos:broader :metamorphic-protolith-unknown-granofels-hornfels ;
    skos:definition "A granofels/hornfels distinguished by the abundance of chlorite minerals. In GSWA usage, this term is reserved for a granofels/hornfels for which a protolith cannot be conclusively established."@en ;
    skos:historyNote "Compiled by the Geological Survey of Western Australia" ;
    skos:inScheme cs: ;
    skos:notation "mec"^^:gswa-rock-code ;
    skos:prefLabel "chloritic granofels/hornfels"@en ;
.

:chloritic-schist
    a skos:Concept ;
    rdfs:isDefinedBy cs: ;
    skos:broader :metamorphic-protolith-unknown-schist ;
    skos:definition "A schist distinguished by the abundance of chlorite minerals. In GSWA usage, this term is reserved for a schist for which a protolith cannot be conclusively established. See also definition of schist/schistose structure in Fettes and Desmons, 2007, p. 193)."@en ;
    skos:historyNote "Based on the IUGS classification of metamorphic rocks (Fettes and Desmons, 2007) and GSWA usage." ;
    skos:inScheme cs: ;
    skos:notation "msc"^^:gswa-rock-code ;
    skos:prefLabel "chloritic schist"@en ;
.

:chromitite
    a skos:Concept ;
    rdfs:isDefinedBy cs: ;
    skos:broader :igneous-ultramafic-intrusive ;
    skos:definition "An ultramafic rock consisting essentially of chromite (Le Maitre et al., 2005, p. 69)."@en ;
    skos:historyNote "Based on the IUGS classification of igneous rocks (Le Maitre et al., 2005)." ;
    skos:inScheme cs: ;
    skos:notation "ac"^^:gswa-rock-code ;
    skos:prefLabel "chromitite"@en ;
.

:claystone
    a skos:Concept ;
    rdfs:isDefinedBy cs: ;
    skos:altLabel "argillite"@en ;
    skos:broader :mudstone ;
    skos:definition "An indurated mud with 66% or more clay-sized minerals, and the composition of shale but lacking its fine lamination or fissility; a massive mudstone in which clay predominates over silt; a nonfissile clay shale. Adapted from Glossary of geology (5th edition revised; Neuendorf et al., 2011)."@en ;
    skos:exactMatch
        <http://inspire.ec.europa.eu/codelist/LithologyValue/claystone> ,
        <http://resource.geosciml.org/classifier/cgi/lithology/claystone> ;
    skos:historyNote "Pettijohn, FJ 1957, Sedimentary rocks, Harper and Brothers, New York, 718p." ;
    skos:inScheme cs: ;
    skos:notation "sly"^^:gswa-rock-code ;
    skos:prefLabel "claystone"@en ;
    schema:citation "https://glossary.americangeosciences.org/term/claystonesed"^^xsd:anyURI ;
.

:clinopyroxene-gabbro
    a skos:Concept ;
    rdfs:isDefinedBy cs: ;
    skos:broader :igneous-mafic-intrusive ;
    skos:definition "A gabbro sensu strictu, i.e. a mafic intrusive rock (or the coarse-grained part of an extrusive succession) defined modally in QAPF field 10 (Fig. 2.4, p. 22) and consisting of plagioclase more calcic than An50 and clinopyroxene (augite), with less than 5% each of olivine and orthopyroxene in its mode (cf. Le Maitre et al., 2005, p. 24–25)."@en ;
    skos:historyNote "Based on the IUGS classification of igneous rocks (Le Maitre et al., 2005)." ;
    skos:inScheme cs: ;
    skos:notation "oc"^^:gswa-rock-code ;
    skos:prefLabel "clinopyroxene gabbro"@en ;
.

:clinopyroxenite
    a skos:Concept ;
    rdfs:isDefinedBy cs: ;
    skos:broader :igneous-ultramafic-intrusive ;
    skos:definition "An ultramafic intrusive rock consisting almost entirely of clinopyroxene. Now defined modally in the ultramafic rock classification (Fig. 2.9, p. 28). (cf. Le Maitre et al., 2005, p. 69)"@en ;
    skos:historyNote "Based on the IUGS classification of igneous rocks (Le Maitre et al., 2005)." ;
    skos:inScheme cs: ;
    skos:notation "axc"^^:gswa-rock-code ;
    skos:prefLabel "clinopyroxenite"@en ;
    schema:citation "https://glossary.americangeosciences.org/term/clinopyroxenite"^^xsd:anyURI ;
.

:cobble-conglomerate
    a skos:Concept ;
    rdfs:isDefinedBy cs: ;
    skos:altLabel "cobblestone"@en ;
    skos:broader :conglomerate ;
    skos:definition "A consolidated rock consisting mainly of cobbles (64–256 mm or -4 to -8  phi units) being somewhat rounded or otherwise modified by abrasion in the course of transport. Adapted from Glossary of geology (5th edition revised; Neuendorf et al., 2011)."@en ;
    skos:historyNote "Wentworth, CK 1922, A scale of grade and class terms for clastic sediments: The Journal of Geology, v. 30, no. 5, p. 377–392, doi:10.1086/622910." ;
    skos:inScheme cs: ;
    skos:notation "so"^^:gswa-rock-code ;
    skos:prefLabel "cobble conglomerate"@en ;
    schema:citation
        "https://glossary.americangeosciences.org/term/cobbleconglomerate"^^xsd:anyURI ,
        "https://glossary.americangeosciences.org/term/cobblepartsize"^^xsd:anyURI ;
.

:conglomerate-plus-sandstone
    a skos:Concept ;
    rdfs:isDefinedBy cs: ;
    skos:broader :sedimentary-siliciclastic ;
    skos:definition "Conglomerate and sandstone beds/intervals interleaved at outcrop scale."@en ;
    skos:historyNote "Compiled by the Geological Survey of Western Australia" ;
    skos:inScheme cs: ;
    skos:notation "sg"^^:gswa-rock-code ;
    skos:prefLabel "conglomerate + sandstone"@en ;
.

:conglomerate-with-other-siliciclastic-rock
    a skos:Concept ;
    rdfs:isDefinedBy cs: ;
    skos:broader :sedimentary-siliciclastic ;
    skos:definition "Conglomerate interleaved with other siliciclastic rocks/beds/intervals at outcrop scale."@en ;
    skos:historyNote "Compiled by the Geological Survey of Western Australia" ;
    skos:inScheme cs: ;
    skos:notation "sm"^^:gswa-rock-code ;
    skos:prefLabel "conglomerate + other siliciclastic rock"@en ;
.

:coquina
    a skos:Concept ;
    rdfs:isDefinedBy cs: ;
    skos:altLabel
        "coquinite"@en ,
        "coquinoid limestone"@en ,
        "microcoquina"@en ;
    skos:broader :limestone ;
    skos:definition "A detrital limestone composed wholly or chiefly of mechanically sorted fossil debris that experienced abrasion and transport before reaching the depositional site. The term is derived from the Spanish word for \"cockle\" and \"shellfish\". Adapted from Glossary of geology (5th edition revised; Neuendorf et al., 2011)."@en ;
    skos:historyNote "Based on the Glossary of geology (5th edition, revised; Neuendorf et al. 2011)." ;
    skos:inScheme cs: ;
    skos:notation "klq"^^:gswa-rock-code ;
    skos:prefLabel "coquina"@en ;
    schema:citation
        "https://en.wikipedia.org/wiki/Coquina"^^xsd:anyURI ,
        "https://glossary.americangeosciences.org/term/coquina"^^xsd:anyURI ;
.

:crush-breccia
    a skos:Concept ;
    rdfs:isDefinedBy cs: ;
    skos:broader :metamorphic-protolith-unknown-fault-rock ;
    skos:definition "A cohesive fault breccia formed by deformation that caused the fragmentation of the rock in place or nearly in place. In the classification of Fossen (2016) crush breccia specifically refers to occurrences where fragments are larger than 5 mm; GSWA usage of the term is for rocks of unknown protolith, and includes 'fine crush breccia' (fragments between 1 and 5 mm) and 'crush microbreccia' (fragments less than 1 mm). Crush breccias have less than 10% matrix and fragments are usually glued together by cement (typically quartz or calcite) and/or microfragments of minerals that have been crushed during faulting. Adapted from Fossen (2016) and Fettes and Desmons (2007, p. 143)."@en ;
    skos:historyNote "Fossen, H 2016, Structural geology (2nd edition): Cambridge University Press, Cambridge, United Kingdom, 524p." ;
    skos:inScheme cs: ;
    skos:notation "myh"^^:gswa-rock-code ;
    skos:prefLabel "crush breccia"@en ;
    schema:citation "https://glossary.americangeosciences.org/term/crushbreccia"^^xsd:anyURI ;
.

:crystalline-dolomite
    a skos:Concept ;
    rdfs:isDefinedBy cs: ;
    skos:altLabel "crystalline dolostone"@en ;
    skos:broader :dolomite ;
    skos:definition "A dolomitic sedimentary rock in which the depositional texture is not recognizable, owing to recrystallization and replacement. Adapted from Glossary of geology (5th edition revised; Neuendorf et al., 2011)."@en ;
    skos:historyNote "Compiled by the Geological Survey of Western Australia" ;
    skos:inScheme cs: ;
    skos:notation "kdc"^^:gswa-rock-code ;
    skos:prefLabel "crystalline dolomite"@en ;
    schema:citation "https://glossary.americangeosciences.org/term/crystallinecarbonate"^^xsd:anyURI ;
.

:crystalline-limestone
    a skos:Concept ;
    rdfs:isDefinedBy cs: ;
    skos:broader :limestone ;
    skos:definition "A calcitic sedimentary rock in which the depositional texture is not recognizable, owing to recrystallization and replacement. Adapted from Glossary of geology (5th edition revised; Neuendorf et al., 2011)."@en ;
    skos:historyNote "Compiled by the Geological Survey of Western Australia" ;
    skos:inScheme cs: ;
    skos:notation "klc"^^:gswa-rock-code ;
    skos:prefLabel "crystalline limestone"@en ;
    schema:citation "https://glossary.americangeosciences.org/term/crystallinecarbonate"^^xsd:anyURI ;
.

:dacite
    a skos:Concept ;
    rdfs:isDefinedBy cs: ;
    skos:broader :igneous-felsic-volcanic ;
    skos:definition "A volcanic rock composed of quartz and sodic plagioclase with minor amounts of biotite and/or hornblende and/or pyroxene. The volcanic equivalent of granodiorite and tonalite. Now defined modally in QAPF fields 4 and 5 (Fig. 2.11, p. 31) and, if modes are not available, chemically in TAS field O3 (Fig. 2.14, p. 35). Definition from Le Maitre et al. (2005, p. 72). GSWA's rock classification scheme prefers the use of volcanic terminology for any igneous rock formed on or near the Earth's surface, i.e. for those hypabyssal or subvolcanic rocks such as dykes, sills, and cryptodomes that are demonstrably both spatially and temporally associated with extrusive volcanic rocks."@en ;
    skos:exactMatch
        <http://inspire.ec.europa.eu/codelist/LithologyValue/dacite> ,
        <http://resource.geosciml.org/classifier/cgi/lithology/dacite> ;
    skos:historyNote "Based on the IUGS classification of igneous rocks (Le Maitre et al., 2005)." ;
    skos:inScheme cs: ;
    skos:notation "fd"^^:gswa-rock-code ;
    skos:prefLabel "dacite"@en ;
    schema:citation "https://glossary.americangeosciences.org/term/dacite"^^xsd:anyURI ;
.

:diamictite
    a skos:Concept ;
    rdfs:isDefinedBy cs: ;
    skos:altLabel
        "diamicton"@en ,
        "mixtite"@en ,
        "pebbly mudstone"@en ,
        "puddingstone"@en ;
    skos:broader :sedimentary-siliciclastic ;
    skos:definition "A comprehensive, nongenetic term for an unsorted or poorly sorted, noncalcareous, terrigenous sedimentary rock that contains a wide range of particle sizes, such as a rock with sand and/or larger particles in a muddy matrix; e.g. a tillite or a pebbly mudstone. Adapted from Glossary of geology (5th edition revised; Neuendorf et al., 2011)."@en ;
    skos:exactMatch
        <http://inspire.ec.europa.eu/codelist/LithologyValue/diamictite> ,
        <http://resource.geosciml.org/classifier/cgi/lithology/diamictite> ;
    skos:inScheme cs: ;
    skos:notation "sd"^^:gswa-rock-code ;
    skos:prefLabel "diamictite"@en ;
    schema:citation "https://glossary.americangeosciences.org/term/diamictite"^^xsd:anyURI ;
.

:diamictite-with-other-siliciclastic
    a skos:Concept ;
    rdfs:isDefinedBy cs: ;
    skos:broader :sedimentary-siliciclastic ;
    skos:definition "Diamictite and other siliciclastic rocks/beds/intervals interleaved at outcrop scale."@en ;
    skos:historyNote "Compiled by the Geological Survey of Western Australia" ;
    skos:inScheme cs: ;
    skos:notation "se"^^:gswa-rock-code ;
    skos:prefLabel "diamictite + other siliciclastic"@en ;
.

:diatomite
    a skos:Concept ;
    rdfs:isDefinedBy cs: ;
    skos:altLabel "diatomaceous earth"@en ;
    skos:broader :sedimentary-other-chemical-or-biochemical ;
    skos:definition "A light-coloured, soft, friable, siliceous sedimentary rock, consisting chiefly of opaline diatom frustules, typically white, but also pale yellow, grey, or tan. Its low density enables it to float on water. Some deposits are of lake origin but the largest are marine, and the term is generally reserved for deposits of actual or potential commercial value. Adapted from Glossary of geology (5th edition revised; Neuendorf et al., 2011)."@en ;
    skos:historyNote "Based on the Glossary of geology (5th edition, revised; Neuendorf et al. 2011)." ;
    skos:inScheme cs: ;
    skos:notation "cd"^^:gswa-rock-code ;
    skos:prefLabel "diatomite"@en ;
    schema:citation "https://glossary.americangeosciences.org/term/diatomite"^^xsd:anyURI ;
.

:diopside-leucite-lamproite
    a skos:Concept ;
    rdfs:isDefinedBy cs: ;
    skos:broader :igneous-lamproites ;
    skos:definition "A melanocratic diopside–leucite lamproite (Table 2.7, p. 17) essentially composed of leucite and diopside with minor olivine pseudomorphs, amphibole, phlogopite and rutile. The original name cedricite is not recommended for usage. Adapted from Le Maitre et al. (2005, p. 68)."@en ;
    skos:historyNote "Based on the IUGS classification of igneous rocks (Le Maitre et al., 2005)." ;
    skos:inScheme cs: ;
    skos:notation "ic"^^:gswa-rock-code ;
    skos:prefLabel "diopside-leucite lamproite"@en ;
    schema:citation "https://glossary.americangeosciences.org/term/cedricite"^^xsd:anyURI ;
.

:diopside-leucite-phlogopite-lamproite
    a skos:Concept ;
    rdfs:isDefinedBy cs: ;
    skos:broader :igneous-lamproites ;
    skos:definition "Originally described as a variety of leucitite composed of clinopyroxene, mica and leucite in a glassy matrix. Diopside madupitic lamproite (term preferred to 'madupite') is a more mafic variety. Now regarded as a diopside-leucite-phlogopite lamproite (Table 2.7, p. 17). The original name wyomingite is not recommended for usage. Adapted from Le Maitre et al. (2005, p. 157)."@en ;
    skos:historyNote "Based on the IUGS classification of igneous rocks (Le Maitre et al., 2005)." ;
    skos:inScheme cs: ;
    skos:notation "iy"^^:gswa-rock-code ;
    skos:prefLabel "diopside-leucite-phlogopite lamproite"@en ;
    schema:citation "https://glossary.americangeosciences.org/term/wyomingite"^^xsd:anyURI ;
.

:diopside-leucite-richterite-madupitic-lamproite
    a skos:Concept ;
    rdfs:isDefinedBy cs: ;
    skos:altLabel "diopside-leucite-richterite-phlogopite lamproite"@en ;
    skos:broader :igneous-lamproites ;
    skos:definition "A name for a rock largely composed of leucite, mica and amphibole with subordinate clinopyroxene in a serpentine-rich matrix. Now regarded as a diopside–leucite–richterite madupitic lamproite (Table 2.7, p. 17), with the term 'madupitic' referring to the presence of poikilitic groundmass phlogopite. The original name wolgidite is not recommended for usage. Adapted from Le Maitre et al. (2005, p. 157)."@en ;
    skos:historyNote "Based on the IUGS classification of igneous rocks (Le Maitre et al., 2005)." ;
    skos:inScheme cs: ;
    skos:notation "iw"^^:gswa-rock-code ;
    skos:prefLabel "diopside-leucite-richterite madupitic lamproite"@en ;
    schema:citation "https://glossary.americangeosciences.org/term/wolgidite"^^xsd:anyURI ;
.

:diopside-madupitic-lamproite
    a skos:Concept ;
    rdfs:isDefinedBy cs: ;
    skos:altLabel "diopside-phlogopite lamproite"@en ;
    skos:broader :igneous-lamproites ;
    skos:definition "Originally described as a melanocratic variety of leucitite essentially composed of diopside and phlogopite in a glassy matrix, which has the composition of nepheline and leucite. Wyomingite is a more felsic variety. Now regarded as a diopside madupitic lamproite (Table 2.7, p. 17), with the term 'madupitic' referring to the presence of poikilitic groundmass phlogopite. The original name madupite is not recommended for usage. Adapted from Le Maitre et al. (2005, p. 107)."@en ;
    skos:historyNote "Based on the IUGS classification of igneous rocks (Le Maitre et al., 2005)." ;
    skos:inScheme cs: ;
    skos:notation "im"^^:gswa-rock-code ;
    skos:prefLabel "diopside madupitic lamproite"@en ;
    schema:citation "https://glossary.americangeosciences.org/term/madupite"^^xsd:anyURI ;
.

:diopside-sanidine-phlogopite-lamproite
    a skos:Concept ;
    rdfs:isDefinedBy cs: ;
    skos:broader :igneous-lamproites ;
    skos:definition "Originally described as a variety of leucite phonolite essentially composed of leucite and alkali feldspar with subordinate clinopyroxene, mica and amphibole. Now regarded as a diopside–sanidine–phlogopite lamproite (Table 2.7, p. 17). The original name orendite is not recommended for usage. (Le Maitre et al., 2005, p. 121)"@en ;
    skos:historyNote "Based on the IUGS classification of igneous rocks (Le Maitre et al., 2005)." ;
    skos:inScheme cs: ;
    skos:notation "io"^^:gswa-rock-code ;
    skos:prefLabel "diopside-sanidine-phlogopite lamproite"@en ;
    schema:citation "https://glossary.americangeosciences.org/term/orendite"^^xsd:anyURI ;
.

:diorite
    a skos:Concept ;
    rdfs:isDefinedBy cs: ;
    skos:broader :igneous-felsic-intrusive ;
    skos:definition "An intrusive rock consisting of intermediate plagioclase, commonly with hornblende and often with biotite or augite. Now defined modally in QAPF field 10 (Fig. 2.4, p. 22). (cf. Le Maitre et al., 2005, p. 73)."@en ;
    skos:exactMatch
        <http://inspire.ec.europa.eu/codelist/LithologyValue/diorite> ,
        <http://resource.geosciml.org/classifier/cgi/lithology/diorite> ;
    skos:historyNote "Based on the IUGS classification of igneous rocks (Le Maitre et al., 2005)." ;
    skos:inScheme cs: ;
    skos:notation "gi"^^:gswa-rock-code ;
    skos:prefLabel "diorite"@en ;
    schema:citation "https://glossary.americangeosciences.org/term/diorite"^^xsd:anyURI ;
.

:dolarenite
    a skos:Concept ;
    rdfs:isDefinedBy cs: ;
    skos:altLabel "dolomitic sandstone"@en ;
    skos:broader :dolomite ;
    skos:definition "A dolomite rock consisting predominantly of detrital dolomite particles of sand size (Folk, 1959, p. 16); a consolidated dolomitic sand (Glossary of geology, 5th edition revised; Neuendorf et al., 2011)."@en ;
    skos:historyNote "Folk, RL 1959, Practical petrographic classification of limestones: American Association of Petroleum Geologists Bulletin No. 43(1), p. 1–38, doi:10.1306/0BDA5C36-16BD-11D7-8645000102C1865D." ;
    skos:inScheme cs: ;
    skos:notation "kda"^^:gswa-rock-code ;
    skos:prefLabel "dolarenite"@en ;
    schema:citation "https://glossary.americangeosciences.org/term/dolarenite"^^xsd:anyURI ;
.

:dolerite
    a skos:Concept ;
    rdfs:isDefinedBy cs: ;
    skos:broader :igneous-mafic-intrusive ;
    skos:definition "A rock intermediate in grain size between basalt and gabbro and composed essentially of plagioclase, pyroxene and opaque minerals; often with ophitic texture. If olivine is present the rock may be called olivine dolerite; if quartz is present, quartz dolerite. Now regarded as being synonymous with diabase and an approved synonym for microgabbro of QAPF field 10 (Fig. 2.4, p. 22). (Le Maitre et al., 2005, p. 74)."@en ;
    skos:historyNote "Based on the IUGS classification of igneous rocks (Le Maitre et al., 2005)." ;
    skos:inScheme cs: ;
    skos:notation "od"^^:gswa-rock-code ;
    skos:prefLabel "dolerite"@en ;
    schema:citation "https://glossary.americangeosciences.org/term/dolerite"^^xsd:anyURI ;
.

:dolobafflestone
    a skos:Concept ;
    rdfs:isDefinedBy cs: ;
    skos:altLabel "dolomite bafflestone"@en ;
    skos:broader :doloboundstone ;
    skos:definition "A type of reef rock or boundstone composed of upright, branching colonies, closely to widely spaced but not in contact, separated by fine sediment or coarse skeletal debris, and in which dolomite is prevalent over other carbonate minerals. In life, the colonies functioned as a sediment trap or baffle. Adapted from Glossary of geology (5th edition revised; Neuendorf et al., 2011)."@en ;
    skos:historyNote """Dunham, RJ 1962, Classification of carbonate rocks according to depositional texture, in Classification of carbonate rocks edited by WE Hamm: American Association of Petroleum Geologists, Tulsa, Oklahoma, USA, p. 108–121.,
Embry, AF, Klovan, JE 1971, A late Devonian reef tract on northeastern Banks Island, N.W.T: Bulletin of Canadian Petroleum Geology, v. 19(4), p. 730–781.""" ;
    skos:inScheme cs: ;
    skos:notation "kdj"^^:gswa-rock-code ;
    skos:prefLabel "dolobafflestone"@en ;
    schema:citation "https://glossary.americangeosciences.org/term/bafflestone"^^xsd:anyURI ;
.

:dolobindstone
    a skos:Concept ;
    rdfs:isDefinedBy cs: ;
    skos:altLabel "dolomite bindstone"@en ;
    skos:broader :doloboundstone ;
    skos:definition "A type of reef rock or boundstone composed of sheet-like colonies encrusting large fossil fragments or finer sediment, forming a layered mass that is partly in-place skeletal and partly bioclastic, and in which dolomite is prevalent over other carbonate minerals. Adapted from Glossary of geology (5th edition revised; Neuendorf et al., 2011)."@en ;
    skos:historyNote """Dunham, RJ 1962, Classification of carbonate rocks according to depositional texture, in Classification of carbonate rocks edited by WE Hamm: American Association of Petroleum Geologists, Tulsa, Oklahoma, USA, p. 108–121.,
Embry, AF, Klovan, JE 1971, A late Devonian reef tract on northeastern Banks Island, N.W.T: Bulletin of Canadian Petroleum Geology, v. 19(4), p. 730–781.""" ;
    skos:inScheme cs: ;
    skos:notation "kdi"^^:gswa-rock-code ;
    skos:prefLabel "dolobindstone"@en ;
    schema:citation "https://glossary.americangeosciences.org/term/bindstone"^^xsd:anyURI ;
.

:dolobreccia
    a skos:Concept ;
    rdfs:isDefinedBy cs: ;
    skos:altLabel "dolomite breccia"@en ;
    skos:broader :dolomite ;
    skos:definition "A sedimentary breccia consisting of dolomite clasts and carbonate cement."@en ;
    skos:historyNote "Compiled by the Geological Survey of Western Australia" ;
    skos:inScheme cs: ;
    skos:notation "kdx"^^:gswa-rock-code ;
    skos:prefLabel "dolobreccia"@en ;
.

:dolofloatstone
    a skos:Concept ;
    rdfs:isDefinedBy cs: ;
    skos:altLabel "dolomite floatstone"@en ;
    skos:broader :dolomite ;
    skos:definition "A carbonate rock with dolomite prevalent over calcite and containing a few bioclasts or other fragments more than 2 mm in diameter, widely spaced, embedded in sand- or mud-size carbonate sediment that forms over 90% of the rock. Adapted from Glossary of geology (5th edition revised; Neuendorf et al., 2011)."@en ;
    skos:historyNote """Dunham, RJ 1962, Classification of carbonate rocks according to depositional texture, in Classification of carbonate rocks edited by WE Hamm: American Association of Petroleum Geologists, Tulsa, Oklahoma, USA, p. 108–121.,
Embry, AF, Klovan, JE 1971, A late Devonian reef tract on northeastern Banks Island, N.W.T: Bulletin of Canadian Petroleum Geology, v. 19(4), p. 730–781.""" ;
    skos:inScheme cs: ;
    skos:notation "kdf"^^:gswa-rock-code ;
    skos:prefLabel "dolofloatstone"@en ;
    schema:citation "https://glossary.americangeosciences.org/term/floatstonesed"^^xsd:anyURI ;
.

:doloframestone
    a skos:Concept ;
    rdfs:isDefinedBy cs: ;
    skos:altLabel "dolomite framestone"@en ;
    skos:broadMatch
        <http://inspire.ec.europa.eu/codelist/LithologyValue/framestone> ,
        <http://resource.geosciml.org/classifier/cgi/lithology/framestone> ;
    skos:broader :doloboundstone ;
    skos:definition "A type of reef rock or boundstone consisting of colonies, shells, or skeletons attached to each other to form a rigid framework or lattice, and consisting mostly of dolomite. Internal cavities are filled with fine sediment, crystalline cement, or coarse skeletal debris. Adapted from Glossary of geology (5th edition revised; Neuendorf et al., 2011)."@en ;
    skos:historyNote """Dunham, RJ 1962, Classification of carbonate rocks according to depositional texture, in Classification of carbonate rocks edited by WE Hamm: American Association of Petroleum Geologists, Tulsa, Oklahoma, USA, p. 108–121.,
Embry, AF, Klovan, JE 1971, A late Devonian reef tract on northeastern Banks Island, N.W.T: Bulletin of Canadian Petroleum Geology, v. 19(4), p. 730–781.""" ;
    skos:inScheme cs: ;
    skos:notation "kde"^^:gswa-rock-code ;
    skos:prefLabel "doloframestone"@en ;
    schema:citation "https://glossary.americangeosciences.org/term/framestone"^^xsd:anyURI ;
.

:dolograinstone
    a skos:Concept ;
    rdfs:isDefinedBy cs: ;
    skos:altLabel "dolomite grainstone"@en ;
    skos:broadMatch
        <http://inspire.ec.europa.eu/codelist/LithologyValue/grainstone> ,
        <http://resource.geosciml.org/classifier/cgi/lithology/grainstone> ;
    skos:broader :dolomite ;
    skos:definition "A mud-free (less than 1% of material with diameters less than 20 μm), grain-supported, carbonate sedimentary rock, with dolomite prevalent over calcite. It may be current-laid or formed by mud being washed out from previously deposited sediment, or it may result from mud being bypassed while locally produced particles accumulated (Dunham, 1962). Adapted from Glossary of geology (5th edition revised; Neuendorf et al., 2011)."@en ;
    skos:historyNote """Dunham, RJ 1962, Classification of carbonate rocks according to depositional texture, in Classification of carbonate rocks edited by WE Hamm: American Association of Petroleum Geologists, Tulsa, Oklahoma, USA, p. 108–121.,
Embry, AF, Klovan, JE 1971, A late Devonian reef tract on northeastern Banks Island, N.W.T: Bulletin of Canadian Petroleum Geology, v. 19(4), p. 730–781.""" ;
    skos:inScheme cs: ;
    skos:notation "kdg"^^:gswa-rock-code ;
    skos:prefLabel "dolograinstone"@en ;
    schema:citation "https://glossary.americangeosciences.org/term/grainstone"^^xsd:anyURI ;
.

:dololutite
    a skos:Concept ;
    rdfs:isDefinedBy cs: ;
    skos:altLabel "dolosiltite"@en ;
    skos:broader :dolomite ;
    skos:definition "A dolomitic rock consisting predominantly of detrital dolomite particles of silt and/or clay size (Folk, 1959, p. 16); a consolidated dolomitic mud. It is commonly interlayered with dense primary dolomites in evaporitic sequences. Adapted from Glossary of geology (5th edition revised; Neuendorf et al., 2011)."@en ;
    skos:historyNote """Grabau, AW 1903, Paleozoic coral reefs: Geological Society of America Bulletin, v. 14, p. 337–352.,
Folk, RL , 1959, Practical petrographic classification of limestones: American Association of Petroleum Geologists Bulletin No. 43(1), p. 1–38, doi:10.1306/0BDA5C36-16BD-11D7-8645000102C1865D.""" ;
    skos:inScheme cs: ;
    skos:notation "kdl"^^:gswa-rock-code ;
    skos:prefLabel "dololutite"@en ;
    schema:citation "https://glossary.americangeosciences.org/term/dololutite"^^xsd:anyURI ;
.

:dolomite-carbonatite
    a skos:Concept ;
    rdfs:isDefinedBy cs: ;
    skos:altLabel "beforsite"@en ;
    skos:broader :igneous-carbonatite ;
    skos:definition "A variety of carbonatite in which the main carbonate is dolomite (section 2.3, p. 10). A medium- to fine-grained variety of dolomite-carbonatite, often occurring as dykes, may be called beforsite. Adapted from Le Maitre et al. (2005, p. 10, 62 and 74)"@en ;
    skos:historyNote "Based on the IUGS classification of igneous rocks (Le Maitre et al., 2005)." ;
    skos:inScheme cs: ;
    skos:notation "rd"^^:gswa-rock-code ;
    skos:prefLabel "dolomite-carbonatite"@en ;
    schema:citation "https://glossary.americangeosciences.org/term/calcitecarbonatite"^^xsd:anyURI ;
.

:dolomitic-sandstone
    a skos:Concept ;
    rdfs:isDefinedBy cs: ;
    skos:broader :sandstone ;
    skos:definition "A terrigenous sandstone that is cemented with dolomite."@en ;
    skos:historyNote "Compiled by the Geological Survey of Western Australia" ;
    skos:inScheme cs: ;
    skos:notation "stj"^^:gswa-rock-code ;
    skos:prefLabel "dolomitic sandstone"@en ;
    schema:citation "https://glossary.americangeosciences.org/term/dolomitic"^^xsd:anyURI ;
.

:dolomudstone
    a skos:Concept ;
    rdfs:isDefinedBy cs: ;
    skos:altLabel
        "dolomicrite"@en ,
        "dolomite mudstone"@en ;
    skos:broadMatch
        <http://inspire.ec.europa.eu/codelist/LithologyValue/carbonateMudstone> ,
        <http://resource.geosciml.org/classifier/cgi/lithology/carbonate_mudstone> ;
    skos:broader :dolomite ;
    skos:definition "A sedimentary rock consisting of clay-sized dolomite crystals, interpreted as a lithified dolomite mud (analogous to calcite mud or micrite), and containing less than 1% allochems (Folk, 1959, p. 14). Adapted from Glossary of geology (5th edition revised; Neuendorf et al., 2011)."@en ;
    skos:historyNote """Dunham, RJ 1962, Classification of carbonate rocks according to depositional texture, in Classification of carbonate rocks edited by WE Hamm: American Association of Petroleum Geologists, Tulsa, Oklahoma, USA, p. 108–121.,
Embry, AF, Klovan, JE 1971, A late Devonian reef tract on northeastern Banks Island, N.W.T: Bulletin of Canadian Petroleum Geology, v. 19(4), p. 730–781.""" ;
    skos:inScheme cs: ;
    skos:notation "kdu"^^:gswa-rock-code ;
    skos:prefLabel "dolomudstone"@en ;
    schema:citation "https://glossary.americangeosciences.org/term/dolomicrite"^^xsd:anyURI ;
.

:dolopackstone
    a skos:Concept ;
    rdfs:isDefinedBy cs: ;
    skos:altLabel "dolomite packstone"@en ;
    skos:broadMatch
        <http://inspire.ec.europa.eu/codelist/LithologyValue/packstone> ,
        <http://resource.geosciml.org/classifier/cgi/lithology/packstone> ;
    skos:broader :dolomite ;
    skos:definition "A term used for a detrital carbonate rock consisting predominantly of dolomite and whose granular material is arranged in a self-supporting framework, yet also contains some matrix of calcareous mud (Dunham, 1962). Adapted from Glossary of geology (5th edition revised; Neuendorf et al., 2011)."@en ;
    skos:historyNote """Dunham, RJ 1962, Classification of carbonate rocks according to depositional texture, in Classification of carbonate rocks edited by WE Hamm: American Association of Petroleum Geologists, Tulsa, Oklahoma, USA, p. 108–121.,
Embry, AF, Klovan, JE 1971, A late Devonian reef tract on northeastern Banks Island, N.W.T: Bulletin of Canadian Petroleum Geology, v. 19(4), p. 730–781.""" ;
    skos:inScheme cs: ;
    skos:notation "kdp"^^:gswa-rock-code ;
    skos:prefLabel "dolopackstone"@en ;
    schema:citation "https://glossary.americangeosciences.org/term/packstone"^^xsd:anyURI ;
.

:dolorudite
    a skos:Concept ;
    rdfs:isDefinedBy cs: ;
    skos:altLabel "dolomite rudite"@en ;
    skos:broader :dolomite ;
    skos:definition "A carbonate rock consisting predominantly of detrital dolomite particles larger than sand size (Folk, 1959, p. 15); a consolidated dolomitic gravel. Adapted from Glossary of geology (5th edition revised; Neuendorf et al., 2011)."@en ;
    skos:historyNote """Grabau, AW 1903, Paleozoic coral reefs: Geological Society of America Bulletin, v. 14, p. 337–352.,
Folk, RL , 1959, Practical petrographic classification of limestones: American Association of Petroleum Geologists Bulletin No. 43(1), p. 1–38, doi:10.1306/0BDA5C36-16BD-11D7-8645000102C1865D.""" ;
    skos:inScheme cs: ;
    skos:notation "kdr"^^:gswa-rock-code ;
    skos:prefLabel "dolorudite"@en ;
    schema:citation "https://glossary.americangeosciences.org/term/dolorudite"^^xsd:anyURI ;
.

:dolorudstone
    a skos:Concept ;
    rdfs:isDefinedBy cs: ;
    skos:altLabel "dolomite rudstone"@en ;
    skos:broader :dolomite ;
    skos:definition "A carbonate rock consisting predominantly of dolomite and composed of detrital bioclasts or other fragments, over 2 mm in diameter, closely packed, in physical contact; the interstices may be open, or filled with fine carbonate sediment or crystalline cement. Adapted from Glossary of geology (5th edition revised; Neuendorf et al., 2011)."@en ;
    skos:historyNote """Dunham, RJ 1962, Classification of carbonate rocks according to depositional texture, in Classification of carbonate rocks edited by WE Hamm: American Association of Petroleum Geologists, Tulsa, Oklahoma, USA, p. 108–121.,
Embry, AF, Klovan, JE 1971, A late Devonian reef tract on northeastern Banks Island, N.W.T: Bulletin of Canadian Petroleum Geology, v. 19(4), p. 730–781.""" ;
    skos:inScheme cs: ;
    skos:notation "kdd"^^:gswa-rock-code ;
    skos:prefLabel "dolorudstone"@en ;
    schema:citation "https://glossary.americangeosciences.org/term/rudstone"^^xsd:anyURI ;
.

:dolowackestone
    a skos:Concept ;
    rdfs:isDefinedBy cs: ;
    skos:altLabel "dolomite wackestone"@en ;
    skos:broadMatch
        <http://inspire.ec.europa.eu/codelist/LithologyValue/carbonateWackestone> ,
        <http://resource.geosciml.org/classifier/cgi/lithology/carbonate_wackestone> ;
    skos:broader :dolomite ;
    skos:definition "A term for a mud-supported detrital carbonate sedimentary rock consisting predominantly of dolomite and containing more than 10% grains (particles with diameters greater than 20 μm). Adapted from Glossary of geology (5th edition revised; Neuendorf et al., 2011)."@en ;
    skos:historyNote """Dunham, RJ 1962, Classification of carbonate rocks according to depositional texture, in Classification of carbonate rocks edited by WE Hamm: American Association of Petroleum Geologists, Tulsa, Oklahoma, USA, p. 108–121.,
Embry, AF, Klovan, JE 1971, A late Devonian reef tract on northeastern Banks Island, N.W.T: Bulletin of Canadian Petroleum Geology, v. 19(4), p. 730–781.""" ;
    skos:inScheme cs: ;
    skos:notation "kdw"^^:gswa-rock-code ;
    skos:prefLabel "dolowackestone"@en ;
    schema:citation "https://glossary.americangeosciences.org/term/wackestone"^^xsd:anyURI ;
.

:dunite-intrusive
    a skos:Concept ;
    rdfs:isDefinedBy cs: ;
    skos:broader :igneous-ultramafic-intrusive ;
    skos:definition "An ultramafic intrusive rock consisting essentially of olivine. Now defined modally in the ultramafic rock classification (Fig. 2.9, p. 28). (cf. Le Maitre et al., 2005, p. 74)"@en ;
    skos:historyNote "Based on the IUGS classification of igneous rocks (Le Maitre et al., 2005)." ;
    skos:inScheme cs: ;
    skos:notation "ad"^^:gswa-rock-code ;
    skos:prefLabel "dunite (intrusive)"@en ;
    schema:citation "https://glossary.americangeosciences.org/term/dunite"^^xsd:anyURI ;
.

:dunite-volcanic
    a skos:Concept ;
    rdfs:isDefinedBy cs: ;
    skos:broader :igneous-ultramafic-volcanic-and-volcaniclastic ;
    skos:definition "An ultramafic igneous rock consisting essentially of olivine. Now defined modally in the ultramafic rock classification (Fig. 2.9, p. 28). Definition adapted from Le Maitre et al., (2007, p. 74). In GSWA usage, an 'extrusive' dunite is identified as one formed from fractionation within thick bodies of ultramafic volcanic or subvolcanic magmas. GSWA's rock classification scheme prefers the use of volcanic terminology for any igneous rock formed on or near the Earth's surface, i.e. for those hypabyssal or subvolcanic rocks such as dykes, sills, and cryptodomes that are demonstrably both spatially and temporally associated with extrusive volcanic rocks."@en ;
    skos:historyNote "Based on the IUGS classification of igneous rocks (Le Maitre et al., 2005)." ;
    skos:inScheme cs: ;
    skos:notation "uu"^^:gswa-rock-code ;
    skos:prefLabel "dunite (volcanic)"@en ;
    schema:citation "https://glossary.americangeosciences.org/term/dunite"^^xsd:anyURI ;
.

:eclogite
    a skos:Concept ;
    rdfs:isDefinedBy cs: ;
    skos:broader :meta-igneous-mafic ;
    skos:definition "Plagioclase-free metamorphic rock composed of ≥75% volume of omphacite and garnet, both of which are present as major constituents, the amount of neither of them being higher than 75% volume. If either omphacite or garnet is present in an amount ≥75%, the rock name is either garnet omphacite or omphacite garnetite. (Fettes and Desmons, 2007, p. 147)"@en ;
    skos:exactMatch
        <http://inspire.ec.europa.eu/codelist/LithologyValue/eclogite> ,
        <http://resource.geosciml.org/classifier/cgi/lithology/eclogite> ;
    skos:historyNote "Based on the IUGS classification of metamorphic rocks (Fettes and Desmons, 2007)." ;
    skos:inScheme cs: ;
    skos:notation "mwp"^^:gswa-rock-code ;
    skos:prefLabel "eclogite"@en ;
    schema:citation "https://glossary.americangeosciences.org/term/eclogite"^^xsd:anyURI ;
.

:endoskarn
    a skos:Concept ;
    rdfs:isDefinedBy cs: ;
    skos:broader :skarn ;
    skos:definition "The portion of skarn that involves metamorphic, metasomatic, and hybrid mixing effects on the igneous side of the contact between an intrusive body and the country rock. Adapted from Glossary of geology (Neuendorf et al., 5th edition, revised); cf. Fettes and Desmons (2007, p. 148)."@en ;
    skos:historyNote "Einaudi, MT and Burt, DM 1982, Introduction – terminology, classification, and composition of skarn deposits: Economic Geology, v. 77, p. 745–754." ;
    skos:inScheme cs: ;
    skos:notation "mjkn"^^:gswa-rock-code ;
    skos:prefLabel "endoskarn"@en ;
    schema:citation "https://glossary.americangeosciences.org/term/endoskarn"^^xsd:anyURI ;
.

:enstatite-sanidine-phlogopite-lamproite
    a skos:Concept ;
    rdfs:isDefinedBy cs: ;
    skos:broader :igneous-lamproites ;
    skos:definition "A variety of potassic lamproite containing normative olivine but no normative leucite (Table 2.7, p. 17). The original name cancalite is not recommended for usage. Adapted from Le Maitre et al. (2005, p. 67)."@en ;
    skos:historyNote "Based on the IUGS classification of igneous rocks (Le Maitre et al., 2005)." ;
    skos:inScheme cs: ;
    skos:notation "ie"^^:gswa-rock-code ;
    skos:prefLabel "enstatite-sanidine-phlogopite lamproite"@en ;
    schema:citation "https://glossary.americangeosciences.org/term/cancalite"^^xsd:anyURI ;
.

:epidote-vein
    a skos:Concept ;
    rdfs:isDefinedBy cs: ;
    skos:broader :hydrothermal ;
    skos:definition "A rock comprising epidote of pegmatitic or hydrothermal origin, as vein-filling material."@en ;
    skos:historyNote "Compiled by the Geological Survey of Western Australia" ;
    skos:inScheme cs: ;
    skos:notation "zd"^^:gswa-rock-code ;
    skos:prefLabel "epidote vein"@en ;
.

:exoskarn
    a skos:Concept ;
    rdfs:isDefinedBy cs: ;
    skos:broader :skarn ;
    skos:definition "The portion of skarn that involves metamorphic and metasomatic effects on the country-rock (non-intrusive) side of the contact between an intrusive body and the country rock. Adapted from Glossary of geology (Neuendorf et al., 5th edition, revised); cf. Fettes and Desmons (2007, p. 150)."@en ;
    skos:historyNote "Einaudi, MT and Burt, DM 1982, Introduction – terminology, classification, and composition of skarn deposits: Economic Geology, v. 77, p. 745–754." ;
    skos:inScheme cs: ;
    skos:notation "mjko"^^:gswa-rock-code ;
    skos:prefLabel "exoskarn"@en ;
    schema:citation "https://glossary.americangeosciences.org/term/exoskarn"^^xsd:anyURI ;
.

:fault-breccia
    a skos:Concept ;
    rdfs:isDefinedBy cs: ;
    skos:broader :metamorphic-protolith-unknown-fault-rock ;
    skos:definition "A fault rock in which the rock mass consists of greater than 30% visible, angular rock fragments resulting from fracturing and frictional slip along a fault; may be cohesive or incohesive. Adapted from Fossen (2016) and Glossary of geology (5th edition revised; Neuendorf et al., 2011). In GSWA usage, this term is reserved for fault rocks for which a protolith cannot be conclusively established."@en ;
    skos:historyNote "Fossen, H 2016, Structural geology (2nd edition): Cambridge University Press, Cambridge, United Kingdom, 524p." ;
    skos:inScheme cs: ;
    skos:notation "myb"^^:gswa-rock-code ;
    skos:prefLabel "fault breccia"@en ;
    schema:citation "https://glossary.americangeosciences.org/term/faultbreccia"^^xsd:anyURI ;
.

:fault-gouge
    a skos:Concept ;
    rdfs:isDefinedBy cs: ;
    skos:broader :metamorphic-protolith-unknown-fault-rock ;
    skos:definition "An incohesive fault rock with a high matrix–fragment ratio (visible fragments less than 30% of the rock mass), i.e. a strongly ground down version of the original rock. The term is sometimes also used for strongly reworked clay or shale in the core of faults in sedimentary sequences. Adapted from Fossen (2016). In GSWA usage, this term is reserved for fault rocks for which a protolith cannot be conclusively established."@en ;
    skos:historyNote "Fossen, H 2016, Structural geology (2nd edition): Cambridge University Press, Cambridge, United Kingdom, 524p." ;
    skos:inScheme cs: ;
    skos:notation "mye"^^:gswa-rock-code ;
    skos:prefLabel "fault gouge"@en ;
    schema:citation "https://glossary.americangeosciences.org/term/faultgouge"^^xsd:anyURI ;
.

:fault-rock
    a skos:Concept ;
    rdfs:isDefinedBy cs: ;
    skos:broader :metamorphic-protolith-unknown-fault-rock ;
    skos:definition "Rock formed as a result of deformation in a fault zone, i.e. a zone of sheared, crushed or foliated rock, in which numerous small dislocations have occurred, adding up to an appreciable total offset of the undeformed walls. All gradations may occur, from multiple fault planes to single shear zones. (Fettes and Desmons, 2007, p. 151)"@en ;
    skos:historyNote "Based on the IUGS classification of metamorphic rocks (Fettes and Desmons, 2007)." ;
    skos:inScheme cs: ;
    skos:notation "my"^^:gswa-rock-code ;
    skos:prefLabel "fault rock"@en ;
    schema:citation "https://glossary.americangeosciences.org/term/faultrock"^^xsd:anyURI ;
.

:fearenite
    a skos:Concept ;
    rdfs:isDefinedBy cs: ;
    skos:broader :granular-iron-formation ;
    skos:definition "A granular iron-formation with granules between 0.0625 and 2 mm (i.e. equivalent in size to a sandstone/arenite)."@en ;
    skos:historyNote "Beukes, NJ and Gutzmer, J 2008, Origin and paleoenvironmental significance of major iron formations at the Archean-Paleoproterozoic boundary: Reviews in Economic Geology, v. 15, p. 5–47, doi:10.5382/Rev.15.01." ;
    skos:inScheme cs: ;
    skos:notation "ciga"^^:gswa-rock-code ;
    skos:prefLabel "fearenite"@en ;
.

:feldspathic-fault-rock
    a skos:Concept ;
    rdfs:isDefinedBy cs: ;
    skos:broader :metamorphic-protolith-unknown-fault-rock ;
    skos:definition "A rock formed as a result of deformation in a fault zone and distinguished by the abundance of feldspar mineral phases. In GSWA usage, this term is reserved for fault rocks for which a protolith cannot be conclusively established."@en ;
    skos:historyNote "Compiled by the Geological Survey of Western Australia" ;
    skos:inScheme cs: ;
    skos:notation "myf"^^:gswa-rock-code ;
    skos:prefLabel "feldspathic fault rock"@en ;
.

:feldspathic-gneiss
    a skos:Concept ;
    rdfs:isDefinedBy cs: ;
    skos:broader :metamorphic-protolith-unknown-gneiss ;
    skos:definition "A gneiss distinguished by the abundance of feldspar mineral phases. In GSWA usage, this term is reserved for a gneiss for which a protolith cannot be conclusively established. See also definition of gneiss/gneissose structure in Fettes and Desmons (2007, p. 154–155)."@en ;
    skos:historyNote "Based on the IUGS classification of metamorphic rocks (Fettes and Desmons, 2007) and GSWA usage." ;
    skos:inScheme cs: ;
    skos:notation "mnf"^^:gswa-rock-code ;
    skos:prefLabel "feldspathic gneiss"@en ;
    schema:citation "https://glossary.americangeosciences.org/term/gneiss"^^xsd:anyURI ;
.

:feldspathic-granofels-hornfels
    a skos:Concept ;
    rdfs:isDefinedBy cs: ;
    skos:broader :metamorphic-protolith-unknown-granofels-hornfels ;
    skos:definition "A granofels/hornfels distinguished by the abundance of feldspar mineral phases. In GSWA usage, this term is reserved for a granofels/hornfels for which a protolith cannot be conclusively established."@en ;
    skos:historyNote "Compiled by the Geological Survey of Western Australia" ;
    skos:inScheme cs: ;
    skos:notation "mef"^^:gswa-rock-code ;
    skos:prefLabel "feldspathic granofels/hornfels"@en ;
.

:feldspathic-litharenite
    a skos:Concept ;
    rdfs:isDefinedBy cs: ;
    skos:altLabel "arkosic arenite"@en ;
    skos:broader :arenite ;
    skos:definition "A litharenite containing appreciable feldspar; specifically with less than 75% quartz and having a ratio of feldspar:lithic grains between 1:1 and 1:3. Adapted from Glossary of geology (5th edition revised; Neuendorf et al., 2011)"@en ;
    skos:historyNote "Folk, RL 1968, Petrology of Sedimentary Rocks: Austin, Hemphill Publishing Company, 170p." ;
    skos:inScheme cs: ;
    skos:notation "saa"^^:gswa-rock-code ;
    skos:prefLabel "feldspathic litharenite"@en ;
    schema:citation "https://glossary.americangeosciences.org/term/feldspathiclitharenite"^^xsd:anyURI ;
.

:feldspathic-metasiliciclastic-rock
    a skos:Concept ;
    rdfs:isDefinedBy cs: ;
    skos:broader :metasedimentary-siliciclastic ;
    skos:definition "A metamorphosed siliciclastic rock with a high feldspar content."@en ;
    skos:historyNote "Compiled by the Geological Survey of Western Australia" ;
    skos:inScheme cs: ;
    skos:notation "mdf"^^:gswa-rock-code ;
    skos:prefLabel "feldspathic metasiliciclastic rock"@en ;
.

:feldspathic-schist
    a skos:Concept ;
    rdfs:isDefinedBy cs: ;
    skos:broader :metamorphic-protolith-unknown-schist ;
    skos:definition "A schist distinguished by the abundance of feldspar mineral phases. In GSWA usage, this term is reserved for a schist for which a protolith cannot be conclusively established. See also definition of schist/schistose structure in Fettes and Desmons, 2007, p. 193)."@en ;
    skos:historyNote "Based on the IUGS classification of metamorphic rocks (Fettes and Desmons, 2007) and GSWA usage." ;
    skos:inScheme cs: ;
    skos:notation "msf"^^:gswa-rock-code ;
    skos:prefLabel "feldspathic schist"@en ;
.

:feldspathic-wacke
    a skos:Concept ;
    rdfs:isDefinedBy cs: ;
    skos:altLabel
        "arkosic wacke"@en ,
        "feldspathic graywacke"@en ;
    skos:broader :wacke ;
    skos:definition "A wacke containing more than 5% feldspar in which the feldspar grains are more abundant than rock/lithic fragments. Adapted from Glossary of geology (5th edition revised; Neuendorf et al., 2011)."@en ;
    skos:historyNote "Pettijohn, FJ 1975, Sedimentary Rocks: New York, Harper and Row, 628p." ;
    skos:inScheme cs: ;
    skos:notation "swa"^^:gswa-rock-code ;
    skos:prefLabel "feldspathic wacke"@en ;
.

:feldspathoid-bearing-volcanic-rock
    a skos:Concept ;
    rdfs:isDefinedBy cs: ;
    skos:broader :igneous-feldspathoid-bearing-volcanic ;
    skos:definition "A silica-undersaturated volcanic rock containing feldspathoid minerals in a modal volume greater than 0%, otherwise uncategorized. GSWA's rock classification scheme prefers the use of volcanic terminology for any igneous rock formed on or near the Earth's surface, i.e. for those hypabyssal or subvolcanic rocks such as dykes, sills, and cryptodomes that are demonstrably both spatially and temporally associated with extrusive volcanic rocks."@en ;
    skos:historyNote "Based on the IUGS classification of igneous rocks (Le Maitre et al., 2005)." ;
    skos:inScheme cs: ;
    skos:notation "l"^^:gswa-rock-code ;
    skos:prefLabel "feldspathoid-bearing volcanic rock"@en ;
.

:felsic-gneiss
    a skos:Concept ;
    rdfs:isDefinedBy cs: ;
    skos:broader :meta-igneous-felsic ;
    skos:definition "A metamorphosed felsic igneous rock displaying a gneissose structure, i.e. a gneiss derived from an igneous felsic but otherwise unspecified rock (i.e. the intrusive, extrusive or volcaniclastic nature of the protolith cannot be conclusively established). See also definition of gneiss/gneissose structure in Fettes and Desmons (2007, p. 154–155)."@en ;
    skos:historyNote "Based on the IUGS classification of metamorphic rocks (Fettes and Desmons, 2007)." ;
    skos:inScheme cs: ;
    skos:notation "mrn"^^:gswa-rock-code ;
    skos:prefLabel "felsic gneiss"@en ;
.

:felsic-gneiss-derived-from-volcanic-rock
    a skos:Concept ;
    rdfs:isDefinedBy cs: ;
    skos:altLabel "orthogneiss"@en ;
    skos:broader :meta-igneous-felsic-volcanic ;
    skos:definition "A metamorphosed felsic volcanic rock displaying a gneissose structure, i.e. a gneiss derived from a volcanic rock with one or more felsic minerals as the main component(s). See also definition of gneiss/gneissose structure in Fettes and Desmons (2007, p. 154–155). GSWA's rock classification scheme prefers the use of volcanic terminology for any igneous rock formed on or near the Earth's surface, i.e. for those hypabyssal or subvolcanic rocks such as dykes, sills, and cryptodomes that are demonstrably both spatially and temporally associated with extrusive volcanic rocks."@en ;
    skos:historyNote "Based on the IUGS classification of metamorphic rocks (Fettes and Desmons, 2007)." ;
    skos:inScheme cs: ;
    skos:notation "mfn"^^:gswa-rock-code ;
    skos:prefLabel "felsic gneiss derived from volcanic rock"@en ;
.

:felsic-granofels-hornfels
    a skos:Concept ;
    rdfs:isDefinedBy cs: ;
    skos:broader :meta-igneous-felsic ;
    skos:definition "General term for granofelsic or hornfelsed felsic igneous rocks for which an intrusive, extrusive or volcaniclastic protolith cannot be conclusively identified."@en ;
    skos:historyNote "Compiled by the Geological Survey of Western Australia" ;
    skos:inScheme cs: ;
    skos:notation "mre"^^:gswa-rock-code ;
    skos:prefLabel "felsic granofels/hornfels"@en ;
.

:felsic-granofels-hornfels-derived-from-volcanic-rock
    a skos:Concept ;
    rdfs:isDefinedBy cs: ;
    skos:broader :meta-igneous-felsic-volcanic ;
    skos:definition "A metamorphosed felsic volcanic rock displaying a granofelsic structure, i.e. a granofels/hornfels derived from a volcanic rock with one or more felsic minerals as the main components. See definition of granofels/granofelsic structure in Fettes and Desmons (2007, p. 156); hornfels are granofels formed by contact metamorphism (Fettes and Desmons, 2007, p. 159). GSWA's rock classification scheme prefers the use of volcanic terminology for any igneous rock formed on or near the Earth's surface, i.e. for those hypabyssal or subvolcanic rocks such as dykes, sills, and cryptodomes that are demonstrably both spatially and temporally associated with extrusive volcanic rocks."@en ;
    skos:historyNote "Based on the IUGS classification of metamorphic rocks (Fettes and Desmons, 2007)." ;
    skos:inScheme cs: ;
    skos:notation "mfe"^^:gswa-rock-code ;
    skos:prefLabel "felsic granofels/hornfels derived from volcanic rock"@en ;
.

:felsic-granulite
    a skos:Concept ;
    rdfs:isDefinedBy cs: ;
    skos:broadMatch
        <http://inspire.ec.europa.eu/codelist/LithologyValue/granulite> ,
        <http://resource.geosciml.org/classifier/cgi/lithology/granulite> ;
    skos:broader :meta-igneous-felsic ;
    skos:definition "Type of granulite with less than 30% mafic minerals (dominantly pyroxene) (Fettes and Desmons, 2007, p. 151). Mafic minerals is a collective term for modal ferromagnesian and other non-felsic minerals."@en ;
    skos:historyNote "Based on the IUGS classification of metamorphic rocks (Fettes and Desmons, 2007)." ;
    skos:inScheme cs: ;
    skos:notation "mro"^^:gswa-rock-code ;
    skos:prefLabel "felsic granulite"@en ;
.

:felsic-migmatite
    a skos:Concept ;
    rdfs:isDefinedBy cs: ;
    skos:broader :meta-igneous-felsic ;
    skos:definition "Composite silicate metamorphic rock derived from a felsic igneous but otherwise uncertain protolith, pervasively heterogeneous on a meso- to megascopic scale. It typically consists of darker (melanosome) and lighter (leucosome) parts. The darker parts usually exhibit features of metamorphic rocks, whereas the lighter parts are of igneous appearance. (Cf. Fettes and Desmond, 2007, p. 176)"@en ;
    skos:historyNote "Based on the IUGS classification of metamorphic rocks (Fettes and Desmons, 2007)." ;
    skos:inScheme cs: ;
    skos:notation "mri"^^:gswa-rock-code ;
    skos:prefLabel "felsic migmatite"@en ;
.

:felsic-migmatite-protolith-unknown
    a skos:Concept ;
    rdfs:isDefinedBy cs: ;
    skos:broader :migmatite-protolith-unknown ;
    skos:definition "Composite silicate metamorphic rock derived from a felsic but otherwise uncertain protolith, pervasively heterogeneous on a meso- to megascopic scale. It typically consists of darker (melanosome) and lighter (leucosome) parts. The darker parts usually exhibit features of metamorphic rocks, whereas the lighter parts are of igneous appearance. (Cf. Fettes and Desmond, 2007, p. 176)"@en ;
    skos:historyNote "Compiled by the Geological Survey of Western Australia" ;
    skos:inScheme cs: ;
    skos:notation "migf"^^:gswa-rock-code ;
    skos:prefLabel "felsic migmatite (protolith unknown)"@en ;
    schema:citation "https://geologyscience.com/rocks/metamorphic-rocks/foliated-metamorphic-rocks/migmatite/"^^xsd:anyURI ;
.

:felsic-schist
    a skos:Concept ;
    rdfs:isDefinedBy cs: ;
    skos:broader :meta-igneous-felsic ;
    skos:definition "A metamorphosed felsic rock displaying a schistose structure, i.e. a schist derived from an intrusive, extrusive or volcaniclastic rock with one or more felsic minerals as the main component(s). See also definition of schist/schistose structure in Fettes and Desmons, 2007, p. 193)."@en ;
    skos:historyNote "Based on the IUGS classification of metamorphic rocks (Fettes and Desmons, 2007)." ;
    skos:inScheme cs: ;
    skos:notation "mrs"^^:gswa-rock-code ;
    skos:prefLabel "felsic schist"@en ;
.

:felsic-schist-derived-from-volcanic-rock
    a skos:Concept ;
    rdfs:isDefinedBy cs: ;
    skos:broader :meta-igneous-felsic-volcanic ;
    skos:definition "A metamorphosed felsic volcanic rock displaying a schistose structure, i.e. a schist derived from a volcanic rock with one or more felsic minerals as the main component(s). See also definition of schist/schistose structure in Fettes and Desmons, 2007, p. 193). GSWA's rock classification scheme prefers the use of volcanic terminology for any igneous rock formed on or near the Earth's surface, i.e. for those hypabyssal or subvolcanic rocks such as dykes, sills, and cryptodomes that are demonstrably both spatially and temporally associated with extrusive volcanic rocks."@en ;
    skos:historyNote "Based on the IUGS classification of metamorphic rocks (Fettes and Desmons, 2007)." ;
    skos:inScheme cs: ;
    skos:notation "mfs"^^:gswa-rock-code ;
    skos:prefLabel "felsic schist derived from volcanic rock"@en ;
.

:felsic-volcanic-rock
    a skos:Concept ;
    rdfs:isDefinedBy cs: ;
    skos:broader :igneous-felsic-volcanic ;
    skos:definition "An igneous volcanic rock composed chiefly of one or more felsic, light-coloured minerals in its mode (adapted from Glossary of geology, 5th edition revised; Neuendorf et al., 2011). GSWA's rock classification scheme prefers the use of volcanic terminology for any igneous rock formed on or near the Earth's surface, i.e. for those hypabyssal or subvolcanic rocks such as dykes, sills, and cryptodomes that are demonstrably both spatially and temporally associated with extrusive volcanic rocks."@en ;
    skos:historyNote "Based on the IUGS classification of igneous rocks (Le Maitre et al., 2005) and Glossary of geology (5th edition, revised; Neuendorf et al. 2011)." ;
    skos:inScheme cs: ;
    skos:notation "f"^^:gswa-rock-code ;
    skos:prefLabel "felsic volcanic rock"@en ;
    schema:citation "https://glossary.americangeosciences.org/term/felsic"^^xsd:anyURI ;
.

:felsic-volcanic-rock-undivided
    a skos:Concept ;
    rdfs:isDefinedBy cs: ;
    skos:broader :igneous-felsic-volcanic ;
    skos:definition "A demonstrably felsic igneous volcanic rock, otherwise uncategorized. GSWA usage of this term is restricted to rocks that are partially weathered or are identified using remote sensing imagery, and the use of the related code/notation is limited to GSWA's Explanatory Notes System."@en ;
    skos:historyNote "Based on the IUGS classification of igneous rocks (Le Maitre et al., 2005) and GSWA usage." ;
    skos:inScheme cs: ;
    skos:notation "fn"^^:gswa-rock-code ;
    skos:prefLabel "felsic volcanic rock; undivided"@en ;
.

:felsic-volcaniclastic-breccia
    a skos:Concept ;
    rdfs:isDefinedBy cs: ;
    skos:broader :igneous-felsic-volcanic ;
    skos:definition "A volcaniclastic rock composed mostly of angular fragments greater than 2 mm in size consisting of either (a) pyroclastic detritus or (b) terrigenous volcanic detritus of epiclastic origin, and with an overall felsic composition. 'Volcaniclastic' includes all clastic volcanic materials formed by any process of fragmentation, dispersed by any kind of transporting agent, deposited in any environment, or mixed in any significant portion with non-volcanic fragments."@en ;
    skos:historyNote "Compiled by the Geological Survey of Western Australia" ;
    skos:inScheme cs: ;
    skos:notation "fvb"^^:gswa-rock-code ;
    skos:prefLabel "felsic volcaniclastic breccia"@en ;
    schema:citation
        "https://glossary.americangeosciences.org/term/volcanicbreccia"^^xsd:anyURI ,
        "https://glossary.americangeosciences.org/term/volcaniclastic"^^xsd:anyURI ;
.

:felsic-volcaniclastic-breccia-sandstone
    a skos:Concept ;
    rdfs:isDefinedBy cs: ;
    skos:broader :igneous-felsic-volcanic ;
    skos:definition "A volcaniclastic rock composed mostly of angular fragments of sand size (0.0625 – 2 mm) and above, consisting of either (a) pyroclastic detritus or (b) terrigenous volcanic detritus of epiclastic origin, and with an overall felsic composition. 'Volcaniclastic' includes all clastic volcanic materials formed by any process of fragmentation, dispersed by any kind of transporting agent, deposited in any environment, or mixed in any significant portion with non-volcanic fragments."@en ;
    skos:historyNote "Compiled by the Geological Survey of Western Australia" ;
    skos:inScheme cs: ;
    skos:notation "fvbs"^^:gswa-rock-code ;
    skos:prefLabel "felsic volcaniclastic breccia-sandstone"@en ;
    schema:citation "https://glossary.americangeosciences.org/term/volcaniclastic"^^xsd:anyURI ;
.

:felsic-volcaniclastic-conglomerate
    a skos:Concept ;
    rdfs:isDefinedBy cs: ;
    skos:broader :igneous-felsic-volcanic ;
    skos:definition "A conglomerate consisting of either (a) pyroclastic detritus or (b) terrigenous volcanic detritus of epiclastic origin, and with an overall felsic composition. 'Volcaniclastic' includes all clastic volcanic materials formed by any process of fragmentation, dispersed by any kind of transporting agent, deposited in any environment, or mixed in any significant portion with non-volcanic fragments."@en ;
    skos:historyNote "Compiled by the Geological Survey of Western Australia" ;
    skos:inScheme cs: ;
    skos:notation "fvc"^^:gswa-rock-code ;
    skos:prefLabel "felsic volcaniclastic conglomerate"@en ;
    schema:citation
        "https://glossary.americangeosciences.org/term/volcanicconglomerate"^^xsd:anyURI ,
        "https://glossary.americangeosciences.org/term/volcaniclastic"^^xsd:anyURI ;
.

:felsic-volcaniclastic-granule-pebble-breccia
    a skos:Concept ;
    rdfs:isDefinedBy cs: ;
    skos:broader :igneous-felsic-volcanic ;
    skos:definition "A breccia composed mostly of angular fragments ranging in size from granule (2–4 mm) to pebble (4–32 mm) consisting of either (a) pyroclastic detritus or (b) terrigenous volcanic detritus of epiclastic origin, and with an overall felsic composition. 'Volcaniclastic' includes all clastic volcanic materials formed by any process of fragmentation, dispersed by any kind of transporting agent, deposited in any environment, or mixed in any significant portion with non-volcanic fragments."@en ;
    skos:historyNote "Compiled by the Geological Survey of Western Australia" ;
    skos:inScheme cs: ;
    skos:notation "fvg"^^:gswa-rock-code ;
    skos:prefLabel "felsic volcaniclastic granule/pebble breccia"@en ;
    schema:citation "https://glossary.americangeosciences.org/term/volcaniclastic"^^xsd:anyURI ;
.

:felsic-volcaniclastic-mudstone
    a skos:Concept ;
    rdfs:isDefinedBy cs: ;
    skos:broader :igneous-felsic-volcanic ;
    skos:definition "A mudstone (grain size ranging from silt to clay, i.e. less than 0.0625 mm) consisting of either (a) pyroclastic detritus or (b) terrigenous volcanic detritus of epiclastic origin, and with an overall felsic composition. 'Volcaniclastic' includes all clastic volcanic materials formed by any process of fragmentation, dispersed by any kind of transporting agent, deposited in any environment, or mixed in any significant portion with non-volcanic fragments."@en ;
    skos:historyNote "Compiled by the Geological Survey of Western Australia" ;
    skos:inScheme cs: ;
    skos:notation "fvsn"^^:gswa-rock-code ;
    skos:prefLabel "felsic volcaniclastic mudstone"@en ;
    schema:citation "https://glossary.americangeosciences.org/term/volcaniclastic"^^xsd:anyURI ;
.

:felsic-volcaniclastic-rock
    a skos:Concept ;
    rdfs:isDefinedBy cs: ;
    skos:broader :igneous-felsic-volcanic ;
    skos:definition "A volcaniclastic rock consisting of either (a) pyroclastic detritus or (b) terrigenous volcanic detritus of epiclastic origin and with an overall felsic composition, but otherwise uncategorized. 'Volcaniclastic' includes all clastic volcanic materials formed by any process of fragmentation, dispersed by any kind of transporting agent, deposited in any environment, or mixed in any significant portion with non-volcanic fragments."@en ;
    skos:historyNote "Compiled by the Geological Survey of Western Australia" ;
    skos:inScheme cs: ;
    skos:notation "fvr"^^:gswa-rock-code ;
    skos:prefLabel "felsic volcaniclastic rock"@en ;
    schema:citation "https://glossary.americangeosciences.org/term/volcaniclastic"^^xsd:anyURI ;
.

:felsic-volcaniclastic-sandstone
    a skos:Concept ;
    rdfs:isDefinedBy cs: ;
    skos:broader :igneous-felsic-volcanic ;
    skos:definition "A sandstone (grain size 0.0625 – 2 mm) consisting of either (a) pyroclastic detritus or (b) terrigenous volcanic detritus of epiclastic origin, and with an overall felsic composition. 'Volcaniclastic' includes all clastic volcanic materials formed by any process of fragmentation, dispersed by any kind of transporting agent, deposited in any environment, or mixed in any significant portion with non-volcanic fragments."@en ;
    skos:historyNote "Pettijohn, FJ, Potter, PE, Siever, R 1987, Sand and sandstone: Springer-Verlag New York, Inc, 553p. (p. 205)" ;
    skos:inScheme cs: ;
    skos:notation "fvs"^^:gswa-rock-code ;
    skos:prefLabel "felsic volcaniclastic sandstone"@en ;
    schema:citation
        "https://glossary.americangeosciences.org/term/volcaniclastic"^^xsd:anyURI ,
        "https://glossary.americangeosciences.org/term/volcanicsandstone"^^xsd:anyURI ;
.

:felsic-volcaniclastic-sandstone-siltstone
    a skos:Concept ;
    rdfs:isDefinedBy cs: ;
    skos:broader :igneous-felsic-volcanic ;
    skos:definition "A volcaniclastic rock composed mostly of fragments ranging in size from sand (0.0625 – 2 mm) to silt (0.0039 – 0.0625 mm) of either (a) pyroclastic detritus or (b) terrigenous volcanic detritus of epiclastic origin, and with an overall felsic composition. 'Volcaniclastic' includes all clastic volcanic materials formed by any process of fragmentation, dispersed by any kind of transporting agent, deposited in any environment, or mixed in any significant portion w, and with an overall mafic composition."@en ;
    skos:historyNote "Compiled by the Geological Survey of Western Australia" ;
    skos:inScheme cs: ;
    skos:notation "fvss"^^:gswa-rock-code ;
    skos:prefLabel "felsic volcaniclastic sandstone-siltstone"@en ;
    schema:citation "https://glossary.americangeosciences.org/term/volcaniclastic"^^xsd:anyURI ;
.

:felsic-volcaniclastic-sediment-matrix-breccia
    a skos:Concept ;
    rdfs:isDefinedBy cs: ;
    skos:broader :igneous-felsic-volcanic ;
    skos:definition "A commonly monomictic breccia of overall felsic composition composed of angular, coarse igneous fragments cemented by a fine-grained matrix that is clastic though not necessarily strictly sedimentary in origin. 'Volcaniclastic' includes all clastic volcanic materials formed by any process of fragmentation, dispersed by any kind of transporting agent, deposited in any environment, or mixed in any significant portion with non-volcanic fragments."@en ;
    skos:historyNote "Compiled by the Geological Survey of Western Australia" ;
    skos:inScheme cs: ;
    skos:notation "fvsb"^^:gswa-rock-code ;
    skos:prefLabel "felsic volcaniclastic sediment-matrix breccia"@en ;
    schema:citation "https://doi.org/10.1016/j.jvolgeores.2016.02.007"^^xsd:anyURI ;
.

:felutite
    a skos:Concept ;
    rdfs:isDefinedBy cs: ;
    skos:broader :micritic-iron-formation ;
    skos:definition "A poorly bedded micritic iron-formation with a muddy massive appearance. Adapted from Beukes and Gutzmer (2008)."@en ;
    skos:historyNote "Beukes, NJ and Gutzmer, J 2008, Origin and paleoenvironmental significance of major iron formations at the Archean-Paleoproterozoic boundary: Reviews in Economic Geology, v. 15, p. 5–47, doi:10.5382/Rev.15.01." ;
    skos:inScheme cs: ;
    skos:notation "ciml"^^:gswa-rock-code ;
    skos:prefLabel "felutite"@en ;
.

:fenite
    a skos:Concept ;
    rdfs:isDefinedBy cs: ;
    skos:broader :metasomatic ;
    skos:definition "High-temperature metasomatic rock characterized by the presence of alkali feldspar, sodic amphibole and sodic pyroxene; nepheline, calcite and biotite/phlogopite may also be present, and typical accessories are titanite and apatite. Fenites occur as zoned aureoles around alkaline and carbonatite igneous complexes forming in a wide range of host lithologies. They occur on the metre to kilometre scale. (Fettes and Desmons, 2007, p. 152)"@en ;
    skos:historyNote "Based on the IUGS classification of metamorphic rocks (Fettes and Desmons, 2007)." ;
    skos:inScheme cs: ;
    skos:notation "mjf"^^:gswa-rock-code ;
    skos:prefLabel "fenite"@en ;
    schema:citation
        "https://en.wikipedia.org/wiki/Fenite;"^^xsd:anyURI ,
        "https://glossary.americangeosciences.org/term/fenite"^^xsd:anyURI ;
.

:ferhythmite
    a skos:Concept ;
    rdfs:isDefinedBy cs: ;
    skos:altLabel
        "BMIF"@en ,
        "banded micritic iron-formation"@en ;
    skos:broader :micritic-iron-formation ;
    skos:definition "A microbanded and well-laminated micritic iron-formation. Adapted from Beukes and Gutzmer (2008)."@en ;
    skos:historyNote "Beukes, NJ and Gutzmer, J 2008, Origin and paleoenvironmental significance of major iron formations at the Archean-Paleoproterozoic boundary: Reviews in Economic Geology, v. 15, p. 5–47, doi:10.5382/Rev.15.01." ;
    skos:inScheme cs: ;
    skos:notation "cimh"^^:gswa-rock-code ;
    skos:prefLabel "ferhythmite"@en ;
.

:ferro-carbonatite
    a skos:Concept ;
    rdfs:isDefinedBy cs: ;
    skos:broader :igneous-carbonatite ;
    skos:definition "A variety of carbonatite where the main carbonate is iron-rich. Also used for a chemically derived carbonatite in which weight percent CaO / (CaO+MgO+FeO+Fe₂O₃+MnO) < 0.8 and MgO < (FeO+Fe₂O₃+MnO) (Fig. 2.2, p. 10). Adapted from Le Maitre et al. (2005, p.  10 and 79)."@en ;
    skos:historyNote "Based on the IUGS classification of igneous rocks (Le Maitre et al., 2005)." ;
    skos:inScheme cs: ;
    skos:notation "rf"^^:gswa-rock-code ;
    skos:prefLabel "ferro-carbonatite"@en ;
    schema:citation "https://glossary.americangeosciences.org/term/dolomitecarbonatite"^^xsd:anyURI ;
.

:ferruginous-fault-rock
    a skos:Concept ;
    rdfs:isDefinedBy cs: ;
    skos:broader :metamorphic-protolith-unknown-fault-rock ;
    skos:definition "A rock formed as a result of deformation in a fault zone and distinguished a red or rusty colour due to the presence of ferric oxides. In GSWA usage, this term is reserved for fault rocks for which a protolith cannot be conclusively established."@en ;
    skos:historyNote "Compiled by the Geological Survey of Western Australia" ;
    skos:inScheme cs: ;
    skos:notation "myj"^^:gswa-rock-code ;
    skos:prefLabel "ferruginous fault rock"@en ;
.

:ferruginous-gneiss
    a skos:Concept ;
    rdfs:isDefinedBy cs: ;
    skos:broader :metamorphic-protolith-unknown-gneiss ;
    skos:definition "A gneiss distinguished by a red or rusty colour due to the presence of ferric oxide. In GSWA usage, this term is reserved for a gneiss for which a protolith cannot be conclusively established. See also definition of gneiss/gneissose structure in Fettes and Desmons (2007, p. 154–155)."@en ;
    skos:historyNote "Based on the IUGS classification of metamorphic rocks (Fettes and Desmons, 2007) and GSWA usage." ;
    skos:inScheme cs: ;
    skos:notation "mnj"^^:gswa-rock-code ;
    skos:prefLabel "ferruginous gneiss"@en ;
    schema:citation "https://glossary.americangeosciences.org/term/gneiss"^^xsd:anyURI ;
.

:ferruginous-granofels-hornfels
    a skos:Concept ;
    rdfs:isDefinedBy cs: ;
    skos:broader :metamorphic-protolith-unknown-granofels-hornfels ;
    skos:definition "A granofels/hornfels distinguished by a red or rusty colour due to the presence of ferric oxide. In GSWA usage, this term is reserved for a granofels/hornfels for which a protolith cannot be conclusively established."@en ;
    skos:historyNote "Compiled by the Geological Survey of Western Australia" ;
    skos:inScheme cs: ;
    skos:notation "mej"^^:gswa-rock-code ;
    skos:prefLabel "ferruginous granofels/hornfels"@en ;
.

:ferruginous-schist
    a skos:Concept ;
    rdfs:isDefinedBy cs: ;
    skos:broader :metamorphic-protolith-unknown-schist ;
    skos:definition "A schist distinguished by a red or rusty colour due to the presence of ferric oxide. In GSWA usage, this term is reserved for a schist for which a protolith cannot be conclusively established. See also definition of schist/schistose structure in Fettes and Desmons, 2007, p. 193)."@en ;
    skos:historyNote "Based on the IUGS classification of metamorphic rocks (Fettes and Desmons, 2007) and GSWA usage." ;
    skos:inScheme cs: ;
    skos:notation "msj"^^:gswa-rock-code ;
    skos:prefLabel "ferruginous schist"@en ;
.

:ferudite
    a skos:Concept ;
    rdfs:isDefinedBy cs: ;
    skos:broader :granular-iron-formation ;
    skos:definition "A granular iron formation with granules larger than 2 mm (i.e. equivalent in size to a conglomerate)."@en ;
    skos:historyNote "Beukes, NJ and Gutzmer, J 2008, Origin and paleoenvironmental significance of major iron formations at the Archean-Paleoproterozoic boundary: Reviews in Economic Geology, v. 15, p. 5–47, doi:10.5382/Rev.15.01." ;
    skos:inScheme cs: ;
    skos:notation "cigr"^^:gswa-rock-code ;
    skos:prefLabel "ferudite"@en ;
.

:fluorite-vein
    a skos:Concept ;
    rdfs:isDefinedBy cs: ;
    skos:broader :hydrothermal ;
    skos:definition "A rock comprising fluorite of pegmatitic or hydrothermal origin, as vein-filling material."@en ;
    skos:historyNote "Compiled by the Geological Survey of Western Australia" ;
    skos:inScheme cs: ;
    skos:notation "zf"^^:gswa-rock-code ;
    skos:prefLabel "fluorite vein"@en ;
.

:foid-bearing-alkali-feldspar-syenite
    a skos:Concept ;
    rdfs:isDefinedBy cs: ;
    skos:broader :igneous-foid-bearing-intrusive ;
    skos:definition "A collective term for alkali feldspar syenites containing small amounts of feldspathoids (less than 10% of the felsic minerals). Now defined modally in QAPF field 6' (Fig. 2.4, p. 22). (Le Maitre et al., 2005, p. 81)"@en ;
    skos:historyNote "Based on the IUGS classification of igneous rocks (Le Maitre et al., 2005)." ;
    skos:inScheme cs: ;
    skos:notation "dr"^^:gswa-rock-code ;
    skos:prefLabel "foid-bearing alkali feldspar syenite"@en ;
    schema:citation "https://glossary.americangeosciences.org/term/foidbearing"^^xsd:anyURI ;
.

:foid-bearing-anorthosite
    a skos:Concept ;
    rdfs:isDefinedBy cs: ;
    skos:broader :igneous-foid-bearing-intrusive ;
    skos:definition "A collective term for anorthosites containing small amounts of feldspathoids (less than 10% of the felsic minerals). Now defined modally in QAPF field 10' (Fig. 2.4, p. 22). (Le Maitre et al., 2005, p. 81)"@en ;
    skos:historyNote "Based on the IUGS classification of igneous rocks (Le Maitre et al., 2005)." ;
    skos:inScheme cs: ;
    skos:notation "dw"^^:gswa-rock-code ;
    skos:prefLabel "foid-bearing anorthosite"@en ;
    schema:citation "https://glossary.americangeosciences.org/term/foidbearing"^^xsd:anyURI ;
.

:foid-bearing-diorite
    a skos:Concept ;
    rdfs:isDefinedBy cs: ;
    skos:broader :igneous-foid-bearing-intrusive ;
    skos:definition "A collective term for diorites containing small amounts of feldspathoids (less than 10% of the felsic minerals). Now defined modally in QAPF field 10' (Fig. 2.4, p. 22–23). (Le Maitre et al., 2005, p. 81)"@en ;
    skos:historyNote "Based on the IUGS classification of igneous rocks (Le Maitre et al., 2005)." ;
    skos:inScheme cs: ;
    skos:notation "dd"^^:gswa-rock-code ;
    skos:prefLabel "foid-bearing diorite"@en ;
    schema:citation "https://glossary.americangeosciences.org/term/foidbearing"^^xsd:anyURI ;
.

:foid-bearing-gabbro
    a skos:Concept ;
    rdfs:isDefinedBy cs: ;
    skos:broader :igneous-foid-bearing-intrusive ;
    skos:definition "A collective term for gabbros containing small amounts of feldspathoids (less than 10% of the felsic minerals). Now defined modally in QAPF field 10' (Fig. 2.4, p. 22). (Le Maitre et al., 2005, p. 81)"@en ;
    skos:historyNote "Based on the IUGS classification of igneous rocks (Le Maitre et al., 2005)." ;
    skos:inScheme cs: ;
    skos:notation "du"^^:gswa-rock-code ;
    skos:prefLabel "foid-bearing gabbro"@en ;
    schema:citation "https://glossary.americangeosciences.org/term/foidbearing"^^xsd:anyURI ;
.

:foid-bearing-intrusive-rock
    a skos:Concept ;
    rdfs:isDefinedBy cs: ;
    skos:broader :igneous-foid-bearing-intrusive ;
    skos:definition "A silica-undersaturated, intrusive rock containing feldspathoid minerals in a modal volume greater than 0, otherwise uncategorized."@en ;
    skos:historyNote "Based on the IUGS classification of igneous rocks (Le Maitre et al., 2005)." ;
    skos:inScheme cs: ;
    skos:notation "d"^^:gswa-rock-code ;
    skos:prefLabel "foid-bearing intrusive rock"@en ;
    schema:citation "https://glossary.americangeosciences.org/term/foidbearing"^^xsd:anyURI ;
.

:foid-bearing-intrusive-rock-undivided
    a skos:Concept ;
    rdfs:isDefinedBy cs: ;
    skos:broader :igneous-foid-bearing-intrusive ;
    skos:definition "A silica-undersaturated intrusive rock with a modal content of feldspathoid minerals greater than 0, otherwise uncategorized. GSWA usage of this term is restricted to rocks that are partially weathered or are identified using remote sensing imagery, and the use of the related code/notation is limited to GSWA's Explanatory Notes System."@en ;
    skos:historyNote "Based on the IUGS classification of igneous rocks (Le Maitre et al., 2005) and GSWA usage." ;
    skos:inScheme cs: ;
    skos:notation "dn"^^:gswa-rock-code ;
    skos:prefLabel "foid-bearing intrusive rock; undivided"@en ;
.

:foid-bearing-latite
    a skos:Concept ;
    rdfs:isDefinedBy cs: ;
    skos:broader :igneous-feldspathoid-bearing-volcanic ;
    skos:definition "A collective term for latites containing small amounts of feldspathoids (less than 10% of the felsic minerals). Now defined modally in QAPF field 8' (Fig. 2.11, p. 31). (Le Maitre et al., 2005, p. 82)"@en ;
    skos:historyNote "Based on the IUGS classification of igneous rocks (Le Maitre et al., 2005)." ;
    skos:inScheme cs: ;
    skos:notation "ll"^^:gswa-rock-code ;
    skos:prefLabel "foid-bearing latite"@en ;
.

:foid-bearing-monzodiorite
    a skos:Concept ;
    rdfs:isDefinedBy cs: ;
    skos:broader :igneous-foid-bearing-intrusive ;
    skos:definition "A collective term for monzodiorites containing small amounts of feldspathoids (less than 10% of the felsic minerals). Now defined modally in QAPF field 9' (Fig. 2.4, p. 22). (Le Maitre et al., 2005, p. 82)"@en ;
    skos:historyNote "Based on the IUGS classification of igneous rocks (Le Maitre et al., 2005)." ;
    skos:inScheme cs: ;
    skos:notation "dh"^^:gswa-rock-code ;
    skos:prefLabel "foid-bearing monzodiorite"@en ;
    schema:citation "https://glossary.americangeosciences.org/term/foidbearing"^^xsd:anyURI ;
.

:foid-bearing-monzogabbro
    a skos:Concept ;
    rdfs:isDefinedBy cs: ;
    skos:broader :igneous-foid-bearing-intrusive ;
    skos:definition "A collective term for monzogabbros containing small amounts of feldspathoids (less than 10% of the felsic minerals). Now defined modally in QAPF field 9' (Fig. 2.4, p. 22). (Le Maitre et al., 2005, p. 82)"@en ;
    skos:historyNote "Based on the IUGS classification of igneous rocks (Le Maitre et al., 2005)." ;
    skos:inScheme cs: ;
    skos:notation "dj"^^:gswa-rock-code ;
    skos:prefLabel "foid-bearing monzogabbro"@en ;
    schema:citation "https://glossary.americangeosciences.org/term/foidbearing"^^xsd:anyURI ;
.

:foid-bearing-monzonite
    a skos:Concept ;
    rdfs:isDefinedBy cs: ;
    skos:broader :igneous-foid-bearing-intrusive ;
    skos:definition "A collective term for monzonites containing small amounts of feldspathoids (less than 10% of the felsic minerals). Now defined modally in QAPF field 8' (Fig. 2.4, p. 22). (Le Maitre et al., 2005, p. 82)"@en ;
    skos:historyNote "Based on the IUGS classification of igneous rocks (Le Maitre et al., 2005)." ;
    skos:inScheme cs: ;
    skos:notation "dz"^^:gswa-rock-code ;
    skos:prefLabel "foid-bearing monzonite"@en ;
    schema:citation "https://glossary.americangeosciences.org/term/foidbearing"^^xsd:anyURI ;
.

:foid-bearing-syenite
    a skos:Concept ;
    rdfs:isDefinedBy cs: ;
    skos:broader :igneous-foid-bearing-intrusive ;
    skos:definition "A collective term for syenites containing small amounts of feldspathoids (less than 10% of the felsic minerals). Now defined modally in QAPF field 7' (Fig. 2.4, p. 22). (Le Maitre et al., 2005, p. 82)"@en ;
    skos:historyNote "Based on the IUGS classification of igneous rocks (Le Maitre et al., 2005)." ;
    skos:inScheme cs: ;
    skos:notation "dy"^^:gswa-rock-code ;
    skos:prefLabel "foid-bearing syenite"@en ;
    schema:citation "https://glossary.americangeosciences.org/term/foidbearing"^^xsd:anyURI ;
.

:foid-bearing-trachyte
    a skos:Concept ;
    rdfs:isDefinedBy cs: ;
    skos:broader :igneous-feldspathoid-bearing-volcanic ;
    skos:definition "A collective term for trachytes containing small amounts of feldspathoids (less than 10% of the felsic minerals). Now defined modally in QAPF field7' (Fig. 2.11, p. 31). (Le Maitre et al., 2005, p. 82)"@en ;
    skos:historyNote "Based on the IUGS classification of igneous rocks (Le Maitre et al., 2005)." ;
    skos:inScheme cs: ;
    skos:notation "lt"^^:gswa-rock-code ;
    skos:prefLabel "foid-bearing trachyte"@en ;
.

:foid-bearing-volcanic-rock-undivided
    a skos:Concept ;
    rdfs:isDefinedBy cs: ;
    skos:broader :igneous-feldspathoid-bearing-volcanic ;
    skos:definition "A silica-undersaturated volcanic rock with a modal content of feldspathoid minerals greater than 0%, otherwise uncategorized. GSWA usage of this term is restricted to rocks that are partially weathered or are identified using remote sensing imagery, and the use of the related code/notation is limited to GSWA's Explanatory Notes System."@en ;
    skos:historyNote "Based on the IUGS classification of igneous rocks (Le Maitre et al., 2005) and GSWA usage." ;
    skos:inScheme cs: ;
    skos:notation "ln"^^:gswa-rock-code ;
    skos:prefLabel "foid-bearing volcanic rock; undivided"@en ;
.

:foid-bearing-volcaniclastic-breccia
    a skos:Concept ;
    rdfs:isDefinedBy cs: ;
    skos:broader :igneous-feldspathoid-bearing-volcanic ;
    skos:definition "A volcaniclastic rock composed mostly of angular fragments greater than 2 mm in size consisting of either (a) pyroclastic detritus or (b) terrigenous volcanic detritus of epiclastic origin, and with foid modal content greater than 0%. 'Volcaniclastic' includes all clastic volcanic materials formed by any process of fragmentation, dispersed by any kind of transporting agent, deposited in any environment, or mixed in any significant portion with non-volcanic fragments."@en ;
    skos:historyNote "Compiled by the Geological Survey of Western Australia" ;
    skos:inScheme cs: ;
    skos:notation "lvb"^^:gswa-rock-code ;
    skos:prefLabel "foid-bearing volcaniclastic breccia"@en ;
.

:foid-bearing-volcaniclastic-breccia-sandstone
    a skos:Concept ;
    rdfs:isDefinedBy cs: ;
    skos:broader :igneous-feldspathoid-bearing-volcanic ;
    skos:definition "A volcaniclastic rock composed mostly of angular fragments ranging in size from sand (0.0625 – 2 mm) and above, consisting of either (a) pyroclastic detritus or (b) terrigenous volcanic detritus of epiclastic origin, and with a foid modal content greater than 0%. 'Volcaniclastic' includes all clastic volcanic materials formed by any process of fragmentation, dispersed by any kind of transporting agent, deposited in any environment, or mixed in any significant portion w, and with an overall mafic composition."@en ;
    skos:historyNote "Compiled by the Geological Survey of Western Australia" ;
    skos:inScheme cs: ;
    skos:notation "lvbs"^^:gswa-rock-code ;
    skos:prefLabel "foid-bearing volcaniclastic breccia-sandstone"@en ;
.

:foid-bearing-volcaniclastic-conglomerate
    a skos:Concept ;
    rdfs:isDefinedBy cs: ;
    skos:broader :igneous-feldspathoid-bearing-volcanic ;
    skos:definition "A conglomerate consisting of either (a) pyroclastic detritus or (b) terrigenous volcanic detritus of epiclastic origin, and with a foid modal content greater than 0%. 'Volcaniclastic' includes all clastic volcanic materials formed by any process of fragmentation, dispersed by any kind of transporting agent, deposited in any environment, or mixed in any significant portion with non-volcanic fragments."@en ;
    skos:historyNote "Compiled by the Geological Survey of Western Australia" ;
    skos:inScheme cs: ;
    skos:notation "lvc"^^:gswa-rock-code ;
    skos:prefLabel "foid-bearing volcaniclastic conglomerate"@en ;
.

:foid-bearing-volcaniclastic-granule-pebble-breccia
    a skos:Concept ;
    rdfs:isDefinedBy cs: ;
    skos:broader :igneous-feldspathoid-bearing-volcanic ;
    skos:definition "A breccia composed mostly of angular fragments ranging in size from granule (2–4 mm) to pebble (4–32 mm) consisting of either (a) pyroclastic detritus or (b) terrigenous volcanic detritus of epiclastic origin, and with a foid modal content greater than 0%. 'Volcaniclastic' includes all clastic volcanic materials formed by any process of fragmentation, dispersed by any kind of transporting agent, deposited in any environment, or mixed in any significant portion with non-volcanic fragments."@en ;
    skos:historyNote "Compiled by the Geological Survey of Western Australia" ;
    skos:inScheme cs: ;
    skos:notation "lvg"^^:gswa-rock-code ;
    skos:prefLabel "foid-bearing volcaniclastic granule/pebble breccia"@en ;
.

:foid-bearing-volcaniclastic-mudstone
    a skos:Concept ;
    rdfs:isDefinedBy cs: ;
    skos:broader :igneous-feldspathoid-bearing-volcanic ;
    skos:definition "A mudstone (grain size ranging from silt to clay, i.e. less than 0.0625 mm) consisting of either (a) pyroclastic detritus or (b) terrigenous volcanic detritus of epiclastic origin, and with a foid modal content greater than 0%. 'Volcaniclastic' includes all clastic volcanic materials formed by any process of fragmentation, dispersed by any kind of transporting agent, deposited in any environment, or mixed in any significant portion with non-volcanic fragments."@en ;
    skos:historyNote "Compiled by the Geological Survey of Western Australia" ;
    skos:inScheme cs: ;
    skos:notation "lvsm"^^:gswa-rock-code ;
    skos:prefLabel "foid-bearing volcaniclastic mudstone"@en ;
.

:foid-bearing-volcaniclastic-rock
    a skos:Concept ;
    rdfs:isDefinedBy cs: ;
    skos:broader :igneous-feldspathoid-bearing-volcanic ;
    skos:definition "A volcaniclastic rock consisting of either (a) pyroclastic detritus or (b) terrigenous volcanic detritus of epiclastic origin, and with a foid modal content greater than 0%, but otherwise uncategorized. 'Volcaniclastic' includes all clastic volcanic materials formed by any process of fragmentation, dispersed by any kind of transporting agent, deposited in any environment, or mixed in any significant portion with non-volcanic fragments."@en ;
    skos:historyNote "Compiled by the Geological Survey of Western Australia" ;
    skos:inScheme cs: ;
    skos:notation "lvr"^^:gswa-rock-code ;
    skos:prefLabel "foid-bearing volcaniclastic rock"@en ;
.

:foid-bearing-volcaniclastic-sandstone
    a skos:Concept ;
    rdfs:isDefinedBy cs: ;
    skos:broader :igneous-feldspathoid-bearing-volcanic ;
    skos:definition "A sandstone (grain size 0.0625 – 2 mm) consisting of either (a) pyroclastic detritus or (b) terrigenous volcanic detritus of epiclastic origin, and with a foid modal content greater than 0%. 'Volcaniclastic' includes all clastic volcanic materials formed by any process of fragmentation, dispersed by any kind of transporting agent, deposited in any environment, or mixed in any significant portion with non-volcanic fragments."@en ;
    skos:historyNote "Compiled by the Geological Survey of Western Australia" ;
    skos:inScheme cs: ;
    skos:notation "lvs"^^:gswa-rock-code ;
    skos:prefLabel "foid-bearing volcaniclastic sandstone"@en ;
.

:foid-bearing-volcaniclastic-sandstone-siltstone
    a skos:Concept ;
    rdfs:isDefinedBy cs: ;
    skos:broader :igneous-feldspathoid-bearing-volcanic ;
    skos:definition "A volcaniclastic rock composed mostly of fragments ranging in size from sand (0.0625 – 2 mm) to silt (0.0039 – 0.0625 mm) of either (a) pyroclastic detritus or (b) terrigenous volcanic detritus of epiclastic origin, and with a foid modal content greater than 0%. 'Volcaniclastic' includes all clastic volcanic materials formed by any process of fragmentation, dispersed by any kind of transporting agent, deposited in any environment, or mixed in any significant portion w, and with an overall mafic composition."@en ;
    skos:historyNote "Compiled by the Geological Survey of Western Australia" ;
    skos:inScheme cs: ;
    skos:notation "lvss"^^:gswa-rock-code ;
    skos:prefLabel "foid-bearing volcaniclastic sandstone-siltstone"@en ;
.

:foid-bearing-volcaniclastic-sediment-matrix-breccia
    a skos:Concept ;
    rdfs:isDefinedBy cs: ;
    skos:broader :igneous-feldspathoid-bearing-volcanic ;
    skos:definition "A commonly monomictic breccia with a foid modal content greater than 0% and composed of angular, coarse igneous fragments cemented by a fine-grained matrix that is clastic though not necessarily strictly sedimentary in origin"@en ;
    skos:historyNote "Compiled by the Geological Survey of Western Australia" ;
    skos:inScheme cs: ;
    skos:notation "lvsb"^^:gswa-rock-code ;
    skos:prefLabel "foid-bearing volcaniclastic sediment-matrix breccia"@en ;
.

:foid-diorite
    a skos:Concept ;
    rdfs:isDefinedBy cs: ;
    skos:broader :igneous-foid-bearing-intrusive ;
    skos:definition "A collective term for alkaline intrusive rocks consisting of feldspathoids (10–60% of the felsic minerals), intermediate plagioclase and large amounts of mafic minerals. Now defined modally in QAPF field 14 (Fig. 2.4, p. 22). (Le Maitre et al., 2005, p. 80)"@en ;
    skos:exactMatch
        <http://inspire.ec.europa.eu/codelist/LithologyValue/foidDiorite> ,
        <http://resource.geosciml.org/classifier/cgi/lithology/foid_diorite> ;
    skos:historyNote "Based on the IUGS classification of igneous rocks (Le Maitre et al., 2005)." ;
    skos:inScheme cs: ;
    skos:notation "dt"^^:gswa-rock-code ;
    skos:prefLabel "foid diorite"@en ;
    schema:citation "https://glossary.americangeosciences.org/term/foiddiorite"^^xsd:anyURI ;
.

:foid-gabbro
    a skos:Concept ;
    rdfs:isDefinedBy cs: ;
    skos:broader :igneous-foid-bearing-intrusive ;
    skos:definition "A collective term for basic alkaline intrusive rocks consisting of feldspathoids (10–60% of the felsic minerals), calcic plagioclase and large amounts of mafic minerals. Now defined modally in QAPF field 14 (Fig. 2.4, p. 22). (Le Maitre et al., 2005, p. 81)"@en ;
    skos:exactMatch
        <http://inspire.ec.europa.eu/codelist/LithologyValue/foidGabbro> ,
        <http://resource.geosciml.org/classifier/cgi/lithology/foid_gabbro> ;
    skos:historyNote "Based on the IUGS classification of igneous rocks (Le Maitre et al., 2005)." ;
    skos:inScheme cs: ;
    skos:notation "dg"^^:gswa-rock-code ;
    skos:prefLabel "foid gabbro"@en ;
    schema:citation "https://glossary.americangeosciences.org/term/foidgabbro"^^xsd:anyURI ;
.

:foid-monzodiorite
    a skos:Concept ;
    rdfs:isDefinedBy cs: ;
    skos:broader :igneous-foid-bearing-intrusive ;
    skos:definition "A collective term for alkaline intrusive rocks consisting of feldspathoids (10–60% of the felsic minerals), intermediate plagioclase with subordinate alkali feldspar and large amounts of mafic minerals. Now defined modally in QAPF field 13 (Fig. 2.4, p. 22). (Le Maitre et al., 2005, p. 81)"@en ;
    skos:exactMatch
        <http://inspire.ec.europa.eu/codelist/LithologyValue/foidMonzodiorite> ,
        <http://resource.geosciml.org/classifier/cgi/lithology/foid_monzodiorite> ;
    skos:historyNote "Based on the IUGS classification of igneous rocks (Le Maitre et al., 2005)." ;
    skos:inScheme cs: ;
    skos:notation "dm"^^:gswa-rock-code ;
    skos:prefLabel "foid monzodiorite"@en ;
    schema:citation "https://glossary.americangeosciences.org/term/foidmonzodiorite"^^xsd:anyURI ;
.

:foid-monzogabbro
    a skos:Concept ;
    rdfs:isDefinedBy cs: ;
    skos:broader :igneous-foid-bearing-intrusive ;
    skos:definition "A collective term for basic alkaline intrusive rocks consisting of feldspathoids (10–60% of the felsic minerals), calcic plagioclase with subordinate alkali feldspar and large amounts of mafic minerals. Now defined modally in QAPF field 13 (Fig. 2.4, p. 22). (Le Maitre et al., 2005, p. 81)"@en ;
    skos:exactMatch
        <http://inspire.ec.europa.eu/codelist/LithologyValue/foidMonzogabbro> ,
        <http://resource.geosciml.org/classifier/cgi/lithology/foid_monzogabbro> ;
    skos:historyNote "Based on the IUGS classification of igneous rocks (Le Maitre et al., 2005)." ;
    skos:inScheme cs: ;
    skos:notation "dk"^^:gswa-rock-code ;
    skos:prefLabel "foid monzogabbro"@en ;
    schema:citation "https://glossary.americangeosciences.org/term/foidmonzogabbro"^^xsd:anyURI ;
.

:foid-monzosyenite
    a skos:Concept ;
    rdfs:isDefinedBy cs: ;
    skos:broader :igneous-foid-bearing-intrusive ;
    skos:definition "A collective term for rare alkaline intrusive rocks consisting of feldspathoids, alkali feldspar, plagioclase and mafic minerals. Now defined modally in QAPF field 12 (Fig. 2.4, p. 22). (Le Maitre et al., 2005, p. 81)"@en ;
    skos:exactMatch
        <http://inspire.ec.europa.eu/codelist/LithologyValue/foidMonzosyenite> ,
        <http://resource.geosciml.org/classifier/cgi/lithology/foid_monzosyenite> ;
    skos:historyNote "Based on the IUGS classification of igneous rocks (Le Maitre et al., 2005)." ;
    skos:inScheme cs: ;
    skos:notation "ds"^^:gswa-rock-code ;
    skos:prefLabel "foid monzosyenite"@en ;
    schema:citation "https://glossary.americangeosciences.org/term/foidmonzosyenite"^^xsd:anyURI ;
.

:foid-syenite
    a skos:Concept ;
    rdfs:isDefinedBy cs: ;
    skos:broader :igneous-foid-bearing-intrusive ;
    skos:definition "A collective term for leucocratic alkaline intrusive rocks consisting of feldspathoids (10–60% of the felsic minerals), alkali feldspar and mafic minerals. Now defined modally in QAPF field 11 (Fig. 2.4, p. 22). (Le Maitre et al., 2005, p. 81)"@en ;
    skos:exactMatch
        <http://inspire.ec.europa.eu/codelist/LithologyValue/foidSyenite> ,
        <http://resource.geosciml.org/classifier/cgi/lithology/foid_syenite> ;
    skos:historyNote "Based on the IUGS classification of igneous rocks (Le Maitre et al., 2005)." ;
    skos:inScheme cs: ;
    skos:notation "df"^^:gswa-rock-code ;
    skos:prefLabel "foid syenite"@en ;
    schema:citation "https://glossary.americangeosciences.org/term/foidsyenite"^^xsd:anyURI ;
.

:foliated-gouge
    a skos:Concept ;
    rdfs:isDefinedBy cs: ;
    skos:broader :metamorphic-protolith-unknown-fault-rock ;
    skos:definition "An incohesive fault rock with a high matrix–fragment ratio (visible fragments less than 30% of the rock mass), i.e. a strongly ground down version of the original rock, with a distinct planar anisotropy (i.e. foliation). The term is sometimes also used for strongly reworked clay or shale in the core of faults in sedimentary sequences. Adapted from Fossen (2016). In GSWA usage, this term is reserved for fault rocks for which a protolith cannot be conclusively established."@en ;
    skos:historyNote "Fossen, H 2016, Structural geology (2nd edition): Cambridge University Press, Cambridge, United Kingdom, 524p." ;
    skos:inScheme cs: ;
    skos:notation "myl"^^:gswa-rock-code ;
    skos:prefLabel "foliated gouge"@en ;
.

:foliated-metagranite
    a skos:Concept ;
    rdfs:isDefinedBy cs: ;
    skos:broader :meta-igneous-felsic-intrusive ;
    skos:definition "A demonstrably felsic intrusive rock, otherwise uncategorized, with a preferred planar orientation of inequant mineral grains or grain aggregates (cf. definition of foliation in Fettes and Desmons, 2007, p. 153)"@en ;
    skos:historyNote "Based on the IUGS classification of metamorphic rocks (Fettes and Desmons, 2007)." ;
    skos:inScheme cs: ;
    skos:notation "mgss"^^:gswa-rock-code ;
    skos:prefLabel "foliated metagranite"@en ;
.

:foliated-quartz-vein
    a skos:Concept ;
    rdfs:isDefinedBy cs: ;
    skos:broader :metamorphosed-quartz-vein ;
    skos:definition "A metamorphosed quartz vein with a repetitively occurring or penetrative planar feature (cf. Fettes and Desmons, 2007, p. 153)."@en ;
    skos:historyNote "Compiled by the Geological Survey of Western Australia" ;
    skos:inScheme cs: ;
    skos:notation "mzqs"^^:gswa-rock-code ;
    skos:prefLabel "foliated quartz vein"@en ;
.

:gabbro
    a skos:Concept ;
    rdfs:isDefinedBy cs: ;
    skos:broader :igneous-mafic-intrusive ;
    skos:definition "A coarse-grained intrusive rock (and including coarse-grained parts of extrusive successions) composed essentially of calcic plagioclase, pyroxene and iron oxides. If olivine is an essential constituent it is olivine gabbro; if quartz is an essential constituent it is quartz gabbro. Now defined modally in QAPF field 10 (Fig. 2.4, p. 22). (cf. Le Maitre et al., 2005, p.  83)"@en ;
    skos:exactMatch
        <http://inspire.ec.europa.eu/codelist/LithologyValue/gabbro> ,
        <http://resource.geosciml.org/classifier/cgi/lithology/gabbro> ;
    skos:historyNote "Based on the IUGS classification of igneous rocks (Le Maitre et al., 2005)." ;
    skos:inScheme cs: ;
    skos:notation "og"^^:gswa-rock-code ;
    skos:prefLabel "gabbro"@en ;
    schema:citation "https://glossary.americangeosciences.org/term/gabbro"^^xsd:anyURI ;
.

:gabbronorite
    a skos:Concept ;
    rdfs:isDefinedBy cs: ;
    skos:broader :igneous-mafic-intrusive ;
    skos:definition "A collective name for an intrusive rock consisting of calcic plagioclase and roughly equal amounts of clinopyroxene and orthopyroxene. Now defined modally in the gabbroic rock classification (Fig. 2.6, p. 25). (Le Maitre et al., 2005, p. 83)"@en ;
    skos:historyNote "Based on the IUGS classification of igneous rocks (Le Maitre et al., 2005)." ;
    skos:inScheme cs: ;
    skos:notation "om"^^:gswa-rock-code ;
    skos:prefLabel "gabbronorite"@en ;
    schema:citation "https://glossary.americangeosciences.org/term/gabbronorite"^^xsd:anyURI ;
.

:gneiss
    a skos:Concept ;
    rdfs:isDefinedBy cs: ;
    skos:broader :metamorphic-protolith-unknown-gneiss ;
    skos:definition "A metamorphic rock for which a protolith cannot be conclusively identified and displaying a gneissose structure, i.e. a foliated rock formed by regional metamorphism in which bands or lenticles of granular minerals alternate with bands or lenticles in which minerals having flaky or elongate prismatic habits predominate. Generally less than 50% of the minerals show preferred parallel orientation. Definition adapted from Fettes and Desmons (2007, p. 154–155) and Glossary of geology 2011, 5th edition revised)."@en ;
    skos:exactMatch
        <http://inspire.ec.europa.eu/codelist/LithologyValue/gneiss> ,
        <http://resource.geosciml.org/classifier/cgi/lithology/gneiss> ;
    skos:historyNote "Based on the IUGS classification of metamorphic rocks (Fettes and Desmons, 2007)." ;
    skos:inScheme cs: ;
    skos:notation "mn"^^:gswa-rock-code ;
    skos:prefLabel "gneiss"@en ;
    schema:citation "https://glossary.americangeosciences.org/term/gneiss"^^xsd:anyURI ;
.

:gneissose-granulite
    a skos:Concept ;
    rdfs:isDefinedBy cs: ;
    skos:broader :metamorphic-protolith-unknown-gneiss ;
    skos:definition "A high-grade metamorphic rock, with a granoblastic texture and little foliation/lineation and in which Fe–Mg silicates are dominantly hydroxyl-free, feldspar is a critical phase, and primary muscovite is absent. In GSWA usage, this term is reserved for a gneiss for which a protolith cannot be conclusively established. See also definition of gneiss/gneissose structure in Fettes and Desmons (2007, p. 154–155)."@en ;
    skos:historyNote "Based on the IUGS classification of metamorphic rocks (Fettes and Desmons, 2007) and GSWA usage." ;
    skos:inScheme cs: ;
    skos:notation "mno"^^:gswa-rock-code ;
    skos:prefLabel "gneissose granulite"@en ;
    schema:citation "https://glossary.americangeosciences.org/term/gneiss"^^xsd:anyURI ;
.

:gneissose-hydrothermal-rock
    a skos:Concept ;
    rdfs:isDefinedBy cs: ;
    skos:broader :metamorphosed-hydrothermal ;
    skos:definition "A metamorphosed hydrothermal igneous rock displaying a gneissose structure. See also definition of gneiss/gneissose structure in Fettes and Desmons (2007, p. 154–155)."@en ;
    skos:historyNote "Based on the IUGS classification of metamorphic rocks (Fettes and Desmons, 2007) and GSWA usage." ;
    skos:inScheme cs: ;
    skos:notation "mzn"^^:gswa-rock-code ;
    skos:prefLabel "gneissose hydrothermal rock"@en ;
    schema:citation
        "https://glossary.americangeosciences.org/term/gneiss"^^xsd:anyURI ,
        "https://glossary.americangeosciences.org/term/hydrothermalalteration"^^xsd:anyURI ;
.

:gneissose-marble
    a skos:Concept ;
    rdfs:isDefinedBy cs: ;
    skos:broader :marble ;
    skos:definition "A metamorphosed sedimentary carbonate rock consisting of more than 50% volume of carbonate minerals (calcite and/or aragonite and/or dolomite) and displaying a gneissose structure. See also definition of gneiss/gneissose structure in Fettes and Desmons (2007, p. 154–155)."@en ;
    skos:historyNote "Compiled by the Geological Survey of Western Australia" ;
    skos:inScheme cs: ;
    skos:notation "mkkn"^^:gswa-rock-code ;
    skos:prefLabel "gneissose marble"@en ;
.

:gneissose-meta-iron-formation
    a skos:Concept ;
    rdfs:isDefinedBy cs: ;
    skos:altLabel
        "itabirite"@en ,
        "taconite"@en ;
    skos:broader :metasedimentary-other-chemical-meta-iron-formation ;
    skos:definition "A metamorphosed iron formation displaying a gneissose structure, i.e. a gneiss derived from a chemical or biochemical sedimentary protolith containing at least 15% iron of sedimentary origin. See also definition of gneiss/gneissose structure in Fettes and Desmons (2007, p. 154–155)."@en ;
    skos:historyNote "Based on the IUGS classification of metamorphic rocks (Fettes and Desmons, 2007) and GSWA usage." ;
    skos:inScheme cs: ;
    skos:notation "min"^^:gswa-rock-code ;
    skos:prefLabel "gneissose meta-iron formation"@en ;
    schema:citation "https://glossary.americangeosciences.org/term/gneiss"^^xsd:anyURI ;
.

:gneissose-metacarbonatite
    a skos:Concept ;
    rdfs:isDefinedBy cs: ;
    skos:broader :meta-igneous-carbonatite ;
    skos:definition "A gneiss derived by metamorphism of an igneous protolith containing a modal amount of primary carbonate minerals greater than 50%. See also definition of gneiss/gneissose structure in Fettes and Desmons (2007, p. 154–155)."@en ;
    skos:inScheme cs: ;
    skos:notation "mqn"^^:gswa-rock-code ;
    skos:prefLabel "gneissose metacarbonatite"@en ;
.

:gneissose-metachert
    a skos:Concept ;
    rdfs:isDefinedBy cs: ;
    skos:broader :metasedimentary-other-chemical ;
    skos:definition "A metamorphosed chert displaying a gneissose structure, i.e. a gneiss from a chemical or biochemical sedimentary rock largely consisting of silica and/or quartz. See also definition of gneiss/gneissose structure in Fettes and Desmons (2007, p. 154–155)."@en ;
    skos:historyNote "Compiled by the Geological Survey of Western Australia" ;
    skos:inScheme cs: ;
    skos:notation "mcn"^^:gswa-rock-code ;
    skos:prefLabel "gneissose metachert"@en ;
.

:gneissose-para-amphibolite-carbonate
    a skos:Concept ;
    rdfs:isDefinedBy cs: ;
    skos:broader :para-amphibolite-derived-from-carbonate-rock ;
    skos:definition "A metamorphosed amphibole-rich rock derived from a sedimentary carbonate protolith and displaying a gneissose structure. See also definition of gneiss/gneissose structure in Fettes and Desmons (2007, p. 154–155)."@en ;
    skos:historyNote "Compiled by the Geological Survey of Western Australia" ;
    skos:inScheme cs: ;
    skos:notation "mkan"^^:gswa-rock-code ;
    skos:prefLabel "gneissose para-amphibolite (carbonate)"@en ;
.

:gneissose-para-amphibolite-siliciclastic
    a skos:Concept ;
    rdfs:isDefinedBy cs: ;
    skos:broader :para-amphibolite ;
    skos:definition "A metamorphosed amphibole-rich rock derived from a sedimentary siliciclastic protolith and displaying a gneissose structure. See also definition of gneiss/gneissose structure in Fettes and Desmons (2007, p. 154–155)."@en ;
    skos:historyNote "Compiled by the Geological Survey of Western Australia" ;
    skos:inScheme cs: ;
    skos:notation "mdan"^^:gswa-rock-code ;
    skos:prefLabel "gneissose para-amphibolite (siliciclastic)"@en ;
.

:goethite-hematite-vein
    a skos:Concept ;
    rdfs:isDefinedBy cs: ;
    skos:broader :hydrothermal ;
    skos:definition "A rock comprising goethite and/or hematite of hydrothermal origin, as vein-filling material."@en ;
    skos:historyNote "Compiled by the Geological Survey of Western Australia" ;
    skos:inScheme cs: ;
    skos:notation "zi"^^:gswa-rock-code ;
    skos:prefLabel "goethite/hematite vein"@en ;
.

:granitic-gneiss
    a skos:Concept ;
    rdfs:isDefinedBy cs: ;
    skos:broader :meta-igneous-felsic-intrusive ;
    skos:definition "A metamorphosed felsic intrusive rock displaying a gneissose structure, i.e. a gneiss derived from an intrusive rock with one or more felsic minerals as the main component(s). See also definition of gneiss/gneissose structure in Fettes and Desmons (2007, p. 154–155)."@en ;
    skos:historyNote "Based on the IUGS classification of metamorphic rocks (Fettes and Desmons, 2007)." ;
    skos:inScheme cs: ;
    skos:notation "mgn"^^:gswa-rock-code ;
    skos:prefLabel "granitic gneiss"@en ;
.

:granitic-granofels-hornfels
    a skos:Concept ;
    rdfs:isDefinedBy cs: ;
    skos:broader :meta-igneous-felsic-intrusive ;
    skos:definition "A metamorphosed felsic intrusive rock displaying a granofelsic structure, i.e. a granofels/hornfels derived from an intrusive rock with one or more felsic minerals as the main components. See also definition of granofels/granofelsic structure in Fettes and Desmons (2007, p. 156); hornfels are granofels formed by contact metamorphism (Fettes and Desmons, 2007, p. 159)."@en ;
    skos:historyNote "Based on the IUGS classification of metamorphic rocks (Fettes and Desmons, 2007)." ;
    skos:inScheme cs: ;
    skos:notation "mge"^^:gswa-rock-code ;
    skos:prefLabel "granitic granofels/hornfels"@en ;
.

:granitic-rock
    a skos:Concept ;
    rdfs:isDefinedBy cs: ;
    skos:broader :igneous-felsic-intrusive ;
    skos:definition "In GSWA usage, a generic term for an igneous intrusive rock composed chiefly of one or more felsic, light-coloured minerals in its mode and with quartz modal content between 0 and 60%, otherwise uncategorized."@en ;
    skos:historyNote "Compiled by the Geological Survey of Western Australia" ;
    skos:inScheme cs: ;
    skos:notation "g"^^:gswa-rock-code ;
    skos:prefLabel "granitic rock"@en ;
    schema:citation "https://glossary.americangeosciences.org/term/granitepetrology"^^xsd:anyURI ;
.

:granitic-rock-undivided
    a skos:Concept ;
    rdfs:isDefinedBy cs: ;
    skos:broader :igneous-felsic-intrusive ;
    skos:definition "A demonstrably felsic igneous intrusive rocks, otherwise uncategorized. GSWA usage of this term is restricted to rocks that are partially weathered or are identified using remote sensing imagery, and the use of the related code/notation is limited to GSWA's Explanatory Notes System."@en ;
    skos:historyNote "Based on the IUGS classification of igneous rocks (Le Maitre et al., 2005) and GSWA usage." ;
    skos:inScheme cs: ;
    skos:notation "gn"^^:gswa-rock-code ;
    skos:prefLabel "granitic rock; undivided"@en ;
.

:granitic-schist
    a skos:Concept ;
    rdfs:isDefinedBy cs: ;
    skos:broader :meta-igneous-felsic-intrusive ;
    skos:definition "A metamorphosed felsic intrusive rock displaying a schistose structure, i.e. a schist derived from an intrusive rock with one or more felsic minerals as the main component(s). See also definition of schist/schistose structure in Fettes and Desmons, 2007, p. 193)."@en ;
    skos:historyNote "Based on the IUGS classification of metamorphic rocks (Fettes and Desmons, 2007)." ;
    skos:inScheme cs: ;
    skos:notation "mgs"^^:gswa-rock-code ;
    skos:prefLabel "granitic schist"@en ;
.

:granodiorite
    a skos:Concept ;
    rdfs:isDefinedBy cs: ;
    skos:broader :igneous-felsic-intrusive ;
    skos:definition "An intrusive rock consisting essentially of quartz, sodic plagioclase and lesser amounts of alkali feldspar with minor amounts of hornblende and biotite. Now defined modally in QAPF field 4 (Fig. 2.4, p. 22). (cf. Le Maitre et al., 2005, p. 86)"@en ;
    skos:exactMatch
        <http://inspire.ec.europa.eu/codelist/LithologyValue/granodiorite> ,
        <http://resource.geosciml.org/classifier/cgi/lithology/granodiorite> ;
    skos:historyNote "Based on the IUGS classification of igneous rocks (Le Maitre et al., 2005)." ;
    skos:inScheme cs: ;
    skos:notation "gg"^^:gswa-rock-code ;
    skos:prefLabel "granodiorite"@en ;
    schema:citation "https://glossary.americangeosciences.org/term/granodiorite"^^xsd:anyURI ;
.

:granofels-hornfels
    a skos:Concept ;
    rdfs:isDefinedBy cs: ;
    skos:broader :metamorphic-protolith-unknown-granofels-hornfels ;
    skos:definition "A metamorphic rock for which a protolith cannot be conclusively established and displaying a granofelsic structure, i.e. a structure resulting from the absence of schistosity such that the mineral grains and aggregates of mineral grains are equant (for example quartz, feldspar, garnet and pyroxene) or, if inequant, have a random orientation. Mineralogical or lithological layering may be present. Definition adapted from Fettes and Desmons (2007, p. 156). Hornfels are granofels that are typically formed by contact metasomatism and occur mostly (though not exclusively) in the innermost part of contact aureoles. Definition adapted from Fettes and Desmons (2007, p. 159) and Glossary of geology (5th edition revised; Neuendorf et al., 2011)."@en ;
    skos:historyNote "Based on the IUGS classification of metamorphic rocks (Fettes and Desmons, 2007)." ;
    skos:inScheme cs: ;
    skos:narrowMatch
        <http://inspire.ec.europa.eu/codelist/LithologyValue/granofels> ,
        <http://inspire.ec.europa.eu/codelist/LithologyValue/hornfels> ,
        <http://resource.geosciml.org/classifier/cgi/lithology/granofels> ,
        <http://resource.geosciml.org/classifier/cgi/lithology/hornfels> ;
    skos:notation "me"^^:gswa-rock-code ;
    skos:prefLabel "granofels/hornfels"@en ;
    schema:citation
        "https://glossary.americangeosciences.org/term/granofels"^^xsd:anyURI ,
        "https://glossary.americangeosciences.org/term/hornfels"^^xsd:anyURI ;
.

:granofelsic-granulite
    a skos:Concept ;
    rdfs:isDefinedBy cs: ;
    skos:broader :metamorphic-protolith-unknown-granofels-hornfels ;
    skos:definition "A high-grade metamorphic rock, with a granoblastic texture and little foliation/lineation and in which Fe–Mg silicates are dominantly hydroxyl-free, feldspar is a critical phase, and primary muscovite is absent (cf. Fettes and Desmons, 2007, p. 156). In GSWA usage, this term is reserved for a granofels/hornfels for which a protolith cannot be conclusively established."@en ;
    skos:historyNote "Based on the IUGS classification of metamorphic rocks (Fettes and Desmons, 2007)." ;
    skos:inScheme cs: ;
    skos:notation "meo"^^:gswa-rock-code ;
    skos:prefLabel "granofelsic granulite"@en ;
.

:granofelsic-hornfelsic-hydrothermal-rock
    a skos:Concept ;
    rdfs:isDefinedBy cs: ;
    skos:broader :metamorphosed-hydrothermal ;
    skos:definition "A metamorphosed hydrothermal rock displaying a granofelsic structure, i.e. a granofels/hornfels derived from a hydrothermal protolith. See also definition of granofels/granofelsic structure in Fettes and Desmons (2007, p. 156); hornfels are granofels formed by contact metamorphism (Fettes and Desmons, 2007, p. 159)."@en ;
    skos:historyNote "Based on the IUGS classification of metamorphic rocks (Fettes and Desmons, 2007) and GSWA usage." ;
    skos:inScheme cs: ;
    skos:notation "mze"^^:gswa-rock-code ;
    skos:prefLabel "granofelsic/hornfelsic hydrothermal rock"@en ;
    schema:citation
        "https://en.wikipedia.org/wiki/Hornfels"^^xsd:anyURI ,
        "https://glossary.americangeosciences.org/term/granofels"^^xsd:anyURI ,
        "https://glossary.americangeosciences.org/term/hornfels;"^^xsd:anyURI ,
        "https://glossary.americangeosciences.org/term/hydrothermalalteration"^^xsd:anyURI ;
.

:granofelsic-hornfelsic-marble
    a skos:Concept ;
    rdfs:isDefinedBy cs: ;
    skos:broader :marble ;
    skos:definition "A metamorphosed sedimentary carbonate rock consisting of more than 50% volume of carbonate minerals (calcite and/or aragonite and/or dolomite) and displaying a granofelsic/hornfelsic structure. See also definition of granofels/granofelsic structure in Fettes and Desmons (2007, p. 156); hornfels are granofels formed by contact metamorphism (Fettes and Desmons, 2007, p. 159)."@en ;
    skos:historyNote "Compiled by the Geological Survey of Western Australia" ;
    skos:inScheme cs: ;
    skos:notation "mkke"^^:gswa-rock-code ;
    skos:prefLabel "granofelsic/hornfelsic marble"@en ;
.

:granofelsic-hornfelsic-meta-iron-formation
    a skos:Concept ;
    rdfs:isDefinedBy cs: ;
    skos:altLabel
        "itabirite"@en ,
        "taconite"@en ;
    skos:broader :metasedimentary-other-chemical-meta-iron-formation ;
    skos:definition "A metamorphosed iron formation displaying a granofelsic structure, i.e. a granofels/hornfels derived from a chemical or biochemical sedimentary protolith containing at least 15% iron of sedimentary origin. See also definition of granofels/granofelsic structure in Fettes and Desmons (2007, p. 156); hornfels are granofels formed by contact metamorphism (Fettes and Desmons, 2007, p. 159)."@en ;
    skos:historyNote "Based on the IUGS classification of metamorphic rocks (Fettes and Desmons, 2007) and GSWA usage." ;
    skos:inScheme cs: ;
    skos:notation "mie"^^:gswa-rock-code ;
    skos:prefLabel "granofelsic/hornfelsic meta-iron formation"@en ;
    schema:citation
        "https://glossary.americangeosciences.org/term/granofels"^^xsd:anyURI ,
        "https://glossary.americangeosciences.org/term/hornfels"^^xsd:anyURI ;
.

:granofelsic-hornfelsic-metachert
    a skos:Concept ;
    rdfs:isDefinedBy cs: ;
    skos:broader :metasedimentary-other-chemical ;
    skos:definition "A metamorphosed chert displaying a granofelsic structure, i.e. a granofels/hornfels derived from a chemical or biochemical sedimentary rock largely consisting of silica and/or quartz. See also definition of granofels/granofelsic structure in Fettes and Desmons (2007, p. 156); hornfels are granofels formed by contact metamorphism (Fettes and Desmons, 2007, p. 159)."@en ;
    skos:historyNote "Compiled by the Geological Survey of Western Australia" ;
    skos:inScheme cs: ;
    skos:notation "mce"^^:gswa-rock-code ;
    skos:prefLabel "granofelsic/hornfelsic metachert"@en ;
.

:granofelsic-hornfelsic-para-amphibolite-carbonate
    a skos:Concept ;
    rdfs:isDefinedBy cs: ;
    skos:broader :para-amphibolite-derived-from-carbonate-rock ;
    skos:definition "A metamorphosed amphibole-rich rock derived from a sedimentary carbonate protolith and displaying a granofelsic/hornfelsic structure. See also definition of granofels/granofelsic structure in Fettes and Desmons (2007, p. 156); hornfels are granofels formed by contact metamorphism (Fettes and Desmons, 2007, p. 159)."@en ;
    skos:historyNote "Compiled by the Geological Survey of Western Australia" ;
    skos:inScheme cs: ;
    skos:notation "mkae"^^:gswa-rock-code ;
    skos:prefLabel "granofelsic/hornfelsic para-amphibolite (carbonate)"@en ;
.

:granofelsic-hornfelsic-para-amphibolite-siliciclastic
    a skos:Concept ;
    rdfs:isDefinedBy cs: ;
    skos:broader :para-amphibolite ;
    skos:definition "A metamorphosed amphibole-rich rock derived from a sedimentary siliciclastic protolith and displaying a granofelsic structure. See also definition of granofels/granofelsic structure in Fettes and Desmons (2007, p. 156); hornfels are granofels formed by contact metamorphism (Fettes and Desmons, 2007, p. 159)."@en ;
    skos:historyNote "Compiled by the Geological Survey of Western Australia" ;
    skos:inScheme cs: ;
    skos:notation "mdae"^^:gswa-rock-code ;
    skos:prefLabel "granofelsic/hornfelsic para-amphibolite (siliciclastic)"@en ;
.

:granophyre
    a skos:Concept ;
    rdfs:isDefinedBy cs: ;
    skos:broader :igneous-felsic-intrusive ;
    skos:definition "A porphyritic rock of granite composition in which the groundmass alkali feldspar and quartz are in micrographic intergrowth (Le Maitre et al., 2005, p. 86). A strict and limited usage of the term is encouraged in the GSWA scheme."@en ;
    skos:historyNote "Based on the IUGS classification of igneous rocks (Le Maitre et al., 2005) and GSWA usage." ;
    skos:inScheme cs: ;
    skos:notation "gv"^^:gswa-rock-code ;
    skos:prefLabel "granophyre"@en ;
    schema:citation "https://glossary.americangeosciences.org/term/granophyre"^^xsd:anyURI ;
.

:granule-conglomerate
    a skos:Concept ;
    rdfs:isDefinedBy cs: ;
    skos:altLabel
        "granulestone"@en ,
        "gritstone"@en ,
        "very fine pebble conglomerate"@en ;
    skos:broader :conglomerate ;
    skos:definition "A consolidated rock consisting mainly of granules that are larger than a very coarse sand grain and smaller than a pebble (2–4 mm or -1 to -2 phi units) being somewhat rounded or otherwise modified by abrasion in the course of transport; a consolidated granule gravel. The term very fine pebble conglomerate has been used as a synonym. Adapted from Glossary of geology (5th edition revised; Neuendorf et al., 2011)."@en ;
    skos:historyNote "Wentworth, CK 1922, A scale of grade and class terms for clastic sediments: The Journal of Geology, v. 30, no. 5, p. 377–392, doi:10.1086/622910." ;
    skos:inScheme cs: ;
    skos:notation "su"^^:gswa-rock-code ;
    skos:prefLabel "granule conglomerate"@en ;
    schema:citation "https://glossary.americangeosciences.org/term/granulesed"^^xsd:anyURI ;
.

:graphitic-fault-rock
    a skos:Concept ;
    rdfs:isDefinedBy cs: ;
    skos:broader :metamorphic-protolith-unknown-fault-rock ;
    skos:definition "A rock formed as a result of deformation in a fault zone and distinguished by the presence of graphite/carbon. In GSWA usage, this term is reserved for fault rocks for which a protolith cannot be conclusively established."@en ;
    skos:historyNote "Compiled by the Geological Survey of Western Australia" ;
    skos:inScheme cs: ;
    skos:notation "myg"^^:gswa-rock-code ;
    skos:prefLabel "graphitic fault rock"@en ;
.

:graphitic-gneiss
    a skos:Concept ;
    rdfs:isDefinedBy cs: ;
    skos:broader :metamorphic-protolith-unknown-gneiss ;
    skos:definition "A gneiss distinguished by the presence of graphite/carbon. In GSWA usage, this term is reserved for a gneiss for which a protolith cannot be conclusively established. See also definition of gneiss/gneissose structure in Fettes and Desmons (2007, p.  154–155)."@en ;
    skos:historyNote "Based on the IUGS classification of metamorphic rocks (Fettes and Desmons, 2007) and GSWA usage." ;
    skos:inScheme cs: ;
    skos:notation "mng"^^:gswa-rock-code ;
    skos:prefLabel "graphitic gneiss"@en ;
    schema:citation "https://glossary.americangeosciences.org/term/gneiss"^^xsd:anyURI ;
.

:graphitic-granofels-hornfels
    a skos:Concept ;
    rdfs:isDefinedBy cs: ;
    skos:broader :metamorphic-protolith-unknown-granofels-hornfels ;
    skos:definition "A granofels/hornfels distinguished by the presence of graphite/carbon. In GSWA usage, this term is reserved for a granofels/hornfels for which a protolith cannot be conclusively established."@en ;
    skos:historyNote "Compiled by the Geological Survey of Western Australia" ;
    skos:inScheme cs: ;
    skos:notation "meg"^^:gswa-rock-code ;
    skos:prefLabel "graphitic granofels/hornfels"@en ;
.

:graphitic-schist
    a skos:Concept ;
    rdfs:isDefinedBy cs: ;
    skos:broader :metamorphic-protolith-unknown-schist ;
    skos:definition "A schist distinguished by the presence of graphite/carbon. In GSWA usage, this term is reserved for a schist for which a protolith cannot be conclusively established. See also definition of schist/schistose structure in Fettes and Desmons, 2007, p.  193)."@en ;
    skos:historyNote "Based on the IUGS classification of metamorphic rocks (Fettes and Desmons, 2007) and GSWA usage." ;
    skos:inScheme cs: ;
    skos:notation "msg"^^:gswa-rock-code ;
    skos:prefLabel "graphitic schist"@en ;
.

:greisen
    a skos:Concept ;
    rdfs:isDefinedBy cs: ;
    skos:broader :metasomatic ;
    skos:definition "Medium-temperature metasomatic rock characterized by the presence of quartz and white mica, commonly with topaz, fluorite, tourmaline and locally with amazonite, orthoclase, andalusite and diaspore. Typically greisens may host B, W, Mo, Sn and Ta mineralization. They are associated with high-level late orogenic leucogranites, and form as replacements either in the granite body and/or in a wide range of country rocks. (Fettes and Desmons, 2007, p. 157). Zoning may be present and is characterized by gradients from coarse, crystalline granite, commonly vuggy with miarolitic cavities, through to quartz- and muscovite-rich rocks, which may be locally rich in accessory minerals (e.g. topaz, tourmaline, cassiterite, fluorite, beryl, wolframite, siderite, molybdenite and other sulfide minerals). They may occur as small to large veins, or large zones in the roof of some granites. Greisen is formed by self-generated alteration of a granite and is a class of moderate- to high-temperature magmatic-hydrothermal alteration related to the late-stage release of volatiles dissolved in a magma during the solidification of that magma (https://en.wikipedia.org/wiki/Greisen)."@en ;
    skos:historyNote "Based on the IUGS classification of metamorphic rocks (Fettes and Desmons, 2007)." ;
    skos:inScheme cs: ;
    skos:notation "mjr"^^:gswa-rock-code ;
    skos:prefLabel "greisen"@en ;
    schema:citation
        "https://en.wikipedia.org/wiki/Greisen"^^xsd:anyURI ,
        "https://glossary.americangeosciences.org/term/greisen;"^^xsd:anyURI ;
.

:gypsum-evaporite
    a skos:Concept ;
    rdfs:isDefinedBy cs: ;
    skos:altLabel "gypsum evaporite"@en ;
    skos:broadMatch
        <http://inspire.ec.europa.eu/codelist/LithologyValue/rockGypsumOrAnhydrite> ,
        <http://resource.geosciml.org/classifier/cgi/lithology/rock_gypsum_or_anhydrite> ;
    skos:broader :evaporite ;
    skos:definition "An evaporite consisting predominantly of the mineral gypsum, i.e. of aquated calcium sulfate (CaSO₄·2H₂O)."@en ;
    skos:historyNote "Compiled by the Geological Survey of Western Australia" ;
    skos:inScheme cs: ;
    skos:notation "cvy"^^:gswa-rock-code ;
    skos:prefLabel "gypsum (evaporite)"@en ;
    schema:citation "https://glossary.americangeosciences.org/term/gypsum"^^xsd:anyURI ;
.

:halite-evaporite
    a skos:Concept ;
    rdfs:isDefinedBy cs: ;
    skos:altLabel "halite evaporite"@en ;
    skos:broader :evaporite ;
    skos:definition "An evaporite consisting predominantly of the mineral halite, i.e. of sodium chloride (NaCl)."@en ;
    skos:historyNote "Compiled by the Geological Survey of Western Australia" ;
    skos:inScheme cs: ;
    skos:notation "cvs"^^:gswa-rock-code ;
    skos:prefLabel "halite (evaporite)"@en ;
    schema:citation "https://glossary.americangeosciences.org/term/halite"^^xsd:anyURI ;
.

:harzburgite
    a skos:Concept ;
    rdfs:isDefinedBy cs: ;
    skos:broader :igneous-ultramafic-intrusive ;
    skos:definition "An ultramafic intrusive rock composed essentially of olivine and orthopyroxene. Now defined modally in the ultramafic rock classification (Fig. 2.9, p. 28). (cf. Le Maitre et al., 2005, p. 88)"@en ;
    skos:historyNote "Based on the IUGS classification of igneous rocks (Le Maitre et al., 2005)." ;
    skos:inScheme cs: ;
    skos:notation "aph"^^:gswa-rock-code ;
    skos:prefLabel "harzburgite"@en ;
    schema:citation "https://glossary.americangeosciences.org/term/harzburgite"^^xsd:anyURI ;
.

:hornblende-gabbro
    a skos:Concept ;
    rdfs:isDefinedBy cs: ;
    skos:broader :igneous-mafic-intrusive ;
    skos:definition "A variety of gabbro in which primary hornblende occurs. Now defined modally in the gabbroic rock classification (Fig. 2.6, p. 25). (Le Maitre et al., 2005, p. 90)"@en ;
    skos:historyNote "Based on the IUGS classification of igneous rocks (Le Maitre et al., 2005)." ;
    skos:inScheme cs: ;
    skos:notation "oh"^^:gswa-rock-code ;
    skos:prefLabel "hornblende gabbro"@en ;
    schema:citation "https://glossary.americangeosciences.org/term/hornblendegabbro"^^xsd:anyURI ;
.

:hornblende-peridotite
    a skos:Concept ;
    rdfs:isDefinedBy cs: ;
    skos:broader :igneous-ultramafic-intrusive ;
    skos:definition "An ultramafic intrusive rock consisting essentially of olivine with up to 60% hornblende. Now defined modally in the ultramafic rock classification (Fig. 2.9, p. 28). Adapted from Le Maitre et al. (2005, p. 90)."@en ;
    skos:historyNote "Based on the IUGS classification of igneous rocks (Le Maitre et al., 2005)." ;
    skos:inScheme cs: ;
    skos:notation "ae"^^:gswa-rock-code ;
    skos:prefLabel "hornblende peridotite"@en ;
    schema:citation "https://glossary.americangeosciences.org/term/hornblendeperidotite"^^xsd:anyURI ;
.

:hornblende-pyroxenite
    a skos:Concept ;
    rdfs:isDefinedBy cs: ;
    skos:broader :igneous-ultramafic-intrusive ;
    skos:definition "A collective term for pyroxenites containing up to 40% of amphibole. Now defined modally in the ultramafic rock classification (Fig. 2.9, p. 28). (Le Maitre et al., 2005, p. 90)"@en ;
    skos:historyNote "Based on the IUGS classification of igneous rocks (Le Maitre et al., 2005)." ;
    skos:inScheme cs: ;
    skos:notation "al"^^:gswa-rock-code ;
    skos:prefLabel "hornblende pyroxenite"@en ;
    schema:citation "https://glossary.americangeosciences.org/term/hornblendepyroxenite"^^xsd:anyURI ;
.

:hornblendite
    a skos:Concept ;
    rdfs:isDefinedBy cs: ;
    skos:broader :igneous-ultramafic-intrusive ;
    skos:definition "An ultramafic intrusive rock composed almost entirely of hornblende. Now defined modally in the ultramafic rock classification (Fig. 2.9, p. 28). (Le Maitre et al., 2005, p. 91)"@en ;
    skos:exactMatch
        <http://inspire.ec.europa.eu/codelist/LithologyValue/hornblendite> ,
        <http://resource.geosciml.org/classifier/cgi/lithology/hornblendite> ;
    skos:historyNote "Based on the IUGS classification of igneous rocks (Le Maitre et al., 2005)." ;
    skos:inScheme cs: ;
    skos:notation "ah"^^:gswa-rock-code ;
    skos:prefLabel "hornblendite"@en ;
    schema:citation "https://glossary.americangeosciences.org/term/hornblendite"^^xsd:anyURI ;
.

:hyalo-enstatite-phlogopite-lamproite
    a skos:Concept ;
    rdfs:isDefinedBy cs: ;
    skos:broader :igneous-lamproites ;
    skos:definition "Originally described as a variety of trachyte characterized by the presence of phlogopite and bronzite (= enstatite). Now regarded as an hyalo–enstatite–phlogopite lamproite (Table 2.7, p. 17), where hyalo refers to the presence of glass. The original name fortunite is not recommended for usage. (Le Maitre et al., 2005, p. 82)"@en ;
    skos:historyNote "Based on the IUGS classification of igneous rocks (Le Maitre et al., 2005)." ;
    skos:inScheme cs: ;
    skos:notation "ih"^^:gswa-rock-code ;
    skos:prefLabel "hyalo-enstatite-phlogopite lamproite"@en ;
    schema:citation "https://glossary.americangeosciences.org/term/fortunite"^^xsd:anyURI ;
.

:hyalo-olivine-diopside-phlogopite-lamproite
    a skos:Concept ;
    rdfs:isDefinedBy cs: ;
    skos:broader :igneous-lamproites ;
    skos:definition "Originally described as a black pitch-like rock, associated with an extrusive mass of fortunite [a variety of trachyte characterized by the presence of phlogopite and bronzite (= enstatite). Now regarded as an hyalo-enstatite–phlogopite lamproite], and consisting of phenocrysts of phlogopite and olivine in a glassy matrix containing microlites of diopside and phlogopite. Now regarded as a hyalo-olivine–diopside–phlogopite lamproite (Table 2.7, p. 17). The original name verite is not recommended for usage. (Le Maitre et al., 2005, p. 154)"@en ;
    skos:historyNote "Based on the IUGS classification of igneous rocks (Le Maitre et al., 2005)." ;
    skos:inScheme cs: ;
    skos:notation "iv"^^:gswa-rock-code ;
    skos:prefLabel "hyalo-olivine-diopside-phlogopite lamproite"@en ;
    schema:citation "https://glossary.americangeosciences.org/term/verite"^^xsd:anyURI ;
.

:hydrothermal-breccia
    a skos:Concept ;
    rdfs:isDefinedBy cs: ;
    skos:broader :hydrothermal ;
    skos:definition "A rock composed of angular broken rock fragments held together by a mineral cement / fine-grained matrix forming from the interaction of a rock with hydrothermal (typically water-rich) solutions."@en ;
    skos:historyNote "Jébrak, M 1997, Hydrothermal breccias in vein-type ore deposits: A review of mechanisms, morphology and size distribution: Ore Geology Reviews, v. 12, no. 3, p. 111–134, doi:10.1016/S0169-1368(97)00009-7." ;
    skos:inScheme cs: ;
    skos:notation "zx"^^:gswa-rock-code ;
    skos:prefLabel "hydrothermal breccia"@en ;
    schema:citation "https://en.wikipedia.org/wiki/Breccia"^^xsd:anyURI ;
.

:hydrothermal-chert
    a skos:Concept ;
    rdfs:isDefinedBy cs: ;
    skos:broader :hydrothermal ;
    skos:definition "A fine-grained siliceous rock that precipitated originally from a hydrothermal fluid related to seafloor or sub-seafloor volcanism."@en ;
    skos:historyNote "Compiled by the Geological Survey of Western Australia" ;
    skos:inScheme cs: ;
    skos:notation "zc"^^:gswa-rock-code ;
    skos:prefLabel "hydrothermal chert"@en ;
.

:hydrothermal-rock
    a skos:Concept ;
    rdfs:isDefinedBy cs: ;
    skos:broader :hydrothermal ;
    skos:definition "A rock formed from precipitation from a hot hydrous solution, with or without demonstrable association with igneous processes, otherwise uncategorized."@en ;
    skos:historyNote "Compiled by the Geological Survey of Western Australia" ;
    skos:inScheme cs: ;
    skos:notation "z"^^:gswa-rock-code ;
    skos:prefLabel "hydrothermal rock"@en ;
    schema:citation "https://glossary.americangeosciences.org/term/hydrothermalpetrology"^^xsd:anyURI ;
.

:hydrothermal-rock-undivided
    a skos:Concept ;
    rdfs:isDefinedBy cs: ;
    skos:broader :hydrothermal ;
    skos:definition "A rock formed from precipitation from a hot hydrous solution, with or without demonstrable association with igneous processes, otherwise uncategorized. GSWA usage of this term is restricted to rocks that are partially altered/weathered or are identified using remote sensing imagery."@en ;
    skos:historyNote "Compiled by the Geological Survey of Western Australia" ;
    skos:inScheme cs: ;
    skos:notation "zn"^^:gswa-rock-code ;
    skos:prefLabel "hydrothermal rock; undivided"@en ;
.

:igneous-rock
    a skos:Concept ;
    rdfs:isDefinedBy cs: ;
    skos:broader :igneous ;
    skos:definition "In GSWA usage, a rock of igneous but otherwise unspecified origin, i.e. a rock for which an igneous protolith is interpreted but commonly too weathered to make further distinctions."@en ;
    skos:exactMatch
        <http://inspire.ec.europa.eu/codelist/LithologyValue/igneousRock> ,
        <http://resource.geosciml.org/classifier/cgi/lithology/igneous_rock> ;
    skos:historyNote "Compiled by the Geological Survey of Western Australia" ;
    skos:inScheme cs: ;
    skos:notation "ign"^^:gswa-rock-code ;
    skos:prefLabel "igneous rock"@en ;
.

:impact-melt-rock
    a skos:Concept ;
    rdfs:isDefinedBy cs: ;
    skos:broader :metamorphic-protolith-unknown-impactite ;
    skos:definition "Crystalline, semihyaline or hyaline rock solidified from impact melt and containing variable amounts of clastic debris of different degree of shock metamorphism (Fettes and Desmons, 2007, p. 162)."@en ;
    skos:historyNote "Based on the IUGS classification of metamorphic rocks (Fettes and Desmons, 2007)." ;
    skos:inScheme cs: ;
    skos:notation "mpe"^^:gswa-rock-code ;
    skos:prefLabel "impact-melt rock"@en ;
    schema:citation "https://glossary.americangeosciences.org/term/impactmeltrock"^^xsd:anyURI ;
.

:impactite
    a skos:Concept ;
    rdfs:isDefinedBy cs: ;
    skos:broader :metamorphic-protolith-unknown-impactite ;
    skos:definition "Rock produced by impact metamorphism, otherwise uncategorized. It includes shocked rocks, impact breccias, impact melt rocks, (micro)tektites, and airfall beds (cf. Fettes and Desmons, 2007, p. 162)."@en ;
    skos:historyNote "Based on the IUGS classification of metamorphic rocks (Fettes and Desmons, 2007)." ;
    skos:inScheme cs: ;
    skos:notation "mp"^^:gswa-rock-code ;
    skos:prefLabel "impactite"@en ;
    schema:citation "https://glossary.americangeosciences.org/term/impactite"^^xsd:anyURI ;
.

:impactoclastic-airfall-bed
    a skos:Concept ;
    rdfs:isDefinedBy cs: ;
    skos:broader :distal-impactite ;
    skos:definition "Pelitic sedimentary layer containing a certain fraction of shock-metamorphosed material, e.g. shocked minerals and melt particles, which has been ejected from an impact crater and deposited by interaction with the atmosphere over large regions of a planet or globally. (Fettes and Desmons, 2007, p. 162)"@en ;
    skos:historyNote "Based on the IUGS classification of metamorphic rocks (Fettes and Desmons, 2007)." ;
    skos:inScheme cs: ;
    skos:notation "mpa"^^:gswa-rock-code ;
    skos:prefLabel "impactoclastic airfall bed"@en ;
.

:impactoclastic-deposit
    a skos:Concept ;
    rdfs:isDefinedBy cs: ;
    skos:broader :metamorphic-protolith-unknown-impactite ;
    skos:definition "Consolidated or unconsolidated sediment resulting from ballistic excavation, transport, and deposition of rocks at impact craters. It may contain glassy or crystallized particles of impact melt. (Fettes and Desmons, 2007, p. 162)"@en ;
    skos:historyNote "Based on the IUGS classification of metamorphic rocks (Fettes and Desmons, 2007)." ;
    skos:inScheme cs: ;
    skos:notation "mpo"^^:gswa-rock-code ;
    skos:prefLabel "impactoclastic deposit"@en ;
.

:intrusive-rock
    a skos:Concept ;
    rdfs:isDefinedBy cs: ;
    skos:broader :igneous-intrusive ;
    skos:definition "A rock of igneous intrusive origin but commonly too weathered to make further distinctions."@en ;
    skos:historyNote "Compiled by the Geological Survey of Western Australia" ;
    skos:inScheme cs: ;
    skos:notation "igni"^^:gswa-rock-code ;
    skos:prefLabel "intrusive rock"@en ;
.

:ironstone
    a skos:Concept ;
    rdfs:isDefinedBy cs: ;
    skos:broader :sedimentary-other-chemical-or-biochemical ;
    skos:definition "Any rock containing a substantial proportion of an iron compound, or any iron ore from which the metal may be smelted commercially; specifically an iron-rich sedimentary rock, either deposited directly as a ferruginous sediment or resulting from chemical replacement. The term is customarily applied to a hard, coarsely banded or non-banded, and non-cherty sedimentary rock of post-Precambrian age, in contrast with iron formation. The iron minerals may be oxides (limonite, hematite, magnetite), carbonate (siderite), or silicate (chamosite); most ironstones containing iron oxides or chamosite are oolitic. Adapted from Glossary of geology (5th edition revised; Neuendorf et al., 2011)."@en ;
    skos:historyNote "Based on the Glossary of geology (5th edition, revised; Neuendorf et al. 2011)." ;
    skos:inScheme cs: ;
    skos:notation "ce"^^:gswa-rock-code ;
    skos:prefLabel "ironstone"@en ;
    schema:citation "https://glossary.americangeosciences.org/term/ironstone"^^xsd:anyURI ;
.

:jaspilite
    a skos:Concept ;
    rdfs:isDefinedBy cs: ;
    skos:broader :iron-formation ;
    skos:definition "A banded compact siliceous rock containing at least 25% iron, occurring with iron ores, and resembling jasper, i.e. the variety of chert containing iron-oxide impurities that give it a characteristic red colour."@en ;
    skos:historyNote "Beukes, NJ and Gutzmer, J 2008, Origin and paleoenvironmental significance of major iron formations at the Archean-Paleoproterozoic boundary: Reviews in Economic Geology, v. 15, p. 5–47, doi:10.5382/Rev.15.01." ;
    skos:inScheme cs: ;
    skos:notation "cij"^^:gswa-rock-code ;
    skos:prefLabel "jaspilite"@en ;
    schema:citation "https://glossary.americangeosciences.org/term/jaspilite"^^xsd:anyURI ;
.

:kalsilite-leucite-olivine-melilitite
    a skos:Concept ;
    rdfs:isDefinedBy cs: ;
    skos:broader :igneous-kalsilitic ;
    skos:definition "A potassic melanocratic variety of olivine melilitite composed essentially of olivine and melilite with subordinate leucite, kalsilite, nepheline and perovskite in a glassy matrix. The historical term katungite is considered obsolete. Cf. Tables 2.5 & 2.6 on p. 12, and p. 96 in Le Maitre et al. (2005)."@en ;
    skos:historyNote "Based on the IUGS classification of igneous rocks (Le Maitre et al., 2005). See also https://academic.oup.com/petrology/article/63/5/egac026/6553206." ;
    skos:inScheme cs: ;
    skos:notation "wk"^^:gswa-rock-code ;
    skos:prefLabel "kalsilite-leucite-olivine melilitite"@en ;
    schema:citation "https://glossary.americangeosciences.org/term/katungite"^^xsd:anyURI ;
.

:kalsilite-phlogopite-melilitite
    a skos:Concept ;
    rdfs:isDefinedBy cs: ;
    skos:broader :igneous-kalsilitic ;
    skos:definition "An olivine-free, extrusive melilitite containing small clinopyroxene phenocrysts in a holocrystalline groundmass of melilite, clinopyroxene and phlogopite. The historical term coppaelite is considered obsolete. Cf. Tables 2.5 & 2.6 on p. 12, and p. 70 in Le Maitre et al. (2005)."@en ;
    skos:historyNote "Based on the IUGS classification of igneous rocks (Le Maitre et al., 2005). See also https://academic.oup.com/petrology/article/63/5/egac026/6553206." ;
    skos:inScheme cs: ;
    skos:notation "wc"^^:gswa-rock-code ;
    skos:prefLabel "kalsilite-phlogopite melilitite"@en ;
    schema:citation "https://glossary.americangeosciences.org/term/coppaelite"^^xsd:anyURI ;
.

:kalsilite-phlogopite-olivine-leucite-melilitite
    a skos:Concept ;
    rdfs:isDefinedBy cs: ;
    skos:broader :igneous-kalsilitic ;
    skos:definition "A melanocratic variety of leucite olivine melilitite largely composed of melilite, leucite, kalsilite and olivine. The historical term venanzite is considered obsolete. Cf. Tables 2.5 & 2.6 on p. 12, and p. 154 in Le Maitre et al. (2005)."@en ;
    skos:historyNote "Based on the IUGS classification of igneous rocks (Le Maitre et al., 2005). See also https://academic.oup.com/petrology/article/63/5/egac026/6553206." ;
    skos:inScheme cs: ;
    skos:notation "wv"^^:gswa-rock-code ;
    skos:prefLabel "kalsilite-phlogopite-olivine-leucite melilitite"@en ;
    schema:citation "https://glossary.americangeosciences.org/term/venanzite"^^xsd:anyURI ;
.

:kalsilitite-undivided
    a skos:Concept ;
    rdfs:isDefinedBy cs: ;
    skos:broader :igneous-kalsilitic ;
    skos:definition "An ultramafic volcanic rock defined in the kalsilite-bearing rock classification as a rock containing kalsilite, but no leucite or melilite (Le Maitre et al., 2005, p. 94), but otherwise uncategorized. GSWA's rock classification scheme prefers the use of volcanic terminology for any igneous rock formed on or near the Earth's surface, i.e. for those hypabyssal or subvolcanic rocks such as dykes, sills, and cryptodomes that are demonstrably both spatially and temporally associated with extrusive volcanic rocks. GSWA usage of this term is restricted to rocks that are partially weathered or are identified using remote sensing imagery, and the use of the related code/notation is limited to GSWA's Explanatory Notes System."@en ;
    skos:historyNote "Based on the IUGS classification of igneous rocks (Le Maitre et al., 2005). See also https://academic.oup.com/petrology/article/63/5/egac026/6553206." ;
    skos:inScheme cs: ;
    skos:notation "wn"^^:gswa-rock-code ;
    skos:prefLabel "kalsilitite; undivided"@en ;
.

:kersantite
    a skos:Concept ;
    rdfs:isDefinedBy cs: ;
    skos:broader :igneous-lamprophyres ;
    skos:definition "A variety of lamprophyre consisting of phenocrysts of Mg-biotite, with or without hornblende, olivine or pyroxene in a groundmass of the same minerals plus plagioclase and occasional alkali feldspar. Now defined in the lamprophyre classification (Table 2.9, p. 19). (Le Maitre et al., 2005, p. 97)"@en ;
    skos:historyNote "Based on the IUGS classification of igneous rocks (Le Maitre et al., 2005)." ;
    skos:inScheme cs: ;
    skos:notation "yk"^^:gswa-rock-code ;
    skos:prefLabel "kersantite"@en ;
.

:kimberlite
    a skos:Concept ;
    rdfs:isDefinedBy cs: ;
    skos:broader :igneous-kimberlite ;
    skos:definition "An ultramafic rock consisting of major amounts of serpentinized olivine with variable amounts of phlogopite, orthopyroxene, clinopyroxene, carbonate and chromite. Characteristic accessory minerals include pyrope garnet, monticellite, rutile and perovskite. It cannot be defined but is characterized by the mineralogical criteria given in section 2.6, p. 13. (Le Maitre et al., 2005, p. 97)"@en ;
    skos:historyNote "Based on the IUGS classification of igneous rocks (Le Maitre et al., 2005)." ;
    skos:inScheme cs: ;
    skos:notation "p"^^:gswa-rock-code ;
    skos:prefLabel "kimberlite"@en ;
    schema:citation "https://glossary.americangeosciences.org/glossary-search?search_api_views_fulltext=kimberlite"^^xsd:anyURI ;
.

:kimberlitic-rock-undivided
    a skos:Concept ;
    rdfs:isDefinedBy cs: ;
    skos:broader :igneous-kimberlite ;
    skos:definition "A rock of kimberlitic affinity (i.e. defined as containing at least 35% olivine and no leucite), but otherwise uncategorized. GSWA usage of this term is restricted to rocks that are partially weathered or are identified using remote sensing imagery, and the use of the related code/notation is limited to GSWA's Explanatory Notes System."@en ;
    skos:historyNote "Based on the IUGS classification of igneous rocks (Le Maitre et al., 2005) and GSWA usage." ;
    skos:inScheme cs: ;
    skos:notation "pn"^^:gswa-rock-code ;
    skos:prefLabel "kimberlitic rock; undivided"@en ;
.

:kimberlitic-volcaniclastic-breccia
    a skos:Concept ;
    rdfs:isDefinedBy cs: ;
    skos:broader :igneous-kimberlite ;
    skos:definition "A volcaniclastic rock of kimberlitic affinity composed mostly of angular fragments greater than 2 mm in size consisting of either (a) pyroclastic detritus or (b) terrigenous volcanic detritus of epiclastic origin. 'Volcaniclastic' includes all clastic volcanic materials formed by any process of fragmentation, dispersed by any kind of transporting agent, deposited in any environment, or mixed in any significant portion with non-volcanic fragments."@en ;
    skos:historyNote "Compiled by the Geological Survey of Western Australia" ;
    skos:inScheme cs: ;
    skos:notation "pvb"^^:gswa-rock-code ;
    skos:prefLabel "kimberlitic volcaniclastic breccia"@en ;
.

:kimberlitic-volcaniclastic-breccia-sandstone
    a skos:Concept ;
    rdfs:isDefinedBy cs: ;
    skos:broader :igneous-kimberlite ;
    skos:definition "A volcaniclastic rock of kimberlitic affinity composed mostly of angular fragments ranging in size from sand (0.0625 – 2 mm) and above, consisting of either (a) pyroclastic detritus or (b) terrigenous volcanic detritus of epiclastic origin. 'Volcaniclastic' includes all clastic volcanic materials formed by any process of fragmentation, dispersed by any kind of transporting agent, deposited in any environment, or mixed in any significant portion with non-volcanic fragments."@en ;
    skos:historyNote "Compiled by the Geological Survey of Western Australia" ;
    skos:inScheme cs: ;
    skos:notation "pvbs"^^:gswa-rock-code ;
    skos:prefLabel "kimberlitic volcaniclastic breccia-sandstone"@en ;
.

:kimberlitic-volcaniclastic-conglomerate
    a skos:Concept ;
    rdfs:isDefinedBy cs: ;
    skos:broader :igneous-kimberlite ;
    skos:definition "A conglomerate of kimberlitic affinity consisting of either (a) pyroclastic detritus or (b) terrigenous volcanic detritus of epiclastic origin. 'Volcaniclastic' includes all clastic volcanic materials formed by any process of fragmentation, dispersed by any kind of transporting agent, deposited in any environment, or mixed in any significant portion with non-volcanic fragments."@en ;
    skos:historyNote "Compiled by the Geological Survey of Western Australia" ;
    skos:inScheme cs: ;
    skos:notation "pvc"^^:gswa-rock-code ;
    skos:prefLabel "kimberlitic volcaniclastic conglomerate"@en ;
.

:kimberlitic-volcaniclastic-granule-pebble-breccia
    a skos:Concept ;
    rdfs:isDefinedBy cs: ;
    skos:broader :igneous-kimberlite ;
    skos:definition "A breccia of kimberlitic affinity composed mostly of angular fragments ranging in size from granule (2–4 mm) to pebble (4–32 mm) consisting of either (a) pyroclastic detritus or (b) terrigenous volcanic detritus of epiclastic origin. 'Volcaniclastic' includes all clastic volcanic materials formed by any process of fragmentation, dispersed by any kind of transporting agent, deposited in any environment, or mixed in any significant portion with non-volcanic fragments."@en ;
    skos:historyNote "Compiled by the Geological Survey of Western Australia" ;
    skos:inScheme cs: ;
    skos:notation "pvg"^^:gswa-rock-code ;
    skos:prefLabel "kimberlitic volcaniclastic granule/pebble breccia"@en ;
.

:kimberlitic-volcaniclastic-mudstone
    a skos:Concept ;
    rdfs:isDefinedBy cs: ;
    skos:broader :igneous-kimberlite ;
    skos:definition "A mudstone (grain size ranging from silt to clay, i.e. less than 0.0625 mm) of kimberlitic affinity consisting of either (a) pyroclastic detritus or (b) terrigenous volcanic detritus of epiclastic origin. 'Volcaniclastic' includes all clastic volcanic materials formed by any process of fragmentation, dispersed by any kind of transporting agent, deposited in any environment, or mixed in any significant portion with non-volcanic fragments."@en ;
    skos:historyNote "Compiled by the Geological Survey of Western Australia" ;
    skos:inScheme cs: ;
    skos:notation "pvsm"^^:gswa-rock-code ;
    skos:prefLabel "kimberlitic volcaniclastic mudstone"@en ;
.

:kimberlitic-volcaniclastic-rock
    a skos:Concept ;
    rdfs:isDefinedBy cs: ;
    skos:broader :igneous-kimberlite ;
    skos:definition "A volcaniclastic rock of kimberlitic affinity consisting of either (a) pyroclastic detritus or (b) terrigenous volcanic detritus of epiclastic origin, but otherwise uncategorized. 'Volcaniclastic' includes all clastic volcanic materials formed by any process of fragmentation, dispersed by any kind of transporting agent, deposited in any environment, or mixed in any significant portion with non-volcanic fragments."@en ;
    skos:historyNote "Compiled by the Geological Survey of Western Australia" ;
    skos:inScheme cs: ;
    skos:notation "pvr"^^:gswa-rock-code ;
    skos:prefLabel "kimberlitic volcaniclastic rock"@en ;
.

:kimberlitic-volcaniclastic-sandstone
    a skos:Concept ;
    rdfs:isDefinedBy cs: ;
    skos:broader :igneous-kimberlite ;
    skos:definition "A sandstone (grain size 0.0625 – 2 mm) of kimberlitic affinity consisting of either (a) pyroclastic detritus or (b) terrigenous volcanic detritus of epiclastic origin. 'Volcaniclastic' includes all clastic volcanic materials formed by any process of fragmentation, dispersed by any kind of transporting agent, deposited in any environment, or mixed in any significant portion with non-volcanic fragments."@en ;
    skos:historyNote "Compiled by the Geological Survey of Western Australia" ;
    skos:inScheme cs: ;
    skos:notation "pvs"^^:gswa-rock-code ;
    skos:prefLabel "kimberlitic volcaniclastic sandstone"@en ;
.

:kimberlitic-volcaniclastic-sandstone-siltstone
    a skos:Concept ;
    rdfs:isDefinedBy cs: ;
    skos:broader :igneous-kimberlite ;
    skos:definition "A volcaniclastic rock of komatiitic affinity composed mostly of fragments ranging in size from sand (0.0625 – 2 mm) to silt (0.0039 – 0.0625 mm) of either (a) pyroclastic detritus or (b) terrigenous volcanic detritus of epiclastic origin, and with an overall mafic composition. 'Volcaniclastic' includes all clastic volcanic materials formed by any process of fragmentation, dispersed by any kind of transporting agent, deposited in any environment, or mixed in any significant portion w, and with an overall mafic composition."@en ;
    skos:historyNote "Compiled by the Geological Survey of Western Australia" ;
    skos:inScheme cs: ;
    skos:notation "pvss"^^:gswa-rock-code ;
    skos:prefLabel "kimberlitic volcaniclastic sandstone-siltstone"@en ;
.

:kimberlitic-volcaniclastic-sediment-matrix-breccia
    a skos:Concept ;
    rdfs:isDefinedBy cs: ;
    skos:broader :igneous-kimberlite ;
    skos:definition "A commonly monomictic breccia of kimberlitic affinity composed of angular, coarse igneous fragments cemented by a fine-grained matrix that is clastic though not necessarily strictly sedimentary in origin. 'Volcaniclastic' includes all clastic volcanic materials formed by any process of fragmentation, dispersed by any kind of transporting agent, deposited in any environment, or mixed in any significant portion with non-volcanic fragments."@en ;
    skos:historyNote "Compiled by the Geological Survey of Western Australia" ;
    skos:inScheme cs: ;
    skos:notation "pvsb"^^:gswa-rock-code ;
    skos:prefLabel "kimberlitic volcaniclastic sediment-matrix breccia"@en ;
.

:komatiite
    a skos:Concept ;
    rdfs:isDefinedBy cs: ;
    skos:broader :igneous-ultramafic-volcanic-and-volcaniclastic ;
    skos:definition "A variety of ultramafic lavas that crystallizes from high temperature magmas with 18% to 32% MgO. They commonly form pillows and have chilled flow-tops and usually display well-developed spinifex textures with intergrown skeletal and bladed olivine and pyroxene crystals set in abundant glass. The more highly magnesian varieties are often termed peridotitic komatiite. Now defined chemically in the TAS classification (Fig. 2.13, p. 34). (Le Maitre et al., 2005, p. 98)"@en ;
    skos:historyNote "Based on the IUGS classification of igneous rocks (Le Maitre et al., 2005)." ;
    skos:inScheme cs: ;
    skos:notation "uk"^^:gswa-rock-code ;
    skos:prefLabel "komatiite"@en ;
    schema:citation "https://glossary.americangeosciences.org/term/komatiite"^^xsd:anyURI ;
.

:komatiitic-basalt
    a skos:Concept ;
    rdfs:isDefinedBy cs: ;
    skos:altLabel "basaltic komatiite"@en ;
    skos:broader :igneous-mafic-volcanic ;
    skos:definition "A member of the komatiite series with MgO in the range 5 to 15%, typically displaying pyroxene spinifex texture and evidence of rapid quenching of high-temperature magma. Chemically these rocks are intermediate between tholeiitic basalt and boninite and are thought to have been komatiite magmas contaminated by crustal material. Definition adapted from Le Maitre et al. (2005, p. 61). GSWA usage of the term is restricted to basaltic rocks related to komatiites where petrography or geochemistry has also confirmed a high-magnesium composition."@en ;
    skos:historyNote "Based on the IUGS classification of igneous rocks (Le Maitre et al., 2005)." ;
    skos:inScheme cs: ;
    skos:notation "bk"^^:gswa-rock-code ;
    skos:prefLabel "komatiitic basalt"@en ;
    schema:citation "https://glossary.americangeosciences.org/term/basaltickomatiite"^^xsd:anyURI ;
.

:lamproite
    a skos:Concept ;
    rdfs:isDefinedBy cs: ;
    skos:broader :igneous-lamproites ;
    skos:definition "A hypabyssal or extrusive rock rich in potassium and magnesium, otherwise uncategorized."@en ;
    skos:historyNote "Based on the IUGS classification of igneous rocks (Le Maitre et al., 2005) and GSWA usage." ;
    skos:inScheme cs: ;
    skos:notation "i"^^:gswa-rock-code ;
    skos:prefLabel "lamproite"@en ;
    schema:citation "https://glossary.americangeosciences.org/term/lamproite"^^xsd:anyURI ;
.

:lamproitic-rock-undivided
    a skos:Concept ;
    rdfs:isDefinedBy cs: ;
    skos:broader :igneous-lamproites ;
    skos:definition "A demonstrably felsic igneous volcanic rocks, otherwise uncategorized. GSWA usage of this term is restricted to rocks that are partially weathered or are identified using remote sensing imagery, and the use of the related code/notation is limited to GSWA's Explanatory Notes System. GSWA's rock classification scheme prefers the use of volcanic terminology for any igneous rock formed on or near the Earth's surface, i.e. for those hypabyssal or subvolcanic rocks such as dykes, sills, and cryptodomes that are demonstrably both spatially and temporally associated with extrusive volcanic rocks."@en ;
    skos:historyNote "Based on the IUGS classification of igneous rocks (Le Maitre et al., 2005) and GSWA usage." ;
    skos:inScheme cs: ;
    skos:notation "in"^^:gswa-rock-code ;
    skos:prefLabel "lamproitic rock; undivided"@en ;
.

:lamproitic-volcaniclastic-breccia
    a skos:Concept ;
    rdfs:isDefinedBy cs: ;
    skos:broader :igneous-lamproites ;
    skos:definition "A volcaniclastic rock composed mostly of angular fragments greater than 2 mm in size consisting of either (a) pyroclastic detritus or (b) terrigenous volcanic detritus of epiclastic origin, and with a lamproitic composition. 'Volcaniclastic' includes all clastic volcanic materials formed by any process of fragmentation, dispersed by any kind of transporting agent, deposited in any environment, or mixed in any significant portion with non-volcanic fragments."@en ;
    skos:historyNote "Compiled by the Geological Survey of Western Australia" ;
    skos:inScheme cs: ;
    skos:notation "ivb"^^:gswa-rock-code ;
    skos:prefLabel "lamproitic volcaniclastic breccia"@en ;
.

:lamproitic-volcaniclastic-breccia-sandstone
    a skos:Concept ;
    rdfs:isDefinedBy cs: ;
    skos:broader :igneous-lamproites ;
    skos:definition "A volcaniclastic rock composed mostly of angular fragments ranging in size from sand (0.0625 – 2 mm) and above, consisting of either (a) pyroclastic detritus or (b) terrigenous volcanic detritus of epiclastic origin, and with a lamproitic composition. 'Volcaniclastic' includes all clastic volcanic materials formed by any process of fragmentation, dispersed by any kind of transporting agent, deposited in any environment, or mixed in any significant portion with non-volcanic fragments."@en ;
    skos:historyNote "Compiled by the Geological Survey of Western Australia" ;
    skos:inScheme cs: ;
    skos:notation "ivbs"^^:gswa-rock-code ;
    skos:prefLabel "lamproitic volcaniclastic breccia-sandstone"@en ;
.

:lamproitic-volcaniclastic-conglomerate
    a skos:Concept ;
    rdfs:isDefinedBy cs: ;
    skos:broader :igneous-lamproites ;
    skos:definition "A conglomerate consisting of either (a) pyroclastic detritus or (b) terrigenous volcanic detritus of epiclastic origin, and with a lamproitic composition. 'Volcaniclastic' includes all clastic volcanic materials formed by any process of fragmentation, dispersed by any kind of transporting agent, deposited in any environment, or mixed in any significant portion with non-volcanic fragments."@en ;
    skos:historyNote "Compiled by the Geological Survey of Western Australia" ;
    skos:inScheme cs: ;
    skos:notation "ivc"^^:gswa-rock-code ;
    skos:prefLabel "lamproitic volcaniclastic conglomerate"@en ;
.

:lamproitic-volcaniclastic-granule-pebble-breccia
    a skos:Concept ;
    rdfs:isDefinedBy cs: ;
    skos:broader :igneous-lamproites ;
    skos:definition "A breccia composed mostly of angular fragments ranging in size from granule (2–4 mm) to pebble (4–32 mm) consisting of either (a) pyroclastic detritus or (b) terrigenous volcanic detritus of epiclastic origin, and with a lamproitic composition. 'Volcaniclastic' includes all clastic volcanic materials formed by any process of fragmentation, dispersed by any kind of transporting agent, deposited in any environment, or mixed in any significant portion with non-volcanic fragments."@en ;
    skos:historyNote "Compiled by the Geological Survey of Western Australia" ;
    skos:inScheme cs: ;
    skos:notation "ivg"^^:gswa-rock-code ;
    skos:prefLabel "lamproitic volcaniclastic granule/pebble breccia"@en ;
.

:lamproitic-volcaniclastic-mudstone
    a skos:Concept ;
    rdfs:isDefinedBy cs: ;
    skos:broader :igneous-lamproites ;
    skos:definition "A mudstone (grain size ranging from silt to clay, i.e. less than 0.0625 mm) consisting of either (a) pyroclastic detritus or (b) terrigenous volcanic detritus of epiclastic origin, and a lamproitic composition. 'Volcaniclastic' includes all clastic volcanic materials formed by any process of fragmentation, dispersed by any kind of transporting agent, deposited in any environment, or mixed in any significant portion with non-volcanic fragments."@en ;
    skos:historyNote "Compiled by the Geological Survey of Western Australia" ;
    skos:inScheme cs: ;
    skos:notation "ivsm"^^:gswa-rock-code ;
    skos:prefLabel "lamproitic volcaniclastic mudstone"@en ;
.

:lamproitic-volcaniclastic-rock
    a skos:Concept ;
    rdfs:isDefinedBy cs: ;
    skos:broader :igneous-lamproites ;
    skos:definition "A volcaniclastic rock consisting of either (a) pyroclastic detritus or (b) terrigenous volcanic detritus of epiclastic origin, and with a lamproitic composition, but otherwise uncategorized. 'Volcaniclastic' includes all clastic volcanic materials formed by any process of fragmentation, dispersed by any kind of transporting agent, deposited in any environment, or mixed in any significant portion with non-volcanic fragments."@en ;
    skos:historyNote "Compiled by the Geological Survey of Western Australia" ;
    skos:inScheme cs: ;
    skos:notation "ivr"^^:gswa-rock-code ;
    skos:prefLabel "lamproitic volcaniclastic rock"@en ;
.

:lamproitic-volcaniclastic-sandstone
    a skos:Concept ;
    rdfs:isDefinedBy cs: ;
    skos:broader :igneous-lamproites ;
    skos:definition "A sandstone (grain size 0.0625 – 2 mm) consisting of either (a) pyroclastic detritus or (b) terrigenous volcanic detritus of epiclastic origin, and with a lamproitic composition. 'Volcaniclastic' includes all clastic volcanic materials formed by any process of fragmentation, dispersed by any kind of transporting agent, deposited in any environment, or mixed in any significant portion with non-volcanic fragments."@en ;
    skos:historyNote "Compiled by the Geological Survey of Western Australia" ;
    skos:inScheme cs: ;
    skos:notation "ivs"^^:gswa-rock-code ;
    skos:prefLabel "lamproitic volcaniclastic sandstone"@en ;
.

:lamproitic-volcaniclastic-sandstone-siltstone
    a skos:Concept ;
    rdfs:isDefinedBy cs: ;
    skos:broader :igneous-lamproites ;
    skos:definition "A volcaniclastic rock composed mostly of fragments ranging in size from sand (0.0625 – 2 mm) to silt (0.0039 – 0.0625 mm) of either (a) pyroclastic detritus or (b) terrigenous volcanic detritus of epiclastic origin, and with a lamproitic composition. 'Volcaniclastic' includes all clastic volcanic materials formed by any process of fragmentation, dispersed by any kind of transporting agent, deposited in any environment, or mixed in any significant portion with non-volcanic fragments."@en ;
    skos:historyNote "Compiled by the Geological Survey of Western Australia" ;
    skos:inScheme cs: ;
    skos:notation "ivss"^^:gswa-rock-code ;
    skos:prefLabel "lamproitic volcaniclastic sandstone-siltstone"@en ;
.

:lamproitic-volcaniclastic-sediment-matrix-breccia
    a skos:Concept ;
    rdfs:isDefinedBy cs: ;
    skos:broader :igneous-lamproites ;
    skos:definition "A commonly monomictic breccia of overall lamproitic composition, composed of angular, coarse igneous fragments cemented by a fine-grained matrix that is clastic though not necessarily strictly sedimentary in origin. 'Volcaniclastic' includes all clastic volcanic materials formed by any process of fragmentation, dispersed by any kind of transporting agent, deposited in any environment, or mixed in any significant portion with non-volcanic fragments."@en ;
    skos:historyNote "Compiled by the Geological Survey of Western Australia" ;
    skos:inScheme cs: ;
    skos:notation "ivsb"^^:gswa-rock-code ;
    skos:prefLabel "lamproitic volcaniclastic sediment-matrix breccia"@en ;
.

:lamprophyre
    a skos:Concept ;
    rdfs:isDefinedBy cs: ;
    skos:broader :igneous-lamprophyres ;
    skos:definition "A porphyritic, meso- to melanocratic igneous rock with mafic minerals as phenocrysts, typically containing essential biotite (or Fe-phlogopite) and/or amphibole and sometimes clinopyroxene, with feldspars and/or feldspathoid (when present) restricted to the groundmass, but otherwise uncategorized. They are commonly altered and normally occur as dykes. Adapted from Le Maitre et al. (2005, p. 19)."@en ;
    skos:historyNote "Based on the IUGS classification of igneous rocks (Le Maitre et al., 2005)." ;
    skos:inScheme cs: ;
    skos:notation "y"^^:gswa-rock-code ;
    skos:prefLabel "lamprophyre"@en ;
    schema:citation "https://glossary.americangeosciences.org/term/lamprophyre"^^xsd:anyURI ;
.

:lamprophyre-undivided
    a skos:Concept ;
    rdfs:isDefinedBy cs: ;
    skos:broader :igneous-lamprophyres ;
    skos:definition "A lamprophyric rock, otherwise uncategorized. GSWA usage of this term is restricted to rocks that are partially weathered or are identified using remote sensing imagery, and the use of the related code/notation is limited to GSWA's Explanatory Notes System."@en ;
    skos:historyNote "Based on the IUGS classification of igneous rocks (Le Maitre et al., 2005) and GSWA usage." ;
    skos:inScheme cs: ;
    skos:notation "yn"^^:gswa-rock-code ;
    skos:prefLabel "lamprophyre; undivided"@en ;
.

:latite
    a skos:Concept ;
    rdfs:isDefinedBy cs: ;
    skos:broader :igneous-felsic-volcanic ;
    skos:definition "A term originally proposed for a rock which chemically lies between trachyte and andesite, but later used as a volcanic rock composed of approximately equal amounts of alkali feldspar and sodic plagioclase, i.e. the volcanic equivalent of monzonite. Now defined modally in QAPF field 8 (Fig. 2.11, p. 31) and, if modes are not available, chemically as the potassic variety of trachyandesite in TAS field S3 (Fig. 2.14, p. 35). Definition from Le Maitre et al. (2005, p. 101). GSWA's rock classification scheme prefers the use of volcanic terminology for any igneous rock formed on or near the Earth's surface, i.e. for those hypabyssal or subvolcanic rocks such as dykes, sills, and cryptodomes that are demonstrably both spatially and temporally associated with extrusive volcanic rocks."@en ;
    skos:exactMatch
        <http://inspire.ec.europa.eu/codelist/LithologyValue/latite> ,
        <http://resource.geosciml.org/classifier/cgi/lithology/latite> ;
    skos:historyNote "Based on the IUGS classification of igneous rocks (Le Maitre et al., 2005)." ;
    skos:inScheme cs: ;
    skos:notation "fl"^^:gswa-rock-code ;
    skos:prefLabel "latite"@en ;
    schema:citation "https://glossary.americangeosciences.org/term/latite"^^xsd:anyURI ;
.

:leucite-phlogopite-lamproite
    a skos:Concept ;
    rdfs:isDefinedBy cs: ;
    skos:broader :igneous-lamproites ;
    skos:definition "A lamproite (Table 2.7, p. 17) consisting essentially of leucite and phlogopite in a chlorite-rich groundmass. The original name fitzroyite is not recommended for usage. Adapted from Le Maitre et al. (2005, p. 80)."@en ;
    skos:historyNote "Based on the IUGS classification of igneous rocks (Le Maitre et al., 2005)." ;
    skos:inScheme cs: ;
    skos:notation "if"^^:gswa-rock-code ;
    skos:prefLabel "leucite-phlogopite lamproite"@en ;
    schema:citation "https://glossary.americangeosciences.org/term/fitzroyite"^^xsd:anyURI ;
.

:leucite-richterite-lamproite
    a skos:Concept ;
    rdfs:isDefinedBy cs: ;
    skos:broader :igneous-lamproites ;
    skos:definition "Originally described as a rock consisting essentially of leucite and magnophorite (= titanian potassian richterite) with subordinate phlogopite in a glassy matrix. Now regarded as a leucite–richterite lamproite (Table 2.7, p. 17). The original name mamilite is not recommended for usage. Adapted from Le Maitre et al. (2005, p. 108)."@en ;
    skos:historyNote "Based on the IUGS classification of igneous rocks (Le Maitre et al., 2005)." ;
    skos:inScheme cs: ;
    skos:notation "ir"^^:gswa-rock-code ;
    skos:prefLabel "leucite-richterite lamproite"@en ;
.

:lherzolite
    a skos:Concept ;
    rdfs:isDefinedBy cs: ;
    skos:broader :igneous-ultramafic-intrusive ;
    skos:definition "An ultramafic intrusive rock composed of olivine with subordinate orthopyroxene and clinopyroxene. Now defined modally in the ultramafic rock classification (Fig. 2.9, p. 28). (cf. Le Maitre et al., 2005, p. 104)"@en ;
    skos:historyNote "Based on the IUGS classification of igneous rocks (Le Maitre et al., 2005)." ;
    skos:inScheme cs: ;
    skos:notation "apl"^^:gswa-rock-code ;
    skos:prefLabel "lherzolite"@en ;
    schema:citation "https://glossary.americangeosciences.org/term/lherzolite"^^xsd:anyURI ;
.

:lignite
    a skos:Concept ;
    rdfs:isDefinedBy cs: ;
    skos:altLabel "brown coal"@en ;
    skos:broader :coal ;
    skos:definition "A brownish-black coal that is intermediate in coalification between peat and sub-bituminous coal; consolidated coal with a calorific value less than 8 300 BTU/lb (19.31 MJ/kg), on a moist, mineral-matter-free basis. Adapted from Glossary of geology (5th edition revised; Neuendorf et al., 2011)."@en ;
    skos:exactMatch
        <http://inspire.ec.europa.eu/codelist/LithologyValue/lignite> ,
        <http://resource.geosciml.org/classifier/cgi/lithology/lignite> ;
    skos:historyNote "Forsman, JP and Hunt, JM 1958, Insoluble organic matter (kerogen) in sedimentary rocks: Geochimica et Cosmochimica Acta, v. 15(3), p. 170–182, doi.org/10.1016/0016-7037(58)90055-3." ;
    skos:inScheme cs: ;
    skos:notation "con"^^:gswa-rock-code ;
    skos:prefLabel "lignite"@en ;
    schema:citation "https://glossary.americangeosciences.org/term/lignite"^^xsd:anyURI ;
.

:limestone-bafflestone
    a skos:Concept ;
    rdfs:isDefinedBy cs: ;
    skos:altLabel "bafflestone"@en ;
    skos:broader :limestone-boundstone ;
    skos:definition "A type of reef rock or boundstone composed of upright, branching colonies, closely to widely spaced but not in contact, separated by fine sediment or coarse skeletal debris, in which calcite is prevalent over other carbonate minerals. In life, the colonies functioned as a sediment trap or baffle. Adapted from Glossary of geology (5th edition revised; Neuendorf et al., 2011). The limestone prefix is commonly omitted since it is implied by Dunham's (1962) classification."@en ;
    skos:historyNote """Dunham, RJ 1962, Classification of carbonate rocks according to depositional texture, in Classification of carbonate rocks edited by WE Hamm: American Association of Petroleum Geologists, Tulsa, Oklahoma, USA, p. 108–121.,
Embry, AF, Klovan, JE 1971, A late Devonian reef tract on northeastern Banks Island, N.W.T: Bulletin of Canadian Petroleum Geology, v. 19(4), p. 730–781.""" ;
    skos:inScheme cs: ;
    skos:notation "klj"^^:gswa-rock-code ;
    skos:prefLabel "limestone bafflestone"@en ;
    schema:citation "https://glossary.americangeosciences.org/term/bafflestone"^^xsd:anyURI ;
.

:limestone-bindstone
    a skos:Concept ;
    rdfs:isDefinedBy cs: ;
    skos:altLabel "bindstone"@en ;
    skos:broader :limestone-boundstone ;
    skos:definition "A type of reef rock or boundstone composed of sheet-like colonies encrusting large fossil fragments or finer sediment, forming a layered mass that is partly in-place skeletal and partly bioclastic, and in which calcite is prevalent over other carbonate minerals. Adapted from Glossary of geology (5th edition revised; Neuendorf et al., 2011). The limestone prefix is commonly omitted since it is implied by Dunham's (1962) classification."@en ;
    skos:historyNote """Dunham, RJ 1962, Classification of carbonate rocks according to depositional texture, in Classification of carbonate rocks edited by WE Hamm: American Association of Petroleum Geologists, Tulsa, Oklahoma, USA, p. 108–121.,
Embry, AF, Klovan, JE 1971, A late Devonian reef tract on northeastern Banks Island, N.W.T: Bulletin of Canadian Petroleum Geology, v. 19(4), p. 730–781.""" ;
    skos:inScheme cs: ;
    skos:notation "kli"^^:gswa-rock-code ;
    skos:prefLabel "limestone bindstone"@en ;
    schema:citation "https://glossary.americangeosciences.org/term/bindstone"^^xsd:anyURI ;
.

:limestone-breccia
    a skos:Concept ;
    rdfs:isDefinedBy cs: ;
    skos:broader :limestone ;
    skos:definition "A sedimentary breccia consisting of angular limestone clasts and carbonate cement."@en ;
    skos:historyNote "Compiled by the Geological Survey of Western Australia" ;
    skos:inScheme cs: ;
    skos:notation "klx"^^:gswa-rock-code ;
    skos:prefLabel "limestone breccia"@en ;
.

:limestone-floatstone
    a skos:Concept ;
    rdfs:isDefinedBy cs: ;
    skos:altLabel "floatstone"@en ;
    skos:broader :limestone ;
    skos:definition "A carbonate rock with dominant calcite and containing a few bioclasts or other fragments more than 2 mm in diameter, widely spaced, embedded in sand- or mud-size carbonate sediment that forms over 90% of the rock. Adapted from Glossary of geology (5th edition revised; Neuendorf et al., 2011). The limestone prefix is commonly omitted since it is implied by Dunham's (1962) classification."@en ;
    skos:historyNote """Dunham, RJ 1962, Classification of carbonate rocks according to depositional texture, in Classification of carbonate rocks edited by WE Hamm: American Association of Petroleum Geologists, Tulsa, Oklahoma, USA, p. 108–121.,
Embry, AF, Klovan, JE 1971, A late Devonian reef tract on northeastern Banks Island, N.W.T: Bulletin of Canadian Petroleum Geology, v. 19(4), p. 730–781.""" ;
    skos:inScheme cs: ;
    skos:notation "klf"^^:gswa-rock-code ;
    skos:prefLabel "limestone floatstone"@en ;
    schema:citation "https://glossary.americangeosciences.org/term/floatstonesed"^^xsd:anyURI ;
.

:limestone-framestone
    a skos:Concept ;
    rdfs:isDefinedBy cs: ;
    skos:altLabel "framestone"@en ;
    skos:broadMatch
        <http://inspire.ec.europa.eu/codelist/LithologyValue/framestone> ,
        <http://resource.geosciml.org/classifier/cgi/lithology/framestone> ;
    skos:broader :limestone-boundstone ;
    skos:definition "A type of reef rock or boundstone consisting of colonies, shells, or skeletons attached to each other to form a rigid framework or lattice, and consisting mostly of calcite. Internal cavities are filled with fine sediment, crystalline cement, or coarse skeletal debris. Adapted from Glossary of geology (5th edition revised; Neuendorf et al., 2011). The limestone prefix is commonly omitted since it is implied by Dunham's (1962) classification."@en ;
    skos:historyNote """Dunham, RJ 1962, Classification of carbonate rocks according to depositional texture, in Classification of carbonate rocks edited by WE Hamm: American Association of Petroleum Geologists, Tulsa, Oklahoma, USA, p. 108–121.,
Embry, AF, Klovan, JE 1971, A late Devonian reef tract on northeastern Banks Island, N.W.T: Bulletin of Canadian Petroleum Geology, v. 19(4), p. 730–781.""" ;
    skos:inScheme cs: ;
    skos:notation "kle"^^:gswa-rock-code ;
    skos:prefLabel "limestone framestone"@en ;
    schema:citation "https://glossary.americangeosciences.org/term/framestone"^^xsd:anyURI ;
.

:limestone-grainstone
    a skos:Concept ;
    rdfs:isDefinedBy cs: ;
    skos:altLabel "grainstone"@en ;
    skos:broadMatch
        <http://inspire.ec.europa.eu/codelist/LithologyValue/grainstone> ,
        <http://resource.geosciml.org/classifier/cgi/lithology/grainstone> ;
    skos:broader :limestone ;
    skos:definition "A mud-free (less than 1% of material with diameters less than 20 μm), grain-supported, carbonate sedimentary rock, and consisting mostly of calcite. It may be current-laid or formed by mud being washed out from previously deposited sediment, or it may result from mud being bypassed while locally produced particles accumulated (Dunham, 1962). Adapted from Glossary of geology (5th edition revised; Neuendorf et al., 2011). The limestone prefix is commonly omitted since it is implied by Dunham's (1962) classification."@en ;
    skos:historyNote """Dunham, RJ 1962, Classification of carbonate rocks according to depositional texture, in Classification of carbonate rocks edited by WE Hamm: American Association of Petroleum Geologists, Tulsa, Oklahoma, USA, p. 108–121.,
Embry, AF, Klovan, JE 1971, A late Devonian reef tract on northeastern Banks Island, N.W.T: Bulletin of Canadian Petroleum Geology, v. 19(4), p. 730–781.""" ;
    skos:inScheme cs: ;
    skos:notation "klg"^^:gswa-rock-code ;
    skos:prefLabel "limestone grainstone"@en ;
    schema:citation "https://glossary.americangeosciences.org/term/grainstone"^^xsd:anyURI ;
.

:limestone-mudstone
    a skos:Concept ;
    rdfs:isDefinedBy cs: ;
    skos:altLabel
        "micritic limestone"@en ,
        "mudstone"@en ;
    skos:broadMatch
        <http://inspire.ec.europa.eu/codelist/LithologyValue/carbonateMudstone> ,
        <http://resource.geosciml.org/classifier/cgi/lithology/carbonate_mudstone> ;
    skos:broader :limestone ;
    skos:definition "A fairly pure (93–99% calcium carbonate), mainly non-porous and impermeable, texturally uniform limestone whose main constituent (75–85%) is calcite mud (micrite) (Dunham, 1962). Adapted from Glossary of geology (5th edition revised; Neuendorf et al., 2011). The limestone prefix is commonly omitted since it is implied by Dunham's (1962) classification."@en ;
    skos:historyNote """Folk, RL 1959, Practical petrographic classification of limestones: American Association of Petroleum Geologists Bulletin No. 43(1), p. 1–38, doi:10.1306/0BDA5C36-16BD-11D7-8645000102C1865D.,
Dunham, RJ 1962, Classification of carbonate rocks according to depositional texture, in Classification of carbonate rocks edited by WE Hamm: American Association of Petroleum Geologists, Tulsa, Oklahoma, USA, p. 108–121.""" ;
    skos:inScheme cs: ;
    skos:notation "klu"^^:gswa-rock-code ;
    skos:prefLabel "limestone mudstone"@en ;
    schema:citation "https://glossary.americangeosciences.org/term/limemudstone"^^xsd:anyURI ;
.

:limestone-packstone
    a skos:Concept ;
    rdfs:isDefinedBy cs: ;
    skos:altLabel "packstone"@en ;
    skos:broadMatch
        <http://inspire.ec.europa.eu/codelist/LithologyValue/packstone> ,
        <http://resource.geosciml.org/classifier/cgi/lithology/packstone> ;
    skos:broader :limestone ;
    skos:definition "A term used for a sedimentary carbonate rock consisting predominantly of calcite and whose granular material is arranged in a self-supporting framework, yet which also contains some matrix of calcareous mud (Dunham, 1962). Adapted from Glossary of geology (5th edition revised; Neuendorf et al., 2011). The limestone prefix is commonly omitted since it is implied by Dunham's (1962) classification."@en ;
    skos:historyNote """Dunham, RJ 1962, Classification of carbonate rocks according to depositional texture, in Classification of carbonate rocks edited by WE Hamm: American Association of Petroleum Geologists, Tulsa, Oklahoma, USA, p. 108–121.,
Embry, AF, Klovan, JE 1971, A late Devonian reef tract on northeastern Banks Island, N.W.T: Bulletin of Canadian Petroleum Geology, v. 19(4), p. 730–781.""" ;
    skos:inScheme cs: ;
    skos:notation "klp"^^:gswa-rock-code ;
    skos:prefLabel "limestone packstone"@en ;
    schema:citation "https://glossary.americangeosciences.org/term/packstone"^^xsd:anyURI ;
.

:limestone-rudstone
    a skos:Concept ;
    rdfs:isDefinedBy cs: ;
    skos:altLabel "rudstone"@en ;
    skos:broader :limestone ;
    skos:definition "A carbonate rock consisting predominantly of calcite and composed of bioclasts or other fragments, over 2 mm in diameter, closely packed, in physical contact; the interstices may be open, or filled with fine carbonate sediment or crystalline cement. Adapted from Glossary of geology (5th edition revised; Neuendorf et al., 2011). The limestone prefix is commonly omitted since it is implied by Dunham's (1962) classification."@en ;
    skos:historyNote """Dunham, RJ 1962, Classification of carbonate rocks according to depositional texture, in Classification of carbonate rocks edited by WE Hamm: American Association of Petroleum Geologists, Tulsa, Oklahoma, USA, p. 108–121.,
Embry, AF, Klovan, JE 1971, A late Devonian reef tract on northeastern Banks Island, N.W.T: Bulletin of Canadian Petroleum Geology, v. 19(4), p. 730–781.""" ;
    skos:inScheme cs: ;
    skos:notation "kld"^^:gswa-rock-code ;
    skos:prefLabel "limestone rudstone"@en ;
    schema:citation "https://glossary.americangeosciences.org/term/rudstone"^^xsd:anyURI ;
.

:limestone-wackestone
    a skos:Concept ;
    rdfs:isDefinedBy cs: ;
    skos:altLabel "wackestone"@en ;
    skos:broadMatch
        <http://inspire.ec.europa.eu/codelist/LithologyValue/carbonateWackestone> ,
        <http://resource.geosciml.org/classifier/cgi/lithology/carbonate_wackestone> ;
    skos:broader :limestone ;
    skos:definition "A term for a mud-supported carbonate sedimentary rock consisting predominantly of calcite and containing more than 10% grains (particles with diameters greater than 20 μm). Adapted from Glossary of geology (5th edition revised; Neuendorf et al., 2011). The limestone prefix is commonly omitted since it is implied by Dunham's (1962) classification."@en ;
    skos:historyNote """Dunham, RJ 1962, Classification of carbonate rocks according to depositional texture, in Classification of carbonate rocks edited by WE Hamm: American Association of Petroleum Geologists, Tulsa, Oklahoma, USA, p. 108–121.,
Embry, AF, Klovan, JE 1971, A late Devonian reef tract on northeastern Banks Island, N.W.T: Bulletin of Canadian Petroleum Geology, v. 19(4), p. 730–781.""" ;
    skos:inScheme cs: ;
    skos:notation "klw"^^:gswa-rock-code ;
    skos:prefLabel "limestone wackestone"@en ;
    schema:citation "https://glossary.americangeosciences.org/term/wackestone"^^xsd:anyURI ;
.

:litharenite
    a skos:Concept ;
    rdfs:isDefinedBy cs: ;
    skos:altLabel "lithic arenite"@en ;
    skos:broader :arenite ;
    skos:definition "A type of arenite containing less than 75% quartz (excluding detrital chert grains), more than 25% rock/lithic fragments and a feldspar:lithic ratio less than 1:1. The term is a shortened form of lithic arenite. Adapted from Glossary of geology (5th edition revised; Neuendorf et al., 2011)"@en ;
    skos:historyNote "Pettijohn, FJ 1975, Sedimentary Rocks: New York, Harper and Row, 628p." ;
    skos:inScheme cs: ;
    skos:notation "sas"^^:gswa-rock-code ;
    skos:prefLabel "litharenite"@en ;
    schema:citation "https://glossary.americangeosciences.org/term/litharenite"^^xsd:anyURI ;
.

:lithic-arkose
    a skos:Concept ;
    rdfs:isDefinedBy cs: ;
    skos:altLabel
        "feldspathic litharenite"@en ,
        "impure arkose"@en ;
    skos:broader :arkose ;
    skos:definition "An arkose containing appreciable rock fragments; specifically containing less than 75% quartz and having a ratio of feldspar:lithic grains between 3:1 and 1:1. Adapted from Glossary of geology (5th edition revised; Neuendorf et al., 2011)."@en ;
    skos:historyNote "Folk, RL 1968, Petrology of Sedimentary Rocks: Austin, Hemphill Publishing Company, 170p." ;
    skos:inScheme cs: ;
    skos:notation "sjs"^^:gswa-rock-code ;
    skos:prefLabel "lithic arkose"@en ;
    schema:citation "https://glossary.americangeosciences.org/term/lithicarkose"^^xsd:anyURI ;
.

:lithic-impact-breccia
    a skos:Concept ;
    rdfs:isDefinedBy cs: ;
    skos:broader :impact-breccia ;
    skos:definition "Polymictic impact breccia with clastic matrix containing shocked and unshocked mineral and lithic clasts, but lacking cogenetic impact melt particles. Synonymous with, and supersedes, fragmental breccia. (Fettes and Desmons, 2007, p. 169)."@en ;
    skos:historyNote "Based on the IUGS classification of metamorphic rocks (Fettes and Desmons, 2007)." ;
    skos:inScheme cs: ;
    skos:notation "mpl"^^:gswa-rock-code ;
    skos:prefLabel "lithic impact breccia"@en ;
.

:lithic-wacke
    a skos:Concept ;
    rdfs:isDefinedBy cs: ;
    skos:altLabel
        "lithic graywacke"@en ,
        "lithic greywacke"@en ;
    skos:broader :wacke ;
    skos:definition "A wacke containing greater then 5% rock/lithic grains and a ratio of feldspar: rock/lithic grains less than 1:1. Adapted from Glossary of geology (5th edition revised; Neuendorf et al., 2011)."@en ;
    skos:historyNote "Pettijohn, FJ 1975, Sedimentary Rocks: New York, Harper and Row, 628p." ;
    skos:inScheme cs: ;
    skos:notation "sws"^^:gswa-rock-code ;
    skos:prefLabel "lithic wacke"@en ;
    schema:citation "https://glossary.americangeosciences.org/term/lithicwacke"^^xsd:anyURI ;
.

:mafic-gneiss
    a skos:Concept ;
    rdfs:isDefinedBy cs: ;
    skos:broader :meta-igneous-mafic ;
    skos:definition "A metamorphosed mafic igneous rock displaying a gneissose structure, i.e. a gneiss derived from an igneous mafic but otherwise unspecified rock (i.e. the intrusive, extrusive or volcaniclastic nature of the protolith cannot be conclusively established). See also definition of gneiss/gneissose structure in Fettes and Desmons (2007, p. 154–155)."@en ;
    skos:historyNote "Based on the IUGS classification of metamorphic rocks (Fettes and Desmons, 2007)." ;
    skos:inScheme cs: ;
    skos:notation "mwn"^^:gswa-rock-code ;
    skos:prefLabel "mafic gneiss"@en ;
    schema:citation
        "https://glossary.americangeosciences.org/term/gneiss"^^xsd:anyURI ,
        "https://glossary.americangeosciences.org/term/mafic"^^xsd:anyURI ;
.

:mafic-gneiss-derived-from-intrusive-rock
    a skos:Concept ;
    rdfs:isDefinedBy cs: ;
    skos:broader :meta-igneous-mafic-intrusive ;
    skos:definition "A metamorphosed mafic intrusive (or coarse-grained parts of extrusive successions) displaying a gneissose structure, i.e. a gneiss derived from an intrusive rock with one or more mafic minerals as the main component(s). See also definition of gneiss/gneissose structure in Fettes and Desmons (2007, p. 154–155)."@en ;
    skos:historyNote "Based on the IUGS classification of metamorphic rocks (Fettes and Desmons, 2007)." ;
    skos:inScheme cs: ;
    skos:notation "mon"^^:gswa-rock-code ;
    skos:prefLabel "mafic gneiss derived from intrusive rock"@en ;
.

:mafic-gneiss-derived-from-volcanic-rock
    a skos:Concept ;
    rdfs:isDefinedBy cs: ;
    skos:broader :meta-igneous-mafic-volcanic ;
    skos:definition "A metamorphosed mafic volcanic rock displaying a gneissose structure, i.e. a gneiss derived from a volcanic rock with one or more mafic minerals as the main component(s). See also definition of gneiss/gneissose structure in Fettes and Desmons (2007, p. 154–155). GSWA's rock classification scheme prefers the use of volcanic terminology for any igneous rock formed on or near the Earth's surface, i.e. for those hypabyssal or subvolcanic rocks such as dykes, sills, and cryptodomes that are demonstrably both spatially and temporally associated with extrusive volcanic rocks."@en ;
    skos:historyNote "Based on the IUGS classification of metamorphic rocks (Fettes and Desmons, 2007)." ;
    skos:inScheme cs: ;
    skos:notation "mbn"^^:gswa-rock-code ;
    skos:prefLabel "mafic gneiss derived from volcanic rock"@en ;
.

:mafic-granofels-hornfels
    a skos:Concept ;
    rdfs:isDefinedBy cs: ;
    skos:broader :meta-igneous-mafic ;
    skos:definition "General term for granofelsic or hornfelsed mafic igneous rocks for which an intrusive, extrusive or volcaniclastic protolith cannot be conclusively identified. Commonly the main components are plagioclase and one or more mafic minerals; pyroxene(s) and minor olivine are common under the relatively dry conditions existing in the aureoles of many basic intrusions, whereas hornblende ± biotite form preferentially in more hydrated conditions, as in most aureoles of intermediate to acid intrusions. Mafic hornfelses include, among others, rocks known in the literature as beerbachite, granoblast, muscovadite and sudburite, as well as contact rocks called pyroxene-granulites by some British petrologists. Adapted from Fettes and Desmons (2007, p. 170)."@en ;
    skos:historyNote "Based on the IUGS classification of metamorphic rocks (Fettes and Desmons, 2007)." ;
    skos:inScheme cs: ;
    skos:notation "mwe"^^:gswa-rock-code ;
    skos:prefLabel "mafic granofels/hornfels"@en ;
    schema:citation "https://glossary.americangeosciences.org/term/mafic"^^xsd:anyURI ;
.

:mafic-granofels-hornfels-derived-from-intrusive-rock
    a skos:Concept ;
    rdfs:isDefinedBy cs: ;
    skos:broader :meta-igneous-mafic-intrusive ;
    skos:definition "A metamorphosed mafic intrusive rock displaying a granofelsic structure, i.e. a granofels/hornfels derived from an intrusive (or coarse-grained part of an extrusive succession) rock with one or more mafic minerals as the main components (adapted from Fettes and Desmons, 2007, p. 202). See also definition of granofels/granofelsic structure in Fettes and Desmons (2007, p. 156); hornfels are granofels formed by contact metamorphism (Fettes and Desmons, 2007, p. 159)."@en ;
    skos:historyNote "Based on the IUGS classification of metamorphic rocks (Fettes and Desmons, 2007)." ;
    skos:inScheme cs: ;
    skos:notation "moe"^^:gswa-rock-code ;
    skos:prefLabel "mafic granofels/hornfels derived from intrusive rock"@en ;
.

:mafic-granofels-hornfels-derived-from-volcanic-rock
    a skos:Concept ;
    rdfs:isDefinedBy cs: ;
    skos:broader :meta-igneous-mafic-volcanic ;
    skos:definition "A metamorphosed mafic volcanic rock displaying a granofelsic structure, i.e. a granofels/hornfels derived from a volcanic rock with one or more mafic minerals as the main components (adapted from Fettes and Desmons, 2007, p. 202). See also definition of granofels/granofelsic structure in Fettes and Desmons (2007, p. 156); hornfels are granofels formed by contact metamorphism (Fettes and Desmons, 2007, p. 159). GSWA's rock classification scheme prefers the use of volcanic terminology for any igneous rock formed on or near the Earth's surface, i.e. for those hypabyssal or subvolcanic rocks such as dykes, sills, and cryptodomes that are demonstrably both spatially and temporally associated with extrusive volcanic rocks."@en ;
    skos:historyNote "Based on the IUGS classification of metamorphic rocks (Fettes and Desmons, 2007)." ;
    skos:inScheme cs: ;
    skos:notation "mbe"^^:gswa-rock-code ;
    skos:prefLabel "mafic granofels/hornfels derived from volcanic rock"@en ;
.

:mafic-granulite
    a skos:Concept ;
    rdfs:isDefinedBy cs: ;
    skos:broadMatch
        <http://inspire.ec.europa.eu/codelist/LithologyValue/granulite> ,
        <http://resource.geosciml.org/classifier/cgi/lithology/granulite> ;
    skos:broader :meta-igneous-mafic ;
    skos:definition "Type of granulite with more than 30% mafic minerals (dominantly pyroxene), i.e. greater than 30% modal ferromagnesian and other non-felsic minerals (Fettes and Desmons, 2007, p. 170)."@en ;
    skos:historyNote "Based on the IUGS classification of metamorphic rocks (Fettes and Desmons, 2007)." ;
    skos:inScheme cs: ;
    skos:notation "mwo"^^:gswa-rock-code ;
    skos:prefLabel "mafic granulite"@en ;
    schema:citation
        "https://glossary.americangeosciences.org/term/granulitemeta"^^xsd:anyURI ,
        "https://glossary.americangeosciences.org/term/mafic"^^xsd:anyURI ;
.

:mafic-intrusive-rock
    a skos:Concept ;
    rdfs:isDefinedBy cs: ;
    skos:broader :igneous-mafic-intrusive ;
    skos:definition "An igneous intrusive rock (and including coarse-grained parts of extrusive successions) composed chiefly of one or more ferromagnesian, dark-coloured minerals in its mode, otherwise uncategorized (adapted from Glossary of geology, 5th edition revised; Neuendorf et al., 2011)."@en ;
    skos:historyNote "Based on the IUGS classification of igneous rocks (Le Maitre et al., 2005) and Glossary of geology (5th edition, revised; Neuendorf et al. 2011)." ;
    skos:inScheme cs: ;
    skos:notation "o"^^:gswa-rock-code ;
    skos:prefLabel "mafic intrusive rock"@en ;
    schema:citation "https://glossary.americangeosciences.org/term/mafic"^^xsd:anyURI ;
.

:mafic-intrusive-rock-undivided
    a skos:Concept ;
    rdfs:isDefinedBy cs: ;
    skos:broader :igneous-mafic-intrusive ;
    skos:definition "A demonstrably mafic intrusive or a coarse-grained constituent of an extrusive succession, otherwise uncategorized. GSWA usage of this term is restricted to rocks that are partially weathered or are identified using remote sensing imagery, and the use of the related code/notation is limited to GSWA's Explanatory Notes System."@en ;
    skos:historyNote "Based on the IUGS classification of igneous rocks (Le Maitre et al., 2005) and GSWA usage." ;
    skos:inScheme cs: ;
    skos:notation "on"^^:gswa-rock-code ;
    skos:prefLabel "mafic intrusive rock; undivided"@en ;
.

:mafic-schist
    a skos:Concept ;
    rdfs:isDefinedBy cs: ;
    skos:broader :meta-igneous-mafic ;
    skos:definition "A metamorphosed mafic rock displaying a schistose structure, i.e. a schist derived from an intrusive, extrusive or volcaniclastic rock with one or more mafic minerals as the main component(s). See also definition of schist/schistose structure in Fettes and Desmons (2007, p. 193)."@en ;
    skos:historyNote "Based on the IUGS classification of metamorphic rocks (Fettes and Desmons, 2007)." ;
    skos:inScheme cs: ;
    skos:notation "mws"^^:gswa-rock-code ;
    skos:prefLabel "mafic schist"@en ;
    schema:citation
        "https://glossary.americangeosciences.org/term/mafic"^^xsd:anyURI ,
        "https://glossary.americangeosciences.org/term/schist"^^xsd:anyURI ;
.

:mafic-schist-derived-from-intrusive-rock
    a skos:Concept ;
    rdfs:isDefinedBy cs: ;
    skos:broader :meta-igneous-mafic-intrusive ;
    skos:definition "A metamorphosed mafic intrusive rock (or coarse-grained parts of extrusive successions) displaying a schistose structure, i.e. a schist derived from an intrusive rock with one or more mafic minerals as the main component(s). See also definition of schist/schistose structure in Fettes and Desmons, 2007, p. 193)."@en ;
    skos:historyNote "Based on the IUGS classification of metamorphic rocks (Fettes and Desmons, 2007)." ;
    skos:inScheme cs: ;
    skos:notation "mos"^^:gswa-rock-code ;
    skos:prefLabel "mafic schist derived from intrusive rock"@en ;
.

:mafic-schist-derived-from-volcanic-rock
    a skos:Concept ;
    rdfs:isDefinedBy cs: ;
    skos:broader :meta-igneous-mafic-volcanic ;
    skos:definition "A metamorphosed mafic volcanic rock displaying a schistose structure, i.e. a schist derived from a volcanic rock with one or more mafic minerals as the main component(s). See also definition of schist/schistose structure in Fettes and Desmons, 2007, p. 193). GSWA's rock classification scheme prefers the use of volcanic terminology for any igneous rock formed on or near the Earth's surface, i.e. for those hypabyssal or subvolcanic rocks such as dykes, sills, and cryptodomes that are demonstrably both spatially and temporally associated with extrusive volcanic rocks."@en ;
    skos:historyNote "Based on the IUGS classification of metamorphic rocks (Fettes and Desmons, 2007)." ;
    skos:inScheme cs: ;
    skos:notation "mbs"^^:gswa-rock-code ;
    skos:prefLabel "mafic schist derived from volcanic rock"@en ;
.

:mafic-volcanic-rock
    a skos:Concept ;
    rdfs:isDefinedBy cs: ;
    skos:broader :igneous-mafic-volcanic ;
    skos:definition "An igneous volcanic rock composed chiefly of one or more ferromagnesian, dark-coloured minerals in its mode (adapted from Glossary of geology, 5th edition revised; Neuendorf et al., 2011). The GSWA's rock classification scheme prefers the use of volcanic terminology for any igneous rock formed on or near the Earth's surface, i.e. for those hypabyssal or subvolcanic rocks such as dykes, sills, and cryptodomes that are demonstrably both spatially and temporally associated with extrusive volcanic rocks."@en ;
    skos:historyNote "Based on the IUGS classification of igneous rocks (Le Maitre et al., 2005)." ;
    skos:inScheme cs: ;
    skos:notation "b"^^:gswa-rock-code ;
    skos:prefLabel "mafic volcanic rock"@en ;
    schema:citation "https://glossary.americangeosciences.org/term/mafic"^^xsd:anyURI ;
.

:mafic-volcanic-rock-undivided
    a skos:Concept ;
    rdfs:isDefinedBy cs: ;
    skos:broader :igneous-mafic-volcanic ;
    skos:definition "A demonstrably mafic igneous volcanic rocks, otherwise uncategorized. GSWA usage of this term is restricted to rocks that are partially weathered or are identified using remote sensing imagery, and the use of the related code/notation is limited to GSWA's Explanatory Notes System."@en ;
    skos:historyNote "Based on the IUGS classification of igneous rocks (Le Maitre et al., 2005) and GSWA usage." ;
    skos:inScheme cs: ;
    skos:notation "bn"^^:gswa-rock-code ;
    skos:prefLabel "mafic volcanic rock; undivided"@en ;
.

:mafic-volcaniclastic-breccia
    a skos:Concept ;
    rdfs:isDefinedBy cs: ;
    skos:broader :igneous-mafic-volcanic ;
    skos:definition "A volcaniclastic rock composed mostly of angular fragments greater than 2 mm in size consisting of either (a) pyroclastic detritus or (b) terrigenous volcanic detritus of epiclastic origin, and with an overall mafic composition. 'Volcaniclastic' includes all clastic volcanic materials formed by any process of fragmentation, dispersed by any kind of transporting agent, deposited in any environment, or mixed in any significant portion with non-volcanic fragments."@en ;
    skos:historyNote "Compiled by the Geological Survey of Western Australia" ;
    skos:inScheme cs: ;
    skos:notation "bvb"^^:gswa-rock-code ;
    skos:prefLabel "mafic volcaniclastic breccia"@en ;
    schema:citation
        "https://glossary.americangeosciences.org/term/volcanicbreccia"^^xsd:anyURI ,
        "https://glossary.americangeosciences.org/term/volcaniclastic"^^xsd:anyURI ;
.

:mafic-volcaniclastic-breccia-sandstone
    a skos:Concept ;
    rdfs:isDefinedBy cs: ;
    skos:broader :igneous-mafic-volcanic ;
    skos:definition "A volcaniclastic rock composed mostly of angular fragments ranging in size from sand (0.0625 – 2 mm) and above, consisting of either (a) pyroclastic detritus or (b) terrigenous volcanic detritus of epiclastic origin, and with an overall mafic composition. 'Volcaniclastic' includes all clastic volcanic materials formed by any process of fragmentation, dispersed by any kind of transporting agent, deposited in any environment, or mixed in any significant portion with non-volcanic fragments."@en ;
    skos:historyNote "Compiled by the Geological Survey of Western Australia" ;
    skos:inScheme cs: ;
    skos:notation "bvbs"^^:gswa-rock-code ;
    skos:prefLabel "mafic volcaniclastic breccia-sandstone"@en ;
    schema:citation "https://glossary.americangeosciences.org/term/volcaniclastic"^^xsd:anyURI ;
.

:mafic-volcaniclastic-conglomerate
    a skos:Concept ;
    rdfs:isDefinedBy cs: ;
    skos:broader :igneous-mafic-volcanic ;
    skos:definition "A conglomerate consisting of either (a) pyroclastic detritus or (b) terrigenous volcanic detritus of epiclastic origin, and with an overall mafic composition. 'Volcaniclastic' includes all clastic volcanic materials formed by any process of fragmentation, dispersed by any kind of transporting agent, deposited in any environment, or mixed in any significant portion with non-volcanic fragments."@en ;
    skos:historyNote "Compiled by the Geological Survey of Western Australia" ;
    skos:inScheme cs: ;
    skos:notation "bvc"^^:gswa-rock-code ;
    skos:prefLabel "mafic volcaniclastic conglomerate"@en ;
    schema:citation
        "https://glossary.americangeosciences.org/term/volcanicconglomerate"^^xsd:anyURI ,
        "https://glossary.americangeosciences.org/term/volcaniclastic"^^xsd:anyURI ;
.

:mafic-volcaniclastic-granule-pebble-breccia
    a skos:Concept ;
    rdfs:isDefinedBy cs: ;
    skos:broader :igneous-mafic-volcanic ;
    skos:definition "A breccia composed mostly of angular fragments ranging in size from granule (2–4 mm) to pebble (4–32 mm) consisting of either (a) pyroclastic detritus or (b) terrigenous volcanic detritus of epiclastic origin, and with an overall mafic composition. 'Volcaniclastic' includes all clastic volcanic materials formed by any process of fragmentation, dispersed by any kind of transporting agent, deposited in any environment, or mixed in any significant portion with non-volcanic fragments."@en ;
    skos:historyNote "Compiled by the Geological Survey of Western Australia" ;
    skos:inScheme cs: ;
    skos:notation "bvg"^^:gswa-rock-code ;
    skos:prefLabel "mafic volcaniclastic granule/pebble breccia"@en ;
    schema:citation "https://glossary.americangeosciences.org/term/volcaniclastic"^^xsd:anyURI ;
.

:mafic-volcaniclastic-mudstone
    a skos:Concept ;
    rdfs:isDefinedBy cs: ;
    skos:broader :igneous-mafic-volcanic ;
    skos:definition "A mudstone (grain size ranging from silt to clay, i.e. less than 0.0625 mm) consisting of either (a) pyroclastic detritus or (b) terrigenous volcanic detritus of epiclastic origin, and with an overall mafic composition. 'Volcaniclastic' includes all clastic volcanic materials formed by any process of fragmentation, dispersed by any kind of transporting agent, deposited in any environment, or mixed in any significant portion with non-volcanic fragments."@en ;
    skos:historyNote "Compiled by the Geological Survey of Western Australia" ;
    skos:inScheme cs: ;
    skos:notation "bvsm"^^:gswa-rock-code ;
    skos:prefLabel "mafic volcaniclastic mudstone"@en ;
    schema:citation "https://glossary.americangeosciences.org/term/volcaniclastic"^^xsd:anyURI ;
.

:mafic-volcaniclastic-rock
    a skos:Concept ;
    rdfs:isDefinedBy cs: ;
    skos:broader :igneous-mafic-volcanic ;
    skos:definition "A volcaniclastic rock consisting of either (a) pyroclastic detritus or (b) terrigenous volcanic detritus of epiclastic origin and with an overall mafic composition, but otherwise uncategorized. 'Volcaniclastic' includes all clastic volcanic materials formed by any process of fragmentation, dispersed by any kind of transporting agent, deposited in any environment, or mixed in any significant portion with non-volcanic fragments."@en ;
    skos:historyNote "Compiled by the Geological Survey of Western Australia" ;
    skos:inScheme cs: ;
    skos:notation "bvr"^^:gswa-rock-code ;
    skos:prefLabel "mafic volcaniclastic rock"@en ;
    schema:citation "https://glossary.americangeosciences.org/term/volcaniclastic"^^xsd:anyURI ;
.

:mafic-volcaniclastic-sandstone
    a skos:Concept ;
    rdfs:isDefinedBy cs: ;
    skos:broader :igneous-mafic-volcanic ;
    skos:definition "A sandstone (grain size 0.0625 – 2 mm) consisting of either (a) pyroclastic detritus or (b) terrigenous volcanic detritus of epiclastic origin, and with an overall mafic composition. 'Volcaniclastic' includes all clastic volcanic materials formed by any process of fragmentation, dispersed by any kind of transporting agent, deposited in any environment, or mixed in any significant portion with non-volcanic fragments."@en ;
    skos:historyNote "Pettijohn, FJ, Potter, PE, Siever, R 1987, Sand and sandstone: Springer-Verlag New York, Inc, 553p. (p. 205)" ;
    skos:inScheme cs: ;
    skos:notation "bvs"^^:gswa-rock-code ;
    skos:prefLabel "mafic volcaniclastic sandstone"@en ;
    schema:citation
        "https://glossary.americangeosciences.org/term/volcaniclastic"^^xsd:anyURI ,
        "https://glossary.americangeosciences.org/term/volcanicsandstone"^^xsd:anyURI ;
.

:mafic-volcaniclastic-sandstone-siltstone
    a skos:Concept ;
    rdfs:isDefinedBy cs: ;
    skos:broader :igneous-mafic-volcanic ;
    skos:definition "A volcaniclastic rock composed mostly of fragments ranging in size from sand (0.0625 – 2 mm) to silt (0.0039 – 0.0625 mm) of either (a) pyroclastic detritus or (b) terrigenous volcanic detritus of epiclastic origin, and with an overall mafic composition. 'Volcaniclastic' includes all clastic volcanic materials formed by any process of fragmentation, dispersed by any kind of transporting agent, deposited in any environment, or mixed in any significant portion w, and with an overall mafic composition."@en ;
    skos:historyNote "Compiled by the Geological Survey of Western Australia" ;
    skos:inScheme cs: ;
    skos:notation "bvss"^^:gswa-rock-code ;
    skos:prefLabel "mafic volcaniclastic sandstone-siltstone"@en ;
    schema:citation "https://glossary.americangeosciences.org/term/volcaniclastic"^^xsd:anyURI ;
.

:mafic-volcaniclastic-sediment-matrix-breccia
    a skos:Concept ;
    rdfs:isDefinedBy cs: ;
    skos:broader :igneous-mafic-volcanic ;
    skos:definition "A commonly monomictic breccia of overall mafic composition composed of angular, coarse igneous fragments cemented by a fine-grained matrix that is clastic though not necessarily strictly sedimentary in origin. 'Volcaniclastic' includes all clastic volcanic materials formed by any process of fragmentation, dispersed by any kind of transporting agent, deposited in any environment, or mixed in any significant portion with non-volcanic fragments."@en ;
    skos:historyNote "Compiled by the Geological Survey of Western Australia" ;
    skos:inScheme cs: ;
    skos:notation "bvsb"^^:gswa-rock-code ;
    skos:prefLabel "mafic volcaniclastic sediment-matrix breccia"@en ;
    schema:citation "https://doi.org/10.1016/j.jvolgeores.2016.02.007"^^xsd:anyURI ;
.

:magnesite
    a skos:Concept ;
    rdfs:isDefinedBy cs: ;
    skos:broader :sedimentary-carbonate ;
    skos:definition "A concentration of magnesium carbonate (MgCO3), derived from the alteration of dolomite rocks or magnesium-silicate rich rocks. Commonly found as white to greyish, yellow, or brown earthy masses or irregular veins. Adapted from Glossary of geology (5th edition revised; Neuendorf et al., 2011)."@en ;
    skos:historyNote "Compiled by the Geological Survey of Western Australia" ;
    skos:inScheme cs: ;
    skos:notation "km"^^:gswa-rock-code ;
    skos:prefLabel "magnesite"@en ;
    schema:citation "https://glossary.americangeosciences.org/term/magnesite"^^xsd:anyURI ;
.

:magnetite-gabbro
    a skos:Concept ;
    rdfs:isDefinedBy cs: ;
    skos:broader :igneous-mafic-intrusive ;
    skos:definition "A gabbro with a high proportion (greater than 20%) of magnetite or Fe–Ti oxides."@en ;
    skos:historyNote "Compiled by the Geological Survey of Western Australia" ;
    skos:inScheme cs: ;
    skos:notation "ogj"^^:gswa-rock-code ;
    skos:prefLabel "magnetite gabbro"@en ;
.

:magnetitite
    a skos:Concept ;
    rdfs:isDefinedBy cs: ;
    skos:broader :igneous-ultramafic-intrusive ;
    skos:definition "An ultramafic rock consisting essentially of magnetite (Le Maitre et al., 2005, p. 107)."@en ;
    skos:historyNote "Based on the IUGS classification of igneous rocks (Le Maitre et al., 2005)." ;
    skos:inScheme cs: ;
    skos:notation "am"^^:gswa-rock-code ;
    skos:prefLabel "magnetitite"@en ;
.

:marlstone
    a skos:Concept ;
    rdfs:isDefinedBy cs: ;
    skos:altLabel
        "calcareous mudstone"@en ,
        "dolomitic mudstone"@en ;
    skos:broader :sedimentary-carbonate ;
    skos:closeMatch
        <http://inspire.ec.europa.eu/codelist/LithologyValue/carbonateRichMudstone> ,
        <http://resource.geosciml.org/classifier/cgi/lithology/carbonate_rich_mudstone> ;
    skos:definition "An indurated rock of about the same composition as marl, called an earthy or impure argillaceous limestone. It has a blocky subconchoidal fracture, and is less fissile than shale. Adapted from Glossary of geology (5th edition revised; Neuendorf et al., 2011). Use of marl as a lithology should be avoided as it refers to unlithified marlstone."@en ;
    skos:historyNote "Compiled by the Geological Survey of Western Australia" ;
    skos:inScheme cs: ;
    skos:notation "kr"^^:gswa-rock-code ;
    skos:prefLabel "marlstone"@en ;
    schema:citation "https://glossary.americangeosciences.org/term/marlstone"^^xsd:anyURI ;
.

:massive-sulfide
    a skos:Concept ;
    rdfs:isDefinedBy cs: ;
    skos:broader :hydrothermal ;
    skos:definition "A rock comprising abundant sulfide minerals, commonly making up at least 60 % of the mineral assemblage."@en ;
    skos:historyNote "Compiled by the Geological Survey of Western Australia" ;
    skos:inScheme cs: ;
    skos:notation "zs"^^:gswa-rock-code ;
    skos:prefLabel "massive sulfide"@en ;
    schema:citation "https://en.wikipedia.org/wiki/Massive_sulfide_deposits"^^xsd:anyURI ;
.

:melilitolite
    a skos:Concept ;
    rdfs:isDefinedBy cs: ;
    skos:broader :igneous-melilitic ;
    skos:definition "An ultramafic intrusive rock consisting essentially of melilite, pyroxene and olivine, otherwise uncategorized. Now defined as a general term for intrusive rocks in the melilite-bearing rocks classification. Definition from Le Maitre et al. (2005, p. 110). Specific names apply based on the percentages of different mineral phases (Le Maitre et al., 2005, p. 11)."@en ;
    skos:historyNote "Based on the IUGS classification of igneous rocks (Le Maitre et al., 2005)." ;
    skos:inScheme cs: ;
    skos:notation "e"^^:gswa-rock-code ;
    skos:prefLabel "melilitolite"@en ;
.

:melilitolite-undivided
    a skos:Concept ;
    rdfs:isDefinedBy cs: ;
    skos:broader :igneous-melilitic ;
    skos:definition "A demonstrably ultramafic intrusive rock consisting essentially of melilite, pyroxene and olivine, otherwise uncategorized. GSWA usage of this term is restricted to rocks that are partially weathered or are identified using remote sensing imagery, and the use of the related code/notation is limited to GSWA's Explanatory Notes System."@en ;
    skos:historyNote "Based on the IUGS classification of igneous rocks (Le Maitre et al., 2005) and GSWA usage." ;
    skos:inScheme cs: ;
    skos:notation "en"^^:gswa-rock-code ;
    skos:prefLabel "melilitolite; undivided"@en ;
.

:meta-andesite
    a skos:Concept ;
    rdfs:isDefinedBy cs: ;
    skos:broader :meta-igneous-felsic-volcanic ;
    skos:definition "A metamorphosed intermediate volcanic rock, usually porphyritic, derived from a protolith consisting of plagioclase (frequently zoned from labradorite to oligoclase), pyroxene, hornblende and/or biotite. Igneous protolith defined modally in QAPF fields 9 and 10, and, if modes are not available, chemically in TAS field O2 (Le Maitre et al., 2005, p. 56). GSWA's rock classification scheme prefers the use of volcanic terminology for any igneous rock formed on or near the Earth's surface, i.e. for those hypabyssal or subvolcanic rocks such as dykes, sills, and cryptodomes that are demonstrably both spatially and temporally associated with extrusive volcanic rocks."@en ;
    skos:historyNote "Based on the IUGS classification of metamorphic (Fettes and Desmons, 2007) and igneous rocks (Le Maitre et al., 2005)." ;
    skos:inScheme cs: ;
    skos:notation "mfa"^^:gswa-rock-code ;
    skos:prefLabel "meta-andesite"@en ;
.

:meta-anorthosite
    a skos:Concept ;
    rdfs:isDefinedBy cs: ;
    skos:broader :meta-igneous-mafic-intrusive ;
    skos:definition "A metamorphosed leucocratic intrusive rock derived from a protolith consisting essentially of plagioclase commonly with small amounts of pyroxene. Igneous protolith defined modally in QAPF field 10 and in the gabbroic rock classification of Le Maitre et al. (2005, p. 22 and 24)."@en ;
    skos:historyNote "Based on the IUGS classification of metamorphic (Fettes and Desmons, 2007) and igneous rocks (Le Maitre et al., 2005)." ;
    skos:inScheme cs: ;
    skos:notation "mof"^^:gswa-rock-code ;
    skos:prefLabel "meta-anorthosite"@en ;
.

:meta-arkose
    a skos:Concept ;
    rdfs:isDefinedBy cs: ;
    skos:broader :metasedimentary-siliciclastic-psammite ;
    skos:definition "A metamorphosed rock derived from a siliciclastic sedimentary protolith rich in feldspar and with grain size between 0.0625 and 2 mm."@en ;
    skos:historyNote "Compiled by the Geological Survey of Western Australia" ;
    skos:inScheme cs: ;
    skos:notation "mtf"^^:gswa-rock-code ;
    skos:prefLabel "meta-arkose"@en ;
.

:meta-banded-chert
    a skos:Concept ;
    rdfs:isDefinedBy cs: ;
    skos:broader :metasedimentary-other-chemical ;
    skos:definition "A metamorphosed banded chert."@en ;
    skos:historyNote "Compiled by the Geological Survey of Western Australia" ;
    skos:inScheme cs: ;
    skos:notation "mcb"^^:gswa-rock-code ;
    skos:prefLabel "meta-banded chert"@en ;
.

:meta-banded-iron-formation
    a skos:Concept ;
    rdfs:isDefinedBy cs: ;
    skos:altLabel
        "itabirite"@en ,
        "taconite"@en ;
    skos:broader :metasedimentary-other-chemical-meta-iron-formation ;
    skos:definition "A metamorphosed banded iron-formation, i.e. a metamorphosed iron formation that shows marked banding (generally of iron-rich minerals and chert or fine-grained quartz)."@en ;
    skos:historyNote "Compiled by the Geological Survey of Western Australia" ;
    skos:inScheme cs: ;
    skos:notation "mib"^^:gswa-rock-code ;
    skos:prefLabel "meta-banded iron formation"@en ;
.

:meta-igneous-rock
    a skos:Concept ;
    rdfs:isDefinedBy cs: ;
    skos:broader :meta-igneous ;
    skos:definition "A metamorphosed rock of igneous but otherwise unspecified origin, i.e. a rock for which an igneous protolith is interpreted but commonly too weathered or altered to make further distinctions."@en ;
    skos:historyNote "Compiled by the Geological Survey of Western Australia" ;
    skos:inScheme cs: ;
    skos:notation "mign"^^:gswa-rock-code ;
    skos:prefLabel "meta-igneous rock"@en ;
.

:meta-iron-formation
    a skos:Concept ;
    rdfs:isDefinedBy cs: ;
    skos:altLabel
        "itabirite"@en ,
        "taconite"@en ;
    skos:broader :metasedimentary-other-chemical-meta-iron-formation ;
    skos:definition "A metamorphosed rocks derived from a chemical sedimentary protolith containing at least 15% iron of sedimentary origin."@en ;
    skos:historyNote "Compiled by the Geological Survey of Western Australia" ;
    skos:inScheme cs: ;
    skos:notation "mi"^^:gswa-rock-code ;
    skos:prefLabel "meta-iron formation"@en ;
.

:meta-olivine-gabbro
    a skos:Concept ;
    rdfs:isDefinedBy cs: ;
    skos:broader :meta-igneous-mafic-intrusive ;
    skos:definition "A metamorphosed intrusive rock (or coarse-grained parts of extrusive successions), derived from a gabbro containing essential olivine. Igneous protolith defined modally in the gabbroic rock classification (Le Maitre et al., 2005, p. 119)."@en ;
    skos:historyNote "Based on the IUGS classification of metamorphic (Fettes and Desmons, 2007) and igneous rocks (Le Maitre et al., 2005)." ;
    skos:inScheme cs: ;
    skos:notation "moo"^^:gswa-rock-code ;
    skos:prefLabel "meta-olivine gabbro"@en ;
.

:meta-pyroxene-spinifex-textured-basalt
    a skos:Concept ;
    rdfs:isDefinedBy cs: ;
    skos:broader :meta-igneous-mafic-volcanic ;
    skos:definition "A metamorphosed volcanic basaltic rock with recognisable pyroxene spinifex texture, i.e. an igneous texture consisting of needle-like pyroxene crystals usually forming a criss-crossing pattern, the result of rapid quenching from unusually high temperatures (cf. https://glossary.americangeosciences.org/term/spinifextexture). GSWA's rock classification scheme prefers the use of volcanic terminology for any igneous rock formed on or near the Earth's surface, i.e. for those hypabyssal or subvolcanic rocks such as dykes, sills, and cryptodomes that are demonstrably both spatially and temporally associated with extrusive volcanic rocks."@en ;
    skos:historyNote "Based on the IUGS classification of metamorphic (Fettes and Desmons, 2007) and igneous rocks (Le Maitre et al., 2005)." ;
    skos:inScheme cs: ;
    skos:notation "mbp"^^:gswa-rock-code ;
    skos:prefLabel "meta-pyroxene spinifex textured basalt"@en ;
.

:meta-quartz-diorite
    a skos:Concept ;
    rdfs:isDefinedBy cs: ;
    skos:broader :meta-igneous-felsic-intrusive ;
    skos:definition "A metamorphosed felsic intrusive rock derived from a protolith having the composition of diorite but with an appreciable amount of quartz, i.e. between 5 and 20% of the felsic minerals (defined modally in QAPF field 10*; Le Maitre et al., 2005, p. 134)."@en ;
    skos:historyNote "Based on the IUGS classification of metamorphic (Fettes and Desmons, 2007) and igneous rocks (Le Maitre et al., 2005)." ;
    skos:inScheme cs: ;
    skos:notation "mgiq"^^:gswa-rock-code ;
    skos:prefLabel "meta-quartz diorite"@en ;
.

:meta-quartz-latite
    a skos:Concept ;
    rdfs:isDefinedBy cs: ;
    skos:broader :meta-igneous-felsic-volcanic ;
    skos:definition "A term originally used for a volcanic rock composed of phenocrysts of quartz, plagioclase, biotite and hornblende in a glassy matrix potentially of quartz and alkali feldspar. Now commonly used for volcanic rocks composed of alkali feldspar and plagioclase in roughly equal amounts, quartz and mafic minerals. Now defined modally in QAPF field 8* (Fig. 2.4, p. 22). Definition from Le Maitre et al. (2005, p. 135) GSWA's rock classification scheme prefers the use of volcanic terminology for any igneous rock formed on or near the Earth's surface, i.e. for those hypabyssal or subvolcanic rocks such as dykes, sills, and cryptodomes that are demonstrably both spatially and temporally associated with extrusive volcanic rocks."@en ;
    skos:historyNote "Based on the IUGS classification of metamorphic (Fettes and Desmons, 2007) and igneous rocks (Le Maitre et al., 2005)." ;
    skos:inScheme cs: ;
    skos:notation "mflq"^^:gswa-rock-code ;
    skos:prefLabel "meta-quartz latite"@en ;
.

:meta-quartz-trachyte
    a skos:Concept ;
    rdfs:isDefinedBy cs: ;
    skos:broader :meta-igneous-felsic-volcanic ;
    skos:definition "A metamorphosed volcanic rock derived from a protolith consisting of phenocrysts of alkali feldspar and quartz in a cryptocrystalline or glassy matrix. Igneous protolith defined modally in QAPF field 7* (Le Maitre et al., 2005, p. 135). GSWA's rock classification scheme prefers the use of volcanic terminology for any igneous rock formed on or near the Earth's surface, i.e. for those hypabyssal or subvolcanic rocks such as dykes, sills, and cryptodomes that are demonstrably both spatially and temporally associated with extrusive volcanic rocks."@en ;
    skos:historyNote "Based on the IUGS classification of metamorphic (Fettes and Desmons, 2007) and igneous rocks (Le Maitre et al., 2005)." ;
    skos:inScheme cs: ;
    skos:notation "mftq"^^:gswa-rock-code ;
    skos:prefLabel "meta-quartz trachyte"@en ;
.

:meta-ultramafic-intrusive-rock
    a skos:Concept ;
    rdfs:isDefinedBy cs: ;
    skos:broader :meta-igneous-ultramafic-intrusive ;
    skos:definition "A metamorphosed rock consisting essentially of mafic minerals and derived from an ultramafic igneous (intrusive or coarse-grained extrusive) protolith, but otherwise uncategorized."@en ;
    skos:historyNote "Based on the IUGS classification of metamorphic (Fettes and Desmons, 2007) and igneous rocks (Le Maitre et al., 2005)." ;
    skos:inScheme cs: ;
    skos:notation "ma"^^:gswa-rock-code ;
    skos:prefLabel "meta-ultramafic intrusive rock"@en ;
    schema:citation "https://glossary.americangeosciences.org/term/ultramaficrock"^^xsd:anyURI ;
.

:meta-ultramafic-volcanic-rock
    a skos:Concept ;
    rdfs:isDefinedBy cs: ;
    skos:broader :meta-igneous-ultramafic-volcanic ;
    skos:definition "A metamorphosed igneous volcanic or volcaniclastic rock derived from a protolith composed chiefly of one or more ferromagnesian, dark-coloured minerals in its mode, but otherwise uncategorized (adapted from Glossary of geology, 5th edition revised; Neuendorf et al., 2011). Igneous protolith defined as a rock with M greater than 90%, where M represents the volume modal percentage of mafic and related minerals (Le Maitre et al., 2005, p. 4 and 153). GSWA's rock classification scheme prefers the use of volcanic terminology for any igneous rock formed on or near the Earth's surface, i.e. for those hypabyssal or subvolcanic rocks such as dykes, sills, and cryptodomes that are demonstrably both spatially and temporally associated with extrusive volcanic rocks."@en ;
    skos:historyNote "Based on the IUGS classification of metamorphic (Fettes and Desmons, 2007) and igneous rocks (Le Maitre et al., 2005)." ;
    skos:inScheme cs: ;
    skos:notation "mu"^^:gswa-rock-code ;
    skos:prefLabel "meta-ultramafic volcanic rock"@en ;
.

:meta-ultramafic-volcaniclastic-rock
    a skos:Concept ;
    rdfs:isDefinedBy cs: ;
    skos:broader :meta-igneous-ultramafic-volcanic ;
    skos:definition "A metamorphosed ultramafic volcaniclastic rock consisting of either (a) pyroclastic detritus or (b) terrigenous volcanic detritus of epiclastic origin and with an overall mafic composition, but otherwise uncategorized. 'Volcaniclastic' includes all clastic volcanic materials formed by any process of fragmentation, dispersed by any kind of transporting agent, deposited in any environment, or mixed in any significant portion with non-volcanic fragments."@en ;
    skos:historyNote "Compiled by the Geological Survey of Western Australia" ;
    skos:inScheme cs: ;
    skos:notation "muv"^^:gswa-rock-code ;
    skos:prefLabel "meta-ultramafic volcaniclastic rock"@en ;
.

:metabasalt
    a skos:Concept ;
    rdfs:isDefinedBy cs: ;
    skos:broader :meta-igneous-mafic-volcanic ;
    skos:definition "A fine-grained metamorphosed mafic volcanic rock consisting essentially of calcic plagioclase and pyroxene. Igneous protolith defined modally in QAPF fields 9 and 10 (Le Maitre et al., 2005, p. 31). GSWA's rock classification scheme prefers the use of volcanic terminology for any igneous rock formed on or near the Earth's surface, i.e. for those hypabyssal or subvolcanic rocks such as dykes, sills, and cryptodomes that are demonstrably both spatially and temporally associated with extrusive volcanic rocks."@en ;
    skos:historyNote "Based on the IUGS classification of metamorphic (Fettes and Desmons, 2007) and igneous rocks (Le Maitre et al., 2005)." ;
    skos:inScheme cs: ;
    skos:notation "mbb"^^:gswa-rock-code ;
    skos:prefLabel "metabasalt"@en ;
.

:metabasaltic-andesite
    a skos:Concept ;
    rdfs:isDefinedBy cs: ;
    skos:broader :meta-igneous-mafic-volcanic ;
    skos:definition "A fine-grained metamorphosed mafic volcanic rock with plagioclase of variable composition and the ferromagnesian minerals more commonly found in basalts, e.g. olivine. Igneous protolith defined chemically in TAS field O1 (Le Maitre et al., 2005, p. 61). GSWA's rock classification scheme prefers the use of volcanic terminology for any igneous rock formed on or near the Earth's surface, i.e. for those hypabyssal or subvolcanic rocks such as dykes, sills, and cryptodomes that are demonstrably both spatially and temporally associated with extrusive volcanic rocks."@en ;
    skos:historyNote "Based on the IUGS classification of metamorphic (Fettes and Desmons, 2007) and igneous rocks (Le Maitre et al., 2005)." ;
    skos:inScheme cs: ;
    skos:notation "mbd"^^:gswa-rock-code ;
    skos:prefLabel "metabasaltic andesite"@en ;
.

:metacarbonate-rock
    a skos:Concept ;
    rdfs:isDefinedBy cs: ;
    skos:broader :metasedimentary-carbonate ;
    skos:definition "A metamorphosed rock consisting essentially of carbonate minerals and derived from a carbonate protolith, but otherwise uncategorized."@en ;
    skos:historyNote "Compiled by the Geological Survey of Western Australia" ;
    skos:inScheme cs: ;
    skos:notation "mk"^^:gswa-rock-code ;
    skos:prefLabel "metacarbonate rock"@en ;
.

:metacarbonate-with-lesser-siliciclastic
    a skos:Concept ;
    rdfs:isDefinedBy cs: ;
    skos:broader :metasedimentary-carbonate ;
    skos:definition "Metamorphosed carbonate rocks interleaved at outcrop scale with subordinate metamorphosed siliciclastic rocks."@en ;
    skos:historyNote "Compiled by the Geological Survey of Western Australia" ;
    skos:inScheme cs: ;
    skos:notation "mkt"^^:gswa-rock-code ;
    skos:prefLabel "metacarbonate with lesser siliciclastic"@en ;
.

:metacarbonatite
    a skos:Concept ;
    rdfs:isDefinedBy cs: ;
    skos:broader :meta-igneous-carbonatite ;
    skos:definition "A collective term for a metamorphosed igneous (intrusive, extrusive or volcaniclastic) rock in which the protolith had a modal amount of primary carbonate minerals greater than 50%, but otherwise uncategorized (section 2.3, p. 10). (Cf. Le Maitre et al., 2005, p. 68)"@en ;
    skos:historyNote "Compiled by the Geological Survey of Western Australia" ;
    skos:inScheme cs: ;
    skos:notation "mq"^^:gswa-rock-code ;
    skos:prefLabel "metacarbonatite"@en ;
.

:metacarbonatite-granofels-hornfels
    a skos:Concept ;
    rdfs:isDefinedBy cs: ;
    skos:broader :meta-igneous-carbonatite ;
    skos:definition "A granofels/hornfels derived by (contact) metamorphism of a carbonatite, i.e. an igneous protolith containing a modal amount of primary carbonate minerals greater than 50%. See also definition of granofels/granofelsic structure in Fettes and Desmons (2007, p. 156); hornfels are granofels formed by contact metamorphism (Fettes and Desmons, 2007, p. 159)."@en ;
    skos:inScheme cs: ;
    skos:notation "mqe"^^:gswa-rock-code ;
    skos:prefLabel "metacarbonatite granofels/hornfels"@en ;
.

:metachert
    a skos:Concept ;
    rdfs:isDefinedBy cs: ;
    skos:broader :metasedimentary-other-chemical ;
    skos:definition "A metamorphosed chert."@en ;
    skos:historyNote "Compiled by the Geological Survey of Western Australia" ;
    skos:inScheme cs: ;
    skos:notation "mc"^^:gswa-rock-code ;
    skos:prefLabel "metachert"@en ;
.

:metaconglomerate
    a skos:Concept ;
    rdfs:isDefinedBy cs: ;
    skos:broader :metasedimentary-siliciclastic-psephite ;
    skos:definition "A metamorphosed rock derived from a siliciclastic sedimentary protolith with grain size greater than 2 mm, i.e. coarser than sand."@en ;
    skos:historyNote "Compiled by the Geological Survey of Western Australia" ;
    skos:inScheme cs: ;
    skos:notation "mx"^^:gswa-rock-code ;
    skos:prefLabel "metaconglomerate"@en ;
    schema:citation "https://glossary.americangeosciences.org/term/psephite"^^xsd:anyURI ;
.

:metadacite
    a skos:Concept ;
    rdfs:isDefinedBy cs: ;
    skos:broader :meta-igneous-felsic-volcanic ;
    skos:definition "A metamorphosed volcanic rock derived from a protolith composed of quartz and sodic plagioclase with minor amounts of biotite and/or hornblende and/or pyroxene (volcanic equivalent of granodiorite and tonalite). Igneous protolith defined modally in QAPF fields 4 and 5, and, if modes are not available, chemically in TAS field O3 (Le Maitre et al., 2005, p. 72). GSWA's rock classification scheme prefers the use of volcanic terminology for any igneous rock formed on or near the Earth's surface, i.e. for those hypabyssal or subvolcanic rocks such as dykes, sills, and cryptodomes that are demonstrably both spatially and temporally associated with extrusive volcanic rocks."@en ;
    skos:historyNote "Based on the IUGS classification of metamorphic (Fettes and Desmons, 2007) and igneous rocks (Le Maitre et al., 2005)." ;
    skos:inScheme cs: ;
    skos:notation "mfd"^^:gswa-rock-code ;
    skos:prefLabel "metadacite"@en ;
.

:metadiorite
    a skos:Concept ;
    rdfs:isDefinedBy cs: ;
    skos:broader :meta-igneous-felsic-intrusive ;
    skos:definition "A metamorphosed felsic intrusive rock derived from a protolith consisting of intermediate plagioclase, commonly with hornblende and often with biotite or augite. Igneous protolith defined modally in QAPF field 10 (Le Maitre et al., 2005, p. 73)."@en ;
    skos:historyNote "Based on the IUGS classification of metamorphic (Fettes and Desmons, 2007) and igneous rocks (Le Maitre et al., 2005)." ;
    skos:inScheme cs: ;
    skos:notation "mgi"^^:gswa-rock-code ;
    skos:prefLabel "metadiorite"@en ;
.

:metadolerite
    a skos:Concept ;
    rdfs:isDefinedBy cs: ;
    skos:broader :meta-igneous-mafic-intrusive ;
    skos:definition "A metamorphosed mafic intrusive rock (or coarse-grained part of extrusive successions) derived from a protolith intermediate in grain size between basalt and gabbro and composed essentially of plagioclase, pyroxene and opaque minerals with varying amounts of quartz and possibly olivine; often with ophitic texture. Igneous protolith defined modally in QAPF (Le Maitre et al., 2005, p. 74)."@en ;
    skos:historyNote "Based on the IUGS classification of metamorphic (Fettes and Desmons, 2007) and igneous rocks (Le Maitre et al., 2005)." ;
    skos:inScheme cs: ;
    skos:notation "mod"^^:gswa-rock-code ;
    skos:prefLabel "metadolerite"@en ;
.

:metadunite-derived-from-intrusive-rock
    a skos:Concept ;
    rdfs:isDefinedBy cs: ;
    skos:broader :meta-igneous-ultramafic-intrusive ;
    skos:definition "A metamorphosed ultramafic igneous (intrusive or coarse-grained extrusive) rock consisting essentially of olivine. Igneous protolith defined modally in the ultramafic rock classification of Le Maitre et al. (2005, p. 28)."@en ;
    skos:historyNote "Based on the IUGS classification of metamorphic (Fettes and Desmons, 2007) and igneous rocks (Le Maitre et al., 2005)." ;
    skos:inScheme cs: ;
    skos:notation "mad"^^:gswa-rock-code ;
    skos:prefLabel "metadunite derived from intrusive rock"@en ;
.

:metadunite-derived-from-volcanic-rock
    a skos:Concept ;
    rdfs:isDefinedBy cs: ;
    skos:broader :meta-igneous-ultramafic-volcanic ;
    skos:definition "A metamorphosed ultramafic volcanic rock consisting essentially of olivine. Igneous protolith defined modally in the ultramafic rock classification (cf. Le Maitre et al., 2005, p. 74). In GSWA usage this term refers to a metamorphosed dunite identified as formed from fractionation within thick bodies of ultramafic volcanic or subvolcanic magmas. GSWA's rock classification scheme prefers the use of volcanic terminology for any igneous rock formed on or near the Earth's surface, i.e. for those hypabyssal or subvolcanic rocks such as dykes, sills, and cryptodomes that are demonstrably both spatially and temporally associated with extrusive volcanic rocks."@en ;
    skos:historyNote "Based on the IUGS classification of metamorphic (Fettes and Desmons, 2007) and igneous rocks (Le Maitre et al., 2005)." ;
    skos:inScheme cs: ;
    skos:notation "mud"^^:gswa-rock-code ;
    skos:prefLabel "metadunite derived from volcanic rock"@en ;
.

:metafelsic-rock
    a skos:Concept ;
    rdfs:isDefinedBy cs: ;
    skos:broader :meta-igneous-felsic ;
    skos:definition "A metamorphosed felsic rock of igneous but otherwise unspecified origin, i.e. a felsic rock for which an igneous protolith (intrusive, extrusive or volcaniclastic) is interpreted but commonly too weathered or altered to make further distinctions."@en ;
    skos:historyNote "Compiled by the Geological Survey of Western Australia" ;
    skos:inScheme cs: ;
    skos:notation "mr"^^:gswa-rock-code ;
    skos:prefLabel "metafelsic rock"@en ;
    schema:citation "https://glossary.americangeosciences.org/term/felsic"^^xsd:anyURI ;
.

:metafelsic-volcanic-rock
    a skos:Concept ;
    rdfs:isDefinedBy cs: ;
    skos:broader :meta-igneous-felsic-volcanic ;
    skos:definition "A metamorphosed rock consisting essentially of felsic minerals and derived from a felsic volcanic protolith, but otherwise uncategorized. GSWA's rock classification scheme prefers the use of volcanic terminology for any igneous rock formed on or near the Earth's surface, i.e. for those hypabyssal or subvolcanic rocks such as dykes, sills, and cryptodomes that are demonstrably both spatially and temporally associated with extrusive volcanic rocks."@en ;
    skos:historyNote "Compiled by the Geological Survey of Western Australia" ;
    skos:inScheme cs: ;
    skos:notation "mf"^^:gswa-rock-code ;
    skos:prefLabel "metafelsic volcanic rock"@en ;
    schema:citation "https://glossary.americangeosciences.org/term/felsic"^^xsd:anyURI ;
.

:metafelsic-volcaniclastic-rock
    a skos:Concept ;
    rdfs:isDefinedBy cs: ;
    skos:broader :meta-igneous-felsic-volcanic ;
    skos:definition "A metamorphosed volcaniclastic rock consisting of either (a) pyroclastic detritus or (b) terrigenous volcanic detritus of epiclastic origin and with an overall felsic composition, but otherwise uncategorized. 'Volcaniclastic' includes all clastic volcanic materials formed by any process of fragmentation, dispersed by any kind of transporting agent, deposited in any environment, or mixed in any significant portion with non-volcanic fragments."@en ;
    skos:historyNote "Compiled by the Geological Survey of Western Australia" ;
    skos:inScheme cs: ;
    skos:notation "mfv"^^:gswa-rock-code ;
    skos:prefLabel "metafelsic volcaniclastic rock"@en ;
.

:metagabbro
    a skos:Concept ;
    rdfs:isDefinedBy cs: ;
    skos:broader :meta-igneous-mafic-intrusive ;
    skos:definition "A metamorphosed intrusive rock (or coarse-grained parts of extrusive successions), derived from a protolith composed essentially of calcic plagioclase, pyroxene and iron oxides, with varying amounts of quartz and possibly olivine. Igneous protolith defined modally in QAPF field 10 (cf. Le Maitre et al., 2005, p. 83)."@en ;
    skos:historyNote "Based on the IUGS classification of metamorphic (Fettes and Desmons, 2007) and igneous rocks (Le Maitre et al., 2005)." ;
    skos:inScheme cs: ;
    skos:notation "mog"^^:gswa-rock-code ;
    skos:prefLabel "metagabbro"@en ;
.

:metagabbronorite
    a skos:Concept ;
    rdfs:isDefinedBy cs: ;
    skos:broader :meta-igneous-mafic-intrusive ;
    skos:definition "A metamorphosed mafic intrusive rock (or coarse-grained parts of extrusive successions) derived from a protolith consisting of calcic plagioclase and roughly equal amounts of clinopyroxene and orthopyroxene. Igneous protolith defined modally in the gabbroic rock classification (Le Maitre et al., 2005, p. 83)."@en ;
    skos:historyNote "Based on the IUGS classification of metamorphic (Fettes and Desmons, 2007) and igneous rocks (Le Maitre et al., 2005)." ;
    skos:inScheme cs: ;
    skos:notation "mom"^^:gswa-rock-code ;
    skos:prefLabel "metagabbronorite"@en ;
.

:metagranitic-rock
    a skos:Concept ;
    rdfs:isDefinedBy cs: ;
    skos:broader :meta-igneous-felsic-intrusive ;
    skos:definition "In GSWA usage, a generic term for a metamorphosed rock derived from an igneous intrusive protolith composed chiefly of one or more felsic, light-coloured minerals in its mode and with quartz modal content between 0 and 60%, otherwise uncategorized."@en ;
    skos:historyNote "Based on the IUGS classification of metamorphic (Fettes and Desmons, 2007) and igneous rocks (Le Maitre et al., 2005)." ;
    skos:inScheme cs: ;
    skos:notation "mg"^^:gswa-rock-code ;
    skos:prefLabel "metagranitic rock"@en ;
.

:metagranodiorite
    a skos:Concept ;
    rdfs:isDefinedBy cs: ;
    skos:broader :meta-igneous-felsic-intrusive ;
    skos:definition "A metamorphosed felsic intrusive rock derived from a protolith consisting essentially of quartz, sodic plagioclase and lesser amounts of alkali feldspar with minor amounts of hornblende and biotite. Igneous protolith defined modally in QAPF field 4 (Le Maitre et al., 2005, p. 86)."@en ;
    skos:historyNote "Based on the IUGS classification of metamorphic (Fettes and Desmons, 2007) and igneous rocks (Le Maitre et al., 2005)." ;
    skos:inScheme cs: ;
    skos:notation "mgg"^^:gswa-rock-code ;
    skos:prefLabel "metagranodiorite"@en ;
.

:metahydrothermal-chert
    a skos:Concept ;
    rdfs:isDefinedBy cs: ;
    skos:broader :metamorphosed-hydrothermal ;
    skos:definition "A metamorphosed, fine-grained siliceous rock that precipitated originally from a hydrothermal fluid related to seafloor or sub-seafloor volcanism."@en ;
    skos:historyNote "Compiled by the Geological Survey of Western Australia" ;
    skos:inScheme cs: ;
    skos:notation "mzc"^^:gswa-rock-code ;
    skos:prefLabel "metahydrothermal chert"@en ;
    schema:citation
        "Adachi"^^xsd:anyURI ,
        "Hydrothermal chert and associated siliceous rocks from the northern Pacific their geological significance as indication od ocean ridge activity: Sedimentary Geology"^^xsd:anyURI ,
        "K"^^xsd:anyURI ,
        "M"^^xsd:anyURI ,
        "R 1986"^^xsd:anyURI ,
        "Sugisaki"^^xsd:anyURI ,
        "Yamamoto"^^xsd:anyURI ,
        "doi.org/10.1016/0037-0738(86)90075-8."^^xsd:anyURI ,
        "https://doi.org/10.3390/min12101333"^^xsd:anyURI ,
        "p. 125-148"^^xsd:anyURI ,
        "vol. 47(1–2)"^^xsd:anyURI ;
.

:metakomatiite
    a skos:Concept ;
    rdfs:isDefinedBy cs: ;
    skos:broader :meta-igneous-ultramafic-volcanic ;
    skos:definition "A metamorphosed ultramafic extrusive rock derived from lavas that crystallize from high temperature magmas with 18% to 32% MgO. Pillows, chilled flow-tops and spinifex textures are commonly preserved. Igneous protolith defined chemically in the TAS classification (cf. Le Maitre et al., 2005, p. 98)."@en ;
    skos:historyNote "Based on the IUGS classification of metamorphic (Fettes and Desmons, 2007) and igneous rocks (Le Maitre et al., 2005)." ;
    skos:inScheme cs: ;
    skos:notation "muk"^^:gswa-rock-code ;
    skos:prefLabel "metakomatiite"@en ;
.

:metakomatiitic-basalt
    a skos:Concept ;
    rdfs:isDefinedBy cs: ;
    skos:broader :meta-igneous-mafic-volcanic ;
    skos:definition "A metamorphosed member of the komatiite series derived from a volcanic rock characterized by MgO in the range 5–15%, typically displaying spinifex texture and evidence of rapid quenching of high-temperature magma (cf. Le Maitre et al., 2005, p. 61) and this vocabulary for a definition of the igneous protolith. GSWA's rock classification scheme prefers the use of volcanic terminology for any igneous rock formed on or near the Earth's surface, i.e. for those hypabyssal or subvolcanic rocks such as dykes, sills, and cryptodomes that are demonstrably both spatially and temporally associated with extrusive volcanic rocks."@en ;
    skos:historyNote "Based on the IUGS classification of metamorphic (Fettes and Desmons, 2007) and igneous rocks (Le Maitre et al., 2005)." ;
    skos:inScheme cs: ;
    skos:notation "mbm"^^:gswa-rock-code ;
    skos:prefLabel "metakomatiitic basalt"@en ;
.

:metalatite
    a skos:Concept ;
    rdfs:isDefinedBy cs: ;
    skos:broader :meta-igneous-felsic-volcanic ;
    skos:definition "A metamorphosed rock derived from a protolith chemically lying between trachyte and andesite, i.e. derived from a volcanic rock composed of approximately equal amounts of alkali feldspar and sodic plagioclase. Igneous protolith defined modally in QAPF field 8 and, if modes are not available, chemically as the potassic variety of trachyandesite in TAS field S3 (Le Maitre et al., 2005, p. 101). GSWA's rock classification scheme prefers the use of volcanic terminology for any igneous rock formed on or near the Earth's surface, i.e. for those hypabyssal or subvolcanic rocks such as dykes, sills, and cryptodomes that are demonstrably both spatially and temporally associated with extrusive volcanic rocks."@en ;
    skos:historyNote "Based on the IUGS classification of metamorphic (Fettes and Desmons, 2007) and igneous rocks (Le Maitre et al., 2005)." ;
    skos:inScheme cs: ;
    skos:notation "mfl"^^:gswa-rock-code ;
    skos:prefLabel "metalatite"@en ;
.

:metamafic-intrusive-rock
    a skos:Concept ;
    rdfs:isDefinedBy cs: ;
    skos:broader :meta-igneous-mafic-intrusive ;
    skos:definition "A metamorphosed rock consisting essentially of mafic minerals and derived from a mafic intrusive protolith or from coarse-grained parts of extrusive successions, but otherwise uncategorized."@en ;
    skos:historyNote "Compiled by the Geological Survey of Western Australia" ;
    skos:inScheme cs: ;
    skos:notation "mo"^^:gswa-rock-code ;
    skos:prefLabel "metamafic intrusive rock"@en ;
.

:metamafic-rock
    a skos:Concept ;
    rdfs:isDefinedBy cs: ;
    skos:broader :meta-igneous-mafic ;
    skos:definition "A metamorphosed mafic rock, i.e. the metamorphosed equivalent of an igneous intrusive, extrusive or volcaniclastic rock mainly consisting of mafic minerals for which an igneous protolith is interpreted but commonly too weathered or altered to make further distinctions (cf. Fettes and Desmons, 2007, p.170)."@en ;
    skos:historyNote "Based on the IUGS classification of metamorphic rocks (Fettes and Desmons, 2007) and GSWA usage." ;
    skos:inScheme cs: ;
    skos:notation "mw"^^:gswa-rock-code ;
    skos:prefLabel "metamafic rock"@en ;
    schema:citation "https://glossary.americangeosciences.org/term/mafic"^^xsd:anyURI ;
.

:metamafic-volcanic-rock
    a skos:Concept ;
    rdfs:isDefinedBy cs: ;
    skos:broader :meta-igneous-mafic-volcanic ;
    skos:definition "A metamorphosed rock consisting essentially of mafic minerals and derived from a mafic volcanic protolith, but otherwise uncategorized. GSWA's rock classification scheme prefers the use of volcanic terminology for any igneous rock formed on or near the Earth's surface, i.e. for those hypabyssal or subvolcanic rocks such as dykes, sills, and cryptodomes that are demonstrably both spatially and temporally associated with extrusive volcanic rocks."@en ;
    skos:historyNote "Based on the IUGS classification of metamorphic (Fettes and Desmons, 2007) and igneous rocks (Le Maitre et al., 2005)." ;
    skos:inScheme cs: ;
    skos:notation "mb"^^:gswa-rock-code ;
    skos:prefLabel "metamafic volcanic rock"@en ;
    schema:citation "https://glossary.americangeosciences.org/term/mafic"^^xsd:anyURI ;
.

:metamafic-volcaniclastic-rock
    a skos:Concept ;
    rdfs:isDefinedBy cs: ;
    skos:broader :meta-igneous-mafic-volcanic ;
    skos:definition "A metamorphosed volcaniclastic rock consisting of either (a) pyroclastic detritus or (b) terrigenous volcanic detritus of epiclastic origin and with an overall mafic composition, but otherwise uncategorized. 'Volcaniclastic' includes all clastic volcanic materials formed by any process of fragmentation, dispersed by any kind of transporting agent, deposited in any environment, or mixed in any significant portion with non-volcanic fragments."@en ;
    skos:historyNote "Compiled by the Geological Survey of Western Australia" ;
    skos:inScheme cs: ;
    skos:notation "mbv"^^:gswa-rock-code ;
    skos:prefLabel "metamafic volcaniclastic rock"@en ;
.

:metamonzodiorite
    a skos:Concept ;
    rdfs:isDefinedBy cs: ;
    skos:broader :meta-igneous-felsic-intrusive ;
    skos:definition "A metamorphosed felsic intrusive rock derived from a protolith intermediate between monzonite and diorite. Igneous protolith defined modally in QAPF field 9 (Le Maitre et al., 2005, p. 113)."@en ;
    skos:historyNote "Based on the IUGS classification of metamorphic (Fettes and Desmons, 2007) and igneous rocks (Le Maitre et al., 2005)." ;
    skos:inScheme cs: ;
    skos:notation "mgh"^^:gswa-rock-code ;
    skos:prefLabel "metamonzodiorite"@en ;
    schema:citation "https://glossary.americangeosciences.org/term/monzodiorite"^^xsd:anyURI ;
.

:metamonzogranite
    a skos:Concept ;
    rdfs:isDefinedBy cs: ;
    skos:broader :meta-igneous-felsic-intrusive ;
    skos:definition "A metamorphosed felsic intrusive rock derived from a monzogranite, i.e. from a variety of granite in QAPF field 3b having roughly equal amounts of alkali feldspar and plagioclase (cf. Le Maitre et al., 2005, p. 113)."@en ;
    skos:historyNote "Based on the IUGS classification of metamorphic (Fettes and Desmons, 2007) and igneous rocks (Le Maitre et al., 2005)." ;
    skos:inScheme cs: ;
    skos:notation "mgm"^^:gswa-rock-code ;
    skos:prefLabel "metamonzogranite"@en ;
.

:metamonzonite
    a skos:Concept ;
    rdfs:isDefinedBy cs: ;
    skos:broader :meta-igneous-felsic-intrusive ;
    skos:definition "A metamorphosed felsic intrusive rock derived from a monzonite, i.e. an intrusive rock containing almost equal amounts of plagioclase and alkali feldspar with minor amphibole and/or pyroxene. Igneous protolith defined modally in QAPF field 8 (Le Maitre et al., 2005, p. 113)."@en ;
    skos:historyNote "Based on the IUGS classification of metamorphic (Fettes and Desmons, 2007) and igneous rocks (Le Maitre et al., 2005)." ;
    skos:inScheme cs: ;
    skos:notation "mgz"^^:gswa-rock-code ;
    skos:prefLabel "metamonzonite"@en ;
.

:metamorphic-rock
    a skos:Concept ;
    rdfs:isDefinedBy cs: ;
    skos:broader :metamorphic ;
    skos:definition "A metamorphic rock so deeply altered/weathered that no inference can be made as to the protolith and with no discernible structures."@en ;
    skos:exactMatch
        <http://inspire.ec.europa.eu/codelist/LithologyValue/metamorphicRock> ,
        <http://resource.geosciml.org/classifier/cgi/lithology/metamorphic_rock> ;
    skos:historyNote "Compiled by the Geological Survey of Western Australia" ;
    skos:inScheme cs: ;
    skos:notation "m"^^:gswa-rock-code ;
    skos:prefLabel "metamorphic rock"@en ;
.

:metamorphosed-hydrothermal-rock
    a skos:Concept ;
    rdfs:isDefinedBy cs: ;
    skos:broader :metamorphosed-hydrothermal ;
    skos:definition "A hydrothermal rock that has undergone metamorphism, otherwise uncategorized."@en ;
    skos:historyNote "Compiled by the Geological Survey of Western Australia" ;
    skos:inScheme cs: ;
    skos:notation "mz"^^:gswa-rock-code ;
    skos:prefLabel "metamorphosed hydrothermal rock"@en ;
.

:metanorite
    a skos:Concept ;
    rdfs:isDefinedBy cs: ;
    skos:broader :meta-igneous-mafic-intrusive ;
    skos:definition "A metamorphosed mafic intrusive rock (or coarse-grained parts of extrusive successions) derived from a norite, i.e. a rock composed essentially of bytownite, labradorite or andesine and orthopyroxene. Igneous protolith defined modally in the gabbroic rock classification (Le Maitre et al., 2005, p. 117)."@en ;
    skos:historyNote "Based on the IUGS classification of metamorphic (Fettes and Desmons, 2007) and igneous rocks (Le Maitre et al., 2005)." ;
    skos:inScheme cs: ;
    skos:notation "mow"^^:gswa-rock-code ;
    skos:prefLabel "metanorite"@en ;
.

:metapegmatite
    a skos:Concept ;
    rdfs:isDefinedBy cs: ;
    skos:broader :meta-igneous-felsic-intrusive ;
    skos:definition "The metamorphosed equivalent of a pegmatite, i.e. an exceptionally coarse-grained igneous rock with interlocking crystals, usually found as irregular dykes, lenses, or veins, especially at the margins of batholiths and of granitic composition (cf. Le Maitre et al., 2005, p. 125)."@en ;
    skos:historyNote "Based on the IUGS classification of metamorphic (Fettes and Desmons, 2007) and igneous rocks (Le Maitre et al., 2005)." ;
    skos:inScheme cs: ;
    skos:notation "mgp"^^:gswa-rock-code ;
    skos:prefLabel "metapegmatite"@en ;
.

:metaperidotite-derived-from-intrusive-rock
    a skos:Concept ;
    rdfs:isDefinedBy cs: ;
    skos:broader :meta-igneous-ultramafic-intrusive ;
    skos:definition "A metamorphosed ultramafic igneous (intrusive or coarse-grained extrusive) rock consisting essentially of olivine, pyroxene and/or amphibole. Igneous protolith defined modally in the ultramafic rock classification of Le Maitre et al. (2005, p. 28)."@en ;
    skos:historyNote "Based on the IUGS classification of metamorphic (Fettes and Desmons, 2007) and igneous rocks (Le Maitre et al., 2005)." ;
    skos:inScheme cs: ;
    skos:notation "map"^^:gswa-rock-code ;
    skos:prefLabel "metaperidotite derived from intrusive rock"@en ;
.

:metaperidotite-derived-from-volcanic-rock
    a skos:Concept ;
    rdfs:isDefinedBy cs: ;
    skos:broader :meta-igneous-ultramafic-volcanic ;
    skos:definition "A collective term for metamorphosed ultramafic volcanic rocks derived from a protolith consisting essentially of olivine, pyroxene and/or amphibole. Igneous protolith defined modally in the ultramafic rock classification of Le Maitre et al. (2005, p. 28 and 126). In GSWA usage this term refers to a metamorphosed peridotite identified as formed from fractionation within thick bodies of ultramafic volcanic or subvolcanic magmas."@en ;
    skos:historyNote "Based on the IUGS classification of metamorphic (Fettes and Desmons, 2007) and igneous rocks (Le Maitre et al., 2005)." ;
    skos:inScheme cs: ;
    skos:notation "mup"^^:gswa-rock-code ;
    skos:prefLabel "metaperidotite derived from volcanic rock"@en ;
.

:metapyroxenite-derived-from-intrusive-rock
    a skos:Concept ;
    rdfs:isDefinedBy cs: ;
    skos:broader :meta-igneous-ultramafic-intrusive ;
    skos:definition "Metamorphic rock consisting of more than 90% modal pyroxene (Fettes and Desmons, 2007, p. 190), i.e. a metamorphosed ultramafic igneous (intrusive or coarse-grained extrusive) rock composed almost entirely of one or more pyroxenes and occasionally biotite, hornblende and olivine. Igneous protolith defined modally in the ultramafic rock classification of Le Maitre et al. (2005, p. 28)."@en ;
    skos:historyNote "Based on the IUGS classification of metamorphic (Fettes and Desmons, 2007) and igneous rocks (Le Maitre et al., 2005)." ;
    skos:inScheme cs: ;
    skos:notation "max"^^:gswa-rock-code ;
    skos:prefLabel "metapyroxenite derived from intrusive rock"@en ;
.

:metapyroxenite-derived-from-volcanic-rock
    a skos:Concept ;
    rdfs:isDefinedBy cs: ;
    skos:broader :meta-igneous-ultramafic-volcanic ;
    skos:definition "A metamorphosed ultramafic volcanic or volcaniclastic rock derived from a protolith composed almost entirely of one or more pyroxenes (greater than 90% modal pyroxenes) and occasionally biotite, hornblende and olivine; igneous protolith defined modally in the ultramafic rock classification (cf. Le Maitre et al., 2005, p. 28 and 134; Fettes and Desmons, 2007, p. 190). In GSWA usage this term refers to a metamorphosed pyroxenite identified as formed from fractionation within thick bodies of ultramafic volcanic or subvolcanic magmas."@en ;
    skos:historyNote "Based on the IUGS classification of metamorphic (Fettes and Desmons, 2007) and igneous rocks (Le Maitre et al., 2005)." ;
    skos:inScheme cs: ;
    skos:notation "mux"^^:gswa-rock-code ;
    skos:prefLabel "metapyroxenite derived from volcanic rock"@en ;
.

:metarhyodacite
    a skos:Concept ;
    rdfs:isDefinedBy cs: ;
    skos:broader :meta-igneous-felsic-volcanic ;
    skos:definition "A metamorphosed volcanic rock derived from a protolith intermediate between rhyolite and dacite. Igneous protolith defined as consisting of phenocrysts of quartz, plagioclase and a few ferromagnesian minerals in a microcrystalline groundmass (Le Maitre et al., 2005, p. 137). GSWA's rock classification scheme prefers the use of volcanic terminology for any igneous rock formed on or near the Earth's surface, i.e. for those hypabyssal or subvolcanic rocks such as dykes, sills, and cryptodomes that are demonstrably both spatially and temporally associated with extrusive volcanic rocks."@en ;
    skos:historyNote "Based on the IUGS classification of metamorphic (Fettes and Desmons, 2007) and igneous rocks (Le Maitre et al., 2005)." ;
    skos:inScheme cs: ;
    skos:notation "mfc"^^:gswa-rock-code ;
    skos:prefLabel "metarhyodacite"@en ;
.

:metarhyolite
    a skos:Concept ;
    rdfs:isDefinedBy cs: ;
    skos:broader :meta-igneous-felsic-volcanic ;
    skos:definition "A metamorphosed silicic volcanic rocks derived from a rhyolitic protolith, i.e. a rock consisting of phenocrysts of quartz and alkali feldspar, often with minor plagioclase and biotite, in a microcrystalline or glassy groundmass and having the chemical composition of granite. Igneous protolith defined modally in QAPF field 3 and, if modes are not available, chemically in TAS field R (Le Maitre et al., 2005, p. 137). GSWA's rock classification scheme prefers the use of volcanic terminology for any igneous rock formed on or near the Earth's surface, i.e. for those hypabyssal or subvolcanic rocks such as dykes, sills, and cryptodomes that are demonstrably both spatially and temporally associated with extrusive volcanic rocks."@en ;
    skos:historyNote "Based on the IUGS classification of metamorphic (Fettes and Desmons, 2007) and igneous rocks (Le Maitre et al., 2005)." ;
    skos:inScheme cs: ;
    skos:notation "mfr"^^:gswa-rock-code ;
    skos:prefLabel "metarhyolite"@en ;
.

:metasandstone
    a skos:Concept ;
    rdfs:isDefinedBy cs: ;
    skos:broader :metasedimentary-siliciclastic-psammite ;
    skos:definition "A metamorphosed rock derived from a siliciclastic sedimentary protolith with grain size between 0.0625 and 2 mm."@en ;
    skos:historyNote "Compiled by the Geological Survey of Western Australia" ;
    skos:inScheme cs: ;
    skos:notation "mt"^^:gswa-rock-code ;
    skos:prefLabel "metasandstone"@en ;
.

:metasedimentary-rock
    a skos:Concept ;
    rdfs:isDefinedBy cs: ;
    skos:broader :metasedimentary ;
    skos:definition "A metamorphosed rock of sedimentary but otherwise unspecified origin, i.e. a rock for which a clastic or chemical/biochemical derivation cannot be conclusively established (e.g. due to weathering )."@en ;
    skos:historyNote "Compiled by the Geological Survey of Western Australia" ;
    skos:inScheme cs: ;
    skos:notation "msed"^^:gswa-rock-code ;
    skos:prefLabel "metasedimentary rock"@en ;
    schema:citation "https://glossary.americangeosciences.org/term/sedimentary"^^xsd:anyURI ;
.

:metasiliciclastic-rock
    a skos:Concept ;
    rdfs:isDefinedBy cs: ;
    skos:broader :metasedimentary-siliciclastic ;
    skos:definition "A metamorphosed rock derived from a siliciclastic protolith, i.e. from silicon-bearing (in the form of quartz and silicates), clastic non-carbonate rocks, but otherwise uncategorized. Adapted from Glossary of geology (5th edition revised; Neuendorf et al., 2011)"@en ;
    skos:historyNote "Compiled by the Geological Survey of Western Australia" ;
    skos:inScheme cs: ;
    skos:notation "md"^^:gswa-rock-code ;
    skos:prefLabel "metasiliciclastic rock"@en ;
    schema:citation
        "https://glossary.americangeosciences.org/term/clastic"^^xsd:anyURI ,
        "https://glossary.americangeosciences.org/term/siliciclastic"^^xsd:anyURI ;
.

:metasiltstone-metamudstone-metashale
    a skos:Concept ;
    rdfs:isDefinedBy cs: ;
    skos:broader :metasedimentary-siliciclastic-pelite ;
    skos:definition "A metamorphosed rock derived from a siliciclastic sedimentary protolith with grains less than 0.0625 mm in size."@en ;
    skos:historyNote "Compiled by the Geological Survey of Western Australia" ;
    skos:inScheme cs: ;
    skos:notation "ml"^^:gswa-rock-code ;
    skos:prefLabel "metasiltstone/metamudstone/metashale"@en ;
.

:metasomatic-gneiss
    a skos:Concept ;
    rdfs:isDefinedBy cs: ;
    skos:broader :metasomatic ;
    skos:definition "A metasomatic gneissose rock for which the protolith cannot be established. The timing of metasomatism is not implied and may precede or follow the development of gneissosity during regional metamorphism. A gneiss is a layered rock formed by regional metamorphism, in which bands or lenticles of granular minerals alternate with bands or lenticles in which minerals having flaky or elongate prismatic habits predominate (Fettes and Desmon, 2007, p. 154)."@en ;
    skos:historyNote "Based on the IUGS classification of metamorphic rocks (Fettes and Desmons, 2007)." ;
    skos:inScheme cs: ;
    skos:notation "mjn"^^:gswa-rock-code ;
    skos:prefLabel "metasomatic gneiss"@en ;
    schema:citation
        "https://glossary.americangeosciences.org/term/gneiss"^^xsd:anyURI ,
        "https://glossary.americangeosciences.org/term/metasomaticrock"^^xsd:anyURI ;
.

:metasomatic-granofels-hornfels
    a skos:Concept ;
    rdfs:isDefinedBy cs: ;
    skos:broader :metasomatic ;
    skos:definition "A metasomatic rock composed of a mosaic of equidimensional grains without preferred orientation and for which the original protolith cannot be identified. Granofels are metamorphic rocks defined by their granofelsic structure, i.e. the absence of schistosity, such that the mineral grains and aggregates of mineral grains are equant or, if inequant, have random orientation. Mineralogical or lithological layering may be present. (Fettes and Desmons, 2007, p. 156); hornfels are granofels that formed as a result of contact metamorphism (Fettes and Desmons, 2007, p. 159)."@en ;
    skos:historyNote "Based on the IUGS classification of metamorphic rocks (Fettes and Desmons, 2007)." ;
    skos:inScheme cs: ;
    skos:notation "mje"^^:gswa-rock-code ;
    skos:prefLabel "metasomatic granofels/hornfels"@en ;
    schema:citation
        "https://en.wikipedia.org/wiki/Hornfels"^^xsd:anyURI ,
        "https://glossary.americangeosciences.org/term/granofels"^^xsd:anyURI ,
        "https://glossary.americangeosciences.org/term/hornfels;"^^xsd:anyURI ,
        "https://glossary.americangeosciences.org/term/metasomaticrock"^^xsd:anyURI ;
.

:metasomatic-rock
    a skos:Concept ;
    rdfs:isDefinedBy cs: ;
    skos:altLabel "metasomatite"@en ;
    skos:broader :metasomatic ;
    skos:definition "Metamorphic rock whose mineral and chemical bulk compositions have been substantially changed by metasomatism, i.e. the metamorphic process by which the chemical composition of a rock or rock portion is altered in a pervasive manner by the introduction and/or removal of chemical components as a result of interaction with aqueous fluids/solutions ((usually hydrothermal or static fluids); during metasomatism the rock remains in a solid state (Fettes and Desmons, 2007, p. 174)."@en ;
    skos:exactMatch
        <http://inspire.ec.europa.eu/codelist/LithologyValue/metasomaticRock> ,
        <http://resource.geosciml.org/classifier/cgi/lithology/metasomatic_rock> ;
    skos:historyNote "Based on the IUGS classification of metamorphic rocks (Fettes and Desmons, 2007)." ;
    skos:inScheme cs: ;
    skos:notation "mj"^^:gswa-rock-code ;
    skos:prefLabel "metasomatic rock"@en ;
    schema:citation "https://glossary.americangeosciences.org/term/metasomaticrock"^^xsd:anyURI ;
.

:metasomatic-schist
    a skos:Concept ;
    rdfs:isDefinedBy cs: ;
    skos:broader :metasomatic ;
    skos:definition "A metasomatic schistose rock for which the protolith cannot be established. The timing of metasomatism is not implied and may precede or follow the development of schistosity during regional metamorphism. A schist is a metamorphic rock displaying schistosity, i.e. a preferred orientation of inequant mineral grains or grain aggregates, such that the rock will split on a scale of less than a centimetre (well-developed schistosity), or on a scale of more than one centimetre (poorly-developed schistosity) (Fettes and Desmon, 2007, p. 193)."@en ;
    skos:historyNote "Based on the IUGS classification of metamorphic rocks (Fettes and Desmons, 2007)." ;
    skos:inScheme cs: ;
    skos:notation "mjs"^^:gswa-rock-code ;
    skos:prefLabel "metasomatic schist"@en ;
    schema:citation
        "https://glossary.americangeosciences.org/term/metasomaticrock"^^xsd:anyURI ,
        "https://glossary.americangeosciences.org/term/schist"^^xsd:anyURI ;
.

:metasyenite
    a skos:Concept ;
    rdfs:isDefinedBy cs: ;
    skos:broader :meta-igneous-felsic-intrusive ;
    skos:definition "A metamorphosed felsic intrusive rock derived from a syenite, i.e. an intrusive rock consisting mainly of alkali feldspar with subordinate sodic plagioclase, biotite, pyroxene, amphibole and occasional fayalite. Minor quartz or nepheline may also be present. Igneous protolith defined modally in QAPF field 7 (Le Maitre et al., 2005, p. 145)."@en ;
    skos:historyNote "Based on the IUGS classification of metamorphic (Fettes and Desmons, 2007) and igneous rocks (Le Maitre et al., 2005)." ;
    skos:inScheme cs: ;
    skos:notation "mgw"^^:gswa-rock-code ;
    skos:prefLabel "metasyenite"@en ;
.

:metasyenogranite
    a skos:Concept ;
    rdfs:isDefinedBy cs: ;
    skos:broader :meta-igneous-felsic-intrusive ;
    skos:definition "A metamorphosed felsic intrusive rock derived from a syenogranite, i.e. from a variety of granite in QAPF field 3a consisting of alkali feldspar with subordinate plagioclase (Le Maitre et al., 2005, p. 146)."@en ;
    skos:historyNote "Based on the IUGS classification of metamorphic (Fettes and Desmons, 2007) and igneous rocks (Le Maitre et al., 2005)." ;
    skos:inScheme cs: ;
    skos:notation "mgr"^^:gswa-rock-code ;
    skos:prefLabel "metasyenogranite"@en ;
.

:metatonalite
    a skos:Concept ;
    rdfs:isDefinedBy cs: ;
    skos:broader :meta-igneous-felsic-intrusive ;
    skos:definition "A metamorphosed felsic intrusive rock derived from a tonalite, i.e. an intrusive rock consisting essentially of quartz and intermediate plagioclase, usually with biotite and amphibole. Igneous protolith defined modally in QAPF field 5 (Le Maitre et al., 2005, p. 149)."@en ;
    skos:historyNote "Based on the IUGS classification of metamorphic (Fettes and Desmons, 2007) and igneous rocks (Le Maitre et al., 2005)." ;
    skos:inScheme cs: ;
    skos:notation "mgt"^^:gswa-rock-code ;
    skos:prefLabel "metatonalite"@en ;
.

:metatrachyte
    a skos:Concept ;
    rdfs:isDefinedBy cs: ;
    skos:broader :meta-igneous-felsic-volcanic ;
    skos:definition "A metamorphosed volcanic rock derived from a protolith consisting essentially of alkali feldspar. Igneous protolith defined modally in QAPF field 7 and, if modes are not available, chemically in TAS field T (Le Maitre et al., 2005, p. 151). GSWA's rock classification scheme prefers the use of volcanic terminology for any igneous rock formed on or near the Earth's surface, i.e. for those hypabyssal or subvolcanic rocks such as dykes, sills, and cryptodomes that are demonstrably both spatially and temporally associated with extrusive volcanic rocks."@en ;
    skos:historyNote "Based on the IUGS classification of metamorphic (Fettes and Desmons, 2007) and igneous rocks (Le Maitre et al., 2005)." ;
    skos:inScheme cs: ;
    skos:notation "mft"^^:gswa-rock-code ;
    skos:prefLabel "metatrachyte"@en ;
.

:metatroctolite
    a skos:Concept ;
    rdfs:isDefinedBy cs: ;
    skos:broader :meta-igneous-mafic-intrusive ;
    skos:definition "A metamorphosed mafic intrusive rock (or coarse-grained parts of extrusive successions) derived from a troctolite, i.e. a variety of gabbro composed essentially of highly calcic plagioclase and olivine with little or no pyroxene. Igneous protolith defined modally in the gabbroic rock classification (Le Maitre et al., 2005, p. 151)."@en ;
    skos:historyNote "Based on the IUGS classification of metamorphic (Fettes and Desmons, 2007) and igneous rocks (Le Maitre et al., 2005)." ;
    skos:inScheme cs: ;
    skos:notation "mot"^^:gswa-rock-code ;
    skos:prefLabel "metatroctolite"@en ;
.

:metavolcanic-and-metavolcaniclastic-rock
    a skos:Concept ;
    rdfs:isDefinedBy cs: ;
    skos:broader :meta-igneous-volcanic-or-volcaniclastic ;
    skos:definition "A metamorphosed rock derived from a volcanic or volcaniclastic protolith, but otherwise uncategorized in terms or composition or grain size."@en ;
    skos:historyNote "Compiled by the Geological Survey of Western Australia" ;
    skos:inScheme cs: ;
    skos:notation "mv"^^:gswa-rock-code ;
    skos:prefLabel "metavolcanic and metavolcaniclastic rock"@en ;
.

:micaceous-fault-rock
    a skos:Concept ;
    rdfs:isDefinedBy cs: ;
    skos:broader :metamorphic-protolith-unknown-fault-rock ;
    skos:definition "A rock formed as a result of deformation in a fault zone and distinguished by the abundance of micaceous mineral phases. In GSWA usage, this term is reserved for fault rocks for which a protolith cannot be conclusively established."@en ;
    skos:historyNote "Compiled by the Geological Survey of Western Australia" ;
    skos:inScheme cs: ;
    skos:notation "mym"^^:gswa-rock-code ;
    skos:prefLabel "micaceous fault rock"@en ;
.

:micaceous-gneiss
    a skos:Concept ;
    rdfs:isDefinedBy cs: ;
    skos:broader :metamorphic-protolith-unknown-gneiss ;
    skos:definition "A gneiss distinguished by the abundance of micaceous mineral phases. In GSWA usage, this term is reserved for a gneiss for which a protolith cannot be conclusively established. See also definition of gneiss/gneissose structure in Fettes and Desmons (2007, p. 154–155)."@en ;
    skos:historyNote "Based on the IUGS classification of metamorphic rocks (Fettes and Desmons, 2007) and GSWA usage." ;
    skos:inScheme cs: ;
    skos:notation "mnm"^^:gswa-rock-code ;
    skos:prefLabel "micaceous gneiss"@en ;
    schema:citation "https://glossary.americangeosciences.org/term/gneiss"^^xsd:anyURI ;
.

:micaceous-granofels-hornfels
    a skos:Concept ;
    rdfs:isDefinedBy cs: ;
    skos:broader :metamorphic-protolith-unknown-granofels-hornfels ;
    skos:definition "A granofels/hornfels distinguished by the abundance of micaceous mineral phases. In GSWA usage, this term is reserved for a granofels/hornfels for which a protolith cannot be conclusively established."@en ;
    skos:historyNote "Compiled by the Geological Survey of Western Australia" ;
    skos:inScheme cs: ;
    skos:notation "mem"^^:gswa-rock-code ;
    skos:prefLabel "micaceous granofels/hornfels"@en ;
.

:micaceous-schist
    a skos:Concept ;
    rdfs:isDefinedBy cs: ;
    skos:broader :metamorphic-protolith-unknown-schist ;
    skos:definition "A schist distinguished by the abundance of micaceous mineral phases. In GSWA usage, this term is reserved for a schist for which a protolith cannot be conclusively established. See also definition of schist/schistose structure in Fettes and Desmons, 2007, p.  193)."@en ;
    skos:historyNote "Based on the IUGS classification of metamorphic rocks (Fettes and Desmons, 2007) and GSWA usage." ;
    skos:inScheme cs: ;
    skos:notation "msm"^^:gswa-rock-code ;
    skos:prefLabel "micaceous schist"@en ;
.

:micro-alkali-feldspar-granite
    a skos:Concept ;
    rdfs:isDefinedBy cs: ;
    skos:broader :igneous-felsic-intrusive ;
    skos:definition "An alkali feldspar granite with a grain size of less than 3 mm. Includes porphyritic varieties."@en ;
    skos:historyNote "Based on the IUGS classification of igneous rocks (Le Maitre et al., 2005) and GSWA usage." ;
    skos:inScheme cs: ;
    skos:notation "gfa"^^:gswa-rock-code ;
    skos:prefLabel "micro alkali feldspar granite"@en ;
.

:micro-alkali-feldspar-syenite
    a skos:Concept ;
    rdfs:isDefinedBy cs: ;
    skos:broader :igneous-felsic-intrusive ;
    skos:definition "An alkali feldspar syenite with a grain size of less than 3 mm. Includes porphyritic varieties."@en ;
    skos:historyNote "Based on the IUGS classification of igneous rocks (Le Maitre et al., 2005) and GSWA usage." ;
    skos:inScheme cs: ;
    skos:notation "gsa"^^:gswa-rock-code ;
    skos:prefLabel "micro alkali feldspar syenite"@en ;
.

:micro-granitic-rock-undivided
    a skos:Concept ;
    rdfs:isDefinedBy cs: ;
    skos:broader :igneous-felsic-intrusive ;
    skos:definition "A granitic rock, undivided, with a grain size of less than 3 mm. Includes porphyritic varieties."@en ;
    skos:historyNote "Based on the IUGS classification of igneous rocks (Le Maitre et al., 2005) and GSWA usage." ;
    skos:inScheme cs: ;
    skos:notation "gna"^^:gswa-rock-code ;
    skos:prefLabel "micro granitic rock; undivided"@en ;
.

:micro-quartz-alkali-feldspar-syenite
    a skos:Concept ;
    rdfs:isDefinedBy cs: ;
    skos:broader :igneous-felsic-intrusive ;
    skos:definition "A quartz alkali feldspar syenite with a grain size of less than 3 mm. Includes porphyritic varieties."@en ;
    skos:historyNote "Based on the IUGS classification of igneous rocks (Le Maitre et al., 2005) and GSWA usage." ;
    skos:inScheme cs: ;
    skos:notation "gqa"^^:gswa-rock-code ;
    skos:prefLabel "micro quartz alkali feldspar syenite"@en ;
.

:micro-quartz-anorthosite
    a skos:Concept ;
    rdfs:isDefinedBy cs: ;
    skos:broader :igneous-felsic-intrusive ;
    skos:definition "A quartz anorthosite with a grain size of less than 3 mm. Includes porphyritic varieties."@en ;
    skos:historyNote "Based on the IUGS classification of igneous rocks (Le Maitre et al., 2005) and GSWA usage." ;
    skos:inScheme cs: ;
    skos:notation "goa"^^:gswa-rock-code ;
    skos:prefLabel "micro quartz anorthosite"@en ;
.

:micro-quartz-diorite
    a skos:Concept ;
    rdfs:isDefinedBy cs: ;
    skos:broader :igneous-felsic-intrusive ;
    skos:definition "A quartz diorite with a grain size of less than 3 mm. Includes porphyritic varieties."@en ;
    skos:historyNote "Based on the IUGS classification of igneous rocks (Le Maitre et al., 2005) and GSWA usage." ;
    skos:inScheme cs: ;
    skos:notation "gda"^^:gswa-rock-code ;
    skos:prefLabel "micro quartz diorite"@en ;
.

:micro-quartz-gabbro
    a skos:Concept ;
    rdfs:isDefinedBy cs: ;
    skos:broader :igneous-felsic-intrusive ;
    skos:definition "A quartz gabbro with a grain size of less than 3 mm. Includes porphyritic varieties."@en ;
    skos:historyNote "Based on the IUGS classification of igneous rocks (Le Maitre et al., 2005) and GSWA usage." ;
    skos:inScheme cs: ;
    skos:notation "gua"^^:gswa-rock-code ;
    skos:prefLabel "micro quartz gabbro"@en ;
.

:micro-quartz-monzodiorite
    a skos:Concept ;
    rdfs:isDefinedBy cs: ;
    skos:broader :igneous-felsic-intrusive ;
    skos:definition "A quartz monzodiorite with a grain size of less than 3 mm. Includes porphyritic varieties."@en ;
    skos:historyNote "Based on the IUGS classification of igneous rocks (Le Maitre et al., 2005) and GSWA usage." ;
    skos:inScheme cs: ;
    skos:notation "gka"^^:gswa-rock-code ;
    skos:prefLabel "micro quartz monzodiorite"@en ;
.

:micro-quartz-monzogabbro
    a skos:Concept ;
    rdfs:isDefinedBy cs: ;
    skos:broader :igneous-felsic-intrusive ;
    skos:definition "A quartz monzogabbro with a grain size of less than 3 mm. Includes porphyritic varieties."@en ;
    skos:historyNote "Based on the IUGS classification of igneous rocks (Le Maitre et al., 2005) and GSWA usage." ;
    skos:inScheme cs: ;
    skos:notation "gla"^^:gswa-rock-code ;
    skos:prefLabel "micro quartz monzogabbro"@en ;
.

:micro-quartz-monzonite
    a skos:Concept ;
    rdfs:isDefinedBy cs: ;
    skos:broader :igneous-felsic-intrusive ;
    skos:definition "A quartz monzonite with a grain size of less than 3 mm. Includes porphyritic varieties."@en ;
    skos:historyNote "Based on the IUGS classification of igneous rocks (Le Maitre et al., 2005) and GSWA usage." ;
    skos:inScheme cs: ;
    skos:notation "gca"^^:gswa-rock-code ;
    skos:prefLabel "micro quartz monzonite"@en ;
.

:micro-quartz-syenite
    a skos:Concept ;
    rdfs:isDefinedBy cs: ;
    skos:broader :igneous-felsic-intrusive ;
    skos:definition "A quartz syenite with a grain size of less than 3 mm. Includes porphyritic varieties."@en ;
    skos:historyNote "Based on the IUGS classification of igneous rocks (Le Maitre et al., 2005) and GSWA usage." ;
    skos:inScheme cs: ;
    skos:notation "gea"^^:gswa-rock-code ;
    skos:prefLabel "micro quartz syenite"@en ;
.

:microbialitic-dolomite
    a skos:Concept ;
    rdfs:isDefinedBy cs: ;
    skos:broader :dolomite ;
    skos:definition "A dolomitic rock distinguished by the presence of microbialites, i.e. 'organosedimentary deposits that have accreted as a result of a benthic microbial community trapping and binding detrital sediment and/or forming the locus of mineral precipitation' (Burne and Moore, 1987, p. 241–242). Note that past workers (including GSWA) commonly used the term ‘stromatolite’ to refer to all types of microbialite structures, whereas current usage restricts ‘stromatolite’ to those microbialites with a layered/laminated fabric (see Grey and Awramik 2020, p. 4); therefore, legacy usage of ‘stromatolitic dolomite’ or ‘stromatolitic dolostone’ is best considered equivalent to this lithology."@en ;
    skos:historyNote """Burne, RV and Moore, LS 1987, Microbialites: Organosedimentary deposits of benthic microbial communities: Palaios, v. 2, p. 241–245.,
Grey, K and Awramik, SM 2020, Handbook for the study and description of microbialites: Geological Survey of Western Australia, Bulletin 147, 278p.""" ;
    skos:inScheme cs: ;
    skos:notation "kds"^^:gswa-rock-code ;
    skos:prefLabel "microbialitic dolomite"@en ;
    schema:citation "https://glossary.americangeosciences.org/term/stromatolite"^^xsd:anyURI ;
.

:microbialitic-limestone
    a skos:Concept ;
    rdfs:isDefinedBy cs: ;
    skos:broader :limestone ;
    skos:definition "A limestone distinguished by the presence of microbialites, i.e. 'organosedimentary deposits that have accreted as a result of a benthic microbial community trapping and binding detrital sediment and/or forming the locus of mineral precipitation' (Burne and Moore, 1987, p. 241–242). Note that past workers (including GSWA) commonly used the term ‘stromatolite’ to refer to all types of microbialite structures, whereas current usage restricts ‘stromatolite’ to those microbialites with a layered/laminated fabric (see Grey and Awramik 2020, p. 4); therefore, legacy usage of ‘stromatolitic limestone’ is best considered equivalent to this lithology."@en ;
    skos:historyNote """Burne, RV and Moore, LS 1987, Microbialites: Organosedimentary deposits of benthic microbial communities: Palaios, v. 2, p. 241–245.,
Grey, K and Awramik, SM 2020, Handbook for the study and description of microbialites: Geological Survey of Western Australia, Bulletin 147, 278p.""" ;
    skos:inScheme cs: ;
    skos:notation "kls"^^:gswa-rock-code ;
    skos:prefLabel "microbialitic limestone"@en ;
    schema:citation "https://glossary.americangeosciences.org/term/stromatolite"^^xsd:anyURI ;
.

:microbially-laminated-dolomite
    a skos:Concept ;
    rdfs:isDefinedBy cs: ;
    skos:broader :dolomite ;
    skos:definition "Laminated dolomite rock where the laminae have formed by the trapping of grains and precipitation of dolomite mud through the effects of eubacteria, cyanobacteria, and/or fungi in a microbial mat. Adapted from Glossary of geology (5th edition revised; Neuendorf et al., 2011)."@en ;
    skos:historyNote "Grey, K and Awramik, SM 2020, Handbook for the study and description of microbialites: Geological Survey of Western Australia, Bulletin 147, 278p." ;
    skos:inScheme cs: ;
    skos:notation "kdm"^^:gswa-rock-code ;
    skos:prefLabel "microbially laminated dolomite"@en ;
    schema:citation "https://glossary.americangeosciences.org/term/microbiallaminite"^^xsd:anyURI ;
.

:microbially-laminated-limestone
    a skos:Concept ;
    rdfs:isDefinedBy cs: ;
    skos:broader :limestone ;
    skos:definition "Laminated limestone where the laminae have formed by the trapping of grains and precipitation of calcite mud through the effects of eubacteria, cyanobacteria, and/or fungi in a microbial mat. Adapted from Glossary of geology (5th edition revised; Neuendorf et al., 2011)."@en ;
    skos:historyNote "Based on the Glossary of geology (5th edition, revised; Neuendorf et al. 2011)." ;
    skos:inScheme cs: ;
    skos:notation "klm"^^:gswa-rock-code ;
    skos:prefLabel "microbially laminated limestone"@en ;
    schema:citation "https://glossary.americangeosciences.org/term/microbiallaminite"^^xsd:anyURI ;
.

:microdiorite
    a skos:Concept ;
    rdfs:isDefinedBy cs: ;
    skos:broader :igneous-felsic-intrusive ;
    skos:definition "A diorite with a grain size of less than 3 mm. Includes porphyritic varieties."@en ;
    skos:historyNote "Based on the IUGS classification of igneous rocks (Le Maitre et al., 2005) and GSWA usage." ;
    skos:inScheme cs: ;
    skos:notation "gia"^^:gswa-rock-code ;
    skos:prefLabel "microdiorite"@en ;
.

:microgranodiorite
    a skos:Concept ;
    rdfs:isDefinedBy cs: ;
    skos:broader :igneous-felsic-intrusive ;
    skos:definition "A granodiorite with a grain size of less than 3 mm. Includes porphyritic varieties."@en ;
    skos:historyNote "Based on the IUGS classification of igneous rocks (Le Maitre et al., 2005) and GSWA usage." ;
    skos:inScheme cs: ;
    skos:notation "gga"^^:gswa-rock-code ;
    skos:prefLabel "microgranodiorite"@en ;
.

:micromonzodiorite
    a skos:Concept ;
    rdfs:isDefinedBy cs: ;
    skos:broader :igneous-felsic-intrusive ;
    skos:definition "A monzodiorite with a grain size of less than 3 mm. Includes porphyritic varieties."@en ;
    skos:historyNote "Based on the IUGS classification of igneous rocks (Le Maitre et al., 2005) and GSWA usage." ;
    skos:inScheme cs: ;
    skos:notation "gha"^^:gswa-rock-code ;
    skos:prefLabel "micromonzodiorite"@en ;
.

:micromonzogabbro
    a skos:Concept ;
    rdfs:isDefinedBy cs: ;
    skos:broader :igneous-felsic-intrusive ;
    skos:definition "A monzogabbro with a grain size of less than 3 mm. Includes porphyritic varieties."@en ;
    skos:historyNote "Based on the IUGS classification of igneous rocks (Le Maitre et al., 2005) and GSWA usage." ;
    skos:inScheme cs: ;
    skos:notation "gwa"^^:gswa-rock-code ;
    skos:prefLabel "micromonzogabbro"@en ;
.

:micromonzogranite
    a skos:Concept ;
    rdfs:isDefinedBy cs: ;
    skos:broader :igneous-felsic-intrusive ;
    skos:definition "A monzogranite with a grain size of less than 3 mm. Includes porphyritic varieties."@en ;
    skos:historyNote "Based on the IUGS classification of igneous rocks (Le Maitre et al., 2005) and GSWA usage." ;
    skos:inScheme cs: ;
    skos:notation "gma"^^:gswa-rock-code ;
    skos:prefLabel "micromonzogranite"@en ;
.

:micromonzonite
    a skos:Concept ;
    rdfs:isDefinedBy cs: ;
    skos:broader :igneous-felsic-intrusive ;
    skos:definition "A monzonite with a grain size of less than 3 mm. Includes porphyritic varieties."@en ;
    skos:historyNote "Based on the IUGS classification of igneous rocks (Le Maitre et al., 2005) and GSWA usage." ;
    skos:inScheme cs: ;
    skos:notation "gza"^^:gswa-rock-code ;
    skos:prefLabel "micromonzonite"@en ;
.

:microsyenite
    a skos:Concept ;
    rdfs:isDefinedBy cs: ;
    skos:broader :igneous-felsic-intrusive ;
    skos:definition "A syenite with a grain size of less than 3 mm. Includes porphyritic varieties."@en ;
    skos:historyNote "Based on the IUGS classification of igneous rocks (Le Maitre et al., 2005) and GSWA usage." ;
    skos:inScheme cs: ;
    skos:notation "gya"^^:gswa-rock-code ;
    skos:prefLabel "microsyenite"@en ;
.

:microsyenogranite
    a skos:Concept ;
    rdfs:isDefinedBy cs: ;
    skos:broader :igneous-felsic-intrusive ;
    skos:definition "A syenogranite with a grain size of less than 3 mm. Includes porphyritic varieties."@en ;
    skos:historyNote "Based on the IUGS classification of igneous rocks (Le Maitre et al., 2005) and GSWA usage." ;
    skos:inScheme cs: ;
    skos:notation "gra"^^:gswa-rock-code ;
    skos:prefLabel "microsyenogranite"@en ;
.

:microtonalite
    a skos:Concept ;
    rdfs:isDefinedBy cs: ;
    skos:broader :igneous-felsic-intrusive ;
    skos:definition "A tonalite with a grain size of less than 3 mm. Includes porphyritic varieties."@en ;
    skos:historyNote "Based on the IUGS classification of igneous rocks (Le Maitre et al., 2005) and GSWA usage." ;
    skos:inScheme cs: ;
    skos:notation "gta"^^:gswa-rock-code ;
    skos:prefLabel "microtonalite"@en ;
.

:microtrondhjemite
    a skos:Concept ;
    rdfs:isDefinedBy cs: ;
    skos:broader :igneous-felsic-intrusive ;
    skos:definition "A trondhjemite with a grain size of less than 3 mm. Includes porphyritic varieties."@en ;
    skos:historyNote "Based on the IUGS classification of igneous rocks (Le Maitre et al., 2005) and GSWA usage." ;
    skos:inScheme cs: ;
    skos:notation "gja"^^:gswa-rock-code ;
    skos:prefLabel "microtrondhjemite"@en ;
.

:migmatitic-fault-rock
    a skos:Concept ;
    rdfs:isDefinedBy cs: ;
    skos:broader :metamorphic-protolith-unknown-fault-rock ;
    skos:definition "A fault that developed in a migmatite, under migmatitic conditions. In GSWA usage, this term is reserved for fault rocks for which a protolith cannot be conclusively established."@en ;
    skos:historyNote "Compiled by the Geological Survey of Western Australia" ;
    skos:inScheme cs: ;
    skos:notation "myi"^^:gswa-rock-code ;
    skos:prefLabel "migmatitic fault rock"@en ;
.

:migmatitic-gneiss
    a skos:Concept ;
    rdfs:isDefinedBy cs: ;
    skos:broader :metamorphic-protolith-unknown-gneiss ;
    skos:definition "A metamorphic rock of uncertain protolith and characterized by the presence of both a gneissose structure and migmatitic components. The gneissic part retains a well-developed foliation, whereas the migmatite component includes bands or veins of leucosome within the granofelsic matrix. Adapted from https://geologyscience.com/rocks/metamorphic-rocks/foliated-metamorphic-rocks/migmatite/."@en ;
    skos:historyNote "Compiled by the Geological Survey of Western Australia" ;
    skos:inScheme cs: ;
    skos:notation "mni"^^:gswa-rock-code ;
    skos:prefLabel "migmatitic gneiss"@en ;
    schema:citation
        "https://geologyscience.com/rocks/metamorphic-rocks/foliated-metamorphic-rocks/migmatite/"^^xsd:anyURI ,
        "https://glossary.americangeosciences.org/term/gneiss"^^xsd:anyURI ;
.

:migmatitic-granofels-hornfels
    a skos:Concept ;
    rdfs:isDefinedBy cs: ;
    skos:broader :metamorphic-protolith-unknown-granofels-hornfels ;
    skos:definition "A metamorphic rock of uncertain protolith and characterized by the presence of both a granofelsic structure and migmatitic components. The granofelsic part retains a well-developed foliation, whereas the migmatite component includes bands or veins of leucosome within the granofelsic matrix. Adapted from https://geologyscience.com/rocks/metamorphic-rocks/foliated-metamorphic-rocks/migmatite/."@en ;
    skos:historyNote "Compiled by the Geological Survey of Western Australia" ;
    skos:inScheme cs: ;
    skos:notation "mei"^^:gswa-rock-code ;
    skos:prefLabel "migmatitic granofels/hornfels"@en ;
    schema:citation "https://geologyscience.com/rocks/metamorphic-rocks/foliated-metamorphic-rocks/migmatite/"^^xsd:anyURI ;
.

:migmatitic-metacarbonatite
    a skos:Concept ;
    rdfs:isDefinedBy cs: ;
    skos:broader :meta-igneous-carbonatite ;
    skos:definition "Composite metamorphic rock derived from an igneous protolith containing a modal amount of primary carbonate minerals greater than 50% and pervasively heterogeneous on a meso- to megascopic scale. It typically consists of darker (melanosome) and lighter (leucosome) parts. The darker parts usually exhibit features of metamorphic rocks, whereas the lighter parts are of igneous appearance. See definition of migmatite in Fettes and Desmond (2007, p. 176)."@en ;
    skos:inScheme cs: ;
    skos:notation "mqi"^^:gswa-rock-code ;
    skos:prefLabel "migmatitic metacarbonatite"@en ;
.

:migmatitic-schist
    a skos:Concept ;
    rdfs:isDefinedBy cs: ;
    skos:broader :metamorphic-protolith-unknown-schist ;
    skos:definition "A metamorphic rock of uncertain protolith and characterized by the presence of both a schistose structure and migmatite portions. The schistose part exhibits a foliated texture, whereas the leucosome forms veins or layers within the schist. Adapted from https://geologyscience.com/rocks/metamorphic-rocks/foliated-metamorphic-rocks/migmatite/."@en ;
    skos:historyNote "Compiled by the Geological Survey of Western Australia" ;
    skos:inScheme cs: ;
    skos:notation "msi"^^:gswa-rock-code ;
    skos:prefLabel "migmatitic schist"@en ;
    schema:citation "https://geologyscience.com/rocks/metamorphic-rocks/foliated-metamorphic-rocks/migmatite/"^^xsd:anyURI ;
.

:minette
    a skos:Concept ;
    rdfs:isDefinedBy cs: ;
    skos:broader :igneous-lamprophyres ;
    skos:definition "Originally an old miners’ term for oolitic ironstones. Later used for a variety of lamprophyre consisting of phenocrysts of phlogopite–biotite and occasionally amphiboles in a groundmass of the same minerals plus orthoclase and minor plagioclase. Mg-olivine and diopsidic pyroxene may also be present. Now defined in the lamprophyre classification (Table 2.9, p. 19). (Le Maitre et al., 2005, p. 112)"@en ;
    skos:historyNote "Based on the IUGS classification of igneous rocks (Le Maitre et al., 2005)." ;
    skos:inScheme cs: ;
    skos:notation "ym"^^:gswa-rock-code ;
    skos:prefLabel "minette"@en ;
.

:mixed-carbonate-evaporite
    a skos:Concept ;
    rdfs:isDefinedBy cs: ;
    skos:broader :sedimentary-carbonate ;
    skos:definition "Carbonate and evaporite layers/beds interleaved at outcrop scale."@en ;
    skos:historyNote "Compiled by the Geological Survey of Western Australia" ;
    skos:inScheme cs: ;
    skos:notation "kv"^^:gswa-rock-code ;
    skos:prefLabel "mixed carbonate/evaporite"@en ;
.

:mixed-chert-and-iron-formation
    a skos:Concept ;
    rdfs:isDefinedBy cs: ;
    skos:broader :sedimentary-other-chemical-or-biochemical ;
    skos:definition "Iron formation and chert interleaved at meso- to megascopic scale."@en ;
    skos:historyNote "Compiled by the Geological Survey of Western Australia" ;
    skos:inScheme cs: ;
    skos:notation "cx"^^:gswa-rock-code ;
    skos:prefLabel "mixed chert and iron formation"@en ;
.

:mixed-chert-and-mudstone
    a skos:Concept ;
    rdfs:isDefinedBy cs: ;
    skos:broader :sedimentary-other-chemical-or-biochemical ;
    skos:definition "Chert and mudstone layers/beds interleaved at outcrop scale."@en ;
    skos:historyNote "Compiled by the Geological Survey of Western Australia" ;
    skos:inScheme cs: ;
    skos:notation "cl"^^:gswa-rock-code ;
    skos:prefLabel "mixed chert and mudstone"@en ;
.

:mixed-iron-formation-and-mudstone
    a skos:Concept ;
    rdfs:isDefinedBy cs: ;
    skos:broader :sedimentary-other-chemical-or-biochemical ;
    skos:definition "Iron formation and mudstone interleaved at outcrop scale."@en ;
    skos:historyNote "Compiled by the Geological Survey of Western Australia" ;
    skos:inScheme cs: ;
    skos:notation "ca"^^:gswa-rock-code ;
    skos:prefLabel "mixed iron formation and mudstone"@en ;
.

:mixed-limestone-dolomite
    a skos:Concept ;
    rdfs:isDefinedBy cs: ;
    skos:broader :sedimentary-carbonate ;
    skos:definition "Limestone and dolomite beds/layers/rocks interleaved at outcrop scale."@en ;
    skos:historyNote "Compiled by the Geological Survey of Western Australia" ;
    skos:inScheme cs: ;
    skos:notation "kx"^^:gswa-rock-code ;
    skos:prefLabel "mixed limestone and dolomite"@en ;
.

:mixed-lithology
    a skos:Concept ;
    rdfs:isDefinedBy cs: ;
    skos:broader :mixed ;
    skos:definition "A prefix used in GSWA's Explanatory Notes system (ENS) to characterize interleaved lithologies that cannot be separated at the scale of mapping, with the first code representing the volumetrically most abundant lithology. Typically reserved for (a) lithologies that are tectonically interleaved, and (b) intrusive lithologies and their host. Interlayered lithologies in sedimentary successions are covered under sedimentary rock types, and the prefix 'j' is used specifically to describe lithologies hosting xenolith/inclusion."@en ;
    skos:historyNote "Compiled by the Geological Survey of Western Australia" ;
    skos:inScheme cs: ;
    skos:notation "x"^^:gswa-rock-code ;
    skos:prefLabel "mixed lithology"@en ;
.

:mixed-siliciclastic-and-volcanic-rocks
    a skos:Concept ;
    rdfs:isDefinedBy cs: ;
    skos:broader :sedimentary-siliciclastic ;
    skos:definition "Siliciclastic rocks/beds/intervals and volcanic rocks/beds/intervals interleaved at outcrop scale."@en ;
    skos:historyNote "Compiled by the Geological Survey of Western Australia" ;
    skos:inScheme cs: ;
    skos:notation "sv"^^:gswa-rock-code ;
    skos:prefLabel "mixed siliciclastic and volcanic rocks"@en ;
.

:monchiquite
    a skos:Concept ;
    rdfs:isDefinedBy cs: ;
    skos:broader :igneous-lamprophyres ;
    skos:definition "A variety of lamprophyre similar to camptonite except that the groundmass is feldspar-free and composed of combinations of glass and feldspathoids, especially analcime. Now defined in the lamprophyre classification (Table 2.9, p. 19). (Le Maitre et al., 2005, p. 113)"@en ;
    skos:historyNote "Based on the IUGS classification of igneous rocks (Le Maitre et al., 2005)." ;
    skos:inScheme cs: ;
    skos:notation "yq"^^:gswa-rock-code ;
    skos:prefLabel "monchiquite"@en ;
.

:monomictic-impact-breccia
    a skos:Concept ;
    rdfs:isDefinedBy cs: ;
    skos:broader :impact-breccia ;
    skos:definition "Cataclasite produced by impact and displaying weak or no shock metamorphism. It occurs in the (par)autochthonous floor of an impact crater or (up to the size of blocks and megablocks) within allochthonous (polymictic) impact breccias (Fettes and Desmons, 2007, p. 177)."@en ;
    skos:historyNote "Based on the IUGS classification of metamorphic rocks (Fettes and Desmons, 2007)." ;
    skos:inScheme cs: ;
    skos:notation "mpm"^^:gswa-rock-code ;
    skos:prefLabel "monomictic impact breccia"@en ;
.

:monzodiorite
    a skos:Concept ;
    rdfs:isDefinedBy cs: ;
    skos:broader :igneous-felsic-intrusive ;
    skos:definition "A term suggested to replace syenodiorite for an intrusive rock intermediate between monzonite and diorite. Now defined modally in QAPF field 9 (Fig. 2.4, p. 22). (cf. Le Maitre et al., 2005, p. 113)"@en ;
    skos:exactMatch
        <http://inspire.ec.europa.eu/codelist/LithologyValue/monzodiorite> ,
        <http://resource.geosciml.org/classifier/cgi/lithology/monzodiorite> ;
    skos:historyNote "Based on the IUGS classification of igneous rocks (Le Maitre et al., 2005)." ;
    skos:inScheme cs: ;
    skos:notation "gh"^^:gswa-rock-code ;
    skos:prefLabel "monzodiorite"@en ;
    schema:citation "https://glossary.americangeosciences.org/term/monzodiorite"^^xsd:anyURI ;
.

:monzogabbro
    a skos:Concept ;
    rdfs:isDefinedBy cs: ;
    skos:broader :igneous-felsic-intrusive ;
    skos:definition "A term suggested to replace syenogabbro for an intrusive rock of gabbroic aspect that contains minor but essential orthoclase as well as calcic plagioclase. Now defined modally in QAPF field 9 (Fig. 2.4, p. 22). (Le Maitre et al., 2005, p. 113)"@en ;
    skos:exactMatch
        <http://inspire.ec.europa.eu/codelist/LithologyValue/monzogabbro> ,
        <http://resource.geosciml.org/classifier/cgi/lithology/monzogabbro> ;
    skos:historyNote "Based on the IUGS classification of igneous rocks (Le Maitre et al., 2005)." ;
    skos:inScheme cs: ;
    skos:notation "gw"^^:gswa-rock-code ;
    skos:prefLabel "monzogabbro"@en ;
    schema:citation "https://glossary.americangeosciences.org/term/monzogabbro"^^xsd:anyURI ;
.

:monzogranite
    a skos:Concept ;
    rdfs:isDefinedBy cs: ;
    skos:broader :igneous-felsic-intrusive ;
    skos:definition "An optional term for a variety of granite in QAPF field 3b (Fig. 2.4, p. 22) having roughly equal amounts of alkali feldspar and plagioclase (Le Maitre et al., 2005, p. 113)"@en ;
    skos:exactMatch
        <http://inspire.ec.europa.eu/codelist/LithologyValue/monzogranite> ,
        <http://resource.geosciml.org/classifier/cgi/lithology/monzogranite> ;
    skos:historyNote "Based on the IUGS classification of igneous rocks (Le Maitre et al., 2005)." ;
    skos:inScheme cs: ;
    skos:notation "gm"^^:gswa-rock-code ;
    skos:prefLabel "monzogranite"@en ;
    schema:citation "https://glossary.americangeosciences.org/term/monzogranite"^^xsd:anyURI ;
.

:monzonite
    a skos:Concept ;
    rdfs:isDefinedBy cs: ;
    skos:broader :igneous-felsic-intrusive ;
    skos:definition "An intrusive rock containing almost equal amounts of plagioclase and alkali feldspar with minor amphibole and/or pyroxene. Now defined modally in QAPF field 8 (Fig. 2.4, p. 22). Adapted from Le Maitre et al. (2005, p. 113)."@en ;
    skos:exactMatch
        <http://inspire.ec.europa.eu/codelist/LithologyValue/monzonite> ,
        <http://resource.geosciml.org/classifier/cgi/lithology/monzonite> ;
    skos:historyNote "Based on the IUGS classification of igneous rocks (Le Maitre et al., 2005)." ;
    skos:inScheme cs: ;
    skos:notation "gz"^^:gswa-rock-code ;
    skos:prefLabel "monzonite"@en ;
    schema:citation "https://glossary.americangeosciences.org/term/monzonite"^^xsd:anyURI ;
.

:mylonite
    a skos:Concept ;
    rdfs:isDefinedBy cs: ;
    skos:altLabel "mesomylonite"@en ;
    skos:broader :metamorphic-protolith-unknown-fault-rock ;
    skos:definition "Fault rock that is cohesive and characterized by a well-developed schistosity resulting from tectonic reduction of grain size for 50–90% of the rock volume, and commonly containing rounded porphyroclasts and lithic fragments of similar composition to minerals in the matrix. Fine-scale layering and an associated mineral or stretching lineation are commonly present. Brittle deformation of some minerals may be present, but deformation is commonly by crystal plasticity. Definition adapted from Fossen (2016) and Fettes and Desmons (2007, p. 177)."@en ;
    skos:historyNote "Fossen, H 2016, Structural geology (2nd edition): Cambridge University Press, Cambridge, United Kingdom, 524p." ;
    skos:inScheme cs: ;
    skos:notation "myy"^^:gswa-rock-code ;
    skos:prefLabel "mylonite"@en ;
    schema:citation "https://glossary.americangeosciences.org/term/mylonite"^^xsd:anyURI ;
.

:mylonitized-hydrothermal-rock
    a skos:Concept ;
    rdfs:isDefinedBy cs: ;
    skos:broader :metamorphosed-hydrothermal ;
    skos:definition "A hydrothermal rock characterized by a well-developed schistosity resulting from tectonic reduction of grain size (cf. definition of mylonite in Fettes and Desmons, 2007, p. 177)."@en ;
    skos:historyNote "Compiled by the Geological Survey of Western Australia" ;
    skos:inScheme cs: ;
    skos:notation "mzy"^^:gswa-rock-code ;
    skos:prefLabel "mylonitized hydrothermal rock"@en ;
    schema:citation
        "https://glossary.americangeosciences.org/term/hydrothermalalteration"^^xsd:anyURI ,
        "https://glossary.americangeosciences.org/term/mylonite"^^xsd:anyURI ;
.

:mylonitized-meta-igneous-felsic-rock
    a skos:Concept ;
    rdfs:isDefinedBy cs: ;
    skos:broader :meta-igneous-felsic ;
    skos:definition "A felsic igneous rock characterized by a well-developed schistosity resulting from tectonic reduction of grain size (cf. definition of mylonite in Fettes and Desmons, 2007, p. 177)."@en ;
    skos:historyNote "Compiled by the Geological Survey of Western Australia" ;
    skos:inScheme cs: ;
    skos:notation "mry"^^:gswa-rock-code ;
    skos:prefLabel "mylonitized meta-igneous felsic rock"@en ;
.

:mylonitized-meta-igneous-mafic-rock
    a skos:Concept ;
    rdfs:isDefinedBy cs: ;
    skos:broader :meta-igneous-mafic ;
    skos:definition "A mafic igneous rock characterized by a well-developed schistosity resulting from tectonic reduction of grain size (cf. definition of mylonite in Fettes and Desmons, 2007, p. 177)."@en ;
    skos:historyNote "Compiled by the Geological Survey of Western Australia" ;
    skos:inScheme cs: ;
    skos:notation "mwy"^^:gswa-rock-code ;
    skos:prefLabel "mylonitized meta-igneous mafic rock"@en ;
.

:mylonitized-meta-iron-formation
    a skos:Concept ;
    rdfs:isDefinedBy cs: ;
    skos:altLabel
        "itabirite"@en ,
        "taconite"@en ;
    skos:broader :metasedimentary-other-chemical-meta-iron-formation ;
    skos:definition "An iron formation characterized by a well-developed schistosity resulting from tectonic reduction of grain size (cf. definition of mylonite in Fettes and Desmons, 2007, p. 177)."@en ;
    skos:historyNote "Based on the IUGS classification of metamorphic rocks (Fettes and Desmons, 2007) and GSWA usage." ;
    skos:inScheme cs: ;
    skos:notation "miy"^^:gswa-rock-code ;
    skos:prefLabel "mylonitized meta-iron formation"@en ;
.

:mylonitized-meta-ultramafic-intrusive-rock
    a skos:Concept ;
    rdfs:isDefinedBy cs: ;
    skos:broader :meta-igneous-ultramafic-intrusive ;
    skos:definition "An ultramafic igneous (intrusive or coarse-grained extrusive) rock characterized by a well-developed schistosity resulting from tectonic reduction of grain size (cf. definition of mylonite in Fettes and Desmons, 2007, p. 177)."@en ;
    skos:historyNote "Compiled by the Geological Survey of Western Australia" ;
    skos:inScheme cs: ;
    skos:notation "may"^^:gswa-rock-code ;
    skos:prefLabel "mylonitized meta-ultramafic intrusive rock"@en ;
.

:mylonitized-meta-ultramafic-rock-volcanic-or-undivided
    a skos:Concept ;
    rdfs:isDefinedBy cs: ;
    skos:broader :meta-igneous-ultramafic-volcanic ;
    skos:definition "An ultramafic volcanic or volcaniclastic rock characterized by a well-developed schistosity resulting from tectonic reduction of grain size (cf. definition of mylonite in Fettes and Desmons, 2007, p. 177)."@en ;
    skos:historyNote "Compiled by the Geological Survey of Western Australia" ;
    skos:inScheme cs: ;
    skos:notation "muy"^^:gswa-rock-code ;
    skos:prefLabel "mylonitized meta-ultramafic rock; volcanic or undivided"@en ;
.

:mylonitized-metacarbonate-rock
    a skos:Concept ;
    rdfs:isDefinedBy cs: ;
    skos:broader :metasedimentary-carbonate ;
    skos:definition "A carbonate-rich rock characterized by a well-developed schistosity resulting from tectonic reduction of grain size (cf. definition of mylonite in Fettes and Desmons, 2007, p. 177)."@en ;
    skos:historyNote "Compiled by the Geological Survey of Western Australia" ;
    skos:inScheme cs: ;
    skos:notation "mky"^^:gswa-rock-code ;
    skos:prefLabel "mylonitized metacarbonate rock"@en ;
.

:mylonitized-metacarbonatite
    a skos:Concept ;
    rdfs:isDefinedBy cs: ;
    skos:broader :meta-igneous-carbonatite ;
    skos:definition "A carbonatite characterized by a well-developed schistosity resulting from tectonic reduction of grain size (cf. definition of mylonite in Fettes and Desmons, 2007, p. 177)"@en ;
    skos:inScheme cs: ;
    skos:notation "mqy"^^:gswa-rock-code ;
    skos:prefLabel "mylonitized metacarbonatite"@en ;
.

:mylonitized-metachert
    a skos:Concept ;
    rdfs:isDefinedBy cs: ;
    skos:broader :metasedimentary-other-chemical ;
    skos:definition "A chert rock characterized by a well-developed schistosity resulting from tectonic reduction of grain size (cf. definition of mylonite in Fettes and Desmons, 2007, p. 177)."@en ;
    skos:historyNote "Compiled by the Geological Survey of Western Australia" ;
    skos:inScheme cs: ;
    skos:notation "mcy"^^:gswa-rock-code ;
    skos:prefLabel "mylonitized metachert"@en ;
.

:mylonitized-metaconglomerate
    a skos:Concept ;
    rdfs:isDefinedBy cs: ;
    skos:broader :metasedimentary-siliciclastic-psephite ;
    skos:definition "A siliciclastic rock originally consisting of particles greater than sand size (i.e. a conglomerate) that is characterized by a well-developed schistosity resulting from tectonic reduction of grain size (cf. definition of mylonite in Fettes and Desmons, 2007, p. 177)."@en ;
    skos:historyNote "Compiled by the Geological Survey of Western Australia" ;
    skos:inScheme cs: ;
    skos:notation "mxy"^^:gswa-rock-code ;
    skos:prefLabel "mylonitized metaconglomerate"@en ;
    schema:citation "https://glossary.americangeosciences.org/term/psephite"^^xsd:anyURI ;
.

:mylonitized-metafelsic-volcanic-rock
    a skos:Concept ;
    rdfs:isDefinedBy cs: ;
    skos:broader :meta-igneous-felsic-volcanic ;
    skos:definition "A felsic volcanic rock characterized by a well-developed schistosity resulting from tectonic reduction of grain size (cf. definition of mylonite in Fettes and Desmons, 2007, p. 177). GSWA's rock classification scheme prefers the use of volcanic terminology for any igneous rock formed on or near the Earth's surface, i.e. for those hypabyssal or subvolcanic rocks such as dykes, sills, and cryptodomes that are demonstrably both spatially and temporally associated with extrusive volcanic rocks."@en ;
    skos:historyNote "Compiled by the Geological Survey of Western Australia" ;
    skos:inScheme cs: ;
    skos:notation "mfy"^^:gswa-rock-code ;
    skos:prefLabel "mylonitized metafelsic volcanic rock"@en ;
.

:mylonitized-metagranitic-rock
    a skos:Concept ;
    rdfs:isDefinedBy cs: ;
    skos:broader :meta-igneous-felsic-intrusive ;
    skos:definition "A felsic intrusive rock characterized by a well-developed schistosity resulting from tectonic reduction of grain size (cf. definition of mylonite in Fettes and Desmons, 2007, p. 177)."@en ;
    skos:historyNote "Compiled by the Geological Survey of Western Australia" ;
    skos:inScheme cs: ;
    skos:notation "mgy"^^:gswa-rock-code ;
    skos:prefLabel "mylonitized metagranitic rock"@en ;
.

:mylonitized-metamafic-intrusive-rock
    a skos:Concept ;
    rdfs:isDefinedBy cs: ;
    skos:broader :meta-igneous-mafic-intrusive ;
    skos:definition "A mafic intrusive rock (or coarse-grained parts of extrusive successions) characterized by a well-developed schistosity resulting from tectonic reduction of grain size (cf. definition of mylonite in Fettes and Desmons, 2007, p. 177)."@en ;
    skos:historyNote "Compiled by the Geological Survey of Western Australia" ;
    skos:inScheme cs: ;
    skos:notation "moy"^^:gswa-rock-code ;
    skos:prefLabel "mylonitized metamafic intrusive rock"@en ;
.

:mylonitized-metamafic-volcanic-rock
    a skos:Concept ;
    rdfs:isDefinedBy cs: ;
    skos:broader :meta-igneous-mafic-volcanic ;
    skos:definition "A mafic volcanic rock characterized by a well-developed schistosity resulting from tectonic reduction of grain size (cf. definition of mylonite in Fettes and Desmons, 2007, p. 177). GSWA's rock classification scheme prefers the use of volcanic terminology for any igneous rock formed on or near the Earth's surface, i.e. for those hypabyssal or subvolcanic rocks such as dykes, sills, and cryptodomes that are demonstrably both spatially and temporally associated with extrusive volcanic rocks."@en ;
    skos:historyNote "Compiled by the Geological Survey of Western Australia" ;
    skos:inScheme cs: ;
    skos:notation "mby"^^:gswa-rock-code ;
    skos:prefLabel "mylonitized metamafic volcanic rock"@en ;
.

:mylonitized-metasandstone
    a skos:Concept ;
    rdfs:isDefinedBy cs: ;
    skos:broader :metasedimentary-siliciclastic-psammite ;
    skos:definition "A siliciclastic rock originally consisting of sand-sized particles that is characterized by a well-developed schistosity resulting from tectonic reduction of grain size (cf. definition of mylonite in Fettes and Desmons, 2007, p. 177)."@en ;
    skos:historyNote "Compiled by the Geological Survey of Western Australia" ;
    skos:inScheme cs: ;
    skos:notation "mty"^^:gswa-rock-code ;
    skos:prefLabel "mylonitized metasandstone"@en ;
    schema:citation "https://glossary.americangeosciences.org/term/psammite"^^xsd:anyURI ;
.

:mylonitized-metasiliciclastic-rock
    a skos:Concept ;
    rdfs:isDefinedBy cs: ;
    skos:broader :metasedimentary-siliciclastic ;
    skos:definition "A siliciclastic rock characterized by a well-developed schistosity resulting from tectonic reduction of grain size (cf. definition of mylonite in Fettes and Desmons, 2007, p. 177)."@en ;
    skos:historyNote "Compiled by the Geological Survey of Western Australia" ;
    skos:inScheme cs: ;
    skos:notation "mdy"^^:gswa-rock-code ;
    skos:prefLabel "mylonitized metasiliciclastic rock"@en ;
.

:mylonitized-metasomatic-rock
    a skos:Concept ;
    rdfs:isDefinedBy cs: ;
    skos:broader :metasomatic ;
    skos:definition "A metasomatic rock that has experienced deformation by extreme microbrecciation."@en ;
    skos:historyNote "Compiled by the Geological Survey of Western Australia" ;
    skos:inScheme cs: ;
    skos:notation "mjy"^^:gswa-rock-code ;
    skos:prefLabel "mylonitized metasomatic rock"@en ;
    schema:citation
        "https://glossary.americangeosciences.org/term/metasomaticrock"^^xsd:anyURI ,
        "https://glossary.americangeosciences.org/term/mylonite"^^xsd:anyURI ;
.

:mylonitized-metavolcanic-or-metavolcaniclastic-rock
    a skos:Concept ;
    rdfs:isDefinedBy cs: ;
    skos:broader :meta-igneous-volcanic-or-volcaniclastic ;
    skos:definition "A metamorphosed volcanic or volcaniclastic rock otherwise uncategorized that is characterized by a well-developed schistosity resulting from tectonic reduction of grain size (cf. definition of mylonite in Fettes and Desmons, 2007, p. 177)."@en ;
    skos:historyNote "Compiled by the Geological Survey of Western Australia" ;
    skos:inScheme cs: ;
    skos:notation "mvy"^^:gswa-rock-code ;
    skos:prefLabel "mylonitized metavolcanic or metavolcaniclastic rock"@en ;
.

:mylonitized-pelite
    a skos:Concept ;
    rdfs:isDefinedBy cs: ;
    skos:broader :metasedimentary-siliciclastic-pelite ;
    skos:definition "A fine-grained siliciclastic rock characterized by a well-developed schistosity resulting from tectonic reduction of grain size (cf. definition of mylonite in Fettes and Desmons, 2007, p. 177)."@en ;
    skos:historyNote "Compiled by the Geological Survey of Western Australia" ;
    skos:inScheme cs: ;
    skos:notation "mly"^^:gswa-rock-code ;
    skos:prefLabel "mylonitized pelite"@en ;
    schema:citation "https://glossary.americangeosciences.org/term/pelite"^^xsd:anyURI ;
.

:mylonitized-psammite-and-pelite
    a skos:Concept ;
    rdfs:isDefinedBy cs: ;
    skos:broader :metasedimentary-siliciclastic-psammite-and-pelite-interlayered ;
    skos:definition "A metamorphosed sequence of rocks originally consisting of interleaved sandstone and mudstone beds that is characterized by a well-developed schistosity resulting from tectonic reduction of grain size (cf. definition of mylonite in Fettes and Desmons, 2007, p. 177)."@en ;
    skos:historyNote "Compiled by the Geological Survey of Western Australia" ;
    skos:inScheme cs: ;
    skos:notation "mhy"^^:gswa-rock-code ;
    skos:prefLabel "mylonitized psammite and pelite"@en ;
    schema:citation
        "https://glossary.americangeosciences.org/term/pelite"^^xsd:anyURI ,
        "https://glossary.americangeosciences.org/term/psammite"^^xsd:anyURI ;
.

:mylonitized-semipelite
    a skos:Concept ;
    rdfs:isDefinedBy cs: ;
    skos:broader :metasedimentary-siliciclastic-semipelite ;
    skos:definition "A fine-grained siliciclastic rock characterized by a well-developed schistosity resulting from tectonic reduction of grain size (cf. definition of mylonite in Fettes and Desmons, 2007, p. 177), and with a modal ratio of mica to quartz + feldspar intermediate between a pelite and a psammite."@en ;
    skos:historyNote "Compiled by the Geological Survey of Western Australia" ;
    skos:inScheme cs: ;
    skos:notation "mmy"^^:gswa-rock-code ;
    skos:prefLabel "mylonitized semipelite"@en ;
.

:norite
    a skos:Concept ;
    rdfs:isDefinedBy cs: ;
    skos:broader :igneous-mafic-intrusive ;
    skos:definition "An intrusive rock composed essentially of bytownite, labradorite or andesine and orthopyroxene. Now defined modally in the gabbroic rock classification (Fig. 2.6, p. 25). (Le Maitre et al., 2005, p. 117)"@en ;
    skos:historyNote "Based on the IUGS classification of igneous rocks (Le Maitre et al., 2005)." ;
    skos:inScheme cs: ;
    skos:notation "ow"^^:gswa-rock-code ;
    skos:prefLabel "norite"@en ;
    schema:citation "https://glossary.americangeosciences.org/term/norite"^^xsd:anyURI ;
.

:olivine-clinopyroxene-norite
    a skos:Concept ;
    rdfs:isDefinedBy cs: ;
    skos:broader :igneous-mafic-intrusive ;
    skos:definition "An intrusive rock defined modally in the gabbroic rock classification (Fig. 2.6, p. 25) as a variety of norite in which olivine is between 5% and 85% and clinopyroxene exceeds 5% of the pyroxenes. (cf. Le Maitre et al., 2005, p. 120)"@en ;
    skos:historyNote "Based on the IUGS classification of igneous rocks (Le Maitre et al., 2005)." ;
    skos:inScheme cs: ;
    skos:notation "ov"^^:gswa-rock-code ;
    skos:prefLabel "olivine-clinopyroxene norite"@en ;
.

:olivine-clinopyroxenite
    a skos:Concept ;
    rdfs:isDefinedBy cs: ;
    skos:broader :igneous-ultramafic-intrusive ;
    skos:definition "An ultramafic intrusive rock consisting essentially of clinopyroxene and 10–40% olivine. Now defined modally in the ultramafic rock classification (Fig. 2.9, p. 28). Adapted from Le Maitre et al. (2005, p. 119)."@en ;
    skos:historyNote "Based on the IUGS classification of igneous rocks (Le Maitre et al., 2005)." ;
    skos:inScheme cs: ;
    skos:notation "aoc"^^:gswa-rock-code ;
    skos:prefLabel "olivine clinopyroxenite"@en ;
    schema:citation "https://glossary.americangeosciences.org/term/olivineclinopyroxenite"^^xsd:anyURI ;
.

:olivine-diopside-richterite-madupitic-lamproite
    a skos:Concept ;
    rdfs:isDefinedBy cs: ;
    skos:altLabel "olivine-diopside-richterite-phlogopite lamproite"@en ;
    skos:broader :igneous-lamproites ;
    skos:definition "Originally described as a variety of olivine phonolitic leucitite composed essentially of leucite and diopside, and with subordinate olivine, alkali feldspar and phlogopite. Now regarded as an olivine–diopside–richterite madupitic lamproite (Table 2.7, p. 17), with the term 'madupitic' referring to the presence of poikilitic groundmass phlogopite. The original name jumillite is not recommended for usage. (Le Maitre et al., 2005, p. 94)"@en ;
    skos:historyNote "Based on the IUGS classification of igneous rocks (Le Maitre et al., 2005)." ;
    skos:inScheme cs: ;
    skos:notation "ij"^^:gswa-rock-code ;
    skos:prefLabel "olivine-diopside-richterite madupitic lamproite"@en ;
    schema:citation "https://glossary.americangeosciences.org/term/jumillite"^^xsd:anyURI ;
.

:olivine-gabbro
    a skos:Concept ;
    rdfs:isDefinedBy cs: ;
    skos:broader :igneous-mafic-intrusive ;
    skos:definition "A commonly used name for a gabbro containing essential olivine. Now defined modally in the gabbroic rock classification (Fig. 2.6, p. 25) as a variety of gabbro in which olivine is between 5% and 85%. (Le Maitre et al., 2005, p. 119)"@en ;
    skos:historyNote "Based on the IUGS classification of igneous rocks (Le Maitre et al., 2005)." ;
    skos:inScheme cs: ;
    skos:notation "oo"^^:gswa-rock-code ;
    skos:prefLabel "olivine gabbro"@en ;
    schema:citation "https://glossary.americangeosciences.org/term/olivinegabbro"^^xsd:anyURI ;
.

:olivine-gabbronorite
    a skos:Concept ;
    rdfs:isDefinedBy cs: ;
    skos:broader :igneous-mafic-intrusive ;
    skos:definition "A collective term for intrusive rocks consisting of 10–90% calcic plagioclase and accompanied by olivine, orthopyroxene and clinopyroxene in various amounts. Now defined modally in the gabbroic rock classification (Fig. 2.6, p. 25) as a variety of gabbronorite in which olivine is between 5% and 85%. (Le Maitre et al., 2005, p. 119)"@en ;
    skos:historyNote "Based on the IUGS classification of igneous rocks (Le Maitre et al., 2005)." ;
    skos:inScheme cs: ;
    skos:notation "ol"^^:gswa-rock-code ;
    skos:prefLabel "olivine gabbronorite"@en ;
    schema:citation "https://glossary.americangeosciences.org/term/olivinegabbronorite"^^xsd:anyURI ;
.

:olivine-hornblende-pyroxenite
    a skos:Concept ;
    rdfs:isDefinedBy cs: ;
    skos:broader :igneous-ultramafic-intrusive ;
    skos:definition "An ultramafic intrusive rock consisting of more than 30% pyroxene accompanied by hornblende and olivine in various amounts. Now defined modally in the ultramafic rock classification (Fig. 2.9, p. 28). (cf. Le Maitre et al., 2005, p. 119)"@en ;
    skos:historyNote "Based on the IUGS classification of igneous rocks (Le Maitre et al., 2005)." ;
    skos:inScheme cs: ;
    skos:notation "ai"^^:gswa-rock-code ;
    skos:prefLabel "olivine-hornblende pyroxenite"@en ;
    schema:citation "https://glossary.americangeosciences.org/term/olivinehornblendepyroxenite"^^xsd:anyURI ;
.

:olivine-hornblendite
    a skos:Concept ;
    rdfs:isDefinedBy cs: ;
    skos:broader :igneous-ultramafic-intrusive ;
    skos:definition "An ultramafic intrusive rock consisting essentially of amphibole and up to 40% olivine. Now defined modally in the ultramafic rock classification (Fig. 2.9, p. 28). Adapted from Le Maitre et al. (2005, p. 119)."@en ;
    skos:historyNote "Based on the IUGS classification of igneous rocks (Le Maitre et al., 2005)." ;
    skos:inScheme cs: ;
    skos:notation "av"^^:gswa-rock-code ;
    skos:prefLabel "olivine hornblendite"@en ;
    schema:citation "https://glossary.americangeosciences.org/term/olivinehornblendite"^^xsd:anyURI ;
.

:olivine-melilitolite
    a skos:Concept ;
    rdfs:isDefinedBy cs: ;
    skos:broader :igneous-melilitic ;
    skos:definition "An ultramafic intrusive rock containing at least 10% melilite, at least 10% olivine, and less than 10% clinopyroxene (Glossary of geology, Neuendorf et al., 2011, 5th edition, revised). Note that in Le Maitre et al.'s glossary (2005, p. 120), olivine melilitolite is described as \"originally defined as an ultramafic plutonic rock consisting essentially of melilite and olivine with minor clinopyroxene (see 1st Edition, Fig. B.3, p. 12), but not required by the new melilite-bearing rocks classification (section 2.4.1, p. 11)\"."@en ;
    skos:historyNote "Based on the IUGS classification of igneous rocks (Le Maitre et al., 2005) and Glossary of geology (5th edition, revised; Neuendorf et al. 2011)." ;
    skos:inScheme cs: ;
    skos:notation "eo"^^:gswa-rock-code ;
    skos:prefLabel "olivine melilitolite"@en ;
    schema:citation "https://glossary.americangeosciences.org/term/olivinemelilitolite"^^xsd:anyURI ;
.

:olivine-norite
    a skos:Concept ;
    rdfs:isDefinedBy cs: ;
    skos:broader :igneous-mafic-intrusive ;
    skos:definition "An old term for a norite containing essential olivine. Now defined modally in the gabbroic rock classification (Fig. 2.6, p. 25) as a variety of norite in which olivine is between 5% and 85%. (Le Maitre et al., 2005, p. 120)"@en ;
    skos:historyNote "Based on the IUGS classification of igneous rocks (Le Maitre et al., 2005)." ;
    skos:inScheme cs: ;
    skos:notation "or"^^:gswa-rock-code ;
    skos:prefLabel "olivine norite"@en ;
    schema:citation "https://glossary.americangeosciences.org/term/olivinenorite"^^xsd:anyURI ;
.

:olivine-orthopyroxene-gabbro
    a skos:Concept ;
    rdfs:isDefinedBy cs: ;
    skos:broader :igneous-mafic-intrusive ;
    skos:definition "An intrusive rock defined modally in the gabbroic rock classification (Fig. 2.6, p. 25) as a variety of gabbro in which olivine is between 5% and 85% and orthopyroxene exceeds 5% of the pyroxenes. (cf. olivine gabbro/gabbronorite in Le Maitre et al., 2005, p. 119)"@en ;
    skos:historyNote "Based on the IUGS classification of igneous rocks (Le Maitre et al., 2005)." ;
    skos:inScheme cs: ;
    skos:notation "oj"^^:gswa-rock-code ;
    skos:prefLabel "olivine-orthopyroxene gabbro"@en ;
.

:olivine-orthopyroxenite
    a skos:Concept ;
    rdfs:isDefinedBy cs: ;
    skos:broader :igneous-ultramafic-intrusive ;
    skos:definition "An ultramafic intrusive rock consisting essentially of orthopyroxene and 10–40% olivine. Now defined modally in the ultramafic rock classification (Fig. 2.9, p. 28). Adapted from Le Maitre et al. (2005, p. 120)."@en ;
    skos:historyNote "Based on the IUGS classification of igneous rocks (Le Maitre et al., 2005)." ;
    skos:inScheme cs: ;
    skos:notation "aoo"^^:gswa-rock-code ;
    skos:prefLabel "olivine orthopyroxenite"@en ;
    schema:citation "https://glossary.americangeosciences.org/term/olivineorthopyroxenite"^^xsd:anyURI ;
.

:olivine-pyroxene-hornblendite
    a skos:Concept ;
    rdfs:isDefinedBy cs: ;
    skos:broader :igneous-ultramafic-intrusive ;
    skos:definition "An ultramafic intrusive rock consisting of more than 30% amphibole accompanied by pyroxene and olivine in various amounts. Now defined modally in the ultramafic rock classification (Fig. 2.9, p. 28). (cf. Le Maitre et al., 2005, p. 120)"@en ;
    skos:historyNote "Based on the IUGS classification of igneous rocks (Le Maitre et al., 2005)." ;
    skos:inScheme cs: ;
    skos:notation "at"^^:gswa-rock-code ;
    skos:prefLabel "olivine-pyroxene hornblendite"@en ;
    schema:citation "https://glossary.americangeosciences.org/term/olivinepyroxenehornblendite"^^xsd:anyURI ;
.

:olivine-pyroxene-kalsilitite
    a skos:Concept ;
    rdfs:isDefinedBy cs: ;
    skos:broader :igneous-kalsilitic ;
    skos:definition "An ultrabasic rock consisting of phenocrysts of olivine and minor pyroxene in a groundmass of diopside and kalsilite with small amounts of perovskite, olivine and biotite. The historical term mafurite is considered obsolete. Cf. Tables 2.5 & 2.6 on p. 12, and p. 107 in Le Maitre et al. (2005)."@en ;
    skos:historyNote "Based on the IUGS classification of igneous rocks (Le Maitre et al., 2005). See also https://academic.oup.com/petrology/article/63/5/egac026/6553206." ;
    skos:inScheme cs: ;
    skos:notation "wm"^^:gswa-rock-code ;
    skos:prefLabel "olivine-pyroxene kalsilitite"@en ;
    schema:citation "https://glossary.americangeosciences.org/term/mafurite"^^xsd:anyURI ;
.

:olivine-pyroxene-melilitolite
    a skos:Concept ;
    rdfs:isDefinedBy cs: ;
    skos:broader :igneous-melilitic ;
    skos:definition "In the IUGS classification (Le Maitre et al., 2005, p. 11), an intrusive rock consisting mostly of melilite, olivine, and clinopyroxene, with clinopyroxene > olivine (Glossary of geology, Neuendorf et al., 2011, 5th edition, revised))."@en ;
    skos:historyNote "Based on the IUGS classification of igneous rocks (Le Maitre et al., 2005) and Glossary of geology (5th edition, revised; Neuendorf et al. 2011)." ;
    skos:inScheme cs: ;
    skos:notation "el"^^:gswa-rock-code ;
    skos:prefLabel "olivine-pyroxene melilitolite"@en ;
    schema:citation "https://glossary.americangeosciences.org/term/olivinepyroxenemelilitolite"^^xsd:anyURI ;
.

:olivine-pyroxenite
    a skos:Concept ;
    rdfs:isDefinedBy cs: ;
    skos:broader :igneous-ultramafic-intrusive ;
    skos:definition "An ultramafic intrusive rock consisting essentially of pyroxene and 10–40% olivine. Now defined modally in the ultramafic rock classification (Fig. 2.9, p. 28). Adapted from Le Maitre et al. (2005, p. 120)."@en ;
    skos:historyNote "Based on the IUGS classification of igneous rocks (Le Maitre et al., 2005)." ;
    skos:inScheme cs: ;
    skos:notation "ao"^^:gswa-rock-code ;
    skos:prefLabel "olivine pyroxenite"@en ;
    schema:citation "https://glossary.americangeosciences.org/term/olivinepyroxenite"^^xsd:anyURI ;
.

:olivine-websterite
    a skos:Concept ;
    rdfs:isDefinedBy cs: ;
    skos:broader :igneous-ultramafic-intrusive ;
    skos:definition "An ultramafic intrusive rock consisting of 10–40% olivine with various amounts of clinopyroxene and orthopyroxene. Now defined modally in the ultramafic rock classification (Fig. 2.9, p. 28). (cf. Le Maitre et al., 2005, p. 120)"@en ;
    skos:historyNote "Based on the IUGS classification of igneous rocks (Le Maitre et al., 2005)." ;
    skos:inScheme cs: ;
    skos:notation "aow"^^:gswa-rock-code ;
    skos:prefLabel "olivine websterite"@en ;
    schema:citation "https://glossary.americangeosciences.org/term/olivinewebsterite"^^xsd:anyURI ;
.

:oolitic-peloidal-dolomite
    a skos:Concept ;
    rdfs:isDefinedBy cs: ;
    skos:broader :dolomite ;
    skos:definition "A dolomite rock characterized by the presence of ooliths and/or peloids. Ooliths are small round or ovate accretionary bodies resembling the roe of fish, with a diameter of 0.25 to 2 mm (commonly 0.5 to 1 mm), and usually formed of calcium carbonate (but also dolomite, silica, or other minerals) in successive concentric layers, commonly around a nucleus such as a shell fragment, an algal pellet, or a quartz-sand grain, in shallow, wave-agitated water; ooliths commonly show an internal radiating fibrous structure indicating outward growth or enlargement at the site of deposition, and are frequently formed by inorganic precipitation. Peloids are allochems composed of micrite, irrespective of size or origin, for which an exact origin is unknown (e.g. completely micritized fossils or ooids); other types of peloid include pseudo-ooids and aggregates produced by gas bubbling, by microbial precipitation, or by other intraformational reworking of lithified or semilithified carbonate mud. Adapted from Glossary of geology (2011, 5th edition revised)."@en ;
    skos:historyNote "Based on the Glossary of geology (5th edition, revised; Neuendorf et al. 2011)." ;
    skos:inScheme cs: ;
    skos:notation "kdo"^^:gswa-rock-code ;
    skos:prefLabel "oolitic/peloidal dolomite"@en ;
    schema:citation
        "https://glossary.americangeosciences.org/term/oolith"^^xsd:anyURI ,
        "https://glossary.americangeosciences.org/term/oolitic"^^xsd:anyURI ,
        "https://glossary.americangeosciences.org/term/peloid"^^xsd:anyURI ;
.

:oolitic-peloidal-limestone
    a skos:Concept ;
    rdfs:isDefinedBy cs: ;
    skos:broader :limestone ;
    skos:definition "A limestone characterized by the presence of ooliths and/or peloids. Ooliths are small round or ovate accretionary bodies resembling the roe of fish, with a diameter of 0.25 to 2 mm (commonly 0.5 to 1 mm), and usually formed of calcium carbonate (but also dolomite, silica, or other minerals) in successive concentric layers, commonly around a nucleus such as a shell fragment, an algal pellet, or a quartz-sand grain, in shallow, wave-agitated water; ooliths commonly show an internal radiating fibrous structure indicating outward growth or enlargement at the site of deposition, and are frequently formed by inorganic precipitation. Peloids are allochems composed of micrite, irrespective of size or origin, for which an exact origin is unknown (e.g. completely micritized fossils or ooids); other types of peloid include pseudo-ooids and aggregates produced by gas bubbling, by microbial precipitation, or by other intraformational reworking of lithified or semilithified carbonate mud. Adapted from Glossary of geology (5th edition revised; Neuendorf et al., 2011)."@en ;
    skos:historyNote "Based on the Glossary of geology (5th edition, revised; Neuendorf et al. 2011)." ;
    skos:inScheme cs: ;
    skos:notation "klo"^^:gswa-rock-code ;
    skos:prefLabel "oolitic/peloidal limestone"@en ;
    schema:citation
        "https://glossary.americangeosciences.org/term/oolith"^^xsd:anyURI ,
        "https://glossary.americangeosciences.org/term/oolitic"^^xsd:anyURI ,
        "https://glossary.americangeosciences.org/term/peloid"^^xsd:anyURI ;
.

:orthopyroxene-gabbro
    a skos:Concept ;
    rdfs:isDefinedBy cs: ;
    skos:broader :igneous-mafic-intrusive ;
    skos:definition "A basic intrusive rock consisting mainly of calcic plagioclase, clinopyroxene and minor orthopyroxene. Now defined modally in the gabbroic rock classification (Fig. 2.6, p. 25). (Le Maitre et al., 2005, p. 122)"@en ;
    skos:historyNote "Based on the IUGS classification of igneous rocks (Le Maitre et al., 2005)." ;
    skos:inScheme cs: ;
    skos:notation "op"^^:gswa-rock-code ;
    skos:prefLabel "orthopyroxene gabbro"@en ;
    schema:citation "https://glossary.americangeosciences.org/term/orthopyroxenegabbro"^^xsd:anyURI ;
.

:orthopyroxenite
    a skos:Concept ;
    rdfs:isDefinedBy cs: ;
    skos:broader :igneous-ultramafic-intrusive ;
    skos:definition "An ultramafic intrusive rock consisting almost entirely of orthopyroxene. Now defined modally in the ultramafic rock classification (Fig. 2.9, p. 28). (cf. Le Maitre et al., 2005, p. 122)"@en ;
    skos:historyNote "Based on the IUGS classification of igneous rocks (Le Maitre et al., 2005)." ;
    skos:inScheme cs: ;
    skos:notation "axo"^^:gswa-rock-code ;
    skos:prefLabel "orthopyroxenite"@en ;
    schema:citation "https://glossary.americangeosciences.org/term/orthopyroxenite"^^xsd:anyURI ;
.

:peat
    a skos:Concept ;
    rdfs:isDefinedBy cs: ;
    skos:broader :coal ;
    skos:definition "An unconsolidated deposit of semi-carbonized plant remains in a water-saturated environment, such as a bog or fen, and of persistently high moisture content (at least 75%). It is an early stage or rank in the development of coal; carbon content is about 60% and oxygen content is about 30% (moisture-free). Structures of the vegetal matter may or may not be seen depending on the degree of organic matter degradation. When dried, peat burns freely. Adapted from Glossary of geology (5th edition revised; Neuendorf et al., 2011)."@en ;
    skos:exactMatch
        <http://inspire.ec.europa.eu/codelist/LithologyValue/peat> ,
        <http://resource.geosciml.org/classifier/cgi/lithology/peat> ;
    skos:historyNote "Forsman, JP and Hunt, JM 1958, Insoluble organic matter (kerogen) in sedimentary rocks: Geochimica et Cosmochimica Acta, v. 15(3), p. 170–182, doi.org/10.1016/0016-7037(58)90055-3." ;
    skos:inScheme cs: ;
    skos:notation "cot"^^:gswa-rock-code ;
    skos:prefLabel "peat"@en ;
    schema:citation "https://glossary.americangeosciences.org/term/peat"^^xsd:anyURI ;
.

:pebble-conglomerate
    a skos:Concept ;
    rdfs:isDefinedBy cs: ;
    skos:broader :conglomerate ;
    skos:definition "A consolidated rock consisting mainly of pebbles (2–64 mm or -1 to -4 phi units) being somewhat rounded or otherwise modified by abrasion in the course of transport. Adapted from Glossary of geology (5th edition revised; Neuendorf et al., 2011)."@en ;
    skos:historyNote "Wentworth, CK 1922, A scale of grade and class terms for clastic sediments: The Journal of Geology, v. 30, no. 5, p. 377–392, doi:10.1086/622910." ;
    skos:inScheme cs: ;
    skos:notation "si"^^:gswa-rock-code ;
    skos:prefLabel "pebble conglomerate"@en ;
    schema:citation
        "https://glossary.americangeosciences.org/term/pebbleconglomerate"^^xsd:anyURI ,
        "https://glossary.americangeosciences.org/term/pebblesed"^^xsd:anyURI ;
.

:pebbly-sandstone
    a skos:Concept ;
    rdfs:isDefinedBy cs: ;
    skos:altLabel "conglomeratic sandstone"@en ;
    skos:broader :sedimentary-siliciclastic ;
    skos:definition "A consolidated pebbly sand containing 10–20% pebbles in a matrix-supported framework. Adapted from Glossary of geology (5th edition revised; Neuendorf et al., 2011)."@en ;
    skos:historyNote "Based on the Glossary of geology (5th edition, revised; Neuendorf et al. 2011)." ;
    skos:inScheme cs: ;
    skos:notation "sr"^^:gswa-rock-code ;
    skos:prefLabel "pebbly sandstone"@en ;
    schema:citation "https://glossary.americangeosciences.org/term/pebblysandstone"^^xsd:anyURI ;
.

:pegmatite
    a skos:Concept ;
    rdfs:isDefinedBy cs: ;
    skos:broader :igneous-felsic-intrusive ;
    skos:definition "An exceptionally coarse-grained igneous rock, with interlocking crystals, usually found as irregular dykes, lenses, or veins, especially at the margins of batholiths. Most grains are 1 cm or more in diameter. Although pegmatites having gross compositions similar to other rock types are known, their composition is generally that of granite; the composition may be simple or complex and may include rare minerals rich in such elements as lithium, boron, fluorine, niobium, tantalum, uranium, and rare earths. Definition adapted from Glossary of geology (Neuendorf et al., 2011, 5th edition, revised)."@en ;
    skos:exactMatch
        <http://inspire.ec.europa.eu/codelist/LithologyValue/pegmatite> ,
        <http://resource.geosciml.org/classifier/cgi/lithology/pegmatite> ;
    skos:historyNote "Based on the Glossary of geology (5th edition, revised; Neuendorf et al. 2011)." ;
    skos:inScheme cs: ;
    skos:notation "gp"^^:gswa-rock-code ;
    skos:prefLabel "pegmatite"@en ;
    schema:citation "https://glossary.americangeosciences.org/term/pegmatite"^^xsd:anyURI ;
.

:pelitic-gneiss
    a skos:Concept ;
    rdfs:isDefinedBy cs: ;
    skos:broader :metasedimentary-siliciclastic-pelite ;
    skos:definition "Type of gneiss derived by metamorphism of an aluminium-rich, fine-grained sedimentary or metasedimentary protolith. See also definition of gneiss/gneissose structure in Fettes and Desmons (2007, p. 154–155)."@en ;
    skos:historyNote "Compiled by the Geological Survey of Western Australia" ;
    skos:inScheme cs: ;
    skos:notation "mln"^^:gswa-rock-code ;
    skos:prefLabel "pelitic gneiss"@en ;
    schema:citation "https://glossary.americangeosciences.org/term/pelitic"^^xsd:anyURI ;
.

:pelitic-granofels-hornfels
    a skos:Concept ;
    rdfs:isDefinedBy cs: ;
    skos:altLabel
        "hornfelsed pelite"@en ,
        "peraluminous hornfels"@en ;
    skos:broader :metasedimentary-siliciclastic-pelite ;
    skos:definition "Type of granofels/hornfels derived by (contact) metamorphism of an aluminium-rich, argillaceous or fine-grained sedimentary or metasedimentary protolith. Adapted from Fettes and Desmons (2007, p. 182). See also definition of granofels/granofelsic structure in Fettes and Desmons (2007, p. 156); hornfels are granofels formed by contact metamorphism (Fettes and Desmons, 2007, p. 159)."@en ;
    skos:historyNote "Based on the IUGS classification of metamorphic rocks (Fettes and Desmons, 2007)." ;
    skos:inScheme cs: ;
    skos:notation "mle"^^:gswa-rock-code ;
    skos:prefLabel "pelitic granofels/hornfels"@en ;
    schema:citation "https://glossary.americangeosciences.org/term/pelitic"^^xsd:anyURI ;
.

:pelitic-migmatite
    a skos:Concept ;
    rdfs:isDefinedBy cs: ;
    skos:broader :metasedimentary-siliciclastic-pelite ;
    skos:definition "Composite silicate metamorphic rock derived from a fine-grained siliciclastic sedimentary or metasedimentary protolith, pervasively heterogeneous on a meso- to megascopic scale. It typically consists of darker (melanosome) and lighter (leucosome) parts. The darker parts usually exhibit features of metamorphic rocks, whereas the lighter parts are of igneous appearance. See definition of migmatite in Fettes and Desmond (2007, p. 176)."@en ;
    skos:historyNote "Compiled by the Geological Survey of Western Australia" ;
    skos:inScheme cs: ;
    skos:notation "mli"^^:gswa-rock-code ;
    skos:prefLabel "pelitic migmatite"@en ;
    schema:citation "https://glossary.americangeosciences.org/term/pelitic"^^xsd:anyURI ;
.

:pelitic-schist
    a skos:Concept ;
    rdfs:isDefinedBy cs: ;
    skos:broader :metasedimentary-siliciclastic-pelite ;
    skos:definition "Type of schist derived by metamorphism of an aluminium-rich, fine-grained sedimentary or metasedimentary protolith. See also definition of schist/schistose structure in Fettes and Desmons (2007, p. 193)."@en ;
    skos:historyNote "Compiled by the Geological Survey of Western Australia" ;
    skos:inScheme cs: ;
    skos:notation "mls"^^:gswa-rock-code ;
    skos:prefLabel "pelitic schist"@en ;
    schema:citation "https://glossary.americangeosciences.org/term/pelitic"^^xsd:anyURI ;
.

:peridotite
    a skos:Concept ;
    rdfs:isDefinedBy cs: ;
    skos:broader :igneous-ultramafic-volcanic-and-volcaniclastic ;
    skos:definition "A collective term for ultramafic rocks consisting essentially of olivine with pyroxene and/or amphibole. Now defined modally in the ultramafic rock classification (Fig. 2.9, p. 28). (Le Maitre et al., 2005, p. 126)"@en ;
    skos:exactMatch
        <http://inspire.ec.europa.eu/codelist/LithologyValue/peridotite> ,
        <http://resource.geosciml.org/classifier/cgi/lithology/peridotite> ;
    skos:historyNote "Based on the IUGS classification of igneous rocks (Le Maitre et al., 2005)." ;
    skos:inScheme cs: ;
    skos:notation "up"^^:gswa-rock-code ;
    skos:prefLabel "peridotite"@en ;
    schema:citation "https://glossary.americangeosciences.org/term/peridotite"^^xsd:anyURI ;
.

:phosphorite
    a skos:Concept ;
    rdfs:isDefinedBy cs: ;
    skos:broader :sedimentary-other-chemical-or-biochemical ;
    skos:definition "A sedimentary rock with a high enough content of phosphate minerals to be of economic interest. Most commonly it is a bedded primary or reworked secondary marine rock composed of microcrystalline carbonate fluorapatite in the form of laminae, pellets, oolites, nodules, and skeletal, shell, and bone fragments. Adapted from Glossary of geology (5th edition revised; Neuendorf et al., 2011)."@en ;
    skos:exactMatch
        <http://inspire.ec.europa.eu/codelist/LithologyValue/phosphorite> ,
        <http://resource.geosciml.org/classifier/cgi/lithology/phosphorite> ;
    skos:historyNote "Based on the Glossary of geology (5th edition, revised; Neuendorf et al. 2011)." ;
    skos:inScheme cs: ;
    skos:notation "cf"^^:gswa-rock-code ;
    skos:prefLabel "phosphorite"@en ;
    schema:citation "https://glossary.americangeosciences.org/term/phosphorite"^^xsd:anyURI ;
.

:phyllite
    a skos:Concept ;
    rdfs:isDefinedBy cs: ;
    skos:broader :metasedimentary-siliciclastic-pelite ;
    skos:definition "Fine- to medium-grained metamorphic rock characterized by a lustrous sheen and a well-developed schistosity resulting from the parallel arrangement of phyllosilicates. Phyllite is usually of low metamorphic grade. Originally introduced as an alternative to 'phyllade' (term now superseded) to describe a fine-grained schist composed predominantly of micaceous minerals, and as such forming a transition between a (clay-)slate and a mica schist. (Fettes and Desmons, 2007, p. 183)"@en ;
    skos:exactMatch
        <http://inspire.ec.europa.eu/codelist/LithologyValue/phyllite> ,
        <http://resource.geosciml.org/classifier/cgi/lithology/phyllite> ;
    skos:historyNote "Based on the IUGS classification of metamorphic rocks (Fettes and Desmons, 2007)." ;
    skos:inScheme cs: ;
    skos:notation "mlp"^^:gswa-rock-code ;
    skos:prefLabel "phyllite"@en ;
    schema:citation "https://glossary.americangeosciences.org/term/phyllitepetrology"^^xsd:anyURI ;
.

:phyllonite
    a skos:Concept ;
    rdfs:isDefinedBy cs: ;
    skos:broader :metamorphic-protolith-unknown-fault-rock ;
    skos:definition "Phyllosilicate-rich mylonite that has the lustrous sheen of a phyllite (Fettes and Desmons, 2007, p. 183)."@en ;
    skos:exactMatch
        <http://inspire.ec.europa.eu/codelist/LithologyValue/phyllonite> ,
        <http://resource.geosciml.org/classifier/cgi/lithology/phyllonite> ;
    skos:historyNote "Based on the IUGS classification of metamorphic rocks (Fettes and Desmons, 2007)." ;
    skos:inScheme cs: ;
    skos:notation "myp"^^:gswa-rock-code ;
    skos:prefLabel "phyllonite"@en ;
    schema:citation "https://glossary.americangeosciences.org/term/phyllonite"^^xsd:anyURI ;
.

:pisolite
    a skos:Concept ;
    rdfs:isDefinedBy cs: ;
    skos:broader :sedimentary-other-chemical-or-biochemical ;
    skos:definition "A sedimentary rock made up chiefly of pisoids cemented together. Adapted from Glossary of geology (5th edition revised; Neuendorf et al., 2011)."@en ;
    skos:historyNote "Based on the Glossary of geology (5th edition, revised; Neuendorf et al. 2011)." ;
    skos:inScheme cs: ;
    skos:notation "cp"^^:gswa-rock-code ;
    skos:prefLabel "pisolite"@en ;
    schema:citation "https://glossary.americangeosciences.org/term/pisolitesed"^^xsd:anyURI ;
.

:protocataclasite
    a skos:Concept ;
    rdfs:isDefinedBy cs: ;
    skos:broader :metamorphic-protolith-unknown-fault-rock ;
    skos:definition "A cohesive fault rock with a poorly developed or absent schistosity, characterized by generally angular porphyroclasts and lithic fragments in a finer-grained matrix of similar composition that constitutes between 10 and 50% of the rock volume. Definition adapted from Fossen (2016) and Fettes and Desmons (2007, p. 188)."@en ;
    skos:historyNote "Fossen, H 2016, Structural geology (2nd edition): Cambridge University Press, Cambridge, United Kingdom, 524p." ;
    skos:inScheme cs: ;
    skos:notation "myv"^^:gswa-rock-code ;
    skos:prefLabel "protocataclasite"@en ;
.

:protomylonite
    a skos:Concept ;
    rdfs:isDefinedBy cs: ;
    skos:broader :metamorphic-protolith-unknown-fault-rock ;
    skos:definition "A mylonite in which less than 50% of the rock volume has undergone grain-size reduction (Fettes and Desmons, 2007, p. 188); a mylonite with 10–50% matrix and 50–90% porphyroclasts (Passchier and Trouw, 2005)."@en ;
    skos:historyNote "Passchier, CW and Trouw, RAJ 2005, Microtectonics (2nd edition): Springer, Berlin, 366p." ;
    skos:inScheme cs: ;
    skos:notation "myo"^^:gswa-rock-code ;
    skos:prefLabel "protomylonite"@en ;
    schema:citation "https://glossary.americangeosciences.org/term/protomylonite"^^xsd:anyURI ;
.

:psammite-and-pelite-interlayered
    a skos:Concept ;
    rdfs:isDefinedBy cs: ;
    skos:broader :metasedimentary-siliciclastic-psammite-and-pelite-interlayered ;
    skos:definition "A metamorphosed sequence of rocks derived from a interleaving of sandstone and mudstone, i.e. siliciclastic sedimentary protoliths with grain size between 0.0625 and 2 mm and less than 0.0625 mm respectively."@en ;
    skos:historyNote "Compiled by the Geological Survey of Western Australia" ;
    skos:inScheme cs: ;
    skos:notation "mh"^^:gswa-rock-code ;
    skos:prefLabel "psammite and pelite; interlayered"@en ;
    schema:citation
        "https://glossary.americangeosciences.org/term/pelite"^^xsd:anyURI ,
        "https://glossary.americangeosciences.org/term/psammite"^^xsd:anyURI ;
.

:psammitic-and-pelitic-gneiss-interlayered
    a skos:Concept ;
    rdfs:isDefinedBy cs: ;
    skos:broader :metasedimentary-siliciclastic-psammite-and-pelite-interlayered ;
    skos:definition "A gneissose sequence derived by metamorphism of a sedimentary or metasedimentary succession largely consisting of interleaved sandstone and mudstone beds. See also definition of gneiss/gneissose structure in Fettes and Desmons (2007, p. 154–155)."@en ;
    skos:historyNote "Based on the IUGS classification of metamorphic rocks (Fettes and Desmons, 2007)." ;
    skos:inScheme cs: ;
    skos:notation "mhn"^^:gswa-rock-code ;
    skos:prefLabel "psammitic and pelitic gneiss; interlayered"@en ;
    schema:citation
        "https://glossary.americangeosciences.org/term/pelitic"^^xsd:anyURI ,
        "https://glossary.americangeosciences.org/term/psammitic"^^xsd:anyURI ;
.

:psammitic-and-pelitic-granofels-hornfels-interlayered
    a skos:Concept ;
    rdfs:isDefinedBy cs: ;
    skos:broader :metasedimentary-siliciclastic-psammite-and-pelite-interlayered ;
    skos:definition "A granofels/hornfels derived by (contact) metamorphism of a sedimentary or metasedimentary succession largely consisting of interleaved sandstone and mudstone beds. See also definition of granofels/granofelsic structure in Fettes and Desmons (2007, p. 156); hornfels are granofels formed by contact metamorphism (Fettes and Desmons, 2007, p. 159)."@en ;
    skos:historyNote "Compiled by the Geological Survey of Western Australia" ;
    skos:inScheme cs: ;
    skos:notation "mhe"^^:gswa-rock-code ;
    skos:prefLabel "psammitic and pelitic granofels/hornfels; interlayered"@en ;
    schema:citation
        "https://glossary.americangeosciences.org/term/pelitic"^^xsd:anyURI ,
        "https://glossary.americangeosciences.org/term/psammitic"^^xsd:anyURI ;
.

:psammitic-and-pelitic-migmatite-interlayered
    a skos:Concept ;
    rdfs:isDefinedBy cs: ;
    skos:broader :metasedimentary-siliciclastic-psammite-and-pelite-interlayered ;
    skos:definition "Composite silicate metamorphic rock derived from a siliciclastic sedimentary or metasedimentary succession consisting of interleaved sandstone and mudstone beds, and pervasively heterogeneous on a meso- to megascopic scale. It typically consists of darker (melanosome) and lighter (leucosome) parts. The darker parts usually exhibit features of metamorphic rocks, whereas the lighter parts are of igneous appearance. See definition of migmatite in Fettes and Desmond (2007, p. 176)."@en ;
    skos:historyNote "Compiled by the Geological Survey of Western Australia" ;
    skos:inScheme cs: ;
    skos:notation "mhi"^^:gswa-rock-code ;
    skos:prefLabel "psammitic and pelitic migmatite; interlayered"@en ;
    schema:citation
        "https://glossary.americangeosciences.org/term/pelitic"^^xsd:anyURI ,
        "https://glossary.americangeosciences.org/term/psammitic"^^xsd:anyURI ;
.

:psammitic-and-pelitic-schist-interlayered
    a skos:Concept ;
    rdfs:isDefinedBy cs: ;
    skos:broader :metasedimentary-siliciclastic-psammite-and-pelite-interlayered ;
    skos:definition "A schistose sequence derived by metamorphism of a sedimentary or metasedimentary succession largely consisting of interleaved sandstone and mudstone beds. See also definition of schist/schistose structure in Fettes and Desmons (2007, p. 193)."@en ;
    skos:historyNote "Compiled by the Geological Survey of Western Australia" ;
    skos:inScheme cs: ;
    skos:notation "mhs"^^:gswa-rock-code ;
    skos:prefLabel "psammitic and pelitic schist; interlayered"@en ;
    schema:citation
        "https://glossary.americangeosciences.org/term/pelitic"^^xsd:anyURI ,
        "https://glossary.americangeosciences.org/term/psammitic"^^xsd:anyURI ;
.

:psammitic-gneiss
    a skos:Concept ;
    rdfs:isDefinedBy cs: ;
    skos:broader :metasedimentary-siliciclastic-psammite ;
    skos:definition "Type of gneiss derived by metamorphism of a sedimentary or metasedimentary protolith largely consisting of sand-size particles. See also definition of gneiss/gneissose structure in Fettes and Desmons (2007, p. 154–155)."@en ;
    skos:historyNote "Based on the IUGS classification of metamorphic rocks (Fettes and Desmons, 2007)." ;
    skos:inScheme cs: ;
    skos:notation "mtn"^^:gswa-rock-code ;
    skos:prefLabel "psammitic gneiss"@en ;
    schema:citation "https://glossary.americangeosciences.org/term/psammitic"^^xsd:anyURI ;
.

:psammitic-granofels-hornfels
    a skos:Concept ;
    rdfs:isDefinedBy cs: ;
    skos:broader :metasedimentary-siliciclastic-psammite ;
    skos:definition "Type of granofels/hornfels derived by (contact) metamorphism of a sedimentary or metasedimentary protolith largely consisting of sand-size particles. See also definition of granofels/granofelsic structure in Fettes and Desmons (2007, p. 156); hornfels are granofels formed by contact metamorphism (Fettes and Desmons, 2007, p. 159)."@en ;
    skos:historyNote "Compiled by the Geological Survey of Western Australia" ;
    skos:inScheme cs: ;
    skos:notation "mte"^^:gswa-rock-code ;
    skos:prefLabel "psammitic granofels/hornfels"@en ;
    schema:citation "https://glossary.americangeosciences.org/term/psammitic"^^xsd:anyURI ;
.

:psammitic-migmatite
    a skos:Concept ;
    rdfs:isDefinedBy cs: ;
    skos:broader :metasedimentary-siliciclastic-psammite ;
    skos:definition "Composite silicate metamorphic rock derived from a siliciclastic sedimentary or metasedimentary protolith largely consisting of sand-size particles. Pervasively heterogeneous on a meso- to megascopic scale, it typically consists of darker (melanosome) and lighter (leucosome) parts. The darker parts usually exhibit features of metamorphic rocks, whereas the lighter parts are of igneous appearance. See definition of migmatite in Fettes and Desmond (2007, p. 176)."@en ;
    skos:historyNote "Compiled by the Geological Survey of Western Australia" ;
    skos:inScheme cs: ;
    skos:notation "mti"^^:gswa-rock-code ;
    skos:prefLabel "psammitic migmatite"@en ;
    schema:citation "https://glossary.americangeosciences.org/term/psammitic"^^xsd:anyURI ;
.

:psammitic-schist
    a skos:Concept ;
    rdfs:isDefinedBy cs: ;
    skos:broader :metasedimentary-siliciclastic-psammite ;
    skos:definition "Type of schist derived by metamorphism of a sedimentary or metasedimentary protolith largely consisting of sand-size particles. See also definition of schist/schistose structure in Fettes and Desmons (2007, p. 193)."@en ;
    skos:historyNote "Compiled by the Geological Survey of Western Australia" ;
    skos:inScheme cs: ;
    skos:notation "mts"^^:gswa-rock-code ;
    skos:prefLabel "psammitic schist"@en ;
    schema:citation "https://glossary.americangeosciences.org/term/psammitic"^^xsd:anyURI ;
.

:psephitic-gneiss
    a skos:Concept ;
    rdfs:isDefinedBy cs: ;
    skos:broader :metasedimentary-siliciclastic-psephite ;
    skos:definition "Type of gneiss derived by metamorphism of a sedimentary or metasedimentary protolith largely consisting of conglomerate. See also definition of gneiss/gneissose structure in Fettes and Desmons (2007, p. 154–155)."@en ;
    skos:historyNote "Compiled by the Geological Survey of Western Australia" ;
    skos:inScheme cs: ;
    skos:notation "mxn"^^:gswa-rock-code ;
    skos:prefLabel "psephitic gneiss"@en ;
    schema:citation "https://glossary.americangeosciences.org/term/psephitic"^^xsd:anyURI ;
.

:psephitic-granofels-hornfels
    a skos:Concept ;
    rdfs:isDefinedBy cs: ;
    skos:broader :metasedimentary-siliciclastic-psephite ;
    skos:definition "Type of granofels/hornfels derived by (contact) metamorphism of a sedimentary or metasedimentary protolith largely consisting of particles larger than sand size. See also definition of granofels/granofelsic structure in Fettes and Desmons (2007, p. 156); hornfels are granofels formed by contact metamorphism (Fettes and Desmons, 2007, p. 159)."@en ;
    skos:historyNote "Compiled by the Geological Survey of Western Australia" ;
    skos:inScheme cs: ;
    skos:notation "mxe"^^:gswa-rock-code ;
    skos:prefLabel "psephitic granofels/hornfels"@en ;
    schema:citation "https://glossary.americangeosciences.org/term/psephitic"^^xsd:anyURI ;
.

:psephitic-schist
    a skos:Concept ;
    rdfs:isDefinedBy cs: ;
    skos:broader :metasedimentary-siliciclastic-psephite ;
    skos:definition "Type of schist derived by metamorphism of a sedimentary or metasedimentary protolith largely consisting largely of conglomerate. See also definition of schist/schistose structure in Fettes and Desmons (2007, p. 193)."@en ;
    skos:historyNote "Compiled by the Geological Survey of Western Australia" ;
    skos:inScheme cs: ;
    skos:notation "mxs"^^:gswa-rock-code ;
    skos:prefLabel "psephitic schist"@en ;
    schema:citation "https://glossary.americangeosciences.org/term/psephitic"^^xsd:anyURI ;
.

:pseudotachylite-fault-rock
    a skos:Concept ;
    rdfs:isDefinedBy cs: ;
    skos:altLabel "pseudotachylyte"@en ;
    skos:broader :metamorphic-protolith-unknown-fault-rock ;
    skos:definition "Extremely fine-grained to glassy, dark, cohesive rock occurring as veins or as a matrix to pseudo-conglomerates or breccias, formed through frictional melting and subsequent quenching during earthquakes and large-scale landslides (Trouw et al., 2010). Note the vocabulary has a separate concept for pseudotachylite formed through impact events."@en ;
    skos:historyNote "Trouw, RAJ, Passchier, CW and Wiersma, DJ 2010, Atlas of Mylonites and related microstructures: Springer-Verlag, Berlin, Germany. 322p." ;
    skos:inScheme cs: ;
    skos:notation "myt"^^:gswa-rock-code ;
    skos:prefLabel "pseudotachylite (fault rock)"@en ;
    schema:citation "https://glossary.americangeosciences.org/term/pseudotachylyte"^^xsd:anyURI ;
.

:pseudotachylite-impactite
    a skos:Concept ;
    rdfs:isDefinedBy cs: ;
    skos:altLabel "pseudotachylyte"@en ;
    skos:broader :metamorphic-protolith-unknown-impactite ;
    skos:definition "Pseudotachylite produced by impact metamorphism. Dyke-like breccia formed by frictional melting in the basement of impact craters, resulting often in irregular vein-like networks. Typically, it contains unshocked and shocked mineral and lithic clasts in a fine-grained aphanitic matrix. (Cf. Fettes and Desmons, 2007, p. 162)"@en ;
    skos:historyNote "Based on the IUGS classification of metamorphic rocks (Fettes and Desmons, 2007)." ;
    skos:inScheme cs: ;
    skos:notation "mpt"^^:gswa-rock-code ;
    skos:prefLabel "pseudotachylite (impactite)"@en ;
.

:pyroxene-hornblende-gabbro
    a skos:Concept ;
    rdfs:isDefinedBy cs: ;
    skos:broader :igneous-mafic-intrusive ;
    skos:definition "An intrusive rock (and including coarse-grained parts of extrusive successions) defined modally in the gabbroic rock classification (Fig. 2.6, p. 25) as a variety of gabbro in which hornblende is between 5% and 85% (cf. Le Maitre et al., 2005, p. 133)."@en ;
    skos:historyNote "Based on the IUGS classification of igneous rocks (Le Maitre et al., 2005)." ;
    skos:inScheme cs: ;
    skos:notation "oe"^^:gswa-rock-code ;
    skos:prefLabel "pyroxene-hornblende gabbro"@en ;
.

:pyroxene-hornblende-gabbronorite
    a skos:Concept ;
    rdfs:isDefinedBy cs: ;
    skos:broader :igneous-mafic-intrusive ;
    skos:definition "An intrusive rock (and including coarse-grained parts of extrusive successions) defined modally in the gabbroic rock classification (Fig. 2.6, p. 25) as a variety of gabbronorite in which hornblende is between 5% and 85% (Le Maitre et al., 2005, p. 133)."@en ;
    skos:historyNote "Based on the IUGS classification of igneous rocks (Le Maitre et al., 2005)." ;
    skos:inScheme cs: ;
    skos:notation "ob"^^:gswa-rock-code ;
    skos:prefLabel "pyroxene-hornblende gabbronorite"@en ;
    schema:citation "https://glossary.americangeosciences.org/term/pyroxenehornblendegabbronorite"^^xsd:anyURI ;
.

:pyroxene-hornblende-norite
    a skos:Concept ;
    rdfs:isDefinedBy cs: ;
    skos:broader :igneous-mafic-intrusive ;
    skos:definition "An intrusive rock (and including coarse-grained parts of extrusive successions) defined modally in the gabbroic rock classification (Fig. 2.6, p. 25) as a variety of norite in which hornblende is between 5% and 85% (cf. Le Maitre et al., 2005, p. 133)."@en ;
    skos:historyNote "Based on the IUGS classification of igneous rocks (Le Maitre et al., 2005)." ;
    skos:inScheme cs: ;
    skos:notation "of"^^:gswa-rock-code ;
    skos:prefLabel "pyroxene-hornblende norite"@en ;
.

:pyroxene-hornblende-peridotite
    a skos:Concept ;
    rdfs:isDefinedBy cs: ;
    skos:broader :igneous-ultramafic-intrusive ;
    skos:definition "An ultramafic intrusive rock consisting of 40–90% olivine and various amounts of pyroxene and amphibole. Now defined modally in the ultramafic rock classification (Fig. 2.9, p. 28). (cf. Le Maitre et al., 2005, p. 133)"@en ;
    skos:historyNote "Based on the IUGS classification of igneous rocks (Le Maitre et al., 2005)." ;
    skos:inScheme cs: ;
    skos:notation "au"^^:gswa-rock-code ;
    skos:prefLabel "pyroxene-hornblende peridotite"@en ;
    schema:citation "https://glossary.americangeosciences.org/term/pyroxenehornblendeperidotite"^^xsd:anyURI ;
.

:pyroxene-hornblendite
    a skos:Concept ;
    rdfs:isDefinedBy cs: ;
    skos:broader :igneous-ultramafic-intrusive ;
    skos:definition "A term for ultramafic intrusive rocks composed mainly of amphibole with up to 50% pyroxene. Now defined modally in the ultramafic rock classification (Fig. 2.9, p. 28). (cf. Le Maitre et al., 2005, p. 133)"@en ;
    skos:historyNote "Based on the IUGS classification of igneous rocks (Le Maitre et al., 2005)." ;
    skos:inScheme cs: ;
    skos:notation "ab"^^:gswa-rock-code ;
    skos:prefLabel "pyroxene hornblendite"@en ;
    schema:citation "https://glossary.americangeosciences.org/term/pyroxenehornblendite"^^xsd:anyURI ;
.

:pyroxene-melilitolite
    a skos:Concept ;
    rdfs:isDefinedBy cs: ;
    skos:broader :igneous-melilitic ;
    skos:definition "In the IUGS classification (Le Maitre et al., 2005, p. 11), an ultramafic intrusive rock consisting mostly of melilite and clinopyroxene, with less than 10% olivine (adapted from Glossary of geology, Neuendorf et al., 2011, 5th edition, revised). Note that in Le Maitre et al.'s glossary (2005, p. 133), pyroxene olivine melilitolite is described as \"originally defined as an ultramafic plutonic rock consisting essentially of melilite and clinopyroxene with minor olivine (see 1st Edition, Fig. B.3, p. 12), but not required by the new melilite-bearing rocks classification (section 2.4.1, p. 11).\""@en ;
    skos:historyNote "Based on the IUGS classification of igneous rocks (Le Maitre et al., 2005) and Glossary of geology (5th edition, revised; Neuendorf et al. 2011)." ;
    skos:inScheme cs: ;
    skos:notation "ep"^^:gswa-rock-code ;
    skos:prefLabel "pyroxene melilitolite"@en ;
    schema:citation "https://glossary.americangeosciences.org/term/pyroxenemelilitolite"^^xsd:anyURI ;
.

:pyroxene-olivine-melilitolite
    a skos:Concept ;
    rdfs:isDefinedBy cs: ;
    skos:broader :igneous-melilitic ;
    skos:definition "In the IUGS classification (Le Maitre et al., p. 11), an ultramafic intrusive rock consisting mostly of melilite, olivine, and clinopyroxene, with olivine>clinopyroxene (adapted from Glossary of geology, Neuendorf et al., 2011, 5th edition, revised). Note that in Le Maitre et al.'s glossary (2005, p. 133), pyroxene olivine melilitolite is described as \"originally defined as an ultramafic plutonic rock consisting essentially of melilite, olivine and lesser amounts of clinopyroxene (see 1st Edition, Fig. B.3, p. 12), but not required by the new melilite-bearing rocks classification (section 2.4.1, p. 11)\"."@en ;
    skos:historyNote "Based on the IUGS classification of igneous rocks (Le Maitre et al., 2005) and Glossary of geology (5th edition, revised; Neuendorf et al. 2011)." ;
    skos:inScheme cs: ;
    skos:notation "ey"^^:gswa-rock-code ;
    skos:prefLabel "pyroxene-olivine melilitolite"@en ;
    schema:citation "https://glossary.americangeosciences.org/term/pyroxeneolivinemelilitolite"^^xsd:anyURI ;
.

:pyroxene-peridotite
    a skos:Concept ;
    rdfs:isDefinedBy cs: ;
    skos:broader :igneous-ultramafic-intrusive ;
    skos:definition "A term for intrusive rocks composed mainly of olivine with 10–60% pyroxene. Now defined modally in the ultramafic rock classification (Fig. 2.9, p. 28). Adapted from Le Maitre et al. (2005, p. 134)."@en ;
    skos:historyNote "Based on the IUGS classification of igneous rocks (Le Maitre et al., 2005)." ;
    skos:inScheme cs: ;
    skos:notation "ap"^^:gswa-rock-code ;
    skos:prefLabel "pyroxene peridotite"@en ;
    schema:citation "https://glossary.americangeosciences.org/term/pyroxeneperidotite"^^xsd:anyURI ;
.

:pyroxene-spinifex-textured-basalt
    a skos:Concept ;
    rdfs:isDefinedBy cs: ;
    skos:altLabel
        "high-Mg basalt"@en ,
        "high-magnesium basalt"@en ;
    skos:broader :igneous-mafic-volcanic ;
    skos:definition "A volcanic basaltic rock distinguished by the presence of pyroxene spinifex texture, i.e. an igneous texture consisting of needle-like pyroxene crystals usually forming a criss-crossing pattern, the result of rapid quenching from unusually high temperatures (cf. https://glossary.americangeosciences.org/term/spinifextexture). Note that the term is commonly used as a proxy for high-magnesium basaltic rocks but in GSWA usage it is not synonymous with komatiitic basalt. The GSWA's rock classification scheme prefers the use of volcanic terminology for any igneous rock formed on or near the Earth's surface, i.e. for those hypabyssal or subvolcanic rocks such as dykes, sills, and cryptodomes that are demonstrably both spatially and temporally associated with extrusive volcanic rocks."@en ;
    skos:historyNote "Based on the IUGS classification of igneous rocks (Le Maitre et al., 2005) and GSWA usage." ;
    skos:inScheme cs: ;
    skos:notation "bs"^^:gswa-rock-code ;
    skos:prefLabel "pyroxene spinifex-textured basalt"@en ;
.

:pyroxenite-extrusive
    a skos:Concept ;
    rdfs:isDefinedBy cs: ;
    skos:broader :igneous-ultramafic-volcanic-and-volcaniclastic ;
    skos:definition "An ultramafic igneous rock composed almost entirely of one or more pyroxenes and occasionally biotite, hornblende and olivine. Now defined modally in the ultramafic rock classification (Fig. 2.9, p. 28). Definition adapted from Le Maitre et al. (2005, p. 134). In GSWA usage an 'extrusive' pyroxenite is identified as one formed from fractionation within thick bodies of ultramafic volcanic or subvolcanic magmas. GSWA's rock classification scheme prefers the use of volcanic terminology for any igneous rock formed on or near the Earth's surface, i.e. for those hypabyssal or subvolcanic rocks such as dykes, sills, and cryptodomes that are demonstrably both spatially and temporally associated with extrusive volcanic rocks."@en ;
    skos:historyNote "Based on the IUGS classification of igneous rocks (Le Maitre et al., 2005)." ;
    skos:inScheme cs: ;
    skos:notation "ux"^^:gswa-rock-code ;
    skos:prefLabel "pyroxenite (extrusive)"@en ;
    schema:citation "https://glossary.americangeosciences.org/term/pyroxenite"^^xsd:anyURI ;
.

:pyroxenite-intrusive
    a skos:Concept ;
    rdfs:isDefinedBy cs: ;
    skos:broader :igneous-ultramafic-intrusive ;
    skos:definition "An ultramafic intrusive rocks composed almost entirely of one or more pyroxenes and occasionally biotite, hornblende and olivine. Now defined modally in the ultramafic rock classification (Fig. 2.9, p. 28). Adapted from Le Maitre et al. (2005, p. 134)."@en ;
    skos:historyNote "Based on the IUGS classification of igneous rocks (Le Maitre et al., 2005)." ;
    skos:inScheme cs: ;
    skos:notation "ax"^^:gswa-rock-code ;
    skos:prefLabel "pyroxenite (intrusive)"@en ;
    schema:citation "https://glossary.americangeosciences.org/term/pyroxenite"^^xsd:anyURI ;
.

:pyroxenitic-fault-rock
    a skos:Concept ;
    rdfs:isDefinedBy cs: ;
    skos:broader :metamorphic-protolith-unknown-fault-rock ;
    skos:definition "A rock formed as a result of deformation in a fault zone and distinguished by the abundance of pyroxenes. In GSWA usage, this term is reserved for fault rocks for which a protolith cannot be conclusively established."@en ;
    skos:historyNote "Compiled by the Geological Survey of Western Australia" ;
    skos:inScheme cs: ;
    skos:notation "myr"^^:gswa-rock-code ;
    skos:prefLabel "pyroxenitic fault rock"@en ;
.

:pyroxenitic-gneiss
    a skos:Concept ;
    rdfs:isDefinedBy cs: ;
    skos:broader :metamorphic-protolith-unknown-gneiss ;
    skos:definition "A gneiss distinguished by the abundance of pyroxenes. In GSWA usage, this term is reserved for gneiss for which a protolith cannot be conclusively established. See also definition of gneiss/gneissose structure in Fettes and Desmons (2007, p. 154–155)."@en ;
    skos:historyNote "Based on the IUGS classification of metamorphic rocks (Fettes and Desmons, 2007) and GSWA usage." ;
    skos:inScheme cs: ;
    skos:notation "mnx"^^:gswa-rock-code ;
    skos:prefLabel "pyroxenitic gneiss"@en ;
    schema:citation "https://glossary.americangeosciences.org/term/gneiss"^^xsd:anyURI ;
.

:pyroxenitic-granofels-hornfels
    a skos:Concept ;
    rdfs:isDefinedBy cs: ;
    skos:broader :metamorphic-protolith-unknown-granofels-hornfels ;
    skos:definition "A granofels/hornfels distinguished by the abundance of pyroxenes. In GSWA usage, this term is reserved for a granofels/hornfels for which a protolith cannot be conclusively established."@en ;
    skos:historyNote "Compiled by the Geological Survey of Western Australia" ;
    skos:inScheme cs: ;
    skos:notation "mex"^^:gswa-rock-code ;
    skos:prefLabel "pyroxenitic granofels/hornfels"@en ;
.

:pyroxenitic-schist
    a skos:Concept ;
    rdfs:isDefinedBy cs: ;
    skos:broader :metamorphic-protolith-unknown-schist ;
    skos:definition "A schist distinguished by the abundance of pyroxenes. In GSWA usage, this term is reserved for a schist for which a protolith cannot be conclusively established. See also definition of schist/schistose structure in Fettes and Desmons, 2007, p. 193)."@en ;
    skos:historyNote "Based on the IUGS classification of metamorphic rocks (Fettes and Desmons, 2007) and GSWA usage." ;
    skos:inScheme cs: ;
    skos:notation "msx"^^:gswa-rock-code ;
    skos:prefLabel "pyroxenitic schist"@en ;
.

:quartz-alkali-feldspar-syenite
    a skos:Concept ;
    rdfs:isDefinedBy cs: ;
    skos:broader :igneous-felsic-intrusive ;
    skos:definition "A felsic intrusive rock composed mainly of alkali feldspar, quartz and mafic minerals. Now defined modally in QAPF field 6* (Fig. 2.4, p. 22). (cf. Le Maitre et al., 2005, p. 134)"@en ;
    skos:exactMatch
        <http://inspire.ec.europa.eu/codelist/LithologyValue/quartzAlkaliFeldsparSyenite> ,
        <http://resource.geosciml.org/classifier/cgi/lithology/quartz_alkali_feldspar_syenite> ;
    skos:historyNote "Based on the IUGS classification of igneous rocks (Le Maitre et al., 2005)." ;
    skos:inScheme cs: ;
    skos:notation "gq"^^:gswa-rock-code ;
    skos:prefLabel "quartz alkali feldspar syenite"@en ;
    schema:citation "https://glossary.americangeosciences.org/term/quartzalkalifeldsparsyenite"^^xsd:anyURI ;
.

:quartz-anorthosite
    a skos:Concept ;
    rdfs:isDefinedBy cs: ;
    skos:altLabel "plagioclasite"@en ;
    skos:broader :igneous-felsic-intrusive ;
    skos:definition "A leucocratic intrusive rock consisting essentially of calcic plagioclase, quartz and with small amounts of pyroxene. Now defined modally in QAPF field 10* (Fig. 2.4, p. 22). The term is synonymous with plagioclasite. (cf. Le Maitre et al., 2005, p. 134)"@en ;
    skos:exactMatch
        <http://inspire.ec.europa.eu/codelist/LithologyValue/quartzAnorthosite> ,
        <http://resource.geosciml.org/classifier/cgi/lithology/quartz_anorthosite> ;
    skos:historyNote "Based on the IUGS classification of igneous rocks (Le Maitre et al., 2005)." ;
    skos:inScheme cs: ;
    skos:notation "go"^^:gswa-rock-code ;
    skos:prefLabel "quartz anorthosite"@en ;
    schema:citation "https://glossary.americangeosciences.org/term/quartzanorthosite"^^xsd:anyURI ;
.

:quartz-diorite
    a skos:Concept ;
    rdfs:isDefinedBy cs: ;
    skos:broader :igneous-felsic-intrusive ;
    skos:definition "An intrusive rock having the composition of diorite but with an appreciable amount of quartz, i.e. between 5 and 20% of the felsic minerals, and defined modally in QAPF field 10* (Fig. 2.4, p. 22). Adapted from Le Maitre et al. (2005, p. 134)."@en ;
    skos:exactMatch
        <http://inspire.ec.europa.eu/codelist/LithologyValue/quartzDiorite> ,
        <http://resource.geosciml.org/classifier/cgi/lithology/quartz_diorite> ;
    skos:historyNote "Based on the IUGS classification of igneous rocks (Le Maitre et al., 2005)." ;
    skos:inScheme cs: ;
    skos:notation "gd"^^:gswa-rock-code ;
    skos:prefLabel "quartz diorite"@en ;
    schema:citation "https://glossary.americangeosciences.org/term/quartzdiorite"^^xsd:anyURI ;
.

:quartz-gabbro
    a skos:Concept ;
    rdfs:isDefinedBy cs: ;
    skos:broader :igneous-felsic-intrusive ;
    skos:definition "An intrusive rock composed mainly of calcic plagioclase, clinopyroxene and quartz. Now defined modally in QAPF field 10* (Fig. 2.4, p. 22). (cf. Le Maitre et al., 2005, p. 134)"@en ;
    skos:exactMatch
        <http://inspire.ec.europa.eu/codelist/LithologyValue/quartzGabbro> ,
        <http://resource.geosciml.org/classifier/cgi/lithology/quartz_gabbro> ;
    skos:historyNote "Based on the IUGS classification of igneous rocks (Le Maitre et al., 2005)." ;
    skos:inScheme cs: ;
    skos:notation "gu"^^:gswa-rock-code ;
    skos:prefLabel "quartz gabbro"@en ;
    schema:citation "https://glossary.americangeosciences.org/term/quartzgabbro"^^xsd:anyURI ;
.

:quartz-latite
    a skos:Concept ;
    rdfs:isDefinedBy cs: ;
    skos:broader :igneous-felsic-volcanic ;
    skos:definition "A term originally used for a volcanic rock composed of phenocrysts of quartz, plagioclase, biotite and hornblende in a glassy matrix potentially of quartz and alkali feldspar. Now commonly used for volcanic rocks composed of alkali feldspar and plagioclase in roughly equal amounts, quartz and mafic minerals. Now defined modally in QAPF field 8* (Fig. 2.4, p. 22). Definition from Le Maitre et al. (2005, p. 135). GSWA's rock classification scheme prefers the use of volcanic terminology for any igneous rock formed on or near the Earth's surface, i.e. for those hypabyssal or subvolcanic rocks such as dykes, sills, and cryptodomes that are demonstrably both spatially and temporally associated with extrusive volcanic rocks."@en ;
    skos:exactMatch
        <http://inspire.ec.europa.eu/codelist/LithologyValue/quartzLatite> ,
        <http://resource.geosciml.org/classifier/cgi/lithology/quartz_latite> ;
    skos:historyNote "Based on the IUGS classification of igneous rocks (Le Maitre et al., 2005)." ;
    skos:inScheme cs: ;
    skos:notation "fi"^^:gswa-rock-code ;
    skos:prefLabel "quartz latite"@en ;
    schema:citation "https://glossary.americangeosciences.org/term/quartzlatite"^^xsd:anyURI ;
.

:quartz-mica-schist
    a skos:Concept ;
    rdfs:isDefinedBy cs: ;
    skos:broader :metamorphic-protolith-unknown-schist ;
    skos:definition "A schist distinguished by the abundance of quartz and micaceous mineral phases. In GSWA usage, this term is reserved for a schist for which a protolith cannot be conclusively established. See also definition of schist/schistose structure in Fettes and Desmons, 2007, p. 193)."@en ;
    skos:historyNote "Based on the IUGS classification of metamorphic rocks (Fettes and Desmons, 2007) and GSWA usage." ;
    skos:inScheme cs: ;
    skos:notation "msqm"^^:gswa-rock-code ;
    skos:prefLabel "quartz-mica schist"@en ;
    schema:citation "https://glossary.americangeosciences.org/term/schist"^^xsd:anyURI ;
.

:quartz-monzodiorite
    a skos:Concept ;
    rdfs:isDefinedBy cs: ;
    skos:broader :igneous-felsic-intrusive ;
    skos:definition "An intrusive rock consisting essentially of sodic plagioclase, alkali feldspar, quartz and mafic minerals. Now defined modally in QAPF field 9* (Fig. 2.4, p. 22). (cf. Le Maitre et al., 2005, p. 135)."@en ;
    skos:exactMatch
        <http://inspire.ec.europa.eu/codelist/LithologyValue/quartzMonzodiorite> ,
        <http://resource.geosciml.org/classifier/cgi/lithology/quartz_monzodiorite> ;
    skos:historyNote "Based on the IUGS classification of igneous rocks (Le Maitre et al., 2005)." ;
    skos:inScheme cs: ;
    skos:notation "gk"^^:gswa-rock-code ;
    skos:prefLabel "quartz monzodiorite"@en ;
    schema:citation "https://glossary.americangeosciences.org/term/quartzmonzodiorite"^^xsd:anyURI ;
.

:quartz-monzogabbro
    a skos:Concept ;
    rdfs:isDefinedBy cs: ;
    skos:broader :igneous-felsic-intrusive ;
    skos:definition "An intrusive rock consisting essentially of calcic plagioclase, alkali feldspar, quartz and mafic minerals. Now defined modally in QAPF field 9* (Fig. 2.4, p. 22). (cf. Le Maitre et al., 2005, p. 135)."@en ;
    skos:exactMatch
        <http://inspire.ec.europa.eu/codelist/LithologyValue/quartzMonzogabbro> ,
        <http://resource.geosciml.org/classifier/cgi/lithology/quartz_monzogabbro> ;
    skos:historyNote "Based on the IUGS classification of igneous rocks (Le Maitre et al., 2005)." ;
    skos:inScheme cs: ;
    skos:notation "gl"^^:gswa-rock-code ;
    skos:prefLabel "quartz monzogabbro"@en ;
    schema:citation "https://glossary.americangeosciences.org/term/quartzmonzogabbro"^^xsd:anyURI ;
.

:quartz-monzonite
    a skos:Concept ;
    rdfs:isDefinedBy cs: ;
    skos:broader :igneous-felsic-intrusive ;
    skos:definition "An intrusive rock consisting of approximately equal amounts of alkali feldspar and plagioclase and with essential quartz (5–20% of felsic minerals) but not enough to make the rock a granite. Now defined modally in QAPF field 8* (Fig. 2.4, p. 22). (cf. Le Maitre et al., 2005, p.  135)"@en ;
    skos:exactMatch
        <http://inspire.ec.europa.eu/codelist/LithologyValue/quartzMonzonite> ,
        <http://resource.geosciml.org/classifier/cgi/lithology/quartz_monzonite> ;
    skos:historyNote "Based on the IUGS classification of igneous rocks (Le Maitre et al., 2005)." ;
    skos:inScheme cs: ;
    skos:notation "gc"^^:gswa-rock-code ;
    skos:prefLabel "quartz monzonite"@en ;
    schema:citation "https://glossary.americangeosciences.org/term/quartzmonzonite"^^xsd:anyURI ;
.

:quartz-syenite
    a skos:Concept ;
    rdfs:isDefinedBy cs: ;
    skos:broader :igneous-felsic-intrusive ;
    skos:definition "An intrusive rock consisting essentially of alkali feldspar, quartz and mafic minerals. Now defined modally in QAPF field 7* (Fig. 2.4, p. 22). (cf. Le Maitre et al., 2005, p. 135)"@en ;
    skos:exactMatch
        <http://inspire.ec.europa.eu/codelist/LithologyValue/quartzSyenite> ,
        <http://resource.geosciml.org/classifier/cgi/lithology/quartz_syenite> ;
    skos:historyNote "Based on the IUGS classification of igneous rocks (Le Maitre et al., 2005)." ;
    skos:inScheme cs: ;
    skos:notation "ge"^^:gswa-rock-code ;
    skos:prefLabel "quartz syenite"@en ;
    schema:citation "https://glossary.americangeosciences.org/term/quartzsyenite"^^xsd:anyURI ;
.

:quartz-trachyte
    a skos:Concept ;
    rdfs:isDefinedBy cs: ;
    skos:broader :igneous-felsic-volcanic ;
    skos:definition "A volcanic rock consisting of phenocrysts of alkali feldspar and quartz in a cryptocrystalline or glassy matrix. It is the volcanic equivalent of quartz syenite. Now defined modally in QAPF field 7* (Fig. 2.11, p. 31). Definition from Le Maitre et al. (2005, p. 135). GSWA's rock classification scheme prefers the use of volcanic terminology for any igneous rock formed on or near the Earth's surface, i.e. for those hypabyssal or subvolcanic rocks such as dykes, sills, and cryptodomes that are demonstrably both spatially and temporally associated with extrusive volcanic rocks."@en ;
    skos:exactMatch
        <http://inspire.ec.europa.eu/codelist/LithologyValue/quartzTrachyte> ,
        <http://resource.geosciml.org/classifier/cgi/lithology/quartz_trachyte> ;
    skos:historyNote "Based on the IUGS classification of igneous rocks (Le Maitre et al., 2005)." ;
    skos:inScheme cs: ;
    skos:notation "fy"^^:gswa-rock-code ;
    skos:prefLabel "quartz trachyte"@en ;
    schema:citation "https://glossary.americangeosciences.org/term/quartztrachyte"^^xsd:anyURI ;
.

:quartz-vein
    a skos:Concept ;
    rdfs:isDefinedBy cs: ;
    skos:broader :hydrothermal ;
    skos:definition "A rock comprising quartz crystals of hydrothermal origin, as vein-filling material."@en ;
    skos:historyNote "Compiled by the Geological Survey of Western Australia" ;
    skos:inScheme cs: ;
    skos:notation "zq"^^:gswa-rock-code ;
    skos:prefLabel "quartz vein"@en ;
    schema:citation "https://glossary.americangeosciences.org/term/veinquartz"^^xsd:anyURI ;
.

:quartz-wacke
    a skos:Concept ;
    rdfs:isDefinedBy cs: ;
    skos:altLabel
        "quartzwacke"@en ,
        "subgraywacke"@en ,
        "subgreywacke"@en ;
    skos:broader :wacke ;
    skos:definition "A wacke that contains more than 90% quartz and less than 5% each of feldspar and rock/lithic grains. Adapted from Glossary of geology (5th edition revised; Neuendorf et al., 2011)."@en ;
    skos:historyNote "Pettijohn, FJ 1975, Sedimentary Rocks: New York, Harper and Row, 628p." ;
    skos:inScheme cs: ;
    skos:notation "swq"^^:gswa-rock-code ;
    skos:prefLabel "quartz wacke"@en ;
    schema:citation "https://glossary.americangeosciences.org/term/quartzwacke"^^xsd:anyURI ;
.

:quartzarenite
    a skos:Concept ;
    rdfs:isDefinedBy cs: ;
    skos:altLabel
        "orthoquartzite"@en ,
        "quartz arenite"@en ,
        "quartz sandstone"@en ,
        "quartzite"@en ;
    skos:broader :arenite ;
    skos:definition "An arenite composed primarily of quartz (excluding detrital chert grains); specifically one containing more than 95% quartz framework grains and less than 5% feldspar and rock/lithic grains. The term is essentially equivalent to orthoquartzite, which in some past GSWA usage has been abbreviated to quartzite. GSWA reserves the use of 'quartzite' for a demonstrably metamorphosed rock. Adapted from Glossary of geology (5th edition revised; Neuendorf et al., 2011)."@en ;
    skos:historyNote "Pettijohn, FJ 1975, Sedimentary Rocks: New York, Harper and Row, 628p." ;
    skos:inScheme cs: ;
    skos:notation "saq"^^:gswa-rock-code ;
    skos:prefLabel "quartzarenite"@en ;
    schema:citation "https://glossary.americangeosciences.org/term/quartzarenite"^^xsd:anyURI ;
.

:quartzite
    a skos:Concept ;
    rdfs:isDefinedBy cs: ;
    skos:broader :metasedimentary-siliciclastic-psammite ;
    skos:definition "A granoblastic metamorphic rock consisting mainly of quartz and formed by recrystallization of sandstone or chert by either regional or thermal metamorphism (Glossary of geology, 5th edition revised; Neuendorf et al., 2011). Note that GSWA usage restricts the use of the term quartzite to metamorphic rocks."@en ;
    skos:exactMatch
        <http://inspire.ec.europa.eu/codelist/LithologyValue/quartzite> ,
        <http://resource.geosciml.org/classifier/cgi/lithology/quartzite> ;
    skos:historyNote "Compiled by the Geological Survey of Western Australia" ;
    skos:inScheme cs: ;
    skos:notation "mtq"^^:gswa-rock-code ;
    skos:prefLabel "quartzite"@en ;
    schema:citation "https://glossary.americangeosciences.org/term/quartzitemeta"^^xsd:anyURI ;
.

:quartzofeldspathic-fault-rock
    a skos:Concept ;
    rdfs:isDefinedBy cs: ;
    skos:broader :metamorphic-protolith-unknown-fault-rock ;
    skos:definition "A rock formed as a result of deformation in a fault zone and distinguished by the abundance of quartz and feldspar mineral phases. In GSWA usage, this term is reserved for fault rocks for which a protolith cannot be conclusively established."@en ;
    skos:historyNote "Compiled by the Geological Survey of Western Australia" ;
    skos:inScheme cs: ;
    skos:notation "myqf"^^:gswa-rock-code ;
    skos:prefLabel "quartzofeldspathic fault rock"@en ;
.

:quartzofeldspathic-gneiss
    a skos:Concept ;
    rdfs:isDefinedBy cs: ;
    skos:broader :metamorphic-protolith-unknown-gneiss ;
    skos:definition "A gneiss distinguished by the abundance of quartz and feldspar mineral phases. In GSWA usage, this term is reserved for a gneiss for which a protolith cannot be conclusively established. See also definition of gneiss/gneissose structure in Fettes and Desmons (2007, p. 154–155)."@en ;
    skos:historyNote "Based on the IUGS classification of metamorphic rocks (Fettes and Desmons, 2007) and GSWA usage." ;
    skos:inScheme cs: ;
    skos:notation "mnqf"^^:gswa-rock-code ;
    skos:prefLabel "quartzofeldspathic gneiss"@en ;
    schema:citation "https://glossary.americangeosciences.org/term/gneiss"^^xsd:anyURI ;
.

:quartzofeldspathic-granofels-hornfels
    a skos:Concept ;
    rdfs:isDefinedBy cs: ;
    skos:broader :metamorphic-protolith-unknown-granofels-hornfels ;
    skos:definition "A granofels/hornfels distinguished by the abundance of quartz and feldspar mineral phases. In GSWA usage, this term is reserved for a granofels/hornfels for which a protolith cannot be conclusively established."@en ;
    skos:historyNote "Compiled by the Geological Survey of Western Australia" ;
    skos:inScheme cs: ;
    skos:notation "meqf"^^:gswa-rock-code ;
    skos:prefLabel "quartzofeldspathic granofels/hornfels"@en ;
.

:quartzofeldspathic-schist
    a skos:Concept ;
    rdfs:isDefinedBy cs: ;
    skos:broader :metamorphic-protolith-unknown-schist ;
    skos:definition "A schist distinguished by the abundance of quartz and feldspar mineral phases. In GSWA usage, this term is reserved for a schist for which a protolith cannot be conclusively established. See also definition of schist/schistose structure in Fettes and Desmons, 2007, p. 193)."@en ;
    skos:historyNote "Based on the IUGS classification of metamorphic rocks (Fettes and Desmons, 2007) and GSWA usage." ;
    skos:inScheme cs: ;
    skos:notation "msqf"^^:gswa-rock-code ;
    skos:prefLabel "quartzofeldspathic schist"@en ;
    schema:citation "https://glossary.americangeosciences.org/term/schist"^^xsd:anyURI ;
.

:quartzose-fault-rock
    a skos:Concept ;
    rdfs:isDefinedBy cs: ;
    skos:broader :metamorphic-protolith-unknown-fault-rock ;
    skos:definition "A rock formed as a result of deformation in a fault zone and distinguished by the abundance of quartz. In GSWA usage, this term is reserved for fault rocks for which a protolith cannot be conclusively established."@en ;
    skos:historyNote "Compiled by the Geological Survey of Western Australia" ;
    skos:inScheme cs: ;
    skos:notation "myq"^^:gswa-rock-code ;
    skos:prefLabel "quartzose fault rock"@en ;
.

:quartzose-gneiss
    a skos:Concept ;
    rdfs:isDefinedBy cs: ;
    skos:broader :metamorphic-protolith-unknown-gneiss ;
    skos:definition "A gneiss distinguished by the abundance of quartz. In GSWA usage, this term is reserved for a gneiss for which a protolith cannot be conclusively established. See also definition of gneiss/gneissose structure in Fettes and Desmons (2007, p. 154–155)."@en ;
    skos:historyNote "Based on the IUGS classification of metamorphic rocks (Fettes and Desmons, 2007) and GSWA usage." ;
    skos:inScheme cs: ;
    skos:notation "mnq"^^:gswa-rock-code ;
    skos:prefLabel "quartzose gneiss"@en ;
    schema:citation "https://glossary.americangeosciences.org/term/gneiss"^^xsd:anyURI ;
.

:quartzose-hornfels
    a skos:Concept ;
    rdfs:isDefinedBy cs: ;
    skos:altLabel "contact quartzite"@en ;
    skos:broader :metamorphic-protolith-unknown-granofels-hornfels ;
    skos:definition "Term proposed to distinguish a quartzite formed by contact metamorphism from other types of metamorphic quartzite. (Fettes and Desmons, 2007, p. 190)"@en ;
    skos:historyNote "Compiled by the Geological Survey of Western Australia" ;
    skos:inScheme cs: ;
    skos:notation "meq"^^:gswa-rock-code ;
    skos:prefLabel "quartzose hornfels"@en ;
.

:quartzose-schist
    a skos:Concept ;
    rdfs:isDefinedBy cs: ;
    skos:broader :metamorphic-protolith-unknown-schist ;
    skos:definition "A schist distinguished by the abundance of quartz. In GSWA usage, this term is reserved for a schist for which a protolith cannot be conclusively established. See also definition of schist/schistose structure in Fettes and Desmons, 2007, p. 193)."@en ;
    skos:historyNote "Based on the IUGS classification of metamorphic rocks (Fettes and Desmons, 2007) and GSWA usage." ;
    skos:inScheme cs: ;
    skos:notation "msq"^^:gswa-rock-code ;
    skos:prefLabel "quartzose schist"@en ;
    schema:citation "https://glossary.americangeosciences.org/term/schist"^^xsd:anyURI ;
.

:radiolarite
    a skos:Concept ;
    rdfs:isDefinedBy cs: ;
    skos:altLabel "radiolarian earth"@en ;
    skos:broader :sedimentary-other-chemical-or-biochemical ;
    skos:definition "The comparatively hard, fine-grained, chert-like, homogeneous consolidated equivalent of radiolarian earth; indurated radiolarian ooze. Adapted from Glossary of geology (5th edition revised; Neuendorf et al., 2011)."@en ;
    skos:historyNote "Based on the Glossary of geology (5th edition, revised; Neuendorf et al. 2011)." ;
    skos:inScheme cs: ;
    skos:notation "cr"^^:gswa-rock-code ;
    skos:prefLabel "radiolarite"@en ;
    schema:citation "https://glossary.americangeosciences.org/term/radiolaritesed"^^xsd:anyURI ;
.

:reaction-skarn
    a skos:Concept ;
    rdfs:isDefinedBy cs: ;
    skos:altLabel "bimetasomatic skarn"@en ;
    skos:broader :skarn ;
    skos:definition "A skarn formed by local exchange of material by diffusion and reaction across contacts between carbonate beds and silicate sedimentary or other suitable (chemically different) rock types."@en ;
    skos:historyNote "Einaudi, MT and Burt, DM 1982, Introduction – terminology, classification, and composition of skarn deposits: Economic Geology, v. 77, p. 745–754." ;
    skos:inScheme cs: ;
    skos:notation "mjks"^^:gswa-rock-code ;
    skos:prefLabel "reaction skarn"@en ;
.

:rhyodacite
    a skos:Concept ;
    rdfs:isDefinedBy cs: ;
    skos:broader :igneous-felsic-volcanic ;
    skos:definition "A term used for volcanic rocks intermediate between rhyolite and dacite, usually consisting of phenocrysts of quartz, plagioclase and a few ferromagnesian minerals in a microcrystalline groundmass. Definition from Le Maitre et al. (2005, p. 137). GSWA's rock classification scheme prefers the use of volcanic terminology for any igneous rock formed on or near the Earth's surface, i.e. for those hypabyssal or subvolcanic rocks such as dykes, sills, and cryptodomes that are demonstrably both spatially and temporally associated with extrusive volcanic rocks."@en ;
    skos:historyNote "Based on the IUGS classification of igneous rocks (Le Maitre et al., 2005)." ;
    skos:inScheme cs: ;
    skos:notation "fc"^^:gswa-rock-code ;
    skos:prefLabel "rhyodacite"@en ;
    schema:citation "https://glossary.americangeosciences.org/term/rhyodacite"^^xsd:anyURI ;
.

:rhyolite
    a skos:Concept ;
    rdfs:isDefinedBy cs: ;
    skos:broader :igneous-felsic-volcanic ;
    skos:definition "A collective term for silicic volcanic rocks consisting of phenocrysts of quartz and alkali feldspar, often with minor plagioclase and biotite, in a microcrystalline or glassy groundmass and having the chemical composition of granite. Now defined modally in QAPF field 3 (Fig. 2.11, p. 31) and, if modes are not available, chemically in TAS field R (Fig. 2.14, p. 35). Definition from Le Maitre et al. (2005, p. 137). GSWA's rock classification scheme prefers the use of volcanic terminology for any igneous rock formed on or near the Earth's surface, i.e. for those hypabyssal or subvolcanic rocks such as dykes, sills, and cryptodomes that are demonstrably both spatially and temporally associated with extrusive volcanic rocks."@en ;
    skos:exactMatch
        <http://inspire.ec.europa.eu/codelist/LithologyValue/rhyolite> ,
        <http://resource.geosciml.org/classifier/cgi/lithology/rhyolite> ;
    skos:historyNote "Based on the IUGS classification of igneous rocks (Le Maitre et al., 2005)." ;
    skos:inScheme cs: ;
    skos:notation "fr"^^:gswa-rock-code ;
    skos:prefLabel "rhyolite"@en ;
    schema:citation "https://glossary.americangeosciences.org/term/rhyolite"^^xsd:anyURI ;
.

:rodingite
    a skos:Concept ;
    rdfs:isDefinedBy cs: ;
    skos:broader :metasomatic ;
    skos:definition "Metasomatic rock primarily composed of grossular–andradite garnet and calcic pyroxene; epidote, scapolite and iron ore are characteristic accessories. Rodingite mostly replaces dykes or inclusions of basic rocks within serpentinized ultramafic bodies, such as volcanic rocks or amphibolites associated with ultramafic bodies. (Fettes and Desmons, 2007, p. 191)"@en ;
    skos:historyNote "Based on the IUGS classification of metamorphic rocks (Fettes and Desmons, 2007)." ;
    skos:inScheme cs: ;
    skos:notation "mjo"^^:gswa-rock-code ;
    skos:prefLabel "rodingite"@en ;
    schema:citation
        "https://en.wikipedia.org/wiki/Rodingite;"^^xsd:anyURI ,
        "https://glossary.americangeosciences.org/term/rodingite"^^xsd:anyURI ;
.

:sand
    a skos:Concept ;
    rdfs:isDefinedBy cs: ;
    skos:broader :sedimentary-siliciclastic ;
    skos:definition "A weekly cemented aggregate of mineral or rock particles of sand size, having a diameter in the range of 0.0625 to 2 mm (62–2000 μm, or 4 to -1 phi units). The material is most commonly composed of quartz resulting from rock disintegration, and when the term 'sand' is used without qualification, a siliceous composition is implied; but the particles may be of any mineral composition or mixture of rock or mineral fragments, such as 'coral sand' consisting of limestone fragments. Also, a mass of such material, especially on a beach, a desert or in a stream bed. Adapted from Glossary of geology (5th edition revised; Neuendorf et al., 2011)."@en ;
    skos:exactMatch
        <http://inspire.ec.europa.eu/codelist/LithologyValue/sand> ,
        <http://inspire.ec.europa.eu/codelist/LithologyValue/sandSizeSediment> ,
        <http://resource.geosciml.org/classifier/cgi/lithology/sand> ,
        <http://resource.geosciml.org/classifier/cgi/lithology/sand_size_sediment> ;
    skos:inScheme cs: ;
    skos:notation "sq"^^:gswa-rock-code ;
    skos:prefLabel "sand"@en ;
    schema:citation "https://glossary.americangeosciences.org/term/sandsed"^^xsd:anyURI ;
.

:sandstone-with-conglomerate
    a skos:Concept ;
    rdfs:isDefinedBy cs: ;
    skos:broader :sedimentary-siliciclastic ;
    skos:definition "Sandstone and conglomerate beds/intervals interleaved at outcrop scale."@en ;
    skos:historyNote "Compiled by the Geological Survey of Western Australia" ;
    skos:inScheme cs: ;
    skos:notation "sp"^^:gswa-rock-code ;
    skos:prefLabel "sandstone + conglomerate"@en ;
.

:sandstone-with-other-siliciclastic-rock
    a skos:Concept ;
    rdfs:isDefinedBy cs: ;
    skos:broader :sedimentary-siliciclastic ;
    skos:definition "Dominant sandstone rocks/beds/intervals interleaved at outcrop scale with other subordinate siliciclastic rocks/beds/intervals."@en ;
    skos:historyNote "Compiled by the Geological Survey of Western Australia" ;
    skos:inScheme cs: ;
    skos:notation "sz"^^:gswa-rock-code ;
    skos:prefLabel "sandstone + other siliciclastic rock"@en ;
.

:sandstone-with-siltstone
    a skos:Concept ;
    rdfs:isDefinedBy cs: ;
    skos:broader :sedimentary-siliciclastic ;
    skos:definition "Sandstone and siltstone beds/intervals interleaved at outcrop scale."@en ;
    skos:historyNote "Compiled by the Geological Survey of Western Australia" ;
    skos:inScheme cs: ;
    skos:notation "ss"^^:gswa-rock-code ;
    skos:prefLabel "sandstone + siltstone"@en ;
.

:sannaite
    a skos:Concept ;
    rdfs:isDefinedBy cs: ;
    skos:broader :igneous-lamprophyres ;
    skos:definition "A variety of lamprophyre composed of combinations of olivine, titanian augite, kaersutite and Ti-rich biotite phenocrysts with alkali feldspar dominating over plagioclase in the groundmass that also contains nepheline. Now defined in the lamprophyre classification (Table 2.9, p. 19). (Le Maitre et al., 2005, p. 139)"@en ;
    skos:historyNote "Based on the IUGS classification of igneous rocks (Le Maitre et al., 2005)." ;
    skos:inScheme cs: ;
    skos:notation "ya"^^:gswa-rock-code ;
    skos:prefLabel "sannaite"@en ;
.

:schist
    a skos:Concept ;
    rdfs:isDefinedBy cs: ;
    skos:broader :metamorphic-protolith-unknown-schist ;
    skos:definition "A metamorphic rock for which a protolith cannot be conclusively identified and displaying a schistose structure, i.e. a preferred orientation of inequant mineral grains or grain aggregates produced by metamorphic processes. A schist can be readily split into thin flakes or slabs because of the well-developed parallelism of more than 50% of the minerals present, particularly those of lamellar or elongate prismatic habit (e.g. mica and hornblende). For phyllosilicate-rich rocks the term schist is commonly used for medium- to coarse-grained varieties, whereas finer-grained rocks may be given more specific names such as slates or phyllites. Adapted from Fettes and Desmons (2007, p. 193) and Glossary of geology (5th edition revised; Neuendorf et al., 2011)."@en ;
    skos:exactMatch
        <http://inspire.ec.europa.eu/codelist/LithologyValue/schist> ,
        <http://resource.geosciml.org/classifier/cgi/lithology/schist> ;
    skos:historyNote "Based on the IUGS classification of metamorphic rocks (Fettes and Desmons, 2007)." ;
    skos:inScheme cs: ;
    skos:notation "ms"^^:gswa-rock-code ;
    skos:prefLabel "schist"@en ;
    schema:citation "https://glossary.americangeosciences.org/term/schist"^^xsd:anyURI ;
.

:schistose-fault-rock
    a skos:Concept ;
    rdfs:isDefinedBy cs: ;
    skos:broader :metamorphic-protolith-unknown-fault-rock ;
    skos:definition "A fault rock that retains some fissility. In GSWA usage, this term is reserved for fault rocks for which a protolith cannot be conclusively established."@en ;
    skos:historyNote "Compiled by the Geological Survey of Western Australia" ;
    skos:inScheme cs: ;
    skos:notation "mys"^^:gswa-rock-code ;
    skos:prefLabel "schistose fault rock"@en ;
.

:schistose-granulite
    a skos:Concept ;
    rdfs:isDefinedBy cs: ;
    skos:broader :metamorphic-protolith-unknown-schist ;
    skos:definition "A high-grade metamorphic rock, with a granoblastic texture and in which Fe–Mg silicates are dominantly hydroxyl-free, feldspar is a critical phase, and primary muscovite is absent, and with a superimposed foliation. In GSWA usage, this term is reserved for a schist for which a protolith cannot be conclusively established. See also definition of schist/schistose structure in Fettes and Desmons, 2007, p. 193)."@en ;
    skos:historyNote "Based on the IUGS classification of metamorphic rocks (Fettes and Desmons, 2007) and GSWA usage." ;
    skos:inScheme cs: ;
    skos:notation "mso"^^:gswa-rock-code ;
    skos:prefLabel "schistose granulite"@en ;
.

:schistose-hydrothermal-rock
    a skos:Concept ;
    rdfs:isDefinedBy cs: ;
    skos:broader :metamorphosed-hydrothermal ;
    skos:definition "A metamorphosed hydrothermal rock displaying a schistose structure. See also definition of schist/schistose structure in Fettes and Desmons (2007, p. 193)."@en ;
    skos:historyNote "Based on the IUGS classification of metamorphic rocks (Fettes and Desmons, 2007)." ;
    skos:inScheme cs: ;
    skos:notation "mzs"^^:gswa-rock-code ;
    skos:prefLabel "schistose hydrothermal rock"@en ;
    schema:citation
        "https://glossary.americangeosciences.org/term/hydrothermalalteration"^^xsd:anyURI ,
        "https://glossary.americangeosciences.org/term/schist"^^xsd:anyURI ;
.

:schistose-marble
    a skos:Concept ;
    rdfs:isDefinedBy cs: ;
    skos:broader :marble ;
    skos:definition "A metamorphosed sedimentary carbonate rock consisting of more than 50% volume of carbonate minerals (calcite and/or aragonite and/or dolomite) and displaying a schistose structure. See also definition of gneiss/gneissose structure in Fettes and Desmons (2007, p. 154–155)."@en ;
    skos:historyNote "Compiled by the Geological Survey of Western Australia" ;
    skos:inScheme cs: ;
    skos:notation "mkks"^^:gswa-rock-code ;
    skos:prefLabel "schistose marble"@en ;
.

:schistose-meta-iron-formation
    a skos:Concept ;
    rdfs:isDefinedBy cs: ;
    skos:altLabel
        "itabirite"@en ,
        "taconite"@en ;
    skos:broader :metasedimentary-other-chemical-meta-iron-formation ;
    skos:definition "A metamorphosed iron formation displaying a schistose structure, i.e. a schist derived from a chemical or biochemical sedimentary protolith containing at least 15% iron of sedimentary origin. See also definition of schist/schistose structure in Fettes and Desmons, 2007, p. 193)."@en ;
    skos:historyNote "Based on the IUGS classification of metamorphic rocks (Fettes and Desmons, 2007) and GSWA usage." ;
    skos:inScheme cs: ;
    skos:notation "mis"^^:gswa-rock-code ;
    skos:prefLabel "schistose meta-iron formation"@en ;
    schema:citation "https://glossary.americangeosciences.org/term/schist"^^xsd:anyURI ;
.

:schistose-metacarbonatite
    a skos:Concept ;
    rdfs:isDefinedBy cs: ;
    skos:broader :meta-igneous-carbonatite ;
    skos:definition "A schist derived by metamorphism of an igneous protolith containing a modal amount of primary carbonate minerals greater than 50%. See also definition of schist/schistose structure in Fettes and Desmons (2007, p. 193)."@en ;
    skos:inScheme cs: ;
    skos:notation "mqs"^^:gswa-rock-code ;
    skos:prefLabel "schistose metacarbonatite"@en ;
.

:schistose-metachert
    a skos:Concept ;
    rdfs:isDefinedBy cs: ;
    skos:broader :metasedimentary-other-chemical ;
    skos:definition "A metamorphosed chert displaying a schistose structure, i.e. a schist derived from a chemical or biochemical sedimentary rock largely consisting of silica and/or quartz. See also definition of schist/schistose structure in Fettes and Desmons, 2007, p. 193)."@en ;
    skos:historyNote "Compiled by the Geological Survey of Western Australia" ;
    skos:inScheme cs: ;
    skos:notation "mcs"^^:gswa-rock-code ;
    skos:prefLabel "schistose metachert"@en ;
.

:schistose-para-amphibolite-carbonate
    a skos:Concept ;
    rdfs:isDefinedBy cs: ;
    skos:broader :para-amphibolite-derived-from-carbonate-rock ;
    skos:definition "A metamorphosed amphibole-rich rock derived from a sedimentary carbonate protolith and displaying a schistose structure. See also definition of gneiss/gneissose structure in Fettes and Desmons (2007, p. 154–155)."@en ;
    skos:historyNote "Compiled by the Geological Survey of Western Australia" ;
    skos:inScheme cs: ;
    skos:notation "mkas"^^:gswa-rock-code ;
    skos:prefLabel "schistose para-amphibolite (carbonate)"@en ;
.

:schistose-para-amphibolite-siliciclastic
    a skos:Concept ;
    rdfs:isDefinedBy cs: ;
    skos:broader :para-amphibolite ;
    skos:definition "A metamorphosed amphibole-rich rock derived from a sedimentary siliciclastic protolith and displaying a schistose structure. See also definition of gneiss/gneissose structure in Fettes and Desmons (2007, p. 154–155)."@en ;
    skos:historyNote "Compiled by the Geological Survey of Western Australia" ;
    skos:inScheme cs: ;
    skos:notation "mdas"^^:gswa-rock-code ;
    skos:prefLabel "schistose para-amphibolite (siliciclastic)"@en ;
.

:sedimentary-breccia
    a skos:Concept ;
    rdfs:isDefinedBy cs: ;
    skos:altLabel
        "rubble rock"@en ,
        "sharpstone conglomerate"@en ;
    skos:broader :sedimentary-siliciclastic ;
    skos:definition "A coarse epiclastic rock formed by lithification of angular gravel (in which 30% of large particles are greater than 2 mm). Breccia differs from conglomerate in that the fragments have sharp edges and unworn corners, and may originate as a result of sedimentary processes such as talus accumulation, disturbance during sedimentation (intraclastic breccia), or collapse of rock material (solution breccia, collapse breccia). Excludes breccias formed by volcaniclastic processes. Adapted from Glossary of geology (5th edition revised; Neuendorf et al., 2011)."@en ;
    skos:historyNote "Based on the Glossary of geology (5th edition, revised; Neuendorf et al. 2011)." ;
    skos:inScheme cs: ;
    skos:notation "sx"^^:gswa-rock-code ;
    skos:prefLabel "sedimentary breccia"@en ;
    schema:citation
        "https://glossary.americangeosciences.org/term/brecciageol"^^xsd:anyURI ,
        "https://glossary.americangeosciences.org/term/sedimentarybreccia"^^xsd:anyURI ;
.

:sedimentary-rock
    a skos:Concept ;
    rdfs:isDefinedBy cs: ;
    skos:broader :sedimentary ;
    skos:definition "A rock of sedimentary but otherwise unspecified origin, i.e. a rock for which a clastic or chemical/biochemical derivation cannot be conclusively established (e.g. due to alteration or weathering)."@en ;
    skos:exactMatch
        <http://inspire.ec.europa.eu/codelist/LithologyValue/sedimentaryRock> ,
        <http://resource.geosciml.org/classifier/cgi/lithology/sedimentary_rock> ;
    skos:historyNote "Compiled by the Geological Survey of Western Australia" ;
    skos:inScheme cs: ;
    skos:notation "sed"^^:gswa-rock-code ;
    skos:prefLabel "sedimentary rock"@en ;
    schema:citation "https://glossary.americangeosciences.org/term/sedimentary"^^xsd:anyURI ;
.

:semipelite
    a skos:Concept ;
    rdfs:isDefinedBy cs: ;
    skos:broader :metasedimentary-siliciclastic-semipelite ;
    skos:definition "A metamorphic rock that has a modal ratio of mica to quartz + feldspar intermediate between a pelite and a psammite (adapted from Fettes and Desmons, 2007, p. 194)."@en ;
    skos:historyNote "Based on the IUGS classification of metamorphic rocks (Fettes and Desmons, 2007)." ;
    skos:inScheme cs: ;
    skos:notation "mm"^^:gswa-rock-code ;
    skos:prefLabel "semipelite"@en ;
.

:semipelitic-gneiss
    a skos:Concept ;
    rdfs:isDefinedBy cs: ;
    skos:broader :metasedimentary-siliciclastic-semipelite ;
    skos:definition "Type of gneiss derived by metamorphism of a fine- to medium-grained sedimentary or metasedimentary protolith, and with a modal ratio of mica to quartz + feldspar intermediate between a pelite and a psammite. See also definition of gneiss/gneissose structure in Fettes and Desmons (2007, p. 154–155)."@en ;
    skos:historyNote "Compiled by the Geological Survey of Western Australia" ;
    skos:inScheme cs: ;
    skos:notation "mmn"^^:gswa-rock-code ;
    skos:prefLabel "semipelitic gneiss"@en ;
.

:semipelitic-granofels-hornfels
    a skos:Concept ;
    rdfs:isDefinedBy cs: ;
    skos:altLabel
        "hornfelsed pelite"@en ,
        "peraluminous hornfels"@en ;
    skos:broader :metasedimentary-siliciclastic-semipelite ;
    skos:definition "Type of micaceous granofels/hornfels derived by (contact) metamorphism of a fine- to medium-grained sedimentary or metasedimentary protolith, and with a modal ratio of mica to quartz + feldspar intermediate between a pelite and a psammite. See also definition of granofels/granofelsic structure in Fettes and Desmons (2007, p. 156); hornfels are granofels formed by contact metamorphism (Fettes and Desmons, 2007, p. 159)."@en ;
    skos:historyNote "Compiled by the Geological Survey of Western Australia" ;
    skos:inScheme cs: ;
    skos:notation "mme"^^:gswa-rock-code ;
    skos:prefLabel "semipelitic granofels/hornfels"@en ;
.

:semipelitic-migmatite
    a skos:Concept ;
    rdfs:isDefinedBy cs: ;
    skos:broader :metasedimentary-siliciclastic-semipelite ;
    skos:definition "Composite, micaceous silicate metamorphic rock derived from a fine- to medium-grained siliciclastic sedimentary or metasedimentary protolith, with a modal ratio of mica to quartz + feldspar intermediate between a pelite and a psammite, and pervasively heterogeneous on a meso- to megascopic scale. It typically consists of darker (melanosome) and lighter (leucosome) parts. The darker parts usually exhibit features of metamorphic rocks, whereas the lighter parts are of igneous appearance. See definition of migmatite in Fettes and Desmond (2007, p. 176)."@en ;
    skos:historyNote "Compiled by the Geological Survey of Western Australia" ;
    skos:inScheme cs: ;
    skos:notation "mmi"^^:gswa-rock-code ;
    skos:prefLabel "semipelitic migmatite"@en ;
.

:semipelitic-schist
    a skos:Concept ;
    rdfs:isDefinedBy cs: ;
    skos:broader :metasedimentary-siliciclastic-semipelite ;
    skos:definition "Type of schist derived by metamorphism of a fine- to medium-grained sedimentary or metasedimentary protolith, and with a modal ratio of mica to quartz + feldspar intermediate between a pelite and a psammite. See also definition of schist/schistose structure in Fettes and Desmons (2007, p. 193)."@en ;
    skos:historyNote "Compiled by the Geological Survey of Western Australia" ;
    skos:inScheme cs: ;
    skos:notation "mms"^^:gswa-rock-code ;
    skos:prefLabel "semipelitic schist"@en ;
.

:serpentinite-derived-from-intrusive-rock
    a skos:Concept ;
    rdfs:isDefinedBy cs: ;
    skos:broader :meta-igneous-ultramafic-intrusive ;
    skos:definition "Metamorphic rock composed of more than 75% vol. of minerals of the serpentine group, and demonstrably derived from an igneous (intrusive or coarse-grained extrusive) protolith (adapted from Fettes and Desmons, 2007, p. 194)."@en ;
    skos:historyNote "Based on the IUGS classification of metamorphic rocks (Fettes and Desmons, 2007)." ;
    skos:inScheme cs: ;
    skos:notation "mat"^^:gswa-rock-code ;
    skos:prefLabel "serpentinite derived from intrusive rock"@en ;
.

:serpentinite-derived-from-volcanic-rock
    a skos:Concept ;
    rdfs:isDefinedBy cs: ;
    skos:broader :meta-igneous-ultramafic-volcanic ;
    skos:definition "Metamorphic rock composed of more than 75% vol. of minerals of the serpentine group, and demonstrably derived from an igneous extrusive protolith (adapted from Fettes and Desmons, 2007, p. 194)."@en ;
    skos:historyNote "Based on the IUGS classification of metamorphic rocks (Fettes and Desmons, 2007)." ;
    skos:inScheme cs: ;
    skos:notation "mut"^^:gswa-rock-code ;
    skos:prefLabel "serpentinite derived from volcanic rock"@en ;
.

:shale
    a skos:Concept ;
    rdfs:isDefinedBy cs: ;
    skos:broader :sedimentary-siliciclastic ;
    skos:definition "A laminated, indurated very fine-grained rock with more than 66% clay-sized minerals; a claystone with fissility. GSWA now discourages the use of 'shale' as it is considered predominantly a textural term. Adapted from Glossary of geology (5th edition revised; Neuendorf et al., 2011)."@en ;
    skos:exactMatch
        <http://inspire.ec.europa.eu/codelist/LithologyValue/shale> ,
        <http://resource.geosciml.org/classifier/cgi/lithology/shale> ;
    skos:historyNote "Compiled by the Geological Survey of Western Australia" ;
    skos:inScheme cs: ;
    skos:notation "sh"^^:gswa-rock-code ;
    skos:prefLabel "shale"@en ;
    schema:citation "https://glossary.americangeosciences.org/term/shale"^^xsd:anyURI ;
.

:shocked-target-rock
    a skos:Concept ;
    rdfs:isDefinedBy cs: ;
    skos:broader :metamorphic-protolith-unknown-impactite ;
    skos:definition "Non-brecciated rocks showing unequivocal effects of shock metamorphism, exclusive of whole rock melting (Osinski et al., 2022)."@en ;
    skos:historyNote "Osinski, GR, Grieve, RAF, Ferrière, L, Losiak, A, Pickersgill, AE, Cavosie, AJ, Hibbard, SM, Hill, PJA, Bermudez, JJ, Marion, CL, Newman, JD and Simpson, SL, 2022, Impact Earth: A review of the terrestrial impact record: Earth-Science Reviews, v. 232, 104112, doi.org/10.1016/j.earscirev.2022.104112." ;
    skos:inScheme cs: ;
    skos:notation "mph"^^:gswa-rock-code ;
    skos:prefLabel "shocked target rock"@en ;
.

:siliceous-sinter
    a skos:Concept ;
    rdfs:isDefinedBy cs: ;
    skos:altLabel
        "geyserite"@en ,
        "sinter"@en ;
    skos:broader :sedimentary-other-chemical-or-biochemical ;
    skos:definition "The lightweight porous opaline variety of silica, white or nearly white, deposited as an incrustation by precipitation from the waters of geysers and hot springs. The term has been applied loosely to any deposit made by a geyser or hot spring. Adapted from Glossary of geology (5th edition revised; Neuendorf et al., 2011)."@en ;
    skos:historyNote "Based on the Glossary of geology (5th edition, revised; Neuendorf et al. 2011)." ;
    skos:inScheme cs: ;
    skos:notation "cz"^^:gswa-rock-code ;
    skos:prefLabel "siliceous sinter"@en ;
    schema:citation "https://glossary.americangeosciences.org/term/siliceoussinter"^^xsd:anyURI ;
.

:siliciclastic-gneiss
    a skos:Concept ;
    rdfs:isDefinedBy cs: ;
    skos:altLabel "paragneiss"@en ;
    skos:broader :metasedimentary-siliciclastic ;
    skos:definition "A metamorphosed siliciclastic rock displaying a gneissose structure, i.e. a gneiss from a clastic sedimentary protolith and largely consisting of silicates and quartz. See also definition of gneiss/gneissose structure in Fettes and Desmons (2007, p. 154–155)."@en ;
    skos:historyNote "Based on the IUGS classification of metamorphic rocks (Fettes and Desmons, 2007)." ;
    skos:inScheme cs: ;
    skos:narrowMatch
        <http://inspire.ec.europa.eu/codelist/LithologyValue/paragneiss> ,
        <http://resource.geosciml.org/classifier/cgi/lithology/paragneiss> ;
    skos:notation "mdn"^^:gswa-rock-code ;
    skos:prefLabel "siliciclastic gneiss"@en ;
.

:siliciclastic-granofels-hornfels
    a skos:Concept ;
    rdfs:isDefinedBy cs: ;
    skos:broader :metasedimentary-siliciclastic ;
    skos:definition "A metamorphosed siliciclastic rock displaying a granofelsic structure, i.e. a granofels/hornfels derived from a clastic sedimentary protolith and largely consisting of silicates and quartz. See also definition of granofels/granofelsic structure in Fettes and Desmons (2007, p. 156); hornfels are granofels formed by contact metamorphism (Fettes and Desmons, 2007, p. 159)."@en ;
    skos:historyNote "Based on the IUGS classification of metamorphic rocks (Fettes and Desmons, 2007)." ;
    skos:inScheme cs: ;
    skos:notation "mde"^^:gswa-rock-code ;
    skos:prefLabel "siliciclastic granofels/hornfels"@en ;
.

:siliciclastic-migmatite
    a skos:Concept ;
    rdfs:isDefinedBy cs: ;
    skos:broader :metasedimentary-siliciclastic ;
    skos:definition "Composite silicate metamorphic rock derived from a siliciclastic protolith, pervasively heterogeneous on a meso- to megascopic scale. It typically consists of darker (melanosome) and lighter (leucosome) parts. The darker parts usually exhibit features of metamorphic rocks, whereas the lighter parts are of igneous appearance. Adapted from Fettes and Desmond (2007, p. 176)."@en ;
    skos:historyNote "Based on the IUGS classification of metamorphic rocks (Fettes and Desmons, 2007)." ;
    skos:inScheme cs: ;
    skos:notation "mdi"^^:gswa-rock-code ;
    skos:prefLabel "siliciclastic migmatite"@en ;
.

:siliciclastic-rock
    a skos:Concept ;
    rdfs:isDefinedBy cs: ;
    skos:broader :sedimentary-siliciclastic ;
    skos:closeMatch
        <http://inspire.ec.europa.eu/codelist/LithologyValue/clasticSedimentaryRock> ,
        <http://resource.geosciml.org/classifier/cgi/lithology/clastic_sedimentary_rock> ;
    skos:definition "A sedimentary rock that is silicon-bearing (in the form of quartz and silicates) and is composed principally of broken fragments that are derived from pre-existing rocks or minerals and that have been transported some distance from their places of origin, but otherwise uncategorized. Adapted from Glossary of geology (5th edition revised; Neuendorf et al., 2011)"@en ;
    skos:historyNote "Compiled by the Geological Survey of Western Australia" ;
    skos:inScheme cs: ;
    skos:notation "s"^^:gswa-rock-code ;
    skos:prefLabel "siliciclastic rock"@en ;
    schema:citation
        "https://glossary.americangeosciences.org/term/clastic"^^xsd:anyURI ,
        "https://glossary.americangeosciences.org/term/siliciclastic"^^xsd:anyURI ;
.

:siliciclastic-rock-undivided
    a skos:Concept ;
    rdfs:isDefinedBy cs: ;
    skos:broader :sedimentary-siliciclastic ;
    skos:definition "A sedimentary rock that is silicon-bearing (in the form of quartz and silicates) and is composed principally of broken fragments that are derived from pre-existing rocks or minerals and that have been transported some distance from their places of origin, but otherwise uncategorized. Adapted from Glossary of geology (5th edition revised; Neuendorf et al., 2011). GSWA usage of this term is restricted to rocks that are partially weathered or are identified using remote sensing imagery, and the use of the related code/notation is limited to GSWA's Explanatory Notes System."@en ;
    skos:historyNote "Compiled by the Geological Survey of Western Australia" ;
    skos:inScheme cs: ;
    skos:notation "sn"^^:gswa-rock-code ;
    skos:prefLabel "siliciclastic rock; undivided"@en ;
.

:siliciclastic-schist
    a skos:Concept ;
    rdfs:isDefinedBy cs: ;
    skos:broader :metasedimentary-siliciclastic ;
    skos:definition "A metamorphosed siliciclastic rock displaying a schistose structure, i.e. a schist derived from a clastic sedimentary protolith and largely consisting of silicates and quartz. See also definition of schist/schistose structure in Fettes and Desmons, 2007, p. 193)."@en ;
    skos:historyNote "Based on the IUGS classification of metamorphic rocks (Fettes and Desmons, 2007)." ;
    skos:inScheme cs: ;
    skos:notation "mds"^^:gswa-rock-code ;
    skos:prefLabel "siliciclastic schist"@en ;
.

:siliciclastic-with-lesser-carbonate
    a skos:Concept ;
    rdfs:isDefinedBy cs: ;
    skos:broader :sedimentary-siliciclastic ;
    skos:definition "Siliciclastic rocks/beds/intervals and subordinate carbonate rocks/beds/intervals interleaved at outcrop scale."@en ;
    skos:historyNote "Compiled by the Geological Survey of Western Australia" ;
    skos:inScheme cs: ;
    skos:notation "sk"^^:gswa-rock-code ;
    skos:prefLabel "siliciclastic + lesser carbonate"@en ;
.

:silicified-meta-igneous-felsic-rock
    a skos:Concept ;
    rdfs:isDefinedBy cs: ;
    skos:broader :meta-igneous-felsic ;
    skos:definition "An igneous felsic rock affected by silicification, i.e. hydrothermal alteration resulting in a net addition of silica to the rock, for which an intrusive, extrusive or volcaniclastic protolith cannot be conclusively identified. There is no implication on the timing of alteration relative to other metamorphic processes (e.g. regional metamorphism) that may have affected the rock."@en ;
    skos:historyNote "Compiled by the Geological Survey of Western Australia" ;
    skos:inScheme cs: ;
    skos:notation "mrq"^^:gswa-rock-code ;
    skos:prefLabel "silicified meta-igneous felsic rock"@en ;
.

:silicified-meta-igneous-mafic-rock
    a skos:Concept ;
    rdfs:isDefinedBy cs: ;
    skos:broader :meta-igneous-mafic ;
    skos:definition "An igneous mafic rock affected by silicification, i.e. hydrothermal alteration resulting in a net addition of silica to the rock, for which an intrusive, extrusive or volcaniclastic protolith cannot be conclusively identified. There is no implication on the timing of alteration relative to other metamorphic processes (e.g. regional metamorphism) that may have affected the rock."@en ;
    skos:historyNote "Compiled by the Geological Survey of Western Australia" ;
    skos:inScheme cs: ;
    skos:notation "mwq"^^:gswa-rock-code ;
    skos:prefLabel "silicified meta-igneous mafic rock"@en ;
.

:silicified-meta-iron-formation
    a skos:Concept ;
    rdfs:isDefinedBy cs: ;
    skos:altLabel
        "itabirite"@en ,
        "taconite"@en ;
    skos:broader :metasedimentary-other-chemical-meta-iron-formation ;
    skos:definition "An iron formation affected by silicification, i.e. hydrothermal alteration resulting in a net addition of silica to the rock. There is no implication on the timing of alteration relative to other metamorphic processes (e.g. regional metamorphism) that may have affected the rock."@en ;
    skos:historyNote "Compiled by the Geological Survey of Western Australia" ;
    skos:inScheme cs: ;
    skos:notation "miq"^^:gswa-rock-code ;
    skos:prefLabel "silicified meta-iron formation"@en ;
.

:silicified-meta-ultramafic-intrusive-rock
    a skos:Concept ;
    rdfs:isDefinedBy cs: ;
    skos:broader :meta-igneous-ultramafic-intrusive ;
    skos:definition "An ultramafic igneous (intrusive or coarse-grained extrusive) rock affected by silicification, i.e. hydrothermal alteration resulting in a net addition of silica to the rock. There is no implication on the timing of alteration relative to other metamorphic processes (e.g. regional metamorphism) that may have affected the rock."@en ;
    skos:historyNote "Compiled by the Geological Survey of Western Australia" ;
    skos:inScheme cs: ;
    skos:notation "maq"^^:gswa-rock-code ;
    skos:prefLabel "silicified meta-ultramafic intrusive rock"@en ;
    schema:citation "https://glossary.americangeosciences.org/term/silicificationmeta"^^xsd:anyURI ;
.

:silicified-meta-ultramafic-rock
    a skos:Concept ;
    rdfs:isDefinedBy cs: ;
    skos:broader :meta-igneous-ultramafic-volcanic ;
    skos:definition "An ultramafic volcanic or volcaniclastic rock affected by silicification, i.e. hydrothermal alteration resulting in a net addition of silica to the rock. There is no implication on the timing of alteration relative to other metamorphic processes (e.g. regional metamorphism) that may have affected the rock."@en ;
    skos:historyNote "Compiled by the Geological Survey of Western Australia" ;
    skos:inScheme cs: ;
    skos:notation "muq"^^:gswa-rock-code ;
    skos:prefLabel "silicified meta-ultramafic rock"@en ;
.

:silicified-metacarbonatite
    a skos:Concept ;
    rdfs:isDefinedBy cs: ;
    skos:broader :meta-igneous-carbonatite ;
    skos:definition "A metamorphosed carbonatite affected by silicification, i.e. hydrothermal alteration resulting in a net addition of silica to the rock. There is no implication on the timing of alteration relative to other metamorphic processes (e.g. regional metamorphism) that may have affected the rock."@en ;
    skos:inScheme cs: ;
    skos:notation "mqq"^^:gswa-rock-code ;
    skos:prefLabel "silicified metacarbonatite"@en ;
.

:silicified-metachert
    a skos:Concept ;
    rdfs:isDefinedBy cs: ;
    skos:broader :metasedimentary-other-chemical ;
    skos:definition "A chert affected by silicification, i.e. hydrothermal alteration resulting in a net addition of silica to the rock. There is no implication on the timing of alteration relative to other metamorphic processes (e.g. regional metamorphism) that may have affected the rock."@en ;
    skos:historyNote "Compiled by the Geological Survey of Western Australia" ;
    skos:inScheme cs: ;
    skos:notation "mcq"^^:gswa-rock-code ;
    skos:prefLabel "silicified metachert"@en ;
    schema:citation "https://glossary.americangeosciences.org/term/silicificationmeta"^^xsd:anyURI ;
.

:silicified-metaconglomerate
    a skos:Concept ;
    rdfs:isDefinedBy cs: ;
    skos:broader :metasedimentary-siliciclastic-psephite ;
    skos:definition "A metamorphosed conglomerate affected by silicification, i.e. hydrothermal alteration resulting in a net addition of silica to the rock. There is no implication on the timing of alteration relative to other metamorphic processes (e.g. regional metamorphism) that may have affected the rock."@en ;
    skos:historyNote "Compiled by the Geological Survey of Western Australia" ;
    skos:inScheme cs: ;
    skos:notation "mxq"^^:gswa-rock-code ;
    skos:prefLabel "silicified metaconglomerate"@en ;
    schema:citation "https://glossary.americangeosciences.org/term/psephite"^^xsd:anyURI ;
.

:silicified-metafelsic-volcanic-rock
    a skos:Concept ;
    rdfs:isDefinedBy cs: ;
    skos:broader :meta-igneous-felsic-volcanic ;
    skos:definition "A felsic igneous volcanic rock affected by silicification, i.e. hydrothermal alteration resulting in a net addition of silica to the rock. There is no implication on the timing of alteration relative to other metamorphic processes (e.g. regional metamorphism) that may have affected the rock. GSWA usage restricts the term to those occurrences whereby a more specific lithology (e.g. metarhyolite) cannot be identified. GSWA's rock classification scheme prefers the use of volcanic terminology for any igneous rock formed on or near the Earth's surface, i.e. for those hypabyssal or subvolcanic rocks such as dykes, sills, and cryptodomes that are demonstrably both spatially and temporally associated with extrusive volcanic rocks."@en ;
    skos:historyNote "Compiled by the Geological Survey of Western Australia" ;
    skos:inScheme cs: ;
    skos:notation "mfq"^^:gswa-rock-code ;
    skos:prefLabel "silicified metafelsic volcanic rock"@en ;
.

:silicified-metagranitic-rock
    a skos:Concept ;
    rdfs:isDefinedBy cs: ;
    skos:broader :meta-igneous-felsic-intrusive ;
    skos:definition "A felsic intrusive rock affected by silicification, i.e. hydrothermal alteration resulting in a net addition of silica to the rock. There is no implication on the timing of alteration relative to other metamorphic processes (e.g. regional metamorphism) that may have affected the rock. GSWA usage restricts the term to those occurrences whereby a more specific lithology (e.g. metasyenite) cannot be identified."@en ;
    skos:historyNote "Compiled by the Geological Survey of Western Australia" ;
    skos:inScheme cs: ;
    skos:notation "mgq"^^:gswa-rock-code ;
    skos:prefLabel "silicified metagranitic rock"@en ;
.

:silicified-metamafic-intrusive-rock
    a skos:Concept ;
    rdfs:isDefinedBy cs: ;
    skos:broader :meta-igneous-mafic-intrusive ;
    skos:definition "A mafic intrusive rock affected by silicification, i.e. hydrothermal alteration resulting in a net addition of silica to the rock. There is no implication on the timing of alteration relative to other metamorphic processes (e.g. regional metamorphism) that may have affected the rock. GSWA usage restricts the term to those occurrences whereby a more specific lithology (e.g. metagabbro) cannot be identified."@en ;
    skos:historyNote "Compiled by the Geological Survey of Western Australia" ;
    skos:inScheme cs: ;
    skos:notation "moq"^^:gswa-rock-code ;
    skos:prefLabel "silicified metamafic intrusive rock"@en ;
.

:silicified-metamafic-volcanic-rock
    a skos:Concept ;
    rdfs:isDefinedBy cs: ;
    skos:broader :meta-igneous-mafic-volcanic ;
    skos:definition "A mafic volcanic rock affected by silicification, i.e. hydrothermal alteration resulting in a net addition of silica to the rock. There is no implication on the timing of alteration relative to other metamorphic processes (e.g. regional metamorphism) that may have affected the rock. GSWA usage restricts the term to those occurrences whereby a more specific lithology (e.g. metabasalt) cannot be identified."@en ;
    skos:historyNote "Compiled by the Geological Survey of Western Australia" ;
    skos:inScheme cs: ;
    skos:notation "mbq"^^:gswa-rock-code ;
    skos:prefLabel "silicified metamafic volcanic rock"@en ;
    schema:citation "https://glossary.americangeosciences.org/term/silicificationmeta"^^xsd:anyURI ;
.

:silicified-metasiliciclastic-rock
    a skos:Concept ;
    rdfs:isDefinedBy cs: ;
    skos:broader :metasedimentary-siliciclastic ;
    skos:definition "A siliciclastic rock affected by silicification, i.e. hydrothermal alteration resulting in a net addition of silica to the rock. There is no implication on the timing of alteration relative to other metamorphic processes (e.g. regional metamorphism) that may have affected the rock."@en ;
    skos:historyNote "Compiled by the Geological Survey of Western Australia" ;
    skos:inScheme cs: ;
    skos:notation "mdq"^^:gswa-rock-code ;
    skos:prefLabel "silicified metasiliciclastic rock"@en ;
    schema:citation "https://glossary.americangeosciences.org/term/silicificationmeta"^^xsd:anyURI ;
.

:silicified-metavolcanic-or-metavolcaniclastic-rock
    a skos:Concept ;
    rdfs:isDefinedBy cs: ;
    skos:broader :meta-igneous-volcanic-or-volcaniclastic ;
    skos:definition "A metamorphosed volcanic or volcaniclastic rock otherwise uncategorized and affected by silicification, i.e. hydrothermal alteration resulting in a net addition of silica to the rock. There is no implication on the timing of alteration relative to other metamorphic processes (e.g. regional metamorphism) that may have affected the rock."@en ;
    skos:historyNote "Compiled by the Geological Survey of Western Australia" ;
    skos:inScheme cs: ;
    skos:notation "mvq"^^:gswa-rock-code ;
    skos:prefLabel "silicified metavolcanic or metavolcaniclastic rock"@en ;
.

:silicified-pelite
    a skos:Concept ;
    rdfs:isDefinedBy cs: ;
    skos:broader :metasedimentary-siliciclastic-pelite ;
    skos:definition "A metamorphosed fine-grained siliciclastic rock, otherwise uncategorized, affected by silicification, i.e. hydrothermal alteration resulting in a net addition of silica to the rock. There is no implication on the timing of alteration relative to other metamorphic processes (e.g. regional metamorphism) that may have affected the rock."@en ;
    skos:historyNote "Compiled by the Geological Survey of Western Australia" ;
    skos:inScheme cs: ;
    skos:notation "mlq"^^:gswa-rock-code ;
    skos:prefLabel "silicified pelite"@en ;
    schema:citation "https://glossary.americangeosciences.org/term/pelite"^^xsd:anyURI ;
.

:silicified-psammite-and-pelite-interlayered
    a skos:Concept ;
    rdfs:isDefinedBy cs: ;
    skos:broader :metasedimentary-siliciclastic-psammite-and-pelite-interlayered ;
    skos:definition "A succession of sandstone and mudstone beds affected by silicification, i.e. hydrothermal alteration resulting in a net addition of silica to the rock. There is no implication on the timing of alteration relative to other metamorphic processes (e.g. regional metamorphism) that may have affected the rock."@en ;
    skos:historyNote "Compiled by the Geological Survey of Western Australia" ;
    skos:inScheme cs: ;
    skos:notation "mhq"^^:gswa-rock-code ;
    skos:prefLabel "silicified psammite and pelite; interlayered"@en ;
    schema:citation
        "https://glossary.americangeosciences.org/term/pelite"^^xsd:anyURI ,
        "https://glossary.americangeosciences.org/term/psammite"^^xsd:anyURI ;
.

:silicified-semipelite
    a skos:Concept ;
    rdfs:isDefinedBy cs: ;
    skos:broader :metasedimentary-siliciclastic-semipelite ;
    skos:definition "A metamorphosed fine- to medium-grained siliciclastic rock, otherwise uncategorized, affected by silicification, i.e. hydrothermal alteration resulting in a net addition of silica to the rock. There is no implication on the timing of alteration relative to other metamorphic processes (e.g. regional metamorphism) that may have affected the rock."@en ;
    skos:historyNote "Compiled by the Geological Survey of Western Australia" ;
    skos:inScheme cs: ;
    skos:notation "mmq"^^:gswa-rock-code ;
    skos:prefLabel "silicified semipelite"@en ;
.

:siltstone
    a skos:Concept ;
    rdfs:isDefinedBy cs: ;
    skos:altLabel
        "argillite"@en ,
        "siltite"@en ;
    skos:broader :mudstone ;
    skos:definition "An indurated mud in which silt predominates over clay (clay less than 66%). Siltstone has the grain size and composition of shale but lacks its fine lamination or fissility; it tends to be flaggy, containing hard, durable, generally thin layers, and commonly shows various primary current structures. Adapted from Glossary of geology (5th edition revised; Neuendorf et al., 2011)."@en ;
    skos:historyNote "Pettijohn, FJ 1957, Sedimentary rocks, Harper and Brothers, New York, 718p." ;
    skos:inScheme cs: ;
    skos:notation "slt"^^:gswa-rock-code ;
    skos:prefLabel "siltstone"@en ;
    schema:citation "https://glossary.americangeosciences.org/term/siltstone"^^xsd:anyURI ;
.

:siltstone-with-sandstone
    a skos:Concept ;
    rdfs:isDefinedBy cs: ;
    skos:broader :sedimentary-siliciclastic ;
    skos:definition "Siltstone and sandstone beds/intervals interleaved at outcrop scale."@en ;
    skos:historyNote "Compiled by the Geological Survey of Western Australia" ;
    skos:inScheme cs: ;
    skos:notation "sf"^^:gswa-rock-code ;
    skos:prefLabel "siltstone + sandstone"@en ;
.

:slate
    a skos:Concept ;
    rdfs:isDefinedBy cs: ;
    skos:broader :metasedimentary-siliciclastic-pelite ;
    skos:definition "Ultrafine- or very fine-grained metamorphic rock displaying slaty cleavage, i.e. a type of continuous cleavage in which the individual grains are too small to be seen by the unaided eye. Slate is usually of very low metamorphic grade, although it may also occur under low-grade conditions. (Fettes and Desmons, 2007, p.–195)"@en ;
    skos:historyNote "Based on the IUGS classification of metamorphic rocks (Fettes and Desmons, 2007)." ;
    skos:inScheme cs: ;
    skos:notation "mlv"^^:gswa-rock-code ;
    skos:prefLabel "slate"@en ;
    schema:citation "https://glossary.americangeosciences.org/term/slate"^^xsd:anyURI ;
.

:spessartite
    a skos:Concept ;
    rdfs:isDefinedBy cs: ;
    skos:broader :igneous-lamprophyres ;
    skos:definition "A variety of lamprophyre consisting of phenocrysts of hornblende with or without biotite, olivine or pyroxene in a groundmass of the same minerals plus plagioclase and subordinate alkali feldspar. Now defined in the lamprophyre classification (Table 2.9, p. 19). (Le Maitre et al., 2005, p. 144)"@en ;
    skos:historyNote "Based on the IUGS classification of igneous rocks (Le Maitre et al., 2005)." ;
    skos:inScheme cs: ;
    skos:notation "ys"^^:gswa-rock-code ;
    skos:prefLabel "spessartite"@en ;
.

:spongolite-spicularite
    a skos:Concept ;
    rdfs:isDefinedBy cs: ;
    skos:broader :sedimentary-other-chemical-or-biochemical ;
    skos:definition "A sediment or rock composed principally of the remains of sponges. A sediment predominantly composed of discrete spicules is termed a spicularite, whereas one predominantly composed of rigid bodied sponges is termed a spongolite. Adapted from Gammon (1978) and Glossary of geology (5th edition revised; Neuendorf et al., 2011)."@en ;
    skos:historyNote "Gammon, PR, 1978, Spiculites and spongolites: in Sedimentology, Encyclopedia of Earth Science, Springer Berlin Heidelberg, p. 1130–1134. doi.org/10.1007/3-540-31079-7_219." ;
    skos:inScheme cs: ;
    skos:notation "cs"^^:gswa-rock-code ;
    skos:prefLabel "spongolite/spicularite"@en ;
    schema:citation "https://glossary.americangeosciences.org/term/spongolite"^^xsd:anyURI ;
.

:stromatoporoid-dolomite
    a skos:Concept ;
    rdfs:isDefinedBy cs: ;
    skos:broader :dolomite ;
    skos:definition "A dolomite rock distinguished by the presence of stromatoporoids, i.e. extinct sessile, benthic, reef-forming sponges with calcareous skeletons that were especially abundant from the Paleozoic to the Cretaceous periods."@en ;
    skos:historyNote "Stearn, CL 2015, Paleozoic Stromatoporoidea: general introduction in Selden, PA (ed.), Treatise on Invertebrate Paleontology. Part E (Revised), Porifera, vol. 5: The University of Kansas Paleontological Institute, Lawrence, Kansas, USA, p. 417–418." ;
    skos:inScheme cs: ;
    skos:notation "kdt"^^:gswa-rock-code ;
    skos:prefLabel "stromatoporoid dolomite"@en ;
    schema:citation "https://glossary.americangeosciences.org/term/stromatoporoid"^^xsd:anyURI ;
.

:stromatoporoid-limestone
    a skos:Concept ;
    rdfs:isDefinedBy cs: ;
    skos:broader :limestone ;
    skos:definition "A limestone distinguished by the presence of stromatoporoids, i.e. extinct sessile, benthic, reef-forming sponges with calcareous skeletons that were especially abundant from the Paleozoic to the Cretaceous periods."@en ;
    skos:historyNote "Stearn, CL 2015, Paleozoic Stromatoporoidea: general introduction in Selden, PA (ed.), Treatise on Invertebrate Paleontology. Part E (Revised), Porifera, vol. 5: The University of Kansas Paleontological Institute, Lawrence, Kansas, USA, p. 417–418." ;
    skos:inScheme cs: ;
    skos:notation "klt"^^:gswa-rock-code ;
    skos:prefLabel "stromatoporoid limestone"@en ;
    schema:citation "https://glossary.americangeosciences.org/term/stromatoporoid"^^xsd:anyURI ;
.

:sub-bituminous-coal
    a skos:Concept ;
    rdfs:isDefinedBy cs: ;
    skos:altLabel
        "gloss coal"@en ,
        "metalignitous coal"@en ;
    skos:broader :coal ;
    skos:definition "A black coal, intermediate in rank between lignite and bituminous coals or, in some classifications, the equivalent of black lignite. It is distinguished from lignite by higher carbon and lower moisture content. Further classification of sub-bituminous coal is made on the basis of calorific value. Adapted from Glossary of geology (5th edition revised; Neuendorf et al., 2011)."@en ;
    skos:historyNote "Forsman, JP and Hunt, JM 1958, Insoluble organic matter (kerogen) in sedimentary rocks: Geochimica et Cosmochimica Acta, v. 15(3), p. 170–182, doi.org/10.1016/0016-7037(58)90055-3." ;
    skos:inScheme cs: ;
    skos:notation "cob"^^:gswa-rock-code ;
    skos:prefLabel "sub-bituminous coal"@en ;
    schema:citation "https://glossary.americangeosciences.org/term/subbituminouscoal"^^xsd:anyURI ;
.

:subarkose
    a skos:Concept ;
    rdfs:isDefinedBy cs: ;
    skos:altLabel
        "feldspathic arenite"@en ,
        "feldspathic sandstone"@en ;
    skos:broader :arkose ;
    skos:definition "An arenite that does not have enough feldspar to be classed as an arkose, or that is intermediate in composition between arkose and quartzarenite. Subarkose specifically contains 75–95% quartz and chert, and 5–25% unstable materials in which the ratio of feldspar:lithic grains is greater than 1:1. Adapted from Glossary of geology (5th edition revised; Neuendorf et al., 2011)."@en ;
    skos:historyNote "Pettijohn, FJ 1975, Sedimentary Rocks: New York, Harper and Row, 628p." ;
    skos:inScheme cs: ;
    skos:notation "sja"^^:gswa-rock-code ;
    skos:prefLabel "subarkose"@en ;
    schema:citation "https://glossary.americangeosciences.org/term/subarkose"^^xsd:anyURI ;
.

:sublitharenite
    a skos:Concept ;
    rdfs:isDefinedBy cs: ;
    skos:broader :arenite ;
    skos:definition "An arenite that is intermediate in composition between a litharenite and a quartzarenite; specifically containing 5–25% rock/lithic grains and a feldspar:lithic ratio less than 1:1. Adapted from Glossary of geology (5th edition revised; Neuendorf et al., 2011)."@en ;
    skos:historyNote "Pettijohn, FJ 1975, Sedimentary Rocks: New York, Harper and Row, 628p." ;
    skos:inScheme cs: ;
    skos:notation "sat"^^:gswa-rock-code ;
    skos:prefLabel "sublitharenite"@en ;
    schema:citation "https://glossary.americangeosciences.org/term/sublitharenite"^^xsd:anyURI ;
.

:suevite
    a skos:Concept ;
    rdfs:isDefinedBy cs: ;
    skos:altLabel
        "suevite breccia"@en ,
        "suevitic impact breccia"@en ;
    skos:broader :impact-breccia ;
    skos:definition "Polymictic impact breccia with particulate matrix containing lithic and mineral clasts in all stages of shock metamorphism including cogenetic impact melt particles, which are in a glassy or crystallized state (Fettes and Desmons, 2007, p. 198)."@en ;
    skos:historyNote "Based on the IUGS classification of metamorphic rocks (Fettes and Desmons, 2007)." ;
    skos:inScheme cs: ;
    skos:notation "mpu"^^:gswa-rock-code ;
    skos:prefLabel "suevite"@en ;
    schema:citation "https://glossary.americangeosciences.org/term/suevite"^^xsd:anyURI ;
.

:syenite
    a skos:Concept ;
    rdfs:isDefinedBy cs: ;
    skos:broader :igneous-felsic-intrusive ;
    skos:definition "An intrusive rock consisting mainly of alkali feldspar with subordinate sodic plagioclase, biotite, pyroxene, amphibole and occasional fayalite. Minor quartz or nepheline may also be present. Now defined modally in QAPF field 7 (Fig. 2.4, p. 22). (cf. Le Maitre et al., 2005, p. 145)"@en ;
    skos:exactMatch
        <http://inspire.ec.europa.eu/codelist/LithologyValue/syenite> ,
        <http://resource.geosciml.org/classifier/cgi/lithology/syenite> ;
    skos:historyNote "Based on the IUGS classification of igneous rocks (Le Maitre et al., 2005)." ;
    skos:inScheme cs: ;
    skos:notation "gy"^^:gswa-rock-code ;
    skos:prefLabel "syenite"@en ;
    schema:citation "https://glossary.americangeosciences.org/term/syenite"^^xsd:anyURI ;
.

:syenogranite
    a skos:Concept ;
    rdfs:isDefinedBy cs: ;
    skos:broader :igneous-felsic-intrusive ;
    skos:definition "An optional term for a variety of granite in QAPF field 3a (Fig. 2.4, p. 22) consisting of alkali feldspar with subordinate plagioclase (Le Maitre et al., 2005, p. 146)."@en ;
    skos:exactMatch
        <http://inspire.ec.europa.eu/codelist/LithologyValue/syenogranite> ,
        <http://resource.geosciml.org/classifier/cgi/lithology/syenogranite> ;
    skos:historyNote "Based on the IUGS classification of igneous rocks (Le Maitre et al., 2005)." ;
    skos:inScheme cs: ;
    skos:notation "gr"^^:gswa-rock-code ;
    skos:prefLabel "syenogranite"@en ;
    schema:citation "https://glossary.americangeosciences.org/term/syenogranite"^^xsd:anyURI ;
.

:tektite
    a skos:Concept ;
    rdfs:isDefinedBy cs: ;
    skos:broader :distal-impactite ;
    skos:definition "Impact glass formed at terrestrial impact craters from melt ejected ballistically and deposited as aerodynamically shaped bodies in a strewn field outside the continuous ejecta blanket. The size of tektites ranges from the submillimetre range (microtektites, generally found in deep sea sediments) to the subdecimetre range, rarely to decimetres. (Fettes and Desmons, 2007, p.  200)"@en ;
    skos:historyNote "Based on the IUGS classification of metamorphic rocks (Fettes and Desmons, 2007)." ;
    skos:inScheme cs: ;
    skos:notation "mpk"^^:gswa-rock-code ;
    skos:prefLabel "tektite"@en ;
    schema:citation "https://glossary.americangeosciences.org/term/tektite"^^xsd:anyURI ;
.

:tonalite
    a skos:Concept ;
    rdfs:isDefinedBy cs: ;
    skos:broader :igneous-felsic-intrusive ;
    skos:definition "An intrusive rock consisting essentially of quartz and intermediate plagioclase, usually with biotite and amphibole. Now defined modally in QAPF field 5 (Fig. 2.4, p. 22). (cf. Le Maitre et al., 2005, p. 149)"@en ;
    skos:exactMatch
        <http://inspire.ec.europa.eu/codelist/LithologyValue/tonalite> ,
        <http://resource.geosciml.org/classifier/cgi/lithology/tonalite> ;
    skos:historyNote "Based on the IUGS classification of igneous rocks (Le Maitre et al., 2005)." ;
    skos:inScheme cs: ;
    skos:notation "gt"^^:gswa-rock-code ;
    skos:prefLabel "tonalite"@en ;
    schema:citation "https://glossary.americangeosciences.org/term/tonalite"^^xsd:anyURI ;
.

:tourmaline-vein
    a skos:Concept ;
    rdfs:isDefinedBy cs: ;
    skos:broader :hydrothermal ;
    skos:definition "A rock comprising tourmaline crystals of pegmatitic or hydrothermal origin, as vein-filling material."@en ;
    skos:historyNote "Compiled by the Geological Survey of Western Australia" ;
    skos:inScheme cs: ;
    skos:notation "zt"^^:gswa-rock-code ;
    skos:prefLabel "tourmaline vein"@en ;
.

:trachyte
    a skos:Concept ;
    rdfs:isDefinedBy cs: ;
    skos:broader :igneous-felsic-volcanic ;
    skos:definition "A volcanic rock consisting essentially of alkali feldspar. Now defined modally in QAPF field 7 (Fig. 2.11, p. 31) and, if modes are not available, chemically in TAS field T (Fig. 2.14, p. 35). Definition from Le Maitre et al. (2005, p. 151). GSWA's rock classification scheme prefers the use of volcanic terminology for any igneous rock formed on or near the Earth's surface, i.e. for those hypabyssal or subvolcanic rocks such as dykes, sills, and cryptodomes that are demonstrably both spatially and temporally associated with extrusive volcanic rocks."@en ;
    skos:exactMatch
        <http://inspire.ec.europa.eu/codelist/LithologyValue/trachyte> ,
        <http://resource.geosciml.org/classifier/cgi/lithology/trachyte> ;
    skos:historyNote "Based on the IUGS classification of igneous rocks (Le Maitre et al., 2005)." ;
    skos:inScheme cs: ;
    skos:notation "ft"^^:gswa-rock-code ;
    skos:prefLabel "trachyte"@en ;
.

:travertine
    a skos:Concept ;
    rdfs:isDefinedBy cs: ;
    skos:altLabel
        "calc-sinter"@en ,
        "calcareous sinter"@en ,
        "meteogenic travertine"@en ,
        "tufa"@en ;
    skos:broader :sedimentary-other-chemical-or-biochemical ;
    skos:definition "Biotically and/or abiotically precipitated calcium carbonate (predominantly calcite and aragonite) from spring-fed, heated and/or ambient-temperature waters. The spongy or less compact variety is named tufa. Adapted from Glossary of geology (5th edition revised; Neuendorf et al., 2011)."@en ;
    skos:exactMatch
        <http://inspire.ec.europa.eu/codelist/LithologyValue/travertine> ,
        <http://resource.geosciml.org/classifier/cgi/lithology/travertine> ;
    skos:historyNote "Based on the Glossary of geology (5th edition, revised; Neuendorf et al. 2011)." ;
    skos:inScheme cs: ;
    skos:notation "ct"^^:gswa-rock-code ;
    skos:prefLabel "travertine"@en ;
    schema:citation "https://glossary.americangeosciences.org/term/travertine"^^xsd:anyURI ;
.

:troctolite
    a skos:Concept ;
    rdfs:isDefinedBy cs: ;
    skos:broader :igneous-mafic-intrusive ;
    skos:definition "A variety of gabbro composed essentially of highly calcic plagioclase and olivine with little or no pyroxene. Now defined modally in the gabbroic rock classification (Fig. 2.6, p. 25). (Le Maitre et al., 2005, p. 151)"@en ;
    skos:historyNote "Based on the IUGS classification of igneous rocks (Le Maitre et al., 2005)." ;
    skos:inScheme cs: ;
    skos:notation "ot"^^:gswa-rock-code ;
    skos:prefLabel "troctolite"@en ;
    schema:citation "https://glossary.americangeosciences.org/term/troctolite"^^xsd:anyURI ;
.

:trondjhemite
    a skos:Concept ;
    rdfs:isDefinedBy cs: ;
    skos:altLabel
        "leucocratic tonalite"@en ,
        "plagiogranite;"@en ;
    skos:broader :igneous-felsic-intrusive ;
    skos:definition "A leucocratic variety of tonalite consisting essentially of sodic plagioclase and quartz with minor biotite. Orthoclase is characteristically absent and hornblende is rare. May be used as a synonym for plagiogranite and leucocratic tonalite of QAPF field 5 (p. 23). (Le Maitre et al., 2005, p. 152)"@en ;
    skos:historyNote "Based on the IUGS classification of igneous rocks (Le Maitre et al., 2005)." ;
    skos:inScheme cs: ;
    skos:notation "gj"^^:gswa-rock-code ;
    skos:prefLabel "trondhjemite"@en ;
    schema:citation "https://glossary.americangeosciences.org/term/trondhjemite"^^xsd:anyURI ;
.

:ultracataclasite
    a skos:Concept ;
    rdfs:isDefinedBy cs: ;
    skos:broader :metamorphic-protolith-unknown-fault-rock ;
    skos:definition "A cohesive fault rock with a poorly developed or absent schistosity, characterized by generally angular porphyroclasts and lithic fragments in a finer-grained matrix of similar composition that constitutes more than 90% of the rock volume. Definition adapted from Fossen (2016) and Fettes and Desmons (2007, p. 202)."@en ;
    skos:historyNote "Fossen, H 2016, Structural geology (2nd edition): Cambridge University Press, Cambridge, United Kingdom, 524p." ;
    skos:inScheme cs: ;
    skos:notation "myw"^^:gswa-rock-code ;
    skos:prefLabel "ultracataclasite"@en ;
.

:ultramafic-gneiss-derived-from-intrusive-rock
    a skos:Concept ;
    rdfs:isDefinedBy cs: ;
    skos:broader :meta-igneous-ultramafic-intrusive ;
    skos:definition "A metamorphosed ultramafic igneous (intrusive or coarse-grained extrusive) rock displaying a gneissose structure, i.e. a gneiss derived from an intrusive rock with one or more mafic minerals as the main component(s). See also definition of gneiss/gneissose structure in Fettes and Desmons (2007, p. 154–155)."@en ;
    skos:historyNote "Based on the IUGS classification of metamorphic rocks (Fettes and Desmons, 2007)." ;
    skos:inScheme cs: ;
    skos:notation "man"^^:gswa-rock-code ;
    skos:prefLabel "ultramafic gneiss derived from intrusive rock"@en ;
.

:ultramafic-gneiss-volcanic-or-undivided
    a skos:Concept ;
    rdfs:isDefinedBy cs: ;
    skos:broader :meta-igneous-ultramafic-volcanic ;
    skos:definition "A metamorphosed ultramafic volcanic or volcaniclastic rock displaying a gneissose structure, i.e. a gneiss derived from an extrusive or related rock with one or more mafic minerals as the main component(s). See also definition of gneiss/gneissose structure in Fettes and Desmons (2007, p. 154–155)."@en ;
    skos:historyNote "Based on the IUGS classification of metamorphic rocks (Fettes and Desmons, 2007)." ;
    skos:inScheme cs: ;
    skos:notation "mun"^^:gswa-rock-code ;
    skos:prefLabel "ultramafic gneiss; volcanic or undivided"@en ;
.

:ultramafic-granofels-hornfels-derived-from-intrusive-rock
    a skos:Concept ;
    rdfs:isDefinedBy cs: ;
    skos:broader :meta-igneous-ultramafic-intrusive ;
    skos:definition "A metamorphosed ultramafic igneous (intrusive or coarse-grained extrusive) rock displaying a granofelsic structure, i.e. a granofels/hornfels derived from an intrusive rock with one or more mafic minerals as the main components (adapted from Fettes and Desmons, 2007, p. 202). See also definition of granofels/granofelsic structure in Fettes and Desmons (2007, p. 156); hornfels are granofels formed by contact metamorphism (Fettes and Desmons, 2007, p. 159)."@en ;
    skos:historyNote "Based on the IUGS classification of metamorphic rocks (Fettes and Desmons, 2007)." ;
    skos:inScheme cs: ;
    skos:notation "mae"^^:gswa-rock-code ;
    skos:prefLabel "ultramafic granofels/hornfels derived from intrusive rock"@en ;
.

:ultramafic-granofels-hornfels-volcanic-or-undivided
    a skos:Concept ;
    rdfs:isDefinedBy cs: ;
    skos:broader :meta-igneous-ultramafic-volcanic ;
    skos:definition "A metamorphosed ultramafic volcanic or volcaniclastic rock displaying a granofelsic structure, i.e. a granofels/hornfels derived from an extrusive or related rock with one or more mafic minerals as the main components (adapted from Fettes and Desmons, 2007, p. 202). See also definition of granofels/granofelsic structure in Fettes and Desmons (2007, p. 156); hornfels are granofels formed by contact metamorphism (Fettes and Desmons, 2007, p. 159)."@en ;
    skos:historyNote "Based on the IUGS classification of metamorphic rocks (Fettes and Desmons, 2007)." ;
    skos:inScheme cs: ;
    skos:notation "mue"^^:gswa-rock-code ;
    skos:prefLabel "ultramafic granofels/hornfels; volcanic or undivided"@en ;
.

:ultramafic-intrusive-rock
    a skos:Concept ;
    rdfs:isDefinedBy cs: ;
    skos:broadMatch
        <http://inspire.ec.europa.eu/codelist/LithologyValue/ultramaficIgneousRock> ,
        <http://resource.geosciml.org/classifier/cgi/lithology/ultramafic_igneous_rock> ;
    skos:broader :igneous-ultramafic-intrusive ;
    skos:definition "Originally a term for a rock consisting essentially of mafic minerals, e.g. peridotite, dunite. Now defined as a rock with M>90%. Adapted from Le Maitre et al. (2005, p. 21 and p. 153)."@en ;
    skos:historyNote "Based on the IUGS classification of igneous rocks (Le Maitre et al., 2005)." ;
    skos:inScheme cs: ;
    skos:notation "a"^^:gswa-rock-code ;
    skos:prefLabel "ultramafic intrusive rock"@en ;
.

:ultramafic-intrusive-rock-undivided
    a skos:Concept ;
    rdfs:isDefinedBy cs: ;
    skos:broader :igneous-ultramafic-intrusive ;
    skos:definition "A demonstrably ultramafic (M>90%) intrusive rock, otherwise uncategorized. GSWA usage of this term is restricted to rocks that are partially weathered or are identified using remote sensing imagery, and the use of the related code/notation is limited to GSWA's Explanatory Notes System."@en ;
    skos:historyNote "Based on the IUGS classification of igneous rocks (Le Maitre et al., 2005) and GSWA usage." ;
    skos:inScheme cs: ;
    skos:notation "an"^^:gswa-rock-code ;
    skos:prefLabel "ultramafic intrusive rock; undivided"@en ;
.

:ultramafic-schist-derived-from-intrusive-rock
    a skos:Concept ;
    rdfs:isDefinedBy cs: ;
    skos:broader :meta-igneous-ultramafic-intrusive ;
    skos:definition "A metamorphosed ultramafic igneous (intrusive or coarse-grained extrusive) rock displaying a schistose structure, i.e. a schist derived from an intrusive rock with one or more mafic minerals as the main component(s). See also definition of schist/schistose structure in Fettes and Desmons, 2007, p. 193)."@en ;
    skos:historyNote "Based on the IUGS classification of metamorphic rocks (Fettes and Desmons, 2007)." ;
    skos:inScheme cs: ;
    skos:notation "mas"^^:gswa-rock-code ;
    skos:prefLabel "ultramafic schist derived from intrusive rock"@en ;
.

:ultramafic-schist-volcanic-or-undivided
    a skos:Concept ;
    rdfs:isDefinedBy cs: ;
    skos:broader :meta-igneous-ultramafic-volcanic ;
    skos:definition "A metamorphosed ultramafic volcanic or volcaniclastic rock displaying a schistose structure, i.e. a schist derived from an intrusive rock with one or more mafic minerals as the main component(s). See also definition of schist/schistose structure in Fettes and Desmons, 2007, p. 193)."@en ;
    skos:historyNote "Based on the IUGS classification of metamorphic rocks (Fettes and Desmons, 2007)." ;
    skos:inScheme cs: ;
    skos:notation "mus"^^:gswa-rock-code ;
    skos:prefLabel "ultramafic schist; volcanic or undivided"@en ;
.

:ultramafic-volcanic-rock
    a skos:Concept ;
    rdfs:isDefinedBy cs: ;
    skos:broadMatch
        <http://inspire.ec.europa.eu/codelist/LithologyValue/ultramaficIgneousRock> ,
        <http://resource.geosciml.org/classifier/cgi/lithology/ultramafic_igneous_rock> ;
    skos:broader :igneous-ultramafic-volcanic-and-volcaniclastic ;
    skos:definition "An igneous volcanic rock composed chiefly of one or more ferromagnesian, dark-coloured minerals in its mode (adapted from Glossary of geology, 5th edition revised; Neuendorf et al., 2011). Originally a term for a rock consisting essentially of mafic minerals, e.g. peridotite, dunite. Now defined as a rock with M greater than 90% (section 2.11.2, p. 28), where M represents the volume modal percentage of mafic and related minerals (Le Maitre et al., 2005, p. 4 and 153). GSWA's rock classification scheme prefers the use of volcanic terminology for any igneous rock formed on or near the Earth's surface, i.e. for those hypabyssal or subvolcanic rocks such as dykes, sills, and cryptodomes that are demonstrably both spatially and temporally associated with extrusive volcanic rocks."@en ;
    skos:historyNote "Based on the IUGS classification of igneous rocks (Le Maitre et al., 2005)." ;
    skos:inScheme cs: ;
    skos:notation "u"^^:gswa-rock-code ;
    skos:prefLabel "ultramafic volcanic rock"@en ;
.

:ultramafic-volcanic-rock-undivided
    a skos:Concept ;
    rdfs:isDefinedBy cs: ;
    skos:broader :igneous-ultramafic-volcanic-and-volcaniclastic ;
    skos:definition "A demonstrably ultramafic igneous volcanic rock, otherwise uncategorized. GSWA usage of this term is restricted to rocks that are partially weathered or are identified using remote sensing imagery, and the use of the related code/notation is limited to GSWA's Explanatory Notes System. GSWA's rock classification scheme prefers the use of volcanic terminology for any igneous rock formed on or near the Earth's surface, i.e. for those hypabyssal or subvolcanic rocks such as dykes, sills, and cryptodomes that are demonstrably both spatially and temporally associated with extrusive volcanic rocks."@en ;
    skos:historyNote "Compiled by the Geological Survey of Western Australia" ;
    skos:inScheme cs: ;
    skos:notation "un"^^:gswa-rock-code ;
    skos:prefLabel "ultramafic volcanic rock; undivided"@en ;
.

:ultramafic-volcaniclastic-breccia
    a skos:Concept ;
    rdfs:isDefinedBy cs: ;
    skos:broader :igneous-ultramafic-volcanic-and-volcaniclastic ;
    skos:definition "A volcaniclastic rock composed mostly of angular fragments greater than 2 mm in size consisting of either (a) pyroclastic detritus or (b) terrigenous volcanic detritus of epiclastic origin, and with an overall ultramafic composition. 'Volcaniclastic' includes all clastic volcanic materials formed by any process of fragmentation, dispersed by any kind of transporting agent, deposited in any environment, or mixed in any significant portion with non-volcanic fragments."@en ;
    skos:historyNote "Compiled by the Geological Survey of Western Australia" ;
    skos:inScheme cs: ;
    skos:notation "uvb"^^:gswa-rock-code ;
    skos:prefLabel "ultramafic volcaniclastic breccia"@en ;
.

:ultramafic-volcaniclastic-breccia-sandstone
    a skos:Concept ;
    rdfs:isDefinedBy cs: ;
    skos:broader :igneous-ultramafic-volcanic-and-volcaniclastic ;
    skos:definition "A volcaniclastic rock composed mostly of angular fragments ranging in size from sand (0.0625 – 2 mm) and above, consisting of either (a) pyroclastic detritus or (b) terrigenous volcanic detritus of epiclastic origin, and with an overall ultramafic composition. 'Volcaniclastic' includes all clastic volcanic materials formed by any process of fragmentation, dispersed by any kind of transporting agent, deposited in any environment, or mixed in any significant portion with non-volcanic fragments."@en ;
    skos:historyNote "Compiled by the Geological Survey of Western Australia" ;
    skos:inScheme cs: ;
    skos:notation "uvbs"^^:gswa-rock-code ;
    skos:prefLabel "ultramafic volcaniclastic breccia-sandstone"@en ;
.

:ultramafic-volcaniclastic-conglomerate
    a skos:Concept ;
    rdfs:isDefinedBy cs: ;
    skos:broader :igneous-ultramafic-volcanic-and-volcaniclastic ;
    skos:definition "A conglomerate consisting of either (a) pyroclastic detritus or (b) terrigenous volcanic detritus of epiclastic origin, and with an overall ultramafic composition. 'Volcaniclastic' includes all clastic volcanic materials formed by any process of fragmentation, dispersed by any kind of transporting agent, deposited in any environment, or mixed in any significant portion with non-volcanic fragments."@en ;
    skos:historyNote "Compiled by the Geological Survey of Western Australia" ;
    skos:inScheme cs: ;
    skos:notation "uvc"^^:gswa-rock-code ;
    skos:prefLabel "ultramafic volcaniclastic conglomerate"@en ;
.

:ultramafic-volcaniclastic-granule-pebble-breccia
    a skos:Concept ;
    rdfs:isDefinedBy cs: ;
    skos:broader :igneous-ultramafic-volcanic-and-volcaniclastic ;
    skos:definition "A breccia composed mostly of angular fragments ranging in size from granule (2–4 mm) to pebble (4–32 mm) consisting of either (a) pyroclastic detritus or (b) terrigenous volcanic detritus of epiclastic origin, and with an overall ultramafic composition. 'Volcaniclastic' includes all clastic volcanic materials formed by any process of fragmentation, dispersed by any kind of transporting agent, deposited in any environment, or mixed in any significant portion with non-volcanic fragments."@en ;
    skos:historyNote "Compiled by the Geological Survey of Western Australia" ;
    skos:inScheme cs: ;
    skos:notation "uvg"^^:gswa-rock-code ;
    skos:prefLabel "ultramafic volcaniclastic granule/pebble breccia"@en ;
.

:ultramafic-volcaniclastic-mudstone
    a skos:Concept ;
    rdfs:isDefinedBy cs: ;
    skos:broader :igneous-ultramafic-volcanic-and-volcaniclastic ;
    skos:definition "A mudstone (grain size ranging from silt to clay, i.e. less than 0.0625 mm) consisting of either (a) pyroclastic detritus or (b) terrigenous volcanic detritus of epiclastic origin, and with an overall mafic composition. 'Volcaniclastic' includes all clastic volcanic materials formed by any process of fragmentation, dispersed by any kind of transporting agent, deposited in any environment, or mixed in any significant portion with non-volcanic fragments."@en ;
    skos:historyNote "Compiled by the Geological Survey of Western Australia" ;
    skos:inScheme cs: ;
    skos:notation "uvsm"^^:gswa-rock-code ;
    skos:prefLabel "ultramafic volcaniclastic mudstone"@en ;
.

:ultramafic-volcaniclastic-rock
    a skos:Concept ;
    rdfs:isDefinedBy cs: ;
    skos:broader :igneous-ultramafic-volcanic-and-volcaniclastic ;
    skos:definition "A volcaniclastic rock consisting of either (a) pyroclastic detritus or (b) terrigenous volcanic detritus of epiclastic origin and with an overall mafic composition, but otherwise uncategorized. 'Volcaniclastic' includes all clastic volcanic materials formed by any process of fragmentation, dispersed by any kind of transporting agent, deposited in any environment, or mixed in any significant portion with non-volcanic fragments."@en ;
    skos:historyNote "Compiled by the Geological Survey of Western Australia" ;
    skos:inScheme cs: ;
    skos:notation "uvr"^^:gswa-rock-code ;
    skos:prefLabel "ultramafic volcaniclastic rock"@en ;
.

:ultramafic-volcaniclastic-sandstone
    a skos:Concept ;
    rdfs:isDefinedBy cs: ;
    skos:broader :igneous-ultramafic-volcanic-and-volcaniclastic ;
    skos:definition "A sandstone (grain size 0.0625 – 2 mm) consisting of either (a) pyroclastic detritus or (b) terrigenous volcanic detritus of epiclastic origin, and with an overall ultramafic composition. 'Volcaniclastic' includes all clastic volcanic materials formed by any process of fragmentation, dispersed by any kind of transporting agent, deposited in any environment, or mixed in any significant portion with non-volcanic fragments."@en ;
    skos:historyNote "Compiled by the Geological Survey of Western Australia" ;
    skos:inScheme cs: ;
    skos:notation "uvs"^^:gswa-rock-code ;
    skos:prefLabel "ultramafic volcaniclastic sandstone"@en ;
.

:ultramafic-volcaniclastic-sandstone-siltstone
    a skos:Concept ;
    rdfs:isDefinedBy cs: ;
    skos:broader :igneous-ultramafic-volcanic-and-volcaniclastic ;
    skos:definition "A volcaniclastic rock composed mostly of fragments ranging in size from sand (0.0625 – 2 mm) to silt (0.0039 – 0.0625 mm) of either (a) pyroclastic detritus or (b) terrigenous volcanic detritus of epiclastic origin, and with an overall ultramafic composition. 'Volcaniclastic' includes all clastic volcanic materials formed by any process of fragmentation, dispersed by any kind of transporting agent, deposited in any environment, or mixed in any significant portion."@en ;
    skos:historyNote "Compiled by the Geological Survey of Western Australia" ;
    skos:inScheme cs: ;
    skos:notation "uvss"^^:gswa-rock-code ;
    skos:prefLabel "ultramafic volcaniclastic sandstone-siltstone"@en ;
.

:ultramafic-volcaniclastic-sediment-matrix-breccia
    a skos:Concept ;
    rdfs:isDefinedBy cs: ;
    skos:broader :igneous-ultramafic-volcanic-and-volcaniclastic ;
    skos:definition "A commonly monomictic breccia of overall ultramafic composition composed of angular, coarse igneous fragments cemented by a fine-grained matrix that is clastic though not necessarily strictly sedimentary in origin. 'Volcaniclastic' includes all clastic volcanic materials formed by any process of fragmentation, dispersed by any kind of transporting agent, deposited in any environment, or mixed in any significant portion with non-volcanic fragments."@en ;
    skos:historyNote "Compiled by the Geological Survey of Western Australia" ;
    skos:inScheme cs: ;
    skos:notation "uvsb"^^:gswa-rock-code ;
    skos:prefLabel "ultramafic volcaniclastic sediment-matrix breccia"@en ;
.

:ultramylonite
    a skos:Concept ;
    rdfs:isDefinedBy cs: ;
    skos:broader :metamorphic-protolith-unknown-fault-rock ;
    skos:definition "Mylonite in which more than 90% of the rock volume has undergone grain-size reduction (Fettes and Desmons, 2007, p.  202); a mylonite with over 90% matrix and less than 10% porphyroclasts (Passchier and Trouw, 2005)."@en ;
    skos:historyNote "Passchier, CW and Trouw, RAJ 2005, Microtectonics (2nd edition): Springer, Berlin, 366p." ;
    skos:inScheme cs: ;
    skos:notation "myu"^^:gswa-rock-code ;
    skos:prefLabel "ultramylonite"@en ;
    schema:citation "https://glossary.americangeosciences.org/term/ultramylonite"^^xsd:anyURI ;
.

:unknown-lithology
    a skos:Concept ;
    rdfs:isDefinedBy cs: ;
    skos:broader :unknown ;
    skos:definition "A rock so altered, weathered or of such a fine grain size that an inference on the protolith or origin of the rock cannot be made. Also used to allocate a lithology to sample legacy data where a lithology was not known. The use of the related code/notation is limited to GSWA's Field observation database (WAROX)."@en ;
    skos:historyNote "Compiled by the Geological Survey of Western Australia" ;
    skos:inScheme cs: ;
    skos:notation "nk"^^:gswa-rock-code ;
    skos:prefLabel "unknown lithology"@en ;
.

:vein
    a skos:Concept ;
    rdfs:isDefinedBy cs: ;
    skos:broader :hydrothermal ;
    skos:definition "A distinct sheet-like body of crystallized minerals within a rock. Veins form when mineral constituents carried by an aqueous solution within the rock mass are deposited through precipitation. The hydraulic flow involved is usually due to hydrothermal circulation. (https://en.wikipedia.org/wiki/Vein_(geology))."@en ;
    skos:historyNote "Based on the Glossary of geology (5th edition, revised; Neuendorf et al. 2011)." ;
    skos:inScheme cs: ;
    skos:notation "vein"^^:gswa-rock-code ;
    skos:prefLabel "vein"@en ;
    schema:citation "https://en.wikipedia.org/wiki/Vein_(geology)"^^xsd:anyURI ;
.

:vogesite
    a skos:Concept ;
    rdfs:isDefinedBy cs: ;
    skos:broader :igneous-lamprophyres ;
    skos:definition "A variety of lamprophyre in which amphibole is more abundant than biotite and alkali feldspar is more abundant than plagioclase. Augite is frequently present. Now defined in the lamprophyre classification (Table 2.9, p. 19). (Le Maitre et al., 2005, p. 155)"@en ;
    skos:historyNote "Based on the IUGS classification of igneous rocks (Le Maitre et al., 2005)." ;
    skos:inScheme cs: ;
    skos:notation "yv"^^:gswa-rock-code ;
    skos:prefLabel "vogesite"@en ;
.

:volcanic-rock
    a skos:Concept ;
    rdfs:isDefinedBy cs: ;
    skos:broader :igneous-volcanic ;
    skos:definition "A rock of igneous volcanic/extrusive origin but commonly too weathered to make further distinctions."@en ;
    skos:historyNote "Compiled by the Geological Survey of Western Australia" ;
    skos:inScheme cs: ;
    skos:notation "ignv"^^:gswa-rock-code ;
    skos:prefLabel "volcanic rock"@en ;
.

:websterite
    a skos:Concept ;
    rdfs:isDefinedBy cs: ;
    skos:broader :igneous-ultramafic-intrusive ;
    skos:definition "A variety of pyroxenite consisting largely of varying amounts of orthopyroxene and clinopyroxene, with less than 10% olivine. Now defined modally in the ultramafic rock classification (Fig. 2.9, p. 28). Adapted from Le Maitre et al. (2005, p. 156)."@en ;
    skos:historyNote "Based on the IUGS classification of igneous rocks (Le Maitre et al., 2005)." ;
    skos:inScheme cs: ;
    skos:notation "axw"^^:gswa-rock-code ;
    skos:prefLabel "websterite"@en ;
    schema:citation "https://glossary.americangeosciences.org/term/websteriterock"^^xsd:anyURI ;
.

:wehrlite
    a skos:Concept ;
    rdfs:isDefinedBy cs: ;
    skos:broader :igneous-ultramafic-intrusive ;
    skos:definition "An ultramafic intrusive rock composed of olivine and clinopyroxene often with minor brown hornblende. Now defined modally in the ultramafic rock classification (Fig. 2.9, p. 28). (cf. Le Maitre et al., 2005, p. 156)"@en ;
    skos:historyNote "Based on the IUGS classification of igneous rocks (Le Maitre et al., 2005)." ;
    skos:inScheme cs: ;
    skos:notation "apw"^^:gswa-rock-code ;
    skos:prefLabel "wehrlite"@en ;
    schema:citation "https://glossary.americangeosciences.org/term/wehrliterock"^^xsd:anyURI ;
.

:xenolith-or-inclusion-bearing-lithology
    a skos:Concept ;
    rdfs:isDefinedBy cs: ;
    skos:broader :xenolith-or-inclusion-bearing ;
    skos:definition "A prefix used in GSWA's Explanatory Notes system (ENS) to characterize mixed lithological types (metamorphosed or not), where the first code represents the host rock lithology and the second code represents the dominant lithology of the xenolith/inclusions."@en ;
    skos:historyNote "Compiled by the Geological Survey of Western Australia" ;
    skos:inScheme cs: ;
    skos:notation "j"^^:gswa-rock-code ;
    skos:prefLabel "xenolith- or inclusion-bearing lithology"@en ;
.

:igneous
    a skos:Concept ;
    rdfs:isDefinedBy cs: ;
    skos:definition "A group name for rock types of igneous but otherwise unspecified origin, i.e. including both intrusive and extrusive types."@en ;
    skos:historyNote "Compiled by the Geological Survey of Western Australia" ;
    skos:inScheme cs: ;
    skos:narrower :igneous-rock ;
    skos:notation "ign"^^:gswa-rock-code ;
    skos:prefLabel "igneous"@en ;
    skos:topConceptOf cs: ;
.

:igneous-intrusive
    a skos:Concept ;
    rdfs:isDefinedBy cs: ;
    skos:definition "A group name for rock types of igneous intrusive origin."@en ;
    skos:historyNote "Compiled by the Geological Survey of Western Australia" ;
    skos:inScheme cs: ;
    skos:narrower :intrusive-rock ;
    skos:notation "igni"^^:gswa-rock-code ;
    skos:prefLabel "igneous intrusive"@en ;
    skos:topConceptOf cs: ;
.

:igneous-volcanic
    a skos:Concept ;
    rdfs:isDefinedBy cs: ;
    skos:definition "A group name for rock types of igneous extrusive (or volcanic) origin."@en ;
    skos:historyNote "Compiled by the Geological Survey of Western Australia" ;
    skos:inScheme cs: ;
    skos:narrower :volcanic-rock ;
    skos:notation "ignv"^^:gswa-rock-code ;
    skos:prefLabel "igneous volcanic"@en ;
    skos:topConceptOf cs: ;
.

:meta-igneous
    a skos:Concept ;
    rdfs:isDefinedBy cs: ;
    skos:definition "A group name for rock types of metamorphosed igneous but otherwise unspecified origin, i.e. including both intrusive and extrusive types."@en ;
    skos:historyNote "Compiled by the Geological Survey of Western Australia" ;
    skos:inScheme cs: ;
    skos:narrower :meta-igneous-rock ;
    skos:notation "mign"^^:gswa-rock-code ;
    skos:prefLabel "meta-igneous"@en ;
    skos:topConceptOf cs: ;
.

:metamorphic
    a skos:Concept ;
    rdfs:isDefinedBy cs: ;
    skos:definition "A group name for metamorphic rocks so deeply altered/weathered that no inference can be made as to the protolith and with no discernible structures."@en ;
    skos:historyNote "Compiled by the Geological Survey of Western Australia" ;
    skos:inScheme cs: ;
    skos:narrower :metamorphic-rock ;
    skos:notation "m"^^:gswa-rock-code ;
    skos:prefLabel "metamorphic"@en ;
    skos:topConceptOf cs: ;
.

:metamorphic-protolith-unknown
    a skos:Concept ;
    rdfs:isDefinedBy cs: ;
    skos:definition "A group name for metamorphosed rocks for which the protolith cannot be identified."@en ;
    skos:historyNote "Compiled by the Geological Survey of Western Australia" ;
    skos:inScheme cs: ;
    skos:narrower :migmatite-protolith-unknown ;
    skos:notation "met"^^:gswa-rock-code ;
    skos:prefLabel "metamorphic: protolith unknown"@en ;
    skos:topConceptOf cs: ;
.

:metamorphosed-quartz-vein
    a skos:Concept ;
    rdfs:isDefinedBy cs: ;
    skos:broader :metamorphosed-hydrothermal ;
    skos:definition "A metamorphosed rock comprising quartz crystals of hydrothermal origin as vein-filling material."@en ;
    skos:historyNote "Compiled by the Geological Survey of Western Australia" ;
    skos:inScheme cs: ;
    skos:narrower :foliated-quartz-vein ;
    skos:notation "mzq"^^:gswa-rock-code ;
    skos:prefLabel "metamorphosed quartz vein"@en ;
    schema:citation
        "https://glossary.americangeosciences.org/term/veinquartz"^^xsd:anyURI ,
        "https://glossary.americangeosciences.org/term/veinstrucgeol"^^xsd:anyURI ;
.

:metasedimentary
    a skos:Concept ;
    rdfs:isDefinedBy cs: ;
    skos:definition "A group name for metamorphosed rocks of sedimentary but otherwise unspecified origin, i.e. a rock for which a clastic or chemical/biochemical derivation cannot be conclusively established."@en ;
    skos:historyNote "Compiled by the Geological Survey of Western Australia" ;
    skos:inScheme cs: ;
    skos:narrower :metasedimentary-rock ;
    skos:notation "msed"^^:gswa-rock-code ;
    skos:prefLabel "metasedimentary"@en ;
    skos:topConceptOf cs: ;
    schema:citation "https://glossary.americangeosciences.org/term/sedimentary"^^xsd:anyURI ;
.

:migmatite-protolith-unknown
    a skos:Concept ;
    rdfs:isDefinedBy cs: ;
    skos:broader :metamorphic-protolith-unknown ;
    skos:definition "Composite silicate metamorphic rock of uncertain protolith, pervasively heterogeneous on a meso- to megascopic scale. It typically consists of darker (melanosome) and lighter (leucosome) parts. The darker parts usually exhibit features of metamorphic rocks, whereas the lighter parts are of igneous appearance. Adapted from Fettes and Desmond (2007, p. 176)."@en ;
    skos:historyNote "Based on the IUGS classification of metamorphic rocks (Fettes and Desmons, 2007)." ;
    skos:inScheme cs: ;
    skos:narrower :felsic-migmatite-protolith-unknown ;
    skos:notation "migm"^^:gswa-rock-code ;
    skos:prefLabel "migmatite (protolith unknown)"@en ;
    schema:citation "https://geologyscience.com/rocks/metamorphic-rocks/foliated-metamorphic-rocks/migmatite/"^^xsd:anyURI ;
.

:mixed
    a skos:Concept ;
    rdfs:isDefinedBy cs: ;
    skos:definition "A prefix used in GSWA's Explanatory Notes system (ENS) to characterize the presence of more than one rock type."@en ;
    skos:historyNote "Compiled by the Geological Survey of Western Australia" ;
    skos:inScheme cs: ;
    skos:narrower :mixed-lithology ;
    skos:notation "x"^^:gswa-rock-code ;
    skos:prefLabel "mixed"@en ;
    skos:topConceptOf cs: ;
.

:sedimentary
    a skos:Concept ;
    rdfs:isDefinedBy cs: ;
    skos:definition "A group name for rocks of sedimentary but otherwise unspecified origin, i.e. a rock for which a clastic or chemical/biochemical derivation cannot be conclusively established."@en ;
    skos:historyNote "Compiled by the Geological Survey of Western Australia" ;
    skos:inScheme cs: ;
    skos:narrower :sedimentary-rock ;
    skos:notation "sed"^^:gswa-rock-code ;
    skos:prefLabel "sedimentary"@en ;
    skos:topConceptOf cs: ;
    schema:citation "https://glossary.americangeosciences.org/term/sedimentary"^^xsd:anyURI ;
.

:unknown
    a skos:Concept ;
    rdfs:isDefinedBy cs: ;
    skos:definition "A group name for lithologies so altered, weathered or of such a fine grain size that an inference on the protolith or origin of the rock cannot be made. Also used to allocate a lithology to sample legacy data where a lithology was not known. The use of the related code/notation is limited to GSWA's Field observation database (WAROX)."@en ;
    skos:historyNote "Compiled by the Geological Survey of Western Australia" ;
    skos:inScheme cs: ;
    skos:narrower :unknown-lithology ;
    skos:notation "n"^^:gswa-rock-code ;
    skos:prefLabel "unknown"@en ;
    skos:topConceptOf cs: ;
.

:xenolith-or-inclusion-bearing
    a skos:Concept ;
    rdfs:isDefinedBy cs: ;
    skos:definition "A prefix used in GSWA's Explanatory Notes system (ENS) to characterize mixed rock types (metamorphosed or not) where one of the component is a xenolith or inclusion."@en ;
    skos:historyNote "Compiled by the Geological Survey of Western Australia" ;
    skos:inScheme cs: ;
    skos:narrower :xenolith-or-inclusion-bearing-lithology ;
    skos:notation "j"^^:gswa-rock-code ;
    skos:prefLabel "xenolith- or inclusion-bearing"@en ;
    skos:topConceptOf cs: ;
.

<https://linked.data.gov.au/org/gswa>
    a schema:Organization ;
    schema:name "Geological Survey of Western Australia" ;
    schema:url "https://dmp.wa.gov.au/Geological-Survey/Geological-Survey-262.aspx"^^xsd:anyURI ;
.

:arkose
    a skos:Concept ;
    rdfs:isDefinedBy cs: ;
    skos:altLabel
        "arkosic arenite"@en ,
        "feldspathic sandstone"@en ,
        "sandstone"@en ;
    skos:broader :sedimentary-siliciclastic ;
    skos:definition "A feldspar-rich sandstone, commonly coarse-grained and pink or reddish, that is typically composed of angular to subangular grains that may be either poorly or moderately well sorted, is usually derived from the rapid disintegration of granite or granitic rocks, and often closely resembles granite. Quartz is usually the dominant mineral, with feldspars constituting at least 25%. Cement (silica or calcite) is commonly rare, and matrix material (usually less than 15%) includes clay minerals (especially kaolinite), mica, and iron oxide; fine-grained rock fragments are often present. Adapted from Glossary of geology (5th edition revised; Neuendorf et al., 2011)."@en ;
    skos:historyNote "Folk, RL 1968, Petrology of Sedimentary Rocks: Austin, Hemphill Publishing Company, 170p." ;
    skos:inScheme cs: ;
    skos:narrower
        :lithic-arkose ,
        :subarkose ;
    skos:notation "sj"^^:gswa-rock-code ;
    skos:prefLabel "arkose"@en ;
    schema:citation "https://glossary.americangeosciences.org/term/arkose"^^xsd:anyURI ;
.

:distal-impactite
    a skos:Concept ;
    rdfs:isDefinedBy cs: ;
    skos:broader :metamorphic-protolith-unknown-impactite ;
    skos:definition "Impactite occurring as distal ejecta outside the outer limit of the continuous ejecta blanket. It includes tektite, microtektite and impactoclastic (global) airfall bed. (Fettes and Desmons, p. 147)"@en ;
    skos:historyNote "Based on the IUGS classification of metamorphic rocks (Fettes and Desmons, 2007)." ;
    skos:inScheme cs: ;
    skos:narrower
        :impactoclastic-airfall-bed ,
        :tektite ;
    skos:notation "mpd"^^:gswa-rock-code ;
    skos:prefLabel "distal impactite"@en ;
.

:granular-iron-formation
    a skos:Concept ;
    rdfs:isDefinedBy cs: ;
    skos:altLabel "GIF"@en ;
    skos:broader :iron-formation ;
    skos:definition "Granular iron-formation (GIF) is an iron formation lacking even, continuous bedding and containing sand-sized endoclasts in a finer-grained matrix. GIFs originate from well-sorted chemical sands disrupted by storm waves and currents to generate discontinuous layers; uninterrupted layers thicker than a few metres are rare for GIFs. They generally belong to the oxide or silicate mineral facies. Adapted from https://en.wikipedia.org/wiki/Iron-rich_sedimentary_rocks and Beukes and Gutzmer (2008)."@en ;
    skos:historyNote "Beukes, NJ and Gutzmer, J 2008, Origin and paleoenvironmental significance of major iron formations at the Archean-Paleoproterozoic boundary: Reviews in Economic Geology, v. 15, p. 5–47, doi:10.5382/Rev.15.01." ;
    skos:inScheme cs: ;
    skos:narrower
        :fearenite ,
        :ferudite ;
    skos:notation "cig"^^:gswa-rock-code ;
    skos:prefLabel "granular iron-formation"@en ;
    schema:citation "https://en.wikipedia.org/wiki/Iron-rich_sedimentary_rocks"^^xsd:anyURI ;
.

:micritic-iron-formation
    a skos:Concept ;
    rdfs:isDefinedBy cs: ;
    skos:altLabel
        "MIF"@en ,
        "femicrite"@en ;
    skos:broader :iron-formation ;
    skos:definition "A femicrite / micritic iron-formation (MIF) is an indurated chemical iron-rich mud, i.e. an ironstone or iron-formation consisting predominantly of matrix (micrite) and lacking substantial granules. When distinctly chert-mesobanded, they are referred to as banded micritic iron-formations (BMIF). Adapted from Beukes and Gutzmer (2008)."@en ;
    skos:historyNote "Beukes, NJ and Gutzmer, J 2008, Origin and paleoenvironmental significance of major iron formations at the Archean-Paleoproterozoic boundary: Reviews in Economic Geology, v. 15, p. 5–47, doi:10.5382/Rev.15.01." ;
    skos:inScheme cs: ;
    skos:narrower
        :felutite ,
        :ferhythmite ;
    skos:notation "cim"^^:gswa-rock-code ;
    skos:prefLabel "micritic iron-formation"@en ;
.

:mudstone
    a skos:Concept ;
    rdfs:isDefinedBy cs: ;
    skos:altLabel
        "argillite"@en ,
        "mud rock"@en ;
    skos:broader :sedimentary-siliciclastic ;
    skos:closeMatch
        <http://inspire.ec.europa.eu/codelist/LithologyValue/silicateMudstone> ,
        <http://resource.geosciml.org/classifier/cgi/lithology/silicate_mudstone> ;
    skos:definition "An indurated mud having the texture and composition of shale, but lacking its fine lamination or fissility. A general term that includes clay, silt, claystone, siltstone, shale, and argillite, and that should be used only when the amounts of clay and silt are not known or specified or cannot be precisely identified; or when it is desirable to characterize the whole family of finer-grained sedimentary rocks (as distinguished from sandstones, conglomerates, and limestones). The term specifies neither mineralogic composition nor mud of clastic origin. Historical GSWA usage has incorrectly used mudstone interchangeably with siltstone. Adapted from Glossary of geology (5th edition revised; Neuendorf et al., 2011)."@en ;
    skos:exactMatch
        <http://inspire.ec.europa.eu/codelist/LithologyValue/clasticMudstone> ,
        <http://resource.geosciml.org/classifier/cgi/lithology/clastic_mudstone> ;
    skos:historyNote "Pettijohn, FJ 1975, Sedimentary Rocks: New York, Harper and Row, 628p." ;
    skos:inScheme cs: ;
    skos:narrower
        :claystone ,
        :siltstone ;
    skos:notation "sl"^^:gswa-rock-code ;
    skos:prefLabel "mudstone"@en ;
    schema:citation "https://glossary.americangeosciences.org/term/mudstone"^^xsd:anyURI ;
.

:sandstone
    a skos:Concept ;
    rdfs:isDefinedBy cs: ;
    skos:altLabel
        "arenite"@en ,
        "sandrock"@en ;
    skos:broader :sedimentary-siliciclastic ;
    skos:definition "A sedimentary rock composed of abundant rounded or angular fragments of sand size with or without a fine-grained matrix (silt or clay) and more or less firmly united by a cementing material (commonly silica, iron oxide, or calcium carbonate); the consolidated equivalent of sand, intermediate in texture between conglomerate and mudstone. The sand particles are predominantly quartz, and the term 'sandstone', when used without qualification, indicates a rock containing about 85–90% quartz. Sandstone may be classified according to composition of particles, mineralogic or textural maturity, primary structures, and type of cement. Adapted from Glossary of geology (5th edition revised; Neuendorf et al., 2011)"@en ;
    skos:exactMatch
        <http://inspire.ec.europa.eu/codelist/LithologyValue/clasticSandstone> ,
        <http://resource.geosciml.org/classifier/cgi/lithology/clastic_sandstone> ;
    skos:historyNote """Folk, RL 1968, Petrology of Sedimentary Rocks: Austin, Hemphill Publishing Company, 170p.,
Pettijohn, FJ 1975, Sedimentary Rocks: New York, Harper and Row, 628p.""" ;
    skos:inScheme cs: ;
    skos:narrower
        :calcareous-sandstone ,
        :dolomitic-sandstone ;
    skos:notation "st"^^:gswa-rock-code ;
    skos:prefLabel "sandstone"@en ;
    schema:citation "https://glossary.americangeosciences.org/term/sandstone"^^xsd:anyURI ;
.

:calc-silicate-rock
    a skos:Concept ;
    rdfs:isDefinedBy cs: ;
    skos:broader :metasedimentary-carbonate ;
    skos:definition "Metamorphic rock mainly composed of calc-silicate minerals (i.e. calcium-rich silicate minerals) and containing less than 5% volume of carbonate minerals (calcite and/or aragonite and/or dolomite). Adapted from Fettes and Desmons (2007, p. 137)"@en ;
    skos:historyNote "Based on the IUGS classification of metamorphic rocks (Fettes and Desmons, 2007)." ;
    skos:inScheme cs: ;
    skos:narrower
        :calc-silicate-gneiss ,
        :calc-silicate-granofels-hornfels ,
        :calc-silicate-schist ;
    skos:notation "mkq"^^:gswa-rock-code ;
    skos:prefLabel "calc-silicate rock"@en ;
.

:doloboundstone
    a skos:Concept ;
    rdfs:isDefinedBy cs: ;
    skos:altLabel "dolomite boundstone"@en ;
    skos:broadMatch
        <http://inspire.ec.europa.eu/codelist/LithologyValue/boundstone> ,
        <http://resource.geosciml.org/classifier/cgi/lithology/boundstone> ;
    skos:broader :dolomite ;
    skos:definition "A term used by Dunham (1962) for an autochthonous carbonate sedimentary rock consisting mostly of dolomite whose original components were bound together during deposition and remained substantially in the position of growth (as shown by such features as intergrown skeletal matter and lamination contrary to gravity); e.g. most reef rocks and some biohermal and biostromal rocks. It is composed of bioclasts, over 2 mm in diameter and forming more than 10% of the rock, that are organically attached or cemented to each other; these may form a structural framework or be interspersed among coarse skeletal debris. Adapted from Glossary of geology (5th edition revised; Neuendorf et al., 2011)."@en ;
    skos:historyNote """Dunham, RJ 1962, Classification of carbonate rocks according to depositional texture, in Classification of carbonate rocks edited by WE Hamm: American Association of Petroleum Geologists, Tulsa, Oklahoma, USA, p. 108–121.,
Embry, AF, Klovan, JE 1971, A late Devonian reef tract on northeastern Banks Island, N.W.T: Bulletin of Canadian Petroleum Geology, v. 19(4), p. 730–781.""" ;
    skos:inScheme cs: ;
    skos:narrower
        :dolobafflestone ,
        :dolobindstone ,
        :doloframestone ;
    skos:notation "kdb"^^:gswa-rock-code ;
    skos:prefLabel "doloboundstone"@en ;
    schema:citation "https://glossary.americangeosciences.org/term/boundstone"^^xsd:anyURI ;
.

:impact-breccia
    a skos:Concept ;
    rdfs:isDefinedBy cs: ;
    skos:broader :metamorphic-protolith-unknown-impactite ;
    skos:definition "Monomictic or polymictic breccia that occurs around, inside and below impact craters (Fettes and Desmons, 2007, p. 161). Impact breccias are classified based on the degree of mixing of various target lithologies and their content of melt particles. Lithic breccias and suevites are generally polymictic breccias except for single lithology targets. The matrix of lithic breccias is truly clastic and consists exclusively of lithic and mineral clasts whereas the matrix of suevite additionally contains melt particles. Megabreccias are polymictic impact breccia containing lithic clasts up to the size of several hundred metres as part of the ejecta blanket of an impact crater (Fettes and Desmons, 2007, p. 171)."@en ;
    skos:historyNote "Based on the IUGS classification of metamorphic rocks (Fettes and Desmons, 2007)." ;
    skos:inScheme cs: ;
    skos:narrower
        :lithic-impact-breccia ,
        :monomictic-impact-breccia ,
        :suevite ;
    skos:notation "mpb"^^:gswa-rock-code ;
    skos:prefLabel "impact breccia"@en ;
.

:limestone-boundstone
    a skos:Concept ;
    rdfs:isDefinedBy cs: ;
    skos:altLabel "boundstone"@en ;
    skos:broadMatch
        <http://inspire.ec.europa.eu/codelist/LithologyValue/boundstone> ,
        <http://resource.geosciml.org/classifier/cgi/lithology/boundstone> ;
    skos:broader :limestone ;
    skos:definition "A term used by Dunham (1962) for a sedimentary carbonate rock consisting mostly of calcite whose original components were bound together during deposition and remained substantially in the position of growth (as shown by such features as intergrown skeletal matter and lamination contrary to gravity); e.g. most reef rocks and some biohermal and biostromal rocks. It is composed of bioclasts, over 2 mm in diameter and forming more than 10% of the rock, that are organically attached or cemented to each other; these may form a structural framework or be interspersed among coarse skeletal debris. Adapted from Glossary of geology (5th edition revised; Neuendorf et al., 2011). The limestone prefix is commonly omitted since it is implied by Dunham's (1962) classification."@en ;
    skos:historyNote """Dunham, RJ 1962, Classification of carbonate rocks according to depositional texture, in Classification of carbonate rocks edited by WE Hamm: American Association of Petroleum Geologists, Tulsa, Oklahoma, USA, p. 108–121.,
Embry, AF, Klovan, JE 1971, A late Devonian reef tract on northeastern Banks Island, N.W.T: Bulletin of Canadian Petroleum Geology, v. 19(4), p. 730–781.""" ;
    skos:inScheme cs: ;
    skos:narrower
        :limestone-bafflestone ,
        :limestone-bindstone ,
        :limestone-framestone ;
    skos:notation "klb"^^:gswa-rock-code ;
    skos:prefLabel "limestone boundstone"@en ;
    schema:citation "https://glossary.americangeosciences.org/term/boundstone"^^xsd:anyURI ;
.

:marble
    a skos:Concept ;
    rdfs:isDefinedBy cs: ;
    skos:broader :metasedimentary-carbonate ;
    skos:definition "Metamorphic rock containing more than 50% volume of carbonate minerals (calcite and/or aragonite and/or dolomite). Pure marble contains more than 95% volume of carbonate minerals; a marble containing less than 95% of carbonate minerals is classified as impure marble. Adapted from Fettes and Desmons (2007, p. 170)."@en ;
    skos:exactMatch
        <http://inspire.ec.europa.eu/codelist/LithologyValue/marble> ,
        <http://resource.geosciml.org/classifier/cgi/lithology/marble> ;
    skos:historyNote "Based on the IUGS classification of metamorphic rocks (Fettes and Desmons, 2007)." ;
    skos:inScheme cs: ;
    skos:narrower
        :gneissose-marble ,
        :granofelsic-hornfelsic-marble ,
        :schistose-marble ;
    skos:notation "mkk"^^:gswa-rock-code ;
    skos:prefLabel "marble"@en ;
.

:meta-igneous-volcanic-or-volcaniclastic
    a skos:Concept ;
    rdfs:isDefinedBy cs: ;
    skos:definition "A group name for metamorphosed lithologies derived from volcanic or volcaniclastic protoliths, but otherwise uncategorized in terms of composition or grain size."@en ;
    skos:historyNote "Compiled by the Geological Survey of Western Australia" ;
    skos:inScheme cs: ;
    skos:narrower
        :metavolcanic-and-metavolcaniclastic-rock ,
        :mylonitized-metavolcanic-or-metavolcaniclastic-rock ,
        :silicified-metavolcanic-or-metavolcaniclastic-rock ;
    skos:notation "mv"^^:gswa-rock-code ;
    skos:prefLabel "meta-igneous volcanic or volcaniclastic"@en ;
    skos:topConceptOf cs: ;
.

:para-amphibolite
    a skos:Concept ;
    rdfs:isDefinedBy cs: ;
    skos:broader :metasedimentary-siliciclastic ;
    skos:definition "A metamorphosed amphibole-rich rock derived from a sedimentary siliciclastic protolith, usually characterized by the same equilibrium mineral assemblage as ortho-amphibolite, but with more biotite, quartz and plagioclase."@en ;
    skos:historyNote "Compiled by the Geological Survey of Western Australia" ;
    skos:inScheme cs: ;
    skos:narrower
        :gneissose-para-amphibolite-siliciclastic ,
        :granofelsic-hornfelsic-para-amphibolite-siliciclastic ,
        :schistose-para-amphibolite-siliciclastic ;
    skos:notation "mda"^^:gswa-rock-code ;
    skos:prefLabel "para-amphibolite"@en ;
    schema:citation "https://en.wikipedia.org/wiki/Amphibolite"^^xsd:anyURI ;
.

:para-amphibolite-derived-from-carbonate-rock
    a skos:Concept ;
    rdfs:isDefinedBy cs: ;
    skos:broader :metasedimentary-carbonate ;
    skos:definition "A metamorphosed amphibole-rich rock derived from a sedimentary carbonate protolith, usually characterized by the same equilibrium mineral assemblage as ortho-amphibolite (hornblende, actinolite, plagioclase with or without minor quartz), but with more calcite/aragonite and wollastonite."@en ;
    skos:historyNote "Compiled by the Geological Survey of Western Australia" ;
    skos:inScheme cs: ;
    skos:narrower
        :gneissose-para-amphibolite-carbonate ,
        :granofelsic-hornfelsic-para-amphibolite-carbonate ,
        :schistose-para-amphibolite-carbonate ;
    skos:notation "mka"^^:gswa-rock-code ;
    skos:prefLabel "para-amphibolite derived from carbonate rock"@en ;
    schema:citation "https://en.wikipedia.org/wiki/Amphibolite"^^xsd:anyURI ;
.

:skarn
    a skos:Concept ;
    rdfs:isDefinedBy cs: ;
    skos:altLabel "tactite"@en ;
    skos:broader :metasomatic ;
    skos:definition "Skarns or tactites are coarse-grained metamorphic rocks that form by replacement of carbonate-bearing rocks during regional or contact metamorphism and metasomatism. Skarns may form by metamorphic recrystallization of impure carbonate protoliths, bimetasomatic reaction of different lithologies, and infiltration metasomatism by magmatic-hydrothermal fluids. Skarns tend to be rich in calcium–magnesium–iron–manganese–aluminium silicate minerals, which are also referred to as calc-silicate minerals. (Fettes and Desmons, 2007, p. 195)"@en ;
    skos:historyNote "Einaudi, MT, Meinert, LD and Newberry, RJ, 1981, Skarn deposits: in 75th Anniversary Volume, 1906–1980, edited by BJ Skinner: Society of Economic Geology, Pennsylvania, USA, p. 317–391." ;
    skos:inScheme cs: ;
    skos:narrower
        :endoskarn ,
        :exoskarn ,
        :reaction-skarn ;
    skos:notation "mjk"^^:gswa-rock-code ;
    skos:prefLabel "skarn"@en ;
    schema:citation "https://glossary.americangeosciences.org/term/skarn"^^xsd:anyURI ;
.

:wacke
    a skos:Concept ;
    rdfs:isDefinedBy cs: ;
    skos:altLabel
        "graywacke"@en ,
        "greywacke"@en ,
        "sandstone"@en ;
    skos:broader :sedimentary-siliciclastic ;
    skos:definition "A 'dirty' sandstone that consists of a mixed variety of unsorted or poorly sorted mineral and rock fragments, with 15–75% matrix of medium silt to clay. The term is used for a major category of sandstone, as distinguished from arenite. Adapted from Glossary of geology (5th edition revised; Neuendorf et al., 2011)."@en ;
    skos:exactMatch
        <http://inspire.ec.europa.eu/codelist/LithologyValue/wacke> ,
        <http://resource.geosciml.org/classifier/cgi/lithology/wacke> ;
    skos:historyNote "Pettijohn, FJ 1975, Sedimentary Rocks: New York, Harper and Row, 628p." ;
    skos:inScheme cs: ;
    skos:narrower
        :feldspathic-wacke ,
        :lithic-wacke ,
        :quartz-wacke ;
    skos:notation "sw"^^:gswa-rock-code ;
    skos:prefLabel "wacke"@en ;
    schema:citation
        "https://glossary.americangeosciences.org/term/wacke"^^xsd:anyURI ,
        "https://glossary.americangeosciences.org/term/wackestone"^^xsd:anyURI ;
.

:arenite
    a skos:Concept ;
    rdfs:isDefinedBy cs: ;
    skos:altLabel "sandstone"@en ;
    skos:broader :sedimentary-siliciclastic ;
    skos:definition "A general term used for well-sorted, consolidated sedimentary rocks composed of sand-sized fragments (irrespective of composition) with a pure or nearly pure chemical cement and less than 10% argillaceous matrix; as distinguished from wacke. Further subdivision is based on proportions of quartz (Q), feldspar (F) and rock/lithic fragments (R/L). Adapted from Glossary of geology (5th edition revised; Neuendorf et al., 2011)"@en ;
    skos:exactMatch
        <http://inspire.ec.europa.eu/codelist/LithologyValue/arenite> ,
        <http://resource.geosciml.org/classifier/cgi/lithology/arenite> ;
    skos:historyNote "Pettijohn, FJ 1975, Sedimentary Rocks: New York, Harper and Row, 628p." ;
    skos:inScheme cs: ;
    skos:narrower
        :feldspathic-litharenite ,
        :litharenite ,
        :quartzarenite ,
        :sublitharenite ;
    skos:notation "sa"^^:gswa-rock-code ;
    skos:prefLabel "arenite"@en ;
    schema:citation "https://glossary.americangeosciences.org/term/arenite"^^xsd:anyURI ;
.

:conglomerate
    a skos:Concept ;
    rdfs:isDefinedBy cs: ;
    skos:broader :sedimentary-siliciclastic ;
    skos:definition "A coarse-grained clastic sedimentary rock, composed of rounded to subangular fragments larger than 2 mm in diameter (granules, pebbles, cobbles, boulders) typically containing fine-grained particles (sand, silt, clay) in the interstices, and commonly cemented by iron oxide, silica, carbonate or hardened clay; the consolidated equivalent of gravel both in size range and in the essential roundness and sorting of its constituent particles. The rock or mineral fragments may be of varied composition and range widely in size. Conglomerates may be classified according to nature or composition of fragments, proportion of matrix, degree of size sorting, type of cement, and agent or environment of formation. Adapted from Glossary of geology (5th edition revised; Neuendorf et al., 2011)."@en ;
    skos:exactMatch
        <http://inspire.ec.europa.eu/codelist/LithologyValue/clasticConglomerate> ,
        <http://resource.geosciml.org/classifier/cgi/lithology/clastic_conglomerate> ;
    skos:historyNote "Wentworth, CK 1922, A scale of grade and class terms for clastic sediments: The Journal of Geology, v. 30, no. 5, p. 377–392, doi:10.1086/622910." ;
    skos:inScheme cs: ;
    skos:narrower
        :boulder-conglomerate ,
        :cobble-conglomerate ,
        :granule-conglomerate ,
        :pebble-conglomerate ;
    skos:notation "sc"^^:gswa-rock-code ;
    skos:prefLabel "conglomerate"@en ;
    schema:citation "https://glossary.americangeosciences.org/term/conglomerate"^^xsd:anyURI ;
.

:evaporite
    a skos:Concept ;
    rdfs:isDefinedBy cs: ;
    skos:altLabel "saline deposit"@en ;
    skos:broader :sedimentary-other-chemical-or-biochemical ;
    skos:definition "A sedimentary rock composed primarily of minerals produced from a saline solution as a result of extensive or total evaporation of the solvent. Examples include gypsum, anhydrite, other diverse sulfates, halite (rock salt), primary dolomite, and various nitrates and borates. The term commonly includes rocks with saline minerals formed by other mechanisms, e.g. mixing of waters or temperature change. Mineral grains formed by these mechanisms may be reworked by wind or saline waters as clastic particles but are also considered evaporitic deposits. Adapted from Glossary of geology (5th edition revised; Neuendorf et al., 2011)."@en ;
    skos:exactMatch
        <http://inspire.ec.europa.eu/codelist/LithologyValue/evaporite> ,
        <http://resource.geosciml.org/classifier/cgi/lithology/evaporite> ;
    skos:historyNote "Based on the Glossary of geology (5th edition, revised; Neuendorf et al. 2011)." ;
    skos:inScheme cs: ;
    skos:narrower
        :anhydrite-evaporite ,
        :calcite-evaporite ,
        :gypsum-evaporite ,
        :halite-evaporite ;
    skos:notation "cv"^^:gswa-rock-code ;
    skos:prefLabel "evaporite"@en ;
    schema:citation "https://glossary.americangeosciences.org/term/evaporite"^^xsd:anyURI ;
.

:iron-formation
    a skos:Concept ;
    rdfs:isDefinedBy cs: ;
    skos:broader :sedimentary-other-chemical-or-biochemical ;
    skos:definition "A chemical sedimentary rock, typically thin-bedded and/or finely laminated, containing at least 15% iron of sedimentary origin, and commonly but not necessarily containing layers of chert. Various primary facies (usually not weathered) of iron formation are distinguished on the basis of whether the iron occurs predominantly as oxide, silicate, carbonate, or sulfide. Most iron formation is of Precambrian age and was deposited as chemical muds. Adapted from Glossary of geology (5th edition revised; Neuendorf et al., 2011)."@en ;
    skos:historyNote "Beukes, NJ and Gutzmer, J 2008, Origin and paleoenvironmental significance of major iron formations at the Archean-Paleoproterozoic boundary: Reviews in Economic Geology, v. 15, p. 5–47, doi:10.5382/Rev.15.01." ;
    skos:inScheme cs: ;
    skos:narrower
        :banded-iron-formation ,
        :granular-iron-formation ,
        :jaspilite ,
        :micritic-iron-formation ;
    skos:notation "ci"^^:gswa-rock-code ;
    skos:prefLabel "iron formation"@en ;
    schema:citation "https://glossary.americangeosciences.org/term/ironformation"^^xsd:anyURI ;
.

:coal
    a skos:Concept ;
    rdfs:isDefinedBy cs: ;
    skos:broader :sedimentary-other-chemical-or-biochemical ;
    skos:definition "A readily combustible rock containing more than 50% by weight and more than 70% by volume of carbonaceous material including inherent moisture, formed from compaction and induration of variously altered plant remains similar to those in peat. Differences in the kinds of plant materials (type), in degree of metamorphism (rank), and in the range of impurity (grade) are characteristic of coal and are used in classification. Adapted from Glossary of geology (5th edition revised; Neuendorf et al., 2011)."@en ;
    skos:exactMatch
        <http://inspire.ec.europa.eu/codelist/LithologyValue/coal> ,
        <http://resource.geosciml.org/classifier/cgi/lithology/coal> ;
    skos:historyNote "Forsman, JP and Hunt, JM 1958, Insoluble organic matter (kerogen) in sedimentary rocks: Geochimica et Cosmochimica Acta, v. 15(3), p. 170–182, doi.org/10.1016/0016-7037(58)90055-3." ;
    skos:inScheme cs: ;
    skos:narrower
        :anthracite ,
        :bituminous-coal ,
        :lignite ,
        :peat ,
        :sub-bituminous-coal ;
    skos:notation "co"^^:gswa-rock-code ;
    skos:prefLabel "coal"@en ;
    schema:citation "https://glossary.americangeosciences.org/term/coal"^^xsd:anyURI ;
.

:igneous-kalsilitic
    a skos:Concept ;
    rdfs:isDefinedBy cs: ;
    skos:definition "A group name for a dominantly mafic, melanocratic volcanic rocks consisting essentially of clinopyroxene, kalsilite, leucite, melilite, olivine and phlogopite (cf. Le Maitre et al., 2005, p. 12). GSWA's rock classification scheme prefers the use of volcanic terminology for any igneous rock formed on or near the Earth's surface, i.e. for those hypabyssal or subvolcanic rocks such as dykes, sills, and cryptodomes that are demonstrably both spatially and temporally associated with extrusive volcanic rocks."@en ;
    skos:historyNote "Based on the IUGS classification of igneous rocks (Le Maitre et al., 2005). See also https://academic.oup.com/petrology/article/63/5/egac026/6553206." ;
    skos:inScheme cs: ;
    skos:narrower
        :kalsilite-leucite-olivine-melilitite ,
        :kalsilite-phlogopite-melilitite ,
        :kalsilite-phlogopite-olivine-leucite-melilitite ,
        :kalsilitite-undivided ,
        :olivine-pyroxene-kalsilitite ;
    skos:notation "w"^^:gswa-rock-code ;
    skos:prefLabel "igneous kalsilitic"@en ;
    skos:topConceptOf cs: ;
.

:igneous-melilitic
    a skos:Concept ;
    rdfs:isDefinedBy cs: ;
    skos:definition "A group name for ultramafic intrusive rocks that consist essentially of melilite, pyroxene and olivine. The term is reserved for rocks that contain greater than 10% modal melilite, and, if feldspathoids are present, melilite > feldspathoid; modal content of mafic minerals (M) is usually greater than 90%. Melilites are honey-coloured minerals with the general formula (Na,Ca)₂(Mg,Al)(Si,Al)₂O₇. Definitions adapted from Le Maitre et al. (2005, p. 11) and Glossary of geology (5th edition revised; Neuendorf et al., 2011)."@en ;
    skos:historyNote "Based on the IUGS classification of igneous rocks (Le Maitre et al., 2005) and Glossary of geology (5th edition, revised; Neuendorf et al. 2011)." ;
    skos:inScheme cs: ;
    skos:narrower
        :melilitolite ,
        :melilitolite-undivided ,
        :olivine-melilitolite ,
        :olivine-pyroxene-melilitolite ,
        :pyroxene-melilitolite ,
        :pyroxene-olivine-melilitolite ;
    skos:notation "e"^^:gswa-rock-code ;
    skos:prefLabel "igneous melilitic"@en ;
    skos:topConceptOf cs: ;
    schema:citation "https://glossary.americangeosciences.org/term/melilite"^^xsd:anyURI ;
.

:metasedimentary-siliciclastic-psephite
    a skos:Concept ;
    rdfs:isDefinedBy cs: ;
    skos:altLabel "psephyte"@en ;
    skos:definition "A group name for metamorphosed rocks derived from a sedimentary siliciclastic protolith with grain size greater than 2 mm, i.e. the metamorphosed equivalent of a conglomerate. Acknowledging entrenched practises, GSWA usage allows the use of psephite as a noun for a metamorphosed equivalent of conglomerate lithologies (i.e. grain size greater than 2 mm), as well as an adjective to qualify metamorphic rocks derived from these sedimentary types (e.g. psephitic schist)."@en ;
    skos:historyNote "Compiled by the Geological Survey of Western Australia" ;
    skos:inScheme cs: ;
    skos:narrower
        :metaconglomerate ,
        :mylonitized-metaconglomerate ,
        :psephitic-gneiss ,
        :psephitic-granofels-hornfels ,
        :psephitic-schist ,
        :silicified-metaconglomerate ;
    skos:notation "mx"^^:gswa-rock-code ;
    skos:prefLabel "metasedimentary siliciclastic: psephite"@en ;
    skos:topConceptOf cs: ;
    schema:citation "https://glossary.americangeosciences.org/term/psephite"^^xsd:anyURI ;
.

:meta-igneous-carbonatite
    a skos:Concept ;
    rdfs:isDefinedBy cs: ;
    skos:definition "A group name for metamorphosed rocks derived from carbonatites, i.e. igneous rocks containing more than 50% modal carbonates (cf. Le Maitre et al., 2005, p. 10)."@en ;
    skos:historyNote "Compiled by the Geological Survey of Western Australia" ;
    skos:inScheme cs: ;
    skos:narrower
        :gneissose-metacarbonatite ,
        :metacarbonatite ,
        :metacarbonatite-granofels-hornfels ,
        :migmatitic-metacarbonatite ,
        :mylonitized-metacarbonatite ,
        :schistose-metacarbonatite ,
        :silicified-metacarbonatite ;
    skos:notation "mq"^^:gswa-rock-code ;
    skos:prefLabel "meta-igneous carbonatite"@en ;
    skos:topConceptOf cs: ;
.

:metamorphic-protolith-unknown-impactite
    a skos:Concept ;
    rdfs:isDefinedBy cs: ;
    skos:definition "A group name for all rocks affected by one or more hypervelocity impact(s) resulting from collision(s) of two planetary bodies. Only impactites derived from a single impact (e.g. at terrestrial impact craters) are considered in this vocabulary, impactites resulting from multiple impacts (i.e. as known from the Moon and from meteorites) are not considered. (Osinski et al., 2022)"@en ;
    skos:historyNote "Osinski, GR, Grieve, RAF, Ferrière, L, Losiak, A, Pickersgill, AE, Cavosie, AJ, Hibbard, SM, Hill, PJA, Bermudez, JJ, Marion, CL, Newman, JD and Simpson, SL 2022, Impact Earth: A review of the terrestrial impact record: Earth-Science Reviews, v. 232, 104112, doi.org/10.1016/j.earscirev.2022.104112." ;
    skos:inScheme cs: ;
    skos:narrower
        :distal-impactite ,
        :impact-breccia ,
        :impact-melt-rock ,
        :impactite ,
        :impactoclastic-deposit ,
        :pseudotachylite-impactite ,
        :shocked-target-rock ;
    skos:notation "mp"^^:gswa-rock-code ;
    skos:prefLabel "metamorphic protolith unknown: impactite"@en ;
    skos:topConceptOf cs: ;
    schema:citation "https://doi.org/10.1016/j.earscirev.2022.104112"^^xsd:anyURI ;
.

:metamorphosed-hydrothermal
    a skos:Concept ;
    rdfs:isDefinedBy cs: ;
    skos:definition "A group name for hydrothermal lithologies that have undergone metamorphism."@en ;
    skos:historyNote "Compiled by the Geological Survey of Western Australia" ;
    skos:inScheme cs: ;
    skos:narrower
        :gneissose-hydrothermal-rock ,
        :granofelsic-hornfelsic-hydrothermal-rock ,
        :metahydrothermal-chert ,
        :metamorphosed-hydrothermal-rock ,
        :metamorphosed-quartz-vein ,
        :mylonitized-hydrothermal-rock ,
        :schistose-hydrothermal-rock ;
    skos:notation "mz"^^:gswa-rock-code ;
    skos:prefLabel "metamorphosed hydrothermal"@en ;
    skos:topConceptOf cs: ;
    schema:citation
        "https://glossary.americangeosciences.org/term/hydrothermalalteration"^^xsd:anyURI ,
        "https://glossary.americangeosciences.org/term/metamorphism"^^xsd:anyURI ;
.

:metasedimentary-other-chemical
    a skos:Concept ;
    rdfs:isDefinedBy cs: ;
    skos:definition "A group name for metamorphosed rocks derived from silica- and/or quartz-dominated chemical/biochemical protoliths."@en ;
    skos:historyNote "Compiled by the Geological Survey of Western Australia" ;
    skos:inScheme cs: ;
    skos:narrower
        :gneissose-metachert ,
        :granofelsic-hornfelsic-metachert ,
        :meta-banded-chert ,
        :metachert ,
        :mylonitized-metachert ,
        :schistose-metachert ,
        :silicified-metachert ;
    skos:notation "mc"^^:gswa-rock-code ;
    skos:prefLabel "metasedimentary other chemical"@en ;
    skos:topConceptOf cs: ;
.

:metasedimentary-other-chemical-meta-iron-formation
    a skos:Concept ;
    rdfs:isDefinedBy cs: ;
    skos:definition "A group name for metamorphosed iron formations, i.e. metamorphosed rocks derived from chemical sedimentary protoliths containing at least 15% iron of sedimentary origin."@en ;
    skos:historyNote "Compiled by the Geological Survey of Western Australia" ;
    skos:inScheme cs: ;
    skos:narrower
        :gneissose-meta-iron-formation ,
        :granofelsic-hornfelsic-meta-iron-formation ,
        :meta-banded-iron-formation ,
        :meta-iron-formation ,
        :mylonitized-meta-iron-formation ,
        :schistose-meta-iron-formation ,
        :silicified-meta-iron-formation ;
    skos:notation "mi"^^:gswa-rock-code ;
    skos:prefLabel "metasedimentary other chemical: meta-iron formation"@en ;
    skos:topConceptOf cs: ;
.

:metasedimentary-siliciclastic-psammite-and-pelite-interlayered
    a skos:Concept ;
    rdfs:isDefinedBy cs: ;
    skos:definition "A group name for metamorphosed rocks derived from a succession of interleaved sandstone and mudstone beds, i.e. sedimentary siliciclastic protoliths with grain size between 0.0625 and 2 mm and less than 0.0625 mm respectively. Acknowledging entrenched practises, GSWA usage allows the use of psammite and pelite as nouns for metamorphosed equivalent of sandstone and mudstone lithologies, as well as adjectives to qualify metamorphic rocks derived from these sedimentary types."@en ;
    skos:historyNote "Partly based on the IUGS classification of metamorphic rocks (Fettes and Desmons, 2007)." ;
    skos:inScheme cs: ;
    skos:narrower
        :mylonitized-psammite-and-pelite ,
        :psammite-and-pelite-interlayered ,
        :psammitic-and-pelitic-gneiss-interlayered ,
        :psammitic-and-pelitic-granofels-hornfels-interlayered ,
        :psammitic-and-pelitic-migmatite-interlayered ,
        :psammitic-and-pelitic-schist-interlayered ,
        :silicified-psammite-and-pelite-interlayered ;
    skos:notation "mh"^^:gswa-rock-code ;
    skos:prefLabel "metasedimentary siliciclastic: psammite and pelite; interlayered"@en ;
    skos:topConceptOf cs: ;
    schema:citation
        "https://glossary.americangeosciences.org/term/pelite"^^xsd:anyURI ,
        "https://glossary.americangeosciences.org/term/psammite"^^xsd:anyURI ;
.

:metasedimentary-siliciclastic-semipelite
    a skos:Concept ;
    rdfs:isDefinedBy cs: ;
    skos:definition "A group name for metamorphosed rocks with a modal ratio of mica to quartz + feldspar intermediate between a pelite and a psammite, a crystalloblastic nature, and derived from a fine- to medium-grained siliciclastic sedimentary protolith."@en ;
    skos:historyNote "Based on the IUGS classification of metamorphic rocks (Fettes and Desmons, 2007)." ;
    skos:inScheme cs: ;
    skos:narrower
        :mylonitized-semipelite ,
        :semipelite ,
        :semipelitic-gneiss ,
        :semipelitic-granofels-hornfels ,
        :semipelitic-migmatite ,
        :semipelitic-schist ,
        :silicified-semipelite ;
    skos:notation "mm"^^:gswa-rock-code ;
    skos:prefLabel "metasedimentary siliciclastic: semipelite"@en ;
    skos:topConceptOf cs: ;
    schema:citation "https://glossary.americangeosciences.org/term/pelite"^^xsd:anyURI ;
.

:meta-igneous-felsic
    a skos:Concept ;
    rdfs:isDefinedBy cs: ;
    skos:definition "A group name for metamorphosed igneous lithologies that are composed chiefly of felsic minerals, for which an intrusive or extrusive protolith cannot be conclusively identified. These rocks are derived from igneous or volcaniclastic protoliths with modal quartz and feldspar and M smaller than 90% (cf. Le Maitre et al., 2005, p. 153), where M represents the volume modal percentage of mafic and related minerals (Le Maitre et al., 2005, p. 4)."@en ;
    skos:historyNote "Based on the IUGS classification of metamorphic (Fettes and Desmons, 2007) and igneous rocks (Le Maitre et al., 2005)." ;
    skos:inScheme cs: ;
    skos:narrower
        :felsic-gneiss ,
        :felsic-granofels-hornfels ,
        :felsic-granulite ,
        :felsic-migmatite ,
        :felsic-schist ,
        :metafelsic-rock ,
        :mylonitized-meta-igneous-felsic-rock ,
        :silicified-meta-igneous-felsic-rock ;
    skos:notation "mr"^^:gswa-rock-code ;
    skos:prefLabel "meta-igneous felsic"@en ;
    skos:topConceptOf cs: ;
    schema:citation "https://glossary.americangeosciences.org/term/felsic"^^xsd:anyURI ;
.

:metasedimentary-siliciclastic-psammite
    a skos:Concept ;
    rdfs:isDefinedBy cs: ;
    skos:definition "A group name for metamorphosed rocks derived from a medium-grained siliciclastic sedimentary protolith (grain size between 0.0625 and 2 mm), i.e. the metamorphosed equivalent of a sandstone. Fettes and Desmons (2007, p. 188) identify psammite as a restricted-use term, and define it as \"... a term for a sedimentary rock composed of sand-sized particles. It has also been used locally for the metamorphosed equivalent of these sedimentary rocks, that is, metamorphic rocks with a low modal ratio of mica to quartz + feldspar (Tyrrell, Robertson). The SCMR recommends that it should be used only for sedimentary rocks and the term metapsammite should be used for the metamorphosed equivalents.\" Acknowledging entrenched practises, GSWA usage departs from this recommendation, and allows the use of psammite as a noun for a metamorphosed equivalent of sandstone lithologies (i.e. grain size between 0.0625 and 2 mm), as well as an adjective to qualify metamorphic rocks derived from these sedimentary types (e.g. pelitic schist)."@en ;
    skos:historyNote "Partly based on the IUGS classification of metamorphic rocks (Fettes and Desmons, 2007)." ;
    skos:inScheme cs: ;
    skos:narrower
        :meta-arkose ,
        :metasandstone ,
        :mylonitized-metasandstone ,
        :psammitic-gneiss ,
        :psammitic-granofels-hornfels ,
        :psammitic-migmatite ,
        :psammitic-schist ,
        :quartzite ;
    skos:notation "mt"^^:gswa-rock-code ;
    skos:prefLabel "metasedimentary siliciclastic: psammite"@en ;
    skos:topConceptOf cs: ;
    schema:citation "https://glossary.americangeosciences.org/term/psammite"^^xsd:anyURI ;
.

:igneous-lamprophyres
    a skos:Concept ;
    rdfs:isDefinedBy cs: ;
    skos:definition "A group name for a distinctive group of igneous rocks that are strongly porphyritic in mafic minerals, typically biotite, amphiboles and pyroxenes, with any feldspars being confined to the groundmass. They commonly occur as dykes or small intrusions and commonly show signs of hydrothermal alteration. (Le Maitre et al., 2005, p. 100)"@en ;
    skos:historyNote "Based on the IUGS classification of igneous rocks (Le Maitre et al., 2005)." ;
    skos:inScheme cs: ;
    skos:narrower
        :camptonite ,
        :kersantite ,
        :lamprophyre ,
        :lamprophyre-undivided ,
        :minette ,
        :monchiquite ,
        :sannaite ,
        :spessartite ,
        :vogesite ;
    skos:notation "y"^^:gswa-rock-code ;
    skos:prefLabel "igneous lamprophyres"@en ;
    skos:topConceptOf cs: ;
.

:metasedimentary-carbonate
    a skos:Concept ;
    rdfs:isDefinedBy cs: ;
    skos:definition "A group name for metamorphosed sedimentary rocks originally composed primarily of carbonate minerals and formed by the biotic or abiotic precipitation from aqueous solution of carbonates of calcium and/or magnesium."@en ;
    skos:historyNote "Compiled by the Geological Survey of Western Australia" ;
    skos:inScheme cs: ;
    skos:narrower
        :calc-silicate-rock ,
        :carbonate-gneiss-sedimentary ,
        :carbonate-granofels-hornfels-sedimentary ,
        :carbonate-schist-sedimentary ,
        :marble ,
        :metacarbonate-rock ,
        :metacarbonate-with-lesser-siliciclastic ,
        :mylonitized-metacarbonate-rock ,
        :para-amphibolite-derived-from-carbonate-rock ;
    skos:notation "mk"^^:gswa-rock-code ;
    skos:prefLabel "metasedimentary carbonate"@en ;
    skos:topConceptOf cs: ;
.

:metasedimentary-siliciclastic
    a skos:Concept ;
    rdfs:isDefinedBy cs: ;
    skos:definition "A group name for metamorphosed sedimentary lithologies derived from siliciclastic protoliths, i.e. from silicon-bearing (in the form of quartz and silicates), clastic non-carbonate rocks. Clastic refers to a rock or sediment composed principally of broken fragments that are derived from pre-existing rocks or minerals and that have been transported some distance from their places of origin. Adapted from Glossary of geology (5th edition revised; Neuendorf et al., 2011)"@en ;
    skos:historyNote "Compiled by the Geological Survey of Western Australia" ;
    skos:inScheme cs: ;
    skos:narrower
        :feldspathic-metasiliciclastic-rock ,
        :metasiliciclastic-rock ,
        :mylonitized-metasiliciclastic-rock ,
        :para-amphibolite ,
        :siliciclastic-gneiss ,
        :siliciclastic-granofels-hornfels ,
        :siliciclastic-migmatite ,
        :siliciclastic-schist ,
        :silicified-metasiliciclastic-rock ;
    skos:notation "md"^^:gswa-rock-code ;
    skos:prefLabel "metasedimentary siliciclastic"@en ;
    skos:topConceptOf cs: ;
    schema:citation
        "https://glossary.americangeosciences.org/term/clastic"^^xsd:anyURI ,
        "https://glossary.americangeosciences.org/term/siliciclastic"^^xsd:anyURI ;
.

:metasedimentary-siliciclastic-pelite
    a skos:Concept ;
    rdfs:isDefinedBy cs: ;
    skos:definition "A group name for metamorphosed rocks derived from a fine-grained sedimentary siliciclastic protolith (usually with grain size below 0.0625 mm), i.e. the metamorphosed equivalent of a mudstone. Fettes and Desmons (2007, p. 181) identify pelite as a restricted-use term, and define it as \"... a term for a sedimentary rock composed of clay-sized particles. It has also been used locally for the metamorphosed equivalent of these sedimentary rocks, that is, a metamorphic rock with a high modal ratio of mica to quartz+feldspar. The SCMR recommends that it should be used only for sedimentary rocks and the term metapelite should be used for the metamorphosed equivalents.\" Acknowledging entrenched practises, GSWA usage departs from this recommendation, and allows the use of pelite as a noun for a metamorphosed equivalent of mudstone lithologies, as well as an adjective to qualify metamorphic rocks derived from these sedimentary types (e.g. pelitic schist)."@en ;
    skos:historyNote "Partly based on the IUGS classification of metamorphic rocks (Fettes and Desmons, 2007)." ;
    skos:inScheme cs: ;
    skos:narrower
        :metasiltstone-metamudstone-metashale ,
        :mylonitized-pelite ,
        :pelitic-gneiss ,
        :pelitic-granofels-hornfels ,
        :pelitic-migmatite ,
        :pelitic-schist ,
        :phyllite ,
        :silicified-pelite ,
        :slate ;
    skos:notation "ml"^^:gswa-rock-code ;
    skos:prefLabel "metasedimentary siliciclastic: pelite"@en ;
    skos:topConceptOf cs: ;
    schema:citation "https://glossary.americangeosciences.org/term/pelite"^^xsd:anyURI ;
.

:metasomatic
    a skos:Concept ;
    rdfs:isDefinedBy cs: ;
    skos:definition "A group name for lithologies formed via metasomatic processes, i.e. the open-system metamorphic processes by which the chemical composition of a rock or rock portion is altered in a pervasive manner and which involves the introduction and/or removal of chemical components as a result of the interaction of the rock with aqueous fluids/solutions (usually hydrothermal or static fluids); during metasomatism the rock remains in a solid state (Fettes and Desmons, 2007, p. 174)."@en ;
    skos:historyNote "Based on the IUGS classification of metamorphic rocks (Fettes and Desmons, 2007)." ;
    skos:inScheme cs: ;
    skos:narrower
        :fenite ,
        :greisen ,
        :metasomatic-gneiss ,
        :metasomatic-granofels-hornfels ,
        :metasomatic-rock ,
        :metasomatic-schist ,
        :mylonitized-metasomatic-rock ,
        :rodingite ,
        :skarn ;
    skos:notation "mj"^^:gswa-rock-code ;
    skos:prefLabel "metasomatic"@en ;
    skos:topConceptOf cs: ;
    schema:citation
        "https://en.wikipedia.org/wiki/Metasomatism;"^^xsd:anyURI ,
        "https://glossary.americangeosciences.org/term/metasomatism"^^xsd:anyURI ;
.

:sedimentary-carbonate
    a skos:Concept ;
    rdfs:isDefinedBy cs: ;
    skos:definition "A group name for sedimentary rocks composed primarily of carbonate minerals, formed by the biotic or abiotic precipitation from aqueous solution of carbonates of calcium and/or magnesium, or by detrital reworking of those carbonate rocks."@en ;
    skos:historyNote "Compiled by the Geological Survey of Western Australia" ;
    skos:inScheme cs: ;
    skos:narrower
        :carbonate-rock ,
        :carbonate-rock-undivided ,
        :carbonate-with-lesser-siliciclastic ,
        :dolomite ,
        :limestone ,
        :magnesite ,
        :marlstone ,
        :mixed-carbonate-evaporite ,
        :mixed-limestone-dolomite ;
    skos:notation "k"^^:gswa-rock-code ;
    skos:prefLabel "sedimentary carbonate"@en ;
    skos:topConceptOf cs: ;
    schema:citation "https://glossary.americangeosciences.org/term/carbonatesed"^^xsd:anyURI ;
.

:meta-igneous-ultramafic-intrusive
    a skos:Concept ;
    rdfs:isDefinedBy cs: ;
    skos:definition "A group name for metamorphosed intrusive lithologies or coarse-grained parts of extrusive successions that are composed chiefly of mafic minerals, i.e. derived from intrusive protoliths with M greater than or equal to 90% (cf. Le Maitre et al., 2005, p. 153), where M represents the volume modal percentage of mafic and related minerals (Le Maitre et al., 2005, p. 4)."@en ;
    skos:historyNote "Based on the IUGS classification of metamorphic (Fettes and Desmons, 2007) and igneous rocks (Le Maitre et al., 2005)." ;
    skos:inScheme cs: ;
    skos:narrower
        :meta-ultramafic-intrusive-rock ,
        :metadunite-derived-from-intrusive-rock ,
        :metaperidotite-derived-from-intrusive-rock ,
        :metapyroxenite-derived-from-intrusive-rock ,
        :mylonitized-meta-ultramafic-intrusive-rock ,
        :serpentinite-derived-from-intrusive-rock ,
        :silicified-meta-ultramafic-intrusive-rock ,
        :ultramafic-gneiss-derived-from-intrusive-rock ,
        :ultramafic-granofels-hornfels-derived-from-intrusive-rock ,
        :ultramafic-schist-derived-from-intrusive-rock ;
    skos:notation "ma"^^:gswa-rock-code ;
    skos:prefLabel "meta-igneous ultramafic intrusive"@en ;
    skos:topConceptOf cs: ;
    schema:citation "https://glossary.americangeosciences.org/term/ultramafic"^^xsd:anyURI ;
.

:igneous-kimberlite
    a skos:Concept ;
    rdfs:isDefinedBy cs: ;
    skos:definition "A group name for igneous ultramafic rocks containing at least 35% olivine and no leucite, with one or more of the following in the groundmass: monticellite, phlogopite, carbonate, serpentine, diopside. The majority of kimberlites form as diatreme-filling, diamond-bearing rocks. Adapted from Glossary of geology (Neuendorf et al., 2011, 5th edition, revised)."@en ;
    skos:historyNote "Based on the IUGS classification of igneous rocks (Le Maitre et al., 2005)." ;
    skos:inScheme cs: ;
    skos:narrower
        :kimberlite ,
        :kimberlitic-rock-undivided ,
        :kimberlitic-volcaniclastic-breccia ,
        :kimberlitic-volcaniclastic-breccia-sandstone ,
        :kimberlitic-volcaniclastic-conglomerate ,
        :kimberlitic-volcaniclastic-granule-pebble-breccia ,
        :kimberlitic-volcaniclastic-mudstone ,
        :kimberlitic-volcaniclastic-rock ,
        :kimberlitic-volcaniclastic-sandstone ,
        :kimberlitic-volcaniclastic-sandstone-siltstone ,
        :kimberlitic-volcaniclastic-sediment-matrix-breccia ;
    skos:notation "p"^^:gswa-rock-code ;
    skos:prefLabel "igneous kimberlite"@en ;
    skos:topConceptOf cs: ;
    schema:citation "https://en.wikipedia.org/wiki/Kimberlite"^^xsd:anyURI ;
.

:meta-igneous-mafic
    a skos:Concept ;
    rdfs:isDefinedBy cs: ;
    skos:definition "A group name for metamorphosed igneous lithologies that are composed chiefly of mafic minerals, for which an intrusive, extrusive or volcaniclastic protolith cannot be conclusively identified. These rocks are derived from igneous or volcanic/volcaniclastic protoliths with M smaller than 90% (cf. Le Maitre et al., 2005, p. 153), where M represents the volume modal percentage of mafic and related minerals (Le Maitre et al., 2005, p. 4), and varying amounts of pyroxene, olivine and hornblende (cf. Le Maitre et al., 2005, p. 24)."@en ;
    skos:historyNote "Compiled by the Geological Survey of Western Australia" ;
    skos:inScheme cs: ;
    skos:narrower
        :amphibolite ,
        :blueschist ,
        :carbonate-altered-meta-igneous-mafic-rock ,
        :eclogite ,
        :mafic-gneiss ,
        :mafic-granofels-hornfels ,
        :mafic-granulite ,
        :mafic-schist ,
        :metamafic-rock ,
        :mylonitized-meta-igneous-mafic-rock ,
        :silicified-meta-igneous-mafic-rock ;
    skos:notation "mw"^^:gswa-rock-code ;
    skos:prefLabel "meta-igneous mafic"@en ;
    skos:topConceptOf cs: ;
    schema:citation "https://glossary.americangeosciences.org/term/mafic"^^xsd:anyURI ;
.

:meta-igneous-ultramafic-volcanic
    a skos:Concept ;
    rdfs:isDefinedBy cs: ;
    skos:definition "A group name for metamorphosed volcanic and volcaniclastic lithologies derived from protoliths composed chiefly of one or more ferromagnesian, dark-coloured minerals such as olivine, pyroxene, etc. in their mode, with the volume modal percentage of mafic and related minerals (M) greater than or equal to 90% (cf. Le Maitre et al., 2005, p. 4)."@en ;
    skos:historyNote "Based on the IUGS classification of metamorphic (Fettes and Desmons, 2007) and igneous rocks (Le Maitre et al., 2005)." ;
    skos:inScheme cs: ;
    skos:narrower
        :meta-ultramafic-volcanic-rock ,
        :meta-ultramafic-volcaniclastic-rock ,
        :metadunite-derived-from-volcanic-rock ,
        :metakomatiite ,
        :metaperidotite-derived-from-volcanic-rock ,
        :metapyroxenite-derived-from-volcanic-rock ,
        :mylonitized-meta-ultramafic-rock-volcanic-or-undivided ,
        :serpentinite-derived-from-volcanic-rock ,
        :silicified-meta-ultramafic-rock ,
        :ultramafic-gneiss-volcanic-or-undivided ,
        :ultramafic-granofels-hornfels-volcanic-or-undivided ,
        :ultramafic-schist-volcanic-or-undivided ;
    skos:notation "mu"^^:gswa-rock-code ;
    skos:prefLabel "meta-igneous ultramafic volcanic"@en ;
    skos:topConceptOf cs: ;
.

:hydrothermal
    a skos:Concept ;
    rdfs:isDefinedBy cs: ;
    skos:definition "A group name for lithologies formed from precipitation from a hot hydrous solution, with or without demonstrable association with igneous processes. Adapted from Glossary of geology (Neuendorf et al., 2011, 5th edition, revised)."@en ;
    skos:historyNote "Based on the Glossary of geology (5th edition, revised; Neuendorf et al. 2011)." ;
    skos:inScheme cs: ;
    skos:narrower
        :baryte-vein ,
        :calcite-vein ,
        :epidote-vein ,
        :fluorite-vein ,
        :goethite-hematite-vein ,
        :hydrothermal-breccia ,
        :hydrothermal-chert ,
        :hydrothermal-rock ,
        :hydrothermal-rock-undivided ,
        :massive-sulfide ,
        :quartz-vein ,
        :tourmaline-vein ,
        :vein ;
    skos:notation "z"^^:gswa-rock-code ;
    skos:prefLabel "hydrothermal"@en ;
    skos:topConceptOf cs: ;
    schema:citation "https://glossary.americangeosciences.org/term/hydrothermalpetrology"^^xsd:anyURI ;
.

:igneous-feldspathoid-bearing-volcanic
    a skos:Concept ;
    rdfs:isDefinedBy cs: ;
    skos:definition "A group name for volcanic, silica-undersaturated lithologies that are characterized by the presence of feldspathoid (or foid, F) mineral phases, where the feldspathoid content is between 0 and 10% (cf. Le Maitre et al., 2005, p. 31) and the modal content of mafic and related minerals (M) is less than 90% (Le Maitre et al., 2005, p.  4). Note that the GSWA rock classification scheme does not include volcanic rocks with F greater than 10%. GSWA's rock classification scheme prefers the use of volcanic terminology for any igneous rock formed on or near the Earth's surface, i.e. for those hypabyssal or subvolcanic rocks such as dykes, sills, and cryptodomes that are demonstrably both spatially and temporally associated with extrusive volcanic rocks."@en ;
    skos:historyNote "Based on the IUGS classification of igneous rocks (Le Maitre et al., 2005) and GSWA usage." ;
    skos:inScheme cs: ;
    skos:narrower
        :feldspathoid-bearing-volcanic-rock ,
        :foid-bearing-latite ,
        :foid-bearing-trachyte ,
        :foid-bearing-volcanic-rock-undivided ,
        :foid-bearing-volcaniclastic-breccia ,
        :foid-bearing-volcaniclastic-breccia-sandstone ,
        :foid-bearing-volcaniclastic-conglomerate ,
        :foid-bearing-volcaniclastic-granule-pebble-breccia ,
        :foid-bearing-volcaniclastic-mudstone ,
        :foid-bearing-volcaniclastic-rock ,
        :foid-bearing-volcaniclastic-sandstone ,
        :foid-bearing-volcaniclastic-sandstone-siltstone ,
        :foid-bearing-volcaniclastic-sediment-matrix-breccia ;
    skos:notation "l"^^:gswa-rock-code ;
    skos:prefLabel "igneous feldspathoid-bearing volcanic"@en ;
    skos:topConceptOf cs: ;
.

:meta-igneous-mafic-volcanic
    a skos:Concept ;
    rdfs:isDefinedBy cs: ;
    skos:definition "A group name for metamorphosed volcanic and volcaniclastic lithologies composed chiefly of one or more ferromagnesian, dark-coloured minerals and derived from volcanic protoliths with M less than 90% (cf. Le Maitre et al., 2005, p. 153), where M represents the volume modal percentage of mafic and related minerals (Le Maitre et al., 2005, p. 4). GSWA's rock classification scheme prefers the use of volcanic terminology for any igneous rock formed on or near the Earth's surface, i.e. for those hypabyssal or subvolcanic rocks such as dykes, sills, and cryptodomes that are demonstrably both spatially and temporally associated with extrusive volcanic rocks."@en ;
    skos:historyNote "Based on the IUGS classification of metamorphic (Fettes and Desmons, 2007) and igneous rocks (Le Maitre et al., 2005)." ;
    skos:inScheme cs: ;
    skos:narrower
        :amphibolite-derived-from-volcanic-rock ,
        :carbonate-altered-metamafic-volcanic-rock ,
        :mafic-gneiss-derived-from-volcanic-rock ,
        :mafic-granofels-hornfels-derived-from-volcanic-rock ,
        :mafic-schist-derived-from-volcanic-rock ,
        :meta-pyroxene-spinifex-textured-basalt ,
        :metabasalt ,
        :metabasaltic-andesite ,
        :metakomatiitic-basalt ,
        :metamafic-volcanic-rock ,
        :metamafic-volcaniclastic-rock ,
        :mylonitized-metamafic-volcanic-rock ,
        :silicified-metamafic-volcanic-rock ;
    skos:notation "mb"^^:gswa-rock-code ;
    skos:prefLabel "meta-igneous mafic volcanic"@en ;
    skos:topConceptOf cs: ;
    schema:citation "https://glossary.americangeosciences.org/term/mafic"^^xsd:anyURI ;
.

:metamorphic-protolith-unknown-gneiss
    a skos:Concept ;
    rdfs:isDefinedBy cs: ;
    skos:definition "A group name for metamorphic rocks for which a protolith cannot be conclusively established and displaying a gneissose structure, i.e. a type of structure characterized by a schistosity that is either poorly developed throughout the rock or, if well developed, occurs in broadly spaced zones, such that the rock will split on a scale of more than one centimetre. Mineralogical or lithological layering is commonly present. (Cf. Fettes and Desmons, 2007, p. 154–155)."@en ;
    skos:historyNote "Based on the IUGS classification of metamorphic rocks (Fettes and Desmons, 2007)." ;
    skos:inScheme cs: ;
    skos:narrower
        :amphibolitic-gneiss ,
        :carbonate-gneiss ,
        :chloritic-gneiss ,
        :feldspathic-gneiss ,
        :ferruginous-gneiss ,
        :gneiss ,
        :gneissose-granulite ,
        :graphitic-gneiss ,
        :micaceous-gneiss ,
        :migmatitic-gneiss ,
        :pyroxenitic-gneiss ,
        :quartzofeldspathic-gneiss ,
        :quartzose-gneiss ;
    skos:notation "mn"^^:gswa-rock-code ;
    skos:prefLabel "metamorphic protolith unknown: gneiss"@en ;
    skos:topConceptOf cs: ;
    schema:citation "https://glossary.americangeosciences.org/term/gneiss"^^xsd:anyURI ;
.

:metamorphic-protolith-unknown-granofels-hornfels
    a skos:Concept ;
    rdfs:isDefinedBy cs: ;
    skos:definition "A group name for metamorphic rocks for which a protolith cannot be conclusively established and displaying a granofelsic structure, i.e. a structure resulting from the absence of schistosity such that the mineral grains and aggregates of mineral grains are equant (for example quartz, feldspar, garnet and pyroxene) or, if inequant, have a random orientation. Mineralogical or lithological layering may be present. Definition adapted from Fettes and Desmons (2007, p. 156). Hornfels are granofels that are typically formed by contact metasomatism and occur mostly (though not exclusively) in the innermost part of contact aureoles. Definition adapted from Fettes and Desmons (2007, p. 159) and Glossary of geology 2011, 5th edition revised)."@en ;
    skos:historyNote "Based on the IUGS classification of metamorphic rocks (Fettes and Desmons, 2007)." ;
    skos:inScheme cs: ;
    skos:narrower
        :amphibolitic-granofels-hornfels ,
        :carbonate-granofels-hornfels ,
        :chloritic-granofels-hornfels ,
        :feldspathic-granofels-hornfels ,
        :ferruginous-granofels-hornfels ,
        :granofels-hornfels ,
        :granofelsic-granulite ,
        :graphitic-granofels-hornfels ,
        :micaceous-granofels-hornfels ,
        :migmatitic-granofels-hornfels ,
        :pyroxenitic-granofels-hornfels ,
        :quartzofeldspathic-granofels-hornfels ,
        :quartzose-hornfels ;
    skos:notation "me"^^:gswa-rock-code ;
    skos:prefLabel "metamorphic protolith unknown: granofels/hornfels"@en ;
    skos:topConceptOf cs: ;
    schema:citation
        "https://glossary.americangeosciences.org/term/granofels"^^xsd:anyURI ,
        "https://glossary.americangeosciences.org/term/hornfels"^^xsd:anyURI ;
.

:igneous-carbonatite
    a skos:Concept ;
    rdfs:isDefinedBy cs: ;
    skos:definition "A group name for igneous rocks containing more than 50% modal carbonates. Carbonatites may be either intrusive or volcanic in origin, and are distinguished based on the relative abundance of different carbonate phases. (cf. Le Maitre et al., 2005, p. 10)."@en ;
    skos:historyNote "Based on the IUGS classification of igneous rocks (Le Maitre et al., 2005)." ;
    skos:inScheme cs: ;
    skos:narrower
        :calcite-carbonatite ,
        :carbonatite ,
        :carbonatitic-rock-undivided ,
        :carbonatitic-volcaniclastic-breccia ,
        :carbonatitic-volcaniclastic-breccia-sandstone ,
        :carbonatitic-volcaniclastic-conglomerate ,
        :carbonatitic-volcaniclastic-granule-pebble-breccia ,
        :carbonatitic-volcaniclastic-mudstone ,
        :carbonatitic-volcaniclastic-rock ,
        :carbonatitic-volcaniclastic-sandstone ,
        :carbonatitic-volcaniclastic-sandstone-siltstone ,
        :carbonatitic-volcaniclastic-sediment-matrix-breccia ,
        :dolomite-carbonatite ,
        :ferro-carbonatite ;
    skos:notation "r"^^:gswa-rock-code ;
    skos:prefLabel "igneous carbonatite"@en ;
    skos:topConceptOf cs: ;
    schema:citation "https://glossary.americangeosciences.org/term/carbonatite"^^xsd:anyURI ;
.

:meta-igneous-mafic-intrusive
    a skos:Concept ;
    rdfs:isDefinedBy cs: ;
    skos:definition "A group name for metamorphosed intrusive lithologies (and including coarse-grained parts of extrusive successions) derived from protoliths composed chiefly of one or ferromagnesian, dark-coloured minerals in their mode (cf. Le Maitre et al., 2005, p. 25 and 107) and with the volume modal percentage of mafic and related minerals (M) less then 90%. As for their protolith equivalents, metamorphic lithologies in this group are distinguished by the relative abundance of orthopyroxene, clinopyroxene, olivine and hornblende (cf. Le Maitre et al., 2005, p. 24)."@en ;
    skos:historyNote "Based on the IUGS classification of metamorphic (Fettes and Desmons, 2007) and igneous rocks (Le Maitre et al., 2005)." ;
    skos:inScheme cs: ;
    skos:narrower
        :amphibolite-derived-from-intrusive-rock ,
        :mafic-gneiss-derived-from-intrusive-rock ,
        :mafic-granofels-hornfels-derived-from-intrusive-rock ,
        :mafic-schist-derived-from-intrusive-rock ,
        :meta-anorthosite ,
        :meta-olivine-gabbro ,
        :metadolerite ,
        :metagabbro ,
        :metagabbronorite ,
        :metamafic-intrusive-rock ,
        :metanorite ,
        :metatroctolite ,
        :mylonitized-metamafic-intrusive-rock ,
        :silicified-metamafic-intrusive-rock ;
    skos:notation "mo"^^:gswa-rock-code ;
    skos:prefLabel "meta-igneous mafic intrusive"@en ;
    skos:topConceptOf cs: ;
.

:metamorphic-protolith-unknown-schist
    a skos:Concept ;
    rdfs:isDefinedBy cs: ;
    skos:definition "A group name for metamorphic rocks for which a protolith cannot be conclusively established and displaying a schistose structure, i.e. a type of structure characterized by a schistosity that is either poorly developed throughout the rock or, if well developed, occurs in broadly spaced zones, such that the rock will split on a scale of more than one centimetre. Mineralogical or lithological layering is commonly present. Cf. Fettes and Desmons (2007, p.  193)."@en ;
    skos:historyNote "Based on the IUGS classification of metamorphic rocks (Fettes and Desmons, 2007)." ;
    skos:inScheme cs: ;
    skos:narrower
        :amphibolitic-schist ,
        :carbonate-schist ,
        :chloritic-schist ,
        :feldspathic-schist ,
        :ferruginous-schist ,
        :graphitic-schist ,
        :micaceous-schist ,
        :migmatitic-schist ,
        :pyroxenitic-schist ,
        :quartz-mica-schist ,
        :quartzofeldspathic-schist ,
        :quartzose-schist ,
        :schist ,
        :schistose-granulite ;
    skos:notation "ms"^^:gswa-rock-code ;
    skos:prefLabel "metamorphic protolith unknown: schist"@en ;
    skos:topConceptOf cs: ;
    schema:citation "https://glossary.americangeosciences.org/term/schist"^^xsd:anyURI ;
.

:igneous-mafic-volcanic
    a skos:Concept ;
    rdfs:isDefinedBy cs: ;
    skos:definition "A group name for volcanic and volcaniclastic lithologies composed chiefly of one or more ferromagnesian, dark-coloured minerals such as olivine, pyroxene, etc. in their mode, with the volume modal percentage of mafic and related minerals (M) less than 90% (cf. Le Maitre et al., 2005, p. 4 and 107). GSWA's rock classification scheme prefers the use of volcanic terminology for any igneous rock formed on or near the Earth's surface, i.e. for those hypabyssal or subvolcanic rocks such as dykes, sills, and cryptodomes that are demonstrably both spatially and temporally associated with extrusive volcanic rocks."@en ;
    skos:historyNote "Based on the IUGS classification of igneous rocks (Le Maitre et al., 2005)." ;
    skos:inScheme cs: ;
    skos:narrower
        :basalt ,
        :basaltic-andesite ,
        :komatiitic-basalt ,
        :mafic-volcanic-rock ,
        :mafic-volcanic-rock-undivided ,
        :mafic-volcaniclastic-breccia ,
        :mafic-volcaniclastic-breccia-sandstone ,
        :mafic-volcaniclastic-conglomerate ,
        :mafic-volcaniclastic-granule-pebble-breccia ,
        :mafic-volcaniclastic-mudstone ,
        :mafic-volcaniclastic-rock ,
        :mafic-volcaniclastic-sandstone ,
        :mafic-volcaniclastic-sandstone-siltstone ,
        :mafic-volcaniclastic-sediment-matrix-breccia ,
        :pyroxene-spinifex-textured-basalt ;
    skos:notation "b"^^:gswa-rock-code ;
    skos:prefLabel "igneous mafic volcanic"@en ;
    skos:topConceptOf cs: ;
    schema:citation "https://glossary.americangeosciences.org/term/mafic"^^xsd:anyURI ;
.

:igneous-ultramafic-volcanic-and-volcaniclastic
    a skos:Concept ;
    rdfs:isDefinedBy cs: ;
    skos:definition "A group name for volcanic and volcaniclastic lithologies composed chiefly of one or more ferromagnesian, dark-coloured minerals such as olivine, pyroxene, etc. in their mode, with the volume modal percentage of mafic and related minerals (M) greater than or equal to 90% (cf. Le Maitre et al., 2005, p. 4). GSWA's rock classification scheme prefers the use of volcanic terminology for any igneous rock formed on or near the Earth's surface, i.e. for those hypabyssal or subvolcanic rocks such as dykes, sills, and cryptodomes that are demonstrably both spatially and temporally associated with extrusive volcanic rocks."@en ;
    skos:historyNote "Based on the IUGS classification of igneous rocks (Le Maitre et al., 2005)." ;
    skos:inScheme cs: ;
    skos:narrower
        :dunite-volcanic ,
        :komatiite ,
        :peridotite ,
        :pyroxenite-extrusive ,
        :ultramafic-volcanic-rock ,
        :ultramafic-volcanic-rock-undivided ,
        :ultramafic-volcaniclastic-breccia ,
        :ultramafic-volcaniclastic-breccia-sandstone ,
        :ultramafic-volcaniclastic-conglomerate ,
        :ultramafic-volcaniclastic-granule-pebble-breccia ,
        :ultramafic-volcaniclastic-mudstone ,
        :ultramafic-volcaniclastic-rock ,
        :ultramafic-volcaniclastic-sandstone ,
        :ultramafic-volcaniclastic-sandstone-siltstone ,
        :ultramafic-volcaniclastic-sediment-matrix-breccia ;
    skos:notation "u"^^:gswa-rock-code ;
    skos:prefLabel "igneous ultramafic volcanic and volcaniclastic"@en ;
    skos:topConceptOf cs: ;
.

:meta-igneous-felsic-volcanic
    a skos:Concept ;
    rdfs:isDefinedBy cs: ;
    skos:definition "A group name for metamorphosed volcanic (and volcaniclastic) lithologies composed chiefly of felsic minerals and derived from volcanic protoliths with M less than 90% (cf. Le Maitre et al., 2005, p. 153), where M represents the volume modal percentage of mafic and related minerals (Le Maitre et al., 2005, p. 4). GSWA's rock classification scheme prefers the use of volcanic terminology for any igneous rock formed on or near the Earth's surface, i.e. for those hypabyssal or subvolcanic rocks such as dykes, sills, and cryptodomes that are demonstrably both spatially and temporally associated with extrusive volcanic rocks."@en ;
    skos:historyNote "Based on the IUGS classification of metamorphic (Fettes and Desmons, 2007) and igneous rocks (Le Maitre et al., 2005)." ;
    skos:inScheme cs: ;
    skos:narrower
        :felsic-gneiss-derived-from-volcanic-rock ,
        :felsic-granofels-hornfels-derived-from-volcanic-rock ,
        :felsic-schist-derived-from-volcanic-rock ,
        :meta-andesite ,
        :meta-quartz-latite ,
        :meta-quartz-trachyte ,
        :metadacite ,
        :metafelsic-volcanic-rock ,
        :metafelsic-volcaniclastic-rock ,
        :metalatite ,
        :metarhyodacite ,
        :metarhyolite ,
        :metatrachyte ,
        :mylonitized-metafelsic-volcanic-rock ,
        :silicified-metafelsic-volcanic-rock ;
    skos:notation "mf"^^:gswa-rock-code ;
    skos:prefLabel "meta-igneous felsic volcanic"@en ;
    skos:topConceptOf cs: ;
    schema:citation "https://glossary.americangeosciences.org/term/felsic"^^xsd:anyURI ;
.

:dolomite
    a skos:Concept ;
    rdfs:isDefinedBy cs: ;
    skos:altLabel
        "dolomite rock"@en ,
        "dolostone"@en ;
    skos:broader :sedimentary-carbonate ;
    skos:definition "A carbonate sedimentary rock of which more than 50% by weight or by areal percentages under the microscope consists of the mineral dolomite, or a variety of limestone rich in magnesium carbonate; specifically a carbonate sedimentary rock containing more than 90% dolomite and less than 10% calcite, or one having a Ca/Mg ratio in the range of 1.5 – 1.7 (Chilingar, 1957), or one having an approximate MgO equivalent of 19.5 – 21.6% or magnesium–carbonate equivalent of 41.0 – 45.4% (Pettijohn, 1957, p. 418). Dolomite occurs with well-developed crystalline habits as well as anhedral forms, is clearly associated and commonly interbedded with limestone, and usually represents a post-depositional replacement of limestone. Adapted from Glossary of geology (5th edition revised; Neuendorf et al., 2011). GSWA usage has in the past included the term dolostone as a synonym of dolomite (rock), to avoid confusion with the mineral dolomite; however, dolomite (rock) has technical precedence over dolostone, and use of the latter is discouraged."@en ;
    skos:exactMatch
        <http://inspire.ec.europa.eu/codelist/LithologyValue/dolostone> ,
        <http://resource.geosciml.org/classifier/cgi/lithology/dolostone> ;
    skos:historyNote """Pettijohn, FJ 1957, Sedimentary rocks, Harper and Brothers, New York, 718p.,
Chilingar, GV, Bissell, HJ and Wolf, KH 1967, Chapter 5 Diagenesis of Carbonate Rocks: in Developments in Sedimentology, v. 8, p. 179–322, doi:10.1016/S0070-4571(08)70844-6.""" ;
    skos:inScheme cs: ;
    skos:narrower
        :crystalline-dolomite ,
        :dolarenite ,
        :doloboundstone ,
        :dolobreccia ,
        :dolofloatstone ,
        :dolograinstone ,
        :dololutite ,
        :dolomudstone ,
        :dolopackstone ,
        :dolorudite ,
        :dolorudstone ,
        :dolowackestone ,
        :microbialitic-dolomite ,
        :microbially-laminated-dolomite ,
        :oolitic-peloidal-dolomite ,
        :stromatoporoid-dolomite ;
    skos:notation "kd"^^:gswa-rock-code ;
    skos:prefLabel "dolomite"@en ;
    schema:citation
        "https://en.wikipedia.org/wiki/Dolomite_(rock)"^^xsd:anyURI ,
        "https://glossary.americangeosciences.org/term/dolomitesed"^^xsd:anyURI ;
.

:igneous-foid-bearing-intrusive
    a skos:Concept ;
    rdfs:isDefinedBy cs: ;
    skos:definition "A group name for intrusive, silica-undersaturated lithologies that are characterized by the presence of feldspathoid (or foid, F) mineral phases (e.g. nepheline, leucite, kalsilite, analcime, sodalite, etc.), where the feldspathoid content is between 0 and 100% (cf. Le Maitre et al., 2005, p. 22). When preceding a rock name (syenite, monzonite, etc.) the modifier 'foid-bearing' indicates an intrusive rock with F between 0 and 10% of the modal composition; when F is greater than 10, the term 'foid' is used in front of the rock name."@en ;
    skos:historyNote "Based on the IUGS classification of igneous rocks (Le Maitre et al., 2005)." ;
    skos:inScheme cs: ;
    skos:narrower
        :foid-bearing-alkali-feldspar-syenite ,
        :foid-bearing-anorthosite ,
        :foid-bearing-diorite ,
        :foid-bearing-gabbro ,
        :foid-bearing-intrusive-rock ,
        :foid-bearing-intrusive-rock-undivided ,
        :foid-bearing-monzodiorite ,
        :foid-bearing-monzogabbro ,
        :foid-bearing-monzonite ,
        :foid-bearing-syenite ,
        :foid-diorite ,
        :foid-gabbro ,
        :foid-monzodiorite ,
        :foid-monzogabbro ,
        :foid-monzosyenite ,
        :foid-syenite ;
    skos:notation "d"^^:gswa-rock-code ;
    skos:prefLabel "igneous foid-bearing intrusive"@en ;
    skos:topConceptOf cs: ;
    schema:citation "https://glossary.americangeosciences.org/term/foidbearing"^^xsd:anyURI ;
.

:limestone
    a skos:Concept ;
    rdfs:isDefinedBy cs: ;
    skos:broader :sedimentary-carbonate ;
    skos:definition "A sedimentary rock consisting chiefly (more than 50% by weight or by areal percentages under the microscope) of calcium carbonate, primarily in the form of the mineral calcite, and with or without magnesium carbonate; specifically a carbonate sedimentary rock containing more than 95% calcite and less than 5% dolomite. Common minor constituents include silica (chalcedony), feldspar, clays, pyrite, and siderite. Limestones are formed by either biotic or abiotic processes, and may be detrital, chemical, oolitic, earthy, crystalline, or recrystallized; many are highly fossiliferous and clearly represent ancient shell banks or coral reefs. Adapted from Glossary of geology (5th edition revised; Neuendorf et al., 2011)."@en ;
    skos:exactMatch
        <http://inspire.ec.europa.eu/codelist/LithologyValue/limestone> ,
        <http://resource.geosciml.org/classifier/cgi/lithology/limestone> ;
    skos:historyNote "Based on the Glossary of geology (5th edition, revised; Neuendorf et al. 2011)." ;
    skos:inScheme cs: ;
    skos:narrower
        :calcarenite ,
        :calcilutite ,
        :calcirudite ,
        :coquina ,
        :crystalline-limestone ,
        :limestone-boundstone ,
        :limestone-breccia ,
        :limestone-floatstone ,
        :limestone-grainstone ,
        :limestone-mudstone ,
        :limestone-packstone ,
        :limestone-rudstone ,
        :limestone-wackestone ,
        :microbialitic-limestone ,
        :microbially-laminated-limestone ,
        :oolitic-peloidal-limestone ,
        :stromatoporoid-limestone ;
    skos:notation "kl"^^:gswa-rock-code ;
    skos:prefLabel "limestone"@en ;
    schema:citation "https://glossary.americangeosciences.org/term/limestone"^^xsd:anyURI ;
.

:meta-igneous-felsic-intrusive
    a skos:Concept ;
    rdfs:isDefinedBy cs: ;
    skos:definition "A group name for metamorphosed intrusive lithologies that are composed chiefly of felsic minerals, i.e. derived from intrusive protoliths with modal quartz and feldspar and M smaller than 90% (cf. Le Maitre et al., 2005, p. 153), where M represents the volume modal percentage of mafic and related minerals (Le Maitre et al., 2005, p. 4)."@en ;
    skos:historyNote "Based on the IUGS classification of metamorphic (Fettes and Desmons, 2007) and igneous rocks (Le Maitre et al., 2005)." ;
    skos:inScheme cs: ;
    skos:narrower
        :foliated-metagranite ,
        :granitic-gneiss ,
        :granitic-granofels-hornfels ,
        :granitic-schist ,
        :meta-quartz-diorite ,
        :metadiorite ,
        :metagranitic-rock ,
        :metagranodiorite ,
        :metamonzodiorite ,
        :metamonzogranite ,
        :metamonzonite ,
        :metapegmatite ,
        :metasyenite ,
        :metasyenogranite ,
        :metatonalite ,
        :mylonitized-metagranitic-rock ,
        :silicified-metagranitic-rock ;
    skos:notation "mg"^^:gswa-rock-code ;
    skos:prefLabel "meta-igneous felsic intrusive"@en ;
    skos:topConceptOf cs: ;
.

:igneous-felsic-volcanic
    a skos:Concept ;
    rdfs:isDefinedBy cs: ;
    skos:definition "A group name for volcanic and volcaniclastic lithologies composed chiefly of one or more felsic minerals (i.e. containing modal quartz and feldspar but little or no feldspathoids), with modal content of mafic and related minerals (M) less than 90%. GSWA's rock classification scheme prefers the use of volcanic terminology for any igneous rock formed on or near the Earth's surface, i.e. for those hypabyssal or subvolcanic rocks such as dykes, sills, and cryptodomes that are demonstrably both spatially and temporally associated with extrusive volcanic rocks."@en ;
    skos:historyNote "Based on the IUGS classification of igneous rocks (Le Maitre et al., 2005)." ;
    skos:inScheme cs: ;
    skos:narrower
        :andesite ,
        :dacite ,
        :felsic-volcanic-rock ,
        :felsic-volcanic-rock-undivided ,
        :felsic-volcaniclastic-breccia ,
        :felsic-volcaniclastic-breccia-sandstone ,
        :felsic-volcaniclastic-conglomerate ,
        :felsic-volcaniclastic-granule-pebble-breccia ,
        :felsic-volcaniclastic-mudstone ,
        :felsic-volcaniclastic-rock ,
        :felsic-volcaniclastic-sandstone ,
        :felsic-volcaniclastic-sandstone-siltstone ,
        :felsic-volcaniclastic-sediment-matrix-breccia ,
        :latite ,
        :quartz-latite ,
        :quartz-trachyte ,
        :rhyodacite ,
        :rhyolite ,
        :trachyte ;
    skos:notation "f"^^:gswa-rock-code ;
    skos:prefLabel "igneous felsic volcanic"@en ;
    skos:topConceptOf cs: ;
    schema:citation "https://glossary.americangeosciences.org/term/felsic"^^xsd:anyURI ;
.

:sedimentary-other-chemical-or-biochemical
    a skos:Concept ;
    rdfs:isDefinedBy cs: ;
    skos:definition "A group name for sedimentary rocks composed primarily of material formed directly by (a) precipitation from solution or colloidal suspension (as by evaporation), (b) by the deposition of insoluble precipitates (as by mixing solutions of two soluble salts), or (c) resulting directly or indirectly from the chemical processes and activities of living organisms. Adapted from Glossary of geology (5th edition revised; Neuendorf et al., 2011)."@en ;
    skos:historyNote "Based on the Glossary of geology (5th edition, revised; Neuendorf et al. 2011)." ;
    skos:inScheme cs: ;
    skos:narrower
        :baryte ,
        :chalk ,
        :chemical-or-biochemical-rock ,
        :chemical-or-biochemical-rock-undivided ,
        :chert ,
        :coal ,
        :diatomite ,
        :evaporite ,
        :iron-formation ,
        :ironstone ,
        :mixed-chert-and-iron-formation ,
        :mixed-chert-and-mudstone ,
        :mixed-iron-formation-and-mudstone ,
        :phosphorite ,
        :pisolite ,
        :radiolarite ,
        :siliceous-sinter ,
        :spongolite-spicularite ,
        :travertine ;
    skos:notation "c"^^:gswa-rock-code ;
    skos:prefLabel "sedimentary other chemical or biochemical"@en ;
    skos:topConceptOf cs: ;
    schema:citation "https://openpress.usask.ca/physicalgeology/chapter/9-2-chemical-and-biochemical-sedimentary-rocks-2/"^^xsd:anyURI ;
.

:igneous-mafic-intrusive
    a skos:Concept ;
    rdfs:isDefinedBy cs: ;
    skos:definition "A group name for intrusive lithologies (and including coarse-grained parts of extrusive successions) that are composed chiefly of one or more ferromagnesian, dark-coloured minerals in their mode (cf. Le Maitre et al., 2005, p. 25 and 107) and with the volume modal percentage of mafic and related minerals (M) less then 90%. Individual lithologies within the group are distinguished by the relative abundance of orthopyroxene, clinopyroxene, olivine and hornblende (cf. Le Maitre et al., 2005, p. 24)."@en ;
    skos:historyNote "Based on the IUGS classification of igneous rocks (Le Maitre et al., 2005)." ;
    skos:inScheme cs: ;
    skos:narrower
        :anorthosite ,
        :clinopyroxene-gabbro ,
        :dolerite ,
        :gabbro ,
        :gabbronorite ,
        :hornblende-gabbro ,
        :mafic-intrusive-rock ,
        :mafic-intrusive-rock-undivided ,
        :magnetite-gabbro ,
        :norite ,
        :olivine-clinopyroxene-norite ,
        :olivine-gabbro ,
        :olivine-gabbronorite ,
        :olivine-norite ,
        :olivine-orthopyroxene-gabbro ,
        :orthopyroxene-gabbro ,
        :pyroxene-hornblende-gabbro ,
        :pyroxene-hornblende-gabbronorite ,
        :pyroxene-hornblende-norite ,
        :troctolite ;
    skos:notation "o"^^:gswa-rock-code ;
    skos:prefLabel "igneous mafic intrusive"@en ;
    skos:topConceptOf cs: ;
    schema:citation "https://glossary.americangeosciences.org/term/mafic"^^xsd:anyURI ;
.

:igneous-lamproites
    a skos:Concept ;
    rdfs:isDefinedBy cs: ;
    skos:definition "A group name for hypabyssal or extrusive rocks rich in potassium and magnesium, usually occurring as dyke or small intrusions. The subdivision of the lamproites follows the scheme of Mitchell and Bergman (1991; Petrology of lamproites: Plenum Press, New York, London, 447p.; https://link.springer.com/book/10.1007/978-1-4615-3788-5), in which the historical terminology (e.g. wyomingite, madupite, etc.) is discarded in favour of compound names based on the predominance of phlogopite, richterite, olivine, diopside, sanidine and leucite (Le Maitre et al., 2005, p. 16)."@en ;
    skos:historyNote "Based on the IUGS classification of igneous rocks (Le Maitre et al., 2005)." ;
    skos:inScheme cs: ;
    skos:narrower
        :diopside-leucite-lamproite ,
        :diopside-leucite-phlogopite-lamproite ,
        :diopside-leucite-richterite-madupitic-lamproite ,
        :diopside-madupitic-lamproite ,
        :diopside-sanidine-phlogopite-lamproite ,
        :enstatite-sanidine-phlogopite-lamproite ,
        :hyalo-enstatite-phlogopite-lamproite ,
        :hyalo-olivine-diopside-phlogopite-lamproite ,
        :lamproite ,
        :lamproitic-rock-undivided ,
        :lamproitic-volcaniclastic-breccia ,
        :lamproitic-volcaniclastic-breccia-sandstone ,
        :lamproitic-volcaniclastic-conglomerate ,
        :lamproitic-volcaniclastic-granule-pebble-breccia ,
        :lamproitic-volcaniclastic-mudstone ,
        :lamproitic-volcaniclastic-rock ,
        :lamproitic-volcaniclastic-sandstone ,
        :lamproitic-volcaniclastic-sandstone-siltstone ,
        :lamproitic-volcaniclastic-sediment-matrix-breccia ,
        :leucite-phlogopite-lamproite ,
        :leucite-richterite-lamproite ,
        :olivine-diopside-richterite-madupitic-lamproite ;
    skos:notation "i"^^:gswa-rock-code ;
    skos:prefLabel "igneous lamproites"@en ;
    skos:topConceptOf cs: ;
    schema:citation "https://glossary.americangeosciences.org/term/lamproite"^^xsd:anyURI ;
.

:sedimentary-siliciclastic
    a skos:Concept ;
    rdfs:isDefinedBy cs: ;
    skos:definition "A group name for sedimentary lithologies that are silicon-bearing (in the form of quartz and silicates) and are composed principally of broken fragments that are derived from pre-existing rocks or minerals and that have been transported some distance from their places of origin. Adapted from Glossary of geology (5th edition revised; Neuendorf et al., 2011)"@en ;
    skos:historyNote "Compiled by the Geological Survey of Western Australia" ;
    skos:inScheme cs: ;
    skos:narrower
        :arenite ,
        :arkose ,
        :conglomerate ,
        :conglomerate-plus-sandstone ,
        :conglomerate-with-other-siliciclastic-rock ,
        :diamictite ,
        :diamictite-with-other-siliciclastic ,
        :mixed-siliciclastic-and-volcanic-rocks ,
        :mudstone ,
        :pebbly-sandstone ,
        :sand ,
        :sandstone ,
        :sandstone-with-conglomerate ,
        :sandstone-with-other-siliciclastic-rock ,
        :sandstone-with-siltstone ,
        :sedimentary-breccia ,
        :shale ,
        :siliciclastic-rock ,
        :siliciclastic-rock-undivided ,
        :siliciclastic-with-lesser-carbonate ,
        :siltstone-with-sandstone ,
        :wacke ;
    skos:notation "s"^^:gswa-rock-code ;
    skos:prefLabel "sedimentary siliciclastic"@en ;
    skos:topConceptOf cs: ;
    schema:citation
        "https://glossary.americangeosciences.org/term/clastic"^^xsd:anyURI ,
        "https://glossary.americangeosciences.org/term/siliciclastic"^^xsd:anyURI ;
.

:igneous-ultramafic-intrusive
    a skos:Concept ;
    rdfs:isDefinedBy cs: ;
    skos:definition "A group name for intrusive lithologies composed chiefly of mafic minerals and with M greater than or equal to 90% (cf. Le Maitre et al., 2005, p. 153), where M represents the volume modal percentage of mafic and related minerals (Le Maitre et al., 2005, p. 4)."@en ;
    skos:historyNote "Based on the IUGS classification of igneous rocks (Le Maitre et al., 2005)." ;
    skos:inScheme cs: ;
    skos:narrower
        :chromitite ,
        :clinopyroxenite ,
        :dunite-intrusive ,
        :harzburgite ,
        :hornblende-peridotite ,
        :hornblende-pyroxenite ,
        :hornblendite ,
        :lherzolite ,
        :magnetitite ,
        :olivine-clinopyroxenite ,
        :olivine-hornblende-pyroxenite ,
        :olivine-hornblendite ,
        :olivine-orthopyroxenite ,
        :olivine-pyroxene-hornblendite ,
        :olivine-pyroxenite ,
        :olivine-websterite ,
        :orthopyroxenite ,
        :pyroxene-hornblende-peridotite ,
        :pyroxene-hornblendite ,
        :pyroxene-peridotite ,
        :pyroxenite-intrusive ,
        :ultramafic-intrusive-rock ,
        :ultramafic-intrusive-rock-undivided ,
        :websterite ,
        :wehrlite ;
    skos:notation "a"^^:gswa-rock-code ;
    skos:prefLabel "igneous ultramafic intrusive"@en ;
    skos:topConceptOf cs: ;
    schema:citation "https://glossary.americangeosciences.org/term/ultramafic"^^xsd:anyURI ;
.

:metamorphic-protolith-unknown-fault-rock
    a skos:Concept ;
    rdfs:isDefinedBy cs: ;
    skos:definition "A group name for lithologies physically associated with fault surfaces and genetically linked to fault movements (Glossary of geology, 5th edition revised; Neuendorf et al., 2011)."@en ;
    skos:historyNote "Based on the Glossary of geology (5th edition, revised; Neuendorf et al. 2011)." ;
    skos:inScheme cs: ;
    skos:narrower
        :amphibolitic-fault-rock ,
        :blastomylonite ,
        :carbonate-fault-rock ,
        :cataclasite ,
        :chloritic-fault-rock ,
        :crush-breccia ,
        :fault-breccia ,
        :fault-gouge ,
        :fault-rock ,
        :feldspathic-fault-rock ,
        :ferruginous-fault-rock ,
        :foliated-gouge ,
        :graphitic-fault-rock ,
        :micaceous-fault-rock ,
        :migmatitic-fault-rock ,
        :mylonite ,
        :phyllonite ,
        :protocataclasite ,
        :protomylonite ,
        :pseudotachylite-fault-rock ,
        :pyroxenitic-fault-rock ,
        :quartzofeldspathic-fault-rock ,
        :quartzose-fault-rock ,
        :schistose-fault-rock ,
        :ultracataclasite ,
        :ultramylonite ;
    skos:notation "my"^^:gswa-rock-code ;
    skos:prefLabel "metamorphic protolith unknown: fault rock"@en ;
    skos:topConceptOf cs: ;
    schema:citation "https://glossary.americangeosciences.org/term/faultrock"^^xsd:anyURI ;
.

:igneous-felsic-intrusive
    a skos:Concept ;
    rdfs:isDefinedBy cs: ;
    skos:altLabel "igneous granitic"@en ;
    skos:definition "A group name for intrusive lithologies composed chiefly of one or more felsic minerals (e.g. containing modal quartz, feldspar and feldspathoids), with modal content of mafic and related minerals (M) less than 90%, where M represents the volume modal percentage of mafic and related minerals (Le Maitre et al., 2005, p. 4). Previous GSWA usage of 'igneous granitic' is not recommended."@en ;
    skos:historyNote "Based on the IUGS classification of igneous rocks (Le Maitre et al., 2005) and GSWA usage." ;
    skos:inScheme cs: ;
    skos:narrower
        :alkali-feldspar-granite ,
        :alkali-feldspar-syenite ,
        :diorite ,
        :granitic-rock ,
        :granitic-rock-undivided ,
        :granodiorite ,
        :granophyre ,
        :micro-alkali-feldspar-granite ,
        :micro-alkali-feldspar-syenite ,
        :micro-granitic-rock-undivided ,
        :micro-quartz-alkali-feldspar-syenite ,
        :micro-quartz-anorthosite ,
        :micro-quartz-diorite ,
        :micro-quartz-gabbro ,
        :micro-quartz-monzodiorite ,
        :micro-quartz-monzogabbro ,
        :micro-quartz-monzonite ,
        :micro-quartz-syenite ,
        :microdiorite ,
        :microgranodiorite ,
        :micromonzodiorite ,
        :micromonzogabbro ,
        :micromonzogranite ,
        :micromonzonite ,
        :microsyenite ,
        :microsyenogranite ,
        :microtonalite ,
        :microtrondhjemite ,
        :monzodiorite ,
        :monzogabbro ,
        :monzogranite ,
        :monzonite ,
        :pegmatite ,
        :quartz-alkali-feldspar-syenite ,
        :quartz-anorthosite ,
        :quartz-diorite ,
        :quartz-gabbro ,
        :quartz-monzodiorite ,
        :quartz-monzogabbro ,
        :quartz-monzonite ,
        :quartz-syenite ,
        :syenite ,
        :syenogranite ,
        :tonalite ,
        :trondjhemite ;
    skos:notation "g"^^:gswa-rock-code ;
    skos:prefLabel "igneous felsic intrusive"@en ;
    skos:topConceptOf cs: ;
    schema:citation "https://glossary.americangeosciences.org/term/felsic"^^xsd:anyURI ;
.

:1.0 schema:name "1.0" .

cs:
    a skos:ConceptScheme ;
    reg:status <https://linked.data.gov.au/def/reg-statuses/stable> ;
    owl:versionIRI :1.0 ;
    skos:definition """Listing of rock types and lithological nomenclature (and related codes) used by the Geological Survey of Western Australia (GSWA) for the dual purpose of recording lithologies during mapping / core logging, and for representing mappable lithostratigraphic/lithotectonic units in the State. Rather than attempting to cover for all existing rock types and lithologies, the GSWA’s scheme and terms in this vocabulary are specifically informed by Western Australian geology; a companion vocabulary covers lithological equivalents for regolith materials. 

Apart from the approach to classification of some volcanic (pyroclastic) rocks, GSWA's lithological nomenclature largely conforms to internationally recognized classifications such as Le Maitre et al. (2005) for plutonic/intrusive rocks and Fettes and Desmons (2007) for metamorphic rocks. Note that: a) GSWA prefers the term intrusive to plutonic, as it carries no inference on depth of emplacement; b) GSWA's rock classification scheme prefers the use of volcanic terminology for any igneous rock formed on or near the Earth's surface, i.e. for those hypabyssal or sub-volcanic rocks such as dykes, sills, and cryptodomes that are demonstrably both spatially and temporally associated with extrusive volcanic rocks; c) some intrusive mafic/ultramafic terminology is allowed for cumulate rocks originating from thick volcanic successions. In the absence of a single unified scheme for sedimentary rocks, multiple sources were considered, and definitions rely heavily on the Glossary of geology (5th edition, revised; Neuendorf et al., 2011). Full references listed under History Note.

GSWA’s rock classification scheme is designed to provide consistent terminology within the organization, and primarily relies on features observable in all rocks at outcrop scale, in hand specimen, and in thin section. Additional terms cover for broader combinations of multiple lithologies encountered during mapping (especially for sedimentary rocks, e.g. ‘siliciclastic + lesser carbonate’), and to ensure a coherent approach across different rock types (e.g. use of ‘mylonitized’ for all metamorphic rock groups, even if some would be rare occurrences or difficult to identify in the field). Definitions in this vocabulary are largely compiled or derived from the quoted references and the Glossary of Geology (5th edition, revised, Neuendorf et al., 2011), with adaptions based on recommended GSWA usage; metamorphic lithologies are often derived from definitions of non-metamorphosed equivalents. Some mineralogical/petrological knowledge is expected of the reader.\n Each concept is characterized by a notation consisting of one to four lower-case letters. This notation represents the lithological code used for mapping lithologies and labelling lithostratigraphic units on maps. Note that in the GSWA's scheme, some lithological codes are reserved for use in the Field Observation database (WAROX) or the Explanatory Notes System (ENS) only; the latter are highlighted in the concept definitions and should not be used for field observations. Also note that in ENS codes are supplemented by primary and secondary qualifiers (not covered in this vocabulary); a concerted effort has been made to match WAROX-only codes with those generated via qualifiers in ENS, but in a few instances alphabetical limitations have prevented this (i.e. the code used in WAROX has a slightly different meaning from the same string of letters generated in ENS).

The approach behind GSWA’s rock classification scheme is documented in Tyler at al. (2004; https://dmpbookshop.eruditetechnologies.com.au/product/the-revised-gswa-rock-classification-scheme.do). Details of GSWA’s code construction for ENS can be found in Riganti et al. (2013; https://dmpbookshop.eruditetechnologies.com.au/product/gswa-code-builder-constructing-and-unravelling-gswa-geological-codes.do) and in a companion application, the GSWA Code Builder (ENS codes only), available from the Department’s Data and Software Centre (https://dasc.demirs.wa.gov.au/)."""@en ;
    
    skos:hasTopConcept
        :hydrothermal ,
        :igneous ,
        :igneous-carbonatite ,
        :igneous-feldspathoid-bearing-volcanic ,
        :igneous-felsic-intrusive ,
        :igneous-felsic-volcanic ,
        :igneous-foid-bearing-intrusive ,
        :igneous-intrusive ,
        :igneous-kalsilitic ,
        :igneous-kimberlite ,
        :igneous-lamproites ,
        :igneous-lamprophyres ,
        :igneous-mafic-intrusive ,
        :igneous-mafic-volcanic ,
        :igneous-melilitic ,
        :igneous-ultramafic-intrusive ,
        :igneous-ultramafic-volcanic-and-volcaniclastic ,
        :igneous-volcanic ,
        :meta-igneous ,
        :meta-igneous-carbonatite ,
        :meta-igneous-felsic ,
        :meta-igneous-felsic-intrusive ,
        :meta-igneous-felsic-volcanic ,
        :meta-igneous-mafic ,
        :meta-igneous-mafic-intrusive ,
        :meta-igneous-mafic-volcanic ,
        :meta-igneous-ultramafic-intrusive ,
        :meta-igneous-ultramafic-volcanic ,
        :meta-igneous-volcanic-or-volcaniclastic ,
        :metamorphic ,
        :metamorphic-protolith-unknown ,
        :metamorphic-protolith-unknown-fault-rock ,
        :metamorphic-protolith-unknown-gneiss ,
        :metamorphic-protolith-unknown-granofels-hornfels ,
        :metamorphic-protolith-unknown-impactite ,
        :metamorphic-protolith-unknown-schist ,
        :metamorphosed-hydrothermal ,
        :metasedimentary ,
        :metasedimentary-carbonate ,
        :metasedimentary-other-chemical ,
        :metasedimentary-other-chemical-meta-iron-formation ,
        :metasedimentary-siliciclastic ,
        :metasedimentary-siliciclastic-pelite ,
        :metasedimentary-siliciclastic-psammite ,
        :metasedimentary-siliciclastic-psammite-and-pelite-interlayered ,
        :metasedimentary-siliciclastic-psephite ,
        :metasedimentary-siliciclastic-semipelite ,
        :metasomatic ,
        :mixed ,
        :sedimentary ,
        :sedimentary-carbonate ,
        :sedimentary-other-chemical-or-biochemical ,
        :sedimentary-siliciclastic ,
        :unknown ,
        :xenolith-or-inclusion-bearing ;
    skos:historyNote """Derived from a revision of tables shared by the GSWA's field observation database, WAROX, and GSWA's Explanatory Notes System (ENS): [GEOLOGY].[Warox_REF.RockType], [GEOLOGY].[Warox_REF.RockName], and [GEOLOGY].[ENS_REF].[QUALIFIER] that are integral to GSWA's approach to map lithologies in the field and to code lithostratigraphic/lithotectonic units in the State. NB RockName is considered an equivalent term of lithology.

MAIN REFERENCES used for compilation:
-Fettes, D and Desmons, J 2007, Metamorphic rocks: a classification and glossary of terms: Cambridge University Press, Cambridge, UK, 244p.
-Le Maitre, RW, Streckeisen, A, Zanettin, B, Bas, M, Bonin, B and Bateman, P 2005, Igneous rocks: a classification and glossary of terms: recommendations of the International Union of Geological Sciences Subcommission on the Systematics of Igneous Rocks (2nd edition): Cambridge University Press, Cambridge, UK, 256p., doi:10.1017/CBO9780511535581
-Neuendorf, KKE, Mehl, JP Jr and Jackson, JA (editors), 2011, Glossary of Geology: Alexandria, Virginia, American Geological Institute, 799p.
-Riganti, A, Wallace, DJ, Fadadu, BC, Canham, DM, Gavni, KKR and Hocking, RM 2013, GSWA Code Builder – constructing and unravelling GSWA geological codes: Geological Survey of Western Australia, Record 2013/8, 15p. (https://dmpbookshop.eruditetechnologies.com.au/product/gswa-code-builder-constructing-and-unravelling-gswa-geological-codes.do)
-Tyler, IM. Morris, PA, Thorne, AM, Sheppard, s, Smithies, RH, Riganti, A, Doyle, MG, and Hocking, RM 2004, The revised GSWA rock classification scheme: Western Australia Geological Survey, Annual Review 2003–04, p. 88–94. (https://dmpbookshop.eruditetechnologies.com.au/product/the-revised-gswa-rock-classification-scheme.do)"""@en ;
    skos:prefLabel "GSWA rock classification scheme"@en ;
    prov:qualifiedAttribution
        [
            dcat:hadRole isoroles:custodian ;
            prov:agent
                [
                    a schema:Person ;
                    schema:email ""^^xsd:anyURI ;
                    schema:name "Terry Farrell" ;
                ] ;
        ] ,
        [
            dcat:hadRole isoroles:custodian ;
            prov:agent
                [
                    a schema:Person ;
                    schema:email ""^^xsd:anyURI ;
                    schema:name "Angela Riganti" ;
                ] ;
        ] ,
        [
            dcat:hadRole isoroles:custodian ;
            prov:agent
                [
                    a schema:Person ;
                    schema:email ""^^xsd:anyURI ;
                    schema:name "David Martin" ;
                ] ;
        ] ;
    schema:creator <https://linked.data.gov.au/org/gswa> ;
    schema:dateCreated "2024-06-28"^^xsd:date ;
    schema:dateModified "2024-07-12"^^xsd:date ;
    schema:keywords
        theme:geology-mapping ,
        theme:geology-framework ;
    schema:publisher <https://linked.data.gov.au/org/gswa> ;
    schema:version "1.0" ;
.

<http://inspire.ec.europa.eu/codelist/LithologyValue/alkaliFeldsparGranite> schema:name "alkali feldspar granite" .
<http://inspire.ec.europa.eu/codelist/LithologyValue/alkaliFeldsparSyenite> schema:name "alkali feldspar syenite" .
<http://inspire.ec.europa.eu/codelist/LithologyValue/amphibolite> schema:name "amphibolite" .
<http://inspire.ec.europa.eu/codelist/LithologyValue/andesite> schema:name "andesite" .
<http://inspire.ec.europa.eu/codelist/LithologyValue/anorthosite> schema:name "anorthosite" .
<http://inspire.ec.europa.eu/codelist/LithologyValue/anthraciteCoal> schema:name "anthracite coal" .
<http://inspire.ec.europa.eu/codelist/LithologyValue/arenite> schema:name "arenite" .
<http://inspire.ec.europa.eu/codelist/LithologyValue/basalt> schema:name "basalt" .
<http://inspire.ec.europa.eu/codelist/LithologyValue/bituminousCoal> schema:name "bituminousCoal" .
<http://inspire.ec.europa.eu/codelist/LithologyValue/boundstone> schema:name "boundstone" .
<http://inspire.ec.europa.eu/codelist/LithologyValue/carbonateMudstone> schema:name "carbonate mudstone" .
<http://inspire.ec.europa.eu/codelist/LithologyValue/carbonateRichMudstone> schema:name "carbonate-rich mudstone" .
<http://inspire.ec.europa.eu/codelist/LithologyValue/carbonateSedimentaryRock> schema:name "carbonate sedimentary rock" .
<http://inspire.ec.europa.eu/codelist/LithologyValue/carbonateWackestone> schema:name "carbonate wackestone" .
<http://inspire.ec.europa.eu/codelist/LithologyValue/carbonatite> schema:name "carbonatite" .
<http://inspire.ec.europa.eu/codelist/LithologyValue/chalk> schema:name "chalk" .
<http://inspire.ec.europa.eu/codelist/LithologyValue/clasticConglomerate> schema:name "clastic conglomerate" .
<http://inspire.ec.europa.eu/codelist/LithologyValue/clasticMudstone> schema:name "clastic mudstone" .
<http://inspire.ec.europa.eu/codelist/LithologyValue/clasticSandstone> schema:name "clastic sandstone" .
<http://inspire.ec.europa.eu/codelist/LithologyValue/clasticSedimentaryRock> schema:name "clastic sedimentary rock" .
<http://inspire.ec.europa.eu/codelist/LithologyValue/claystone> schema:name "claystone" .
<http://inspire.ec.europa.eu/codelist/LithologyValue/coal> schema:name "coal" .
<http://inspire.ec.europa.eu/codelist/LithologyValue/dacite> schema:name "dacite" .
<http://inspire.ec.europa.eu/codelist/LithologyValue/diamictite> schema:name "diamictite" .
<http://inspire.ec.europa.eu/codelist/LithologyValue/diorite> schema:name "diorite" .
<http://inspire.ec.europa.eu/codelist/LithologyValue/dolostone> schema:name "dolostone" .
<http://inspire.ec.europa.eu/codelist/LithologyValue/eclogite> schema:name "eclogite" .
<http://inspire.ec.europa.eu/codelist/LithologyValue/evaporite> schema:name "evaporite" .
<http://inspire.ec.europa.eu/codelist/LithologyValue/foidDiorite> schema:name "foidDiorite" .
<http://inspire.ec.europa.eu/codelist/LithologyValue/foidGabbro> schema:name "foidGabbro" .
<http://inspire.ec.europa.eu/codelist/LithologyValue/foidMonzodiorite> schema:name "foid monzodiorite" .
<http://inspire.ec.europa.eu/codelist/LithologyValue/foidMonzogabbro> schema:name "foid monzogabbro" .
<http://inspire.ec.europa.eu/codelist/LithologyValue/foidMonzosyenite> schema:name "foid monzosyenite" .
<http://inspire.ec.europa.eu/codelist/LithologyValue/foidSyenite> schema:name "foidSyenite" .
<http://inspire.ec.europa.eu/codelist/LithologyValue/framestone> schema:name "framestone" .
<http://inspire.ec.europa.eu/codelist/LithologyValue/gabbro> schema:name "gabbro" .
<http://inspire.ec.europa.eu/codelist/LithologyValue/gneiss> schema:name "gneiss" .
<http://inspire.ec.europa.eu/codelist/LithologyValue/grainstone> schema:name "grainstone" .
<http://inspire.ec.europa.eu/codelist/LithologyValue/granodiorite> schema:name "granodiorite" .
<http://inspire.ec.europa.eu/codelist/LithologyValue/granofels> schema:name "granofels" .
<http://inspire.ec.europa.eu/codelist/LithologyValue/granulite> schema:name "granulite" .
<http://inspire.ec.europa.eu/codelist/LithologyValue/hornblendite> schema:name "hornblendite" .
<http://inspire.ec.europa.eu/codelist/LithologyValue/hornfels> schema:name "hornfels" .
<http://inspire.ec.europa.eu/codelist/LithologyValue/igneousRock> schema:name "igneousRock" .
<http://inspire.ec.europa.eu/codelist/LithologyValue/latite> schema:name "latite" .
<http://inspire.ec.europa.eu/codelist/LithologyValue/lignite> schema:name "lignite" .
<http://inspire.ec.europa.eu/codelist/LithologyValue/limestone> schema:name "limestone" .
<http://inspire.ec.europa.eu/codelist/LithologyValue/marble> schema:name "marble" .
<http://inspire.ec.europa.eu/codelist/LithologyValue/metamorphicRock> schema:name "metamorphic rock" .
<http://inspire.ec.europa.eu/codelist/LithologyValue/metasomaticRock> schema:name "metasomatic rock" .
<http://inspire.ec.europa.eu/codelist/LithologyValue/monzodiorite> schema:name "monzodiorite" .
<http://inspire.ec.europa.eu/codelist/LithologyValue/monzogabbro> schema:name "monzogabbro" .
<http://inspire.ec.europa.eu/codelist/LithologyValue/monzogranite> schema:name "monzogranite" .
<http://inspire.ec.europa.eu/codelist/LithologyValue/monzonite> schema:name "monzonite" .
<http://inspire.ec.europa.eu/codelist/LithologyValue/packstone> schema:name "packstone" .
<http://inspire.ec.europa.eu/codelist/LithologyValue/paragneiss> schema:name "paragneiss" .
<http://inspire.ec.europa.eu/codelist/LithologyValue/peat> schema:name "peat" .
<http://inspire.ec.europa.eu/codelist/LithologyValue/pegmatite> schema:name "pegmatite" .
<http://inspire.ec.europa.eu/codelist/LithologyValue/peridotite> schema:name "peridotite" .
<http://inspire.ec.europa.eu/codelist/LithologyValue/phosphorite> schema:name "phosphorite" .
<http://inspire.ec.europa.eu/codelist/LithologyValue/phyllite> schema:name "phyllite" .
<http://inspire.ec.europa.eu/codelist/LithologyValue/phyllonite> schema:name "phyllonite" .
<http://inspire.ec.europa.eu/codelist/LithologyValue/quartzAlkaliFeldsparSyenite> schema:name "quartz alkali feldspar syenite" .
<http://inspire.ec.europa.eu/codelist/LithologyValue/quartzAnorthosite> schema:name "quartz anorthosite" .
<http://inspire.ec.europa.eu/codelist/LithologyValue/quartzDiorite> schema:name "quartz diorite" .
<http://inspire.ec.europa.eu/codelist/LithologyValue/quartzGabbro> schema:name "quartz gabbro" .
<http://inspire.ec.europa.eu/codelist/LithologyValue/quartzLatite> schema:name "quartz latite" .
<http://inspire.ec.europa.eu/codelist/LithologyValue/quartzMonzodiorite> schema:name "quartz monzodiorite" .
<http://inspire.ec.europa.eu/codelist/LithologyValue/quartzMonzogabbro> schema:name "quartz monzogabbro" .
<http://inspire.ec.europa.eu/codelist/LithologyValue/quartzMonzonite> schema:name "quartz monzonite" .
<http://inspire.ec.europa.eu/codelist/LithologyValue/quartzSyenite> schema:name "quartz syenite" .
<http://inspire.ec.europa.eu/codelist/LithologyValue/quartzTrachyte> schema:name "quartz trachyte" .
<http://inspire.ec.europa.eu/codelist/LithologyValue/quartzite> schema:name "quartzite" .
<http://inspire.ec.europa.eu/codelist/LithologyValue/rhyolite> schema:name "rhyolite" .
<http://inspire.ec.europa.eu/codelist/LithologyValue/rockGypsumOrAnhydrite> schema:name "rock gypsum or anhydrite" .
<http://inspire.ec.europa.eu/codelist/LithologyValue/sand> schema:name "sand" .
<http://inspire.ec.europa.eu/codelist/LithologyValue/sandSizeSediment> schema:name "sand-size sediment" .
<http://inspire.ec.europa.eu/codelist/LithologyValue/schist> schema:name "schist" .
<http://inspire.ec.europa.eu/codelist/LithologyValue/sedimentaryRock> schema:name "sedimentary rock" .
<http://inspire.ec.europa.eu/codelist/LithologyValue/shale> schema:name "shale" .
<http://inspire.ec.europa.eu/codelist/LithologyValue/silicateMudstone> schema:name "silicate mudstone" .
<http://inspire.ec.europa.eu/codelist/LithologyValue/syenite> schema:name "syenite" .
<http://inspire.ec.europa.eu/codelist/LithologyValue/syenogranite> schema:name "syenogranite" .
<http://inspire.ec.europa.eu/codelist/LithologyValue/tonalite> schema:name "tonalite" .
<http://inspire.ec.europa.eu/codelist/LithologyValue/trachyte> schema:name "trachyte" .
<http://inspire.ec.europa.eu/codelist/LithologyValue/travertine> schema:name "travertine" .
<http://inspire.ec.europa.eu/codelist/LithologyValue/ultramaficIgneousRock> schema:name "ultramafic igneous rock" .
<http://inspire.ec.europa.eu/codelist/LithologyValue/wacke> schema:name "wacke" .



<http://resource.geosciml.org/classifier/cgi/lithology/alkali_feldspar_granite>
    schema:description "Granitic rock that has a plagioclase to total feldspar ratio less than 0.1. QAPF field 2."@en ;
    schema:name "alkali feldspar granite"@en ;
.

<http://resource.geosciml.org/classifier/cgi/lithology/alkali_feldspar_syenite>
    schema:description "Alkali feldspar syenitic rock that contains 0-5 percent quartz and no feldspathoid in the QAPF fraction. QAPF field 6."@en ;
    schema:name "alkali feldspar syenite"@en ;
.

<http://resource.geosciml.org/classifier/cgi/lithology/amphibolite>
    schema:description "Metamorphic rock mainly consisting of green, brown or black amphibole and plagioclase (including albite), which combined form 75 percent or more of the rock, and both of which are present as major constituents. The amphibole constitutes 50 percent or more of the total mafic constituents and is present in an amount of 30 percent or more; other common minerals include quartz, clinopyroxene, garnet, epidote-group minerals, biotite, titanite and scapolite."@en ;
    schema:name "amphibolite"@en ;
.

<http://resource.geosciml.org/classifier/cgi/lithology/andesite>
    schema:description "Fine-grained igneous rock with less than 20 percent quartz and less than 10 percent feldspathoid minerals in the QAPF fraction, in which the ratio of plagioclase to total feldspar is greater 0.65. Includes rocks defined modally in QAPF fields 9 and 10 or chemically in TAS field O2 as andesite. Basalt and andesite, which share the same QAPF fields, are distinguished chemically based on silica content, with basalt defined to contain less than 52 weight percent silica. If chemical data are not available, the color index is used to distinguish the categories, with basalt defined to contain greater than 35 percent mafic minerals by volume or greater than 40 percent mafic minerals by weight. Typically consists of plagioclase (frequently zoned from labradorite to oligoclase), pyroxene, hornblende and/or biotite. Fine grained equivalent of dioritic rock."@en ;
    schema:name "andesite"@en ;
.

<http://resource.geosciml.org/classifier/cgi/lithology/anorthosite>
    schema:description "Anorthositic rock that contains between 0 and 5 percent quartz and no feldspathoid mineral in the QAPF fraction. QAPF field 10."@en ;
    schema:name "anorthosite"@en ;
.

<http://resource.geosciml.org/classifier/cgi/lithology/anthracite_coal>
    schema:description "Coal that has vitrinite mean random reflectance greater than 2.0% (determined in conformance with ISO 7404-5). Less than 12-14 percent volatiles (dry, ash free), greater than 91 percent fixed carbon (dry, ash free basis). The highest rank coal; very hard, glossy, black, with semimetallic luster, semi conchoidal fracture."@en ;
    schema:name "anthracite"@en ;
.

<http://resource.geosciml.org/classifier/cgi/lithology/arenite>
    schema:description "Clastic sandstone that contains less than 10 percent matrix. Matrix is mud-size silicate minerals (clay, feldspar, quartz, rock fragments, and alteration products) of detrital or diagenetic nature."@en ;
    schema:name "arenite"@en ;
.

<http://resource.geosciml.org/classifier/cgi/lithology/basalt>
    schema:description "Fine-grained or porphyritic igneous rock with less than 20 percent quartz, and less than 10 percent feldspathoid minerals, in which the ratio of plagioclase to total feldspar is greater 0.65. Typically composed of calcic plagioclase and clinopyroxene; phenocrysts typically include one or more of calcic plagioclase, clinopyroxene, orthopyroxene, and olivine. Includes rocks defined modally in QAPF fields 9 and 10 or chemically in TAS field B as basalt. Basalt and andesite are distinguished chemically based on silica content, with basalt defined to contain less than 52 weight percent silica. If chemical data are not available, the color index is used to distinguish the categories, with basalt defined to contain greater than 35 percent mafic minerals by volume or greater than 40 percent mafic minerals by weight."@en ;
    schema:name "basalt"@en ;
.

<http://resource.geosciml.org/classifier/cgi/lithology/bituminous_coal>
    schema:description "Coal that has vitrinite mean random reflectance greater than 0.6% and less than 2.0% (determined in conformance with ISO 7404-5), or has a gross calorific value greater than 24 MJ/kg (determined in conformance with ISO 1928). Hard, black, organic rich sedimentary rock; contains less than 91 percent fixed carbon on a dry, mineral-matter-free basis, and greater than 13-14 percent volatiles (dry, ash free). Formed from the compaction or induration of variously altered plant remains similar to those of peaty deposits."@en ;
    schema:name "bituminous coal"@en ;
.

<http://resource.geosciml.org/classifier/cgi/lithology/boundstone>
    schema:description "Sedimentary carbonate rock with preserved biogenic texture, whose original components were bound and encrusted together during deposition by the action of plants and animals during deposition, and remained substantially in the position of growth."@en ;
    schema:name "boundstone"@en ;
.

<http://resource.geosciml.org/classifier/cgi/lithology/carbonate_mudstone>
    schema:description "Mudstone that consists of greater than 50 percent carbonate minerals of any origin in the mud size fraction."@en ;
    schema:name "carbonate mudstone"@en ;
.

<http://resource.geosciml.org/classifier/cgi/lithology/carbonate_rich_mudstone>
    schema:description "Mudstone that contains between 10 and 50 percent carbonate minerals in the mud size fraction. Carbonate origin is not specified."@en ;
    schema:name "carbonate rich mudstone"@en ;
.

<http://resource.geosciml.org/classifier/cgi/lithology/carbonate_sedimentary_rock>
    schema:description "Sedimentary rock in which at least 50 percent of the primary and/or recrystallized constituents are composed of one (or more) of the carbonate minerals calcite, aragonite, magnesite or dolomite."@en ;
    schema:name "carbonate sedimentary rock"@en ;
.

<http://resource.geosciml.org/classifier/cgi/lithology/carbonate_wackestone>
    schema:description "Carbonate sedimentary rock with discernible mud supported depositional texture and containing greater than 10 percent allochems, and constituent particles are of intrabasinal origin. If particles are not intrabasinal, categorization as a mudstone or wackestone should be considered."@en ;
    schema:name "carbonate wackestone"@en ;
.

<http://resource.geosciml.org/classifier/cgi/lithology/carbonatite>
    schema:description "Igneous rock composed of more than 50 percent modal carbonate minerals."@en ;
    schema:name "carbonatite"@en ;
.

<http://resource.geosciml.org/classifier/cgi/lithology/chalk>
    schema:description "A generally soft, white, very fine-grained, extremely pure, porous limestone. It forms under marine conditions from the gradual accumulation of skeletal elements from minute planktonic green algae (cocoliths), associated with varying proportions of larger microscopic fragments of bivalves, foraminifera and ostracods. It is common to find flint and chert nodules embedded in chalk."@en ;
    schema:name "chalk"@en ;
.

<http://resource.geosciml.org/classifier/cgi/lithology/clastic_conglomerate>
    schema:description "Clastic sedimentary rock composed of at least 30 percent rounded to subangular fragments larger than 2 mm in diameter; typically contains finer grained material in interstices between larger fragments. If more than 15 percent of the fine grained matrix is of indeterminant clastic or diagenetic origin and the fabric is matrix supported, may also be categorized as wackestone. If rock has unsorted or poorly sorted texture with a wide range of particle sizes, may also be categorized as diamictite."@en ;
    schema:name "conglomerate"@en ;
.

<http://resource.geosciml.org/classifier/cgi/lithology/clastic_mudstone>
    schema:description "Clastic sedimentary rock consisting of less than 30 percent gravel-size (2 mm) particles and with a mud to sand ratio greater than 1."@en ;
    schema:name "mudstone"@en ;
.

<http://resource.geosciml.org/classifier/cgi/lithology/clastic_sandstone>
    schema:description "Clastic sedimentary rock in which less than 30 percent of particles are greater than 2 mm in diameter (gravel) and the sand to mud ratio is at least 1."@en ;
    schema:name "sandstone"@en ;
.

<http://resource.geosciml.org/classifier/cgi/lithology/clastic_sedimentary_rock>
    schema:description "Sedimentary rock in which at least 50 percent of the constituent particles were derived from erosion, weathering, or mass-wasting of pre-existing earth materials, and transported to the place of deposition by mechanical agents such as water, wind, ice and gravity."@en ;
    schema:name "clastic sedimentary rock"@en ;
.

<http://resource.geosciml.org/classifier/cgi/lithology/claystone>
    schema:description "Mudstone that contains no detectable silt, inferred to consist virtually entirely of clay-size particles."@en ;
    schema:name "claystone"@en ;
.

<http://resource.geosciml.org/classifier/cgi/lithology/coal>
    schema:description "A consolidated organic sedimentary material having less than 75% moisture. This category includes low, medium, and high rank coals according to International Classification of In-Seam Coal (United Nations, 1998), thus including lignite. Sapropelic coal is not distinguished in this category from humic coals. Formed from the compaction or induration of variously altered plant remains similar to those of peaty deposits."@en ;
    schema:name "coal"@en ;
.

<http://resource.geosciml.org/classifier/cgi/lithology/dacite>
    schema:description "Fine grained or porphyritic crystalline rock that contains less than 90 percent mafic minerals, between 20 and 60 percent quartz in the QAPF fraction, and has a plagioclase to total feldspar ratio greater than 0.65. Includes rocks defined modally in QAPF fields 4 and 5 or chemically in TAS Field O3. Typcially composed of quartz and sodic plagioclase with minor amounts of biotite and/or hornblende and/or pyroxene; fine-grained equivalent of granodiorite and tonalite."@en ;
    schema:name "dacite"@en ;
.

<http://resource.geosciml.org/classifier/cgi/lithology/diamictite>
    schema:description "Unsorted or poorly sorted, clastic sedimentary rock with a wide range of particle sizes including a muddy matrix. Biogenic materials that have such texture are excluded. Distinguished from conglomerate, sandstone, mudstone based on polymodality and lack of structures related to transport and deposition of sediment by moving air or water. If more than 10 percent of the fine grained matrix is of indeterminant clastic or diagenetic origin and the fabric is matrix supported, may also be categorized as wacke."@en ;
    schema:name "diamictite"@en ;
.

<http://resource.geosciml.org/classifier/cgi/lithology/diorite>
    schema:description "Phaneritic crystalline rock consisting of intermediate plagioclase, commonly with hornblende and often with biotite or augite; colour index M less than 90, sodic plagioclase (An0-An50), no feldspathoid, and between 0 and 5 percent quartz. Includes rocks defined modally in QAPF field 10 as diorite."@en ;
    schema:name "diorite"@en ;
.

<http://resource.geosciml.org/classifier/cgi/lithology/dolostone>
    schema:description "Pure carbonate sedimentary rock with a ratio of magnesium carbonate to calcite (plus aragonite) greater than 1 to 1."@en ;
    schema:name "dolomite"@en ;
.

<http://resource.geosciml.org/classifier/cgi/lithology/eclogite>
    schema:description "Metamorphic rock composed of 75 percent or more (by volume) omphacite and garnet, both of which are present as major constituents, the amount of neither of them being higher than 75 percent (by volume); the presence of plagioclase precludes classification as an eclogite."@en ;
    schema:name "eclogite"@en ;
.

<http://resource.geosciml.org/classifier/cgi/lithology/evaporite>
    schema:description "Nonclastic sedimentary rock composed of at least 50 percent non-carbonate salts, including chloride, sulfate or borate minerals; formed through precipitation of mineral salts from a saline solution (non-carbonate salt rock)."@en ;
    schema:name "evaporite"@en ;
.

<http://resource.geosciml.org/classifier/cgi/lithology/foid_diorite>
    schema:description "Foid dioritoid in which the plagioclase to total feldspar ratio is greater than 0.9. Includes rocks defined modally in QAPF field 14."@en ;
    schema:name "foid diorite"@en ;
.

<http://resource.geosciml.org/classifier/cgi/lithology/foid_gabbro>
    schema:description "Foid gabbroid that has a plagioclase to total feldspar ratio greater than 0.9. Includes rocks defined modally in QAPF field 14."@en ;
    schema:name "foid gabbro"@en ;
.

<http://resource.geosciml.org/classifier/cgi/lithology/foid_monzodiorite>
    schema:description "Foid dioritoid in which the plagioclase to total feldspar ratio is between 0.1 and 0.9. Includes rocks defined modally in QAPF field 13."@en ;
    schema:name "foid monzodiorite"@en ;
.

<http://resource.geosciml.org/classifier/cgi/lithology/foid_monzogabbro>
    schema:description "Foid gabbroid that has a plagioclase to total feldspar ratio between 0.5 and 0.9. Includes rocks defined modally in QAPF field 13."@en ;
    schema:name "foid monzogabbro"@en ;
.

<http://resource.geosciml.org/classifier/cgi/lithology/foid_monzosyenite>
    schema:description "Foid syenitoid rock that has a plagioclase to total feldspar ratio of between 0.1 and 0.5. Includes rocks defined modally in QAPF Field 12."@en ;
    schema:name "foid monzosyenite"@en ;
.

<http://resource.geosciml.org/classifier/cgi/lithology/foid_syenite>
    schema:description "Foid syenitoid that has a plagioclase to total feldspar ratio of less than 0.1. Includes rocks defined modally in QAPF field 11."@en ;
    schema:name "foid syenite"@en ;
.

<http://resource.geosciml.org/classifier/cgi/lithology/framestone>
    schema:description "Carbonate reef rock consisting of a rigid framework of colonies, shells or skeletons, with internal cavities filled with fine sediment; usually created through the activities of colonial organisms."@en ;
    schema:name "framestone"@en ;
.

<http://resource.geosciml.org/classifier/cgi/lithology/gabbro>
    schema:description "Gabbroic rock that contains between 0 and 5 percent quartz and no feldspathoid mineral in the QAPF fraction. Includes rocks defined modally in QAPF Field 10 as gabbro."@en ;
    schema:name "gabbro"@en ;
.

<http://resource.geosciml.org/classifier/cgi/lithology/gneiss>
    schema:description "Foliated metamorphic rock with bands or lenticles rich in granular minerals alternating with bands or lenticles rich in minerals with a flaky or elongate prismatic habit. Mylonitic foliation or well developed, continuous schistosity (greater than 50 percent of the rock consists of grains participate in a planar or linear fabric) precludes classification with this concept."@en ;
    schema:name "gneiss"@en ;
.

<http://resource.geosciml.org/classifier/cgi/lithology/grainstone>
    schema:description "Carbonate sedimentary rock with recognizable depositional fabric that is grain-supported, and constituent particles are of intrabasinal origin; contains little or no mud matrix. Distinction from sandstone is based on interpretation of intrabasinal origin of clasts and grain-supported fabric, but grainstone definition does not include a grain size criteria."@en ;
    schema:name "grainstone"@en ;
.

<http://resource.geosciml.org/classifier/cgi/lithology/granodiorite>
    schema:description "Phaneritic crystalline rock consisting essentially of quartz, sodic plagioclase and lesser amounts of alkali feldspar with minor hornblende and biotite. Includes rocks defined modally in QAPF field 4."@en ;
    schema:name "granodiorite"@en ;
.

<http://resource.geosciml.org/classifier/cgi/lithology/granofels>
    schema:description "Metamorphic rock with granoblastic fabric and very little or no foliation (less than 10 percent of the mineral grains in the rock are elements in a planar or linear fabric). Grainsize not specified."@en ;
    schema:name "granofels"@en ;
.

<http://resource.geosciml.org/classifier/cgi/lithology/granulite>
    schema:description "Metamorphic rock of high metamorphic grade in which Fe-Mg silicate minerals are dominantly hydroxl-free; feldspar must be present, and muscovite is absent; rock contains less than 90 percent mafic minerals, less than 75 percent calcite and/or dolomite, less than 75 percent quartz, less than 50 percent iron-bearing minerals (hematite, magnetite, limonite-group, siderite, iron-sulfides), and less than 50 percent calc-silicate minerals."@en ;
    schema:name "granulite"@en ;
.

<http://resource.geosciml.org/classifier/cgi/lithology/hornblendite>
    schema:description "Ultramafic rock that consists of greater than 40 percent hornblende plus pyroxene and has a hornblende to pyroxene ratio greater than 1. Includes olivine hornblendite, olivine-pyroxene hornblendite, pyroxene hornblendite, and hornblendite."@en ;
    schema:name "hornblendite"@en ;
.

<http://resource.geosciml.org/classifier/cgi/lithology/hornfels>
    schema:description "Granofels formed by contact metamorphism, composed of a mosaic of equidimensional grains in a characteristically granoblastic or decussate matrix; porphyroblasts or relict phenocrysts may be present. Typically fine grained."@en ;
    schema:name "hornfels"@en ;
.

<http://resource.geosciml.org/classifier/cgi/lithology/igneous_rock>
    schema:description "rock formed as a result of igneous processes, for example intrusion and cooling of magma in the crust, or volcanic eruption."@en ;
    schema:name "igneous rock"@en ;
.

<http://resource.geosciml.org/classifier/cgi/lithology/latite>
    schema:description "Latitic rock that contains between 0 and 5 percent quartz and no feldspathoid in the QAPF fraction. QAPF field 8."@en ;
    schema:name "latite"@en ;
.

<http://resource.geosciml.org/classifier/cgi/lithology/lignite>
    schema:description "Coal that has a gross calorific value less than 24 MJ/kg (determined in conformance with ISO 1928), and vitrinite mean random reflectance less than 0.6% (determined in conformance with ISO 7404-5). Gross calorific value is recalculated to a moist, ash free basis using bed moisture (determined according to ISO 1015 or ISO 5068). Includes all low-rank coals, including sub-bitiminous coal. A consolidated, dull, soft brown to black coal having many readily discernible plant fragments set in a finer grained organic matrix. Tends to crack and fall apart on drying. Operationally sub-bituminous and bitiminous coal are qualitatively distinguished based on brown streak for sub-bitiminous coal and black streak for bituminous coal."@en ;
    schema:name "lignite"@en ;
.

<http://resource.geosciml.org/classifier/cgi/lithology/limestone>
    schema:description "Pure carbonate sedimentary rock with a calcite (plus aragonite) to dolomite ratio greater than 1 to 1. Includes limestone and dolomitic limestone."@en ;
    schema:name "limestone"@en ;
.

<http://resource.geosciml.org/classifier/cgi/lithology/marble>
    schema:description "Metamorphic rock consisting of greater than 75 percent fine- to coarse-grained recrystallized calcite and/or dolomite; usually with a granoblastic, saccharoidal texture."@en ;
    schema:name "marble"@en ;
.

<http://resource.geosciml.org/classifier/cgi/lithology/metamorphic_rock>
    schema:description "Rock formed by solid-state mineralogical, chemical and/or structural changes to a pre-existing rock, in response to marked changes in temperature, pressure, shearing stress and chemical environment."@en ;
    schema:name "metamorphic rock"@en ;
.

<http://resource.geosciml.org/classifier/cgi/lithology/metasomatic_rock>
    schema:description "Rock that has fabric and composition indicating open-system mineralogical and chemical changes in response to interaction with a fluid phase, typically water rich."@en ;
    schema:name "metasomatic rock"@en ;
.

<http://resource.geosciml.org/classifier/cgi/lithology/monzodiorite>
    schema:description "Phaneritic crystalline igneous rock consisting of sodic plagioclase (An0 to An50), alkali feldspar, hornblende and biotite, with or without pyroxene, and 0 to 5 percent quartz. Includes rocks defined modally in QAPF field 9."@en ;
    schema:name "monzodiorite"@en ;
.

<http://resource.geosciml.org/classifier/cgi/lithology/monzogabbro>
    schema:description "Monzogabbroic rock that contains between 0 an 5 percent quartz and no feldspathoid mineral in the QAPF fraction. Includes rocks defined modally in QAPF field 9 ."@en ;
    schema:name "monzogabbro"@en ;
.

<http://resource.geosciml.org/classifier/cgi/lithology/monzogranite>
    schema:description "Granite that has a plagiolcase to total feldspar ratio between 0.35 and 0.65. QAPF field 3b."@en ;
    schema:name "monzogranite"@en ;
.

<http://resource.geosciml.org/classifier/cgi/lithology/monzonite>
    schema:description "Monzonitic rock that contains 0-5 percent quartz and no feldspathoid mineral in the QAPF fraction. Includes rocks defined modally in QAPF Field 8."@en ;
    schema:name "monzonite"@en ;
.

<http://resource.geosciml.org/classifier/cgi/lithology/packstone>
    schema:description "Carbonate sedimentary rock with discernible grain supported depositional texture, containing greater than 10 percent grains, and constituent particles are of intrabasinal origin; intergranular spaces are filled by matrix."@en ;
    schema:name "packstone"@en ;
.

<http://resource.geosciml.org/classifier/cgi/lithology/paragneiss>
    schema:description "A gneiss with mineralogy and texture indicating derivation from a sedimentary rock protolith. Typically consists of abundant quartz, mica, or calcsilicate minerals; aluminosilicate minerals or garnet commonly present. composition of rock tends to be more variable on a decimetric scale that in orthogneiss."@en ;
    schema:name "paragneiss"@en ;
.

<http://resource.geosciml.org/classifier/cgi/lithology/peat>
    schema:description "Unconsolidated organic-rich sediment composed of at least 50 percent semi-carbonised plant remains; individual remains commonly seen with unaided eye; yellowish brown to brownish black; generally fibrous texture; can be plastic or friable. In its natural state it can be readily cut and has a very high moisture content, generally greater than 90 percent. Liptinite to Inertinite ratio is less than one (Economic commission for Europe, committee on Sustainable Energy- United Nations (ECE-UN), 1998, International Classification of in-Seam Coals: Energy 19, 41 pp.)"@en ;
    schema:name "peat"@en ;
.

<http://resource.geosciml.org/classifier/cgi/lithology/pegmatite>
    schema:description "Exceptionally coarse grained crystalline rock with interlocking crystals; most grains are 1cm or more diameter; composition is generally that of granite, but the term may refer to the coarse grained facies of any type of igneous rock;usually found as irregular dikes, lenses, or veins associated with plutons or batholiths."@en ;
    schema:name "pegmatite"@en ;
.

<http://resource.geosciml.org/classifier/cgi/lithology/peridotite>
    schema:description "Ultramafic rock consisting of more than 40 percent (by volume) olivine with pyroxene and/or amphibole and little or no feldspar. commonly altered to serpentinite. Includes rocks defined modally in the ultramafic rock classification as dunite, harzburgite, lherzolite, wehrlite, olivinite, pyroxene peridotite, pyroxene hornblende peridotite or hornblende peridotite."@en ;
    schema:name "peridotite"@en ;
.

<http://resource.geosciml.org/classifier/cgi/lithology/phosphorite>
    schema:description "Sedimentary rock in which at least 50 percent of the primary or recrystallized constituents are phosphate minerals. Most commonly occurs as a bedded primary or reworked secondary marine rock, composed of microcrystalline carbonate fluorapatite in the form of lamina, pellets, oolites and nodules, and skeletal, shell and bone fragments."@en ;
    schema:name "phosphorite"@en ;
.

<http://resource.geosciml.org/classifier/cgi/lithology/phyllite>
    schema:description "Rock with a well developed, continuous schistosity, an average grain size between 0.1 and 0.5 millimeters, and a silvery sheen on cleavage surfaces. Individual phyllosilicate grains are barely visible with the unaided eye."@en ;
    schema:name "phyllite"@en ;
.

<http://resource.geosciml.org/classifier/cgi/lithology/phyllonite>
    schema:description "Mylonitic rock composed largely of fine-grained mica that imparts a sheen to foliation surfaces; may have flaser lamination, isoclinal folding, and deformed veins, which indicate significant shearing. Macroscopically resembles phyllite, but formed by mechanical degradation of initially coarser rock."@en ;
    schema:name "phyllonite"@en ;
.

<http://resource.geosciml.org/classifier/cgi/lithology/quartz_alkali_feldspar_syenite>
    schema:description "Alkali feldspar syenitic rock that contains 5 to 20 percent quartz and no feldspathoid in the QAPF fraction. QAPF field 6*."@en ;
    schema:name "quartz alkali feldspar syenite"@en ;
.

<http://resource.geosciml.org/classifier/cgi/lithology/quartz_anorthosite>
    schema:description "Anorthositic rock that contains between 5 and 20 percent quartz in the QAPF fraction. QAPF field 10*."@en ;
    schema:name "quartz anorthosite"@en ;
.

<http://resource.geosciml.org/classifier/cgi/lithology/quartz_diorite>
    schema:description "Dioritic rock that contains between 5 to 20 percent quartz in the QAPF fraction. QAPF field 10*."@en ;
    schema:name "quartz diorite"@en ;
.

<http://resource.geosciml.org/classifier/cgi/lithology/quartz_gabbro>
    schema:description "Gabbroic rock that contains between 5 and 20 percent quartz in the QAPF fraction. QAPF field 10*."@en ;
    schema:name "quartz gabbro"@en ;
.

<http://resource.geosciml.org/classifier/cgi/lithology/quartz_latite>
    schema:description "Latitic rock that contains between 5 and 20 percent quartz in the QAPF fraction. QAPF field 8*."@en ;
    schema:name "quartz latite"@en ;
.

<http://resource.geosciml.org/classifier/cgi/lithology/quartz_monzodiorite>
    schema:description "Monzodioritic rock that contains between 5 and 20 percent quartz."@en ;
    schema:name "quartz monzodiorite"@en ;
.

<http://resource.geosciml.org/classifier/cgi/lithology/quartz_monzogabbro>
    schema:description "Monzogabbroic rock that contains between 5 and 20 percent quartz in the QAPF fraction. QAPF field 9*."@en ;
    schema:name "quartz monzogabbro"@en ;
.

<http://resource.geosciml.org/classifier/cgi/lithology/quartz_monzonite>
    schema:description "Monzonitic rock that contains 5-20 percent quartz iin the QAPF fraction. Includes rocks defined modally in QAPF Field 8*."@en ;
    schema:name "quartz monzonite"@en ;
.

<http://resource.geosciml.org/classifier/cgi/lithology/quartz_syenite>
    schema:description "Syenitic rock that contains between 5 and 20 percent quartz in the QAPF fraction. Defined modally in QAPF Field 7*."@en ;
    schema:name "quartz syenite"@en ;
.

<http://resource.geosciml.org/classifier/cgi/lithology/quartz_trachyte>
    schema:description "Trachytic rock that contains between 5 and 20 percent quartz in the QAPF fraction. QAPF field 7*."@en ;
    schema:name "quartz trachyte"@en ;
.

<http://resource.geosciml.org/classifier/cgi/lithology/quartzite>
    schema:description "Metamorphic rock consisting of greater than or equal to 75 percent quartz; typically granoblastic texture."@en ;
    schema:name "quartzite"@en ;
.

<http://resource.geosciml.org/classifier/cgi/lithology/rhyolite>
    schema:description "rhyolitoid in which the ratio of plagioclase to total feldspar is between 0.1 and 0.65."@en ;
    schema:name "rhyolite"@en ;
.

<http://resource.geosciml.org/classifier/cgi/lithology/rock_gypsum_or_anhydrite>
    schema:description "Evaporite composed of at least 50 percent gypsum or anhydrite."@en ;
    schema:name "gypsum or anhydrite"@en ;
.

<http://resource.geosciml.org/classifier/cgi/lithology/sand>
    schema:description "Clastic sediment in which less than 30 percent of particles are gravel (greater than 2 mm in diameter) and the sand to mud ratio is at least 1. More than half of the particles are of epiclastic origin."@en ;
    schema:name "sand"@en ;
.

<http://resource.geosciml.org/classifier/cgi/lithology/sand_size_sediment>
    schema:description "Sediment in which less than 30 percent of particles are gravel (greater than 2 mm in diameter) and the sand to mud ratio is at least 1. composition or genesis of clasts not specified."@en ;
    schema:name "sand size sediment"@en ;
.

<http://resource.geosciml.org/classifier/cgi/lithology/schist>
    schema:description "Foliated phaneritic metamorphic rock with well developed, continuous schistosity, meaning that greater than 50 percent of the rock by volume is mineral grains with a thin tabular, lamellar, or acicular prismatic crystallographic habit that are oriented in a continuous planar or linear fabric."@en ;
    schema:name "schist"@en ;
.

<http://resource.geosciml.org/classifier/cgi/lithology/sedimentary_rock>
    schema:description "Rock formed by accumulation and cementation of solid fragmental material deposited by air, water or ice, or as a result of other natural agents, such as precipitation from solution, the accumulation of organic material, or from biogenic processes, including secretion by organisms. Includes epiclastic deposits."@en ;
    schema:name "sedimentary rock"@en ;
.

<http://resource.geosciml.org/classifier/cgi/lithology/shale>
    schema:description "Laminated mudstone that will part or break along thin, closely spaced layers parallel to stratification."@en ;
    schema:name "shale"@en ;
.

<http://resource.geosciml.org/classifier/cgi/lithology/silicate_mudstone>
    schema:description "Mudstone that contains less than 10 percent carbonate minerals."@en ;
    schema:name "silicate mudstone"@en ;
.

<http://resource.geosciml.org/classifier/cgi/lithology/syenite>
    schema:description "Syenitic rock that contains between 0 and 5 percent quartz and no feldspathoid mineral in the QAPF fraction. Defined modally in QAPF Field 7."@en ;
    schema:name "syenite"@en ;
.

<http://resource.geosciml.org/classifier/cgi/lithology/syenogranite>
    schema:description "Granite that has a plagiolcase to total feldspar ratio between 0.10 and 0.35. QAPF field 3a."@en ;
    schema:name "syenogranite"@en ;
.

<http://resource.geosciml.org/classifier/cgi/lithology/tonalite>
    schema:description "Granitoid consisting of quartz and intermediate plagioclase, usually with biotite and amphibole. Includes rocks defined modally in QAPF field 5; ratio of plagioclase to total feldspar is greater than 0.9."@en ;
    schema:name "tonalite"@en ;
.

<http://resource.geosciml.org/classifier/cgi/lithology/trachyte>
    schema:description "Trachytoid that has a plagioclase to total feldspar ratio between 0.1 and 0.35, between 0 and 5 percent quartz in the QAPF fraction, and no feldspathoid minerals. QAPF field 7."@en ;
    schema:name "trachyte"@en ;
.

<http://resource.geosciml.org/classifier/cgi/lithology/travertine>
    schema:description "Biotically or abiotically precipitated calcium carbonate, from spring-fed, heated, or ambient-temperature water. May be white and spongy, various shades of orange, tan or gray, and ranges to dense, banded or laminated rock. Macrophytes, bryophytes, algae, cyanobacteria and other organisms often colonize the surface of travertine and may be preserved, to produce the porous varieties."@en ;
    schema:name "travertine"@en ;
.

<http://resource.geosciml.org/classifier/cgi/lithology/ultramafic_igneous_rock>
    schema:description "Igneous rock that consists of greater than 90 percent mafic minerals."@en ;
    schema:name "ultramafic igneous rock"@en ;
.

<http://resource.geosciml.org/classifier/cgi/lithology/wacke>
    schema:description "Clastic sandstone with more than 10 percent matrix of indeterminate detrital or diagenetic nature. Matrix is mud size silicate minerals (clay, feldspar, quartz, rock fragments, and alteration products)."@en ;
    schema:name "wacke"@en ;
.

