PREFIX : <https://linked.data.gov.au/def/gswa-vocabulary-themes/>
PREFIX cs: <https://linked.data.gov.au/def/gswa-vocabulary-themes>
PREFIX dcat: <http://www.w3.org/ns/dcat#>
PREFIX isoroles: <https://linked.data.gov.au/def/data-roles/>
PREFIX owl: <http://www.w3.org/2002/07/owl#>
PREFIX prov: <http://www.w3.org/ns/prov#>
PREFIX reg: <http://purl.org/linked-data/registry#>
PREFIX schema: <https://schema.org/>
PREFIX skos: <http://www.w3.org/2004/02/skos/core#>
PREFIX xsd: <http://www.w3.org/2001/XMLSchema#>

:administration
    a skos:Concept ;
    skos:definition "Vocabularies related to the management of the duties and business of the organization (the Geological Survey of Western Australia), i.e. covering the work involved in planning, organizing, directing, controlling and coordinating resources and operations. It includes management of internal day-to-day operations as well as the external-facing fulfillment of functions and responsibilities."@en ;
    skos:inScheme cs: ;
    skos:prefLabel "administration"@en ;
    skos:topConceptOf cs: ;
    schema:citation
        "https://biz.libretexts.org/Bookshelves/Management/Organizational_Behavior_(OpenStax)/01%3A_Management_and_Organizational_Behavior/1.03%3A_The_Nature_of_Management"^^xsd:anyURI ,
        "https://dictionary.cambridge.org/dictionary/english/administration"^^xsd:anyURI ,
        "https://www.britannica.com/dictionary/administration"^^xsd:anyURI ,
        "https://www.geeksforgeeks.org/functions-of-management-planning-organising-staffing-directing-and-controlling/"^^xsd:anyURI ;
.

:data-acquisition
    a skos:Concept ;
    skos:definition "Vocabularies related to the systematic processes of gathering observations and measurements, and related analytical techniques and methodologies, including sample preparation techniques."@en ;
    skos:inScheme cs: ;
    skos:prefLabel "data acquisition"@en ;
    skos:topConceptOf cs: ;
.

:geology-framework
    a skos:Concept ;
    skos:broader :geology ;
    skos:definition "Vocabularies related to the fundamental components that in combination define the spatial and temporal geological architecture of a region, i.e. vocabularies related to the definition, classification and modelling of stratigraphic relationships/units, tectonic/physiographic units, geological events and mineral systems."@en ;
    skos:inScheme cs: ;
    skos:prefLabel "geology - framework"@en ;
.

:geology-geochemistry
    a skos:Concept ;
    skos:broader :geology ;
    skos:definition "Vocabularies related to the distribution and amounts of the chemical elements in minerals, ores, rocks, soils, water, and the atmosphere, and the study of the circulation of the elements in nature, on the basis of the properties of their atoms and ions; also, the study of the distribution and abundance of isotopes, including problems of nuclear frequency and stability in the universe. Adapted from Glossary of geology (Neuendorf et. al., 2011, 5th edition revised)."@en ;
    skos:inScheme cs: ;
    skos:prefLabel "geology - geochemistry"@en ;
    schema:citation "https://glossary.americangeosciences.org/term/geochemistry"^^xsd:anyURI ;
.

:geology-geochronology
    a skos:Concept ;
    skos:broader :geology ;
    skos:definition "Vocabularies related to the numerical and relative age determination of geological events, as well as determining the events' time sequence and duration in the history of the Earth. Adapted from Glossary of geology (Neuendorf et. al., 2011, 5th edition revised)."@en ;
    skos:inScheme cs: ;
    skos:prefLabel "geology - geochronology"@en ;
    schema:citation "https://glossary.americangeosciences.org/term/geochronology"^^xsd:anyURI ;
.

:geology-geophysics
    a skos:Concept ;
    skos:broader :geology ;
    skos:definition "Vocabularies related to the physical properties and processes of the Solid Earth and its surrounding space environment, and the use of quantitative methods for their analysis."@en ;
    skos:inScheme cs: ;
    skos:prefLabel "geology - geophysics"@en ;
    schema:citation "https://en.wikipedia.org/wiki/Geophysics"^^xsd:anyURI ;
.

:geology-paleontology
    a skos:Concept ;
    skos:broader :geology ;
    skos:definition "Vocabularies related to the study of life in past geological time, based on the distribution and form of body fossils and their traces. This includes interpreting their relationships to other organisms both through time and within their original habitat (phylogeny, evolution, paleoecology), their environments (paleoenvironmental reconstruction, paleobiogeography), and the chronology of the Earth's history (biostratigraphy)."@en ;
    skos:inScheme cs: ;
    skos:prefLabel "geology - paleontology"@en ;
.

:geology-mapping
    a skos:Concept ;
    skos:broader :geology ;
    skos:definition "Vocabularies related to the defining of geological elements of a region."@en ;
    skos:inScheme cs: ;
    skos:prefLabel "geology - mapping"@en ;
.

:geology–mapping
    a skos:Concept ;
    skos:broader :geology ;
    skos:definition "Vocabularies related to the compilation of geological maps, i.e. graphic representations of the distribution, composition and structure of geological materials across the Earth's surface and at depth, depicting both observations and interpretations using symbols and colours. Included here are vocabularies related to topography (the practice of accurately and graphically delineating in detail, as on a map or chart or by a model, selected natural and man-made surface features of a region) and geodesy (the science concerned with the determination of the size and shape of the Earth and the precise location of points on its surface and subsurface), which are fundamental for the correct spatial representation of geological information."@en ;
    skos:inScheme cs: ;
    skos:prefLabel "geology – mapping"@en ;
    schema:citation
        "https://geology-hub.com/geologic-mapping-guide-for-professionals-and-students/"^^xsd:anyURI ,
        "https://glossary.americangeosciences.org/term/geodesy"^^xsd:anyURI ,
        "https://glossary.americangeosciences.org/term/topography"^^xsd:anyURI ,
        "https://www.usgs.gov/programs/national-cooperative-geologic-mapping-program/introduction-geologic-mapping"^^xsd:anyURI ;
.

:legislation
    a skos:Concept ;
    skos:definition "Vocabularies related to laws and regulations governing, controlling or affecting the business of the organization, including those the organization is tasked to implement and administer."@en ;
    skos:inScheme cs: ;
    skos:prefLabel "legislation"@en ;
    skos:topConceptOf cs: ;
.

:resources–energy
    a skos:Concept ;
    skos:broader :resources ;
    skos:definition "Vocabularies related to the study, exploration for and exploitation of physical processes and natural concentrations of materials for the main purpose of power generation. Energy resources include (a) concentrations of solid and/or fluid, inorganic or fossilized organic materials naturally occurring on or in the Earth’s crust (e.g. non-renewable fossil fuels such as petroleum, and natural gases); (b) natural physical processes within the Earth’s crust, atmosphere and hydrosphere (i.e. renewable energy resources such as solar, wind, hydro, solar thermal, marine, geothermal) or human-controlled activities (e.g. bioenergy/biomass, energy storage); and (c) nuclear energy. Adapted from Glossary of geology (Neuendorf et. al., 2011, 5th edition revised)."@en ;
    skos:inScheme cs: ;
    skos:prefLabel "resources – energy"@en ;
    schema:citation
        "https://www.eia.gov/energyexplained/us-energy-facts/"^^xsd:anyURI ,
        "https://www.energyfactsaustralia.org.au/explainers/energy-sources/"^^xsd:anyURI ;
.

:resources-mineral
    a skos:Concept ;
    skos:broader :resources ;
    skos:definition "Vocabularies related to the study, exploration for and exploitation of concentrations of natural inorganic or fossilized organic material occurring on or within the Earth’s crust, in sufficient quantity and quality to have reasonable prospects for economic extraction. Mineral resources are non-renewable and include metals (e.g. iron, copper, and aluminium), non-metals (e.g. salt, gypsum, clay, sand, phosphates), and rocks (e.g. dimension stones, basic raw materials)."@en ;
    skos:inScheme cs: ;
    skos:prefLabel "resources – mineral"@en ;
    schema:citation "https://glossary.americangeosciences.org/term/resources"^^xsd:anyURI ;
.

:sample-acquisition-management
    a skos:Concept ;
    skos:definition "Vocabularies related to the collection/procurement, handling, tracking, storing, and retrieving of primary geoscience material (typically, but not exclusively, a rock, mineral, fossil or soil) collected in the field or from materials collected in the field (e.g. drillcore), as well as derived specimens from such materials for the purpose of analysis and research. Included are vocabularies related to collections as single entities."@en ;
    skos:inScheme cs: ;
    skos:prefLabel "sample acquisition and management"@en ;
    skos:topConceptOf cs: ;
.

<https://linked.data.gov.au/org/gswa>
    a schema:Organization ;
    schema:name "Gswa" ;
    schema:url ""^^xsd:anyURI ;
.

:resources
    a skos:Concept ;
    skos:definition "Vocabularies related to the study, exploration for and exploitation of concentrations of solid, liquid, or gaseous materials in or on the Earth's crust in such form and amount that economic extraction of a commodity from the concentration is currently or potentially feasible. Adapted from Glossary of geology (Neuendorf et. al., 2011, 5th edition revised)."@en ;
    skos:inScheme cs: ;
    skos:narrower
        :resources–energy ,
        :resources-mineral ;
    skos:prefLabel "resources"@en ;
    skos:topConceptOf cs: ;
    schema:citation "https://glossary.americangeosciences.org/term/resources"^^xsd:anyURI ;
.

:geology
    a skos:Concept ;
    skos:definition "Vocabularies related to the study of the Solid Earth and the materials of which it is made, the processes that act on these materials, the products formed, and the history of the planet and its life forms since its origin, including the study of physical forces that act on the Earth, the chemistry of its constituent materials, and the biology of its past inhabitants as revealed by fossils. Adapted from Glossary of geology (Neuendorf et. al., 2011, 5th edition revised)."@en ;
    skos:inScheme cs: ;
    skos:narrower
        :geology-framework ,
        :geology-geochemistry ,
        :geology-geochronology ,
        :geology-geophysics ,
        :geology-paleontology ,
        :geology–mapping ;
    skos:prefLabel "geology"@en ;
    skos:topConceptOf cs: ;
    schema:citation
        "https://en.wikipedia.org/wiki/Geology"^^xsd:anyURI ,
        "https://glossary.americangeosciences.org/term/geology"^^xsd:anyURI ;
.

:1.0 schema:name "1.0" .

cs:
    a skos:ConceptScheme ;
    reg:status <https://linked.data.gov.au/def/reg-statuses/stable> ;
    owl:versionIRI :1.0 ;
    skos:definition "The overarching categorization of vocabularies prepared by the Geological Survey of Western Australia (GSWA)."@en ;
    skos:hasTopConcept
        :administration ,
        :data-acquisition ,
        :geology ,
        :legislation ,
        :resources ,
        :sample-acquisition-management ;
    skos:historyNote "Created for the purpose of grouping related vocabularies and to allow easy sorting of published GSWA vocabularies."@en ;
    skos:prefLabel "GSWA vocabulary themes"@en ;
    prov:qualifiedAttribution
        [
            dcat:hadRole isoroles:custodian ;
            prov:agent
                [
                    a schema:Person ;
                    schema:email ""^^xsd:anyURI ;
                    schema:name "Dave Martin" ;
                ] ;
        ] ,
        [
            dcat:hadRole isoroles:custodian ;
            prov:agent
                [
                    a schema:Person ;
                    schema:email ""^^xsd:anyURI ;
                    schema:name "Angela Riganti" ;
                ] ;
        ] ;
    schema:creator <https://linked.data.gov.au/org/gswa> ;
    schema:dateCreated "2024-06-06"^^xsd:date ;
    schema:dateModified "2024-12-02"^^xsd:date ;
    schema:keywords "Administration" ;
    schema:publisher <https://linked.data.gov.au/org/gswa> ;
    schema:version "1.0" ;
.
