PREFIX : <http://resource.geosciml.org/classifier/ics/ischart/>
PREFIX cs: <https://w3id.org/profile/gts-skos>
PREFIX dcterms: <http://purl.org/dc/terms/>
PREFIX owl: <http://www.w3.org/2002/07/owl#>
PREFIX prov: <http://www.w3.org/ns/prov#>
PREFIX rdfs: <http://www.w3.org/2000/01/rdf-schema#>
PREFIX sdo: <https://schema.org/>
PREFIX skos: <http://www.w3.org/2004/02/skos/core#>
PREFIX ts: <http://resource.geosciml.org/vocabulary/timescale/>
PREFIX xsd: <http://www.w3.org/2001/XMLSchema#>

:CMYK
    a owl:Datatype ;
    dcterms:description """The CMYK colour model (also known as process colour, or four colour) is a subtractive colour model, based on the CMY colour model, used in colour printing, and is also used to describe the printing process itself. CMYK refers to the four ink plates used in some colour printing: cyan, magenta, yellow, and key (black).

This datatype uses a microformat of "{C}/{M}/{Y}/{K}" with integer values for {C}, {M} {Y} & {K}."""@en ;
    dcterms:source "https://en.wikipedia.org/wiki/CMYK_colour_model"^^xsd:anyURI ;
    dcterms:title "CMYK colour model" ;
.

:RGB
    a owl:Datatype ;
    dcterms:description """The RGB colour model is an additive colour model in which the red, green, and blue primary colours of light are added together in various ways to reproduce a broad array of colours. The name of the model comes from the initials of the three additive primary colours, red, green, and blue.

This datatype uses a microformat of "{R}/{G}/{B}" with integer values for {R}, {G} & {B} between 0 and 255."""@en ;
    dcterms:source "https://en.wikipedia.org/wiki/RGB_colour_model"^^xsd:anyURI ;
    dcterms:title "CMYK colour notation" ;
.

:RGBHex
    a owl:Datatype ;
    dcterms:description """An 8-bit per channel, hexidecimal representation of RGB colours.

This datatype uses a microformat of "#{R}{G}{B}" with hexidecimal value for {R}, {G} & {B} between 00 and FF."""@en ;
    dcterms:title "CMYK colour notation" ;
.

:Aalenian
    a skos:Concept ;
    rdfs:isDefinedBy ts:gts2020 ;
    skos:altLabel
        "пален"@bg ,
        "Aalen"@cs ,
        "Aalenien"@da ,
        "Aalénium"@de ,
        "Aaleniense"@es ,
        "Aaleni"@et ,
        "Aalen"@fi ,
        "Aalénien"@fr ,
        "aaleni"@hu ,
        "aaleniano"@it ,
        "アーレニアン期"@ja ,
        "Alenis"@lt ,
        "Aaleniën"@nl ,
        "Aalen"@no ,
        "Aalen"@pl ,
        "Aaleniano"@pt ,
        "álen"@sk ,
        "aalenij"@sl ,
        "aalen"@sv ,
        "阿连期"@zh ;
    skos:broader :MiddleJurassic ;
    skos:definition "A time period with the following approximated bounds: older bound -174.1 +|-1.0 Ma, younger bound -170.3 +|-1.4 Ma" ;
    skos:inScheme cs: ;
    skos:prefLabel "Aalenian"@en ;
    prov:wasDerivedFrom ts:gts2020 ;
    sdo:color
        "40/0/5/0"^^:CMYK ,
        "154/217/221"^^:RGB ,
        "#9AD9DD"^^:RGBHex ;
.

:Aeronian
    a skos:Concept ;
    rdfs:isDefinedBy ts:gts2020 ;
    skos:altLabel
        "перон"@bg ,
        "Aeron"@cs ,
        "Aeronien"@da ,
        "Aeronium"@de ,
        "Aeroniense"@es ,
        "Aeroni"@et ,
        "Aeron"@fi ,
        "Aéronien"@fr ,
        "aeroni"@hu ,
        "aeroniano"@it ,
        "アエロニアン期"@ja ,
        "Aeronis"@lt ,
        "Aeroniën"@nl ,
        "Aeronium"@no ,
        "Aeron"@pl ,
        "Aeroniano"@pt ,
        "aerón"@sk ,
        "aeronij"@sl ,
        "aeron"@sv ,
        "埃隆期"@zh ;
    skos:broader :Llandovery ;
    skos:definition "A time period with the following approximated bounds: older bound -440.8 +|-1.2 Ma, younger bound -438.5 +|-1.1 Ma" ;
    skos:inScheme cs: ;
    skos:prefLabel "Aeronian"@en ;
    prov:wasDerivedFrom ts:gts2020 ;
    sdo:color
        "30/0/20/0"^^:CMYK ,
        "179/225/194"^^:RGB ,
        "#B3E1C2"^^:RGBHex ;
.

:Albian
    a skos:Concept ;
    rdfs:isDefinedBy ts:gts2020 ;
    skos:altLabel
        "плб"@bg ,
        "Alb"@cs ,
        "Albien"@da ,
        "Albium"@de ,
        "Albiense"@es ,
        "Albi"@et ,
        "Alb"@fi ,
        "Albien"@fr ,
        "albai"@hu ,
        "albiano"@it ,
        "アルビアン期"@ja ,
        "Albis"@lt ,
        "Albiën"@nl ,
        "Alb"@no ,
        "Alb"@pl ,
        "Albiano"@pt ,
        "alb"@sk ,
        "albij"@sl ,
        "alban"@sv ,
        "阿尔布期"@zh ;
    skos:broader :LowerCretaceous ;
    skos:definition "A time period with the following approximated bounds: older bound -113.0 Ma, younger bound -100.5 Ma" ;
    skos:inScheme cs: ;
    skos:prefLabel "Albian"@en ;
    prov:wasDerivedFrom ts:gts2020 ;
    sdo:color
        "20/0/40/0"^^:CMYK ,
        "204/234/151"^^:RGB ,
        "#CCEA97"^^:RGBHex ;
.

:Anisian
    a skos:Concept ;
    rdfs:isDefinedBy ts:gts2020 ;
    skos:altLabel
        "пниз"@bg ,
        "Anis"@cs ,
        "Anisien"@da ,
        "Anisium"@de ,
        "Anisiense"@es ,
        "Anisi"@et ,
        "Anis"@fi ,
        "Anisien"@fr ,
        "anisusi"@hu ,
        "anisico"@it ,
        "アニシアン期"@ja ,
        "Anizis"@lt ,
        "Anisiën"@nl ,
        "Ansin"@no ,
        "Anizyk"@pl ,
        "Anisiano"@pt ,
        "anis"@sk ,
        "anizij"@sl ,
        "anis"@sv ,
        "安尼期"@zh ;
    skos:broader :MiddleTriassic ;
    skos:definition "A time period with the following approximated bounds: older bound -247.2 Ma, younger bound -242 Ma" ;
    skos:inScheme cs: ;
    skos:prefLabel "Anisian"@en ;
    prov:wasDerivedFrom ts:gts2020 ;
    sdo:color
        "25/50/0/0"^^:CMYK ,
        "188/117/183"^^:RGB ,
        "#BC75B7"^^:RGBHex ;
.

:Aptian
    a skos:Concept ;
    rdfs:isDefinedBy ts:gts2020 ;
    skos:altLabel
        "ппт"@bg ,
        "Apt"@cs ,
        "Aptien"@da ,
        "Aptium"@de ,
        "Aptiense"@es ,
        "Apti"@et ,
        "Apt"@fi ,
        "Aptien"@fr ,
        "apti"@hu ,
        "aptiano"@it ,
        "アプチアン期"@ja ,
        "Aptis"@lt ,
        "Aptiën"@nl ,
        "Apt"@no ,
        "Apt"@pl ,
        "Aptiano"@pt ,
        "apt"@sk ,
        "aptij"@sl ,
        "apt"@sv ,
        "阿普弟期"@zh ;
    skos:broader :LowerCretaceous ;
    skos:definition "A time period with the following approximated bounds: older bound -125.0 Ma, younger bound -113.0 Ma" ;
    skos:inScheme cs: ;
    skos:prefLabel "Aptian"@en ;
    prov:wasDerivedFrom ts:gts2020 ;
    sdo:color
        "25/0/45/0"^^:CMYK ,
        "191/228/138"^^:RGB ,
        "#BFE48A"^^:RGBHex ;
.

:Aquitanian
    a skos:Concept ;
    rdfs:isDefinedBy ts:gts2020 ;
    skos:altLabel
        "пквитан"@bg ,
        "Aquitan"@cs ,
        "Aquitanien"@da ,
        "Aquitanium"@de ,
        "Aquitaninse"@es ,
        "Aquitani"@et ,
        "Aquitan"@fi ,
        "Aquitanien"@fr ,
        "aquitaniai"@hu ,
        "aquitaniano"@it ,
        "アキタニアン期"@ja ,
        "Akvitanis"@lt ,
        "Aquitaniën-Vierland"@nl ,
        "Aquitanium"@no ,
        "Akwitan"@pl ,
        "Aquitaniano"@pt ,
        "akvitán"@sk ,
        "akvitanij"@sl ,
        "aquitan"@sv ,
        "阿启坦期"@zh ;
    skos:broader :Miocene ;
    skos:definition "A time period with the following approximated bounds: older bound -23.03 Ma, younger bound -20.44 Ma" ;
    skos:inScheme cs: ;
    skos:prefLabel "Aquitanian"@en ;
    prov:wasDerivedFrom ts:gts2020 ;
    sdo:color
        "0/0/80/0"^^:CMYK ,
        "255/255/51"^^:RGB ,
        "#FFFF33"^^:RGBHex ;
.

:Artinskian
    a skos:Concept ;
    rdfs:isDefinedBy ts:gts2020 ;
    skos:altLabel
        "пртин"@bg ,
        "Artinsk"@cs ,
        "Artinskien"@da ,
        "Artinskium"@de ,
        "Artinskiense"@es ,
        "Artinski"@et ,
        "Artinsk"@fi ,
        "Artinskien"@fr ,
        "artyinszki"@hu ,
        "artinskiano"@it ,
        "アルティンスキアン期"@ja ,
        "Artinskis"@lt ,
        "Artinskiën"@nl ,
        "Artiskium"@no ,
        "Artinsk"@pl ,
        "Artinskiano"@pt ,
        "artinsk"@sk ,
        "artinskij"@sl ,
        "artinsk"@sv ,
        "亚丁斯克期"@zh ;
    skos:broader :Cisuralian ;
    skos:definition "A time period with the following approximated bounds: older bound -290.1 +|-0.26 Ma, younger bound -283.5 +|-0.6 Ma" ;
    skos:inScheme cs: ;
    skos:prefLabel "Artinskian"@en ;
    prov:wasDerivedFrom ts:gts2020 ;
    sdo:color
        "10/50/45/0"^^:CMYK ,
        "227/123/104"^^:RGB ,
        "#E37B68"^^:RGBHex ;
.

:Asselian
    a skos:Concept ;
    rdfs:isDefinedBy ts:gts2020 ;
    skos:altLabel
        "пѿел"@bg ,
        "Assel"@cs ,
        "Asselien"@da ,
        "Asselium"@de ,
        "Asseliense"@es ,
        "Asseli"@et ,
        "Assel"@fi ,
        "Assélien"@fr ,
        "asszeli"@hu ,
        "asseliano"@it ,
        "アセリアン期"@ja ,
        "Aselis"@lt ,
        "Asseliën"@nl ,
        "Asselium"@no ,
        "Aselsk"@pl ,
        "Asseliano"@pt ,
        "assel"@sk ,
        "asselij"@sl ,
        "assel"@sv ,
        "阿瑟尔期"@zh ;
    skos:broader :Cisuralian ;
    skos:definition "A time period with the following approximated bounds: older bound -298.9 +|-0.15 Ma, younger bound -295.0 +|-0.18 Ma" ;
    skos:inScheme cs: ;
    skos:prefLabel "Asselian"@en ;
    prov:wasDerivedFrom ts:gts2020 ;
    sdo:color
        "10/60/55/0"^^:CMYK ,
        "227/99/80"^^:RGB ,
        "#E36350"^^:RGBHex ;
.

:Bajocian
    a skos:Concept ;
    rdfs:isDefinedBy ts:gts2020 ;
    skos:altLabel
        "Байоѿ"@bg ,
        "Bajok"@cs ,
        "Bajocien"@da ,
        "Bajocium"@de ,
        "Bajociense"@es ,
        "Bajoci"@et ,
        "Bajoc"@fi ,
        "Bajocien"@fr ,
        "bajoci"@hu ,
        "bajociano"@it ,
        "バジョシアン期"@ja ,
        "Bajosis"@lt ,
        "Bajociën"@nl ,
        "Bajoc"@no ,
        "Bajos"@pl ,
        "Bajociano"@pt ,
        "bajok"@sk ,
        "bajocij"@sl ,
        "bajoc"@sv ,
        "巴柔期"@zh ;
    skos:broader :MiddleJurassic ;
    skos:definition "A time period with the following approximated bounds: older bound -170.3 +|-1.4 Ma, younger bound -168.3 +|-1.3 Ma" ;
    skos:inScheme cs: ;
    skos:prefLabel "Bajocian"@en ;
    prov:wasDerivedFrom ts:gts2020 ;
    sdo:color
        "35/0/5/0"^^:CMYK ,
        "166/221/224"^^:RGB ,
        "#A6DDE0"^^:RGBHex ;
.

:Barremian
    a skos:Concept ;
    rdfs:isDefinedBy ts:gts2020 ;
    skos:altLabel
        "Барем"@bg ,
        "Barrem"@cs ,
        "Barremien"@da ,
        "Barrêmium"@de ,
        "Barremiense"@es ,
        "Barremi"@et ,
        "Barrem"@fi ,
        "Barrémien"@fr ,
        "barremi"@hu ,
        "berremiano"@it ,
        "バレミアン期"@ja ,
        "Baremis"@lt ,
        "Barremiën"@nl ,
        "Barremium"@no ,
        "Barrem"@pl ,
        "Barremiano"@pt ,
        "barém"@sk ,
        "barremij"@sl ,
        "barrem"@sv ,
        "巴列姆期"@zh ;
    skos:broader :LowerCretaceous ;
    skos:definition "A time period with the following approximated bounds: older bound -129.4 Ma, younger bound -125.0 Ma" ;
    skos:inScheme cs: ;
    skos:prefLabel "Barremian"@en ;
    prov:wasDerivedFrom ts:gts2020 ;
    sdo:color
        "30/0/50/0"^^:CMYK ,
        "179/223/127"^^:RGB ,
        "#B3DF7F"^^:RGBHex ;
.

:Bartonian
    a skos:Concept ;
    rdfs:isDefinedBy ts:gts2020 ;
    skos:altLabel
        "Бартон"@bg ,
        "Barton"@cs ,
        "Bartonien"@da ,
        "Bartonium"@de ,
        "Bartoniense"@es ,
        "Bartoni"@et ,
        "Barton"@fi ,
        "Bartonien"@fr ,
        "bartoni"@hu ,
        "bartoniano"@it ,
        "バートニアン期"@ja ,
        "Bartonis"@lt ,
        "Bartoniën"@nl ,
        "Barton"@no ,
        "Barton"@pl ,
        "Bartoniano"@pt ,
        "bartón"@sk ,
        "bartonij"@sl ,
        "barton"@sv ,
        "巴尔顿期"@zh ;
    skos:broader :Eocene ;
    skos:definition "A time period with the following approximated bounds: older bound -41.2 Ma, younger bound -37.8 Ma" ;
    skos:inScheme cs: ;
    skos:prefLabel "Bartonian"@en ;
    prov:wasDerivedFrom ts:gts2020 ;
    sdo:color
        "0/25/35/0"^^:CMYK ,
        "253/192/145"^^:RGB ,
        "#FDC091"^^:RGBHex ;
.

:Bashkirian
    a skos:Concept ;
    rdfs:isDefinedBy ts:gts2020 ;
    skos:altLabel
        "Башкир"@bg ,
        "Bashkir"@cs ,
        "Bashkirien"@da ,
        "Bashkirium"@de ,
        "Bashkiriense"@es ,
        "Baškiiri"@et ,
        "Bashkir"@fi ,
        "Bashkirien"@fr ,
        "baskír"@hu ,
        "bashkiriano"@it ,
        "バシキリアン期"@ja ,
        "Bashkirian"@lt ,
        "Bashkiriën"@nl ,
        "Bashkirium"@no ,
        "Baszkir"@pl ,
        "Bashkiriano"@pt ,
        "baškir"@sk ,
        "baškirij"@sl ,
        "bashkir"@sv ,
        "巴什基尔期"@zh ;
    skos:broader :LowerPennsylvanian ;
    skos:definition "A time period with the following approximated bounds: older bound -323.2 +|-0.4 Ma, younger bound -315.2 +|-0.2 Ma" ;
    skos:inScheme cs: ;
    skos:prefLabel "Bashkirian"@en ;
    prov:wasDerivedFrom ts:gts2020 ;
    sdo:color
        "40/10/20/0"^^:CMYK ,
        "153/194/181"^^:RGB ,
        "#99C2B5"^^:RGBHex ;
.

:Bathonian
    a skos:Concept ;
    rdfs:isDefinedBy ts:gts2020 ;
    skos:altLabel
        "Бат"@bg ,
        "Bathon"@cs ,
        "Bathonien"@da ,
        "Bathonium"@de ,
        "Bathoniense"@es ,
        "Bathoni"@et ,
        "Bathon"@fi ,
        "Bathonien"@fr ,
        "bath"@hu ,
        "bathoniano"@it ,
        "バソニアン期"@ja ,
        "Batonis"@lt ,
        "Barthoniën"@nl ,
        "Bathon"@no ,
        "Baton"@pl ,
        "Batoniano"@pt ,
        "bath"@sk ,
        "bathonij"@sl ,
        "bathon"@sv ,
        "巴通期"@zh ;
    skos:broader :MiddleJurassic ;
    skos:definition "A time period with the following approximated bounds: older bound -168.3 +|-1.3 Ma, younger bound -166.1 +|-1.2 Ma" ;
    skos:inScheme cs: ;
    skos:prefLabel "Bathonian"@en ;
    prov:wasDerivedFrom ts:gts2020 ;
    sdo:color
        "30/0/5/0"^^:CMYK ,
        "179/226/227"^^:RGB ,
        "#B3E2E3"^^:RGBHex ;
.

:Berriasian
    a skos:Concept ;
    rdfs:isDefinedBy ts:gts2020 ;
    skos:altLabel
        "Бериаѿ"@bg ,
        "Berrias"@cs ,
        "Berriasien"@da ,
        "Berriasium"@de ,
        "Berriasiense"@es ,
        "Berriasi"@et ,
        "Berrias"@fi ,
        "Berriasien"@fr ,
        "berriasi"@hu ,
        "berriasiano"@it ,
        "ベリアシアン期"@ja ,
        "Beriasis"@lt ,
        "Berrasiën"@nl ,
        "Berriasium"@no ,
        "Berias"@pl ,
        "Berriasiano"@pt ,
        "berias"@sk ,
        "berriasij"@sl ,
        "berrias"@sv ,
        "贝利亚斯期"@zh ;
    skos:broader :LowerCretaceous ;
    skos:definition "A time period with the following approximated bounds: older bound -145.0 Ma, younger bound -139.8 Ma" ;
    skos:inScheme cs: ;
    skos:prefLabel "Berriasian"@en ;
    prov:wasDerivedFrom ts:gts2020 ;
    sdo:color
        "45/0/65/0"^^:CMYK ,
        "140/205/96"^^:RGB ,
        "#8CCD60"^^:RGBHex ;
.

:Burdigalian
    a skos:Concept ;
    rdfs:isDefinedBy ts:gts2020 ;
    skos:altLabel
        "Бурдигал"@bg ,
        "Burdigal"@cs ,
        "Burdigalien"@da ,
        "Burdigalium"@de ,
        "Burdigaliense"@es ,
        "Burdigali"@et ,
        "Burdigal"@fi ,
        "Burdigalien"@fr ,
        "burdigaliai"@hu ,
        "burdigaliano"@it ,
        "バーディガリアン期"@ja ,
        "Burdigalis"@lt ,
        "Burdigaliën-Hemmoor"@nl ,
        "Burdigalium"@no ,
        "Burdygał"@pl ,
        "Burdigaliano"@pt ,
        "burdigal"@sk ,
        "burdigalij"@sl ,
        "burdigal"@sv ,
        "布迪加尔期"@zh ;
    skos:broader :Miocene ;
    skos:definition "A time period with the following approximated bounds: older bound -20.44 Ma, younger bound -15.97 Ma" ;
    skos:inScheme cs: ;
    skos:prefLabel "Burdigalian"@en ;
    prov:wasDerivedFrom ts:gts2020 ;
    sdo:color
        "0/0/75/0"^^:CMYK ,
        "255/255/65"^^:RGB ,
        "#FFFF41"^^:RGBHex ;
.

:Calabrian
    a skos:Concept ;
    rdfs:isDefinedBy ts:gts2020 ;
    skos:altLabel
        "Калабрий"@bg ,
        "Calabr"@cs ,
        "Calabrian"@da ,
        "Calabrium"@de ,
        "Calabriense"@es ,
        "Kalaabria"@et ,
        "Calabria"@fi ,
        "Calabrien"@fr ,
        "kalabriai"@hu ,
        "calabriano"@it ,
        "カラブリア期"@ja ,
        "Kalabris"@lt ,
        "Onder Pleistoceen/ Hoog Terras"@nl ,
        "Calabrium"@no ,
        "Kalambr"@pl ,
        "Calabriano"@pt ,
        "kalábrian"@sk ,
        "calabrij"@sl ,
        "calabr"@sv ,
        "卡拉布里亚期"@zh ;
    skos:broader :Pleistocene ;
    skos:definition "A time period with the following approximated bounds: older bound -1.80 Ma, younger bound -0.781 Ma" ;
    skos:inScheme cs: ;
    skos:prefLabel "Calabrian"@en ;
    prov:wasDerivedFrom ts:gts2020 ;
    sdo:color
        "0/5/25/0"^^:CMYK ,
        "255/242/186"^^:RGB ,
        "#FFF2BA"^^:RGBHex ;
.

:Callovian
    a skos:Concept ;
    rdfs:isDefinedBy ts:gts2020 ;
    skos:altLabel
        "Калов"@bg ,
        "Callov"@cs ,
        "Callovien"@da ,
        "Callovium"@de ,
        "Calloviense"@es ,
        "Callovi"@et ,
        "Callov"@fi ,
        "Callovien"@fr ,
        "callovi"@hu ,
        "calloviano"@it ,
        "カロビアン期"@ja ,
        "Kelovėjis"@lt ,
        "Calloviën"@nl ,
        "Callove"@no ,
        "Kelowej"@pl ,
        "Caloviano"@pt ,
        "kelovej"@sk ,
        "callovij"@sl ,
        "callov"@sv ,
        "卡洛夫期"@zh ;
    skos:broader :MiddleJurassic ;
    skos:definition "A time period with the following approximated bounds: older bound -166.1 +|-1.2 Ma, younger bound -163.5 +|-1.0 Ma" ;
    skos:inScheme cs: ;
    skos:prefLabel "Callovian"@en ;
    prov:wasDerivedFrom ts:gts2020 ;
    sdo:color
        "25/0/5/0"^^:CMYK ,
        "191/231/229"^^:RGB ,
        "#BFE7E5"^^:RGBHex ;
.

:Calymmian
    a skos:Concept ;
    rdfs:isDefinedBy ts:gts2020 ;
    skos:altLabel
        "Калим"@bg ,
        "Calymm"@cs ,
        "Calymmien"@da ,
        "Calymmium"@de ,
        "Calymmiense"@es ,
        "Calymm"@et ,
        "Calym"@fi ,
        "Calymmien"@fr ,
        "calymmi"@hu ,
        "calymmiano"@it ,
        "カリミアン紀"@ja ,
        "Kalymis"@lt ,
        "Calymmiën"@nl ,
        "Kalymmium"@no ,
        "Kalym"@pl ,
        "Calymiano"@pt ,
        "kalymnium"@sk ,
        "calymmij"@sl ,
        "kalymmium"@sv ,
        "盖层纪"@zh ;
    skos:broader :Mesoproterozoic ;
    skos:definition "A time period with the following approximated bounds: older bound -1600 Ma, younger bound -1400 Ma" ;
    skos:inScheme cs: ;
    skos:prefLabel "Calymmian"@en ;
    prov:wasDerivedFrom ts:gts2020 ;
    sdo:color
        "0/24/45/0"^^:CMYK ,
        "253/192/122"^^:RGB ,
        "#FDC07A"^^:RGBHex ;
.

:CambrianStage10
    a skos:Concept ;
    rdfs:isDefinedBy ts:gts2020 ;
    skos:altLabel
        "Камбрий - 10 етаж"@bg ,
        "Kambrium-Stupeň 10"@cs ,
        "Kambrium-Etage 10"@da ,
        "Kambrium-Stufe 10"@de ,
        "Cámbrico-Piso 10"@es ,
        "Kambrium, Lade 10"@et ,
        "Kambri-vaihe 10"@fi ,
        "Cambrien-Etage 10"@fr ,
        "kambrium 10. emelet"@hu ,
        "cambriano - stage 10"@it ,
        "第10期"@ja ,
        "Kambras-Aukštas 10"@lt ,
        "Cambrium, Zone 10"@nl ,
        "Kambrium-etasje10"@no ,
        "Kambr-Piętro 10"@pl ,
        "Câmbrico-Piso 10"@pt ,
        "kambrium, stupeň 10"@sk ,
        "kambrij-stopnja 10"@sl ,
        "kambrium etage 10"@sv ,
        "第十期"@zh ;
    skos:broader :Furongian ;
    skos:definition "A time period with the following approximated bounds: older bound -489.5 Ma, younger bound -485.4 +|-1.9 Ma" ;
    skos:inScheme cs: ;
    skos:prefLabel "Cambrian-Stage 10"@en ;
    prov:wasDerivedFrom ts:gts2020 ;
    sdo:color
        "10/0/20/0"^^:CMYK ,
        "230/245/201"^^:RGB ,
        "#E6F5C9"^^:RGBHex ;
.

:CambrianStage2
    a skos:Concept ;
    rdfs:isDefinedBy ts:gts2020 ;
    skos:altLabel
        "Камбрий - 2 етаж"@bg ,
        "Kambrium-Stupeň 2"@cs ,
        "Kambrium-Etage 2"@da ,
        "Kambrium-Stufe 2"@de ,
        "Cámbrico-Piso 2"@es ,
        "Kambrium, Lade 2"@et ,
        "Kambri-vaihe 2"@fi ,
        "Cambrien-Etage 2"@fr ,
        "kambrium 2. emelet"@hu ,
        "cambriano - stage 2"@it ,
        "第2期"@ja ,
        "Kambras-Aukštas 2"@lt ,
        "Cambrium, Zone 2"@nl ,
        "Kambrium-etasje 2"@no ,
        "Kambr-Piętro 2"@pl ,
        "Câmbrico-Piso 2"@pt ,
        "kambrium, stupeň 2"@sk ,
        "kambrij-stopnja 2"@sl ,
        "kambrium etage 1"@sv ,
        "第二期"@zh ;
    skos:broader :Terreneuvian ;
    skos:definition "A time period with the following approximated bounds: older bound -529 Ma, younger bound -521 Ma" ;
    skos:inScheme cs: ;
    skos:prefLabel "Cambrian-Stage 2"@en ;
    prov:wasDerivedFrom ts:gts2020 ;
    sdo:color
        "35/15/45/0"^^:CMYK ,
        "166/186/128"^^:RGB ,
        "#A6BA80"^^:RGBHex ;
.

:CambrianStage3
    a skos:Concept ;
    rdfs:isDefinedBy ts:gts2020 ;
    skos:altLabel
        "Камбрий - 3 етаж"@bg ,
        "Kambrium-Stupeň 3"@cs ,
        "Kambrium-Etage 3"@da ,
        "Kambrium-Stufe 3"@de ,
        "Cámbrico-Piso 3"@es ,
        "Kambrium, Lade 3"@et ,
        "Kambri-vaihe 3"@fi ,
        "Cambrien-Etage 3"@fr ,
        "kambrium 3. emelet"@hu ,
        "cambriano - stage 3"@it ,
        "第3期"@ja ,
        "Kambras-Aukštas 3"@lt ,
        "Cambrium, Zone3"@nl ,
        "Kambrium-etasje 3"@no ,
        "Kambr-Piętro 3"@pl ,
        "Câmbrico-Piso 3"@pt ,
        "kambrium, stupeň 3"@sk ,
        "kambrij-stopnja 3"@sl ,
        "kambrium etage 3"@sv ,
        "第三期"@zh ;
    skos:broader :CambrianSeries2 ;
    skos:definition "A time period with the following approximated bounds: older bound -521 Ma, younger bound -514 Ma" ;
    skos:inScheme cs: ;
    skos:prefLabel "Cambrian-Stage 3"@en ;
    prov:wasDerivedFrom ts:gts2020 ;
    sdo:color
        "35/10/45/0"^^:CMYK ,
        "166/197/131"^^:RGB ,
        "#A6C583"^^:RGBHex ;
.

:CambrianStage4
    a skos:Concept ;
    rdfs:isDefinedBy ts:gts2020 ;
    skos:altLabel
        "Камбрий - 4 етаж"@bg ,
        "Kambrium-Stupeň 4"@cs ,
        "Kambrium-Etage 4"@da ,
        "Kambrium-Stufe 4"@de ,
        "Cámbrico-Piso 4"@es ,
        "Kambrium, Lade 4"@et ,
        "Kambri-vaihe 4"@fi ,
        "Cambrien-Etage 4"@fr ,
        "kambrium 4. emelet"@hu ,
        "cambriano - stage 4"@it ,
        "第4期"@ja ,
        "Kambras-Aukšts 4"@lt ,
        "Cambrium, Zone 4"@nl ,
        "Kambrium-etasje 4"@no ,
        "Kambr-Piętro 4"@pl ,
        "Câmbrico-Piso 4"@pt ,
        "kambrium, stupeň 4"@sk ,
        "kambrij stopnja 4"@sl ,
        "kambrium etage 4"@sv ,
        "第四期"@zh ;
    skos:broader :CambrianSeries2 ;
    skos:definition "A time period with the following approximated bounds: older bound -514 Ma, younger bound -509 Ma" ;
    skos:inScheme cs: ;
    skos:prefLabel "Cambrian-Stage 4"@en ;
    prov:wasDerivedFrom ts:gts2020 ;
    sdo:color
        "30/10/40/0"^^:CMYK ,
        "179/202/142"^^:RGB ,
        "#B3CA8E"^^:RGBHex ;
.

:Campanian
    a skos:Concept ;
    rdfs:isDefinedBy ts:gts2020 ;
    skos:altLabel
        "Кампан"@bg ,
        "Campan"@cs ,
        "Campanien"@da ,
        "Campanium"@de ,
        "Campaniense"@es ,
        "Campani"@et ,
        "Campan"@fi ,
        "Campanien"@fr ,
        "campaniai"@hu ,
        "campaniano"@it ,
        "カンパニアン期"@ja ,
        "Kampanis"@lt ,
        "Campaniën"@nl ,
        "Campanium"@no ,
        "Kampan"@pl ,
        "Campaniano"@pt ,
        "kampán"@sk ,
        "campanij"@sl ,
        "campan"@sv ,
        "坎佩尼期"@zh ;
    skos:broader :UpperCretaceous ;
    skos:definition "A time period with the following approximated bounds: older bound -83.6 +|-0.2 Ma, younger bound -72.1 +|-0.2 Ma" ;
    skos:inScheme cs: ;
    skos:prefLabel "Campanian"@en ;
    prov:wasDerivedFrom ts:gts2020 ;
    sdo:color
        "10/0/50/0"^^:CMYK ,
        "230/244/127"^^:RGB ,
        "#E6F47F"^^:RGBHex ;
.

:Capitanian
    a skos:Concept ;
    rdfs:isDefinedBy ts:gts2020 ;
    skos:altLabel
        "Капитан"@bg ,
        "Capitan"@cs ,
        "Capitanien"@da ,
        "Capitanium"@de ,
        "Capitaniense"@es ,
        "Capitani"@et ,
        "Capitan"@fi ,
        "Capitanien"@fr ,
        "capitani"@hu ,
        "capitaniano"@it ,
        "カピタニアン期"@ja ,
        "Kapitanis"@lt ,
        "Capitaniën"@nl ,
        "Capitanium"@no ,
        "Kapitan"@pl ,
        "Capitaniano"@pt ,
        "capitan"@sk ,
        "capitanij"@sl ,
        "capitan"@sv ,
        "卡匹敦期"@zh ;
    skos:broader :Guadalupian ;
    skos:definition "A time period with the following approximated bounds: older bound -265.1 +|-0.4 Ma, younger bound -259.1 +|-0.5 Ma" ;
    skos:inScheme cs: ;
    skos:prefLabel "Capitanian"@en ;
    prov:wasDerivedFrom ts:gts2020 ;
    sdo:color
        "0/40/35/0"^^:CMYK ,
        "251/154/133"^^:RGB ,
        "#FB9A85"^^:RGBHex ;
.

:Carnian
    a skos:Concept ;
    rdfs:isDefinedBy ts:gts2020 ;
    skos:altLabel
        "Карн"@bg ,
        "Carn"@cs ,
        "Carnien"@da ,
        "Karnium"@de ,
        "Carniense"@es ,
        "Carni"@et ,
        "Carn"@fi ,
        "Carnien"@fr ,
        "karni"@hu ,
        "carnico"@it ,
        "カーニアン期"@ja ,
        "Karnis"@lt ,
        "Carniën"@nl ,
        "Carn"@no ,
        "Karnik"@pl ,
        "Carniano"@pt ,
        "karn"@sk ,
        "karnij"@sl ,
        "carn"@sv ,
        "卡尼期"@zh ;
    skos:broader :UpperTriassic ;
    skos:definition "A time period with the following approximated bounds: older bound -237 Ma, younger bound -227 Ma" ;
    skos:inScheme cs: ;
    skos:prefLabel "Carnian"@en ;
    prov:wasDerivedFrom ts:gts2020 ;
    sdo:color
        "20/35/0/0"^^:CMYK ,
        "201/155/203"^^:RGB ,
        "#C99BCB"^^:RGBHex ;
.

:Cenomanian
    a skos:Concept ;
    rdfs:isDefinedBy ts:gts2020 ;
    skos:altLabel
        "Ценоман"@bg ,
        "Cenoman"@cs ,
        "Cenomanien"@da ,
        "Cenomanium"@de ,
        "Cenomaniense"@es ,
        "Cenomani"@et ,
        "Cenoman"@fi ,
        "Cénomanien"@fr ,
        "cenoman"@hu ,
        "cenomaniano"@it ,
        "セノマニアン期"@ja ,
        "Cenomanis"@lt ,
        "Laat/Boven Krijt"@nl ,
        "Cenomanium"@no ,
        "Cenoman"@pl ,
        "Cenomaniano"@pt ,
        "cenoman"@sk ,
        "cenomanij"@sl ,
        "cenoman"@sv ,
        "森诺曼期"@zh ;
    skos:broader :UpperCretaceous ;
    skos:definition "A time period with the following approximated bounds: older bound -100.5 Ma, younger bound -93.9 Ma" ;
    skos:inScheme cs: ;
    skos:prefLabel "Cenomanian"@en ;
    prov:wasDerivedFrom ts:gts2020 ;
    sdo:color
        "30/0/70/0"^^:CMYK ,
        "179/222/83"^^:RGB ,
        "#B3DE53"^^:RGBHex ;
.

:Changhsingian
    a skos:Concept ;
    rdfs:isDefinedBy ts:gts2020 ;
    skos:altLabel
        "Чангшинг"@bg ,
        "Changhsing"@cs ,
        "Changhsingien"@da ,
        "Changhsingium"@de ,
        "Changsingiense"@es ,
        "Changhsingi"@et ,
        "Changhsing"@fi ,
        "Changhsingien"@fr ,
        "changhsingi"@hu ,
        "changsingiano"@it ,
        "チャンシンギアン期"@ja ,
        "Čangšinjanis"@lt ,
        "Changhsingiën"@nl ,
        "Changxingium"@no ,
        "Changhsing"@pl ,
        "Changhsingiano"@pt ,
        "Ŀchangsing"@sk ,
        "changhsingij"@sl ,
        "changhsing"@sv ,
        "长兴期"@zh ;
    skos:broader :Lopingian ;
    skos:definition "A time period with the following approximated bounds: older bound -254.14 +|-0.07 Ma, younger bound -251.902 +|-0.024 Ma" ;
    skos:inScheme cs: ;
    skos:prefLabel "Changhsingian"@en ;
    prov:wasDerivedFrom ts:gts2020 ;
    sdo:color
        "0/25/20/0"^^:CMYK ,
        "252/192/178"^^:RGB ,
        "#FCC0B2"^^:RGBHex ;
.

:Chattian
    a skos:Concept ;
    rdfs:isDefinedBy ts:gts2020 ;
    skos:altLabel
        "Хат"@bg ,
        "Chat"@cs ,
        "Chattien"@da ,
        "Chattium"@de ,
        "Chattiense"@es ,
        "Chatti"@et ,
        "Chatt"@fi ,
        "Chattien"@fr ,
        "katti"@hu ,
        "chattiano"@it ,
        "シャティアン期"@ja ,
        "Chatis"@lt ,
        "Chattiën"@nl ,
        "Chattium"@no ,
        "Szat"@pl ,
        "Chatiano"@pt ,
        "chatt"@sk ,
        "chattij"@sl ,
        "chatt"@sv ,
        "恰特期"@zh ;
    skos:broader :Oligocene ;
    skos:definition "A time period with the following approximated bounds: older bound -27.82 Ma, younger bound -23.03 Ma" ;
    skos:inScheme cs: ;
    skos:prefLabel "Chattian"@en ;
    prov:wasDerivedFrom ts:gts2020 ;
    sdo:color
        "0/10/30/0"^^:CMYK ,
        "254/230/170"^^:RGB ,
        "#FEE6AA"^^:RGBHex ;
.

:Chibanian
    a skos:Concept ;
    rdfs:isDefinedBy ts:gts2020 ;
    skos:broader :Pleistocene ;
    skos:definition "A time period with the following approximated bounds: older bound -0.781 Ma, younger bound -0.126 Ma" ;
    skos:inScheme cs: ;
    skos:prefLabel "Chibanian"@en ;
    prov:wasDerivedFrom ts:gts2020 ;
    sdo:color
        "0/5/20/0"^^:CMYK ,
        "255/242/199"^^:RGB ,
        "#FFF2C7"^^:RGBHex ;
.

:Coniacian
    a skos:Concept ;
    rdfs:isDefinedBy ts:gts2020 ;
    skos:altLabel
        "Кониак"@bg ,
        "Coniak"@cs ,
        "Coniacien"@da ,
        "Coniacium"@de ,
        "Coni"@es ,
        "Coniaci"@et ,
        "Coniac"@fi ,
        "Coniacien"@fr ,
        "coniaci"@hu ,
        "coniaciano"@it ,
        "コニアシアン期"@ja ,
        "Konjakis"@lt ,
        "Conaciën"@nl ,
        "Coniacium"@no ,
        "Koniak"@pl ,
        "Coniaciano"@pt ,
        "koňak"@sk ,
        "coniacij"@sl ,
        "coniac"@sv ,
        "科尼亚克期"@zh ;
    skos:broader :UpperCretaceous ;
    skos:definition "A time period with the following approximated bounds: older bound -89.8 +|-0.3 Ma, younger bound -86.3 +|-0.5 Ma" ;
    skos:inScheme cs: ;
    skos:prefLabel "Coniacian"@en ;
    prov:wasDerivedFrom ts:gts2020 ;
    sdo:color
        "20/0/60/0"^^:CMYK ,
        "204/233/104"^^:RGB ,
        "#CCE968"^^:RGBHex ;
.

:Cryogenian
    a skos:Concept ;
    rdfs:isDefinedBy ts:gts2020 ;
    skos:altLabel
        "Криоген"@bg ,
        "Cryogen"@cs ,
        "Cryogenien"@da ,
        "Kryogenium"@de ,
        "Criogeniense"@es ,
        "Krüogeen"@et ,
        "Cryogen"@fi ,
        "Cryogénien"@fr ,
        "cryogeni"@hu ,
        "cryogeniano"@it ,
        "クリオジェニアン紀"@ja ,
        "Kriogenis"@lt ,
        "Cryogeniën"@nl ,
        "Kryogenium"@no ,
        "Kriogen"@pl ,
        "Criogeniano"@pt ,
        "kryogén"@sk ,
        "cryogenij"@sl ,
        "kryogenium"@sv ,
        "成冰纪"@zh ;
    skos:broader :Neoproterozoic ;
    skos:definition "A time period with the following approximated bounds: older bound -720 Ma, younger bound -635 Ma" ;
    skos:inScheme cs: ;
    skos:prefLabel "Cryogenian"@en ;
    prov:wasDerivedFrom ts:gts2020 ;
    sdo:color
        "0/20/60/0"^^:CMYK ,
        "254/204/92"^^:RGB ,
        "#FECC5C"^^:RGBHex ;
.

:Danian
    a skos:Concept ;
    rdfs:isDefinedBy ts:gts2020 ;
    skos:altLabel
        "Дан"@bg ,
        "Dan"@cs ,
        "Danien"@da ,
        "Danium"@de ,
        "Daninese"@es ,
        "Taani"@et ,
        "Dan"@fi ,
        "Danien"@fr ,
        "dániai"@hu ,
        "daniano"@it ,
        "ダニアン期"@ja ,
        "Danis"@lt ,
        "Daniën"@nl ,
        "Danium"@no ,
        "Dan"@pl ,
        "Daniano"@pt ,
        "dán"@sk ,
        "danij"@sl ,
        "dan"@sv ,
        "丹麦期"@zh ;
    skos:broader :Paleocene ;
    skos:definition "A time period with the following approximated bounds: older bound -66.0 Ma, younger bound -61.6 Ma" ;
    skos:inScheme cs: ;
    skos:prefLabel "Danian"@en ;
    prov:wasDerivedFrom ts:gts2020 ;
    sdo:color
        "0/30/55/0"^^:CMYK ,
        "253/180/98"^^:RGB ,
        "#FDB462"^^:RGBHex ;
.

:Dapingian
    a skos:Concept ;
    rdfs:isDefinedBy ts:gts2020 ;
    skos:altLabel
        "Дапинг"@bg ,
        "Daping"@cs ,
        "Dapingien"@da ,
        "Dapingium"@de ,
        "Dapingiense"@es ,
        "Dapingi"@et ,
        "Daping"@fi ,
        "Dapingien"@fr ,
        "dapingi"@hu ,
        "dapingiano"@it ,
        "ダピンギアン期"@ja ,
        "Dapingis"@lt ,
        "Dapingiën"@nl ,
        "Dapingium"@no ,
        "Daping"@pl ,
        "Dapingiano"@pt ,
        "daping"@sk ,
        "dapingij"@sl ,
        "daping"@sv ,
        "大坪期"@zh ;
    skos:broader :MiddleOrdovician ;
    skos:definition "A time period with the following approximated bounds: older bound -470.0 +|-1.4 Ma, younger bound -467.3 +|-1.1 Ma" ;
    skos:inScheme cs: ;
    skos:prefLabel "Dapingian"@en ;
    prov:wasDerivedFrom ts:gts2020 ;
    sdo:color
        "60/0/40/0"^^:CMYK ,
        "102/192/146"^^:RGB ,
        "#66C092"^^:RGBHex ;
.

:Darriwilian
    a skos:Concept ;
    rdfs:isDefinedBy ts:gts2020 ;
    skos:altLabel
        "Даривил"@bg ,
        "Darriwil"@cs ,
        "Darriwilien"@da ,
        "Darriwilium"@de ,
        "Darriwiliense"@es ,
        "Darriwili"@et ,
        "Darriwil"@fi ,
        "Darriwilien"@fr ,
        "darriwili"@hu ,
        "darriwilliano"@it ,
        "ダーリウィリアン期"@ja ,
        "Darivilis"@lt ,
        "Darriwiliën"@nl ,
        "Daewillium"@no ,
        "Darriwil"@pl ,
        "Darriwiliano"@pt ,
        "darriwil"@sk ,
        "darriwilij"@sl ,
        "darriwil"@sv ,
        "达瑞威尔期"@zh ;
    skos:broader :MiddleOrdovician ;
    skos:definition "A time period with the following approximated bounds: older bound -467.3 +|-1.1 Ma, younger bound -458.4 +|-0.9 Ma" ;
    skos:inScheme cs: ;
    skos:prefLabel "Darriwilian"@en ;
    prov:wasDerivedFrom ts:gts2020 ;
    sdo:color
        "55/0/35/0"^^:CMYK ,
        "116/198/156"^^:RGB ,
        "#74C69C"^^:RGBHex ;
.

:Drumian
    a skos:Concept ;
    rdfs:isDefinedBy ts:gts2020 ;
    skos:altLabel
        "Друм"@bg ,
        "Drum"@cs ,
        "Drumien"@da ,
        "Drumium"@de ,
        "Drumiense"@es ,
        "Drumi"@et ,
        "Drum"@fi ,
        "Drumien"@fr ,
        "drumi"@hu ,
        "drumiano"@it ,
        "ドルミアン期"@ja ,
        "Drumis"@lt ,
        "Drumiën"@nl ,
        "Drumium"@no ,
        "Drum"@pl ,
        "Drumiano"@pt ,
        "drum"@sk ,
        "drumij"@sl ,
        "drum"@sv ,
        "鼓山期"@zh ;
    skos:broader :Miaolingian ;
    skos:definition "A time period with the following approximated bounds: older bound -504.5 Ma, younger bound -500.5 Ma" ;
    skos:inScheme cs: ;
    skos:prefLabel "Drumian"@en ;
    prov:wasDerivedFrom ts:gts2020 ;
    sdo:color
        "25/5/35/0"^^:CMYK ,
        "191/217/157"^^:RGB ,
        "#BFD99D"^^:RGBHex ;
.

:Ectasian
    a skos:Concept ;
    rdfs:isDefinedBy ts:gts2020 ;
    skos:altLabel
        "Ектаз"@bg ,
        "Ectas"@cs ,
        "Ectasien"@da ,
        "Ectasium"@de ,
        "Ectasiense"@es ,
        "Ectas"@et ,
        "Ectas"@fi ,
        "Ectasien"@fr ,
        "ectasi"@hu ,
        "ectasiano"@it ,
        "エクタシアン紀"@ja ,
        "Ektasis"@lt ,
        "Ectasiën"@nl ,
        "Ektasium"@no ,
        "Ektas"@pl ,
        "Ectasiano"@pt ,
        "ektazium"@sk ,
        "ectasij"@sl ,
        "ectasium"@sv ,
        "延展纪"@zh ;
    skos:broader :Mesoproterozoic ;
    skos:definition "A time period with the following approximated bounds: older bound -1400 Ma, younger bound -1200 Ma" ;
    skos:inScheme cs: ;
    skos:prefLabel "Ectasian"@en ;
    prov:wasDerivedFrom ts:gts2020 ;
    sdo:color
        "0/20/40/0"^^:CMYK ,
        "253/204/138"^^:RGB ,
        "#FDCC8A"^^:RGBHex ;
.

:Ediacaran
    a skos:Concept ;
    rdfs:isDefinedBy ts:gts2020 ;
    skos:altLabel
        "Едиакар"@bg ,
        "Ediacar"@cs ,
        "Ediacara"@da ,
        "Ediacarium"@de ,
        "Ediacariense"@es ,
        "Ediacara"@et ,
        "Ediacar"@fi ,
        "Ediacarien"@fr ,
        "ediacaranum"@hu ,
        "ediacariano"@it ,
        "エディアカラ紀"@ja ,
        "Ediakaras"@lt ,
        "Ediacaran"@nl ,
        "Ediacara"@no ,
        "Ediakar"@pl ,
        "Ediacariano"@pt ,
        "ediakarium"@sk ,
        "ediacarij"@sl ,
        "ediacara"@sv ,
        "埃迪卡拉纪"@zh ;
    skos:broader :Neoproterozoic ;
    skos:definition "A time period with the following approximated bounds: older bound -635 Ma, younger bound -541.0 +|-1.0 Ma" ;
    skos:inScheme cs: ;
    skos:prefLabel "Ediacaran"@en ;
    prov:wasDerivedFrom ts:gts2020 ;
    sdo:color
        "0/15/55/0"^^:CMYK ,
        "254/217/106"^^:RGB ,
        "#FED96A"^^:RGBHex ;
.

:Eifelian
    a skos:Concept ;
    rdfs:isDefinedBy ts:gts2020 ;
    skos:altLabel
        "пйфел"@bg ,
        "Eifel"@cs ,
        "Eifelien"@da ,
        "Eifelium"@de ,
        "Eifeliense"@es ,
        "Eifeli"@et ,
        "Eifel"@fi ,
        "Eifélien"@fr ,
        "eifeli"@hu ,
        "eifeliano"@it ,
        "アイフェリアン期"@ja ,
        "Eifelis"@lt ,
        "Eifeliën"@nl ,
        "Eifelium"@no ,
        "Eifel"@pl ,
        "Eifeliano"@pt ,
        "eifel"@sk ,
        "eifelij"@sl ,
        "eifel"@sv ,
        "艾菲尔期"@zh ;
    skos:broader :MiddleDevonian ;
    skos:definition "A time period with the following approximated bounds: older bound -393.3 +|-1.2 Ma, younger bound -387.7 +|-0.8 Ma" ;
    skos:inScheme cs: ;
    skos:prefLabel "Eifelian"@en ;
    prov:wasDerivedFrom ts:gts2020 ;
    sdo:color
        "5/15/50/0"^^:CMYK ,
        "241/213/118"^^:RGB ,
        "#F1D576"^^:RGBHex ;
.

:Emsian
    a skos:Concept ;
    rdfs:isDefinedBy ts:gts2020 ;
    skos:altLabel
        "Емѿ"@bg ,
        "Ems"@cs ,
        "Emsien"@da ,
        "Emsium"@de ,
        "Emsiense"@es ,
        "Emsi"@et ,
        "Ems"@fi ,
        "Emsien"@fr ,
        "emsi"@hu ,
        "emsiano"@it ,
        "エムシアン期"@ja ,
        "Emsis"@lt ,
        "Emsiën"@nl ,
        "Emsium"@no ,
        "Ems"@pl ,
        "Emsiano"@pt ,
        "ems"@sk ,
        "emsij"@sl ,
        "ems"@sv ,
        "艾姆斯期"@zh ;
    skos:broader :LowerDevonian ;
    skos:definition "A time period with the following approximated bounds: older bound -407.6 +|-2.6 Ma, younger bound -393.3 +|-1.2 Ma" ;
    skos:inScheme cs: ;
    skos:prefLabel "Emsian"@en ;
    prov:wasDerivedFrom ts:gts2020 ;
    sdo:color
        "10/15/50/0"^^:CMYK ,
        "229/208/117"^^:RGB ,
        "#E5D075"^^:RGBHex ;
.

:Eoarchean
    a skos:Concept ;
    rdfs:isDefinedBy ts:gts2020 ;
    skos:altLabel
        "Еоархай"@bg ,
        "Eoarchaikum"@cs ,
        "Eoarkæisk"@da ,
        "Eoarchaikum"@de ,
        "Eoarchaean"@en-GB ,
        "Eoarchean"@en-US ,
        "Eoarcaico"@es ,
        "Eoarhaikum"@et ,
        "Eoarkeikum"@fi ,
        "Eoarchéen"@fr ,
        "eoarchaikum"@hu ,
        "eoarcheano"@it ,
        "暁始生代"@ja ,
        "Eoarchejus"@lt ,
        "Eo-archaicum"@nl ,
        "Eoarkeikum"@no ,
        "Eoarchaik"@pl ,
        "Eoarcaico"@pt ,
        "eoarchaikum"@sk ,
        "eoarhaik"@sl ,
        "eoarkeikum"@sv ,
        "始太古代"@zh ;
    skos:broader :Archean ;
    skos:definition "A time period with the following approximated bounds: older bound -4000 Ma, younger bound -3600 Ma" ;
    skos:inScheme cs: ;
    skos:prefLabel "Eoarchean"@en ;
    prov:wasDerivedFrom ts:gts2020 ;
    sdo:color
        "10/100/0/0"^^:CMYK ,
        "218/3/127"^^:RGB ,
        "#DA037F"^^:RGBHex ;
.

:Famennian
    a skos:Concept ;
    rdfs:isDefinedBy ts:gts2020 ;
    skos:altLabel
        "Фамен"@bg ,
        "Famen"@cs ,
        "Famennien"@da ,
        "Fammennium"@de ,
        "Fameniense"@es ,
        "Famenne"@et ,
        "Fammenn"@fi ,
        "Famennien"@fr ,
        "famenni"@hu ,
        "famenniano"@it ,
        "ファメニアン期"@ja ,
        "Famenis"@lt ,
        "Famenniën"@nl ,
        "Famennium"@no ,
        "Famen"@pl ,
        "Fameniano"@pt ,
        "famen"@sk ,
        "fammenij"@sl ,
        "famenn"@sv ,
        "法门期"@zh ;
    skos:broader :UpperDevonian ;
    skos:definition "A time period with the following approximated bounds: older bound -372.2 +|-1.6 Ma, younger bound -358.9 +|-0.4 Ma" ;
    skos:inScheme cs: ;
    skos:prefLabel "Famennian"@en ;
    prov:wasDerivedFrom ts:gts2020 ;
    sdo:color
        "5/5/20/0"^^:CMYK ,
        "242/237/179"^^:RGB ,
        "#F2EDB3"^^:RGBHex ;
.

:Floian
    a skos:Concept ;
    rdfs:isDefinedBy ts:gts2020 ;
    skos:altLabel
        "Flo"@cs ,
        "Floian"@da ,
        "Floium"@de ,
        "Floiense"@es ,
        "Floi"@et ,
        "Flo"@fi ,
        "Floien"@fr ,
        "floi"@hu ,
        "floiano"@it ,
        "フロイアン期"@ja ,
        "Flois"@lt ,
        "Floiën"@nl ,
        "Floium"@no ,
        "Flo"@pl ,
        "Floiano"@pt ,
        "flo"@sk ,
        "floij"@sl ,
        "flo"@sv ,
        "弗洛期"@zh ;
    skos:broader :LowerOrdovician ;
    skos:definition "A time period with the following approximated bounds: older bound -477.7 +|-1.4 Ma, younger bound -470.0 +|-1.4 Ma" ;
    skos:inScheme cs: ;
    skos:prefLabel "Floian"@en ;
    prov:wasDerivedFrom ts:gts2020 ;
    sdo:color
        "75/0/45/0"^^:CMYK ,
        "65/176/135"^^:RGB ,
        "#41B087"^^:RGBHex ;
.

:Fortunian
    a skos:Concept ;
    rdfs:isDefinedBy ts:gts2020 ;
    skos:altLabel
        "Фортун"@bg ,
        "Fortun"@cs ,
        "Fortunien"@da ,
        "Fortunium"@de ,
        "Fortuniense"@es ,
        "Fortune"@et ,
        "Fortun"@fi ,
        "Fortunien"@fr ,
        "fortuni"@hu ,
        "fortuniano"@it ,
        "フォルツニアン期"@ja ,
        "Fortunis"@lt ,
        "Fortuniën"@nl ,
        "Fortunium"@no ,
        "Fortun"@pl ,
        "Fortuniano"@pt ,
        "fortun"@sk ,
        "fortunij"@sl ,
        "fortun"@sv ,
        "好运期"@zh ;
    skos:broader :Terreneuvian ;
    skos:definition "A time period with the following approximated bounds: older bound -541.0 +|-1.0 Ma, younger bound -529 Ma" ;
    skos:inScheme cs: ;
    skos:prefLabel "Fortunian"@en ;
    prov:wasDerivedFrom ts:gts2020 ;
    sdo:color
        "40/15/50/0"^^:CMYK ,
        "153/181/117"^^:RGB ,
        "#99B575"^^:RGBHex ;
.

:Frasnian
    a skos:Concept ;
    rdfs:isDefinedBy ts:gts2020 ;
    skos:altLabel
        "Фран"@bg ,
        "Frasn"@cs ,
        "Frasnien"@da ,
        "Frasnium"@de ,
        "Frasniense"@es ,
        "Frasne"@et ,
        "Frasn"@fi ,
        "Frasnien"@fr ,
        "frasni"@hu ,
        "frasniano"@it ,
        "フラスニアン期"@ja ,
        "Franis"@lt ,
        "Frasniën"@nl ,
        "Frasneium"@no ,
        "Fran"@pl ,
        "Frasniano"@pt ,
        "frasn"@sk ,
        "frasnij"@sl ,
        "frasn"@sv ,
        "弗拉斯期"@zh ;
    skos:broader :UpperDevonian ;
    skos:definition "A time period with the following approximated bounds: older bound -382.7 +|-1.6 Ma, younger bound -372.2 +|-1.6 Ma" ;
    skos:inScheme cs: ;
    skos:prefLabel "Frasnian"@en ;
    prov:wasDerivedFrom ts:gts2020 ;
    sdo:color
        "5/5/30/0"^^:CMYK ,
        "242/237/173"^^:RGB ,
        "#F2EDAD"^^:RGBHex ;
.

:Gelasian
    a skos:Concept ;
    rdfs:isDefinedBy ts:gts2020 ;
    skos:altLabel
        "Gelas"@cs ,
        "Gelasian"@da ,
        "Gelasium"@de ,
        "Gelasiense"@es ,
        "Gelasi"@et ,
        "Gelas"@fi ,
        "Gelasien"@fr ,
        "gelasi"@hu ,
        "gelasiano"@it ,
        "ゲラシアン期"@ja ,
        "Gelasis"@lt ,
        "Pretigliën + Tigliën"@nl ,
        "Gelasium"@no ,
        "Gelas"@pl ,
        "Gelasiano"@pt ,
        "gelas"@sk ,
        "gelasij"@sl ,
        "gelas"@sv ,
        "格拉斯期"@zh ;
    skos:broader :Pleistocene ;
    skos:definition "A time period with the following approximated bounds: older bound -2.58 Ma, younger bound -1.80 Ma" ;
    skos:inScheme cs: ;
    skos:prefLabel "Gelasian"@en ;
    prov:wasDerivedFrom ts:gts2020 ;
    sdo:color
        "0/5/30/0"^^:CMYK ,
        "255/237/179"^^:RGB ,
        "#FFEDB3"^^:RGBHex ;
.

:Givetian
    a skos:Concept ;
    rdfs:isDefinedBy ts:gts2020 ;
    skos:altLabel
        "Живет"@bg ,
        "Givet"@cs ,
        "Givetien"@da ,
        "Givetium"@de ,
        "Givetiense"@es ,
        "Givet"@et ,
        "Givet"@fi ,
        "Givétien"@fr ,
        "giveti"@hu ,
        "givetiano"@it ,
        "ジベーチアン期"@ja ,
        "Živetis"@lt ,
        "Givetiën"@nl ,
        "Givetium"@no ,
        "Żywet"@pl ,
        "Givetiano"@pt ,
        "givet"@sk ,
        "givetij"@sl ,
        "givet"@sv ,
        "吉维特期"@zh ;
    skos:broader :MiddleDevonian ;
    skos:definition "A time period with the following approximated bounds: older bound -387.7 +|-0.8 Ma, younger bound -382.7 +|-1.6 Ma" ;
    skos:inScheme cs: ;
    skos:prefLabel "Givetian"@en ;
    prov:wasDerivedFrom ts:gts2020 ;
    sdo:color
        "5/10/45/0"^^:CMYK ,
        "241/225/133"^^:RGB ,
        "#F1E185"^^:RGBHex ;
.

:Gorstian
    a skos:Concept ;
    rdfs:isDefinedBy ts:gts2020 ;
    skos:altLabel
        "Горѿт"@bg ,
        "Gorst"@cs ,
        "Gorstien"@da ,
        "Gorstium"@de ,
        "Gorstiense"@es ,
        "Gorsti"@et ,
        "Gorst"@fi ,
        "Gorstien"@fr ,
        "gorsti"@hu ,
        "gorstiano"@it ,
        "ゴースティアン期"@ja ,
        "Gorstis"@lt ,
        "Gorstiën"@nl ,
        "Gorstium"@no ,
        "Gorst"@pl ,
        "Gorstiano"@pt ,
        "gorst"@sk ,
        "gorstij"@sl ,
        "gorst"@sv ,
        "格斯特期"@zh ;
    skos:broader :Ludlow ;
    skos:definition "A time period with the following approximated bounds: older bound -427.4 +|-0.5 Ma, younger bound -425.6 +|-0.9 Ma" ;
    skos:inScheme cs: ;
    skos:prefLabel "Gorstian"@en ;
    prov:wasDerivedFrom ts:gts2020 ;
    sdo:color
        "20/0/10/0"^^:CMYK ,
        "204/236/221"^^:RGB ,
        "#CCECDD"^^:RGBHex ;
.

:Greenlandian
    a skos:Concept ;
    rdfs:isDefinedBy ts:gts2020 ;
    skos:broader :Holocene ;
    skos:definition "A time period with the following approximated bounds: older bound -0.0117 Ma, younger bound -0.0082 Ma" ;
    skos:inScheme cs: ;
    skos:prefLabel "Greenlandian"@en ;
    prov:wasDerivedFrom ts:gts2020 ;
    sdo:color
        "0/10/15/0"^^:CMYK ,
        "254/236/219"^^:RGB ,
        "#FEECDB"^^:RGBHex ;
.

:Guzhangian
    a skos:Concept ;
    rdfs:isDefinedBy ts:gts2020 ;
    skos:altLabel
        "Жужанг"@bg ,
        "Guzhang"@cs ,
        "Guzhangien"@da ,
        "Guzhangium"@de ,
        "Guzhangiense"@es ,
        "Guzhangi"@et ,
        "Guzhang"@fi ,
        "Guzhangien"@fr ,
        "guzhangi"@hu ,
        "guzhangiano"@it ,
        "グザンギアン期"@ja ,
        "Gužangis"@lt ,
        "Guzhangiën"@nl ,
        "Guzhangium"@no ,
        "Gużang"@pl ,
        "Guzhangiano"@pt ,
        "gužang"@sk ,
        "guzhangij"@sl ,
        "guzhang"@sv ,
        "古丈期"@zh ;
    skos:broader :Miaolingian ;
    skos:definition "A time period with the following approximated bounds: older bound -500.5 Ma, younger bound -497 Ma" ;
    skos:inScheme cs: ;
    skos:prefLabel "Guzhangian"@en ;
    prov:wasDerivedFrom ts:gts2020 ;
    sdo:color
        "20/5/30/0"^^:CMYK ,
        "204/223/170"^^:RGB ,
        "#CCDFAA"^^:RGBHex ;
.

:Gzhelian
    a skos:Concept ;
    rdfs:isDefinedBy ts:gts2020 ;
    skos:altLabel
        "Гжел"@bg ,
        "Gzhel"@cs ,
        "Gzhelien"@da ,
        "Gzhelium"@de ,
        "Gzeliense"@es ,
        "Gzheli"@et ,
        "Gzhel"@fi ,
        "Gzhélien"@fr ,
        "gzseli"@hu ,
        "gzheliano"@it ,
        "グゼリアン期"@ja ,
        "Gželis"@lt ,
        "Gzheliën"@nl ,
        "Gzhelium"@no ,
        "Gżel"@pl ,
        "Gzeliano"@pt ,
        "gžel"@sk ,
        "gželij"@sl ,
        "gzhel"@sv ,
        "格热尔期"@zh ;
    skos:broader :UpperPennsylvanian ;
    skos:definition "A time period with the following approximated bounds: older bound -303.7 +|-0.1 Ma, younger bound -298.9 +|-0.15 Ma" ;
    skos:inScheme cs: ;
    skos:prefLabel "Gzhelian"@en ;
    prov:wasDerivedFrom ts:gts2020 ;
    sdo:color
        "20/10/15/0"^^:CMYK ,
        "204/212/199"^^:RGB ,
        "#CCD4C7"^^:RGBHex ;
.

:Hadean
    a skos:Concept ;
    rdfs:isDefinedBy ts:gts2020 ;
    skos:altLabel
        "Hád (spodní hranice není definována)"@cs ,
        "Hadean"@da ,
        "Hadaikum"@de ,
        "Hadeánico"@es ,
        "Hadesi??"@et ,
        "Hadea"@fi ,
        "Hadéen"@fr ,
        "hadei"@hu ,
        "adeano"@it ,
        "冥王代（非公式の）"@ja ,
        "Hadejus (neoficialus)"@lt ,
        "Hadeïcum"@nl ,
        "Hadeikum"@no ,
        "Hadean (Nieformalny)"@pl ,
        "Hadeano"@pt ,
        "hadaikum"@sk ,
        "hadej (neformalno)"@sl ,
        "hadeikum"@sv ,
        "冥古宙（非正式）"@zh ;
    skos:broader :Precambrian ;
    skos:definition "A time period with the following approximated bounds: older bound -4567 +|-1 Ma, younger bound -4000 Ma" ;
    skos:inScheme cs: ;
    skos:prefLabel "Hadean"@en ;
    prov:wasDerivedFrom ts:gts2020 ;
    sdo:color
        "30/100/0/0"^^:CMYK ,
        "174/2/126"^^:RGB ,
        "#AE027E"^^:RGBHex ;
.

:Hauterivian
    a skos:Concept ;
    rdfs:isDefinedBy ts:gts2020 ;
    skos:altLabel
        "Хотрив"@bg ,
        "Hauteriv"@cs ,
        "Hauterivien"@da ,
        "Hauterivium"@de ,
        "Hauteviriense"@es ,
        "Hauterivi"@et ,
        "Hauteriv"@fi ,
        "Hauterivien"@fr ,
        "hauterivi"@hu ,
        "hauteriviano"@it ,
        "オーテリビアン期"@ja ,
        "Hoterivis"@lt ,
        "Hauteriviën"@nl ,
        "Hauterivium"@no ,
        "Hoteryw"@pl ,
        "Hauteriviano"@pt ,
        "hauteriv"@sk ,
        "hauterivij"@sl ,
        "hauteriv"@sv ,
        "豪特里维期"@zh ;
    skos:broader :LowerCretaceous ;
    skos:definition "A time period with the following approximated bounds: older bound -132.9 Ma, younger bound -129.4 Ma" ;
    skos:inScheme cs: ;
    skos:prefLabel "Hauterivian"@en ;
    prov:wasDerivedFrom ts:gts2020 ;
    sdo:color
        "35/0/55/0"^^:CMYK ,
        "166/217/117"^^:RGB ,
        "#A6D975"^^:RGBHex ;
.

:Hettangian
    a skos:Concept ;
    rdfs:isDefinedBy ts:gts2020 ;
    skos:altLabel
        "Хетанж"@bg ,
        "Hettang"@cs ,
        "Hettangien"@da ,
        "Hettangium"@de ,
        "Hettagiense"@es ,
        "Hettangi"@et ,
        "Hettang"@fi ,
        "Hettangien"@fr ,
        "hettangi"@hu ,
        "hettangiano"@it ,
        "ヘッタンギアン期"@ja ,
        "Hetangis"@lt ,
        "Hettangiën"@nl ,
        "Hettang"@no ,
        "Hetang"@pl ,
        "Hetangiano"@pt ,
        "hetanž"@sk ,
        "hettangij"@sl ,
        "hettang"@sv ,
        "赫唐期"@zh ;
    skos:broader :LowerJurassic ;
    skos:definition "A time period with the following approximated bounds: older bound -201.3 +|-0.2 Ma, younger bound -199.3 +|-0.3 Ma" ;
    skos:inScheme cs: ;
    skos:prefLabel "Hettangian"@en ;
    prov:wasDerivedFrom ts:gts2020 ;
    sdo:color
        "70/5/0/0"^^:CMYK ,
        "78/179/211"^^:RGB ,
        "#4EB3D3"^^:RGBHex ;
.

:Hirnantian
    a skos:Concept ;
    rdfs:isDefinedBy ts:gts2020 ;
    skos:altLabel
        "Хирнант"@bg ,
        "Hirnant"@cs ,
        "Hirnantien"@da ,
        "Hirnantium"@de ,
        "Hirnantiense"@es ,
        "Hirnantia"@et ,
        "Hirnant"@fi ,
        "Hirnantien"@fr ,
        "hirnanti"@hu ,
        "hirnantiano"@it ,
        "ヒルナンティアン期"@ja ,
        "Hirnantis"@lt ,
        "Hirnantiën"@nl ,
        "Hirnatium"@no ,
        "Hirnant"@pl ,
        "Hirnantiano"@pt ,
        "hirnant"@sk ,
        "hirnantij"@sl ,
        "hirnant"@sv ,
        "赫南特期"@zh ;
    skos:broader :UpperOrdovician ;
    skos:definition "A time period with the following approximated bounds: older bound -445.2 +|-1.4 Ma, younger bound -443.8 +|-1.5 Ma" ;
    skos:inScheme cs: ;
    skos:prefLabel "Hirnantian"@en ;
    prov:wasDerivedFrom ts:gts2020 ;
    sdo:color
        "35/0/30/0"^^:CMYK ,
        "166/219/171"^^:RGB ,
        "#A6DBAB"^^:RGBHex ;
.

:Homerian
    a skos:Concept ;
    rdfs:isDefinedBy ts:gts2020 ;
    skos:altLabel
        "Хомер"@bg ,
        "Homer"@cs ,
        "Homerien"@da ,
        "Homerium"@de ,
        "Homeriense"@es ,
        "Homeri"@et ,
        "Homer"@fi ,
        "Homérien"@fr ,
        "homeri"@hu ,
        "homeriano"@it ,
        "ホメリアン期"@ja ,
        "Homeris"@lt ,
        "Homeriën"@nl ,
        "Homer"@no ,
        "Homer"@pl ,
        "Homeriano"@pt ,
        "homer"@sk ,
        "homerij"@sl ,
        "homer"@sv ,
        "侯默期"@zh ;
    skos:broader :Wenlock ;
    skos:definition "A time period with the following approximated bounds: older bound -430.5 +|-0.7 Ma, younger bound -427.4 +|-0.5 Ma" ;
    skos:inScheme cs: ;
    skos:prefLabel "Homerian"@en ;
    prov:wasDerivedFrom ts:gts2020 ;
    sdo:color
        "20/0/15/0"^^:CMYK ,
        "204/235/209"^^:RGB ,
        "#CCEBD1"^^:RGBHex ;
.

:Induan
    a skos:Concept ;
    rdfs:isDefinedBy ts:gts2020 ;
    skos:altLabel
        "Инд"@bg ,
        "Indu"@cs ,
        "Induen"@da ,
        "Indusium"@de ,
        "Induense"@es ,
        "Indu"@et ,
        "Indus"@fi ,
        "Induen"@fr ,
        "indusi"@hu ,
        "induano"@it ,
        "インドゥアン期"@ja ,
        "Indis"@lt ,
        "Induiën"@nl ,
        "Indu"@no ,
        "Ind"@pl ,
        "Induano"@pt ,
        "indu"@sk ,
        "indij"@sl ,
        "indu"@sv ,
        "印度期"@zh ;
    skos:broader :LowerTriassic ;
    skos:definition "A time period with the following approximated bounds: older bound -251.902 +|-0.024 Ma, younger bound -251.2 Ma" ;
    skos:inScheme cs: ;
    skos:prefLabel "Induan"@en ;
    prov:wasDerivedFrom ts:gts2020 ;
    sdo:color
        "35/70/0/0"^^:CMYK ,
        "164/70/159"^^:RGB ,
        "#A4469F"^^:RGBHex ;
.

:Jiangshanian
    a skos:Concept ;
    rdfs:isDefinedBy ts:gts2020 ;
    skos:altLabel "江山期"@zh ;
    skos:broader :Furongian ;
    skos:definition "A time period with the following approximated bounds: older bound -494 Ma, younger bound -489.5 Ma" ;
    skos:inScheme cs: ;
    skos:prefLabel "Jiangshanian"@en ;
    prov:wasDerivedFrom ts:gts2020 ;
    sdo:color
        "15/0/25/0"^^:CMYK ,
        "217/240/187"^^:RGB ,
        "#D9F0BB"^^:RGBHex ;
.

:Kasimovian
    a skos:Concept ;
    rdfs:isDefinedBy ts:gts2020 ;
    skos:altLabel
        "Каѿимов"@bg ,
        "Kasimov"@cs ,
        "Kasimovien"@da ,
        "Kasimovium"@de ,
        "Kasimoviense"@es ,
        "Kasimovi"@et ,
        "Kasimov"@fi ,
        "Kasimovien"@fr ,
        "kaszimovi"@hu ,
        "kasimoviano"@it ,
        "カシモビアン期"@ja ,
        "Kasimovis"@lt ,
        "Kasimoviën"@nl ,
        "Kasimovium"@no ,
        "Kasimow"@pl ,
        "Kasimoviano"@pt ,
        "kasimov"@sk ,
        "kasimovij"@sl ,
        "kasimov"@sv ,
        "卡西莫夫期"@zh ;
    skos:broader :UpperPennsylvanian ;
    skos:definition "A time period with the following approximated bounds: older bound -307 +|-0.1 Ma, younger bound -303.7 +|-0.1 Ma" ;
    skos:inScheme cs: ;
    skos:prefLabel "Kasimovian"@en ;
    prov:wasDerivedFrom ts:gts2020 ;
    sdo:color
        "25/10/15/0"^^:CMYK ,
        "191/208/197"^^:RGB ,
        "#BFD0C5"^^:RGBHex ;
.

:Katian
    a skos:Concept ;
    rdfs:isDefinedBy ts:gts2020 ;
    skos:altLabel
        "Кат"@bg ,
        "Kat"@cs ,
        "Katien"@da ,
        "Katium"@de ,
        "Katiense"@es ,
        "Kati"@et ,
        "Kat"@fi ,
        "Katien"@fr ,
        "kati"@hu ,
        "katiano"@it ,
        "カティアン期"@ja ,
        "Katis"@lt ,
        "Katiën"@nl ,
        "Katium"@no ,
        "Kat"@pl ,
        "Katiano"@pt ,
        "kat"@sk ,
        "katij"@sl ,
        "kat"@sv ,
        "凯迪期"@zh ;
    skos:broader :UpperOrdovician ;
    skos:definition "A time period with the following approximated bounds: older bound -453 +|-0.7 Ma, younger bound -445.2 +|-1.4 Ma" ;
    skos:inScheme cs: ;
    skos:prefLabel "Katian"@en ;
    prov:wasDerivedFrom ts:gts2020 ;
    sdo:color
        "40/0/35/0"^^:CMYK ,
        "153/214/159"^^:RGB ,
        "#99D69F"^^:RGBHex ;
.

:Kimmeridgian
    a skos:Concept ;
    rdfs:isDefinedBy ts:gts2020 ;
    skos:altLabel
        "Кимеридж"@bg ,
        "Kimmeridž"@cs ,
        "Kimmeridgien"@da ,
        "Kimmeridgium"@de ,
        "Kimmeridgiense"@es ,
        "Kimmeridge"@et ,
        "Kimmeridge"@fi ,
        "Kimméridgien"@fr ,
        "kimmeridgei"@hu ,
        "kimmeridgiano"@it ,
        "キンメリッジアン期"@ja ,
        "Kimeridis"@lt ,
        "Kimmeridgiën"@nl ,
        "Kimmeridge"@no ,
        "Kimeryd"@pl ,
        "Kimeridgiano"@pt ,
        "kimeridž"@sk ,
        "kimmeridgij"@sl ,
        "kimmeridge"@sv ,
        "启莫里支期"@zh ;
    skos:broader :UpperJurassic ;
    skos:definition "A time period with the following approximated bounds: older bound -157.3 +|-1.0 Ma, younger bound -152.1 +|-0.9 Ma" ;
    skos:inScheme cs: ;
    skos:prefLabel "Kimmeridgian"@en ;
    prov:wasDerivedFrom ts:gts2020 ;
    sdo:color
        "20/0/0/0"^^:CMYK ,
        "204/236/244"^^:RGB ,
        "#CCECF4"^^:RGBHex ;
.

:Kungurian
    a skos:Concept ;
    rdfs:isDefinedBy ts:gts2020 ;
    skos:altLabel
        "Кунгур"@bg ,
        "Kungur"@cs ,
        "Kungurien"@da ,
        "Kungurium"@de ,
        "Kunguriense"@es ,
        "Kunguri"@et ,
        "Kungur"@fi ,
        "Kungurien"@fr ,
        "kunguri"@hu ,
        "kungurianno"@it ,
        "クングリアン期"@ja ,
        "Kunguris"@lt ,
        "Kunguriën"@nl ,
        "Kungurium"@no ,
        "Kungur"@pl ,
        "Kunguriano"@pt ,
        "kungur"@sk ,
        "kungurij"@sl ,
        "kungur"@sv ,
        "孔古尔期"@zh ;
    skos:broader :Cisuralian ;
    skos:definition "A time period with the following approximated bounds: older bound -283.5 +|-0.6 Ma, younger bound -272.95 +|-0.11 Ma" ;
    skos:inScheme cs: ;
    skos:prefLabel "Kungurian"@en ;
    prov:wasDerivedFrom ts:gts2020 ;
    sdo:color
        "10/45/40/0"^^:CMYK ,
        "227/135/118"^^:RGB ,
        "#E38776"^^:RGBHex ;
.

:Ladinian
    a skos:Concept ;
    rdfs:isDefinedBy ts:gts2020 ;
    skos:altLabel
        "Ладин"@bg ,
        "Ladin"@cs ,
        "Ladinien"@da ,
        "Ladinium"@de ,
        "Ladiniense"@es ,
        "Ladini"@et ,
        "Ladin"@fi ,
        "Ladinien"@fr ,
        "ladin"@hu ,
        "ladinico"@it ,
        "ラディニアン期"@ja ,
        "Ladinis"@lt ,
        "Ladiniën"@nl ,
        "Ladin"@no ,
        "Ladyn"@pl ,
        "Ladiniano"@pt ,
        "ladin"@sk ,
        "ladinij"@sl ,
        "ladin"@sv ,
        "拉迪尼亚期"@zh ;
    skos:broader :MiddleTriassic ;
    skos:definition "A time period with the following approximated bounds: older bound -242 Ma, younger bound -237 Ma" ;
    skos:inScheme cs: ;
    skos:prefLabel "Ladinian"@en ;
    prov:wasDerivedFrom ts:gts2020 ;
    sdo:color
        "20/45/0/0"^^:CMYK ,
        "201/131/191"^^:RGB ,
        "#C983BF"^^:RGBHex ;
.

:Langhian
    a skos:Concept ;
    rdfs:isDefinedBy ts:gts2020 ;
    skos:altLabel
        "Ланг"@bg ,
        "Langh"@cs ,
        "Langhien"@da ,
        "Langhium"@de ,
        "Langhiense"@es ,
        "Langhi"@et ,
        "Langh"@fi ,
        "Langhien"@fr ,
        "langhei"@hu ,
        "langhiano"@it ,
        "ランギアン期"@ja ,
        "Langis"@lt ,
        "Langhiën-Reinbek"@nl ,
        "Langhium"@no ,
        "Lang"@pl ,
        "Langhiano"@pt ,
        "langh"@sk ,
        "langhij"@sl ,
        "langh"@sv ,
        "兰海期"@zh ;
    skos:broader :Miocene ;
    skos:definition "A time period with the following approximated bounds: older bound -15.97 Ma, younger bound -13.82 Ma" ;
    skos:inScheme cs: ;
    skos:prefLabel "Langhian"@en ;
    prov:wasDerivedFrom ts:gts2020 ;
    sdo:color
        "0/0/70/0"^^:CMYK ,
        "255/255/77"^^:RGB ,
        "#FFFF4D"^^:RGBHex ;
.

:Lochkovian
    a skos:Concept ;
    rdfs:isDefinedBy ts:gts2020 ;
    skos:altLabel
        "Ложков"@bg ,
        "Lochkov"@cs ,
        "Lochkovien"@da ,
        "Lochkovium"@de ,
        "Lochkoviense"@es ,
        "Lochkovi"@et ,
        "Lochkov"@fi ,
        "Lochkovien"@fr ,
        "lochkovi"@hu ,
        "lochkoviano"@it ,
        "ロッコビアン期"@ja ,
        "Lochkovis"@lt ,
        "Lochkoviën"@nl ,
        "Lochkovium"@no ,
        "Lochkow"@pl ,
        "Lochkoviano"@pt ,
        "lochkov"@sk ,
        "lochkovij"@sl ,
        "lochkov"@sv ,
        "洛赫科夫期"@zh ;
    skos:broader :LowerDevonian ;
    skos:definition "A time period with the following approximated bounds: older bound -419.2 +|-3.2 Ma, younger bound -410.8 +|-2.8 Ma" ;
    skos:inScheme cs: ;
    skos:prefLabel "Lochkovian"@en ;
    prov:wasDerivedFrom ts:gts2020 ;
    sdo:color
        "10/25/60/0"^^:CMYK ,
        "229/183/90"^^:RGB ,
        "#E5B75A"^^:RGBHex ;
.

:Ludfordian
    a skos:Concept ;
    rdfs:isDefinedBy ts:gts2020 ;
    skos:altLabel
        "Лудфорд"@bg ,
        "Ludford"@cs ,
        "Ludfordien"@da ,
        "Ludfordium"@de ,
        "Ludfordiense"@es ,
        "Ludfordi"@et ,
        "Ludford"@fi ,
        "Ludfordien"@fr ,
        "ludfordi"@hu ,
        "ludfordiano"@it ,
        "ルドフォーディアン期"@ja ,
        "Lutfordis"@lt ,
        "Ludfordiën"@nl ,
        "Ludford"@no ,
        "Ludford"@pl ,
        "Ludfordiano"@pt ,
        "ludford"@sk ,
        "ludfordij"@sl ,
        "ludford"@sv ,
        "卢德福德期"@zh ;
    skos:broader :Ludlow ;
    skos:definition "A time period with the following approximated bounds: older bound -425.6 +|-0.9 Ma, younger bound -423 +|-2.3 Ma" ;
    skos:inScheme cs: ;
    skos:prefLabel "Ludfordian"@en ;
    prov:wasDerivedFrom ts:gts2020 ;
    sdo:color
        "15/0/10/0"^^:CMYK ,
        "217/240/223"^^:RGB ,
        "#D9F0DF"^^:RGBHex ;
.

:Lutetian
    a skos:Concept ;
    rdfs:isDefinedBy ts:gts2020 ;
    skos:altLabel
        "Лютеѿ"@bg ,
        "Lutet"@cs ,
        "Lutetien"@da ,
        "Lutetium"@de ,
        "Luteciense"@es ,
        "Luteti"@et ,
        "Lutet"@fi ,
        "Lutétien"@fr ,
        "lutetiai"@hu ,
        "leteziano"@it ,
        "ルテシアン期"@ja ,
        "Liutetis"@lt ,
        "Lutetiën"@nl ,
        "Litetium"@no ,
        "Lutet"@pl ,
        "Luteciano"@pt ,
        "lutét"@sk ,
        "lutecij"@sl ,
        "lutet"@sv ,
        "卢台特期"@zh ;
    skos:broader :Eocene ;
    skos:definition "A time period with the following approximated bounds: older bound -47.8 Ma, younger bound -41.2 Ma" ;
    skos:inScheme cs: ;
    skos:prefLabel "Lutetian"@en ;
    prov:wasDerivedFrom ts:gts2020 ;
    sdo:color
        "0/30/40/0"^^:CMYK ,
        "253/180/130"^^:RGB ,
        "#FDB482"^^:RGBHex ;
.

:Maastrichtian
    a skos:Concept ;
    rdfs:isDefinedBy ts:gts2020 ;
    skos:altLabel
        "Маѿтрихт"@bg ,
        "Maastricht"@cs ,
        "Maastrichtien"@da ,
        "Maastrichtium"@de ,
        "Maastrichtiense"@es ,
        "Maastrichti"@et ,
        "Maastricht"@fi ,
        "Maastrichtien"@fr ,
        "maastrichti"@hu ,
        "maastrichtiano"@it ,
        "マーストリヒシアン期"@ja ,
        "Mastrichtis"@lt ,
        "Maastrichtiën"@nl ,
        "Maastricht"@no ,
        "Mastrycht"@pl ,
        "Maestrichtiano"@pt ,
        "mástricht"@sk ,
        "maastrichtij"@sl ,
        "maastricht"@sv ,
        "马斯特里赫特期"@zh ;
    skos:broader :UpperCretaceous ;
    skos:definition "A time period with the following approximated bounds: older bound -72.1 +|-0.2 Ma, younger bound -66.0 Ma" ;
    skos:inScheme cs: ;
    skos:prefLabel "Maastrichtian"@en ;
    prov:wasDerivedFrom ts:gts2020 ;
    sdo:color
        "5/0/45/0"^^:CMYK ,
        "242/250/140"^^:RGB ,
        "#F2FA8C"^^:RGBHex ;
.

:Meghalayan
    a skos:Concept ;
    rdfs:isDefinedBy ts:gts2020 ;
    skos:broader :Holocene ;
    skos:definition "A time period with the following approximated bounds: older bound -0.0042 Ma, younger bound 0 Ma" ;
    skos:inScheme cs: ;
    skos:prefLabel "Meghalayan"@en ;
    prov:wasDerivedFrom ts:gts2020 ;
    sdo:color
        "0/10/5/0"^^:CMYK ,
        "253/237/236"^^:RGB ,
        "#FDEDEC"^^:RGBHex ;
.

:Mesoarchean
    a skos:Concept ;
    rdfs:isDefinedBy ts:gts2020 ;
    skos:altLabel
        "Мезоархай"@bg ,
        "Mezoarchaikum"@cs ,
        "Mesoarkæisk"@da ,
        "Mesoarchaikum"@de ,
        "Mesoarchaean"@en-GB ,
        "Mesoarchean"@en-US ,
        "Mesoarcaico"@es ,
        "Mesoarhaikum"@et ,
        "Mesoarkeikum"@fi ,
        "Mésoarchéen"@fr ,
        "mezoarchai"@hu ,
        "mesoarcheano"@it ,
        "中始生代"@ja ,
        "Mezoarchejus"@lt ,
        "Meso-archaicum"@nl ,
        "Mesoarkeikum"@no ,
        "Mezoarchaik"@pl ,
        "Mesoarcaico"@pt ,
        "mezoarchaikum"@sk ,
        "mezoarhaik"@sl ,
        "mesoarkeikum"@sv ,
        "中太古代"@zh ;
    skos:broader :Archean ;
    skos:definition "A time period with the following approximated bounds: older bound -3200 Ma, younger bound -2800 Ma" ;
    skos:inScheme cs: ;
    skos:prefLabel "Mesoarchean"@en ;
    prov:wasDerivedFrom ts:gts2020 ;
    sdo:color
        "0/60/5/0"^^:CMYK ,
        "247/104/169"^^:RGB ,
        "#F768A9"^^:RGBHex ;
.

:Messinian
    a skos:Concept ;
    rdfs:isDefinedBy ts:gts2020 ;
    skos:altLabel
        "Меѿин"@bg ,
        "Messin"@cs ,
        "Messinien"@da ,
        "Messinium"@de ,
        "Messiniense"@es ,
        "Messini"@et ,
        "Messina"@fi ,
        "Messinien"@fr ,
        "messinai"@hu ,
        "messiniano"@it ,
        "メッシニアン期"@ja ,
        "Mesinis"@lt ,
        "Susteriën"@nl ,
        "Messinium"@no ,
        "Messyn"@pl ,
        "Messiniano"@pt ,
        "messin"@sk ,
        "messinij"@sl ,
        "messin"@sv ,
        "墨西拿期"@zh ;
    skos:broader :Miocene ;
    skos:definition "A time period with the following approximated bounds: older bound -7.246 Ma, younger bound -5.333 Ma" ;
    skos:inScheme cs: ;
    skos:prefLabel "Messinian"@en ;
    prov:wasDerivedFrom ts:gts2020 ;
    sdo:color
        "0/0/55/0"^^:CMYK ,
        "255/255/115"^^:RGB ,
        "#FFFF73"^^:RGBHex ;
.

:Moscovian
    a skos:Concept ;
    rdfs:isDefinedBy ts:gts2020 ;
    skos:altLabel
        "Моѿков"@bg ,
        "Moscov"@cs ,
        "Moscovien"@da ,
        "Moskovium"@de ,
        "Moscoviense"@es ,
        "Moskva"@et ,
        "Moskova"@fi ,
        "Moscovien"@fr ,
        "moszkvai"@hu ,
        "moscoviano"@it ,
        "モスコビアン期"@ja ,
        "Moskovis"@lt ,
        "Moscoviën"@nl ,
        "Moskovium"@no ,
        "Moskow"@pl ,
        "Moscoviano"@pt ,
        "moskov"@sk ,
        "moskovij"@sl ,
        "moscov"@sv ,
        "莫斯科期"@zh ;
    skos:broader :MiddlePennsylvanian ;
    skos:definition "A time period with the following approximated bounds: older bound -315.2 +|-0.2 Ma, younger bound -307 +|-0.1 Ma" ;
    skos:inScheme cs: ;
    skos:prefLabel "Moscovian"@en ;
    prov:wasDerivedFrom ts:gts2020 ;
    sdo:color
        "30/10/20/0"^^:CMYK ,
        "179/203/185"^^:RGB ,
        "#B3CBB9"^^:RGBHex ;
.

:Neoarchean
    a skos:Concept ;
    rdfs:isDefinedBy ts:gts2020 ;
    skos:altLabel
        "пеоархай"@bg ,
        "Neoarchaikum"@cs ,
        "Neoarkæisk"@da ,
        "Neoarchaikum"@de ,
        "Neoarchaean"@en-GB ,
        "Neoarchean"@en-US ,
        "Neoarcaico"@es ,
        "Neoarhaikum"@et ,
        "Neoarkeikum"@fi ,
        "Néoarchéen"@fr ,
        "neoarchaikum"@hu ,
        "neoarcheano"@it ,
        "新始生代"@ja ,
        "Neoarchejus"@lt ,
        "Neo-archaicum"@nl ,
        "Neoarkeikum"@no ,
        "Neoarchaik"@pl ,
        "Neoarcaico"@pt ,
        "neoarchaikum"@sk ,
        "neoarhaik"@sl ,
        "neoarkeikum"@sv ,
        "新太古代"@zh ;
    skos:broader :Archean ;
    skos:definition "A time period with the following approximated bounds: older bound -2800 Ma, younger bound -2500 Ma" ;
    skos:inScheme cs: ;
    skos:prefLabel "Neoarchean"@en ;
    prov:wasDerivedFrom ts:gts2020 ;
    sdo:color
        "0/40/5/0"^^:CMYK ,
        "249/155/193"^^:RGB ,
        "#F99BC1"^^:RGBHex ;
.

:Norian
    a skos:Concept ;
    rdfs:isDefinedBy ts:gts2020 ;
    skos:altLabel
        "пор"@bg ,
        "Nor"@cs ,
        "Norien"@da ,
        "Norium"@de ,
        "Noriense"@es ,
        "Nori"@et ,
        "Nor"@fi ,
        "Norien"@fr ,
        "nori"@hu ,
        "norico"@it ,
        "ノーリアン期"@ja ,
        "Noris"@lt ,
        "Noriën"@nl ,
        "Nor"@no ,
        "Noryk"@pl ,
        "Noriano"@pt ,
        "norik"@sk ,
        "norij"@sl ,
        "nor"@sv ,
        "诺利克期"@zh ;
    skos:broader :UpperTriassic ;
    skos:definition "A time period with the following approximated bounds: older bound -227 Ma, younger bound -208.5 Ma" ;
    skos:inScheme cs: ;
    skos:prefLabel "Norian"@en ;
    prov:wasDerivedFrom ts:gts2020 ;
    sdo:color
        "15/30/0/0"^^:CMYK ,
        "214/170/211"^^:RGB ,
        "#D6AAD3"^^:RGBHex ;
.

:Northgrippian
    a skos:Concept ;
    rdfs:isDefinedBy ts:gts2020 ;
    skos:broader :Holocene ;
    skos:definition "A time period with the following approximated bounds: older bound -0.0082 Ma, younger bound -0.0042 Ma" ;
    skos:inScheme cs: ;
    skos:prefLabel "Northgrippian"@en ;
    prov:wasDerivedFrom ts:gts2020 ;
    sdo:color
        "0/10/10/0"^^:CMYK ,
        "253/236/228"^^:RGB ,
        "#FDECE4"^^:RGBHex ;
.

:Olenekian
    a skos:Concept ;
    rdfs:isDefinedBy ts:gts2020 ;
    skos:altLabel
        "Оленек"@bg ,
        "Olenek"@cs ,
        "Olenekien"@da ,
        "Olenekium"@de ,
        "Olenekiense"@es ,
        "Oleneki"@et ,
        "Olenek"@fi ,
        "Olénekien"@fr ,
        "olenyoki"@hu ,
        "olenekiano"@it ,
        "オレネキアン期"@ja ,
        "Olenekis"@lt ,
        "Olenekiën"@nl ,
        "Olenek"@no ,
        "Olenek"@pl ,
        "Olenekiano"@pt ,
        "olenek"@sk ,
        "olenekij"@sl ,
        "olenek"@sv ,
        "奥伦尼克期"@zh ;
    skos:broader :LowerTriassic ;
    skos:definition "A time period with the following approximated bounds: older bound -251.2 Ma, younger bound -247.2 Ma" ;
    skos:inScheme cs: ;
    skos:prefLabel "Olenekian"@en ;
    prov:wasDerivedFrom ts:gts2020 ;
    sdo:color
        "30/65/0/0"^^:CMYK ,
        "176/81/165"^^:RGB ,
        "#B051A5"^^:RGBHex ;
.

:Orosirian
    a skos:Concept ;
    rdfs:isDefinedBy ts:gts2020 ;
    skos:altLabel
        "Ороѿир"@bg ,
        "Orosir"@cs ,
        "Orosirien"@da ,
        "Orosirium"@de ,
        "Orosiriense"@es ,
        "Orosir"@et ,
        "Orosir"@fi ,
        "Orosirien"@fr ,
        "orosiri"@hu ,
        "orosiriano"@it ,
        "オロシリアン紀"@ja ,
        "Orosiris"@lt ,
        "Orosiriën"@nl ,
        "Orosirium"@no ,
        "Orosir"@pl ,
        "Orosiriano"@pt ,
        "orosirium"@sk ,
        "orosijrij"@sl ,
        "orosirium"@sv ,
        "造山纪"@zh ;
    skos:broader :Paleoproterozoic ;
    skos:definition "A time period with the following approximated bounds: older bound -2050 Ma, younger bound -1800 Ma" ;
    skos:inScheme cs: ;
    skos:prefLabel "Orosirian"@en ;
    prov:wasDerivedFrom ts:gts2020 ;
    sdo:color
        "0/60/15/0"^^:CMYK ,
        "247/104/152"^^:RGB ,
        "#F76898"^^:RGBHex ;
.

:Oxfordian
    a skos:Concept ;
    rdfs:isDefinedBy ts:gts2020 ;
    skos:altLabel
        "Окѿфорд"@bg ,
        "Oxford"@cs ,
        "Oxfordien"@da ,
        "Oxfordium"@de ,
        "Oxfordiense"@es ,
        "Oxfordi"@et ,
        "Oxford"@fi ,
        "Oxfordien"@fr ,
        "oxfordi"@hu ,
        "oxfordiano"@it ,
        "オックスフォーディアン期"@ja ,
        "Oksfordis"@lt ,
        "Oxfordiën"@nl ,
        "Oxford"@no ,
        "Oksford"@pl ,
        "Oxfordiano"@pt ,
        "oxford"@sk ,
        "oxfordij"@sl ,
        "oxford"@sv ,
        "牛津期"@zh ;
    skos:broader :UpperJurassic ;
    skos:definition "A time period with the following approximated bounds: older bound -163.5 +|-1.0 Ma, younger bound -157.3 +|-1.0 Ma" ;
    skos:inScheme cs: ;
    skos:prefLabel "Oxfordian"@en ;
    prov:wasDerivedFrom ts:gts2020 ;
    sdo:color
        "25/0/0/0"^^:CMYK ,
        "191/231/241"^^:RGB ,
        "#BFE7F1"^^:RGBHex ;
.

:Paibian
    a skos:Concept ;
    rdfs:isDefinedBy ts:gts2020 ;
    skos:altLabel
        "Паиб"@bg ,
        "Paib"@cs ,
        "Paibien"@da ,
        "Paibium"@de ,
        "Paibiense"@es ,
        "Paibi"@et ,
        "Paib"@fi ,
        "Paibien"@fr ,
        "paibi"@hu ,
        "paibiano"@it ,
        "パイビアン期"@ja ,
        "Paibis"@lt ,
        "Paibiën"@nl ,
        "Paibium"@no ,
        "Paib"@pl ,
        "Paibiano"@pt ,
        "pajb"@sk ,
        "paibij"@sl ,
        "paib"@sv ,
        "排碧期"@zh ;
    skos:broader :Furongian ;
    skos:definition "A time period with the following approximated bounds: older bound -497 Ma, younger bound -494 Ma" ;
    skos:inScheme cs: ;
    skos:prefLabel "Paibian"@en ;
    prov:wasDerivedFrom ts:gts2020 ;
    sdo:color
        "20/0/35/0"^^:CMYK ,
        "204/235/174"^^:RGB ,
        "#CCEBAE"^^:RGBHex ;
.

:Paleoarchean
    a skos:Concept ;
    rdfs:isDefinedBy ts:gts2020 ;
    skos:altLabel
        "Палеоархай"@bg ,
        "Paleoarchaikum"@cs ,
        "Palæoarkæisk"@da ,
        "Paläoarchaikum"@de ,
        "Palaeoarchaean"@en-GB ,
        "Paleoarchean"@en-US ,
        "Paleoarcaico"@es ,
        "Paleoarhaikum"@et ,
        "Paleoarkeikum"@fi ,
        "Paléoarchéen"@fr ,
        "paleoarchai"@hu ,
        "paleoarcheano"@it ,
        "古始生代"@ja ,
        "Paleoarchejus"@lt ,
        "Paleo-archaicum"@nl ,
        "Paleoarkeikum"@no ,
        "Paleoarchaik"@pl ,
        "Paleoarcaico"@pt ,
        "paleoarchaikum"@sk ,
        "paleoarhaik"@sl ,
        "paleoarkeikum"@sv ,
        "古太古代"@zh ;
    skos:broader :Archean ;
    skos:definition "A time period with the following approximated bounds: older bound -3600 Ma, younger bound -3200 Ma" ;
    skos:inScheme cs: ;
    skos:prefLabel "Paleoarchean"@en ;
    prov:wasDerivedFrom ts:gts2020 ;
    sdo:color
        "0/75/0/0"^^:CMYK ,
        "244/68/159"^^:RGB ,
        "#F4449F"^^:RGBHex ;
.

:Piacenzian
    a skos:Concept ;
    rdfs:isDefinedBy ts:gts2020 ;
    skos:altLabel
        "Пиачен"@bg ,
        "Piacenz"@cs ,
        "Piacenzien"@da ,
        "Piacenzium"@de ,
        "Plazenciense"@es ,
        "Piacenzi"@et ,
        "Piacenz"@fi ,
        "Piacenzien"@fr ,
        "piacenzai"@hu ,
        "piacenziano"@it ,
        "ﾋﾟｱｾﾝｼﾞｱﾝ期"@ja ,
        "PiaĿenzis"@lt ,
        "Reuveriën"@nl ,
        "Piecenzium"@no ,
        "Piacenz"@pl ,
        "Placenciano"@pt ,
        "piaĿenz"@sk ,
        "piacenzij"@sl ,
        "piacenz"@sv ,
        "皮亚琴期"@zh ;
    skos:broader :Pliocene ;
    skos:definition "A time period with the following approximated bounds: older bound -3.6 Ma, younger bound -2.58 Ma" ;
    skos:inScheme cs: ;
    skos:prefLabel "Piacenzian"@en ;
    prov:wasDerivedFrom ts:gts2020 ;
    sdo:color
        "0/0/25/0"^^:CMYK ,
        "255/255/191"^^:RGB ,
        "#FFFFBF"^^:RGBHex ;
.

:Pliensbachian
    a skos:Concept ;
    rdfs:isDefinedBy ts:gts2020 ;
    skos:altLabel
        "Плиинѿбах"@bg ,
        "Pliensbach"@cs ,
        "Pliensbachien"@da ,
        "Pliensbachium"@de ,
        "Pliensbachiense"@es ,
        "Pliensbachi"@et ,
        "Plienbach"@fi ,
        "Pliensbachien"@fr ,
        "pliensbachi"@hu ,
        "pliensbachiano"@it ,
        "プリンスバッキアン期"@ja ,
        "Plynsbachis"@lt ,
        "Pliënsbachiën"@nl ,
        "Pliensbach"@no ,
        "Pliensbach"@pl ,
        "Pliensbaquiano"@pt ,
        "pliensbach"@sk ,
        "pleinsbachij"@sl ,
        "pliensbach"@sv ,
        "普连斯巴奇期"@zh ;
    skos:broader :LowerJurassic ;
    skos:definition "A time period with the following approximated bounds: older bound -190.8 +|-1.0 Ma, younger bound -182.7 +|-0.7 Ma" ;
    skos:inScheme cs: ;
    skos:prefLabel "Pliensbachian"@en ;
    prov:wasDerivedFrom ts:gts2020 ;
    sdo:color
        "50/5/0/0"^^:CMYK ,
        "128/197/221"^^:RGB ,
        "#80C5DD"^^:RGBHex ;
.

:Pragian
    a skos:Concept ;
    rdfs:isDefinedBy ts:gts2020 ;
    skos:altLabel
        "Праг"@bg ,
        "Prag"@cs ,
        "Pragien"@da ,
        "Pragium"@de ,
        "Praguiense"@es ,
        "Praha"@et ,
        "Praha"@fi ,
        "Praguien"@fr ,
        "prágai"@hu ,
        "pragiano"@it ,
        "プラギアン期"@ja ,
        "Pragis"@lt ,
        "Pragiën"@nl ,
        "Pragium"@no ,
        "Prag"@pl ,
        "Pragiano"@pt ,
        "prág"@sk ,
        "pragij"@sl ,
        "prag"@sv ,
        "布拉格期"@zh ;
    skos:broader :LowerDevonian ;
    skos:definition "A time period with the following approximated bounds: older bound -410.8 +|-2.8 Ma, younger bound -407.6 +|-2.6 Ma" ;
    skos:inScheme cs: ;
    skos:prefLabel "Pragian"@en ;
    prov:wasDerivedFrom ts:gts2020 ;
    sdo:color
        "10/20/55/0"^^:CMYK ,
        "229/196/104"^^:RGB ,
        "#E5C468"^^:RGBHex ;
.

:Priabonian
    a skos:Concept ;
    rdfs:isDefinedBy ts:gts2020 ;
    skos:altLabel
        "Приабон"@bg ,
        "Priabon"@cs ,
        "Priabonien"@da ,
        "Priabonium"@de ,
        "Priaboniense"@es ,
        "Priaboni"@et ,
        "Priabon"@fi ,
        "Priabonien"@fr ,
        "priabonai"@hu ,
        "priaboniano"@it ,
        "プリアボニアン期"@ja ,
        "Priabonis"@lt ,
        "Priaboniën"@nl ,
        "Priabon"@no ,
        "Priabon"@pl ,
        "Priaboniano"@pt ,
        "priabón"@sk ,
        "priabonij"@sl ,
        "priabon"@sv ,
        "普里阿邦期"@zh ;
    skos:broader :Eocene ;
    skos:definition "A time period with the following approximated bounds: older bound -37.8 Ma, younger bound -33.9 Ma" ;
    skos:inScheme cs: ;
    skos:prefLabel "Priabonian"@en ;
    prov:wasDerivedFrom ts:gts2020 ;
    sdo:color
        "0/20/30/0"^^:CMYK ,
        "253/205/161"^^:RGB ,
        "#FDCDA1"^^:RGBHex ;
.

:Pridoli
    a skos:Concept ;
    rdfs:isDefinedBy ts:gts2020 ;
    skos:altLabel
        "Пржидол"@bg ,
        "Přídolí"@cs ,
        "Pridoli"@da ,
        "Pridoli"@de ,
        "Prídoli"@es ,
        "Pridoli"@et ,
        "Pridoli"@fi ,
        "Pridoli"@fr ,
        "pridoli"@hu ,
        "pridoli"@it ,
        "プリドリアン世"@ja ,
        "Pržidolis"@lt ,
        "Pridoli"@nl ,
        "Pridoli"@no ,
        "Przydol"@pl ,
        "Pridoli"@pt ,
        "přídol"@sk ,
        "pridolij"@sl ,
        "pridoli"@sv ,
        "普里多利世"@zh ;
    skos:broader :Silurian ;
    skos:definition "A time period with the following approximated bounds: older bound -423 +|-2.3 Ma, younger bound -419.2 +|-3.2 Ma" ;
    skos:inScheme cs: ;
    skos:prefLabel "Pridoli"@en ;
    prov:wasDerivedFrom ts:gts2020 ;
    sdo:color
        "10/0/10/0"^^:CMYK ,
        "230/245/225"^^:RGB ,
        "#E6F5E1"^^:RGBHex ;
.

:Rhaetian
    a skos:Concept ;
    rdfs:isDefinedBy ts:gts2020 ;
    skos:altLabel
        "Рет"@bg ,
        "Rhaet"@cs ,
        "Rhaetien"@da ,
        "Rhätium"@de ,
        "Rhetiense"@es ,
        "Rhaeti"@et ,
        "Rhaet"@fi ,
        "Rhétien"@fr ,
        "rhaeti"@hu ,
        "retico"@it ,
        "レーティアン期"@ja ,
        "Retis"@lt ,
        "Rhaetiën"@nl ,
        "Ræt"@no ,
        "Retyk"@pl ,
        "Reciano"@pt ,
        "rét"@sk ,
        "retij"@sl ,
        "rät"@sv ,
        "瑞替期"@zh ;
    skos:broader :UpperTriassic ;
    skos:definition "A time period with the following approximated bounds: older bound -208.5 Ma, younger bound -201.3 +|-0.2 Ma" ;
    skos:inScheme cs: ;
    skos:prefLabel "Rhaetian"@en ;
    prov:wasDerivedFrom ts:gts2020 ;
    sdo:color
        "10/25/0/0"^^:CMYK ,
        "227/185/219"^^:RGB ,
        "#E3B9DB"^^:RGBHex ;
.

:Rhuddanian
    a skos:Concept ;
    rdfs:isDefinedBy ts:gts2020 ;
    skos:altLabel
        "Рудан"@bg ,
        "Rhuddan"@cs ,
        "Rhuddanien"@da ,
        "Rhuddanium"@de ,
        "Rhuddaniense"@es ,
        "Rhuddani"@et ,
        "Rhuddan"@fi ,
        "Rhuddanien"@fr ,
        "rhuddani"@hu ,
        "rhuddaniano"@it ,
        "ルダニアン期"@ja ,
        "Rudanis"@lt ,
        "Rhuddaniën"@nl ,
        "Rhuddanium"@no ,
        "Rhuddan"@pl ,
        "Rudaniano"@pt ,
        "rhuddan"@sk ,
        "rhuddanij"@sl ,
        "rhuddan"@sv ,
        "鲁丹期"@zh ;
    skos:broader :Llandovery ;
    skos:definition "A time period with the following approximated bounds: older bound -443.8 +|-1.5 Ma, younger bound -440.8 +|-1.2 Ma" ;
    skos:inScheme cs: ;
    skos:prefLabel "Rhuddanian"@en ;
    prov:wasDerivedFrom ts:gts2020 ;
    sdo:color
        "35/0/25/0"^^:CMYK ,
        "166/220/181"^^:RGB ,
        "#A6DCB5"^^:RGBHex ;
.

:Rhyacian
    a skos:Concept ;
    rdfs:isDefinedBy ts:gts2020 ;
    skos:altLabel
        "Риац"@bg ,
        "Rhyak"@cs ,
        "Rhyacien"@da ,
        "Rhyacium"@de ,
        "Ryaciense"@es ,
        "Rhyac"@et ,
        "Ryak"@fi ,
        "Rhyacien"@fr ,
        "rhyaci"@hu ,
        "rhyaciano"@it ,
        "リヤシアン紀"@ja ,
        "Riacis"@lt ,
        "Rhyaciën"@nl ,
        "Ryasium"@no ,
        "Riak"@pl ,
        "Riaciano"@pt ,
        "rhyacium"@sk ,
        "rhyacij"@sl ,
        "ryacium"@sv ,
        "层侵纪"@zh ;
    skos:broader :Paleoproterozoic ;
    skos:definition "A time period with the following approximated bounds: older bound -2300 Ma, younger bound -2050 Ma" ;
    skos:inScheme cs: ;
    skos:prefLabel "Rhyacian"@en ;
    prov:wasDerivedFrom ts:gts2020 ;
    sdo:color
        "0/65/20/0"^^:CMYK ,
        "247/91/137"^^:RGB ,
        "#F75B89"^^:RGBHex ;
.

:Roadian
    a skos:Concept ;
    rdfs:isDefinedBy ts:gts2020 ;
    skos:altLabel
        "Роад"@bg ,
        "Road"@cs ,
        "Roadien"@da ,
        "Roadium"@de ,
        "Roadiense"@es ,
        "Roadi"@et ,
        "Road"@fi ,
        "Roadien"@fr ,
        "roadi"@hu ,
        "roadiano"@it ,
        "ローディアン期"@ja ,
        "Roadis"@lt ,
        "Roadiën"@nl ,
        "Roadium"@no ,
        "Road"@pl ,
        "Roadiano"@pt ,
        "road"@sk ,
        "roadij"@sl ,
        "road"@sv ,
        "罗德期"@zh ;
    skos:broader :Guadalupian ;
    skos:definition "A time period with the following approximated bounds: older bound -272.95 +|-0.11 Ma, younger bound -268.8 +|-0.5 Ma" ;
    skos:inScheme cs: ;
    skos:prefLabel "Roadian"@en ;
    prov:wasDerivedFrom ts:gts2020 ;
    sdo:color
        "0/50/45/0"^^:CMYK ,
        "251/128/105"^^:RGB ,
        "#FB8069"^^:RGBHex ;
.

:Rupelian
    a skos:Concept ;
    rdfs:isDefinedBy ts:gts2020 ;
    skos:altLabel
        "Рупел"@bg ,
        "Rupel"@cs ,
        "Rupelien"@da ,
        "Rupelium"@de ,
        "Rupeliense"@es ,
        "Rupeli"@et ,
        "Rupel"@fi ,
        "Rupélien"@fr ,
        "rupeli"@hu ,
        "rupeliano"@it ,
        "ルペル期"@ja ,
        "Rupelis"@lt ,
        "Rupeliën"@nl ,
        "Rupel"@no ,
        "Rupel"@pl ,
        "Rupeliano"@pt ,
        "rupel"@sk ,
        "rupelij"@sl ,
        "rupel"@sv ,
        "鲁珀利期"@zh ;
    skos:broader :Oligocene ;
    skos:definition "A time period with the following approximated bounds: older bound -33.9 Ma, younger bound -28.1 Ma" ;
    skos:inScheme cs: ;
    skos:prefLabel "Rupelian"@en ;
    prov:wasDerivedFrom ts:gts2020 ;
    sdo:color
        "0/15/35/0"^^:CMYK ,
        "254/217/154"^^:RGB ,
        "#FED99A"^^:RGBHex ;
.

:Sakmarian
    a skos:Concept ;
    rdfs:isDefinedBy ts:gts2020 ;
    skos:altLabel
        "Сакмар"@bg ,
        "Sakmar"@cs ,
        "Sakmarien"@da ,
        "Sakmarium"@de ,
        "Sakmariense"@es ,
        "Sakmaria"@et ,
        "Sakmar"@fi ,
        "Sakmarien"@fr ,
        "szakmarai"@hu ,
        "sakmariano"@it ,
        "サクマリアン期"@ja ,
        "Sakmaris"@lt ,
        "Sakmariën"@nl ,
        "Samarkium"@no ,
        "Sakmar"@pl ,
        "Sakmariano"@pt ,
        "sakmar"@sk ,
        "sakmarij"@sl ,
        "sakmar"@sv ,
        "萨克马尔期"@zh ;
    skos:broader :Cisuralian ;
    skos:definition "A time period with the following approximated bounds: older bound -295.0 +|-0.18 Ma, younger bound -290.1 +|-0.26 Ma" ;
    skos:inScheme cs: ;
    skos:prefLabel "Sakmarian"@en ;
    prov:wasDerivedFrom ts:gts2020 ;
    sdo:color
        "10/55/50/0"^^:CMYK ,
        "227/111/92"^^:RGB ,
        "#E36F5C"^^:RGBHex ;
.

:Sandbian
    a skos:Concept ;
    rdfs:isDefinedBy ts:gts2020 ;
    skos:altLabel
        "Сандб"@bg ,
        "Sandby"@cs ,
        "Sandbien"@da ,
        "Sandbium"@de ,
        "Sandbiense"@es ,
        "Sandbi"@et ,
        "Sandb"@fi ,
        "Sandbien"@fr ,
        "sandbi"@hu ,
        "sandbiano"@it ,
        "サンドビアン期"@ja ,
        "Sandbis"@lt ,
        "Sandbiën"@nl ,
        "Sandbyium"@no ,
        "Sandb"@pl ,
        "Sandbiano"@pt ,
        "sandb"@sk ,
        "sandbij"@sl ,
        "sandby"@sv ,
        "桑比期"@zh ;
    skos:broader :UpperOrdovician ;
    skos:definition "A time period with the following approximated bounds: older bound -458.4 +|-0.9 Ma, younger bound -453.0 +|-0.7 Ma" ;
    skos:inScheme cs: ;
    skos:prefLabel "Sandbian"@en ;
    prov:wasDerivedFrom ts:gts2020 ;
    sdo:color
        "45/0/40/0"^^:CMYK ,
        "140/208/148"^^:RGB ,
        "#8CD094"^^:RGBHex ;
.

:Santonian
    a skos:Concept ;
    rdfs:isDefinedBy ts:gts2020 ;
    skos:altLabel
        "Сантон"@bg ,
        "Santon"@cs ,
        "Santonien"@da ,
        "Santonium"@de ,
        "Santoniense"@es ,
        "Santoni"@et ,
        "Santon"@fi ,
        "Santonien"@fr ,
        "santoni"@hu ,
        "santoniano"@it ,
        "サントニアン期"@ja ,
        "Santonis"@lt ,
        "Santoniën"@nl ,
        "Santonium"@no ,
        "Santon"@pl ,
        "Santoniano"@pt ,
        "santón"@sk ,
        "santonij"@sl ,
        "santon"@sv ,
        "桑托期"@zh ;
    skos:broader :UpperCretaceous ;
    skos:definition "A time period with the following approximated bounds: older bound -86.3 +|-0.5 Ma, younger bound -83.6 +|-0.2 Ma" ;
    skos:inScheme cs: ;
    skos:prefLabel "Santonian"@en ;
    prov:wasDerivedFrom ts:gts2020 ;
    sdo:color
        "15/0/55/0"^^:CMYK ,
        "217/239/116"^^:RGB ,
        "#D9EF74"^^:RGBHex ;
.

:Selandian
    a skos:Concept ;
    rdfs:isDefinedBy ts:gts2020 ;
    skos:altLabel
        "Селанд"@bg ,
        "Seland"@cs ,
        "Selandien"@da ,
        "Selandium"@de ,
        "Selandiense"@es ,
        "Selandi"@et ,
        "Seland"@fi ,
        "Sélandien"@fr ,
        "selandi"@hu ,
        "selandiano"@it ,
        "セランディアン期"@ja ,
        "Selandis"@lt ,
        "Selandiën"@nl ,
        "Selandium"@no ,
        "Zeland"@pl ,
        "Selandiano"@pt ,
        "seland"@sk ,
        "selandij"@sl ,
        "seland"@sv ,
        "塞兰特期"@zh ;
    skos:broader :Paleocene ;
    skos:definition "A time period with the following approximated bounds: older bound -61.6 Ma, younger bound -59.2 Ma" ;
    skos:inScheme cs: ;
    skos:prefLabel "Selandian"@en ;
    prov:wasDerivedFrom ts:gts2020 ;
    sdo:color
        "0/25/55/0"^^:CMYK ,
        "254/191/101"^^:RGB ,
        "#FEBF65"^^:RGBHex ;
.

:Serpukhovian
    a skos:Concept ;
    rdfs:isDefinedBy ts:gts2020 ;
    skos:altLabel
        "Серпухов"@bg ,
        "Serpukhov"@cs ,
        "Serpukhovien"@da ,
        "Serpukhovium"@de ,
        "Serpulkhoviense"@es ,
        "Serpuhhovi"@et ,
        "Serpukhov"@fi ,
        "Serpukhovien"@fr ,
        "szerpuhovi"@hu ,
        "serpukhoviano"@it ,
        "サプコビアン期"@ja ,
        "Serpuchovis"@lt ,
        "Serpukhoviën"@nl ,
        "Serpukovium"@no ,
        "Serpuchow"@pl ,
        "Serpukoviano"@pt ,
        "serpuchov"@sk ,
        "serpukhovij"@sl ,
        "serpukhov"@sv ,
        "谢尔普霍夫期"@zh ;
    skos:broader :UpperMississippian ;
    skos:definition "A time period with the following approximated bounds: older bound -330.9 +|-0.2 Ma, younger bound -323.2 +|-0.4 Ma" ;
    skos:inScheme cs: ;
    skos:prefLabel "Serpukhovian"@en ;
    prov:wasDerivedFrom ts:gts2020 ;
    sdo:color
        "25/15/55/0"^^:CMYK ,
        "191/194/107"^^:RGB ,
        "#BFC26B"^^:RGBHex ;
.

:Serravallian
    a skos:Concept ;
    rdfs:isDefinedBy ts:gts2020 ;
    skos:altLabel
        "Саравал"@bg ,
        "Serraval"@cs ,
        "Serravallien"@da ,
        "Serravallium"@de ,
        "Serravalliense"@es ,
        "Serravalli"@et ,
        "Serravall"@fi ,
        "Serravallien"@fr ,
        "serravallei"@hu ,
        "serravaliano"@it ,
        "サーラバリアン期"@ja ,
        "Seravalis"@lt ,
        "Serravalliën - Langeveld"@nl ,
        "Servallium"@no ,
        "Serrawal"@pl ,
        "Serravaliano"@pt ,
        "serravall"@sk ,
        "serravallij"@sl ,
        "serravall"@sv ,
        "塞拉瓦尔期"@zh ;
    skos:broader :Miocene ;
    skos:definition "A time period with the following approximated bounds: older bound -13.82 Ma, younger bound -11.63 Ma" ;
    skos:inScheme cs: ;
    skos:prefLabel "Serravallian"@en ;
    prov:wasDerivedFrom ts:gts2020 ;
    sdo:color
        "0/0/65/0"^^:CMYK ,
        "255/255/89"^^:RGB ,
        "#FFFF59"^^:RGBHex ;
.

:Sheinwoodian
    a skos:Concept ;
    rdfs:isDefinedBy ts:gts2020 ;
    skos:altLabel
        "Шейнуд"@bg ,
        "Sheinwood"@cs ,
        "Sheinwoodien"@da ,
        "Sheinwoodium"@de ,
        "Sheinwoodiense"@es ,
        "Sheinwoodi"@et ,
        "Sheinwood"@fi ,
        "Sheinwoodien"@fr ,
        "sheinwoodi"@hu ,
        "sheinwoodiano"@it ,
        "シェインウッディアン期"@ja ,
        "Šeinvudis"@lt ,
        "Sheinwoodiën"@nl ,
        "Sheinwood"@no ,
        "Sheinwood"@pl ,
        "Sheinwoodiano"@pt ,
        "sheinwood"@sk ,
        "sheinwodij"@sl ,
        "sheinwood"@sv ,
        "申伍德期"@zh ;
    skos:broader :Wenlock ;
    skos:definition "A time period with the following approximated bounds: older bound -433.4 +|-0.8 Ma, younger bound -430.5 +|-0.7 Ma" ;
    skos:inScheme cs: ;
    skos:prefLabel "Sheinwoodian"@en ;
    prov:wasDerivedFrom ts:gts2020 ;
    sdo:color
        "25/0/20/0"^^:CMYK ,
        "191/230/195"^^:RGB ,
        "#BFE6C3"^^:RGBHex ;
.

:Siderian
    a skos:Concept ;
    rdfs:isDefinedBy ts:gts2020 ;
    skos:altLabel
        "Сидер"@bg ,
        "Sider"@cs ,
        "Siderien"@da ,
        "Siderium"@de ,
        "Sideriense"@es ,
        "Sider"@et ,
        "Sider"@fi ,
        "Sidérien"@fr ,
        "sideri"@hu ,
        "sideriano"@it ,
        "シデリアン紀"@ja ,
        "Sideris"@lt ,
        "Sideriën"@nl ,
        "Siderium"@no ,
        "Sider"@pl ,
        "Sideriano"@pt ,
        "siderium"@sk ,
        "siderij"@sl ,
        "siderium"@sv ,
        "成铁纪"@zh ;
    skos:broader :Paleoproterozoic ;
    skos:definition "A time period with the following approximated bounds: older bound -2500 Ma, younger bound -2300 Ma" ;
    skos:inScheme cs: ;
    skos:prefLabel "Siderian"@en ;
    prov:wasDerivedFrom ts:gts2020 ;
    sdo:color
        "0/70/25/0"^^:CMYK ,
        "247/79/124"^^:RGB ,
        "#F74F7C"^^:RGBHex ;
.

:Sinemurian
    a skos:Concept ;
    rdfs:isDefinedBy ts:gts2020 ;
    skos:altLabel
        "Синемур"@bg ,
        "Sinemur"@cs ,
        "Sinemurien"@da ,
        "Sinémurium"@de ,
        "Sinemuriense"@es ,
        "Sinemuri"@et ,
        "Sinemur"@fi ,
        "Sinémurien"@fr ,
        "sinemuri"@hu ,
        "sinemuriano"@it ,
        "シネムール期"@ja ,
        "Sinemiūris"@lt ,
        "Sinemuriën"@nl ,
        "Sinemur"@no ,
        "Synemur"@pl ,
        "Sinemuriano"@pt ,
        "sinemúr"@sk ,
        "sinemurij"@sl ,
        "sinemur"@sv ,
        "辛涅穆尔期"@zh ;
    skos:broader :LowerJurassic ;
    skos:definition "A time period with the following approximated bounds: older bound -199.3 +|-0.3 Ma, younger bound -190.8 +|-1.0 Ma" ;
    skos:inScheme cs: ;
    skos:prefLabel "Sinemurian"@en ;
    prov:wasDerivedFrom ts:gts2020 ;
    sdo:color
        "60/5/0/0"^^:CMYK ,
        "103/188/216"^^:RGB ,
        "#67BCD8"^^:RGBHex ;
.

:Statherian
    a skos:Concept ;
    rdfs:isDefinedBy ts:gts2020 ;
    skos:altLabel
        "Статер"@bg ,
        "Stather"@cs ,
        "Statherien"@da ,
        "Statherium"@de ,
        "Statheriense"@es ,
        "Stather"@et ,
        "Stather"@fi ,
        "Stathérien"@fr ,
        "statheri"@hu ,
        "statheriano"@it ,
        "スタテリアン紀"@ja ,
        "Stateris"@lt ,
        "Statheriën"@nl ,
        "Staterium"@no ,
        "Stater"@pl ,
        "Stateriano"@pt ,
        "staterium"@sk ,
        "statherij"@sl ,
        "staterium"@sv ,
        "固结纪"@zh ;
    skos:broader :Paleoproterozoic ;
    skos:definition "A time period with the following approximated bounds: older bound -1800 Ma, younger bound -1600 Ma" ;
    skos:inScheme cs: ;
    skos:prefLabel "Statherian"@en ;
    prov:wasDerivedFrom ts:gts2020 ;
    sdo:color
        "0/55/10/0"^^:CMYK ,
        "248/117/167"^^:RGB ,
        "#F875A7"^^:RGBHex ;
.

:Stenian
    a skos:Concept ;
    rdfs:isDefinedBy ts:gts2020 ;
    skos:altLabel
        "Стен"@bg ,
        "Sten"@cs ,
        "Stenien"@da ,
        "Stenium"@de ,
        "Esteniense"@es ,
        "Sten"@et ,
        "Sten"@fi ,
        "Sténien"@fr ,
        "steni"@hu ,
        "steniano"@it ,
        "ステニアン紀"@ja ,
        "Stenis"@lt ,
        "Steniën"@nl ,
        "Stenium"@no ,
        "Sten"@pl ,
        "Steniano"@pt ,
        "stenium"@sk ,
        "stenij"@sl ,
        "stenium"@sv ,
        "狭带纪"@zh ;
    skos:broader :Mesoproterozoic ;
    skos:definition "A time period with the following approximated bounds: older bound -1200 Ma, younger bound -1000 Ma" ;
    skos:inScheme cs: ;
    skos:prefLabel "Stenian"@en ;
    prov:wasDerivedFrom ts:gts2020 ;
    sdo:color
        "0/15/35/0"^^:CMYK ,
        "254/217/154"^^:RGB ,
        "#FED99A"^^:RGBHex ;
.

:Telychian
    a skos:Concept ;
    rdfs:isDefinedBy ts:gts2020 ;
    skos:altLabel
        "Телич"@bg ,
        "Telych"@cs ,
        "Telychien"@da ,
        "Telychium"@de ,
        "Telychiense"@es ,
        "Telychi"@et ,
        "Telych"@fi ,
        "Télychien"@fr ,
        "telychi"@hu ,
        "telychiano"@it ,
        "テリチアン期"@ja ,
        "TelyĿis"@lt ,
        "Telychiën"@nl ,
        "Telychium"@no ,
        "Telych"@pl ,
        "Telychiano"@pt ,
        "telych"@sk ,
        "telychij"@sl ,
        "telych"@sv ,
        "特列奇期"@zh ;
    skos:broader :Llandovery ;
    skos:definition "A time period with the following approximated bounds: older bound -438.5 +|-1.1 Ma, younger bound -433.4 +|-0.8 Ma" ;
    skos:inScheme cs: ;
    skos:prefLabel "Telychian"@en ;
    prov:wasDerivedFrom ts:gts2020 ;
    sdo:color
        "25/0/15/0"^^:CMYK ,
        "191/230/207"^^:RGB ,
        "#BFE6CF"^^:RGBHex ;
.

:Thanetian
    a skos:Concept ;
    rdfs:isDefinedBy ts:gts2020 ;
    skos:altLabel
        "Танет"@bg ,
        "Thanet"@cs ,
        "Thanetien"@da ,
        "Thanetium"@de ,
        "Thanetiense"@es ,
        "Thaneti"@et ,
        "Thanet"@fi ,
        "Thanétien"@fr ,
        "thaneti"@hu ,
        "thanetiano"@it ,
        "サネティアン期"@ja ,
        "Tanetis"@lt ,
        "Thanetiën"@nl ,
        "Thanetium"@no ,
        "Tanet"@pl ,
        "Tanetiano"@pt ,
        "tanet"@sk ,
        "thanetij"@sl ,
        "thanet"@sv ,
        "塔内提期"@zh ;
    skos:broader :Paleocene ;
    skos:definition "A time period with the following approximated bounds: older bound -59.2 Ma, younger bound -56 Ma" ;
    skos:inScheme cs: ;
    skos:prefLabel "Thanetian"@en ;
    prov:wasDerivedFrom ts:gts2020 ;
    sdo:color
        "0/25/50/0"^^:CMYK ,
        "253/191/111"^^:RGB ,
        "#FDBF6F"^^:RGBHex ;
.

:Tithonian
    a skos:Concept ;
    rdfs:isDefinedBy ts:gts2020 ;
    skos:altLabel
        "Титон"@bg ,
        "Tithon"@cs ,
        "Tithonien"@da ,
        "Tithonium"@de ,
        "Tithoniense"@es ,
        "Tithoni"@et ,
        "Tithon"@fi ,
        "Tithonien"@fr ,
        "tithon"@hu ,
        "titoniano"@it ,
        "チトニアン期"@ja ,
        "Titonis"@lt ,
        "Tithoniën"@nl ,
        "Tithonium"@no ,
        "Tyton"@pl ,
        "Titoniano"@pt ,
        "titón"@sk ,
        "tithonij"@sl ,
        "tithon"@sv ,
        "提通期"@zh ;
    skos:broader :UpperJurassic ;
    skos:definition "A time period with the following approximated bounds: older bound -152.1 +|-0.9 Ma, younger bound -145.0 Ma" ;
    skos:inScheme cs: ;
    skos:prefLabel "Tithonian"@en ;
    prov:wasDerivedFrom ts:gts2020 ;
    sdo:color
        "15/0/0/0"^^:CMYK ,
        "217/241/247"^^:RGB ,
        "#D9F1F7"^^:RGBHex ;
.

:Toarcian
    a skos:Concept ;
    rdfs:isDefinedBy ts:gts2020 ;
    skos:altLabel
        "Тоар"@bg ,
        "Toark"@cs ,
        "Toarcien"@da ,
        "Toarcium"@de ,
        "Toarciense"@es ,
        "Toarci"@et ,
        "Toarc"@fi ,
        "Toarcien"@fr ,
        "toarci"@hu ,
        "toarciano"@it ,
        "トアルシアン期"@ja ,
        "Toaris"@lt ,
        "Toarciën"@nl ,
        "Toarc"@no ,
        "Toark"@pl ,
        "Toarciano"@pt ,
        "toark"@sk ,
        "toarcij"@sl ,
        "toarc"@sv ,
        "托阿尔期"@zh ;
    skos:broader :LowerJurassic ;
    skos:definition "A time period with the following approximated bounds: older bound -182.7 +|-0.7 Ma, younger bound -174.1 +|-1.0 Ma" ;
    skos:inScheme cs: ;
    skos:prefLabel "Toarcian"@en ;
    prov:wasDerivedFrom ts:gts2020 ;
    sdo:color
        "40/5/0/0"^^:CMYK ,
        "153/206/227"^^:RGB ,
        "#99CEE3"^^:RGBHex ;
.

:Tonian
    a skos:Concept ;
    rdfs:isDefinedBy ts:gts2020 ;
    skos:altLabel
        "Тон"@bg ,
        "Ton"@cs ,
        "Tonien"@da ,
        "Tonium"@de ,
        "Toniense"@es ,
        "Ton"@et ,
        "Ton"@fi ,
        "Tonien"@fr ,
        "toni"@hu ,
        "toniano"@it ,
        "トニアン紀"@ja ,
        "Tonis"@lt ,
        "Toniën"@nl ,
        "Tonium"@no ,
        "Ton"@pl ,
        "Toniano"@pt ,
        "tonium"@sk ,
        "tonij"@sl ,
        "tonium"@sv ,
        "拉伸纪"@zh ;
    skos:broader :Neoproterozoic ;
    skos:definition "A time period with the following approximated bounds: older bound -1000 Ma, younger bound -720 Ma" ;
    skos:inScheme cs: ;
    skos:prefLabel "Tonian"@en ;
    prov:wasDerivedFrom ts:gts2020 ;
    sdo:color
        "0/25/65/0"^^:CMYK ,
        "254/191/78"^^:RGB ,
        "#FEBF4E"^^:RGBHex ;
.

:Tortonian
    a skos:Concept ;
    rdfs:isDefinedBy ts:gts2020 ;
    skos:altLabel
        "Тортон"@bg ,
        "Torton"@cs ,
        "Tortonien"@da ,
        "Tortonium"@de ,
        "Tortoniense"@es ,
        "Tortoni"@et ,
        "Torton"@fi ,
        "Tortonien"@fr ,
        "tortonai"@hu ,
        "toroniano"@it ,
        "トートニアン期"@ja ,
        "Tortonis"@lt ,
        "Tortoniën - Linne"@nl ,
        "Tortonium"@no ,
        "Torton"@pl ,
        "Tortoniano"@pt ,
        "tortón"@sk ,
        "tortonij"@sl ,
        "torton"@sv ,
        "托尔顿期"@zh ;
    skos:broader :Miocene ;
    skos:definition "A time period with the following approximated bounds: older bound -11.63 Ma, younger bound -7.246 Ma" ;
    skos:inScheme cs: ;
    skos:prefLabel "Tortonian"@en ;
    prov:wasDerivedFrom ts:gts2020 ;
    sdo:color
        "0/0/60/0"^^:CMYK ,
        "255/255/102"^^:RGB ,
        "#FFFF66"^^:RGBHex ;
.

:Tournaisian
    a skos:Concept ;
    rdfs:isDefinedBy ts:gts2020 ;
    skos:altLabel
        "Турней"@bg ,
        "Tournai"@cs ,
        "Tournaisien"@da ,
        "Tournaisium"@de ,
        "Tournaisiense"@es ,
        "Tournais"@et ,
        "Tournais"@fi ,
        "Tournaisien"@fr ,
        "tournaisi"@hu ,
        "tournasiano"@it ,
        "トルネージアン期"@ja ,
        "Turnėjis"@lt ,
        "Tournaisiën"@nl ,
        "Tournasium"@no ,
        "Turnej"@pl ,
        "Turnaisiano"@pt ,
        "turnén"@sk ,
        "tournaisij"@sl ,
        "tournas"@sv ,
        "杜内期"@zh ;
    skos:broader :LowerMississippian ;
    skos:definition "A time period with the following approximated bounds: older bound -358.9 +|-0.4 Ma, younger bound -346.7 +|-0.4 Ma" ;
    skos:inScheme cs: ;
    skos:prefLabel "Tournaisian"@en ;
    prov:wasDerivedFrom ts:gts2020 ;
    sdo:color
        "45/15/55/0"^^:CMYK ,
        "140/176/108"^^:RGB ,
        "#8CB06C"^^:RGBHex ;
.

:Tremadocian
    a skos:Concept ;
    rdfs:isDefinedBy ts:gts2020 ;
    skos:altLabel
        "Тремадок"@bg ,
        "Tremadok"@cs ,
        "Tremadocien"@da ,
        "Tremadocium"@de ,
        "Tremadociense"@es ,
        "Tremadoci"@et ,
        "Tremadoc"@fi ,
        "Trémadocien"@fr ,
        "tremadoci"@hu ,
        "tremadociano"@it ,
        "トレマドキアン期"@ja ,
        "Tremadokis"@lt ,
        "Tremadociën"@nl ,
        "Tremadoc"@no ,
        "Tremadok"@pl ,
        "Tremadociano"@pt ,
        "tremadok"@sk ,
        "tremadocij"@sl ,
        "tremadoc"@sv ,
        "特马豆克期"@zh ;
    skos:broader :LowerOrdovician ;
    skos:definition "A time period with the following approximated bounds: older bound -485.4 +|-1.9 Ma, younger bound -477.7 +|-1.4 Ma" ;
    skos:inScheme cs: ;
    skos:prefLabel "Tremadocian"@en ;
    prov:wasDerivedFrom ts:gts2020 ;
    sdo:color
        "80/0/50/0"^^:CMYK ,
        "51/169/126"^^:RGB ,
        "#33A97E"^^:RGBHex ;
.

:Turonian
    a skos:Concept ;
    rdfs:isDefinedBy ts:gts2020 ;
    skos:altLabel
        "Турон"@bg ,
        "Turon"@cs ,
        "Turonien"@da ,
        "Turonium"@de ,
        "Turoniense"@es ,
        "Turoni"@et ,
        "Turon"@fi ,
        "Turonien"@fr ,
        "turon"@hu ,
        "turoniano"@it ,
        "チュロニアン期"@ja ,
        "Turonis"@lt ,
        "Tuironiën"@nl ,
        "Turonium"@no ,
        "Turon"@pl ,
        "Turoniano"@pt ,
        "turón"@sk ,
        "turonij"@sl ,
        "turon"@sv ,
        "土仑期"@zh ;
    skos:broader :UpperCretaceous ;
    skos:definition "A time period with the following approximated bounds: older bound -93.9 Ma, younger bound -89.8 +|-0.3 Ma" ;
    skos:inScheme cs: ;
    skos:prefLabel "Turonian"@en ;
    prov:wasDerivedFrom ts:gts2020 ;
    sdo:color
        "25/0/65/0"^^:CMYK ,
        "191/227/93"^^:RGB ,
        "#BFE35D"^^:RGBHex ;
.

:UpperPleistocene
    a skos:Concept ;
    rdfs:isDefinedBy ts:gts2020 ;
    skos:altLabel
        "Къѿен плейѿтоцен"@bg ,
        "Pozdní pleistocén"@cs ,
        "Sen Pleistocæn"@da ,
        "Spätes Pleistozän"@de ,
        "Hiline pleistotseen"@et ,
        "Myöhäis-Pleistoseeni"@fi ,
        "késő pleisztocén"@hu ,
        "後期更新世"@ja ,
        "Apatinis Pleistocenas"@lt ,
        "Laat Pleistoceen"@nl ,
        "Yngre pleistocen"@no ,
        "Późny Plejstocen"@pl ,
        "mladší pleistocén"@sk ,
        "pozni pleistocen"@sl ,
        "yngre pleistocen"@sv ,
        "晚更新世"@zh ;
    skos:broader :Pleistocene ;
    skos:definition "A time period with the following approximated bounds: older bound -0.126 Ma, younger bound -0.0117 Ma" ;
    skos:inScheme cs: ;
    skos:prefLabel "Late Pleistocene"@en ;
    prov:wasDerivedFrom ts:gts2020 ;
    sdo:color
        "0/5/15/0"^^:CMYK ,
        "255/242/211"^^:RGB ,
        "#FFF2D3"^^:RGBHex ;
.

:Valanginian
    a skos:Concept ;
    rdfs:isDefinedBy ts:gts2020 ;
    skos:altLabel
        "Валанжин"@bg ,
        "Valangin"@cs ,
        "Valanginien"@da ,
        "Valanginium"@de ,
        "Valanginiense"@es ,
        "Valangini"@et ,
        "Valangin"@fi ,
        "Valanginien"@fr ,
        "valangini"@hu ,
        "valanginiano"@it ,
        "バランギニアン期"@ja ,
        "Valendis"@lt ,
        "Vanlangiën"@nl ,
        "Valanginium"@no ,
        "Walanżyn"@pl ,
        "Valanginiano"@pt ,
        "valanžin"@sk ,
        "valanginij"@sl ,
        "valangin"@sv ,
        "凡兰吟期"@zh ;
    skos:broader :LowerCretaceous ;
    skos:definition "A time period with the following approximated bounds: older bound -139.8 Ma, younger bound -132.9 Ma" ;
    skos:inScheme cs: ;
    skos:prefLabel "Valanginian"@en ;
    prov:wasDerivedFrom ts:gts2020 ;
    sdo:color
        "40/0/60/0"^^:CMYK ,
        "153/211/106"^^:RGB ,
        "#99D36A"^^:RGBHex ;
.

:Visean
    a skos:Concept ;
    rdfs:isDefinedBy ts:gts2020 ;
    skos:altLabel
        "Визей"@bg ,
        "Visé"@cs ,
        "Viseen"@da ,
        "Viseum"@de ,
        "Viseense"@es ,
        "Vise"@et ,
        "Vis"@fi ,
        "Viséen"@fr ,
        "viséi"@hu ,
        "viseano"@it ,
        "ビゼアン期"@ja ,
        "Vizejis"@lt ,
        "Vise-iën"@nl ,
        "Viseium"@no ,
        "Wizen"@pl ,
        "Viseano"@pt ,
        "visén"@sk ,
        "viseij"@sl ,
        "vis"@sv ,
        "韦宪期"@zh ;
    skos:broader :MiddleMississippian ;
    skos:definition "A time period with the following approximated bounds: older bound -346.7 +|-0.4 Ma, younger bound -330.9 +|-0.2 Ma" ;
    skos:inScheme cs: ;
    skos:prefLabel "Visean"@en ;
    prov:wasDerivedFrom ts:gts2020 ;
    sdo:color
        "35/15/55/0"^^:CMYK ,
        "166/185/108"^^:RGB ,
        "#A6B96C"^^:RGBHex ;
.

:Wordian
    a skos:Concept ;
    rdfs:isDefinedBy ts:gts2020 ;
    skos:altLabel
        "Уорд"@bg ,
        "Word"@cs ,
        "Wordien"@da ,
        "Wordium"@de ,
        "Wordiense"@es ,
        "Wordi"@et ,
        "Word"@fi ,
        "Wordien"@fr ,
        "wordi"@hu ,
        "wordiano"@it ,
        "ワーディアン期"@ja ,
        "Vordis"@lt ,
        "Wordiën"@nl ,
        "Wordium"@no ,
        "Word"@pl ,
        "Wordiano"@pt ,
        "word"@sk ,
        "wordij"@sl ,
        "word"@sv ,
        "沃德期"@zh ;
    skos:broader :Guadalupian ;
    skos:definition "A time period with the following approximated bounds: older bound -268.8 +|-0.5 Ma, younger bound -265.1 +|-0.4 Ma" ;
    skos:inScheme cs: ;
    skos:prefLabel "Wordian"@en ;
    prov:wasDerivedFrom ts:gts2020 ;
    sdo:color
        "0/45/40/0"^^:CMYK ,
        "251/141/118"^^:RGB ,
        "#FB8D76"^^:RGBHex ;
.

:Wuchiapingian
    a skos:Concept ;
    rdfs:isDefinedBy ts:gts2020 ;
    skos:altLabel
        "Вучиапинг"@bg ,
        "Wuchiaping"@cs ,
        "Wuchiapingien"@da ,
        "Wuchiapingium"@de ,
        "Wuchiapingiense"@es ,
        "Wuchiapingi"@et ,
        "Wuchiaiping"@fi ,
        "Wuchiapingien"@fr ,
        "wuchiapingi"@hu ,
        "wuchiapingiano"@it ,
        "ウキアピンギアン期"@ja ,
        "VuĿiapingis"@lt ,
        "Wuchiapingiën"@nl ,
        "Wuchianpingum"@no ,
        "Wuchiaping"@pl ,
        "Wuchiapingiano"@pt ,
        "wuťiapching"@sk ,
        "wuchiapingij"@sl ,
        "wuchiaping"@sv ,
        "吴家坪期"@zh ;
    skos:broader :Lopingian ;
    skos:definition "A time period with the following approximated bounds: older bound -259.1 +|-0.5 Ma, younger bound -254.14 +|-0.07 Ma" ;
    skos:inScheme cs: ;
    skos:prefLabel "Wuchiapingian"@en ;
    prov:wasDerivedFrom ts:gts2020 ;
    sdo:color
        "0/30/25/0"^^:CMYK ,
        "252/180/162"^^:RGB ,
        "#FCB4A2"^^:RGBHex ;
.

:Wuliuan
    a skos:Concept ;
    rdfs:isDefinedBy ts:gts2020 ;
    skos:broader :Miaolingian ;
    skos:definition "A time period with the following approximated bounds: older bound -509 Ma, younger bound -504.5 Ma" ;
    skos:inScheme cs: ;
    skos:prefLabel "Wuliuan"@en ;
    prov:wasDerivedFrom ts:gts2020 ;
    sdo:color
        "30/5/40/0"^^:CMYK ,
        "179/212/146"^^:RGB ,
        "#B3D492"^^:RGBHex ;
.

:Ypresian
    a skos:Concept ;
    rdfs:isDefinedBy ts:gts2020 ;
    skos:altLabel
        "Ипреѿ"@bg ,
        "Ypres"@cs ,
        "Ypresien"@da ,
        "Ypersium"@de ,
        "Ypresiense"@es ,
        "Ypresi"@et ,
        "Ypres"@fi ,
        "Yprésien"@fr ,
        "ypresi"@hu ,
        "ypresiano"@it ,
        "イプレシアン期"@ja ,
        "Ypris"@lt ,
        "Ypresiën"@nl ,
        "Ypres"@no ,
        "Ipr"@pl ,
        "Ipresiano"@pt ,
        "ypres"@sk ,
        "ypresij"@sl ,
        "ypres"@sv ,
        "伊普雷斯期"@zh ;
    skos:broader :Eocene ;
    skos:definition "A time period with the following approximated bounds: older bound -56 Ma, younger bound -47.8 Ma" ;
    skos:inScheme cs: ;
    skos:prefLabel "Ypresian"@en ;
    prov:wasDerivedFrom ts:gts2020 ;
    sdo:color
        "0/35/45/0"^^:CMYK ,
        "252/167/115"^^:RGB ,
        "#FCA773"^^:RGBHex ;
.

:Zanclean
    a skos:Concept ;
    rdfs:isDefinedBy ts:gts2020 ;
    skos:altLabel
        "Занклѿки"@bg ,
        "Zancl"@cs ,
        "Zanclien"@da ,
        "Zanclium"@de ,
        "Zanclayense"@es ,
        "Zancle"@et ,
        "Zancl"@fi ,
        "Zancléen"@fr ,
        "zanclai"@hu ,
        "zancleano"@it ,
        "ザンクレアン期"@ja ,
        "Zanklis"@lt ,
        "Brunssummiën"@nl ,
        "Zancleium"@no ,
        "Zankl"@pl ,
        "Zancleano"@pt ,
        "zanclean"@sk ,
        "zanclij"@sl ,
        "zancl"@sv ,
        "赞克勒期"@zh ;
    skos:broader :Pliocene ;
    skos:definition "A time period with the following approximated bounds: older bound -5.333 Ma, younger bound -3.6 Ma" ;
    skos:inScheme cs: ;
    skos:prefLabel "Zanclean"@en ;
    prov:wasDerivedFrom ts:gts2020 ;
    sdo:color
        "0/0/30/0"^^:CMYK ,
        "255/255/179"^^:RGB ,
        "#FFFFB3"^^:RGBHex ;
.

:LowerMississippian
    a skos:Concept ;
    rdfs:isDefinedBy ts:gts2020 ;
    skos:altLabel
        "前期ミシシッピアン紀"@ja ,
        "早密西西比世"@zh ;
    skos:broader :Mississippian ;
    skos:definition "A time period with the following approximated bounds: older bound -358.9 +|-0.4 Ma, younger bound -346.7 +|-0.4 Ma" ;
    skos:inScheme cs: ;
    skos:narrower :Tournaisian ;
    skos:prefLabel "Early Mississippian"@en ;
    prov:wasDerivedFrom ts:gts2020 ;
    sdo:color
        "45/15/55/0"^^:CMYK ,
        "128/171/108"^^:RGB ,
        "#80AB6C"^^:RGBHex ;
.

:LowerPennsylvanian
    a skos:Concept ;
    rdfs:isDefinedBy ts:gts2020 ;
    skos:altLabel
        "前期ペンシルバニア紀"@ja ,
        "早宾夕法尼亚世"@zh ;
    skos:broader :Pennsylvanian ;
    skos:definition "A time period with the following approximated bounds: older bound -323.2 +|-0.4 Ma, younger bound -315.2 +|-0.2 Ma" ;
    skos:inScheme cs: ;
    skos:narrower :Bashkirian ;
    skos:prefLabel "Early Pennsylvanian"@en ;
    prov:wasDerivedFrom ts:gts2020 ;
    sdo:color
        "45/10/20/0"^^:CMYK ,
        "140/190/180"^^:RGB ,
        "#8CBEB4"^^:RGBHex ;
.

:MiddleMississippian
    a skos:Concept ;
    rdfs:isDefinedBy ts:gts2020 ;
    skos:altLabel
        "中期ミシシッピアン紀"@ja ,
        "中密西西比世"@zh ;
    skos:broader :Mississippian ;
    skos:definition "A time period with the following approximated bounds: older bound -346.7 +|-0.4 Ma, younger bound -330.9 +|-0.2 Ma" ;
    skos:inScheme cs: ;
    skos:narrower :Visean ;
    skos:prefLabel "Middle Mississippian"@en ;
    prov:wasDerivedFrom ts:gts2020 ;
    sdo:color
        "35/15/55/0"^^:CMYK ,
        "153/180/108"^^:RGB ,
        "#99B46C"^^:RGBHex ;
.

:MiddlePennsylvanian
    a skos:Concept ;
    rdfs:isDefinedBy ts:gts2020 ;
    skos:altLabel
        "中期ペンシルバニア紀"@ja ,
        "中宾夕法尼亚世"@zh ;
    skos:broader :Pennsylvanian ;
    skos:definition "A time period with the following approximated bounds: older bound -315.2 +|-0.2 Ma, younger bound -307 +|-0.1 Ma" ;
    skos:inScheme cs: ;
    skos:narrower :Moscovian ;
    skos:prefLabel "Middle Pennsylvanian"@en ;
    prov:wasDerivedFrom ts:gts2020 ;
    sdo:color
        "30/10/20/0"^^:CMYK ,
        "166/199/183"^^:RGB ,
        "#A6C7B7"^^:RGBHex ;
.

:UpperMississippian
    a skos:Concept ;
    rdfs:isDefinedBy ts:gts2020 ;
    skos:altLabel
        "後期ミシシッピアン紀"@ja ,
        "晚密西西比世"@zh ;
    skos:broader :Mississippian ;
    skos:definition "A time period with the following approximated bounds: older bound -330.9 +|-0.2 Ma, younger bound -298.9 +|-0.15 Ma" ;
    skos:inScheme cs: ;
    skos:narrower :Serpukhovian ;
    skos:prefLabel "Late Mississippian"@en ;
    prov:wasDerivedFrom ts:gts2020 ;
    sdo:color
        "25/15/55/0"^^:CMYK ,
        "179/190/108"^^:RGB ,
        "#B3BE6C"^^:RGBHex ;
.

<https://linked.data.gov.au/org/ics>
    a sdo:Organization ;
    sdo:name "International Commission on Stratigraphy" ;
    sdo:url "https://stratigraphy.org"^^xsd:anyURI ;
.

:CambrianSeries2
    a skos:Concept ;
    rdfs:isDefinedBy ts:gts2020 ;
    skos:altLabel
        "Камбрий - 2 ѿериѿ"@bg ,
        "Kambrium-Oddělení 2"@cs ,
        "Kambrium-Serie 2"@da ,
        "Kambrium-Serie 2"@de ,
        "Cámbrico-Serie 2"@es ,
        "Kambrium, Ladestik 2"@et ,
        "Kambri-sarja 2"@fi ,
        "Cambrien-Séries 2"@fr ,
        "kambrium 2. sorozat"@hu ,
        "cambriano - serie 2"@it ,
        "第2世"@ja ,
        "Kambras-Serija 2"@lt ,
        "Cambrium, Zone 2"@nl ,
        "Kambrium -serie 2"@no ,
        "Kambr-Oddział 2"@pl ,
        "Câmbrico-Série 2"@pt ,
        "kambrium - séria 2"@sk ,
        "kambrij-serija 2"@sl ,
        "kambrium serie 2"@sv ,
        "第二世"@zh ;
    skos:broader :Cambrian ;
    skos:definition "A time period with the following approximated bounds: older bound -521 Ma, younger bound -509 Ma" ;
    skos:inScheme cs: ;
    skos:narrower
        :CambrianStage3 ,
        :CambrianStage4 ;
    skos:prefLabel "Cambrian Series 2"@en ;
    prov:wasDerivedFrom ts:gts2020 ;
    sdo:color
        "40/10/50/0"^^:CMYK ,
        "153/192/120"^^:RGB ,
        "#99C078"^^:RGBHex ;
.

:Carboniferous
    a skos:Concept ;
    rdfs:isDefinedBy ts:gts2020 ;
    skos:altLabel
        "Карбон"@bg ,
        "Karbon"@cs ,
        "Karbon"@da ,
        "Karbon"@de ,
        "Carbonífero"@es ,
        "Karbon"@et ,
        "Kivihiili"@fi ,
        "Carbonifère"@fr ,
        "karbon"@hu ,
        "carbonifero"@it ,
        "石炭紀"@ja ,
        "Karbonas"@lt ,
        "Carboon"@nl ,
        "Karbon"@no ,
        "Karbon"@pl ,
        "Carbónico"@pt ,
        "karbón"@sk ,
        "karbon"@sl ,
        "karbon"@sv ,
        "石炭纪"@zh ;
    skos:broader :Paleozoic ;
    skos:definition "A time period with the following approximated bounds: older bound -358.9 +|-0.4 Ma, younger bound -298.9 +|-0.15 Ma" ;
    skos:inScheme cs: ;
    skos:narrower
        :Mississippian ,
        :Pennsylvanian ;
    skos:prefLabel "Carboniferous"@en ;
    prov:wasDerivedFrom ts:gts2020 ;
    sdo:color
        "60/15/30/0"^^:CMYK ,
        "103/165/153"^^:RGB ,
        "#67A599"^^:RGBHex ;
.

:Cretaceous
    a skos:Concept ;
    rdfs:isDefinedBy ts:gts2020 ;
    skos:altLabel
        "Креда"@bg ,
        "Křída"@cs ,
        "Kridt"@da ,
        "Kreide"@de ,
        "Cretácico"@es ,
        "Kriit"@et ,
        "Liitu"@fi ,
        "Crétacé"@fr ,
        "kréta"@hu ,
        "cretacico"@it ,
        "白亜紀"@ja ,
        "Kreida"@lt ,
        "Krijt"@nl ,
        "Kritt"@no ,
        "Kreda"@pl ,
        "Cretácico"@pt ,
        "krieda"@sk ,
        "kreda"@sl ,
        "krita"@sv ,
        "白垩纪"@zh ;
    skos:broader :Mesozoic ;
    skos:definition "A time period with the following approximated bounds: older bound -145.0 Ma, younger bound -66.0 Ma" ;
    skos:inScheme cs: ;
    skos:narrower
        :LowerCretaceous ,
        :UpperCretaceous ;
    skos:prefLabel "Cretaceous"@en ;
    prov:wasDerivedFrom ts:gts2020 ;
    sdo:color
        "50/0/75/0"^^:CMYK ,
        "127/198/78"^^:RGB ,
        "#7FC64E"^^:RGBHex ;
.

:Lopingian
    a skos:Concept ;
    rdfs:isDefinedBy ts:gts2020 ;
    skos:altLabel
        "Лопинг"@bg ,
        "Loping"@cs ,
        "Lopingien"@da ,
        "Lopingium"@de ,
        "Lopingiense"@es ,
        "Loping"@et ,
        "Loping"@fi ,
        "Lopingien"@fr ,
        "lopingi"@hu ,
        "lopingiano"@it ,
        "ロピンギアン世"@ja ,
        "Lopingis"@lt ,
        "Lopingiën"@nl ,
        "Lopingium"@no ,
        "Loping"@pl ,
        "Lopingiano"@pt ,
        "loping"@sk ,
        "lopingij"@sl ,
        "loping"@sv ,
        "乐平世"@zh ;
    skos:broader :Permian ;
    skos:definition "A time period with the following approximated bounds: older bound -259.1 +|-0.5 Ma, younger bound -251.902 +|-0.024 Ma" ;
    skos:inScheme cs: ;
    skos:narrower
        :Changhsingian ,
        :Wuchiapingian ;
    skos:prefLabel "Lopingian"@en ;
    prov:wasDerivedFrom ts:gts2020 ;
    sdo:color
        "0/35/30/0"^^:CMYK ,
        "251/167/148"^^:RGB ,
        "#FBA794"^^:RGBHex ;
.

:LowerOrdovician
    a skos:Concept ;
    rdfs:isDefinedBy ts:gts2020 ;
    skos:altLabel
        "Ранен Ордовик"@bg ,
        "brzy ordovik"@cs ,
        "Tidlig Ordovicium"@da ,
        "Fühes Ordovizium"@de ,
        "Ordovícico temprano"@es ,
        "Vara-Ordoviitsium"@et ,
        "Varhais-Ordoviikki"@fi ,
        "Ordovicien précoce"@fr ,
        "kora-ordovícium"@hu ,
        "ordoviciano precoce"@it ,
        "オルドビス紀前期"@ja ,
        "Ankstyvasis Ordovikas"@lt ,
        "Vroeg Ordovicium"@nl ,
        "Tidlig ordovicium"@no ,
        "Wczesny Ordowik"@pl ,
        "Ordovícista adiantado"@pt ,
        "raný ordovik"@sk ,
        "zgodnji ordovicij"@sl ,
        "äldre ordovicium"@sv ,
        "早奥陶世"@zh ;
    skos:broader :Ordovician ;
    skos:definition "A time period with the following approximated bounds: older bound -485.4 +|-1.9 Ma, younger bound -470.0 +|-1.4 Ma" ;
    skos:inScheme cs: ;
    skos:narrower
        :Floian ,
        :Tremadocian ;
    skos:prefLabel "Early Ordovician"@en ;
    prov:wasDerivedFrom ts:gts2020 ;
    sdo:color
        "90/0/60/0"^^:CMYK ,
        "26/157/111"^^:RGB ,
        "#1A9D6F"^^:RGBHex ;
.

:LowerTriassic
    a skos:Concept ;
    rdfs:isDefinedBy ts:gts2020 ;
    skos:altLabel
        "Раннен Триаѿ"@bg ,
        "brzy trias"@cs ,
        "Tidlig Triassisk"@da ,
        "Frühe Trias (Buntsandstein)"@de ,
        "Triásico temprano"@es ,
        "Vara-Triias"@et ,
        "Varhais-Trias"@fi ,
        "Trias précoce"@fr ,
        "kora-triász"@hu ,
        "triassico precoce"@it ,
        "三畳紀前期"@ja ,
        "Ankstyvasis Triasas"@lt ,
        "Vroeg Trias"@nl ,
        "Tidlig trias"@no ,
        "Wczesny Trias"@pl ,
        "Triássico primitivo"@pt ,
        "raný trias"@sk ,
        "zgodnji trias"@sl ,
        "äldre trias"@sv ,
        "早三叠世"@zh ;
    skos:broader :Triassic ;
    skos:definition "A time period with the following approximated bounds: older bound -251.902 +|-0.024 Ma, younger bound -247.2 Ma" ;
    skos:inScheme cs: ;
    skos:narrower
        :Induan ,
        :Olenekian ;
    skos:prefLabel "Early Triassic"@en ;
    prov:wasDerivedFrom ts:gts2020 ;
    sdo:color
        "40/75/0/0"^^:CMYK ,
        "152/57/153"^^:RGB ,
        "#983999"^^:RGBHex ;
.

:Ludlow
    a skos:Concept ;
    rdfs:isDefinedBy ts:gts2020 ;
    skos:altLabel
        "Лудлоу"@bg ,
        "Ludlow"@cs ,
        "Ludlow"@da ,
        "Ludlow"@de ,
        "Ludlow"@es ,
        "Ludlow"@et ,
        "Ludlow"@fi ,
        "Ludlow"@fr ,
        "ludlowi"@hu ,
        "ludlow"@it ,
        "ルーロビアン世"@ja ,
        "Ludlovis"@lt ,
        "Ludlow"@nl ,
        "Ludlow"@no ,
        "Ludlow"@pl ,
        "Ludlow"@pt ,
        "ludlow"@sk ,
        "ludlowij"@sl ,
        "ludlow"@sv ,
        "卢德洛世"@zh ;
    skos:broader :Silurian ;
    skos:definition "A time period with the following approximated bounds: older bound -427.4 +|-0.5 Ma, younger bound -423 +|-2.3 Ma" ;
    skos:inScheme cs: ;
    skos:narrower
        :Gorstian ,
        :Ludfordian ;
    skos:prefLabel "Ludlow"@en ;
    prov:wasDerivedFrom ts:gts2020 ;
    sdo:color
        "25/0/15/0"^^:CMYK ,
        "191/230/207"^^:RGB ,
        "#BFE6CF"^^:RGBHex ;
.

:MiddleDevonian
    a skos:Concept ;
    rdfs:isDefinedBy ts:gts2020 ;
    skos:altLabel
        "Среден Девон"@bg ,
        "Střední devon"@cs ,
        "Mellem Devon"@da ,
        "Mitteldevon"@de ,
        "Devónico Medio"@es ,
        "Kesk-Devon"@et ,
        "Keski-Devoni"@fi ,
        "Dévonien moyen"@fr ,
        "középső-devon"@hu ,
        "devoniano medio"@it ,
        "中期デボン紀"@ja ,
        "Vidurinis Devonas"@lt ,
        "Midden Devoon"@nl ,
        "Midtre devon"@no ,
        "Środkowy Dewon"@pl ,
        "Devónico Médio"@pt ,
        "stredný devón"@sk ,
        "srednji devon"@sl ,
        "mellersta devon"@sv ,
        "中泥盆世"@zh ;
    skos:broader :Devonian ;
    skos:definition "A time period with the following approximated bounds: older bound -393.3 +|-1.2 Ma, younger bound -382.7 +|-1.6 Ma" ;
    skos:inScheme cs: ;
    skos:narrower
        :Eifelian ,
        :Givetian ;
    skos:prefLabel "Middle Devonian"@en ;
    prov:wasDerivedFrom ts:gts2020 ;
    sdo:color
        "5/20/55/0"^^:CMYK ,
        "241/200/104"^^:RGB ,
        "#F1C868"^^:RGBHex ;
.

:MiddleOrdovician
    a skos:Concept ;
    rdfs:isDefinedBy ts:gts2020 ;
    skos:altLabel
        "Среден Ордовик"@bg ,
        "Střední ordovik"@cs ,
        "Mellem Ordovicium"@da ,
        "Mittleres Ordovizium"@de ,
        "Ordovícico Medio"@es ,
        "Kesk-Ordoviitsium"@et ,
        "Keski-Ordoviikki"@fi ,
        "Ordovicien moyen"@fr ,
        "középső-ordovícium"@hu ,
        "ordoviciano medio"@it ,
        "中期オルドビス紀"@ja ,
        "Vidurinis Ordovikas"@lt ,
        "Midden Ordovicium"@nl ,
        "Midtre ordovicium"@no ,
        "Środkowy Ordowik"@pl ,
        "Ordovícico Médio"@pt ,
        "stredný ordovik"@sk ,
        "srednji ordovicij"@sl ,
        "mellersta ordovicium"@sv ,
        "中奥陶世"@zh ;
    skos:broader :Ordovician ;
    skos:definition "A time period with the following approximated bounds: older bound -470.0 +|-1.4 Ma, younger bound -458.4 +|-0.9 Ma" ;
    skos:inScheme cs: ;
    skos:narrower
        :Dapingian ,
        :Darriwilian ;
    skos:prefLabel "Middle Ordovician"@en ;
    prov:wasDerivedFrom ts:gts2020 ;
    sdo:color
        "70/0/50/0"^^:CMYK ,
        "77/180/126"^^:RGB ,
        "#4DB47E"^^:RGBHex ;
.

:MiddleTriassic
    a skos:Concept ;
    rdfs:isDefinedBy ts:gts2020 ;
    skos:altLabel
        "Среден Триаѿ"@bg ,
        "Střední trias"@cs ,
        "Mellem Triassisk"@da ,
        "Mittlere Trias"@de ,
        "Triásico Medio"@es ,
        "Kesk-Triias"@et ,
        "Keski-Trias"@fi ,
        "Trias moyen"@fr ,
        "középső-triász"@hu ,
        "triassico medio"@it ,
        "中期三畳紀"@ja ,
        "Vidurinis Triasas"@lt ,
        "Midden Trias"@nl ,
        "Midtre trias"@no ,
        "Środkowy Trias"@pl ,
        "Triásico Médio"@pt ,
        "stredný trias"@sk ,
        "srednji trias"@sl ,
        "mellersta trias"@sv ,
        "中三叠世"@zh ;
    skos:broader :Triassic ;
    skos:definition "A time period with the following approximated bounds: older bound -247.2 Ma, younger bound -237 Ma" ;
    skos:inScheme cs: ;
    skos:narrower
        :Anisian ,
        :Ladinian ;
    skos:prefLabel "Middle Triassic"@en ;
    prov:wasDerivedFrom ts:gts2020 ;
    sdo:color
        "30/55/0/0"^^:CMYK ,
        "177/104/177"^^:RGB ,
        "#B168B1"^^:RGBHex ;
.

:Neogene
    a skos:Concept ;
    rdfs:isDefinedBy ts:gts2020 ;
    skos:altLabel
        "пеоген"@bg ,
        "Neogén"@cs ,
        "Neogen"@da ,
        "Neogen"@de ,
        "Neógeno"@es ,
        "Neogeen"@et ,
        "Neogeeni"@fi ,
        "Néogène"@fr ,
        "neogén"@hu ,
        "neogene"@it ,
        "新第三紀"@ja ,
        "Neogenas"@lt ,
        "Neogeen"@nl ,
        "Neogen"@no ,
        "Neogen"@pl ,
        "Neogénico"@pt ,
        "neogén"@sk ,
        "neogen"@sl ,
        "neogen"@sv ,
        "晚第三纪"@zh ;
    skos:broader :Cenozoic ;
    skos:definition "A time period with the following approximated bounds: older bound -23.03 Ma, younger bound -2.58 Ma" ;
    skos:inScheme cs: ;
    skos:narrower
        :Miocene ,
        :Pliocene ;
    skos:prefLabel "Neogene"@en ;
    prov:wasDerivedFrom ts:gts2020 ;
    sdo:color
        "0/10/90/0"^^:CMYK ,
        "255/230/25"^^:RGB ,
        "#FFE619"^^:RGBHex ;
.

:Oligocene
    a skos:Concept ;
    rdfs:isDefinedBy ts:gts2020 ;
    skos:altLabel
        "Олигоцен"@bg ,
        "Oligocén"@cs ,
        "Oligocæn"@da ,
        "Oligozän"@de ,
        "Oligoceno"@es ,
        "Oligotseen"@et ,
        "Oligoseeni"@fi ,
        "Oligocène"@fr ,
        "oligocén"@hu ,
        "oligocene"@it ,
        "漸新世"@ja ,
        "Oligocenas"@lt ,
        "Oliogoceen"@nl ,
        "Oligocen"@no ,
        "Oligocen"@pl ,
        "Oligocénico"@pt ,
        "oligocén"@sk ,
        "oligocen"@sl ,
        "oligocen"@sv ,
        "渐新世"@zh ;
    skos:broader :Paleogene ;
    skos:definition "A time period with the following approximated bounds: older bound -33.9 Ma, younger bound -23.03 Ma" ;
    skos:inScheme cs: ;
    skos:narrower
        :Chattian ,
        :Rupelian ;
    skos:prefLabel "Oligocene"@en ;
    prov:wasDerivedFrom ts:gts2020 ;
    sdo:color
        "0/25/45/0"^^:CMYK ,
        "254/192/122"^^:RGB ,
        "#FEC07A"^^:RGBHex ;
.

:Pliocene
    a skos:Concept ;
    rdfs:isDefinedBy ts:gts2020 ;
    skos:altLabel
        "Плиоцен"@bg ,
        "Pliocén"@cs ,
        "Pliocæn"@da ,
        "Pliozän"@de ,
        "Ploceno"@es ,
        "Pliotseen"@et ,
        "Plioseeni"@fi ,
        "Pliocène"@fr ,
        "pliocén"@hu ,
        "pliocene"@it ,
        "鮮新世"@ja ,
        "Pliocenas"@lt ,
        "Plioceen"@nl ,
        "Pliocen"@no ,
        "Pliocen"@pl ,
        "Pliocénico"@pt ,
        "pliocén"@sk ,
        "pliocen"@sl ,
        "pliocen"@sv ,
        "上新世"@zh ;
    skos:broader :Neogene ;
    skos:definition "A time period with the following approximated bounds: older bound -5.333 Ma, younger bound -2.58 Ma" ;
    skos:inScheme cs: ;
    skos:narrower
        :Piacenzian ,
        :Zanclean ;
    skos:prefLabel "Pliocene"@en ;
    prov:wasDerivedFrom ts:gts2020 ;
    sdo:color
        "0/0/40/0"^^:CMYK ,
        "255/255/153"^^:RGB ,
        "#FFFF99"^^:RGBHex ;
.

:Quaternary
    a skos:Concept ;
    rdfs:isDefinedBy ts:gts2020 ;
    skos:altLabel
        "Кватернер"@bg ,
        "Kvartér"@cs ,
        "Kvartær"@da ,
        "Quartär"@de ,
        "Cuaternario"@es ,
        "Kvaternaar"@et ,
        "Kvartääri"@fi ,
        "Quaternaire"@fr ,
        "negyedidőszak"@hu ,
        "quaternario"@it ,
        "第四紀"@ja ,
        "Kvarteras"@lt ,
        "Kwartair"@nl ,
        "Kvartær"@no ,
        "Czwartorzęd"@pl ,
        "Quaternário"@pt ,
        "kvartér"@sk ,
        "kvartar"@sl ,
        "kvartär"@sv ,
        "第四纪"@zh ;
    skos:broader :Cenozoic ;
    skos:definition "A time period with the following approximated bounds: older bound -2.58 Ma, younger bound -0.0 Ma" ;
    skos:inScheme cs: ;
    skos:narrower
        :Holocene ,
        :Pleistocene ;
    skos:prefLabel "Quaternary"@en ;
    prov:wasDerivedFrom ts:gts2020 ;
    sdo:color
        "0/0/50/0"^^:CMYK ,
        "249/249/127"^^:RGB ,
        "#F9F97F"^^:RGBHex ;
.

:Terreneuvian
    a skos:Concept ;
    rdfs:isDefinedBy ts:gts2020 ;
    skos:altLabel
        "Теренеув"@bg ,
        "Terreneuv"@cs ,
        "Terreneuvien"@da ,
        "Terreneuvium"@de ,
        "Terreneuviense"@es ,
        "Terreneuvi"@et ,
        "Terreneuv"@fi ,
        "Terreneuvien"@fr ,
        "terreneuvi"@hu ,
        "terreneuviano"@it ,
        "テレニュービアン世"@ja ,
        "Tereniuvis"@lt ,
        "Terreneuviën"@nl ,
        "Terreneuvium"@no ,
        "Terenew"@pl ,
        "Terreneuviano"@pt ,
        "terreneuv"@sk ,
        "terreneuvij"@sl ,
        "terreneuv"@sv ,
        "纽芬兰世"@zh ;
    skos:broader :Cambrian ;
    skos:definition "A time period with the following approximated bounds: older bound -541.0 +|-1.0 Ma, younger bound -521 Ma" ;
    skos:inScheme cs: ;
    skos:narrower
        :CambrianStage2 ,
        :Fortunian ;
    skos:prefLabel "Terreneuvian"@en ;
    prov:wasDerivedFrom ts:gts2020 ;
    sdo:color
        "45/15/55/0"^^:CMYK ,
        "140/176/108"^^:RGB ,
        "#8CB06C"^^:RGBHex ;
.

:UpperDevonian
    a skos:Concept ;
    rdfs:isDefinedBy ts:gts2020 ;
    skos:altLabel
        "Къѿен Девон"@bg ,
        "Svrchní devon"@cs ,
        "Sen Devon"@da ,
        "Spätes Devon"@de ,
        "Hilis-Devon"@et ,
        "Myöhäis-Devoni"@fi ,
        "késő-devon"@hu ,
        "後期デボン紀"@ja ,
        "Vėlyvasis Devonas"@lt ,
        "Laat Devoon"@nl ,
        "Sen devon"@no ,
        "Późny Dewon"@pl ,
        "mladší devón"@sk ,
        "pozni devon"@sl ,
        "yngre devon"@sv ,
        "晚泥盆世"@zh ;
    skos:broader :Devonian ;
    skos:definition "A time period with the following approximated bounds: older bound -382.7 +|-1.6 Ma, younger bound -358.9 +|-0.4 Ma" ;
    skos:inScheme cs: ;
    skos:narrower
        :Famennian ,
        :Frasnian ;
    skos:prefLabel "Late Devonian"@en ;
    prov:wasDerivedFrom ts:gts2020 ;
    sdo:color
        "5/10/35/0"^^:CMYK ,
        "241/225/157"^^:RGB ,
        "#F1E19D"^^:RGBHex ;
.

:UpperPennsylvanian
    a skos:Concept ;
    rdfs:isDefinedBy ts:gts2020 ;
    skos:altLabel
        "Къѿен Пенѿилван"@bg ,
        "Pozdní pennsylván"@cs ,
        "Sen Pennsylvanien"@da ,
        "Spätes Pennsylvanium"@de ,
        "Hilis-Pennsylvania"@et ,
        "Myöhäis-Pennsylvania"@fi ,
        "késő-pennsylvaniai"@hu ,
        "後期ペンシルバニア紀"@ja ,
        "Vėlyvasis Pensilvanis"@lt ,
        "Laat Pennsylvaniën"@nl ,
        "Sen pennsylvanium"@no ,
        "Późny Pensylwan"@pl ,
        "mladší penssylván"@sk ,
        "pozni pennsylvanij"@sl ,
        "yngre pennsylvan"@sv ,
        "晚宾夕法尼亚世"@zh ;
    skos:broader :Pennsylvanian ;
    skos:definition "A time period with the following approximated bounds: older bound -307 +|-0.1 Ma, younger bound -298.9 +|-0.15 Ma" ;
    skos:inScheme cs: ;
    skos:narrower
        :Gzhelian ,
        :Kasimovian ;
    skos:prefLabel "Late Pennsylvanian"@en ;
    prov:wasDerivedFrom ts:gts2020 ;
    sdo:color
        "25/10/20/0"^^:CMYK ,
        "191/208/186"^^:RGB ,
        "#BFD0BA"^^:RGBHex ;
.

:Wenlock
    a skos:Concept ;
    rdfs:isDefinedBy ts:gts2020 ;
    skos:altLabel
        "Венлок"@bg ,
        "Wenlock"@cs ,
        "Wenlock"@da ,
        "Wenlock"@de ,
        "Wenlock"@es ,
        "Wenlock"@et ,
        "Wenlock"@fi ,
        "Wenlock"@fr ,
        "wenlocki"@hu ,
        "wenlockiano"@it ,
        "ウェンロッキアン世"@ja ,
        "Uenlokis"@lt ,
        "Wenlock"@nl ,
        "Welnlock"@no ,
        "Wenlok"@pl ,
        "Wenlock"@pt ,
        "wenlock"@sk ,
        "wenlockij"@sl ,
        "wenlock"@sv ,
        "温洛克世"@zh ;
    skos:broader :Silurian ;
    skos:definition "A time period with the following approximated bounds: older bound -433.4 +|-0.8 Ma, younger bound -427.4 +|-0.5 Ma" ;
    skos:inScheme cs: ;
    skos:narrower
        :Homerian ,
        :Sheinwoodian ;
    skos:prefLabel "Wenlock"@en ;
    prov:wasDerivedFrom ts:gts2020 ;
    sdo:color
        "30/0/20/0"^^:CMYK ,
        "179/225/194"^^:RGB ,
        "#B3E1C2"^^:RGBHex ;
.

:Cenozoic
    a skos:Concept ;
    rdfs:isDefinedBy ts:gts2020 ;
    skos:altLabel
        "пеозой"@bg ,
        "Kenozoikum"@cs ,
        "Kænozoisk"@da ,
        "Känozoikum"@de ,
        "Cainozoic"@en-GB ,
        "Cenozoic"@en-US ,
        "Cenozoico"@es ,
        "Kainosoikum"@et ,
        "Kenotsoikum"@fi ,
        "Cénozoïque"@fr ,
        "kainozoikum"@hu ,
        "cenozoico"@it ,
        "新生代"@ja ,
        "Cenozojus"@lt ,
        "Kaenozoïcum"@nl ,
        "Kenozoikum"@no ,
        "Kenozoik"@pl ,
        "Cenozóico"@pt ,
        "kenozoikum"@sk ,
        "kenozoik"@sl ,
        "kenozoikum"@sv ,
        "新生代"@zh ;
    skos:broader :Phanerozoic ;
    skos:definition "A time period with the following approximated bounds: older bound -66.0 Ma, younger bound -0.0 Ma" ;
    skos:inScheme cs: ;
    skos:narrower
        :Neogene ,
        :Paleogene ,
        :Quaternary ;
    skos:prefLabel "Cenozoic"@en ;
    prov:wasDerivedFrom ts:gts2020 ;
    sdo:color
        "40/0/5/0"^^:CMYK ,
        "242/249/29"^^:RGB ,
        "#F2F91D"^^:RGBHex ;
.

:Devonian
    a skos:Concept ;
    rdfs:isDefinedBy ts:gts2020 ;
    skos:altLabel
        "Девон"@bg ,
        "Devon"@cs ,
        "Devon"@da ,
        "Devon"@de ,
        "Devónico"@es ,
        "Devon"@et ,
        "Devoni"@fi ,
        "Dévonien"@fr ,
        "devon"@hu ,
        "devoniano"@it ,
        "デボン紀"@ja ,
        "Devonas"@lt ,
        "Devoon"@nl ,
        "Devon"@no ,
        "Dewon"@pl ,
        "Devónico"@pt ,
        "devón"@sk ,
        "devon"@sl ,
        "devon"@sv ,
        "泥盆纪"@zh ;
    skos:broader :Paleozoic ;
    skos:definition "A time period with the following approximated bounds: older bound -419.2 +|-3.2 Ma, younger bound -358.9 +|-0.4 Ma" ;
    skos:inScheme cs: ;
    skos:narrower
        :LowerDevonian ,
        :MiddleDevonian ,
        :UpperDevonian ;
    skos:prefLabel "Devonian"@en ;
    prov:wasDerivedFrom ts:gts2020 ;
    sdo:color
        "20/40/75/0"^^:CMYK ,
        "203/140/55"^^:RGB ,
        "#CB8C37"^^:RGBHex ;
.

:Furongian
    a skos:Concept ;
    rdfs:isDefinedBy ts:gts2020 ;
    skos:altLabel
        "Фуронг"@bg ,
        "Furong"@cs ,
        "Furongien"@da ,
        "Furongium"@de ,
        "Furogiense"@es ,
        "Furong"@et ,
        "Furong"@fi ,
        "Furongien"@fr ,
        "furongi"@hu ,
        "furongiano"@it ,
        "フロンギアン世"@ja ,
        "Furongis"@lt ,
        "Furongiën"@nl ,
        "Furongium"@no ,
        "Furong"@pl ,
        "Furongiano"@pt ,
        "furong"@sk ,
        "furongij"@sl ,
        "furong"@sv ,
        "芙蓉世"@zh ;
    skos:broader :Cambrian ;
    skos:definition "A time period with the following approximated bounds: older bound -497 Ma, younger bound -485.4 +|-1.9 Ma" ;
    skos:inScheme cs: ;
    skos:narrower
        :CambrianStage10 ,
        :Jiangshanian ,
        :Paibian ;
    skos:prefLabel "Furongian"@en ;
    prov:wasDerivedFrom ts:gts2020 ;
    sdo:color
        "30/0/40/0"^^:CMYK ,
        "179/224/149"^^:RGB ,
        "#B3E095"^^:RGBHex ;
.

:Guadalupian
    a skos:Concept ;
    rdfs:isDefinedBy ts:gts2020 ;
    skos:altLabel
        "Гуадалуп"@bg ,
        "Guadalup"@cs ,
        "Guadalupien"@da ,
        "Guadalupium"@de ,
        "Guadalupiense"@es ,
        "Guadalup"@et ,
        "Guadalup"@fi ,
        "Guadalupéen"@fr ,
        "guadalupei"@hu ,
        "guadalupiano"@it ,
        "ガダリューピアン世"@ja ,
        "Gvadalupis"@lt ,
        "Guadalupiën"@nl ,
        "Guadalupium"@no ,
        "Gwadelup"@pl ,
        "Guadalupiano"@pt ,
        "guadalup"@sk ,
        "guadalupij"@sl ,
        "guadalup"@sv ,
        "瓜德鲁普世"@zh ;
    skos:broader :Permian ;
    skos:definition "A time period with the following approximated bounds: older bound -272.95 +|-0.11 Ma, younger bound -259.1 +|-0.5 Ma" ;
    skos:inScheme cs: ;
    skos:narrower
        :Capitanian ,
        :Roadian ,
        :Wordian ;
    skos:prefLabel "Guadalupian"@en ;
    prov:wasDerivedFrom ts:gts2020 ;
    sdo:color
        "0/55/50/0"^^:CMYK ,
        "251/116/92"^^:RGB ,
        "#FB745C"^^:RGBHex ;
.

:Holocene
    a skos:Concept ;
    rdfs:isDefinedBy ts:gts2020 ;
    skos:altLabel
        "Холоцен"@bg ,
        "Holocén"@cs ,
        "Holocæn"@da ,
        "Holozän"@de ,
        "Holoceno"@es ,
        "Holotseen"@et ,
        "Holoseeni"@fi ,
        "Holocène"@fr ,
        "holocén"@hu ,
        "olocene"@it ,
        "完新世"@ja ,
        "Holocenas"@lt ,
        "Holoceen"@nl ,
        "Holocen"@no ,
        "Holocen"@pl ,
        "Holocénico"@pt ,
        "holocén"@sk ,
        "holocen"@sl ,
        "holocen"@sv ,
        "全新世"@zh ;
    skos:broader :Quaternary ;
    skos:definition "A time period with the following approximated bounds: older bound -0.0117 Ma, younger bound -0.0 Ma" ;
    skos:inScheme cs: ;
    skos:narrower
        :Greenlandian ,
        :Meghalayan ,
        :Northgrippian ;
    skos:prefLabel "Holocene"@en ;
    prov:wasDerivedFrom ts:gts2020 ;
    sdo:color
        "0/10/20/0"^^:CMYK ,
        "254/235/210"^^:RGB ,
        "#FEEBD2"^^:RGBHex ;
.

:Jurassic
    a skos:Concept ;
    rdfs:isDefinedBy ts:gts2020 ;
    skos:altLabel
        "Юра"@bg ,
        "Jura"@cs ,
        "Jurassisk"@da ,
        "Jura"@de ,
        "Jurásico"@es ,
        "Juura"@et ,
        "Jura"@fi ,
        "Jurassique"@fr ,
        "jura"@hu ,
        "giurassico"@it ,
        "ジュラ紀"@ja ,
        "Jura"@lt ,
        "Jura"@nl ,
        "Jura"@no ,
        "Jura"@pl ,
        "Jurássico"@pt ,
        "jura, jurský"@sk ,
        "jura"@sl ,
        "jura"@sv ,
        "侏罗纪"@zh ;
    skos:broader :Mesozoic ;
    skos:definition "A time period with the following approximated bounds: older bound -201.3 +|-0.2 Ma, younger bound -145.0 Ma" ;
    skos:inScheme cs: ;
    skos:narrower
        :LowerJurassic ,
        :MiddleJurassic ,
        :UpperJurassic ;
    skos:prefLabel "Jurassic"@en ;
    prov:wasDerivedFrom ts:gts2020 ;
    sdo:color
        "80/0/5/0"^^:CMYK ,
        "52/178/201"^^:RGB ,
        "#34B2C9"^^:RGBHex ;
.

:Llandovery
    a skos:Concept ;
    rdfs:isDefinedBy ts:gts2020 ;
    skos:altLabel
        "Лиандовери"@bg ,
        "Llandovery"@cs ,
        "Llandovery"@da ,
        "Llandovery"@de ,
        "Llandovery"@es ,
        "Llandovery"@et ,
        "Llandovery"@fi ,
        "Llandovery"@fr ,
        "llandoveryi"@hu ,
        "llandovery"@it ,
        "ランドベリアン世"@ja ,
        "Landoveris"@lt ,
        "Llandovery"@nl ,
        "Llandovery"@no ,
        "Landower"@pl ,
        "Llandovery"@pt ,
        "llandover"@sk ,
        "llandoverij"@sl ,
        "llandovery"@sv ,
        "兰多维列世"@zh ;
    skos:broader :Silurian ;
    skos:definition "A time period with the following approximated bounds: older bound -443.8 +|-1.5 Ma, younger bound -433.4 +|-0.8 Ma" ;
    skos:inScheme cs: ;
    skos:narrower
        :Aeronian ,
        :Rhuddanian ,
        :Telychian ;
    skos:prefLabel "Llandovery"@en ;
    prov:wasDerivedFrom ts:gts2020 ;
    sdo:color
        "40/0/25/0"^^:CMYK ,
        "153/215/179"^^:RGB ,
        "#99D7B3"^^:RGBHex ;
.

:LowerDevonian
    a skos:Concept ;
    rdfs:isDefinedBy ts:gts2020 ;
    skos:altLabel
        "Ранен Девон"@bg ,
        "brzy devon"@cs ,
        "Tidlig Devon"@da ,
        "Frühes Devon"@de ,
        "Devónico temprano"@es ,
        "Vara-Devon"@et ,
        "Varhais-Devoni"@fi ,
        "Dévonien précoce"@fr ,
        "kora-devon"@hu ,
        "devoniano precoce"@it ,
        "デボン紀前期"@ja ,
        "Ankstyvasis Devonas"@lt ,
        "Vroeg Devoon"@nl ,
        "Tidlig devon"@no ,
        "Wczesny Dewon"@pl ,
        "Devoniano primitivo"@pt ,
        "raný devón"@sk ,
        "zgodnji devon"@sl ,
        "äldre devon"@sv ,
        "早泥盆世"@zh ;
    skos:broader :Devonian ;
    skos:definition "A time period with the following approximated bounds: older bound -419.2 +|-3.2 Ma, younger bound -393.3 +|-1.2 Ma" ;
    skos:inScheme cs: ;
    skos:narrower
        :Emsian ,
        :Lochkovian ,
        :Pragian ;
    skos:prefLabel "Early Devonian"@en ;
    prov:wasDerivedFrom ts:gts2020 ;
    sdo:color
        "10/30/65/0"^^:CMYK ,
        "229/172/77"^^:RGB ,
        "#E5AC4D"^^:RGBHex ;
.

:Mesoproterozoic
    a skos:Concept ;
    rdfs:isDefinedBy ts:gts2020 ;
    skos:altLabel
        "Мезопротерозой"@bg ,
        "Mezoproterozoikum"@cs ,
        "Mesoproterozoisk"@da ,
        "Mesoproterozoikum"@de ,
        "Mesoproterozoico"@es ,
        "Mesoproterosoikum"@et ,
        "Mesoproterotsoikum"@fi ,
        "Mésoprotérozoïque"@fr ,
        "mezoproterozoikum"@hu ,
        "mesoproterozoico"@it ,
        "原生代中期"@ja ,
        "Mezoproterozojus"@lt ,
        "Mesoproterozoïcum"@nl ,
        "Mesoproterozoikum"@no ,
        "Mezoproterozoik"@pl ,
        "Mesoproterozóico"@pt ,
        "mezoproterozoikum"@sk ,
        "mezoproterozoik"@sl ,
        "mesoproterozoikum"@sv ,
        "中元古代"@zh ;
    skos:broader :Proterozoic ;
    skos:definition "A time period with the following approximated bounds: older bound -1600 Ma, younger bound -1000 Ma" ;
    skos:inScheme cs: ;
    skos:narrower
        :Calymmian ,
        :Ectasian ,
        :Stenian ;
    skos:prefLabel "Mesoproterozoic"@en ;
    prov:wasDerivedFrom ts:gts2020 ;
    sdo:color
        "0/30/55/0"^^:CMYK ,
        "253/180/98"^^:RGB ,
        "#FDB462"^^:RGBHex ;
.

:Mesozoic
    a skos:Concept ;
    rdfs:isDefinedBy ts:gts2020 ;
    skos:altLabel
        "Мезозой"@bg ,
        "Mezozoikum"@cs ,
        "Mesozoisk"@da ,
        "Mesozoikum"@de ,
        "Mesozoico"@es ,
        "Mesosoikum"@et ,
        "Mesotsoikum"@fi ,
        "Mésozoïque"@fr ,
        "mezozoikum"@hu ,
        "mesozoico"@it ,
        "中生代"@ja ,
        "Mezozojus"@lt ,
        "Mesozoïcum"@nl ,
        "Mesozoikum"@no ,
        "Mezozoik"@pl ,
        "Mesozóico"@pt ,
        "mezozoikum"@sk ,
        "mezozoik"@sl ,
        "mesozoikum"@sv ,
        "中生代"@zh ;
    skos:broader :Phanerozoic ;
    skos:definition "A time period with the following approximated bounds: older bound -251.902 +|-0.024 Ma, younger bound -66.0 Ma" ;
    skos:inScheme cs: ;
    skos:narrower
        :Cretaceous ,
        :Jurassic ,
        :Triassic ;
    skos:prefLabel "Mesozoic"@en ;
    prov:wasDerivedFrom ts:gts2020 ;
    sdo:color
        "60/0/10/0"^^:CMYK ,
        "103/197/202"^^:RGB ,
        "#67C5CA"^^:RGBHex ;
.

:Miaolingian
    a skos:Concept ;
    rdfs:isDefinedBy ts:gts2020 ;
    skos:broader :Cambrian ;
    skos:definition "A time period with the following approximated bounds: older bound -509 Ma, younger bound -497 Ma" ;
    skos:inScheme cs: ;
    skos:narrower
        :Drumian ,
        :Guzhangian ,
        :Wuliuan ;
    skos:prefLabel "Miaolingian"@en ;
    prov:wasDerivedFrom ts:gts2020 ;
    sdo:color
        "35/5/45/0"^^:CMYK ,
        "166/207/134"^^:RGB ,
        "#A6CF86"^^:RGBHex ;
.

:Mississippian
    a skos:Concept ;
    rdfs:isDefinedBy ts:gts2020 ;
    skos:altLabel
        "Миѿиѿип"@bg ,
        "Mississip"@cs ,
        "Mississippien"@da ,
        "Mississippium"@de ,
        "Mississippiense"@es ,
        "Mississippi"@et ,
        "Mississippi"@fi ,
        "Mississippien"@fr ,
        "mississippi"@hu ,
        "mississippiano"@it ,
        "ミシシッピアン紀"@ja ,
        "Misisipis"@lt ,
        "Mississippiën"@nl ,
        "Mississippium"@no ,
        "Missisip"@pl ,
        "Mississipiano"@pt ,
        "mississip"@sk ,
        "mississippij"@sl ,
        "mississippi"@sv ,
        "密西西比亚纪"@zh ;
    skos:broader :Carboniferous ;
    skos:definition "A time period with the following approximated bounds: older bound -358.9 +|-0.4 Ma, younger bound -323.2 +|-0.4 Ma" ;
    skos:inScheme cs: ;
    skos:narrower
        :LowerMississippian ,
        :MiddleMississippian ,
        :UpperMississippian ;
    skos:prefLabel "Mississippian"@en ;
    prov:wasDerivedFrom ts:gts2020 ;
    sdo:color
        "60/25/55/0"^^:CMYK ,
        "103/143/102"^^:RGB ,
        "#678F66"^^:RGBHex ;
.

:Neoproterozoic
    a skos:Concept ;
    rdfs:isDefinedBy ts:gts2020 ;
    skos:altLabel
        "пеопротерозой"@bg ,
        "Neoproterozoikum"@cs ,
        "Neoproterozoisk"@da ,
        "Neoproterozoikum"@de ,
        "Neoproerozoico"@es ,
        "Neoproterosoikum"@et ,
        "Neoproterotsoikum"@fi ,
        "Néoprotérozoïque"@fr ,
        "neoproterozoikum"@hu ,
        "neoproterozoico"@it ,
        "原生代後期"@ja ,
        "Neoproterozojus"@lt ,
        "Neoproterozoïcum"@nl ,
        "Neoproterozoikum"@no ,
        "Neoproterozoik"@pl ,
        "Neoproterozóico"@pt ,
        "neoproterozoikum"@sk ,
        "neoproterozoik"@sl ,
        "neoproterozoikum"@sv ,
        "新元古代"@zh ;
    skos:broader :Proterozoic ;
    skos:definition "A time period with the following approximated bounds: older bound -1000 Ma, younger bound -541.0 +|-1.0 Ma" ;
    skos:inScheme cs: ;
    skos:narrower
        :Cryogenian ,
        :Ediacaran ,
        :Tonian ;
    skos:prefLabel "Neoproterozoic"@en ;
    prov:wasDerivedFrom ts:gts2020 ;
    sdo:color
        "0/30/70/0"^^:CMYK ,
        "254/179/66"^^:RGB ,
        "#FEB342"^^:RGBHex ;
.

:Ordovician
    a skos:Concept ;
    rdfs:isDefinedBy ts:gts2020 ;
    skos:altLabel
        "Ордовик"@bg ,
        "Ordovik"@cs ,
        "Ordovicium"@da ,
        "Ordovizium"@de ,
        "Ordovícico"@es ,
        "Ordoviitsium"@et ,
        "Ordoviikki"@fi ,
        "Ordovicien"@fr ,
        "ordovícium"@hu ,
        "ordoviciano"@it ,
        "オルドビス紀"@ja ,
        "Ordovikas"@lt ,
        "Ordovicium"@nl ,
        "Ordovicium"@no ,
        "Ordowik"@pl ,
        "Ordovícico"@pt ,
        "ordovik"@sk ,
        "ordovicij"@sl ,
        "ordovicium"@sv ,
        "奥陶纪"@zh ;
    skos:broader :Paleozoic ;
    skos:definition "A time period with the following approximated bounds: older bound -485.4 +|-1.9 Ma, younger bound -443.8 +|-1.5 Ma" ;
    skos:inScheme cs: ;
    skos:narrower
        :LowerOrdovician ,
        :MiddleOrdovician ,
        :UpperOrdovician ;
    skos:prefLabel "Ordovician"@en ;
    prov:wasDerivedFrom ts:gts2020 ;
    sdo:color
        "100/0/60/0"^^:CMYK ,
        "0/146/112"^^:RGB ,
        "#009270"^^:RGBHex ;
.

:Paleocene
    a skos:Concept ;
    rdfs:isDefinedBy ts:gts2020 ;
    skos:altLabel
        "Палеоцен"@bg ,
        "Paleocén"@cs ,
        "Paleocæn"@da ,
        "Paläozän"@de ,
        "Palaeocene"@en-GB ,
        "Paleocene"@en-US ,
        "Paleoceno"@es ,
        "Paleotseen"@et ,
        "Paleoseeni"@fi ,
        "Paléocène"@fr ,
        "paleocén"@hu ,
        "paleocene"@it ,
        "暁新世"@ja ,
        "Paleocenas"@lt ,
        "Paleoceen"@nl ,
        "Paleocen"@no ,
        "Paleocen"@pl ,
        "Paleocénico"@pt ,
        "paleocén"@sk ,
        "paleocen"@sl ,
        "paleocen"@sv ,
        "古新世"@zh ;
    skos:broader :Paleogene ;
    skos:definition "A time period with the following approximated bounds: older bound -66.0 Ma, younger bound -56 Ma" ;
    skos:inScheme cs: ;
    skos:narrower
        :Danian ,
        :Selandian ,
        :Thanetian ;
    skos:prefLabel "Paleocene"@en ;
    prov:wasDerivedFrom ts:gts2020 ;
    sdo:color
        "0/40/60/0"^^:CMYK ,
        "253/167/95"^^:RGB ,
        "#FDA75F"^^:RGBHex ;
.

:Paleogene
    a skos:Concept ;
    rdfs:isDefinedBy ts:gts2020 ;
    skos:altLabel
        "Палеоген"@bg ,
        "Paleogén"@cs ,
        "Palæogen"@da ,
        "Paläogen"@de ,
        "Palaeogene"@en-GB ,
        "Paleogene"@en-US ,
        "Paleógeno"@es ,
        "Paleogeen"@et ,
        "Paleogeeni"@fi ,
        "Paléogène"@fr ,
        "paleogén"@hu ,
        "paleogene"@it ,
        "古第三紀"@ja ,
        "Paleogenas"@lt ,
        "Paleogeen"@nl ,
        "Paleogen"@no ,
        "Paleogen"@pl ,
        "Paleogénico"@pt ,
        "paleogén"@sk ,
        "paleogen"@sl ,
        "paleogen"@sv ,
        "早第三纪"@zh ;
    skos:broader :Cenozoic ;
    skos:definition "A time period with the following approximated bounds: older bound -66.0 Ma, younger bound -23.03 Ma" ;
    skos:inScheme cs: ;
    skos:narrower
        :Eocene ,
        :Oligocene ,
        :Paleocene ;
    skos:prefLabel "Paleogene"@en ;
    prov:wasDerivedFrom ts:gts2020 ;
    sdo:color
        "5/0/90/0"^^:CMYK ,
        "253/154/82"^^:RGB ,
        "#FD9A52"^^:RGBHex ;
.

:Pennsylvanian
    a skos:Concept ;
    rdfs:isDefinedBy ts:gts2020 ;
    skos:altLabel
        "Пенѿилван"@bg ,
        "Pennsylván"@cs ,
        "Pennsylvanien"@da ,
        "Pennsylvanium"@de ,
        "Pennsylvaniense"@es ,
        "Pennsylvania"@et ,
        "Pennsylvania"@fi ,
        "Pennsylvanien"@fr ,
        "pennsylvaniai"@hu ,
        "pennsylvaniano"@it ,
        "ペンシルバニア紀"@ja ,
        "Pensilvanis"@lt ,
        "Pennsylvaniën"@nl ,
        "Pennsylvanium"@no ,
        "Pensylwan"@pl ,
        "Pensilvaniano"@pt ,
        "penssylván"@sk ,
        "pennsylvanij"@sl ,
        "pennsylvan"@sv ,
        "宾夕法尼亚亚纪"@zh ;
    skos:broader :Carboniferous ;
    skos:definition "A time period with the following approximated bounds: older bound -323.2 +|-0.4 Ma, younger bound -298.9 +|-0.15 Ma" ;
    skos:inScheme cs: ;
    skos:narrower
        :LowerPennsylvanian ,
        :MiddlePennsylvanian ,
        :UpperPennsylvanian ;
    skos:prefLabel "Pennsylvanian"@en ;
    prov:wasDerivedFrom ts:gts2020 ;
    sdo:color
        "50/10/20/0"^^:CMYK ,
        "126/188/198"^^:RGB ,
        "#7EBCC6"^^:RGBHex ;
.

:Permian
    a skos:Concept ;
    rdfs:isDefinedBy ts:gts2020 ;
    skos:altLabel
        "Перм"@bg ,
        "Perm"@cs ,
        "Perm"@da ,
        "Perm"@de ,
        "Pérmico"@es ,
        "Perm"@et ,
        "Permi"@fi ,
        "Permien"@fr ,
        "perm"@hu ,
        "permiano"@it ,
        "ペルム紀"@ja ,
        "Permas"@lt ,
        "Perm"@nl ,
        "Perm"@no ,
        "Perm"@pl ,
        "Pérmico"@pt ,
        "perm"@sk ,
        "perm"@sl ,
        "perm"@sv ,
        "二叠纪"@zh ;
    skos:broader :Paleozoic ;
    skos:definition "A time period with the following approximated bounds: older bound -298.9 +|-0.15 Ma, younger bound -251.902 +|-0.024 Ma" ;
    skos:inScheme cs: ;
    skos:narrower
        :Cisuralian ,
        :Guadalupian ,
        :Lopingian ;
    skos:prefLabel "Permian"@en ;
    prov:wasDerivedFrom ts:gts2020 ;
    sdo:color
        "5/75/75/0"^^:CMYK ,
        "240/64/40"^^:RGB ,
        "#F04028"^^:RGBHex ;
.

:Phanerozoic
    a skos:Concept ;
    rdfs:isDefinedBy ts:gts2020 ;
    skos:altLabel
        "Фанерозой"@bg ,
        "Fanerozoikum"@cs ,
        "Phanerozoisk"@da ,
        "Phanerozoikum"@de ,
        "Fanerozoico"@es ,
        "Fanerosoikum"@et ,
        "Fanerotsoikum"@fi ,
        "Phanérozoïque"@fr ,
        "fanerozoikum"@hu ,
        "fanerozoico"@it ,
        "顕生代"@ja ,
        "Fanerozojus"@lt ,
        "Phanerozoïcum"@nl ,
        "Fanerozoikum"@no ,
        "Fanerozoik"@pl ,
        "Fanerozóico"@pt ,
        "fanerozoikum"@sk ,
        "fanerozoik"@sl ,
        "fanerozoikum"@sv ,
        "显生宙"@zh ;
    skos:definition "A time period with the following approximated bounds: older bound -541.0 +|-1.0 Ma, younger bound -0.0 Ma" ;
    skos:inScheme cs: ;
    skos:narrower
        :Cenozoic ,
        :Mesozoic ,
        :Paleozoic ;
    skos:prefLabel "Phanerozoic"@en ;
    prov:wasDerivedFrom ts:gts2020 ;
    sdo:color
        "40/0/5/0"^^:CMYK ,
        "154/217/221"^^:RGB ,
        "#9AD9DD"^^:RGBHex ;
.

:Precambrian
    a skos:Concept ;
    rdfs:isDefinedBy ts:gts2020 ;
    skos:altLabel
        "Прекамбрий"@bg ,
        "Prekambrium"@cs ,
        "Prækambrium"@da ,
        "Präkambrium"@de ,
        "Precámbrico"@es ,
        "Prekambrium"@et ,
        "Prekambri"@fi ,
        "Précambrien"@fr ,
        "prekambrium"@hu ,
        "precambriano"@it ,
        "先カンブリア時代"@ja ,
        "Prekambras"@lt ,
        "Precambrium"@nl ,
        "Prekambrium"@no ,
        "Prekambr"@pl ,
        "Precâmbrico"@pt ,
        "prekambrium"@sk ,
        "predkambrij"@sl ,
        "prekambrium"@sv ,
        "前寒武纪"@zh ;
    skos:definition "A time period with the following approximated bounds: older bound -4567 +|-1 Ma, younger bound -541.0 +|-1.0 Ma" ;
    skos:inScheme cs: ;
    skos:narrower
        :Archean ,
        :Hadean ,
        :Proterozoic ;
    skos:prefLabel "Precambrian"@en ;
    prov:wasDerivedFrom ts:gts2020 ;
    sdo:color
        "0/75/30/0"^^:CMYK ,
        "247/67/112"^^:RGB ,
        "#F74370"^^:RGBHex ;
.

:Proterozoic
    a skos:Concept ;
    rdfs:isDefinedBy ts:gts2020 ;
    skos:altLabel
        "Протерозой"@bg ,
        "Proterozoikum"@cs ,
        "Proterozoikum"@da ,
        "Proterozoikum"@de ,
        "Proterozoico"@es ,
        "Proterosoikum"@et ,
        "Proterotsoikum"@fi ,
        "Protérozoïque"@fr ,
        "proterozoos"@hu ,
        "proterozoico"@it ,
        "原生代"@ja ,
        "Proterozojus"@lt ,
        "Proterozoïcum"@nl ,
        "Proterozoisk"@no ,
        "Proterozoik"@pl ,
        "Proterozóico"@pt ,
        "proterozoikum"@sk ,
        "proterozoik"@sl ,
        "proterozoikum"@sv ,
        "元古宙"@zh ;
    skos:broader :Precambrian ;
    skos:definition "A time period with the following approximated bounds: older bound -2500 Ma, younger bound -541.0 +|-1.0 Ma" ;
    skos:inScheme cs: ;
    skos:narrower
        :Mesoproterozoic ,
        :Neoproterozoic ,
        :Paleoproterozoic ;
    skos:prefLabel "Proterozoic"@en ;
    prov:wasDerivedFrom ts:gts2020 ;
    sdo:color
        "0/80/35/0"^^:CMYK ,
        "247/53/99"^^:RGB ,
        "#F73563"^^:RGBHex ;
.

:Triassic
    a skos:Concept ;
    rdfs:isDefinedBy ts:gts2020 ;
    skos:altLabel
        "Триаѿ"@bg ,
        "Trias"@cs ,
        "Triassisk"@da ,
        "Trias"@de ,
        "Triásico"@es ,
        "Triias"@et ,
        "Trias"@fi ,
        "Trias"@fr ,
        "triász"@hu ,
        "triassico"@it ,
        "三畳紀"@ja ,
        "Triasas"@lt ,
        "Trias"@nl ,
        "Trias"@no ,
        "Trias"@pl ,
        "Triásico"@pt ,
        "trias"@sk ,
        "trias"@sl ,
        "trias"@sv ,
        "三叠纪"@zh ;
    skos:broader :Mesozoic ;
    skos:definition "A time period with the following approximated bounds: older bound -251.902 +|-0.024 Ma, younger bound -201.3 +|-0.2 Ma" ;
    skos:inScheme cs: ;
    skos:narrower
        :LowerTriassic ,
        :MiddleTriassic ,
        :UpperTriassic ;
    skos:prefLabel "Triassic"@en ;
    prov:wasDerivedFrom ts:gts2020 ;
    sdo:color
        "50/80/0/0"^^:CMYK ,
        "129/43/146"^^:RGB ,
        "#812B92"^^:RGBHex ;
.

:UpperJurassic
    a skos:Concept ;
    rdfs:isDefinedBy ts:gts2020 ;
    skos:altLabel
        "Къѿна Юра"@bg ,
        "Pozdní jura"@cs ,
        "Sen Jurassisk"@da ,
        "Später Jura"@de ,
        "Hilis-Juura"@et ,
        "Myöhäis-Jura"@fi ,
        "késő-jura"@hu ,
        "後期ジュラ紀"@ja ,
        "Vėlyvoji Jura"@lt ,
        "Laat Jura"@nl ,
        "Sen jura"@no ,
        "Późna Jura"@pl ,
        "mladšia jura"@sk ,
        "pozna jura"@sl ,
        "yngre jura"@sv ,
        "晚侏罗世"@zh ;
    skos:broader :Jurassic ;
    skos:definition "A time period with the following approximated bounds: older bound -163.5 +|-1.0 Ma, younger bound -145.0 Ma" ;
    skos:inScheme cs: ;
    skos:narrower
        :Kimmeridgian ,
        :Oxfordian ,
        :Tithonian ;
    skos:prefLabel "Late Jurassic"@en ;
    prov:wasDerivedFrom ts:gts2020 ;
    sdo:color
        "30/0/0/0"^^:CMYK ,
        "179/227/238"^^:RGB ,
        "#B3E3EE"^^:RGBHex ;
.

:UpperOrdovician
    a skos:Concept ;
    rdfs:isDefinedBy ts:gts2020 ;
    skos:altLabel
        "Къѿен Ордовик"@bg ,
        "Pozdní ordovik"@cs ,
        "Sen Ordovicium"@da ,
        "Spätes Ordovizium"@de ,
        "Hilis-Ordoviitsium"@et ,
        "Myöhäis-Ordoviikki"@fi ,
        "késő-ordovícium"@hu ,
        "後期オルドビス紀"@ja ,
        "Vėlyvasis Ordovikas"@lt ,
        "Laat Ordovicium"@nl ,
        "Sen ordovicium"@no ,
        "Późny Ordowik"@pl ,
        "mladší ordovik"@sk ,
        "starejši ordovicij"@sl ,
        "yngre ordovicium"@sv ,
        "晚奥陶世"@zh ;
    skos:broader :Ordovician ;
    skos:definition "A time period with the following approximated bounds: older bound -458.4 +|-0.9 Ma, younger bound -443.8 +|-1.5 Ma" ;
    skos:inScheme cs: ;
    skos:narrower
        :Hirnantian ,
        :Katian ,
        :Sandbian ;
    skos:prefLabel "Late Ordovician"@en ;
    prov:wasDerivedFrom ts:gts2020 ;
    sdo:color
        "50/0/40/0"^^:CMYK ,
        "127/202/147"^^:RGB ,
        "#7FCA93"^^:RGBHex ;
.

:UpperTriassic
    a skos:Concept ;
    rdfs:isDefinedBy ts:gts2020 ;
    skos:altLabel
        "Къѿен Триаѿ"@bg ,
        "Pozdní trias"@cs ,
        "Sen Triassisk"@da ,
        "Späte Trias"@de ,
        "Hilis-Triias"@et ,
        "Myöhäis-Trias"@fi ,
        "késő-triász"@hu ,
        "後期三畳紀"@ja ,
        "Vėlyvasis Triasas"@lt ,
        "Laat Trias"@nl ,
        "Sen trias"@no ,
        "Późny Trias"@pl ,
        "mladší trias"@sk ,
        "pozni trias"@sl ,
        "yngre trias"@sv ,
        "晚三叠世"@zh ;
    skos:broader :Triassic ;
    skos:definition "A time period with the following approximated bounds: older bound -237 Ma, younger bound -201.3 +|-0.2 Ma" ;
    skos:inScheme cs: ;
    skos:narrower
        :Carnian ,
        :Norian ,
        :Rhaetian ;
    skos:prefLabel "Late Triassic"@en ;
    prov:wasDerivedFrom ts:gts2020 ;
    sdo:color
        "25/40/0/0"^^:CMYK ,
        "189/140/195"^^:RGB ,
        "#BD8CC3"^^:RGBHex ;
.

:Archean
    a skos:Concept ;
    rdfs:isDefinedBy ts:gts2020 ;
    skos:altLabel
        "прхай"@bg ,
        "Archaikum"@cs ,
        "Arkæisk"@da ,
        "Archaikum"@de ,
        "Archaean"@en-GB ,
        "Archean"@en-US ,
        "Arcaico"@es ,
        "Arhaikum"@et ,
        "Arkeikum"@fi ,
        "Archéen"@fr ,
        "archaikum"@hu ,
        "archeano"@it ,
        "始生代"@ja ,
        "Archejus"@lt ,
        "Archaïcum"@nl ,
        "Arkeikum"@no ,
        "Archaik"@pl ,
        "Arcaico"@pt ,
        "archaikum, prahory"@sk ,
        "arhaik"@sl ,
        "arkeikum"@sv ,
        "太古宙"@zh ;
    skos:broader :Precambrian ;
    skos:definition "A time period with the following approximated bounds: older bound -4000 Ma, younger bound -2500 Ma" ;
    skos:inScheme cs: ;
    skos:narrower
        :Eoarchean ,
        :Mesoarchean ,
        :Neoarchean ,
        :Paleoarchean ;
    skos:prefLabel "Archean"@en ;
    prov:wasDerivedFrom ts:gts2020 ;
    sdo:color
        "0/100/0/0"^^:CMYK ,
        "240/4/127"^^:RGB ,
        "#F0047F"^^:RGBHex ;
.

:Cambrian
    a skos:Concept ;
    rdfs:isDefinedBy ts:gts2020 ;
    skos:altLabel
        "Камбрий"@bg ,
        "Kambrium"@cs ,
        "Kambrium"@da ,
        "Kambrium"@de ,
        "Cámbrico"@es ,
        "Kambrium"@et ,
        "Kambri"@fi ,
        "Cambrien"@fr ,
        "kambriumi"@hu ,
        "cambriano"@it ,
        "カンブリア紀"@ja ,
        "Kambras"@lt ,
        "Cambrium"@nl ,
        "Cambrium"@no ,
        "Kambr"@pl ,
        "Câmbrico"@pt ,
        "kambrium"@sk ,
        "kambrij"@sl ,
        "kambrium"@sv ,
        "寒武纪"@zh ;
    skos:broader :Paleozoic ;
    skos:definition "A time period with the following approximated bounds: older bound -541.0 +|-1.0 Ma, younger bound -485.4 +|-1.9 Ma" ;
    skos:inScheme cs: ;
    skos:narrower
        :CambrianSeries2 ,
        :Furongian ,
        :Miaolingian ,
        :Terreneuvian ;
    skos:prefLabel "Cambrian"@en ;
    prov:wasDerivedFrom ts:gts2020 ;
    sdo:color
        "50/20/65/0"^^:CMYK ,
        "127/160/86"^^:RGB ,
        "#7FA056"^^:RGBHex ;
.

:Cisuralian
    a skos:Concept ;
    rdfs:isDefinedBy ts:gts2020 ;
    skos:altLabel
        "Циѿурал"@bg ,
        "Cisural"@cs ,
        "Cisuralien"@da ,
        "Cisuralium"@de ,
        "Cisuraliense"@es ,
        "Cisural"@et ,
        "Cisural"@fi ,
        "Cisuralien"@fr ,
        "ciszurali"@hu ,
        "cisuraliano"@it ,
        "キスラリアン世"@ja ,
        "Kisuralis"@lt ,
        "Cisuraliën"@nl ,
        "Cisuralium"@no ,
        "Cisural"@pl ,
        "Cisuraliano"@pt ,
        "cisural"@sk ,
        "cisuralij"@sl ,
        "cisural"@sv ,
        "乌拉尔世"@zh ;
    skos:broader :Permian ;
    skos:definition "A time period with the following approximated bounds: older bound -298.9 +|-0.15 Ma, younger bound -272.95 +|-0.11 Ma" ;
    skos:inScheme cs: ;
    skos:narrower
        :Artinskian ,
        :Asselian ,
        :Kungurian ,
        :Sakmarian ;
    skos:prefLabel "Cisuralian"@en ;
    prov:wasDerivedFrom ts:gts2020 ;
    sdo:color
        "5/65/60/0"^^:CMYK ,
        "239/88/69"^^:RGB ,
        "#EF5845"^^:RGBHex ;
.

:Eocene
    a skos:Concept ;
    rdfs:isDefinedBy ts:gts2020 ;
    skos:altLabel
        "Еоцен"@bg ,
        "Eocén"@cs ,
        "Eocæn"@da ,
        "Eozän"@de ,
        "Eoceno"@es ,
        "Eotseen"@et ,
        "Eoseeni"@fi ,
        "Eocène"@fr ,
        "eocén"@hu ,
        "eocene"@it ,
        "始新世"@ja ,
        "Eocenas"@lt ,
        "Eoceen"@nl ,
        "Eocen"@no ,
        "Eocen"@pl ,
        "Eocénico"@pt ,
        "eocén"@sk ,
        "eocen"@sl ,
        "eocen"@sv ,
        "始新世"@zh ;
    skos:broader :Paleogene ;
    skos:definition "A time period with the following approximated bounds: older bound -56 Ma, younger bound -33.9 Ma" ;
    skos:inScheme cs: ;
    skos:narrower
        :Bartonian ,
        :Lutetian ,
        :Priabonian ,
        :Ypresian ;
    skos:prefLabel "Eocene"@en ;
    prov:wasDerivedFrom ts:gts2020 ;
    sdo:color
        "0/30/50/0"^^:CMYK ,
        "253/180/108"^^:RGB ,
        "#FDB46C"^^:RGBHex ;
.

:LowerJurassic
    a skos:Concept ;
    rdfs:isDefinedBy ts:gts2020 ;
    skos:altLabel
        "Ранна Юра"@bg ,
        "brzy jura"@cs ,
        "Tidlig Jurassisk"@da ,
        "Früher Jura"@de ,
        "Jurásico temprano"@es ,
        "Vara-Juura"@et ,
        "Varhais-Jura"@fi ,
        "Jurassique précoce"@fr ,
        "kora-jura"@hu ,
        "giurassico precoce"@it ,
        "ジュラ紀前期"@ja ,
        "Ankstyvoji Jura"@lt ,
        "Vroeg Jura"@nl ,
        "Tidlig jura"@no ,
        "Wczesna Jura"@pl ,
        "Jurássico primitivo"@pt ,
        "raná jura"@sk ,
        "zgodnja jura"@sl ,
        "äldre jura"@sv ,
        "早侏罗世"@zh ;
    skos:broader :Jurassic ;
    skos:definition "A time period with the following approximated bounds: older bound -201.3 +|-0.2 Ma, younger bound -174.1 +|-1.0 Ma" ;
    skos:inScheme cs: ;
    skos:narrower
        :Hettangian ,
        :Pliensbachian ,
        :Sinemurian ,
        :Toarcian ;
    skos:prefLabel "Early Jurassic"@en ;
    prov:wasDerivedFrom ts:gts2020 ;
    sdo:color
        "75/5/0/0"^^:CMYK ,
        "66/174/208"^^:RGB ,
        "#42AED0"^^:RGBHex ;
.

:MiddleJurassic
    a skos:Concept ;
    rdfs:isDefinedBy ts:gts2020 ;
    skos:altLabel
        "Средна Юра"@bg ,
        "Střední jura"@cs ,
        "Mellem Jurassisk"@da ,
        "Mittlerer Jura"@de ,
        "Jurásico Medio"@es ,
        "Kesk-Juura"@et ,
        "Keski-Jura"@fi ,
        "Jurassique moyen"@fr ,
        "középső-jura"@hu ,
        "giurassico medio"@it ,
        "中期ジュラ紀"@ja ,
        "Vidurinė Jura"@lt ,
        "Midden Jura"@nl ,
        "Midtre jura"@no ,
        "Środkowa Jura"@pl ,
        "Jurássico Médio"@pt ,
        "stredná jura"@sk ,
        "srednja jura"@sl ,
        "mellersta jura"@sv ,
        "中侏罗世"@zh ;
    skos:broader :Jurassic ;
    skos:definition "A time period with the following approximated bounds: older bound -174.1 +|-1.0 Ma, younger bound -163.5 +|-1.0 Ma" ;
    skos:inScheme cs: ;
    skos:narrower
        :Aalenian ,
        :Bajocian ,
        :Bathonian ,
        :Callovian ;
    skos:prefLabel "Middle Jurassic"@en ;
    prov:wasDerivedFrom ts:gts2020 ;
    sdo:color
        "50/0/5/0"^^:CMYK ,
        "128/207/216"^^:RGB ,
        "#80CFD8"^^:RGBHex ;
.

:Paleoproterozoic
    a skos:Concept ;
    rdfs:isDefinedBy ts:gts2020 ;
    skos:altLabel
        "Палеопротерозой"@bg ,
        "Paleoproterozoikum"@cs ,
        "Palæoproterozoisk"@da ,
        "Paläoproteroizoikum"@de ,
        "Palaeoproterozoic"@en-GB ,
        "Paleoproterozoic"@en-US ,
        "Paleoproterozoico"@es ,
        "Paleoproterosoikum"@et ,
        "Paleoproterotsoikum"@fi ,
        "Paléoprotérozoïque"@fr ,
        "paleoproterozikum"@hu ,
        "paleoproterozoico"@it ,
        "原生代前期"@ja ,
        "Paleoproterozojus"@lt ,
        "paleoproterozoïcum"@nl ,
        "Paleoproterozoikum"@no ,
        "Paleoproterozoik"@pl ,
        "Paleoproterozóico"@pt ,
        "paleoproterozoikum"@sk ,
        "paleoproterozoik"@sl ,
        "paleoproterozoikum"@sv ,
        "古元古代"@zh ;
    skos:broader :Proterozoic ;
    skos:definition "A time period with the following approximated bounds: older bound -2500 Ma, younger bound -1600 Ma" ;
    skos:inScheme cs: ;
    skos:narrower
        :Orosirian ,
        :Rhyacian ,
        :Siderian ,
        :Statherian ;
    skos:prefLabel "Paleoproterozoic"@en ;
    prov:wasDerivedFrom ts:gts2020 ;
    sdo:color
        "0/75/30/0"^^:CMYK ,
        "247/67/112"^^:RGB ,
        "#F74370"^^:RGBHex ;
.

:Pleistocene
    a skos:Concept ;
    rdfs:isDefinedBy ts:gts2020 ;
    skos:altLabel
        "Плейѿтоцен"@bg ,
        "Pleistocén"@cs ,
        "Pleistocæn"@da ,
        "Pleistozän"@de ,
        "Pleistoceno"@es ,
        "Pleistotseen"@et ,
        "Pleistoseeni"@fi ,
        "Pléistocène"@fr ,
        "pleisztocén"@hu ,
        "pleistocene"@it ,
        "更新世"@ja ,
        "Pleistocenas"@lt ,
        "Pleistoceen"@nl ,
        "Pleistocen"@no ,
        "Plejstocen"@pl ,
        "Plistocénico"@pt ,
        "pleistocén"@sk ,
        "pleistocen"@sl ,
        "pleistocen"@sv ,
        "更新世"@zh ;
    skos:broader :Quaternary ;
    skos:definition "A time period with the following approximated bounds: older bound -2.58 Ma, younger bound -0.0117 Ma" ;
    skos:inScheme cs: ;
    skos:narrower
        :Calabrian ,
        :Chibanian ,
        :Gelasian ,
        :UpperPleistocene ;
    skos:prefLabel "Pleistocene"@en ;
    prov:wasDerivedFrom ts:gts2020 ;
    sdo:color
        "0/5/40/0"^^:CMYK ,
        "255/239/175"^^:RGB ,
        "#FFEFAF"^^:RGBHex ;
.

:Silurian
    a skos:Concept ;
    rdfs:isDefinedBy ts:gts2020 ;
    skos:altLabel
        "Силур"@bg ,
        "Silur"@cs ,
        "Silur"@da ,
        "Silur"@de ,
        "Silúrcio"@es ,
        "Silur"@et ,
        "Siluuri"@fi ,
        "Silurien"@fr ,
        "szilur"@hu ,
        "siluriano"@it ,
        "シルル紀"@ja ,
        "Silūras"@lt ,
        "Siluur"@nl ,
        "Silur"@no ,
        "Sylur"@pl ,
        "Silúrico"@pt ,
        "silúr"@sk ,
        "silur"@sl ,
        "silur"@sv ,
        "志留纪"@zh ;
    skos:broader :Paleozoic ;
    skos:definition "A time period with the following approximated bounds: older bound -443.8 +|-1.5 Ma, younger bound -419.2 +|-3.2 Ma" ;
    skos:inScheme cs: ;
    skos:narrower
        :Llandovery ,
        :Ludlow ,
        :Pridoli ,
        :Wenlock ;
    skos:prefLabel "Silurian"@en ;
    prov:wasDerivedFrom ts:gts2020 ;
    sdo:color
        "30/0/25/0"^^:CMYK ,
        "179/225/182"^^:RGB ,
        "#B3E1B6"^^:RGBHex ;
.

:LowerCretaceous
    a skos:Concept ;
    rdfs:isDefinedBy ts:gts2020 ;
    skos:altLabel
        "Ранна Креда"@bg ,
        "Tidlig Kridt"@da ,
        "Frühe Kreide"@de ,
        "Cretácico temprano"@es ,
        "Varajane kriit"@et ,
        "Varhais-Liitu"@fi ,
        "Crétacé précoce"@fr ,
        "kora-kréta"@hu ,
        "Cretaceo precoce"@it ,
        "白亜紀前期"@ja ,
        "Ankstyvoji Kreida"@lt ,
        "Vroeg Krijt"@nl ,
        "Wczesna Kreda"@pl ,
        "Cretáceo Primitivo"@pt ,
        "raná  krieda"@sk ,
        "zgodnja kreda"@sl ,
        "äldre krita"@sv ,
        "早白垩世"@zh ;
    skos:broader :Cretaceous ;
    skos:definition "A time period with the following approximated bounds: older bound -145.0 Ma, younger bound -100.5 Ma" ;
    skos:inScheme cs: ;
    skos:narrower
        :Albian ,
        :Aptian ,
        :Barremian ,
        :Berriasian ,
        :Hauterivian ,
        :Valanginian ;
    skos:prefLabel "Early Cretaceous"@en ;
    prov:wasDerivedFrom ts:gts2020 ;
    sdo:color
        "45/0/70/0"^^:CMYK ,
        "140/205/87"^^:RGB ,
        "#8CCD57"^^:RGBHex ;
.

:Miocene
    a skos:Concept ;
    rdfs:isDefinedBy ts:gts2020 ;
    skos:altLabel
        "Миоцен"@bg ,
        "Miocén"@cs ,
        "Miocæn"@da ,
        "Miozän"@de ,
        "Mioceno"@es ,
        "Miotseen"@et ,
        "Mioseeni"@fi ,
        "Miocène"@fr ,
        "miocén"@hu ,
        "miocene"@it ,
        "中新世"@ja ,
        "Miocenas"@lt ,
        "Mioceen"@nl ,
        "Miocen"@no ,
        "Miocen"@pl ,
        "Miocénico"@pt ,
        "miocén"@sk ,
        "miocen"@sl ,
        "miocen"@sv ,
        "中新世"@zh ;
    skos:broader :Neogene ;
    skos:definition "A time period with the following approximated bounds: older bound -23.03 Ma, younger bound -5.333 Ma" ;
    skos:inScheme cs: ;
    skos:narrower
        :Aquitanian ,
        :Burdigalian ,
        :Langhian ,
        :Messinian ,
        :Serravallian ,
        :Tortonian ;
    skos:prefLabel "Miocene"@en ;
    prov:wasDerivedFrom ts:gts2020 ;
    sdo:color
        "0/0/100/0"^^:CMYK ,
        "255/255/0"^^:RGB ,
        "#FFFF00"^^:RGBHex ;
.

:Paleozoic
    a skos:Concept ;
    rdfs:isDefinedBy ts:gts2020 ;
    skos:altLabel
        "Палеозой"@bg ,
        "Paleozoikum"@cs ,
        "Palæozoisk"@da ,
        "Paläozoikum"@de ,
        "Palaeozoic"@en-GB ,
        "Paleozoic"@en-US ,
        "Palozoico"@es ,
        "Paleosoikum"@et ,
        "Paleotsoikum"@fi ,
        "Paléozoïque"@fr ,
        "paleozoikum"@hu ,
        "paleozoico"@it ,
        "古生代"@ja ,
        "Paleozojus"@lt ,
        "Paleozoïcum"@nl ,
        "Paleozoikum"@no ,
        "Paleozoik"@pl ,
        "Paleozóico"@pt ,
        "paleozoikum"@sk ,
        "paleozoik"@sl ,
        "paleozoikum"@sv ,
        "古生代"@zh ;
    skos:broader :Phanerozoic ;
    skos:definition "A time period with the following approximated bounds: older bound -541.0 +|-1.0 Ma, younger bound -251.902 +|-0.024 Ma" ;
    skos:inScheme cs: ;
    skos:narrower
        :Cambrian ,
        :Carboniferous ,
        :Devonian ,
        :Ordovician ,
        :Permian ,
        :Silurian ;
    skos:prefLabel "Paleozoic"@en ;
    prov:wasDerivedFrom ts:gts2020 ;
    sdo:color
        "40/10/40/0"^^:CMYK ,
        "153/192/141"^^:RGB ,
        "#99C08D"^^:RGBHex ;
.

:UpperCretaceous
    a skos:Concept ;
    rdfs:isDefinedBy ts:gts2020 ;
    skos:altLabel
        "Къѿна Креда"@bg ,
        "Pozdní křída"@cs ,
        "Sen Kridt"@da ,
        "Späte Kreide"@de ,
        "Hilis-Kriit"@et ,
        "Myöhäis-Liitu"@fi ,
        "késő-kréta"@hu ,
        "後期白亜紀"@ja ,
        "Vėlyva kreida"@lt ,
        "Laat Krijt"@nl ,
        "Sen kritt"@no ,
        "Późna Kreda"@pl ,
        "mladšia krieda"@sk ,
        "pozna kreda"@sl ,
        "yngre krita"@sv ,
        "晚白垩世"@zh ;
    skos:broader :Cretaceous ;
    skos:definition "A time period with the following approximated bounds: older bound -100.5 Ma, younger bound -66.0 Ma" ;
    skos:inScheme cs: ;
    skos:narrower
        :Campanian ,
        :Cenomanian ,
        :Coniacian ,
        :Maastrichtian ,
        :Santonian ,
        :Turonian ;
    skos:prefLabel "Late Cretaceous"@en ;
    prov:wasDerivedFrom ts:gts2020 ;
    sdo:color
        "35/0/75/0"^^:CMYK ,
        "166/216/74"^^:RGB ,
        "#A6D84A"^^:RGBHex ;
.

cs:
    a skos:ConceptScheme ;
    sdo:dateCreated "2020-06-05"^^xsd:date ;
    sdo:creator <https://linked.data.gov.au/org/ics> ;
    sdo:license <https://creativecommons.org/licenses/by/4.0/> ;
    sdo:dateModified "2022-11-28"^^xsd:date ;
    sdo:publisher <https://linked.data.gov.au/org/ics> ;
    sdo:copyrightHolder <https://linked.data.gov.au/org/ics> ;
    sdo:copyrightNotice "Original version Copyright © 2020 International Commission on Stratigraphy"@en ;
    sdo:citation "https://stratigraphy.org/chart"^^xsd:anyURI ;
    owl:versionIRI cs:0.2 ;
    owl:versionInfo """0.2: Includes colour information

0.1: Initial release""" ;
    skos:definition """This is a simplified representation of the more detailed RDF representation of the 2020 Geologic Time Scale (http://resource.geosciml.org/vocabulary/timescale/gts2020).

This representation uses mainly just SKOS model elements to represent the Time Scale as a hierarchical taxonomy of Concepts and does not include the temporal relationships that the more detailed representation does. This version is optimised for simple vocabulary tooling.

This representation of the Time Scale uses the same objects identifiers - IRIs - as the more detailed RDF representation of the Geologic Time Scale and no conflicting data is presented so objects described here may be used interchangeably with the more detailed RDF representation."""@en ;
    skos:hasTopConcept
        :Phanerozoic ,
        :Precambrian ;
    skos:prefLabel "Geologic Time Scale (2020)"@en ;
.
