PREFIX : <https://linked.data.gov.au/def/JORC-Code/>
PREFIX cs: <https://linked.data.gov.au/def/JORC-Code>
PREFIX dcat: <http://www.w3.org/ns/dcat#>
PREFIX dataroles: <https://linked.data.gov.au/def/data-roles/>
PREFIX owl: <http://www.w3.org/2002/07/owl#>
PREFIX prov: <http://www.w3.org/ns/prov#>
PREFIX rdfs: <http://www.w3.org/2000/01/rdf-schema#>
PREFIX reg: <http://purl.org/linked-data/registry#>
PREFIX schema: <https://schema.org/>
PREFIX skos: <http://www.w3.org/2004/02/skos/core#>
PREFIX xsd: <http://www.w3.org/2001/XMLSchema#>
PREFIX theme: <https://linked.data.gov.au/def/gswa-vocabulary-themes/>

:Competent-Person
    a skos:Concept ;
    rdfs:isDefinedBy cs: ;
    skos:closeMatch <https://linked.data.gov.au/def/CRIRSCO-mineral-resource-reporting/Competent-Person> ;
    skos:definition "A ‘Competent Person’ is a minerals industry professional who is a Member or Fellow of The Australasian Institute of Mining and Metallurgy, or of the Australian Institute of Geoscientists, or of a ‘Recognised Professional Organisation’ (RPO), as included in a list available on the JORC and ASX websites. These organisations have enforceable disciplinary processes including the powers to suspend or expel a member. A Competent Person must have a minimum of five years relevant experience in the style of mineralisation or type of deposit under consideration and in the activity which that person is undertaking. If the Competent Person is preparing documentation on Exploration Results, the relevant experience must be in exploration. If the Competent Person is estimating, or supervising the estimation of Mineral Resources, the relevant experience must be in the estimation, assessment and evaluation of Mineral Resources. If the Competent Person is estimating, or supervising the estimation of Ore Reserves, the relevant experience must be in the estimation, assessment, evaluation and economic extraction of Ore Reserves."@en ;
    skos:historyNote "Defined as part of the 2012 JORC Code, the legally binding Australasian Code for Public Reporting of Exploration Results, Mineral Resources and Ore Reserves (https://jorc.org/)" ;
    skos:inScheme cs: ;
    skos:prefLabel "Competent Person"@en ;
    skos:topConceptOf cs: ;
    schema:citation "https://jorc.org/docs/JORC_code_2012.pdf"^^xsd:anyURI ;
.

:Exploration-Results
    a skos:Concept ;
    rdfs:isDefinedBy cs: ;
    skos:closeMatch <https://linked.data.gov.au/def/CRIRSCO-mineral-resource-reporting/Exploration-Results> ;
    skos:definition "Exploration Results include data and information generated by mineral exploration programmes that might be of use to investors but which do not form part of a declaration of Mineral Resources or Ore Reserves."@en ;
    skos:historyNote "Defined as part of the 2012 JORC Code, the legally binding Australasian Code for Public Reporting of Exploration Results, Mineral Resources and Ore Reserves (https://jorc.org/)" ;
    skos:inScheme cs: ;
    skos:prefLabel "Exploration Results"@en ;
    skos:topConceptOf cs: ;
    schema:citation "https://jorc.org/docs/JORC_code_2012.pdf"^^xsd:anyURI ;
.

:Exploration-Target
    a skos:Concept ;
    rdfs:isDefinedBy cs: ;
    skos:closeMatch <https://linked.data.gov.au/def/CRIRSCO-mineral-resource-reporting/Exploration-Target> ;
    skos:definition "An Exploration Target is a statement or estimate of the exploration potential of a mineral deposit in a defined geological setting where the statement or estimate, quoted as a range of tonnes and a range of grade (or quality), relates to mineralisation for which there has been insufficient exploration to estimate a Mineral Resource."@en ;
    skos:historyNote "Defined as part of the 2012 JORC Code, the legally binding Australasian Code for Public Reporting of Exploration Results, Mineral Resources and Ore Reserves (https://jorc.org/)" ;
    skos:inScheme cs: ;
    skos:prefLabel "Exploration Target"@en ;
    skos:topConceptOf cs: ;
    schema:citation "https://jorc.org/docs/JORC_code_2012.pdf"^^xsd:anyURI ;
.

:Feasibility-Study
    a skos:Concept ;
    rdfs:isDefinedBy cs: ;
    skos:closeMatch <https://linked.data.gov.au/def/CRIRSCO-mineral-resource-reporting/Feasibility-Study> ;
    skos:definition "A Feasibility Study is a comprehensive technical and economic study of the selected development option for a mineral project that includes appropriately detailed assessments of applicable Modifying Factors together with any other relevant operational factors and detailed financial analysis that are necessary to demonstrate at the time of reporting that extraction is reasonably justified (economically mineable). The results of the study may reasonably serve as the basis for a final decision by a proponent or financial institution to proceed with, or finance, the development of the project. The confidence level of the study will be higher than that of a Pre-Feasibility Study."@en ;
    skos:historyNote "Defined as part of the 2012 JORC Code, the legally binding Australasian Code for Public Reporting of Exploration Results, Mineral Resources and Ore Reserves (https://jorc.org/)" ;
    skos:inScheme cs: ;
    skos:prefLabel "Feasibility Study"@en ;
    skos:topConceptOf cs: ;
    schema:citation "https://jorc.org/docs/JORC_code_2012.pdf"^^xsd:anyURI ;
.

:Indicated-Mineral-Resource
    a skos:Concept ;
    rdfs:isDefinedBy cs: ;
    skos:closeMatch <https://linked.data.gov.au/def/CRIRSCO-mineral-resource-reporting/Indicated-Resource> ;
    skos:definition "An ‘Indicated Mineral Resource’ is that part of a Mineral Resource for which quantity, grade (or quality), densities, shape and physical characteristics are estimated with sufficient confidence to allow the application of Modifying Factors in sufficient detail to support mine planning and evaluation of the economic viability of the deposit. Geological evidence is derived from adequately detailed and reliable exploration, sampling and testing gathered through appropriate techniques from locations such as outcrops, trenches, pits, workings and drill holes, and is sufficient to assume geological and grade (or quality) continuity between points of observation where data and samples are gathered. An Indicated Mineral Resource has a lower level of confidence than that applying to a Measured Mineral Resource and may only be converted to a Probable Ore Reserve."@en ;
    skos:historyNote "Defined as part of the 2012 JORC Code, the legally binding Australasian Code for Public Reporting of Exploration Results, Mineral Resources and Ore Reserves (https://jorc.org/)" ;
    skos:inScheme cs: ;
    skos:prefLabel "Indicated Mineral Resource"@en ;
    schema:citation "https://jorc.org/docs/JORC_code_2012.pdf"^^xsd:anyURI ;
.

:Inferred-Mineral-Resource
    a skos:Concept ;
    rdfs:isDefinedBy cs: ;
    skos:closeMatch <https://linked.data.gov.au/def/CRIRSCO-mineral-resource-reporting/Inferred-Resource> ;
    skos:definition "An ‘Inferred Mineral Resource’ is that part of a Mineral Resource for which quantity and grade (or quality) are estimated on the basis of limited geological evidence and sampling. Geological evidence is sufficient to imply but not verify geological and grade (or quality) continuity. It is based on exploration, sampling and testing information gathered through appropriate techniques from locations such as outcrops, trenches, pits, workings and drill holes. An Inferred Mineral Resource has a lower level of confidence than that applying to an Indicated Mineral Resource and must not be converted to an Ore Reserve. It is reasonably expected that the majority of Inferred Mineral Resources could be upgraded to Indicated Mineral Resources with continued exploration."@en ;
    skos:historyNote "Defined as part of the 2012 JORC Code, the legally binding Australasian Code for Public Reporting of Exploration Results, Mineral Resources and Ore Reserves (https://jorc.org/)" ;
    skos:inScheme cs: ;
    skos:prefLabel "Inferred Mineral Resource"@en ;
    schema:citation "https://jorc.org/docs/JORC_code_2012.pdf"^^xsd:anyURI ;
.

:Measured-Mineral-Resource
    a skos:Concept ;
    rdfs:isDefinedBy cs: ;
    skos:closeMatch <https://linked.data.gov.au/def/CRIRSCO-mineral-resource-reporting/Measured-Resource> ;
    skos:definition "A ‘Measured Mineral Resource’ is that part of a Mineral Resource for which quantity, grade (or quality), densities, shape, and physical characteristics are estimated with confidence sufficient to allow the application of Modifying Factors to support detailed mine planning and final evaluation of the economic viability of the deposit. Geological evidence is derived from detailed and reliable exploration, sampling and testing gathered through appropriate techniques from locations such as outcrops, trenches, pits, workings and drill holes, and is sufficient to confirm geological and grade (or quality) continuity between points of observation where data and samples are gathered. A Measured Mineral Resource has a higher level of confidence than that applying to either an Indicated Mineral Resource or an Inferred Mineral Resource. It may be converted to a Proved Ore Reserve or under certain circumstances to a Probable Ore Reserve."@en ;
    skos:historyNote "Defined as part of the 2012 JORC Code, the legally binding Australasian Code for Public Reporting of Exploration Results, Mineral Resources and Ore Reserves (https://jorc.org/)" ;
    skos:inScheme cs: ;
    skos:prefLabel "Measured Mineral Resource"@en ;
    schema:citation "https://jorc.org/docs/JORC_code_2012.pdf"^^xsd:anyURI ;
.

:Mineral-Resource
    a skos:Concept ;
    rdfs:isDefinedBy cs: ;
    skos:closeMatch <https://linked.data.gov.au/def/CRIRSCO-mineral-resource-reporting/Mineral-Resource> ;
    skos:definition "A ‘Mineral Resource’ is a concentration or occurrence of solid material of economic interest in or on the Earth’s crust in such form, grade (or quality), and quantity that there are reasonable prospects for eventual economic extraction. The location, quantity, grade (or quality), continuity and other geological characteristics of a Mineral Resource are known, estimated or interpreted from specific geological evidence and knowledge, including sampling. Mineral Resources are subdivided, in order of increasing geological confidence, into Inferred, Indicated and Measured categories."@en ;
    skos:historyNote "Defined as part of the 2012 JORC Code, the legally binding Australasian Code for Public Reporting of Exploration Results, Mineral Resources and Ore Reserves (https://jorc.org/)" ;
    skos:inScheme cs: ;
    skos:narrower
        :Indicated-Mineral-Resource ,
        :Inferred-Mineral-Resource ,
        :Measured-Mineral-Resource ;
    skos:prefLabel "Mineral Resource"@en ;
    skos:topConceptOf cs: ;
    schema:citation "https://jorc.org/docs/JORC_code_2012.pdf"^^xsd:anyURI ;
.

:Modifying-Factors
    a skos:Concept ;
    rdfs:isDefinedBy cs: ;
    skos:closeMatch <https://linked.data.gov.au/def/CRIRSCO-mineral-resource-reporting/Modifying-Factors> ;
    skos:definition "‘Modifying Factors’ are considerations used to convert Mineral Resources to Ore Reserves. These include, but are not restricted to, mining, processing, metallurgical, infrastructure, economic, marketing, legal, environmental, social and governmental factors."@en ;
    skos:historyNote "Defined as part of the 2012 JORC Code, the legally binding Australasian Code for Public Reporting of Exploration Results, Mineral Resources and Ore Reserves (https://jorc.org/)" ;
    skos:inScheme cs: ;
    skos:prefLabel "Modifying Factors"@en ;
    skos:topConceptOf cs: ;
    schema:citation "https://jorc.org/docs/JORC_code_2012.pdf"^^xsd:anyURI ;
.

:Ore-Reserve
    a skos:Concept ;
    rdfs:isDefinedBy cs: ;
    skos:altLabel "Mineral Reserve"@en ;
    skos:closeMatch <https://linked.data.gov.au/def/CRIRSCO-mineral-resource-reporting/Mineral-Reserve> ;
    skos:definition "An ‘Ore Reserve’ is the economically mineable part of a Measured and/or Indicated Mineral Resource. It includes diluting materials and allowances for losses, which may occur when the material is mined or extracted and is defined by studies at Pre-Feasibility or Feasibility level as appropriate that include application of Modifying Factors. Such studies demonstrate that, at the time of reporting, extraction could reasonably be justified. The reference point at which Reserves are defined, usually the point where the ore is delivered to the processing plant, must be stated. It is important that, in all situations where the reference point is different, such as for a saleable product, a clarifying statement is included to ensure that the reader is fully informed as to what is being reported."@en ;
    skos:historyNote "Defined as part of the 2012 JORC Code, the legally binding Australasian Code for Public Reporting of Exploration Results, Mineral Resources and Ore Reserves (https://jorc.org/)" ;
    skos:inScheme cs: ;
    skos:narrower
        :Probable-Ore-Reserve ,
        :Proved-Ore-Reserve ;
    skos:prefLabel "Ore Reserve"@en ;
    skos:topConceptOf cs: ;
    schema:citation "https://jorc.org/docs/JORC_code_2012.pdf"^^xsd:anyURI ;
.

:Pre-Feasibility-Study
    a skos:Concept ;
    rdfs:isDefinedBy cs: ;
    skos:closeMatch <https://linked.data.gov.au/def/CRIRSCO-mineral-resource-reporting/Pre-Feasibility-Study> ;
    skos:definition "A Preliminary Feasibility Study (Pre-Feasibility Study) is a comprehensive study of a range of options for the technical and economic viability of a mineral project that has advanced to a stage where a preferred mining method, in the case of underground mining, or the pit configuration, in the case of an open pit, is established and an effective method of mineral processing is determined. It includes a financial analysis based on reasonable assumptions on the Modifying Factors and the evaluation of any other relevant factors which are sufficient for a Competent Person, acting reasonably, to determine if all or part of the Mineral Resources may be converted to an Ore Reserve at the time of reporting. A Pre-Feasibility Study is at a lower confidence level than a Feasibility Study."@en ;
    skos:historyNote "Defined as part of the 2012 JORC Code, the legally binding Australasian Code for Public Reporting of Exploration Results, Mineral Resources and Ore Reserves (https://jorc.org/)" ;
    skos:inScheme cs: ;
    skos:prefLabel "Pre-Feasibility Study"@en ;
    skos:topConceptOf cs: ;
    schema:citation "https://jorc.org/docs/JORC_code_2012.pdf"^^xsd:anyURI ;
.

:Probable-Ore-Reserve
    a skos:Concept ;
    rdfs:isDefinedBy cs: ;
    skos:closeMatch <https://linked.data.gov.au/def/CRIRSCO-mineral-resource-reporting/Probable-Reserve> ;
    skos:definition "A ‘Probable Ore Reserve’ is the economically mineable part of an Indicated, and in some circumstances, a Measured Mineral Resource. The confidence in the Modifying Factors applying to a Probable Ore Reserve is lower than that applying to a Proved Ore Reserve."@en ;
    skos:historyNote "Defined as part of the 2012 JORC Code, the legally binding Australasian Code for Public Reporting of Exploration Results, Mineral Resources and Ore Reserves (https://jorc.org/)" ;
    skos:inScheme cs: ;
    skos:prefLabel "Probable Ore Reserve"@en ;
    schema:citation "https://jorc.org/docs/JORC_code_2012.pdf"^^xsd:anyURI ;
.

:Proved-Ore-Reserve
    a skos:Concept ;
    rdfs:isDefinedBy cs: ;
    skos:closeMatch <https://linked.data.gov.au/def/CRIRSCO-mineral-resource-reporting/Proved-Reserve> ;
    skos:definition "A ‘Proved Ore Reserve’ is the economically mineable part of a Measured Mineral Resource. A Proved Ore Reserve implies a high degree of confidence in the Modifying Factors."@en ;
    skos:historyNote "Defined as part of the 2012 JORC Code, the legally binding Australasian Code for Public Reporting of Exploration Results, Mineral Resources and Ore Reserves (https://jorc.org/)" ;
    skos:inScheme cs: ;
    skos:prefLabel "Proved Ore Reserve"@en ;
    schema:citation "https://jorc.org/docs/JORC_code_2012.pdf"^^xsd:anyURI ;
.

:Public-reports
    a skos:Concept ;
    rdfs:isDefinedBy cs: ;
    skos:closeMatch <https://linked.data.gov.au/def/CRIRSCO-mineral-resource-reporting/Public-reports> ;
    skos:definition "Public Reports are reports prepared for the purpose of informing investors or potential investors and their advisers on Exploration Results, Mineral Resources or Ore Reserves. They include, but are not limited to, annual and quarterly company reports, press releases, information memoranda, technical papers, website postings and public presentations."@en ;
    skos:historyNote "Defined as part of the 2012 JORC Code, the legally binding Australasian Code for Public Reporting of Exploration Results, Mineral Resources and Ore Reserves (https://jorc.org/)" ;
    skos:inScheme cs: ;
    skos:prefLabel "Public reports"@en ;
    skos:topConceptOf cs: ;
    schema:citation "https://jorc.org/docs/JORC_code_2012.pdf"^^xsd:anyURI ;
.

:Scoping-Study
    a skos:Concept ;
    rdfs:isDefinedBy cs: ;
    skos:closeMatch <https://linked.data.gov.au/def/CRIRSCO-mineral-resource-reporting/Scoping-Study> ;
    skos:definition "A Scoping Study is an order of magnitude technical and economic study of the potential viability of Mineral Resources. It includes appropriate assessments of realistically assumed Modifying Factors together with any other relevant operational factors that are necessary to demonstrate at the time of reporting that progress to a Pre-Feasibility Study can be reasonably justified."@en ;
    skos:historyNote "Defined as part of the 2012 JORC Code, the legally binding Australasian Code for Public Reporting of Exploration Results, Mineral Resources and Ore Reserves (https://jorc.org/)" ;
    skos:inScheme cs: ;
    skos:prefLabel "Scoping Study"@en ;
    skos:topConceptOf cs: ;
    schema:citation "https://jorc.org/docs/JORC_code_2012.pdf"^^xsd:anyURI ;
.

<https://linked.data.gov.au/org/gswa>
    a schema:Organization ;
    schema:name "Geological Survey of Western Australia" ;
    schema:url "https://www.dmp.wa.gov.au/Geological-Survey/Geological-Survey-262.aspx"^^xsd:anyURI ;
.

:1.1 schema:name "1.1" .

cs:
    a skos:ConceptScheme ;
    owl:versionIRI :1.1 ;
    reg:status <https://linked.data.gov.au/def/reg-statuses/accepted> ;
    skos:definition "The Australasian Code for Reporting of Exploration Results, Mineral Resources and Ore Reserves ('the JORC Code') is a professional code of practice that sets mandatory, minimum standards for Public Reporting of minerals Exploration Results, Mineral Resources and Ore Reserves, according to the levels of confidence in geological knowledge and technical and economic considerations. The JORC Code is prepared by the Joint Ore Reserves Committee of the Australasian Institute of Mining and Metallurgy, the Australian Institute of Geoscientists and the Minerals Council of Australia as in force from time to time (JORC; https://jorc.org/) and was last updated in 2012 (https://jorc.org/docs/JORC_code_2012.pdf). The JORC Committee was established in 1971, and is sponsored by the Australian mining industry and its professional organisations. The JORC Committee is a member of CRIRSCO, the Committee for Mineral Reserves International Reporting Standards (CRIRSCO; https://www.crirsco.com/)."@en ;
    skos:hasTopConcept
        :Competent-Person ,
        :Exploration-Results ,
        :Exploration-Target ,
        :Feasibility-Study ,
        :Mineral-Resource ,
        :Modifying-Factors ,
        :Ore-Reserve ,
        :Pre-Feasibility-Study ,
        :Public-reports ,
        :Scoping-Study ;
    skos:historyNote """The Mines and Mineral Deposits (MINEDEX) system maintained by the Geological Survey of Western Australia requires exploration and mining companies operating in the State to submit Resource information based on the JORC or equivalent Codes. As of May 2023, the Mining Act 1978 requires submissions to be compliant with the 2004 JORC Code; the 2012 version of the JORC Code (https://jorc.org/docs/JORC_code_2012.pdf) is covered in this vocabulary and there are no term differences between the two.

The JORC Code vocabulary covers [MINEDEX].[ResourceEstimate.ResourceCategory], i.e. resource or reserve, and [MINEDEX].[ResourceEstimate.ResourceStatus], i.e. the status of resource/reserve (e.g. inferred, measured)."""@en ;
    skos:prefLabel "JORC Code"@en ;
    prov:qualifiedAttribution
        [
            dcat:hadRole dataroles:custodian ;
            prov:agent
                [
                    a schema:Person ;
                    schema:email ""^^xsd:anyURI ;
                    schema:name "Angela Riganti" ;
                ] ;
        ] ,
        [
            dcat:hadRole dataroles:custodian ;
            prov:agent
                [
                    a schema:Person ;
                    schema:email ""^^xsd:anyURI ;
                    schema:name "Erin Gray" ;
                ] ;
        ] ;
    schema:creator <https://linked.data.gov.au/org/gswa> ;
    schema:dateCreated "2023-11-01"^^xsd:date ;
    schema:dateModified "2023-12-04"^^xsd:date ;
    schema:publisher <https://linked.data.gov.au/org/gswa> ;
    schema:version "1.1: updated IRI to use lowercase characters" ;
    schema:keywords
        theme:resources-mineral ,
        theme:legislation ;
.
