PREFIX : <https://linked.data.gov.au/def/metamorphic-stage/>
PREFIX astatus: <https://linked.data.gov.au/def/reg-statuses/>
PREFIX cs: <https://linked.data.gov.au/def/metamorphic-stage>
PREFIX dataroles: <https://linked.data.gov.au/def/data-roles/>
PREFIX owl: <http://www.w3.org/2002/07/owl#>
PREFIX prov: <http://www.w3.org/ns/prov#>
PREFIX rdfs: <http://www.w3.org/2000/01/rdf-schema#>
PREFIX reg: <http://purl.org/linked-data/registry#>
PREFIX schema: <https://schema.org/>
PREFIX skos: <http://www.w3.org/2004/02/skos/core#>
PREFIX themes: <https://linked.data.gov.au/def/gswa-vocabulary-themes/>
PREFIX xsd: <http://www.w3.org/2001/XMLSchema#>

<https://linked.data.gov.au/def/metamorphic-stage/?peak>
    a skos:Concept ;
    rdfs:isDefinedBy cs: ;
    skos:definition "Typically reserved for use when: a) overprinting or unclear spatial–textural relationships do not allow discernment of whether all or some of the minerals preserved in the rock are indicative of the highest temperature equilibrium mineral assemblage; or b) the possibility of polymetamorphism is likely. This ambiguity arises, for example, when sluggish reaction kinetics in porphyroblastic minerals at low to moderate pressure/temperature metamorphic conditions lead to metastability."@en ;
    skos:inScheme cs: ;
    skos:prefLabel "?peak"@en ;
    skos:topConceptOf cs: ;
.

<https://linked.data.gov.au/def/metamorphic-stage/?prograde>
    a skos:Concept ;
    rdfs:isDefinedBy cs: ;
    skos:definition "The mineral assemblage of the rock is tentatively interpreted to represent a (relict) prograde mineral assemblage. This term is used when metamorphic information is cryptically preserved, e.g. within inclusions in porphyroblastic minerals, or there is ambiguity about polymetamorphism."@en ;
    skos:inScheme cs: ;
    skos:prefLabel "?prograde"@en ;
    skos:topConceptOf cs: ;
.

<https://linked.data.gov.au/def/metamorphic-stage/?retrograde>
    a skos:Concept ;
    rdfs:isDefinedBy cs: ;
    skos:altLabel "?retrogressive"@en ;
    skos:definition "The mineral assemblage of the rock is tentatively interpreted to represent a (relict) retrograde mineral assemblage. Typically used when the possibility of polymetamorphism is high and/or unclear, i.e. when it cannot be ascertained whether lower temperature metamorphic minerals overprinting a higher grade assemblage formed during the same, single metamorphic cycle, or whether a later, lower temperature event (i.e. retrogressive) overprinted the higher grade assemblage."@en ;
    skos:inScheme cs: ;
    skos:prefLabel "?retrograde"@en ;
    skos:topConceptOf cs: ;
.

:peak
    a skos:Concept ;
    schema:citation
        "244p."^^xsd:anyURI ,
        "Adapted from:"^^xsd:anyURI ,
        "D and Desmons"^^xsd:anyURI ,
        "Fettes"^^xsd:anyURI ,
        "J (eds.) 2007"^^xsd:anyURI ,
        "Metamorphic Rocks: a classification and glossary of terms — Recommendations of the International Union of Geological Sciences Subcommission on the Systematics of Metamorphic Rocks: Cambridge University Press"^^xsd:anyURI ;
    rdfs:isDefinedBy cs: ;
    skos:definition "Metamorphic conditions taken to be the thermal maximum reached during a metamorphic cycle or evolution, regardless of the P–T trajectory."@en ;
    skos:inScheme cs: ;
    skos:prefLabel "peak"@en ;
    skos:topConceptOf cs: ;
.

:prograde
    a skos:Concept ;
    schema:citation
        "244p."^^xsd:anyURI ,
        "Adapted from:"^^xsd:anyURI ,
        "D and Desmons"^^xsd:anyURI ,
        "Fettes"^^xsd:anyURI ,
        "J (eds.) 2007"^^xsd:anyURI ,
        "Metamorphic Rocks: a classification and glossary of terms — Recommendations of the International Union of Geological Sciences Subcommission on the Systematics of Metamorphic Rocks: Cambridge University Press"^^xsd:anyURI ;
    rdfs:isDefinedBy cs: ;
    skos:definition "Metamorphism giving rise to the formation of minerals that are typical of a higher metamorphic grade, i.e. higher temperature, than the former mineral assemblage. That is, a sequential increase in metamorphic grade with time (within a single metamorphic event) that is recognizable or inferred in a rock. It is that part of the metamorphic cycle up to the thermal maximum (peak metamorphic conditions)."@en ;
    skos:inScheme cs: ;
    skos:prefLabel "prograde"@en ;
    skos:topConceptOf cs: ;
.

:retrograde
    a skos:Concept ;
    schema:citation
        "244p."^^xsd:anyURI ,
        "Adapted from:"^^xsd:anyURI ,
        "D and Desmons"^^xsd:anyURI ,
        "Fettes"^^xsd:anyURI ,
        "J (eds.) 2007"^^xsd:anyURI ,
        "Metamorphic Rocks: a classification and glossary of terms — Recommendations of the International Union of Geological Sciences Subcommission on the Systematics of Metamorphic Rocks: Cambridge University Press"^^xsd:anyURI ;
    rdfs:isDefinedBy cs: ;
    skos:definition "Metamorphism giving rise to the formation of minerals that are typical of a lower grade, i.e. lower temperature, than the former mineral assemblage. That is, a sequential decrease in metamorphic grade with time (within a single metamorphic event) that is recognizable or inferred in a rock. It is that part of the metamorphic cycle after the thermal maximum (or peak metamorphic conditions) has been reached."@en ;
    skos:inScheme cs: ;
    skos:prefLabel "retrograde"@en ;
    skos:topConceptOf cs: ;
.

:retrogressive
    a skos:Concept ;
    schema:citation
        "244p."^^xsd:anyURI ,
        "Adapted from:"^^xsd:anyURI ,
        "D and Desmons"^^xsd:anyURI ,
        "Fettes"^^xsd:anyURI ,
        "J (eds.) 2007"^^xsd:anyURI ,
        "Metamorphic Rocks: a classification and glossary of terms — Recommendations of the International Union of Geological Sciences Subcommission on the Systematics of Metamorphic Rocks: Cambridge University Press"^^xsd:anyURI ;
    rdfs:isDefinedBy cs: ;
    skos:definition "Metamorphism giving rise to the formation of minerals that are typical of a lower grade, i.e. lower temperature, than the former mineral assemblage. It is distinguished from retrograde metamorphism by the fact that the development of a lower grade mineral assemblage is ascribed to a separate, discrete metamorphic event that takes place at lower temperatures and a later time than the first metamorphic event."@en ;
    skos:inScheme cs: ;
    skos:prefLabel "retrogressive"@en ;
    skos:topConceptOf cs: ;
.

:unknown
    a skos:Concept ;
    rdfs:isDefinedBy cs: ;
    skos:definition "It is not clear what stage of the metamorphic evolution the minerals in the rock represent, usually because of poor preservation of metamorphic minerals due to excessive alteration or weathering, or due to ambiguous mineralogical relationships that are suggestive of polymetamorphism."@en ;
    skos:inScheme cs: ;
    skos:prefLabel "unknown"@en ;
    skos:topConceptOf cs: ;
.

:1 rdfs:label "1" .

cs:
    a skos:ConceptScheme ;
    schema:dateCreated "2023-11-01"^^xsd:date ;
    schema:creator <https://linked.data.gov.au/org/gswa> ;
    schema:dateModified "2023-11-01"^^xsd:date ;
    schema:publisher <https://linked.data.gov.au/org/gswa> ;
    owl:versionIRI :1 ;
    owl:versionInfo "1" ;
    reg:status astatus:stable ;
    skos:definition """Terms used to describe the stage of metamorphism of rocks based on the nature of the change in pressure and temperature conditions to which the rocks are subjected. Definitions are taken or derived from:
Fettes, D and Desmons, J (eds.) 2007, Metamorphic Rocks: a classification and glossary of terms — Recommendations of the International Union of Geological Sciences Subcommission on the Systematics of Metamorphic Rocks: Cambridge University Press, 244p."""@en ;
    skos:hasTopConcept
        <https://linked.data.gov.au/def/metamorphic-stage/?peak> ,
        <https://linked.data.gov.au/def/metamorphic-stage/?prograde> ,
        <https://linked.data.gov.au/def/metamorphic-stage/?retrograde> ,
        :peak ,
        :prograde ,
        :retrograde ,
        :retrogressive ,
        :unknown ;
    skos:historyNote "Based on the authoritative lists [GEOLOGY].[WAROX_REF].[MetaStage] and [WAGIMS].[ReferenceData].[MetamorphicStage] used in the Geological Survey of Western Australia's field observations (WAROX) and WAGIMS system, the repository for Western Australian geochronology, isotope geology, mineral chemistry and metamorphic history analytical data and information."@en ;
    skos:prefLabel "Metamorphic stage"@en ;
    schema:keywords
        themes:geology ;
    prov:qualifiedAttribution
        [
            prov:hadRole dataroles:custodian ;
            prov:agent <https://orcid.org/0009-0003-0007-8342> ;
        ] ,
        [
            prov:hadRole dataroles:custodian ;
            prov:agent <https://www.linkedin.com/in/david-kelsey-425746137/> ;
        ] ;
.

