PREFIX : <https://linked.data.gov.au/def/wa-coordinate-reference-systems/>
PREFIX agldwgstatus: <https://linked.data.gov.au/def/reg-statuses/>
PREFIX cs: <https://linked.data.gov.au/def/wa-coordinate-reference-systems>
PREFIX dcat: <http://www.w3.org/ns/dcat#>
PREFIX dcterms: <http://purl.org/dc/terms/>
PREFIX dataroles: <https://linked.data.gov.au/def/data-roles/>
PREFIX owl: <http://www.w3.org/2002/07/owl#>
PREFIX prov: <http://www.w3.org/ns/prov#>
PREFIX rdfs: <http://www.w3.org/2000/01/rdf-schema#>
PREFIX reg: <http://purl.org/linked-data/registry#>
PREFIX schema: <https://schema.org/>
PREFIX skos: <http://www.w3.org/2004/02/skos/core#>
PREFIX xsd: <http://www.w3.org/2001/XMLSchema#>
PREFIX theme: <https://linked.data.gov.au/def/gswa-vocabulary-themes/>


:geographic
    a skos:Collection ;
    skos:definition "A geographic coordinate system (GCS) is a coordinate system that uses a three-dimensional (spherical or ellipsoidal) surface  to define locations on the Earth. Any location on Earth can be referenced by a point with longitude and latitude coordinates."@en ;
    skos:historyNote "Includes geographic coordinate systems used in Western Australia" ;
    skos:inScheme cs: ;
    rdfs:isDefinedBy cs: ;
    skos:member
        :Clarke1858 ,
        :agd66 ,
        :agd84 ,
        :gda2020 ,
        :gda94 ,
        :wgs84 ;
    skos:prefLabel "Geographic coordinate systems"@en ;
.

:projected
    a skos:Collection ;
    skos:definition "Projected coordinate systems that apply to the State of Western Australia. A projected coordinate system (PCS) is a projection of the geographic coordinates on a flat, two-dimensional surface (a map). The projection currently used to convert between Australian Geodetic Data and their projected equivalents is the Universal Transverse Mercator (UTM) projection. Unlike ageographic coordinate system, a projected coordinate system has constant lengths, angles and areas across the two dimensions. In a projected coordinate system, locations are identified by x, y coordinates on a grid, with the origin at the centre of the grid. Each position has two values that reference it to that central location. One specifies its horizontal position and the other its vertical position. The two values are called the x-coordinate and y-coordinate. Using this notation, the coordinates at the origin are x = 0 and y = 0."@en ;
    skos:historyNote "Compiled by GSWA to group projected coordinate systems that apply to the State of Western Australia." ;
    skos:inScheme cs: ;
    rdfs:isDefinedBy cs: ;
    skos:member
        :amg66 ,
        :amg66-z49 ,
        :amg66-z50 ,
        :amg66-z51 ,
        :amg66-z52 ,
        :amg84 ,
        :amg84-z49 ,
        :amg84-z50 ,
        :amg84-z51 ,
        :amg84-z52 ,
        :mga2020 ,
        :mga2020-z49 ,
        :mga2020-z50 ,
        :mga2020-z51 ,
        :mga2020-z52 ,
        :mga94 ,
        :mga94-z49 ,
        :mga94-z50 ,
        :mga94-z51 ,
        :mga94-z52 ,
        :wgs84-utm-z49s ,
        :wgs84-utm-z50s ,
        :wgs84-utm-z51s ,
        :wgs84-utm-z52s ;
    skos:prefLabel "Projected coordinate systems"@en ;
.

:wa-utm-zones
    a skos:Collection ;
    skos:definition "The Universal Transverse Mercator (UTM) zones used and referred to within Western Australia. The UTM system divides the Earth into 60 zones, each 6°  longitude in width. Zone 1 covers longitudes 180–174°W; zone numbering increases eastward to zone 60, which covers longitudes 174–180°E. The polar regions south of 80°S and north of 84°N are excluded."@en ;
    skos:historyNote "Compiled by GSWA to group UTM zones that apply to the State of Western Australia." ;
    skos:inScheme cs: ;
    rdfs:isDefinedBy cs: ;
    skos:member
        :utm-z49 ,
        :utm-z50 ,
        :utm-z51 ,
        :utm-z52 ;
    skos:prefLabel "Western Australian UTM zones"@en ;
.

:Clarke1858-z1
    a skos:Concept ;
    skos:altLabel "Clarke 1858 z1"@en ;
    skos:definition "Zone 1 of the Clarke 1858 geodatum, extending from longitudes 113.5°E to 118.5°E."@en ;
    skos:inScheme cs: ;
    skos:prefLabel "Clarke 1858 zone 1"@en ;
.

:Clarke1858-z2
    a skos:Concept ;
    skos:altLabel "Clarke 1858 z2"@en ;
    skos:definition "Zone 2 of the Clarke 1858 geodatum, extending from longitudes 118.5°E to 123.5°E."@en ;
    skos:inScheme cs: ;
    skos:prefLabel "Clarke 1858 zone 2"@en ;
.

:Clarke1858-z3
    a skos:Concept ;
    skos:altLabel "Clarke 1858 z3"@en ;
    skos:definition "Zone 3 of the Clarke 1858 geodatum, extending from longitudes 123.5°E to 128.5°E."@en ;
    skos:inScheme cs: ;
    skos:prefLabel "Clarke 1858 zone 3"@en ;
.

:Clarke1858-z4
    a skos:Concept ;
    skos:altLabel "Clarke 1858 z4"@en ;
    skos:definition "Zone 4 of the Clarke 1858 geodatum, extending from longitudes 128.5°E to 133.5°E."@en ;
    skos:inScheme cs: ;
    skos:prefLabel "Clarke 1858 zone 4"@en ;
.

:local-grid
    a skos:Concept ;
    dcterms:source
        "https://www.propelleraero.com/blog/local-grid-propeller-help-deliver-site-data-local-coordinates/"^^xsd:anyURI ,
        "https://www.propelleraero.com/blog/using-local-grid-coordinates-on-surveys-with-propeller/"^^xsd:anyURI ;
    skos:definition "A local grid is a locally defined coordinate reference system, typically used during mineral exploration. Local grids measure positions relative to an arbitrary, fixed point (usually a GPS base station) on the site/area where the activity is conducted, instead of using a national or global datum."@en ;
    skos:historyNote "Local grids are routinely used in mineral exploration, e.g. when establishing drilling or surface sampling lines. Many legacy maps submitted in legacy exploration reports use local grids (with or without the coordinates of the reference point). It is considered this may be a useful concept for when individual maps may be able to be retrieved from WAMEX." ;
    skos:inScheme cs: ;
    skos:narrower
        :local-grid-base-station-known ,
        :local-grid-base-station-unknown ;
    skos:prefLabel "local grid"@en ;
    skos:topConceptOf cs: ;
.

:local-grid-base-station-known
    a skos:Concept ;
    skos:definition "Locally defined coordinate reference systems, typically used during mineral exploration. Local grids measure positions relative to an arbitrary point (usually a GPS base station) on the site/area where the activity is conducted. The coordinates of the base station point are known."@en ;
    skos:inScheme cs: ;
    skos:prefLabel "local grid, base station known"@en ;
.

:local-grid-base-station-unknown
    a skos:Concept ;
    skos:definition "Locally defined coordinate reference system, typically used during mineral exploration. Local grids measure positions relative to an arbitrary point (usually a GPS base station) on the site/area where the activity is conducted. The coordinates of the base station point are not known."@en ;
    skos:inScheme cs: ;
    skos:prefLabel "local grid, base station unknown"@en ;
.

:unknown
    a skos:Concept ;
    skos:definition "The coordinate reference system is not known or specified."@en ;
    skos:inScheme cs: ;
    skos:prefLabel "unknown"@en ;
    skos:topConceptOf cs: ;
.

:utm
    a skos:Concept ;
    dcterms:source
        "https://en.wikipedia.org/wiki/Universal_Transverse_Mercator_coordinate_system"^^xsd:anyURI ,
        "https://www.icsm.gov.au/education/fundamentals-mapping/projections/commonly-used-map-projections#UTM"^^xsd:anyURI ;
    skos:altLabel "UTM"@en ;
    skos:definition "The Universal Transverse Mercator coordinate system (usually simply called UTM) is a map projection system (not a projection) designed to assign coordinates to locations on the surface of the Earth. It divides the Earth into 60 zones, each 6° of longitude in width. These longitudinal zones are numbered 1 to 60 – east from longitude 180°; the polar regions south of 80°S and north of 84°N are excluded. Each zone is characterized by a central meridian; as a result, within a zone nothing is more than 3° from the central meridian and therefore locations, shapes and sizes and directions between all features are very accurate. The UTM sometimes also uses 20 latitude bands, each 8° high, numbered A to Z (with O and I not being used) – north from Antarctica. The UTM was developed in 1947 by the North Atlantic Treaty Organisation (NATO)."@en ;
    skos:inScheme cs: ;
    skos:narrower
        :utm-z49 ,
        :utm-z50 ,
        :utm-z51 ,
        :utm-z52 ;
    skos:prefLabel "Universal Transverse Mercator System"@en ;
    skos:topConceptOf cs: ;
.

:Clarke1858
    a skos:Concept ;
    dcterms:source "https://epsg.io/7007-ellipsoid"^^xsd:anyURI ;
    skos:definition "Between 1858 and 1966, geodetic surveys in Australia were computed on either a jurisdiction (state or territory) or regional basis using more than four different spheroids and as many as twenty coordinate origins. In Western Australia, the most widely used geodatum and ellipsoid since 1945 was the Clarke 1858; the State was covered by four separate longitudinal zones, numbered 1 (one) to 4 (four), each with a 5° longitude width."@en ;
    skos:historyNote """Linked Document: GS83 - Clarke 1858 projection - 000216.john.kirk.docx (Departmental Use Only)
GSWA has 42 Clarke 1:250k maps out of 163; these were converted in 2013, but hardcopies and scans still preserve the old datum. Northampton 50k series also used Clarke 1858.
Note EPGS registry""" ;
    skos:inScheme cs: ;
    skos:narrower
        :Clarke1858-z1 ,
        :Clarke1858-z2 ,
        :Clarke1858-z3 ,
        :Clarke1858-z4 ;
    skos:prefLabel "Clarke 1858"@en ;
    skos:topConceptOf cs: ;
.

:agd66
    a skos:Concept ;
    dcterms:source
        "http://linked.data.gov.au/def/queensland-crs/agd1966"^^xsd:anyURI ,
        "https://epsg.io/4202"^^xsd:anyURI ,
        "https://www.icsm.gov.au/datum/australian-geodetic-datum-196684-agd"^^xsd:anyURI ,
        "https://www.icsm.gov.au/sites/default/files/The%20Australian%20Map%20Grid%20Technical%20Manual%20-%20Second%20Edition%201972.pdf"^^xsd:anyURI ;
    skos:altLabel
        "AGC 1966"@en ,
        "AGD_1966"@en ,
        "Australian Geodetic Datum 1966"@en ;
    skos:definition "The first official national Australian Geodetic Datum (AGD), proclaimed in the Australian Commonwealth Gazette No. 84 of 6 October 1966. Area of use: Australia onshore and offshore, and Papua New Guinea onshore."@en ;
    skos:exactMatch <https://linked.data.gov.au/def/queensland-crs/agd1966> ;
    skos:inScheme cs: ;
    skos:notation
        "EPSG:4202"^^<https://epsg.io/> ,
        "https://epsg.io/4202"^^<https://epsg.io/> ;
    skos:prefLabel "AGD66"@en ;
    skos:topConceptOf cs: ;
.

:agd84
    a skos:Concept ;
    dcterms:source
        "http://linked.data.gov.au/def/queensland-crs/agd1984"^^xsd:anyURI ,
        "https://epsg.io/4203"^^xsd:anyURI ,
        "https://www.icsm.gov.au/datum/australian-geodetic-datum-196684-agd"^^xsd:anyURI ;
    skos:altLabel
        "AGD 1984"@en ,
        "AGD_1984"@en ,
        "Australian Geodetic Datum 1984"@en ;
    skos:definition "An update to the official Australian Geodetic Datum (AGD), adopted and in effect from 1984. The AGD84 national system replaced AGD66 but was officially adopted only in Queensland, South Australia and Western Australia; it was later replaced by GDA94. Area of use: Australia – Queensland, South Australia, Western Australia, federal areas offshore west of 129°E."@en ;
    skos:exactMatch <https://linked.data.gov.au/def/queensland-crs/agd1984> ;
    skos:inScheme cs: ;
    skos:notation
        "EPSG:4203"^^<https://epsg.io/> ,
        "https://epsg.io/4203"^^<https://epsg.io/> ;
    skos:prefLabel "AGD84"@en ;
    skos:topConceptOf cs: ;
.

:amg66
    a skos:Concept ;
    dcterms:source "https://www.icsm.gov.au/sites/default/files/The%20Australian%20Map%20Grid%20Technical%20Manual%20-%20Second%20Edition%201972.pdf"^^xsd:anyURI ;
    skos:altLabel
        "AMG 66"@en ,
        "AMG_66"@en ,
        "Australian Map Grid 1966"@en ;
    skos:definition "The Australian national map projection accompanying AGD66. The Australian Map Grid (AMG) is derived from a transverse Mercator projection of latitudes and longitudes on the Australian Geodetic Datum (AGD66). The AMG corresponds with the Universal Transverse Mercator (UTM) grid, with a system of rectangular grid coordinates (eastings and northings) expressed in metres. AMG zones are numbered from zone 47 (with central meridian 99°E) to zone 58 (with central meridian 165°E). Each zone is 6° wide with a half degree of overlapping."@en ;
    skos:inScheme cs: ;
    skos:narrower
        :amg66-z49 ,
        :amg66-z50 ,
        :amg66-z51 ,
        :amg66-z52 ;
    skos:prefLabel "AMG66"@en ;
    skos:topConceptOf cs: ;
.

:amg66-z49
    a skos:Concept ;
    dcterms:source "https://epsg.io/20249"^^xsd:anyURI ;
    skos:altLabel
        "AMG66 z49"@en ,
        "AMG66 zone 49"@en ,
        "Australian Map Grid 1966 z49"@en ,
        "Australian Map Grid 1966 zone 49"@en ;
    skos:definition "The accompanying national map projection to AGD66, a transverse Mercator projection that conforms to zone 49 of the internationally accepted Universal Transverse Mercator (UTM) grid system. Area of use for AMG66 zone 49: Australia – onshore and offshore to 200 nautical mile EEZ (Exclusive Economic Zone) boundary between 108°E and 114°E."@en ;
    skos:inScheme cs: ;
    skos:notation
        "EPSG:20249"^^<https://epsg.io/> ,
        "https://epsg.io/20249"^^<https://epsg.io/> ;
    skos:prefLabel "AGD66 / AMG zone 49"@en ;
.

:amg66-z50
    a skos:Concept ;
    dcterms:source "https://epsg.io/20250"^^xsd:anyURI ;
    skos:altLabel
        "AMG66 z50"@en ,
        "AMG66 zone 50"@en ,
        "Australian Map Grid 1966 z50"@en ,
        "Australian Map Grid 1966 zone 50"@en ;
    skos:definition "The accompanying national map projection to AGD66, a transverse Mercator projection that conforms to zone 50 of the internationally accepted Universal Transverse Mercator (UTM) grid system. Area of use for AMG66 zone 50: onshore and offshore to 200 nautical mile EEZ (Exclusive Economic Zone) boundary between 114°E and 120°E."@en ;
    skos:inScheme cs: ;
    skos:notation
        "EPSG:20250"^^<https://epsg.io/> ,
        "https://epsg.io/20250"^^<https://epsg.io/> ;
    skos:prefLabel "AGD66 / AMG zone 50"@en ;
.

:amg66-z51
    a skos:Concept ;
    dcterms:source "https://epsg.io/20251"^^xsd:anyURI ;
    skos:altLabel
        "AMG66 z51"@en ,
        "AMG66 zone 51"@en ,
        "Australian Map Grid 1966 z51"@en ,
        "Australian Map Grid 1966 zone 51"@en ;
    skos:definition "The accompanying national map projection to AGD66, a transverse Mercator projection that conforms to zone 51 of the internationally accepted Universal Transverse Mercator (UTM) grid system. Area of use for AMG66 zone 52: Australia – onshore and offshore between 120°E and 126°E."@en ;
    skos:inScheme cs: ;
    skos:notation
        "EPSG:20251"^^<https://epsg.io/> ,
        "https://epsg.io/20251"^^<https://epsg.io/> ;
    skos:prefLabel "AGD66 / AMG zone 51"@en ;
.

:amg66-z52
    a skos:Concept ;
    dcterms:source "https://epsg.io/20252"^^xsd:anyURI ;
    skos:altLabel
        "AMG66 z52"@en ,
        "AMG66 zone 52"@en ,
        "Australian Map Grid 1966 z52"@en ,
        "Australian Map Grid 1966 zone 52"@en ;
    skos:definition "The accompanying national map projection to AGD66, a transverse Mercator projection that conforms to zone 52 of the internationally accepted Universal Transverse Mercator (UTM) grid system. Area of use for AMG66 zone 52: Australia – onshore and offshore between 126°E and 132°E."@en ;
    skos:inScheme cs: ;
    skos:notation
        "EPSG:20252"^^<https://epsg.io/> ,
        "https://epsg.io/20252"^^<https://epsg.io/> ;
    skos:prefLabel "AGD66 / AMG zone 52"@en ;
.

:amg84
    a skos:Concept ;
    dcterms:source "https://www.icsm.gov.au/sites/default/files/The%20Australian%20Map%20Grid%20Technical%20Manual%20-%20Second%20Edition%201972.pdf"^^xsd:anyURI ;
    skos:altLabel
        "AMG 84"@en ,
        "AMG_84"@en ,
        "Australian Map Grid 1984"@en ;
    skos:definition "The Australian national map projection accompanying AGD84. The Australian Map Grid (AMG) is derived from a transverse Mercator projection of latitudes and longitudes on the Australian Geodetic Datum (AGD84). The AMG corresponds with the Universal Transverse Mercator (UTM) grid, with a system of rectangular grid coordinates (eastings and northings) expressed in metres. AMG zones are numbered from zone 47 (with central meridian 99°E) to zone 58 (with central meridian 165°E). Each zone is 6° wide with a half degree of overlapping."@en ;
    skos:inScheme cs: ;
    skos:narrower
        :amg84-z49 ,
        :amg84-z50 ,
        :amg84-z51 ,
        :amg84-z52 ;
    skos:prefLabel "AMG84"@en ;
    skos:topConceptOf cs: ;
.

:amg84-z49
    a skos:Concept ;
    dcterms:source "https://epsg.io/20349"^^xsd:anyURI ;
    skos:altLabel
        "AMG84 z49"@en ,
        "AMG84 zone 49"@en ,
        "Australian Map Grid 1984 z49"@en ,
        "Australian Map Grid 1984 zone 49"@en ;
    skos:definition "The accompanying national map projection to AGD84, a transverse Mercator projection that conforms to zone 49 of the internationally accepted Universal Transverse Mercator (UTM) grid system. Area of use for AMG84 zone 49: Australia – onshore and offshore to 200 nautical mile EEZ (Exclusive Economic Zone) boundary between 108°E and 114°E."@en ;
    skos:inScheme cs: ;
    skos:notation
        "EPSG:20349"^^<https://epsg.io/> ,
        "https://epsg.io/20349"^^<https://epsg.io/> ;
    skos:prefLabel "AGD84 / AMG zone 49"@en ;
.

:amg84-z50
    a skos:Concept ;
    dcterms:source "https://epsg.io/20350"^^xsd:anyURI ;
    skos:altLabel
        "AMG84 z50"@en ,
        "AMG84 zone 50"@en ,
        "Australian Map Grid 1984 z50"@en ,
        "Australian Map Grid 1984 zone 50"@en ;
    skos:definition "The accompanying national map projection to AGD84, a transverse Mercator projection that conforms to zone 50 of the internationally accepted Universal Transverse Mercator (UTM) grid system. Area of use for AMG84 zone 50: onshore and offshore to 200 nautical mile EEZ (Exclusive Economic Zone) boundary between 114°E and 120°E."@en ;
    skos:inScheme cs: ;
    skos:notation
        "EPSG:20350"^^<https://epsg.io/> ,
        "https://epsg.io/20350"^^<https://epsg.io/> ;
    skos:prefLabel "AGD84 / AMG zone 50"@en ;
.

:amg84-z51
    a skos:Concept ;
    dcterms:source "https://epsg.io/20351"^^xsd:anyURI ;
    skos:altLabel
        "AMG84 z51"@en ,
        "AMG84 zone 51"@en ,
        "Australian Map Grid 1984 z51"@en ,
        "Australian Map Grid 1984 zone 51"@en ;
    skos:definition "The accompanying national map projection to AGD84, a Transverse Mercator projection that conforms to zone 51 of the internationally accepted Universal Transverse Mercator (UTM) grid system. Area of use for AMG84 zone 51: Australia – onshore and offshore between 120°E and 126°E."@en ;
    skos:inScheme cs: ;
    skos:notation
        "EPSG:20351"^^<https://epsg.io/> ,
        "https://epsg.io/20351"^^<https://epsg.io/> ;
    skos:prefLabel "AGD84 / AMG zone 51"@en ;
.

:amg84-z52
    a skos:Concept ;
    dcterms:source "https://epsg.io/20352"^^xsd:anyURI ;
    skos:altLabel
        "AMG84 z52"@en ,
        "AMG84 zone 52"@en ,
        "Australian Map Grid 1984 z52"@en ,
        "Australian Map Grid 1984 zone 52"@en ;
    skos:definition "The accompanying national map projection to AGD84, a transverse Mercator projection that conforms to zone 52 of the internationally accepted Universal Transverse Mercator (UTM) grid system. Area of use for AMG84 zone 52: Western Australia east of 126°E, South Australia west of 132°E, offshore federal waters between 126°E and 129°E."@en ;
    skos:inScheme cs: ;
    skos:notation
        "EPSG:20352"^^<https://epsg.io/> ,
        "https://epsg.io/20352"^^<https://epsg.io/> ;
    skos:prefLabel "AGD84 / AMG zone 52"@en ;
.

:gda2020
    a skos:Concept ;
    dcterms:source
        "https://linked.data.gov.au/def/queensland-crs/gda2020"^^xsd:anyURI ,
        "https://epsg.io/7844"^^xsd:anyURI ,
        "https://www.icsm.gov.au/sites/default/files/GDA2020TechnicalManualV1.1.1.pdf"^^xsd:anyURI ;
    skos:altLabel
        "GDA 2020"@en ,
        "GDA_2020"@en ,
        "Geocentric Datum of Australia 2020"@en ;
    skos:definition "The official geodetic datum adopted nationally in June 2020. GDA2020 is a coordinate reference system with an origin that coincides with a determination of the centre of mass of the earth, hence the term geocentric. GDA2020 is a plate-fixed or static coordinate datum based on the International Terrestrial Reference Frame 1992 (ITRF92), held at the reference epoch of 1 January 2020. Area of use is the same as GDA94, i.e. all the areas contained within Australia’s marine jurisdiction (within 200 nautical miles of Australia) and its external territories, and the areas of Australia’s continental shelf beyond 200 nautical miles as confirmed by the United Nations Commission on the Limits of the Continental Shelf: Australia including Lord Howe Island, Macquarie Island, Ashmore and Cartier Islands, Christmas Island, Cocos (Keeling) Islands, Norfolk Island; all onshore and offshore."@en ;
    skos:exactMatch <https://linked.data.gov.au/def/queensland-crs/gda2020> ;
    skos:inScheme cs: ;
    skos:notation
        "EPSG:7844"^^<https://epsg.io/> ,
        "https://epsg.io/7844"^^<https://epsg.io/> ;
    skos:prefLabel "GDA2020"@en ;
    skos:topConceptOf cs: ;
.

:gda94
    a skos:Concept ;
    dcterms:source
        "http://linked.data.gov.au/def/queensland-crs/gda1994"^^xsd:anyURI ,
        "https://epsg.io/4283"^^xsd:anyURI ,
        "https://www.icsm.gov.au/datum/geocentric-datum-australia-1994-gda94"^^xsd:anyURI ,
        "https://www.icsm.gov.au/sites/default/files/GDA2020TechnicalManualV1.1.1.pdf"^^xsd:anyURI ;
    skos:altLabel
        "GDA 1994"@en ,
        "GDA_1994"@en ,
        "Geocentric Datum of Australia 1994"@en ;
    skos:definition "The official geodetic datum adopted nationally in January 2000. GDA94 replaced the Australian Geodetic Datum 1966 (AGD66) and Australian Geodetic Datum 1984 (AGD84), and was later replaced by GDA2020. GDA94 is a coordinate reference system whose origin coincides with a determination of the centre of mass of the earth, hence the term geocentric. GDA94 is a plate-fixed or static coordinate datum based on the International Terrestrial Reference Frame 1992 (ITRF92), held at the reference epoch of 1 January 1994. The distance between the origin points of GDA94 and AGD is approximately 200 metres. Area of use: Australia including Lord Howe Island, Macquarie Island, Ashmore and Cartier Islands, Christmas Island, Cocos (Keeling) Islands, Norfolk Island; all onshore and offshore."@en ;
    skos:exactMatch <https://linked.data.gov.au/def/queensland-crs/gda1994> ;
    skos:inScheme cs: ;
    skos:notation
        "EPSG:4283"^^<https://epsg.io/> ,
        "https://epsg.io/4283"^^<https://epsg.io/> ;
    skos:prefLabel "GDA94"@en ;
    skos:topConceptOf cs: ;
.

:mga2020
    a skos:Concept ;
    dcterms:source "https://www.ga.gov.au/scientific-topics/positioning-navigation/geodesy/datums-projections/grid2020"^^xsd:anyURI ;
    skos:altLabel
        "MGA2020"@en ,
        "MGA_2020"@en ,
        "Map Grid of Australia 2020"@en ;
    skos:definition "The standard map projection associated with GDA2020 is the Map Grid of Australia 2020 (MGA2020), a transverse Mercator projection that conforms to the internationally standardized Universal Transverse Mercator (UTM) grid system. The UTM system has been used with the GRS80 ellipsoid and Geocentric Datum of Australia (GDA2020) latitudes and longitudes to define MGA2020."@en ;
    skos:inScheme cs: ;
    skos:narrower
        :mga2020-z49 ,
        :mga2020-z50 ,
        :mga2020-z51 ,
        :mga2020-z52 ;
    skos:prefLabel "MGA2020"@en ;
    skos:topConceptOf cs: ;
.

:mga2020-z49
    a skos:Concept ;
    dcterms:source "https://epsg.io/7849"^^xsd:anyURI ;
    skos:altLabel
        "MGA2020 z49"@en ,
        "MGA2020 zone 49"@en ,
        "Map Grid of Australia 2020 z49"@en ,
        "Map Grid of Australia 2020 zone 49"@en ;
    skos:definition "The accompanying national map projection to GDA2020, a transverse Mercator projection that conforms to zone 49 of the internationally accepted Universal Transverse Mercator (UTM) grid system. Area of use for MGA2020 zone 49: Australia – onshore and offshore west of 114°E; Christmas Island – offshore east of 108°E."@en ;
    skos:inScheme cs: ;
    skos:notation
        "EPSG:7849"^^<https://epsg.io/> ,
        "https://epsg.io/7849"^^<https://epsg.io/> ;
    skos:prefLabel "GDA2020 / MGA zone 49"@en ;
.

:mga2020-z50
    a skos:Concept ;
    dcterms:source "https://epsg.io/7850"^^xsd:anyURI ;
    skos:altLabel
        "MGA2020 z50"@en ,
        "MGA2020 zone 50"@en ,
        "Map Grid of Australia 2020 z50"@en ,
        "Map Grid of Australia 2020 zone 50"@en ;
    skos:definition "The accompanying national map projection to GDA2020, a transverse Mercator projection that conforms to zone 50 of the internationally accepted Universal Transverse Mercator (UTM) grid system. Area of use for MGA2020 zone 50: Australia – onshore and offshore between 114°E and 120°E."@en ;
    skos:inScheme cs: ;
    skos:notation
        "EPSG:7850"^^<https://epsg.io/> ,
        "https://epsg.io/7850"^^<https://epsg.io/> ;
    skos:prefLabel "GDA2020 / MGA zone 50"@en ;
.

:mga2020-z51
    a skos:Concept ;
    dcterms:source "https://epsg.io/7851"^^xsd:anyURI ;
    skos:altLabel
        "MGA2020 z51"@en ,
        "MGA2020 zone 51"@en ,
        "Map Grid of Australia 2020 z51"@en ,
        "Map Grid of Australia 2020 zone 51"@en ;
    skos:definition "The accompanying national map projection to GDA2020, a transverse Mercator projection that conforms to zone 51 of the internationally accepted Universal Transverse Mercator (UTM) grid system. Area of use for MGA2020 zone 51: Australia – onshore and offshore between 120°E and 126°E."@en ;
    skos:inScheme cs: ;
    skos:notation
        "EPSG:7851"^^<https://epsg.io/> ,
        "https://epsg.io/7851"^^<https://epsg.io/> ;
    skos:prefLabel "GDA2020 / MGA zone 51"@en ;
.

:mga2020-z52
    a skos:Concept ;
    dcterms:source "https://epsg.io/7852"^^xsd:anyURI ;
    skos:altLabel
        "MGA2020 z52"@en ,
        "MGA2020 zone 52"@en ,
        "Map Grid of Australia 2020 z52"@en ,
        "Map Grid of Australia 2020 zone 52"@en ;
    skos:definition "The accompanying national map projection to GDA2020, a transverse Mercator projection that conforms to zone 52 of the internationally accepted Universal Transverse Mercator (UTM) grid system. Area of use for MGA2020 zone 52: Australia – onshore and offshore between 126°E and 132°E."@en ;
    skos:inScheme cs: ;
    skos:notation
        "EPSG:7852"^^<https://epsg.io/> ,
        "https://epsg.io/7852"^^<https://epsg.io/> ;
    skos:prefLabel "GDA2020 / MGA zone 52"@en ;
.

:mga94
    a skos:Concept ;
    skos:altLabel
        "MGA 94"@en ,
        "MGA_94"@en ,
        "Map Grid of Australia 1994"@en ;
    skos:definition "The standard map projection associated with GDA94 is the Map Grid of Australia 1994 (MGA94), a transverse Mercator projection that conforms to the internationally standardized Universal Transverse Mercator (UTM) grid system. At that time the recommended reference ellipsoid was also changed from ANS to the Geodetic Reference System 1980 (GRS80) ellipsoid. Area of use: Australia including Lord Howe Island, Macquarie Island, Ashmore and Cartier Islands, Christmas Island, Cocos (Keeling) Islands, Norfolk Island; all onshore and offshore."@en ;
    skos:inScheme cs: ;
    skos:narrower
        :mga94-z49 ,
        :mga94-z50 ,
        :mga94-z51 ,
        :mga94-z52 ;
    skos:prefLabel "MGA94"@en ;
    skos:topConceptOf cs: ;
.

:mga94-z49
    a skos:Concept ;
    dcterms:source "https://epsg.io/28349"^^xsd:anyURI ;
    skos:altLabel
        "MGA94 z49"@en ,
        "MGA94 zone 49"@en ,
        "Map Grid of Australia 1994 z49"@en ,
        "Map Grid of Australia 1994 zone 49"@en ;
    skos:definition "The accompanying national map projection to MGA94, a transverse Mercator projection that conforms to zone 49 of the internationally accepted Universal Transverse Mercator (UTM) grid system. Area of use for MGA94 zone 49: Australia - onshore and offshore west of 114° E; Christmas Island - offshore east of 108°E."@en ;
    skos:inScheme cs: ;
    skos:notation
        "EPSG:28349"^^<https://epsg.io/> ,
        "https://epsg.io/28349"^^<https://epsg.io/> ;
    skos:prefLabel "GDA94 / MGA zone 49"@en ;
.

:mga94-z50
    a skos:Concept ;
    dcterms:source "https://epsg.io/28350"^^xsd:anyURI ;
    skos:altLabel
        "MGA94 z50"@en ,
        "MGA94 zone 50"@en ,
        "Map Grid of Australia 1994 z50"@en ,
        "Map Grid of Australia 1994 zone 50"@en ;
    skos:definition "The accompanying national map projection to MGA94, a transverse Mercator projection that conforms to zone 50 of the internationally accepted Universal Transverse Mercator (UTM) grid system. Area of use for MGA94 zone 50: Australia – onshore and offshore between 114°E and 120°E."@en ;
    skos:inScheme cs: ;
    skos:notation
        "EPSG:28350"^^<https://epsg.io/> ,
        "https://epsg.io/28350"^^<https://epsg.io/> ;
    skos:prefLabel "GDA94 / MGA zone 50"@en ;
.

:mga94-z51
    a skos:Concept ;
    dcterms:source "https://epsg.io/28351"^^xsd:anyURI ;
    skos:altLabel
        "MGA94 z51"@en ,
        "MGA94 zone 51"@en ,
        "Map Grid of Australia 1994 z51"@en ,
        "Map Grid of Australia 1994 zone 51"@en ;
    skos:definition "The accompanying national map projection to MGA94, a transverse Mercator projection that conforms to zone 51 of the internationally accepted Universal Transverse Mercator (UTM) grid system. Area of use for MGA94 zone 51: Australia – onshore and offshore between 120°E and 126°E."@en ;
    skos:inScheme cs: ;
    skos:notation
        "EPSG:28351"^^<https://epsg.io/> ,
        "https://epsg.io/28351"^^<https://epsg.io/> ;
    skos:prefLabel "GDA94 / MGA zone 51"@en ;
.

:mga94-z52
    a skos:Concept ;
    dcterms:source "https://epsg.io/28352"^^xsd:anyURI ;
    skos:altLabel
        "MGA94 z52"@en ,
        "MGA94 zone 52"@en ,
        "Map Grid of Australia 1994 z52"@en ,
        "Map Grid of Australia 1994 zone 52"@en ;
    skos:definition "The accompanying national map projection to MGA94, a transverse Mercator projection that conforms to zone 52 of the internationally accepted Universal Transverse Mercator (UTM) grid system. Area of use for MGA94 zone 52: Australia – onshore and offshore between 126°E and 132°E."@en ;
    skos:inScheme cs: ;
    skos:notation
        "EPSG:28352"^^<https://epsg.io/> ,
        "https://epsg.io/28352"^^<https://epsg.io/> ;
    skos:prefLabel "GDA94 / MGA zone 52"@en ;
.

:utm-z49
    a skos:Concept ;
    skos:altLabel
        "UTM zone 49"@en ,
        "Zone 49"@en ,
        "z49"@en ;
    skos:definition "The 49th UTM zone spanning from longitudes 108°E to 114°E. Central meridian 111°E."@en ;
    skos:inScheme cs: ;
    skos:prefLabel "UTM z49"@en ;
.

:utm-z50
    a skos:Concept ;
    skos:altLabel
        "UTM zone 50"@en ,
        "Zone 50"@en ,
        "z50"@en ;
    skos:definition "The 50th UTM zone spanning from longitudes 114°E to 120°E. Central meridian 115°E."@en ;
    skos:inScheme cs: ;
    skos:prefLabel "UTM z50"@en ;
.

:utm-z51
    a skos:Concept ;
    skos:altLabel
        "UTM zone 51"@en ,
        "Zone 51"@en ,
        "z51"@en ;
    skos:definition "The 51st UTM zone spanning from longitudes 120°E to 126°E. Central meridian 121°E."@en ;
    skos:inScheme cs: ;
    skos:prefLabel "UTM z51"@en ;
.

:utm-z52
    a skos:Concept ;
    skos:altLabel
        "UTM zone 52"@en ,
        "Zone 52"@en ,
        "z52"@en ;
    skos:definition "The 49th UTM zone spanning from longitudes 126°E to 132°E. Central meridian 129°E."@en ;
    skos:inScheme cs: ;
    skos:prefLabel "UTM z52"@en ;
.

:wgs84
    a skos:Concept ;
    dcterms:source
        "https://en.wikipedia.org/wiki/World_Geodetic_System"^^xsd:anyURI ,
        "https://epsg.io/4326"^^xsd:anyURI ,
        "https://linked.data.gov.au/def/queensland-crs/wgs1984"^^xsd:anyURI ,
        "https://www.ga.gov.au/scientific-topics/positioning-navigation/wgs84"^^xsd:anyURI ,
        "https://www.icsm.gov.au/sites/default/files/2017-09/gda-v_2.4_0.pdf"^^xsd:anyURI ;
    skos:altLabel
        "WGS 84"@en ,
        "WGS_84"@en ,
        "World Geodetic System 1984"@en ;
    skos:definition "The World Geodetic System 1984 (WGS84) is the reference frame used by the Global Positioning System (GPS). It was developed by the US Department of Defense and is maintained by the US National Geospatial Intelligence Agency (NGA). WGS84 defines an Earth-centred, Earth-fixed coordinate reference system with an origin that coincides with a determination of the centre of mass of the earth, and a geodetic datum. The datum defines meridian 0 as the International Earth Rotation and Reference System Service (IERS) Reference Meridian and the datum surface is an oblate spheroid. Officially adopted as the world geodetic datum in 1984, WGS84 is a dynamic reference frame. WGS84 has been revised several times since its conception and is at present aligned at the centimetre level to the International Terrestrial Reference Frame (ITRF), which generally ensures scientific integrity and compatibility with international standards and conventions. At the beginning of each year, the NGA updates station coordinates to account for plate tectonic motion. This means that WGS84 coordinates derived by users from GPS measurements will appear to move over time. In January 1994, GDA94 and ITRF were coincident, but since Australia is moving up to 7cm per year in a northeasterly direction, there was a 1.8 m difference between the two systems in 2020 — for applications that require uncertainty better than 5 m, GDA94 and WGS84/ITRF cannot be considered equivalent. Area of use: world."@en ;
    skos:exactMatch <https://linked.data.gov.au/def/queensland-crs/wgs1984> ;
    skos:inScheme cs: ;
    skos:narrower
        :wgs84-utm-z49s ,
        :wgs84-utm-z50s ,
        :wgs84-utm-z51s ,
        :wgs84-utm-z52s ;
    skos:notation
        "EPSG:4326"^^<https://epsg.io/> ,
        "https://epsg.io/4326"^^<https://epsg.io/> ;
    skos:prefLabel "WGS84"@en ;
    skos:topConceptOf cs: ;
.

:wgs84-utm-z49s
    a skos:Concept ;
    dcterms:source "https://epsg.io/32749"^^xsd:anyURI ;
    skos:altLabel "WGS84 / UTM z49S"@en ;
    skos:definition "The 49th Universal Transverse Mercator (UTM) zone. Area of use: Between 108°E and 114°E, southern hemisphere between 80°S and equator, onshore and offshore; Australia; Indonesia."@en ;
    skos:inScheme cs: ;
    skos:notation
        "EPSG:32749"^^<https://epsg.io/> ,
        "https://epsg.io/32749"^^<https://epsg.io/> ;
    skos:prefLabel "WGS84 / UTM zone 49S"@en ;
.

:wgs84-utm-z50s
    a skos:Concept ;
    dcterms:source "https://epsg.io/32750"^^xsd:anyURI ;
    skos:altLabel "WGS84 / UTM z50S"@en ;
    skos:definition "The 50th Universal Transverse Mercator (UTM) zone. Area of use: Between 114°E and 120°E, southern hemisphere between 80°S and equator, onshore and offshore; Australia; Indonesia."@en ;
    skos:inScheme cs: ;
    skos:notation
        "EPSG:32750"^^<https://epsg.io/> ,
        "https://epsg.io/32750"^^<https://epsg.io/> ;
    skos:prefLabel "WGS84 / UTM zone 50S"@en ;
.

:wgs84-utm-z51s
    a skos:Concept ;
    dcterms:source "https://epsg.io/32751"^^xsd:anyURI ;
    skos:altLabel "WGS84 / UTM z51S"@en ;
    skos:definition "The 51st Universal Transverse Mercator (UTM) zone. Area of use: Between 120°E and 126°E, southern hemisphere between 80°S and equator, onshore and offshore; Australia; East Timor; Indonesia."@en ;
    skos:inScheme cs: ;
    skos:notation
        "EPSG:32751"^^<https://epsg.io/> ,
        "https://epsg.io/32751"^^<https://epsg.io/> ;
    skos:prefLabel "WGS84 / UTM zone 51S"@en ;
.

:wgs84-utm-z52s
    a skos:Concept ;
    dcterms:source "https://epsg.io/32752"^^xsd:anyURI ;
    skos:altLabel "WGS84 / UTM z52S"@en ;
    skos:definition "The 49th Universal Transverse Mercator (UTM) zone. Area of use: Between 126°E and 132°E, southern hemisphere between 80°S and equator, onshore and offshore; Australia; East Timor; Indonesia."@en ;
    skos:inScheme cs: ;
    skos:notation
        "EPSG:32752"^^<https://epsg.io/> ,
        "https://epsg.io/32752"^^<https://epsg.io/> ;
    skos:prefLabel "WGS84 / UTM zone 52S"@en ;
.

<https://linked.data.gov.au/org/gswa>
    a schema:Organization ;
    schema:name "Geological Survey of Western Australia" ;
    schema:url "https://dmp.wa.gov.au/Geological-Survey/Geological-Survey-262.aspx"^^xsd:anyURI ;
.

:1.0 schema:name "1.0" .

cs:
    a skos:ConceptScheme ;
    dcterms:created "2023-09-13"^^xsd:date ;
    dcterms:creator <https://linked.data.gov.au/org/gswa> ;
    dcterms:identifier "wa-coordinate-reference-systems"^^xsd:token ;
    dcterms:modified "2023-09-13"^^xsd:date ;
    dcterms:publisher <https://linked.data.gov.au/org/gswa> ;
    owl:versionIRI :1.0 ;
    owl:versionInfo "1.0" ;
    reg:status agldwgstatus:stable ;
    skos:definition "The coordinate reference systems (geographic and projected) used and referred to within Western Australia. It includes historical and current reference systems, Universal Transverse Mercator (UTM) zones, and, where applicable, notations based on the EPSG registry (https://epsg.io/). Some concepts are included to account for legacy data/maps with limited information."@en ;
    skos:hasTopConcept
        :Clarke1858 ,
        :agd66 ,
        :agd84 ,
        :amg66 ,
        :amg84 ,
        :gda2020 ,
        :gda94 ,
        :local-grid ,
        :mga2020 ,
        :mga94 ,
        :unknown ,
        :utm ,
        :wgs84 ;
    skos:historyNote "Historical and current coordinate references systems used in maps and publications by the Geological Survey of Western Australia since its inception."@en ;
    skos:prefLabel "Western Australian coordinate reference systems"@en ;
    schema:keywords theme:geology-mapping ;
    prov:qualifiedAttribution
        [
            dcat:hadRole dataroles:custodian ;
            prov:agent [
                    a schema:Person ;
                    schema:email ""^^xsd:anyURI ;
                    schema:name "Erin Gray" ;
                ]
        ] ,
        [
            dcat:hadRole dataroles:custodian ;
            prov:agent [
                    a schema:Person ;
                    schema:email ""^^xsd:anyURI ;
                    schema:name "Angela Riganti" ;
                ]
        ] ;
.

<https://linked.data.gov.au/def/queensland-crs/agd1966> schema:name "AGD66" .
<https://linked.data.gov.au/def/queensland-crs/agd1984> schema:name "AGD84" .
<https://linked.data.gov.au/def/queensland-crs/gda1994> schema:name "GDA94" .
<https://linked.data.gov.au/def/queensland-crs/gda2020> schema:name "GDA2020" .
<https://linked.data.gov.au/def/queensland-crs/wgs1984> schema:name "WGS84" .
