PREFIX : <https://linked.data.gov.au/def/alteration-intensity/>
PREFIX cs: <https://linked.data.gov.au/def/alteration-intensity>
PREFIX dcat: <http://www.w3.org/ns/dcat#>
PREFIX isoroles: <https://linked.data.gov.au/def/data-roles/>
PREFIX owl: <http://www.w3.org/2002/07/owl#>
PREFIX prov: <http://www.w3.org/ns/prov#>
PREFIX rdfs: <http://www.w3.org/2000/01/rdf-schema#>
PREFIX schema: <https://schema.org/>
PREFIX skos: <http://www.w3.org/2004/02/skos/core#>
PREFIX xsd: <http://www.w3.org/2001/XMLSchema#>
PREFIX reg: <http://purl.org/linked-data/registry#>

:intense
    a skos:Concept ;
    rdfs:isDefinedBy cs: ;
    skos:altLabel
        "advanced"@en ,
        "complete"@en ,
        "comprehensive"@en ,
        "extreme"@en ,
        "major"@en ,
        "massive"@en ,
        "pronounced"@en ,
        "severe"@en ,
        "significant"@en ;
    skos:definition "Intense alteration refers to an almost complete to complete replacement of the primary minerals and obliteration of original textures."@en ;
    skos:historyNote "Definition from Pirajno (2009; Pirajno, F 2009, Hydrothermal processes and mineral systems: Springer-Verlag, 1250p)." ;
    skos:inScheme cs: ;
    skos:prefLabel "intense"@en ;
    skos:topConceptOf cs: ;
.

:moderate
    a skos:Concept ;
    rdfs:isDefinedBy cs: ;
    skos:altLabel "medium"@en ;
    skos:definition "Moderate intensity indicates alteration in which several of the primary mineral species have been replaced, with some modification of the original textures."@en ;
    skos:historyNote "Definition from Pirajno (2009; Pirajno, F 2009, Hydrothermal processes and mineral systems: Springer-Verlag, 1250p)." ;
    skos:inScheme cs: ;
    skos:prefLabel "moderate"@en ;
    skos:topConceptOf cs: ;
.

:strong
    a skos:Concept ;
    rdfs:isDefinedBy cs: ;
    skos:altLabel
        "heavy"@en ,
        "high"@en ;
    skos:definition "Strong intensity indicates alteration in which the majority of the primary minerals have been replaced, with considerable modification of the original textures."@en ;
    skos:historyNote "Definition from Pirajno (2009; Pirajno, F 2009, Hydrothermal processes and mineral systems: Springer-Verlag, 1250p)." ;
    skos:inScheme cs: ;
    skos:prefLabel "strong"@en ;
    skos:topConceptOf cs: ;
.

:unaltered
    a skos:Concept ;
    rdfs:isDefinedBy cs: ;
    skos:altLabel "not altered"@en ;
    skos:definition "A rock with no visible signs of alteration, in which primary minerals, fabrics (including primary pore space) and chemistry are unchanged."@en ;
    skos:exactMatch
        <https://linked.data.gov.au/def/alteration-form/unaltered> ,
        <https://linked.data.gov.au/def/alteration-type/unaltered> ;
    skos:historyNote "Compiled by the Geological Survey of Western Australia." ;
    skos:inScheme cs: ;
    skos:prefLabel "unaltered"@en ;
    skos:topConceptOf cs: ;
.

:unknown
    a skos:Concept ;
    rdfs:isDefinedBy cs: ;
    skos:definition "Alteration intensity not specified."@en ;
    skos:inScheme cs: ;
    skos:prefLabel "unknown"@en ;
    skos:topConceptOf cs: ;
.

:weak
    a skos:Concept ;
    rdfs:isDefinedBy cs: ;
    skos:altLabel
        "incipient"@en ,
        "insignificant"@en ,
        "light"@en ,
        "low"@en ,
        "minor"@en ,
        "negligible"@en ,
        "slight"@en ,
        "traces"@en ;
    skos:definition "Weak, or low, intensity indicates alteration in which only a few of the primary mineral species have been replaced, with little or no modification of the original textures."@en ;
    skos:historyNote "Definition from Pirajno (2009; Pirajno, F 2009, Hydrothermal processes and mineral systems: Springer-Verlag, 1250p)." ;
    skos:inScheme cs: ;
    skos:prefLabel "weak"@en ;
    skos:topConceptOf cs: ;
.

<https://orcid.org/0000-0001-5888-5102>
    a schema:Person ;
    schema:email ""^^xsd:anyURI ;
    schema:name "0000 0001 5888 5102" ;
.

<https://orcid.org/0000-0002-7645-5031>
    a schema:Person ;
    schema:email ""^^xsd:anyURI ;
    schema:name "0000 0002 7645 5031" ;
.

<https://linked.data.gov.au/org/gswa>
    a schema:Organization ;
    schema:name "Gswa" ;
    schema:url ""^^xsd:anyURI ;
.

cs:
    a skos:ConceptScheme ;
    reg:status <https://linked.data.gov.au/def/reg-statuses/stable> ;
    owl:versionIRI :1 ;
    skos:definition "A compilation of terms that describe the degree to which (i.e. how much) a rock or a mineral has been affected by alteration. Alteration in this context is considered as a modification of the original lithology caused by meteoric, connate, metamorphic or magmatic-derived fluids, excluding the weathering environment, mineralization and direct magmatic or metamorphic processes. These concepts are generally used as convenient field or petrographic descriptive terms. Definitions are largely from Pirajno (2009) and the Glossary of geology (5th edition revised; Neuendorf et. al., 2011)."@en ;
    skos:hasTopConcept
        :intense ,
        :moderate ,
        :strong ,
        :unaltered ,
        :unknown ,
        :weak ;
    skos:historyNote """Derived from GSWA's WAROX database's table [GEOLOGY].[Warox_REF].[Intensity]. Definitions compiled from:
1) Pirajno, F 2009, Hydrothermal processes and mineral systems: Springer-Verlag, 1250p.
2) Neuendorf, KKE, Mehl Jr, JP and Jackson, JA (editors) 2011, Glossary of geology (5th edition, revised): American Geosciences Institute, Alexandria, Virginia, USA, 800p."""@en ;
    skos:prefLabel "Alteration intensity"@en ;
    prov:qualifiedAttribution
        [
            dcat:hadRole isoroles:custodian ;
            prov:agent <https://orcid.org/0000-0002-7645-5031> ;
        ] ,
        [
            dcat:hadRole isoroles:custodian ;
            prov:agent <https://orcid.org/0000-0001-5888-5102> ;
        ] ;
    schema:creator <https://linked.data.gov.au/org/gswa> ;
    schema:dateCreated "2024-12-02"^^xsd:date ;
    schema:dateModified "2024-12-02"^^xsd:date ;
    schema:keywords <https://linked.data.gov.au/def/gswa-vocabulary-themes/resources-mineral> ;
    schema:publisher <https://linked.data.gov.au/org/gswa> ;
    schema:version "1" ;
.
